# baseURI: http://iso.org/tc211/term/
# imports: http://purl.org/dc/elements/1.1/
# imports: http://purl.org/dc/terms/
# imports: http://purl.org/linked-data/registry
# imports: http://www.w3.org/2004/02/skos/core

@prefix dc: <http://purl.org/dc/elements/1.1/> .
@prefix dct: <http://purl.org/dc/terms/> .
@prefix dcterms: <http://purl.org/dc/terms/> .
@prefix owl: <http://www.w3.org/2002/07/owl#> .
@prefix rdf: <http://www.w3.org/1999/02/22-rdf-syntax-ns#> .
@prefix rdfs: <http://www.w3.org/2000/01/rdf-schema#> .
@prefix reg: <http://purl.org/linked-data/registry#> .
@prefix skos: <http://www.w3.org/2004/02/skos/core#> .
@prefix xsd: <http://www.w3.org/2001/XMLSchema#> .

<http://iso.org/tc211/term/>
  rdf:type owl:Ontology ;
  owl:imports dc: ;
  owl:imports dcterms: ;
  owl:imports <http://purl.org/linked-data/registry> ;
  owl:imports <http://www.w3.org/2004/02/skos/core> ;
.
<http://iso.org/tc211/term/10>
  rdf:type skos:Concept ;
  dcterms:dateAccepted "2008-11-15"^^xsd:date ;
  dcterms:provenance "ISO/TS 19104:2008" ;
  dcterms:source "ISO 1087-1:2000" ;
  reg:status reg:statusValid ;
  rdfs:label "admitted term"@en ;
  skos:changeNote "valid" ;
  skos:editorialNote "preferred"^^xsd:string ;
  skos:notation 10 ;
  skos:prefLabel "admitted term"@en ;
.
<http://iso.org/tc211/term/100>
  rdf:type skos:Concept ;
  dcterms:dateAccepted "2005-08-15"^^xsd:date ;
  dcterms:dateAccepted "2007-11-01"^^xsd:date ;
  dcterms:provenance "KS X ISO 19123" ;
  dcterms:source "ISO 19123:2005" ;
  reg:status reg:statusValid ;
  rdfs:label "coverage geometry"@en ;
  skos:changeNote "valid" ;
  skos:definition "좌표로 기술된 커버리지의 시공간적 영역에 대한 구성"@kr ;
  skos:editorialNote "preferred" ;
  skos:editorialNote "preferred"^^xsd:string ;
  skos:notation "100" ;
  skos:notation 100 ;
  skos:prefLabel "coverage geometry"@en ;
  skos:prefLabel "커버리지 기하"@kr ;
.
<http://iso.org/tc211/term/1000>
  rdf:type skos:Concept ;
  dcterms:dateAccepted "2010-06-15"^^xsd:date ;
  dcterms:source "ISO/TS 19130:2010" ;
  reg:status reg:statusValid ;
  rdfs:comment "Note 1 to entry: This definition also applies for water surfaces."@en ;
  rdfs:label "ground sampling distance"@en ;
  skos:changeNote "valid" ;
  skos:editorialNote "preferred"^^xsd:string ;
  skos:notation 1000 ;
  skos:note "Note 1 to entry: This definition also applies for water surfaces."@en ;
  skos:prefLabel "ground sampling distance"@en ;
.
<http://iso.org/tc211/term/1002>
  rdf:type skos:Concept ;
  dcterms:dateAccepted "2010-06-15"^^xsd:date ;
  dcterms:source "ISO/TS 19130:2010" ;
  reg:status reg:statusValid ;
  rdfs:label "image distortion"@en ;
  skos:changeNote "valid" ;
  skos:editorialNote "preferred"^^xsd:string ;
  skos:notation 1002 ;
  skos:prefLabel "image distortion"@en ;
.
<http://iso.org/tc211/term/1003>
  rdf:type skos:Concept ;
  dcterms:dateAccepted "2010-06-15"^^xsd:date ;
  dcterms:source "ISO/TS 19130:2010" ;
  reg:status reg:statusValid ;
  rdfs:label "impulse response"@en ;
  skos:changeNote "valid" ;
  skos:editorialNote "preferred"^^xsd:string ;
  skos:notation 1003 ;
  skos:prefLabel "impulse response"@en ;
.
<http://iso.org/tc211/term/1004>
  rdf:type skos:Concept ;
  dcterms:dateAccepted "2010-06-15"^^xsd:date ;
  dcterms:source "ISO/TS 19130:2010" ;
  reg:status reg:statusValid ;
  rdfs:label "internal coordinate reference system"@en ;
  skos:changeNote "valid" ;
  skos:editorialNote "preferred"^^xsd:string ;
  skos:notation 1004 ;
  skos:prefLabel "internal coordinate reference system"@en ;
.
<http://iso.org/tc211/term/1005>
  rdf:type skos:Concept ;
  dcterms:dateAccepted "2010-06-15"^^xsd:date ;
  dcterms:source "ISO/TS 19130:2010" ;
  reg:status reg:statusValid ;
  rdfs:label "passive sensor"@en ;
  skos:changeNote "valid" ;
  skos:editorialNote "preferred"^^xsd:string ;
  skos:notation 1005 ;
  skos:prefLabel "passive sensor"@en ;
.
<http://iso.org/tc211/term/1006>
  rdf:type skos:Concept ;
  dcterms:dateAccepted "2010-06-15"^^xsd:date ;
  dcterms:source "ISO/TS 19130:2010" ;
  reg:status reg:statusValid ;
  rdfs:label "platform coordinate reference system"@en ;
  skos:changeNote "valid" ;
  skos:editorialNote "preferred"^^xsd:string ;
  skos:notation 1006 ;
  skos:prefLabel "platform coordinate reference system"@en ;
.
<http://iso.org/tc211/term/1007>
  rdf:type skos:Concept ;
  dcterms:dateAccepted "2010-06-15"^^xsd:date ;
  dcterms:source "ISO/TS 19130:2010" ;
  reg:status reg:statusValid ;
  rdfs:label "principal point of autocollimation"@en ;
  skos:changeNote "valid" ;
  skos:editorialNote "preferred"^^xsd:string ;
  skos:notation 1007 ;
  skos:prefLabel "principal point of autocollimation"@en ;
.
<http://iso.org/tc211/term/1008>
  rdf:type skos:Concept ;
  dcterms:dateAccepted "2010-06-15"^^xsd:date ;
  dcterms:source "ISO/TS 19130:2010" ;
  reg:status reg:statusValid ;
  rdfs:label "projection centre"@en ;
  rdfs:seeAlso "perspective centre" ;
  skos:altLabel "perspective centre"@en ;
  skos:changeNote "valid" ;
  skos:editorialNote "preferred"^^xsd:string ;
  skos:notation 1008 ;
  skos:prefLabel "projection centre"@en ;
.
<http://iso.org/tc211/term/1009>
  rdf:type skos:Concept ;
  dcterms:dateAccepted "2010-06-15"^^xsd:date ;
  dcterms:source "ISO/TS 19130:2010" ;
  reg:status reg:statusValid ;
  rdfs:label "range direction <SAR>"@en ;
  rdfs:seeAlso "slant range direction <SAR>" ;
  skos:altLabel "slant range direction <SAR>"@en ;
  skos:changeNote "valid" ;
  skos:editorialNote "preferred"^^xsd:string ;
  skos:notation 1009 ;
  skos:prefLabel "range direction <SAR>"@en ;
.
<http://iso.org/tc211/term/101>
  rdf:type skos:Concept ;
  dcterms:dateAccepted "2003-05-01"^^xsd:date ;
  dcterms:dateAccepted "2009-12-29"^^xsd:date ;
  dcterms:provenance "KS X ISO 19107" ;
  dcterms:source "ISO 19107:2003" ;
  reg:status reg:statusValid ;
  rdfs:comment "Note 1 to entry: The boundary of a curve is the set of points at either end of the curve. If the curve is a cycle, the two ends are identical, and the curve (if topologically closed) is considered to not have a boundary. The first point is called the start point, and the last is the end point. Connectivity of the curve is guaranteed by the \"continuous image of a line\" clause. A topological theorem states that a continuous image of a connected set is connected."@en ;
  rdfs:comment "비고: 곡선의 경계는 곡선의 양쪽 끝 점의 집합이다. 만약 곡선이 순환한다면(위상적으로 폐합되어 있다면), 두 끝점은 동일하며 곡선은 경계를 갖지 않는다. 첫 번째 점은 시작점으로, 마지막 점은 끝점으로 불린다. 곡선의 연결성은 \"선의 연속 이미지\"라는 절에 기술되어 있으며, \"연결 집합의 연속 이미지는 연결되어 있다\"라고 위상적으로 정의된다."@kr ;
  rdfs:label "curve"@en ;
  skos:changeNote "valid" ;
  skos:definition "선의 연속적 이미지를 표현하는 1차원 기하 원시 객체"@kr ;
  skos:editorialNote "preferred" ;
  skos:editorialNote "preferred"^^xsd:string ;
  skos:notation "101" ;
  skos:notation 101 ;
  skos:note "Note 1 to entry: The boundary of a curve is the set of points at either end of the curve. If the curve is a cycle, the two ends are identical, and the curve (if topologically closed) is considered to not have a boundary. The first point is called the start point, and the last is the end point. Connectivity of the curve is guaranteed by the \"continuous image of a line\" clause. A topological theorem states that a continuous image of a connected set is connected."@en ;
  skos:note "비고: 곡선의 경계는 곡선의 양쪽 끝 점의 집합이다. 만약 곡선이 순환한다면(위상적으로 폐합되어 있다면), 두 끝점은 동일하며 곡선은 경계를 갖지 않는다. 첫 번째 점은 시작점으로, 마지막 점은 끝점으로 불린다. 곡선의 연결성은 \"선의 연속 이미지\"라는 절에 기술되어 있으며, \"연결 집합의 연속 이미지는 연결되어 있다\"라고 위상적으로 정의된다."@kr ;
  skos:prefLabel "curve"@en ;
  skos:prefLabel "곡선"@kr ;
.
<http://iso.org/tc211/term/1010>
  rdf:type skos:Concept ;
  dcterms:dateAccepted "2010-06-15"^^xsd:date ;
  dcterms:source "ISO/TS 19130:2010" ;
  reg:status reg:statusValid ;
  rdfs:comment "Note 1 to entry: For a SAR sensor, it is usually measured in terms of the impulse response of the sensor and processing system. It is a function of the bandwidth of the pulse."@en ;
  rdfs:label "range resolution"@en ;
  skos:changeNote "valid" ;
  skos:editorialNote "preferred"^^xsd:string ;
  skos:notation 1010 ;
  skos:note "Note 1 to entry: For a SAR sensor, it is usually measured in terms of the impulse response of the sensor and processing system. It is a function of the bandwidth of the pulse."@en ;
  skos:prefLabel "range resolution"@en ;
.
<http://iso.org/tc211/term/1011>
  rdf:type skos:Concept ;
  dcterms:dateAccepted "2010-06-15"^^xsd:date ;
  dcterms:source "ISO/TS 19130:2010" ;
  reg:status reg:statusValid ;
  rdfs:label "range vector"@en ;
  skos:changeNote "valid" ;
  skos:editorialNote "preferred"^^xsd:string ;
  skos:notation 1011 ;
  skos:prefLabel "range vector"@en ;
.
<http://iso.org/tc211/term/1012>
  rdf:type skos:Concept ;
  dcterms:dateAccepted "2010-06-15"^^xsd:date ;
  dcterms:source "ISO/TS 19130:2010" ;
  reg:status reg:statusValid ;
  rdfs:label "ScanSAR mode"@en ;
  skos:changeNote "valid" ;
  skos:editorialNote "preferred"^^xsd:string ;
  skos:notation 1012 ;
  skos:prefLabel "ScanSAR mode"@en ;
.
<http://iso.org/tc211/term/1013>
  rdf:type skos:Concept ;
  dcterms:dateAccepted "2010-06-15"^^xsd:date ;
  dcterms:source "ISO/TS 19130:2010" ;
  reg:status reg:statusValid ;
  rdfs:label "sensor model <geopositioning>"@en ;
  skos:changeNote "valid" ;
  skos:editorialNote "preferred"^^xsd:string ;
  skos:notation 1013 ;
  skos:prefLabel "sensor model <geopositioning>"@en ;
.
<http://iso.org/tc211/term/1014>
  rdf:type skos:Concept ;
  dcterms:dateAccepted "2008-07-15"^^xsd:date ;
  dcterms:provenance "ISO 6709:2008" ;
  dcterms:source "ISO 3534-2:2006" ;
  reg:status reg:statusValid ;
  rdfs:label "accuracy"@en ;
  skos:changeNote "valid" ;
  skos:editorialNote "preferred"^^xsd:string ;
  skos:notation 1014 ;
  skos:prefLabel "accuracy"@en ;
.
<http://iso.org/tc211/term/1018>
  rdf:type skos:Concept ;
  dcterms:dateAccepted "2010-10-15"^^xsd:date ;
  dcterms:provenance "ISO 19143:2010" ;
  dcterms:source "ISO 19142:2010" ;
  reg:status reg:statusValid ;
  rdfs:label "feature identifier"@en ;
  skos:changeNote "valid" ;
  skos:editorialNote "preferred"^^xsd:string ;
  skos:notation 1018 ;
  skos:prefLabel "feature identifier"@en ;
.
<http://iso.org/tc211/term/1019>
  rdf:type skos:Concept ;
  dcterms:dateAccepted "2010-10-15"^^xsd:date ;
  dcterms:source "ISO 19143:2010" ;
  reg:status reg:statusValid ;
  rdfs:label "filter capabilities XML"@en ;
  skos:changeNote "valid" ;
  skos:editorialNote "preferred"^^xsd:string ;
  skos:notation 1019 ;
  skos:prefLabel "filter capabilities XML"@en ;
.
<http://iso.org/tc211/term/102>
  rdf:type skos:Concept ;
  dcterms:dateAccepted "2003-05-01"^^xsd:date ;
  dcterms:dateAccepted "2009-12-29"^^xsd:date ;
  dcterms:provenance "KS X ISO 19107" ;
  dcterms:source "ISO 19107:2003" ;
  reg:status reg:statusValid ;
  rdfs:comment "Note 1 to entry: The geometric set represented by a single curve segment is equivalent to a curve."@en ;
  rdfs:comment "비고: 단일 곡선 분절에 의해 표현되는 기하 집합은 곡선과 같다."@kr ;
  rdfs:label "curve segment"@en ;
  skos:changeNote "valid" ;
  skos:definition "동일한 보간법 및 정의 방법으로 곡선의 연속적인 컴포넌트의 표현에 사용되는 1차원 기하객체"@kr ;
  skos:editorialNote "preferred" ;
  skos:editorialNote "preferred"^^xsd:string ;
  skos:notation "102" ;
  skos:notation 102 ;
  skos:note "Note 1 to entry: The geometric set represented by a single curve segment is equivalent to a curve."@en ;
  skos:note "비고: 단일 곡선 분절에 의해 표현되는 기하 집합은 곡선과 같다."@kr ;
  skos:prefLabel "curve segment"@en ;
  skos:prefLabel "곡선 분절"@kr ;
.
<http://iso.org/tc211/term/1020>
  rdf:type skos:Concept ;
  dcterms:dateAccepted "2010-10-15"^^xsd:date ;
  dcterms:source "ISO 19143:2010" ;
  reg:status reg:statusValid ;
  rdfs:label "filter expression"@en ;
  skos:changeNote "valid" ;
  skos:editorialNote "preferred"^^xsd:string ;
  skos:notation 1020 ;
  skos:prefLabel "filter expression"@en ;
.
<http://iso.org/tc211/term/1021>
  rdf:type skos:Concept ;
  dcterms:dateAccepted "2010-10-15"^^xsd:date ;
  dcterms:source "ISO 19143:2010" ;
  reg:status reg:statusValid ;
  rdfs:label "filter expression processor"@en ;
  skos:changeNote "valid" ;
  skos:editorialNote "preferred"^^xsd:string ;
  skos:notation 1021 ;
  skos:prefLabel "filter expression processor"@en ;
.
<http://iso.org/tc211/term/1022>
  rdf:type skos:Concept ;
  dcterms:dateAccepted "2011-10-15"^^xsd:date ;
  dcterms:source "ISO 19118:2011, 4.21" ;
  reg:status reg:statusValid ;
  rdfs:label "identification convention"@en ;
  skos:changeNote "valid" ;
  skos:editorialNote "preferred"^^xsd:string ;
  skos:notation 1022 ;
  skos:prefLabel "identification convention"@en ;
.
<http://iso.org/tc211/term/1028>
  rdf:type skos:Concept ;
  dcterms:dateAccepted "2012-07-01"^^xsd:date ;
  dcterms:provenance "ISO 19144-2:2012, 4.1.9" ;
  dcterms:source "UNFAO LCCS 2:2005" ;
  reg:status reg:statusValid ;
  rdfs:comment "Note 1 to entry: The definition of land use in this way establishes a direct link between land cover and the actions of people in their environment. Multiple land uses can coexist at the same location (e.g. forestry and recreation), contrary to land cover classes that are mutually exclusive."@en ;
  rdfs:label "land use"@en ;
  skos:changeNote "valid" ;
  skos:editorialNote "preferred"^^xsd:string ;
  skos:notation 1028 ;
  skos:note "Note 1 to entry: The definition of land use in this way establishes a direct link between land cover and the actions of people in their environment. Multiple land uses can coexist at the same location (e.g. forestry and recreation), contrary to land cover classes that are mutually exclusive."@en ;
  skos:prefLabel "land use"@en ;
.
<http://iso.org/tc211/term/1029>
  rdf:type skos:Concept ;
  dcterms:dateAccepted "2010-10-15"^^xsd:date ;
  dcterms:source "ISO 19143:2010" ;
  reg:status reg:statusValid ;
  rdfs:comment "Note 1 to entry: This contrasts with a value that is determined by resolving a chain of substitution (e.g. a variable)"@en ;
  rdfs:label "literal value"@en ;
  skos:changeNote "valid" ;
  skos:editorialNote "preferred"^^xsd:string ;
  skos:notation 1029 ;
  skos:note "Note 1 to entry: This contrasts with a value that is determined by resolving a chain of substitution (e.g. a variable)"@en ;
  skos:prefLabel "literal value"@en ;
.
<http://iso.org/tc211/term/103>
  rdf:type skos:Concept ;
  dcterms:dateAccepted "2003-05-01"^^xsd:date ;
  dcterms:dateAccepted "2009-12-29"^^xsd:date ;
  dcterms:provenance "KS X ISO 19107" ;
  dcterms:source "ISO 19107:2003" ;
  reg:status reg:statusValid ;
  rdfs:comment "Note 1 to entry: Cycles are used to describe boundary components (see shell, ring). A cycle has no boundary because it closes on itself, but it is bounded (i.e., it does not have infinite extent).  A circle or a sphere, for example, has no boundary, but is bounded."@en ;
  rdfs:comment "비고: 순환은 경계 컴포넌트(외면, 링)의 기술에 사용된다. 순환은 스스로 완결되어 있지만 묶여 있기 때문에 경계가 없다. 예를 들어 원이나 구는 경계가 없지만 묶여 있다."@kr ;
  rdfs:label "cycle<geometry>"@en ;
  skos:changeNote "valid" ;
  skos:definition "경계가 없는 공간 객체"@kr ;
  skos:editorialNote "preferred" ;
  skos:editorialNote "preferred"^^xsd:string ;
  skos:notation "103" ;
  skos:notation 103 ;
  skos:note "Note 1 to entry: Cycles are used to describe boundary components (see shell, ring). A cycle has no boundary because it closes on itself, but it is bounded (i.e., it does not have infinite extent).  A circle or a sphere, for example, has no boundary, but is bounded."@en ;
  skos:note "비고: 순환은 경계 컴포넌트(외면, 링)의 기술에 사용된다. 순환은 스스로 완결되어 있지만 묶여 있기 때문에 경계가 없다. 예를 들어 원이나 구는 경계가 없지만 묶여 있다."@kr ;
  skos:prefLabel "cycle<geometry>"@en ;
  skos:prefLabel "순환<기하>"@kr ;
.
<http://iso.org/tc211/term/1036>
  rdf:type skos:Concept ;
  dcterms:dateAccepted "2010-12-15"^^xsd:date ;
  dcterms:source "ISO 19142:2010" ;
  reg:status reg:statusValid ;
  rdfs:label "relocate <reference>"@en ;
  skos:changeNote "valid" ;
  skos:editorialNote "preferred"^^xsd:string ;
  skos:notation 1036 ;
  skos:prefLabel "relocate <reference>"@en ;
.
<http://iso.org/tc211/term/104>
  rdf:type skos:Concept ;
  dcterms:dateAccepted "2005-07-15"^^xsd:date ;
  dcterms:dateAccepted "2008-12-19"^^xsd:date ;
  dcterms:provenance "ISO 19118:2011 ,4.8" ;
  dcterms:source "ISO/IEC 2382-1:1993" ;
  reg:status reg:statusValid ;
  rdfs:label "data"@en ;
  skos:changeNote "valid" ;
  skos:definition "정보를 의사소통, 해석, 처리에 적합한 형식으로 재해석 가능하도록 표현한 것"@kr ;
  skos:editorialNote "preferred" ;
  skos:editorialNote "preferred"^^xsd:string ;
  skos:notation "104" ;
  skos:notation 104 ;
  skos:prefLabel "data"@en ;
  skos:prefLabel "데이터"@kr ;
.
<http://iso.org/tc211/term/1042>
  rdf:type skos:Concept ;
  dcterms:dateAccepted "2010-12-15"^^xsd:date ;
  dcterms:source "ISO 19142:2010" ;
  reg:status reg:statusValid ;
  rdfs:comment "Note 1 to entry: This is the schema of feature types that a client can obtain using the DescribeFeatureType operation (see Clause 9)."@en ;
  rdfs:label "response model"@en ;
  skos:changeNote "valid" ;
  skos:editorialNote "preferred"^^xsd:string ;
  skos:notation 1042 ;
  skos:note "Note 1 to entry: This is the schema of feature types that a client can obtain using the DescribeFeatureType operation (see Clause 9)."@en ;
  skos:prefLabel "response model"@en ;
.
<http://iso.org/tc211/term/105>
  rdf:type skos:Concept ;
  dcterms:dateAccepted "2005-07-15"^^xsd:date ;
  dcterms:dateAccepted "2008-12-30"^^xsd:date ;
  dcterms:source "ISO 19118:2005, 4.9" ;
  reg:status reg:statusRetired ;
  rdfs:label "data element"@en ;
  skos:changeNote "retired" ;
  skos:definition "특정 상황에서 더 이상 나누어질 수 없는 데이터 단위"@kr ;
  skos:notation "105" ;
  skos:notation 105 ;
  skos:prefLabel "data element"@en ;
  skos:prefLabel "데이터 요소"@kr ;
.
<http://iso.org/tc211/term/1063>
  rdf:type skos:Concept ;
  dcterms:dateAccepted "2011-12-15"^^xsd:date ;
  dcterms:source "ISO 19156:2011, 4.4" ;
  reg:status reg:statusValid ;
  rdfs:comment "Note 1 to entry: This may be contrasted with observations and sampling features, which are features of types defined for cross-domain purposes."@en ;
  rdfs:label "domain feature"@en ;
  skos:changeNote "valid" ;
  skos:editorialNote "preferred"^^xsd:string ;
  skos:notation 1063 ;
  skos:note "Note 1 to entry: This may be contrasted with observations and sampling features, which are features of types defined for cross-domain purposes."@en ;
  skos:prefLabel "domain feature"@en ;
.
<http://iso.org/tc211/term/1069>
  rdf:type skos:Concept ;
  dcterms:dateAccepted "2009-02-15"^^xsd:date ;
  dcterms:source "ISO 19115-2:2009" ;
  reg:status reg:statusValid ;
  rdfs:label "grid coordinate system"@en ;
  skos:changeNote "valid" ;
  skos:editorialNote "preferred"^^xsd:string ;
  skos:notation 1069 ;
  skos:prefLabel "grid coordinate system"@en ;
.
<http://iso.org/tc211/term/107>
  rdf:type skos:Concept ;
  dcterms:dateAccepted "2005-07-15"^^xsd:date ;
  dcterms:dateAccepted "2008-12-30"^^xsd:date ;
  dcterms:provenance "ISO 19118:2005" ;
  dcterms:source "ISO 19118:2011, 4.9" ;
  reg:status reg:statusValid ;
  rdfs:label "data interchange"@en ;
  skos:changeNote "valid" ;
  skos:definition "데이터의 송수신 및 해석을 위한 처리 과정"@kr ;
  skos:editorialNote "preferred" ;
  skos:editorialNote "preferred"^^xsd:string ;
  skos:notation "107" ;
  skos:notation 107 ;
  skos:prefLabel "data interchange"@en ;
  skos:prefLabel "데이터 교환"@kr ;
.
<http://iso.org/tc211/term/1073>
  rdf:type skos:Concept ;
  dcterms:dateAccepted "2012-02-15"^^xsd:date ;
  dcterms:source "ISO 19148:2012, 4.9" ;
  reg:status reg:statusValid ;
  rdfs:comment "Note 1 to entry: Also known as curvilinear element."@en ;
  rdfs:label "linear element"@en ;
  skos:changeNote "valid" ;
  skos:editorialNote "preferred"^^xsd:string ;
  skos:notation 1073 ;
  skos:note "Note 1 to entry: Also known as curvilinear element."@en ;
  skos:prefLabel "linear element"@en ;
.
<http://iso.org/tc211/term/1079>
  rdf:type skos:Concept ;
  dcterms:dateAccepted "2012-02-15"^^xsd:date ;
  dcterms:source "ISO 19148:2012, 4.12" ;
  reg:status reg:statusValid ;
  rdfs:label "Linear Referencing System"@en ;
  skos:changeNote "valid" ;
  skos:editorialNote "preferred"^^xsd:string ;
  skos:notation 1079 ;
  skos:prefLabel "Linear Referencing System"@en ;
.
<http://iso.org/tc211/term/108>
  rdf:type skos:Concept ;
  dcterms:dateAccepted "2002-07-01"^^xsd:date ;
  dcterms:dateAccepted "2008-12-30"^^xsd:date ;
  dcterms:source "ISO 19101:2002, 4.8" ;
  reg:status reg:statusRetired ;
  rdfs:label "data level"@en ;
  skos:changeNote "retired" ;
  skos:definition "특정 인스턴스를 기술하고 있는 데이터가 포함된 레벨"@kr ;
  skos:notation "108" ;
  skos:notation 108 ;
  skos:prefLabel "data level"@en ;
  skos:prefLabel "데이터 층위"@kr ;
.
<http://iso.org/tc211/term/1081>
  rdf:type skos:Concept ;
  dcterms:dateAccepted "2012-02-15"^^xsd:date ;
  dcterms:source "ISO 19148:2012, 4.14" ;
  reg:status reg:statusValid ;
  rdfs:label "linearly located"@en ;
  skos:changeNote "valid" ;
  skos:editorialNote "preferred"^^xsd:string ;
  skos:notation 1081 ;
  skos:prefLabel "linearly located"@en ;
.
<http://iso.org/tc211/term/1097>
  rdf:type skos:Concept ;
  dcterms:dateAccepted "2012-10-15"^^xsd:date ;
  dcterms:provenance "ISO/TS 19158:2012, 4.3" ;
  dcterms:source "ISO 9000:2005" ;
  reg:status reg:statusValid ;
  rdfs:label "product"@en ;
  skos:changeNote "valid" ;
  skos:editorialNote "preferred"^^xsd:string ;
  skos:notation 1097 ;
  skos:prefLabel "product"@en ;
.
<http://iso.org/tc211/term/11>
  rdf:type skos:Concept ;
  dcterms:dateAccepted "2005-07-15"^^xsd:date ;
  dcterms:dateAccepted "2009-12-29"^^xsd:date ;
  dcterms:provenance "ISO/TS 19103:2005" ;
  dcterms:provenance "KS X ISO 19103" ;
  dcterms:source "ISO/IEC 19501:2005 (Adapted from)" ;
  reg:status reg:statusValid ;
  rdfs:comment "Note 1 to entry: See composition"@en ;
  rdfs:comment "비고: 합성 참고"@kr ;
  rdfs:label "aggregation <UML>"@en ;
  skos:changeNote "valid" ;
  skos:definition "집합체와 컴포넌트 간의 관계를 설명한 연관의 특정 형태"@kr ;
  skos:editorialNote "preferred" ;
  skos:editorialNote "preferred"^^xsd:string ;
  skos:notation "11" ;
  skos:notation 11 ;
  skos:note "Note 1 to entry: See composition"@en ;
  skos:note "비고: 합성 참고"@kr ;
  skos:prefLabel "aggregation <UML>"@en ;
  skos:prefLabel "집합 연관 <UML>"@kr ;
.
<http://iso.org/tc211/term/110>
  rdf:type skos:Concept ;
  dcterms:dateAccepted "2007-04-15"^^xsd:date ;
  dcterms:dateAccepted "2008-12-01"^^xsd:date ;
  dcterms:provenance "KS X ISO 19131" ;
  dcterms:source "ISO 19131:2007" ;
  reg:status reg:statusValid ;
  rdfs:label "data product"@en ;
  skos:changeNote "valid" ;
  skos:definition "데이터 제품 사양을 따르는 데이터셋 또는 데이터셋 시리즈"@kr ;
  skos:editorialNote "preferred" ;
  skos:editorialNote "preferred"^^xsd:string ;
  skos:notation "110" ;
  skos:notation 110 ;
  skos:prefLabel "data product"@en ;
  skos:prefLabel "데이터 제품"@kr ;
.
<http://iso.org/tc211/term/1102>
  rdf:type skos:Concept ;
  dcterms:dateAccepted "2011-04-27"^^xsd:date ;
  dcterms:provenance "ISO/TS 19158" ;
  dcterms:source "ISO 9000:2005" ;
  reg:status reg:statusValid ;
  rdfs:comment "Note 1 to entry: For the purposes of this Technical Specification the quality characteristics of product include: Data quality (the elements of which are described by ISO 19157), Volume of delivery, Schedule of delivery, and Cost of production and/or update."@en ;
  rdfs:label "quality"@en ;
  skos:changeNote "valid" ;
  skos:editorialNote "preferred"^^xsd:string ;
  skos:notation 1102 ;
  skos:note "Note 1 to entry: For the purposes of this Technical Specification the quality characteristics of product include: Data quality (the elements of which are described by ISO 19157), Volume of delivery, Schedule of delivery, and Cost of production and/or update."@en ;
  skos:prefLabel "quality"@en ;
.
<http://iso.org/tc211/term/1108>
  rdf:type skos:Concept ;
  dcterms:dateAccepted "2009-02-15"^^xsd:date ;
  dcterms:provenance "ISO 19115-2:2009" ;
  dcterms:source "ISO/IEC GUIDE 99:2007" ;
  reg:status reg:statusValid ;
  rdfs:label "sensor"@en ;
  skos:changeNote "valid" ;
  skos:editorialNote "preferred"^^xsd:string ;
  skos:notation 1108 ;
  skos:prefLabel "sensor"@en ;
.
<http://iso.org/tc211/term/111>
  rdf:type skos:Concept ;
  dcterms:dateAccepted "2007-04-15"^^xsd:date ;
  dcterms:dateAccepted "2008-12-01"^^xsd:date ;
  dcterms:provenance "KS X ISO 19131" ;
  dcterms:source "ISO 19131:2007" ;
  reg:status reg:statusValid ;
  rdfs:comment "Note 1 to entry: A data product specification provides a description of the universe of discourse and a specification for mapping the universe of discourse to a dataset. It may be used for production, sales, end-use or other purposes."@en ;
  rdfs:comment "비고: 데이터 제품 사양은 논의의 영역에 대한 설명과 그 논의의 영역과 데이터셋을 매핑하기 위한 사양을 제공한다. 데이터 제품 사양은 생산, 판매, 최종 사용 또는 기타 목적을 위해 사용할 수 있다."@kr ;
  rdfs:label "data product specification"@en ;
  skos:changeNote "valid" ;
  skos:definition "데이터 제품에 대하여 제3자가 이를 생성, 공급, 사용하는 데 필요한 정보를 제공하는 데이터셋 또는 데이터셋 시리즈의 상세 설명 "@kr ;
  skos:editorialNote "preferred" ;
  skos:editorialNote "preferred"^^xsd:string ;
  skos:notation "111" ;
  skos:notation 111 ;
  skos:note "Note 1 to entry: A data product specification provides a description of the universe of discourse and a specification for mapping the universe of discourse to a dataset. It may be used for production, sales, end-use or other purposes."@en ;
  skos:note "비고: 데이터 제품 사양은 논의의 영역에 대한 설명과 그 논의의 영역과 데이터셋을 매핑하기 위한 사양을 제공한다. 데이터 제품 사양은 생산, 판매, 최종 사용 또는 기타 목적을 위해 사용할 수 있다."@kr ;
  skos:prefLabel "data product specification"@en ;
  skos:prefLabel "데이터 제품 사양"@kr ;
.
<http://iso.org/tc211/term/1111>
  rdf:type skos:Concept ;
  dcterms:dateAccepted "2012-10-15"^^xsd:date ;
  dcterms:source "ISO/TS 19158:2012, 4.10" ;
  reg:status reg:statusValid ;
  rdfs:comment "Note 1 to entry: Sub-processes can be broken down even further as is deemed necessary to control the quality of the process."@en ;
  rdfs:label "sub-process"@en ;
  skos:changeNote "valid" ;
  skos:editorialNote "preferred"^^xsd:string ;
  skos:notation 1111 ;
  skos:note "Note 1 to entry: Sub-processes can be broken down even further as is deemed necessary to control the quality of the process."@en ;
  skos:prefLabel "sub-process"@en ;
.
<http://iso.org/tc211/term/1118>
  rdf:type skos:Concept ;
  dcterms:dateAccepted "2009-04-01"^^xsd:date ;
  dcterms:source "ISO/TS 19129:2009" ;
  reg:status reg:statusValid ;
  rdfs:comment "Note 1 to entry: Adapted from ANSI T1.523-2001."@en ;
  rdfs:comment "Note 2 to entry: Data compression is probabilistic in nature based on particular instances of imagery, gridded or coverage data and is related to encoding and is outside the scope of this Technical Specification." ;
  rdfs:label "data compression"@en ;
  skos:changeNote "valid" ;
  skos:editorialNote "preferred"^^xsd:string ;
  skos:notation 1118 ;
  skos:note "Note 1 to entry: Adapted from ANSI T1.523-2001."@en ;
  skos:note "Note 2 to entry: Data compression is probabilistic in nature based on particular instances of imagery, gridded or coverage data and is related to encoding and is outside the scope of this Technical Specification."^^<http://www.w3.org/2001/XMLSchema#@en> ;
  skos:prefLabel "data compression"@en ;
.
<http://iso.org/tc211/term/1119>
  rdf:type skos:Concept ;
  dcterms:dateAccepted "2010-06-15"^^xsd:date ;
  dcterms:source "ISO/TS 19130:2010" ;
  reg:status reg:statusValid ;
  rdfs:label "detector"@en ;
  skos:changeNote "valid" ;
  skos:editorialNote "preferred"^^xsd:string ;
  skos:notation 1119 ;
  skos:prefLabel "detector"@en ;
.
<http://iso.org/tc211/term/112>
  rdf:type skos:Concept ;
  dcterms:dateAccepted "2002-12-01"^^xsd:date ;
  dcterms:dateAccepted "2007-11-01"^^xsd:date ;
  dcterms:source "ISO 19113:2002, 4.4" ;
  reg:status reg:statusRetired ;
  rdfs:label "data quality date"@en ;
  skos:changeNote "retired" ;
  skos:definition "데이터 품질 측정을 실시한 일자 또는 범위"@kr ;
  skos:notation "112" ;
  skos:notation 112 ;
  skos:prefLabel "data quality date"@en ;
  skos:prefLabel "데이터 품질 일자"@kr ;
.
<http://iso.org/tc211/term/1121>
  rdf:type skos:Concept ;
  dcterms:dateAccepted "2010-06-15"^^xsd:date ;
  dcterms:source "ISO/TS 19130:2010" ;
  reg:status reg:statusValid ;
  rdfs:label "external coordinate reference system"@en ;
  skos:changeNote "valid" ;
  skos:editorialNote "preferred"^^xsd:string ;
  skos:notation 1121 ;
  skos:prefLabel "external coordinate reference system"@en ;
.
<http://iso.org/tc211/term/1122>
  rdf:type skos:Concept ;
  dcterms:dateAccepted "2010-06-15"^^xsd:date ;
  dcterms:source "ISO/TS 19130:2010" ;
  reg:status reg:statusValid ;
  rdfs:comment "Note 1 to entry: An object mounted on a three-ring gimbal will remain horizontally suspended on a plane between the rings regardless as to the stability of the base."@en ;
  rdfs:label "gimbal"@en ;
  skos:changeNote "valid" ;
  skos:editorialNote "preferred"^^xsd:string ;
  skos:notation 1122 ;
  skos:note "Note 1 to entry: An object mounted on a three-ring gimbal will remain horizontally suspended on a plane between the rings regardless as to the stability of the base."@en ;
  skos:prefLabel "gimbal"@en ;
.
<http://iso.org/tc211/term/1123>
  rdf:type skos:Concept ;
  dcterms:dateAccepted "2010-06-15"^^xsd:date ;
  dcterms:source "ISO/TS 19130:2010" ;
  reg:status reg:statusValid ;
  rdfs:comment "Note 1 to entry:  The rotor spins on a fixed axis while the structure around it rotates or tilts. In airplanes, the pitch and orientation of the airplane is measured against the steady spin of the gyroscope. In space, where the four compass points are meaningless, the gyroscope's axis of rotation is used as a reference point for navigation. An inertial navigation system includes three gimbal-mounted gyroscopes, used to measure roll, pitch, and yaw."@en ;
  rdfs:label "gyroscope"@en ;
  skos:changeNote "valid" ;
  skos:editorialNote "preferred"^^xsd:string ;
  skos:notation 1123 ;
  skos:note "Note 1 to entry:  The rotor spins on a fixed axis while the structure around it rotates or tilts. In airplanes, the pitch and orientation of the airplane is measured against the steady spin of the gyroscope. In space, where the four compass points are meaningless, the gyroscope's axis of rotation is used as a reference point for navigation. An inertial navigation system includes three gimbal-mounted gyroscopes, used to measure roll, pitch, and yaw."@en ;
  skos:prefLabel "gyroscope"@en ;
.
<http://iso.org/tc211/term/1124>
  rdf:type skos:Concept ;
  dcterms:dateAccepted "2010-06-15"^^xsd:date ;
  dcterms:source "ISO/TS 19130:2010" ;
  reg:status reg:statusValid ;
  rdfs:comment "Note 1 to entry: The electromagnetic radiation is at microwave frequencies and is sent in pulses."@en ;
  rdfs:label "Synthetic Aperture Radar"@en ;
  skos:altLabel "SAR"^^<http://www.w3.org/2001/XMLSchema#@en> ;
  skos:changeNote "valid" ;
  skos:editorialNote "preferred"^^xsd:string ;
  skos:notation 1124 ;
  skos:note "Note 1 to entry: The electromagnetic radiation is at microwave frequencies and is sent in pulses."@en ;
  skos:prefLabel "Synthetic Aperture Radar"@en ;
.
<http://iso.org/tc211/term/1125>
  rdf:type skos:Concept ;
  dcterms:dateAccepted "2010-06-15"^^xsd:date ;
  dcterms:source "ISO/TS 19130:2010" ;
  reg:status reg:statusValid ;
  rdfs:comment "Note 1 to entry: Doppler angle in processed products is fixed for all pixels. It provides the ability to collect SAR data over strips of land over a fixed swath of ground range parallel to the direction of flight."@en ;
  rdfs:label "stripmap mode <SAR>"@en ;
  skos:changeNote "valid" ;
  skos:editorialNote "preferred"^^xsd:string ;
  skos:notation 1125 ;
  skos:note "Note 1 to entry: Doppler angle in processed products is fixed for all pixels. It provides the ability to collect SAR data over strips of land over a fixed swath of ground range parallel to the direction of flight."@en ;
  skos:prefLabel "stripmap mode <SAR>"@en ;
.
<http://iso.org/tc211/term/1126>
  rdf:type skos:Concept ;
  dcterms:dateAccepted "2010-06-15"^^xsd:date ;
  dcterms:source "ISO/TS 19130:2010" ;
  reg:status reg:statusValid ;
  rdfs:label "whiskbroom sensor"@en ;
  skos:changeNote "valid" ;
  skos:editorialNote "preferred"^^xsd:string ;
  skos:notation 1126 ;
  skos:prefLabel "whiskbroom sensor"@en ;
.
<http://iso.org/tc211/term/113>
  rdf:type skos:Concept ;
  dcterms:dateAccepted "2002-07-01"^^xsd:date ;
  dcterms:dateAccepted "2008-12-30"^^xsd:date ;
  dcterms:source "ISO 19101:2002, 4.9" ;
  reg:status reg:statusRetired ;
  rdfs:comment "Note 1 to entry: The applicability of a data quality element to a dataset depends on both the dataset's content and its product specification; the result being that all data elements may not be applicable to all datasets."@en ;
  rdfs:comment "비고: 데이터셋에 대한 데이터 품질 요소의 적용 여부는 데이터셋의 내용과 그 제품 사양 모두에 달려 있다. 모든 데이터 요소를 모든 데이터셋에 적용하는 것은 어려울 수 있다."@kr ;
  rdfs:label "data quality element"@en ;
  skos:changeNote "retired" ;
  skos:definition "품질정보를 기술하는 데이터셋의 정량적 컴포넌트"@kr ;
  skos:notation "113" ;
  skos:notation 113 ;
  skos:note "Note 1 to entry: The applicability of a data quality element to a dataset depends on both the dataset's content and its product specification; the result being that all data elements may not be applicable to all datasets."@en ;
  skos:note "비고: 데이터셋에 대한 데이터 품질 요소의 적용 여부는 데이터셋의 내용과 그 제품 사양 모두에 달려 있다. 모든 데이터 요소를 모든 데이터셋에 적용하는 것은 어려울 수 있다."@kr ;
  skos:prefLabel "data quality element"@en ;
  skos:prefLabel "데이터 품질 요소"@kr ;
.
<http://iso.org/tc211/term/114>
  rdf:type skos:Concept ;
  dcterms:dateAccepted "2002-12-01"^^xsd:date ;
  dcterms:dateAccepted "2007-11-01"^^xsd:date ;
  dcterms:source "ISO 19113:2002, 4.6" ;
  reg:status reg:statusRetired ;
  rdfs:label "data quality evaluation procedure"@en ;
  skos:changeNote "retired" ;
  skos:definition "품질 산출 방법을 적용하여 그 결과를 보고하는 절차"@kr ;
  skos:notation "114" ;
  skos:notation 114 ;
  skos:prefLabel "data quality evaluation procedure"@en ;
  skos:prefLabel "데이터 품질 평가 절차"@kr ;
.
<http://iso.org/tc211/term/115>
  rdf:type skos:Concept ;
  dcterms:dateAccepted "2002-12-01"^^xsd:date ;
  dcterms:dateAccepted "2007-11-01"^^xsd:date ;
  dcterms:source "ISO 19113:2002, 4.7" ;
  reg:status reg:statusRetired ;
  rdfs:label "data quality measure"@en ;
  skos:changeNote "retired" ;
  skos:definition "데이터 품질 하위 요소의 산출"@kr ;
  skos:notation "115" ;
  skos:notation 115 ;
  skos:prefLabel "data quality measure"@en ;
  skos:prefLabel "데이터 품질 측정"@kr ;
.
<http://iso.org/tc211/term/1159>
  rdf:type skos:Concept ;
  dcterms:dateAccepted "2013-02-15"^^xsd:date ;
  dcterms:source "ISO 19145:2013, 4.1.1" ;
  reg:status reg:statusValid ;
  rdfs:label "compression"@en ;
  skos:changeNote "valid" ;
  skos:editorialNote "preferred"^^xsd:string ;
  skos:notation 1159 ;
  skos:prefLabel "compression"@en ;
.
<http://iso.org/tc211/term/116>
  rdf:type skos:Concept ;
  dcterms:dateAccepted "2002-07-01"^^xsd:date ;
  dcterms:dateAccepted "2008-12-30"^^xsd:date ;
  dcterms:source "ISO 19101:2002, 4.10" ;
  reg:status reg:statusRetired ;
  rdfs:comment "Note 1 to entry: Information about the purpose, usage, and lineage of a dataset is non-quantitative information."@en ;
  rdfs:comment "비고: 데이터셋의 목적, 사용법, 그리고 연혁에 대한 정보는 비정량적 정보이다."@kr ;
  rdfs:label "data quality overview element"@en ;
  skos:changeNote "retired" ;
  skos:definition "데이터셋의 품질을 기술하는 비정량적 컴포넌트"@kr ;
  skos:notation "116" ;
  skos:notation 116 ;
  skos:note "Note 1 to entry: Information about the purpose, usage, and lineage of a dataset is non-quantitative information."@en ;
  skos:note "비고: 데이터셋의 목적, 사용법, 그리고 연혁에 대한 정보는 비정량적 정보이다."@kr ;
  skos:prefLabel "data quality overview element"@en ;
  skos:prefLabel "데이터 품질 개관 요소"@kr ;
.
<http://iso.org/tc211/term/1160>
  rdf:type skos:Concept ;
  dcterms:dateAccepted "2013-02-15"^^xsd:date ;
  dcterms:source "ISO 19145:2013, 4.1.2" ;
  reg:status reg:statusValid ;
  rdfs:label "compression service"@en ;
  skos:changeNote "valid" ;
  skos:editorialNote "preferred"^^xsd:string ;
  skos:notation 1160 ;
  skos:prefLabel "compression service"@en ;
.
<http://iso.org/tc211/term/1161>
  rdf:type skos:Concept ;
  dcterms:dateAccepted "2013-02-15"^^xsd:date ;
  dcterms:source "ISO 19145:2013, 4.1.3" ;
  reg:status reg:statusValid ;
  rdfs:label "conversion"@en ;
  skos:changeNote "valid" ;
  skos:editorialNote "preferred"^^xsd:string ;
  skos:notation 1161 ;
  skos:prefLabel "conversion"@en ;
.
<http://iso.org/tc211/term/1162>
  rdf:type skos:Concept ;
  dcterms:dateAccepted "2013-02-15"^^xsd:date ;
  dcterms:source "ISO 19145:2013, 4.1.4" ;
  reg:status reg:statusValid ;
  rdfs:label "conversion service"@en ;
  skos:changeNote "valid" ;
  skos:editorialNote "preferred"^^xsd:string ;
  skos:notation 1162 ;
  skos:prefLabel "conversion service"@en ;
.
<http://iso.org/tc211/term/1164>
  rdf:type skos:Concept ;
  dcterms:dateAccepted "2013-02-15"^^xsd:date ;
  dcterms:source "ISO 19145:2013, 4.1.8" ;
  reg:status reg:statusValid ;
  rdfs:label "dynamic conversion"@en ;
  skos:changeNote "valid" ;
  skos:editorialNote "preferred"^^xsd:string ;
  skos:notation 1164 ;
  skos:prefLabel "dynamic conversion"@en ;
.
<http://iso.org/tc211/term/1165>
  rdf:type skos:Concept ;
  dcterms:dateAccepted "2013-02-15"^^xsd:date ;
  dcterms:provenance "ISO 19145:2013, 4.1.9" ;
  dcterms:source "ISO/IEC 2382-15:1999" ;
  reg:status reg:statusValid ;
  rdfs:label "format"@en ;
  skos:changeNote "valid" ;
  skos:editorialNote "preferred"^^xsd:string ;
  skos:notation 1165 ;
  skos:prefLabel "format"@en ;
.
<http://iso.org/tc211/term/1166>
  rdf:type skos:Concept ;
  dcterms:dateAccepted "2013-02-15"^^xsd:date ;
  dcterms:source "ISO 19145:2013, 4.1.11" ;
  reg:status reg:statusValid ;
  rdfs:label "geographic point location"@en ;
  skos:changeNote "valid" ;
  skos:editorialNote "preferred"^^xsd:string ;
  skos:notation 1166 ;
  skos:prefLabel "geographic point location"@en ;
.
<http://iso.org/tc211/term/1167>
  rdf:type skos:Concept ;
  dcterms:dateAccepted "2013-02-15"^^xsd:date ;
  dcterms:source "ISO 19145:2013, 4.1.12" ;
  reg:status reg:statusValid ;
  rdfs:label "geographic point location representation"@en ;
  skos:changeNote "valid" ;
  skos:editorialNote "preferred"^^xsd:string ;
  skos:notation 1167 ;
  skos:prefLabel "geographic point location representation"@en ;
.
<http://iso.org/tc211/term/1168>
  rdf:type skos:Concept ;
  dcterms:dateAccepted "2013-02-15"^^xsd:date ;
  dcterms:source "ISO 19145:2013, 4.1.17" ;
  reg:status reg:statusValid ;
  rdfs:label "static conversion"@en ;
  skos:changeNote "valid" ;
  skos:editorialNote "preferred"^^xsd:string ;
  skos:notation 1168 ;
  skos:prefLabel "static conversion"@en ;
.
<http://iso.org/tc211/term/1169>
  rdf:type skos:Concept ;
  dcterms:dateAccepted "2012-02-15"^^xsd:date ;
  dcterms:source "ISO 19148:2012, 4.1" ;
  reg:status reg:statusValid ;
  rdfs:comment "Note 1 to entry: An attribute event includes the linearly referenced location where the attribute value applies along the attributed feature"@en ;
  rdfs:comment "Note 2 to entry: An attribute event may be qualified by the instant in which, or period during which, the attribute value applied" ;
  rdfs:label "attribute event"@en ;
  skos:changeNote "valid" ;
  skos:editorialNote "preferred"^^xsd:string ;
  skos:notation 1169 ;
  skos:note "Note 1 to entry: An attribute event includes the linearly referenced location where the attribute value applies along the attributed feature"@en ;
  skos:note "Note 2 to entry: An attribute event may be qualified by the instant in which, or period during which, the attribute value applied"^^<http://www.w3.org/2001/XMLSchema#@en> ;
  skos:prefLabel "attribute event"@en ;
.
<http://iso.org/tc211/term/117>
  rdf:type skos:Concept ;
  dcterms:dateAccepted "2002-12-01"^^xsd:date ;
  dcterms:dateAccepted "2007-11-01"^^xsd:date ;
  dcterms:source "ISO 19113:2002, 4.9" ;
  reg:status reg:statusRetired ;
  rdfs:label "data quality result"@en ;
  skos:changeNote "retired" ;
  skos:definition "데이터 품질 측정의 결과 값이나 값의 집합 또는 이를 정해진 적합성 품질 수준에 따라 평가한 결과"@kr ;
  skos:notation "117" ;
  skos:notation 117 ;
  skos:prefLabel "data quality result"@en ;
  skos:prefLabel "데이터 품질 결과"@kr ;
.
<http://iso.org/tc211/term/1170>
  rdf:type skos:Concept ;
  dcterms:dateAccepted "2012-02-15"^^xsd:date ;
  dcterms:source "ISO 19148:2012, 4.2" ;
  reg:status reg:statusValid ;
  rdfs:label "attributed feature"@en ;
  skos:changeNote "valid" ;
  skos:editorialNote "preferred"^^xsd:string ;
  skos:notation 1170 ;
  skos:prefLabel "attributed feature"@en ;
.
<http://iso.org/tc211/term/1171>
  rdf:type skos:Concept ;
  dcterms:dateAccepted "2012-02-15"^^xsd:date ;
  dcterms:source "ISO 19148:2012, 4.5" ;
  reg:status reg:statusValid ;
  rdfs:comment "Note 1 to entry: A feature event includes the linearly referenced location of the located feature along the locating feature."@en ;
  rdfs:comment "Note 2 to entry: A feature event may be qualified by the instant in which, or period during which, the feature event occurred." ;
  rdfs:label "feature event"@en ;
  skos:changeNote "valid" ;
  skos:editorialNote "preferred"^^xsd:string ;
  skos:notation 1171 ;
  skos:note "Note 1 to entry: A feature event includes the linearly referenced location of the located feature along the locating feature."@en ;
  skos:note "Note 2 to entry: A feature event may be qualified by the instant in which, or period during which, the feature event occurred."^^<http://www.w3.org/2001/XMLSchema#@en> ;
  skos:prefLabel "feature event"@en ;
.
<http://iso.org/tc211/term/1172>
  rdf:type skos:Concept ;
  dcterms:dateAccepted "2012-02-15"^^xsd:date ;
  dcterms:source "ISO 19148:2012, 4.10" ;
  reg:status reg:statusValid ;
  rdfs:comment "Note 1 to entry: An alternative to specifying a location as a two- or three- dimensional spatial position."@en ;
  rdfs:label "linear referencing"@en ;
  skos:changeNote "valid" ;
  skos:editorialNote "preferred"^^xsd:string ;
  skos:notation 1172 ;
  skos:note "Note 1 to entry: An alternative to specifying a location as a two- or three- dimensional spatial position."@en ;
  skos:prefLabel "linear referencing"@en ;
.
<http://iso.org/tc211/term/1173>
  rdf:type skos:Concept ;
  dcterms:dateAccepted "2012-02-15"^^xsd:date ;
  dcterms:source "ISO 19148:2012, 4.13" ;
  reg:status reg:statusValid ;
  rdfs:comment "Note 1 to entry: A linear segment is a one-dimensional object without explicit geometry."@en ;
  rdfs:comment "Note 2 to entry: The implicit geometry of the linear segment can be derived from the geometry of the parent feature." ;
  rdfs:label "linear segment"@en ;
  skos:changeNote "valid" ;
  skos:editorialNote "preferred"^^xsd:string ;
  skos:notation 1173 ;
  skos:note "Note 1 to entry: A linear segment is a one-dimensional object without explicit geometry."@en ;
  skos:note "Note 2 to entry: The implicit geometry of the linear segment can be derived from the geometry of the parent feature."^^<http://www.w3.org/2001/XMLSchema#@en> ;
  skos:prefLabel "linear segment"@en ;
.
<http://iso.org/tc211/term/1174>
  rdf:type skos:Concept ;
  dcterms:dateAccepted "2012-02-15"^^xsd:date ;
  dcterms:source "ISO 19148:2012, 4.15" ;
  reg:status reg:statusValid ;
  rdfs:comment "Note 1 to entry: The event location is specified using linearly referenced locations."@en ;
  rdfs:comment "Note 2 to entry: A linearly located event may be qualified by the instant in which, or period during which, the linearly located event occurred." ;
  rdfs:comment "Note 3 to entry: ISO 19108 limits events to a single instant in time and does not include the specification of a location."@en ;
  rdfs:label "linearly located event"@en ;
  skos:changeNote "valid" ;
  skos:editorialNote "preferred"^^xsd:string ;
  skos:notation 1174 ;
  skos:note "Note 1 to entry: The event location is specified using linearly referenced locations."@en ;
  skos:note "Note 2 to entry: A linearly located event may be qualified by the instant in which, or period during which, the linearly located event occurred."^^<http://www.w3.org/2001/XMLSchema#@en> ;
  skos:note "Note 3 to entry: ISO 19108 limits events to a single instant in time and does not include the specification of a location."^^<http://www.w3.org/2001/XMLSchema#@en> ;
  skos:prefLabel "linearly located event"@en ;
.
<http://iso.org/tc211/term/1175>
  rdf:type skos:Concept ;
  dcterms:dateAccepted "2012-02-15"^^xsd:date ;
  dcterms:source "ISO 19148:2012, 4.16" ;
  reg:status reg:statusValid ;
  rdfs:label "linearly referenced location"@en ;
  skos:changeNote "valid" ;
  skos:editorialNote "preferred"^^xsd:string ;
  skos:notation 1175 ;
  skos:prefLabel "linearly referenced location"@en ;
.
<http://iso.org/tc211/term/1176>
  rdf:type skos:Concept ;
  dcterms:dateAccepted "2012-02-15"^^xsd:date ;
  dcterms:source "ISO 19148:2012, 4.17" ;
  reg:status reg:statusValid ;
  rdfs:label "located feature"@en ;
  skos:changeNote "valid" ;
  skos:editorialNote "preferred"^^xsd:string ;
  skos:notation 1176 ;
  skos:prefLabel "located feature"@en ;
.
<http://iso.org/tc211/term/1177>
  rdf:type skos:Concept ;
  dcterms:dateAccepted "2012-02-15"^^xsd:date ;
  dcterms:source "ISO 19148:2012, 4.18" ;
  reg:status reg:statusValid ;
  rdfs:label "locating feature"@en ;
  skos:changeNote "valid" ;
  skos:editorialNote "preferred"^^xsd:string ;
  skos:notation 1177 ;
  skos:prefLabel "locating feature"@en ;
.
<http://iso.org/tc211/term/1178>
  rdf:type skos:Concept ;
  dcterms:dateAccepted "2012-02-15"^^xsd:date ;
  dcterms:source "ISO 19148:2012, 4.22" ;
  reg:status reg:statusValid ;
  rdfs:comment "Note 1 to entry: An alternative to specifying a location as a linearly referenced location."@en ;
  rdfs:label "spatial position"@en ;
  skos:changeNote "valid" ;
  skos:editorialNote "preferred"^^xsd:string ;
  skos:notation 1178 ;
  skos:note "Note 1 to entry: An alternative to specifying a location as a linearly referenced location."@en ;
  skos:prefLabel "spatial position"@en ;
.
<http://iso.org/tc211/term/118>
  rdf:type skos:Concept ;
  dcterms:dateAccepted "2002-12-01"^^xsd:date ;
  dcterms:dateAccepted "2007-11-01"^^xsd:date ;
  dcterms:source "ISO 19113:2002, 4.10" ;
  reg:status reg:statusRetired ;
  rdfs:comment "Note 1 to entry: A data quality scope for a dataset can comprise a dataset series to which the dataset belongs, the dataset itself, or a smaller grouping of data located physically within the dataset sharing common characteristics. Common characteristics can be an identified feature type, feature attribute, or feature relationship; data collection criteria; original source; or a specified geographic or temporal extent."@en ;
  rdfs:comment "비고: 데이터셋에 대한 데이터 품질 범위는 데이터셋에 속하거나, 데이터셋 자체 또는 공통적인 특징을 공유하는 데이터셋 내에 물리적으로 위치하는 보다 작은 그룹의 데이터와 같은 데이터셋 시리즈를 포함한다. 식별된 피처 유형, 피처 속성, 피처 관계(데이터 수집 기준, 원천 데이터, 특정한 지리적 또는 시간적 범위)가 공통적인 특징이 될 수 있다."@kr ;
  rdfs:label "data quality scope"@en ;
  skos:changeNote "retired" ;
  skos:definition "품질 정보가 기록된 데이터의 범위 혹은 특성"@kr ;
  skos:notation "118" ;
  skos:notation 118 ;
  skos:note "Note 1 to entry: A data quality scope for a dataset can comprise a dataset series to which the dataset belongs, the dataset itself, or a smaller grouping of data located physically within the dataset sharing common characteristics. Common characteristics can be an identified feature type, feature attribute, or feature relationship; data collection criteria; original source; or a specified geographic or temporal extent."@en ;
  skos:note "비고: 데이터셋에 대한 데이터 품질 범위는 데이터셋에 속하거나, 데이터셋 자체 또는 공통적인 특징을 공유하는 데이터셋 내에 물리적으로 위치하는 보다 작은 그룹의 데이터와 같은 데이터셋 시리즈를 포함한다. 식별된 피처 유형, 피처 속성, 피처 관계(데이터 수집 기준, 원천 데이터, 특정한 지리적 또는 시간적 범위)가 공통적인 특징이 될 수 있다."@kr ;
  skos:prefLabel "data quality scope"@en ;
  skos:prefLabel "데이터 품질 범위"@kr ;
.
<http://iso.org/tc211/term/119>
  rdf:type skos:Concept ;
  dcterms:dateAccepted "2002-12-01"^^xsd:date ;
  dcterms:dateAccepted "2007-11-01"^^xsd:date ;
  dcterms:source "ISO 19113:2002, 4.11" ;
  reg:status reg:statusRetired ;
  rdfs:label "data quality subelement"@en ;
  skos:changeNote "retired" ;
  skos:definition "데이터 품질 요소의 특정한 측면을 설명하는 컴포넌트"@kr ;
  skos:notation "119" ;
  skos:notation 119 ;
  skos:prefLabel "data quality subelement"@en ;
  skos:prefLabel "데이터 품질 하위 요소"@kr ;
.
<http://iso.org/tc211/term/1197>
  rdf:type skos:Concept ;
  dcterms:dateAccepted "2012-12-01"^^xsd:date ;
  dcterms:source "ISO 19152:2012, 4.1.18" ;
  reg:status reg:statusValid ;
  rdfs:label "responsibility"@en ;
  skos:changeNote "valid" ;
  skos:editorialNote "preferred"^^xsd:string ;
  skos:notation 1197 ;
  skos:prefLabel "responsibility"@en ;
.
<http://iso.org/tc211/term/12>
  rdf:type skos:Concept ;
  dcterms:dateAccepted "2004-07-01"^^xsd:date ;
  dcterms:dateAccepted "2004-11-05"^^xsd:date ;
  dcterms:provenance "KS X ISO 19116" ;
  dcterms:source "ISO 19116:2004" ;
  reg:status reg:statusSuperseded ;
  rdfs:comment "Note 1 to entry: See ellipsoidal height and gravity-related height."@en ;
  rdfs:comment "Note 2 to entry: Height of a point outside the surface treated as positive; negative height is designated as depth." ;
  rdfs:comment "비고 1: 타원체의 높이와 중력과 관련된 높이 참조"@kr ;
  rdfs:label "altitude"@en ;
  rdfs:seeAlso "height" ;
  skos:altLabel "h or H"^^<http://www.w3.org/2001/XMLSchema#@en> ;
  skos:altLabel "h; H"@kr ;
  skos:altLabel "height"@en ;
  skos:changeNote "superseded" ;
  skos:definition "선택된 기준면으로부터 그 면의 수직선으로 연결된 어떤 지점까지의 거리"@kr ;
  skos:notation "12" ;
  skos:notation 12 ;
  skos:note "Note 1 to entry: See ellipsoidal height and gravity-related height."@en ;
  skos:note "Note 2 to entry: Height of a point outside the surface treated as positive; negative height is designated as depth."^^<http://www.w3.org/2001/XMLSchema#@en> ;
  skos:note "비고 1: 타원체의 높이와 중력과 관련된 높이 참조"@kr ;
  skos:note "비고 2: 양으로 여겨지는 표면 외부 지점의 높이, 음의 높이는 깊이라고 불린다. "@kr ;
  skos:prefLabel "altitude"@en ;
  skos:prefLabel "높이"@kr ;
.
<http://iso.org/tc211/term/120>
  rdf:type skos:Concept ;
  dcterms:dateAccepted "2002-12-01"^^xsd:date ;
  dcterms:dateAccepted "2007-11-01"^^xsd:date ;
  dcterms:source "ISO 19113:2002, 4.12" ;
  reg:status reg:statusRetired ;
  rdfs:comment "Note 1 to entry: A data quality value type is always provided for a data quality result."@en ;
  rdfs:comment "비고: 데이터 품질 값 유형은 항상 데이터 품질 결과를 규정한다."@kr ;
  rdfs:label "data quality value type"@en ;
  skos:changeNote "retired" ;
  skos:definition "데이터 품질 결과를 보고하는 값의 유형"@kr ;
  skos:notation "120" ;
  skos:notation 120 ;
  skos:note "Note 1 to entry: A data quality value type is always provided for a data quality result."@en ;
  skos:note "비고: 데이터 품질 값 유형은 항상 데이터 품질 결과를 규정한다."@kr ;
  skos:prefLabel "data quality value type"@en ;
  skos:prefLabel "데이터 품질 값 유형"@kr ;
.
<http://iso.org/tc211/term/1206>
  rdf:type skos:Concept ;
  dcterms:dateAccepted "2014-02-15"^^xsd:date ;
  dcterms:source "ISO 19153:2014, 4.1" ;
  reg:status reg:statusValid ;
  rdfs:label "access control"@en ;
  skos:changeNote "valid" ;
  skos:editorialNote "preferred"^^xsd:string ;
  skos:notation 1206 ;
  skos:prefLabel "access control"@en ;
.
<http://iso.org/tc211/term/1207>
  rdf:type skos:Concept ;
  dcterms:dateAccepted "2014-02-15"^^xsd:date ;
  dcterms:source "ISO 19153:2014, 4.2" ;
  reg:status reg:statusValid ;
  rdfs:label "agency"@en ;
  skos:changeNote "valid" ;
  skos:editorialNote "preferred"^^xsd:string ;
  skos:notation 1207 ;
  skos:prefLabel "agency"@en ;
.
<http://iso.org/tc211/term/1208>
  rdf:type skos:Concept ;
  dcterms:dateAccepted "2014-02-15"^^xsd:date ;
  dcterms:source "ISO 19153:2014, 4.3" ;
  reg:status reg:statusValid ;
  rdfs:label "agent"@en ;
  skos:changeNote "valid" ;
  skos:editorialNote "preferred"^^xsd:string ;
  skos:notation 1208 ;
  skos:prefLabel "agent"@en ;
.
<http://iso.org/tc211/term/121>
  rdf:type skos:Concept ;
  dcterms:dateAccepted "2002-12-01"^^xsd:date ;
  dcterms:dateAccepted "2007-11-01"^^xsd:date ;
  dcterms:source "ISO 19113:2002, 4.13" ;
  reg:status reg:statusRetired ;
  rdfs:comment "Note 1 to entry: A data quality value unit is provided only when applicable for a data quality result."@en ;
  rdfs:comment "비고: 데이터 품질 값 단위는 데이터 품질 결과에 적용 가능할 때만 제공된다."@kr ;
  rdfs:label "data quality value unit"@en ;
  skos:changeNote "retired" ;
  skos:definition "데이터 품질 결과를 보고하는 값의 단위"@kr ;
  skos:notation "121" ;
  skos:notation 121 ;
  skos:note "Note 1 to entry: A data quality value unit is provided only when applicable for a data quality result."@en ;
  skos:note "비고: 데이터 품질 값 단위는 데이터 품질 결과에 적용 가능할 때만 제공된다."@kr ;
  skos:prefLabel "data quality value unit"@en ;
  skos:prefLabel "데이터 품질 값 단위"@kr ;
.
<http://iso.org/tc211/term/1210>
  rdf:type skos:Concept ;
  dcterms:dateAccepted "2014-02-15"^^xsd:date ;
  dcterms:provenance "ISO 19153:2014, 4.4" ;
  dcterms:source "W3C, Web Services Glossary" ;
  reg:status reg:statusValid ;
  rdfs:label "authentication"@en ;
  skos:changeNote "valid" ;
  skos:editorialNote "preferred"^^xsd:string ;
  skos:notation 1210 ;
  skos:prefLabel "authentication"@en ;
.
<http://iso.org/tc211/term/1211>
  rdf:type skos:Concept ;
  dcterms:dateAccepted "2014-02-15"^^xsd:date ;
  dcterms:source "ISO 19153:2014, 4.5" ;
  reg:status reg:statusValid ;
  rdfs:comment "Note 1 to entry:  Usually, authorization is in the context of authentication. Once a subject is authenticated, it can be authorized to perform different types of access."@en ;
  rdfs:label "authorization"@en ;
  skos:changeNote "valid" ;
  skos:editorialNote "preferred"^^xsd:string ;
  skos:notation 1211 ;
  skos:note "Note 1 to entry:  Usually, authorization is in the context of authentication. Once a subject is authenticated, it can be authorized to perform different types of access."@en ;
  skos:prefLabel "authorization"@en ;
.
<http://iso.org/tc211/term/1212>
  rdf:type skos:Concept ;
  dcterms:dateAccepted "2014-02-15"^^xsd:date ;
  dcterms:provenance "ISO 19153:2014, 4.6" ;
  dcterms:source "W3C, Web Services Glossary" ;
  reg:status reg:statusValid ;
  rdfs:comment "Note 1 to entry:  Security systems are bypassed usually by using security faults in the operating system. Such infringements are more an aspect of the operating system than of the security system. To correct this, the relationship between the security system and the operating system shall be modified to prevent bypass mechanisms."@en ;
  rdfs:label "bypass"@en ;
  skos:changeNote "valid" ;
  skos:editorialNote "preferred"^^xsd:string ;
  skos:notation 1212 ;
  skos:note "Note 1 to entry:  Security systems are bypassed usually by using security faults in the operating system. Such infringements are more an aspect of the operating system than of the security system. To correct this, the relationship between the security system and the operating system shall be modified to prevent bypass mechanisms."@en ;
  skos:prefLabel "bypass"@en ;
.
<http://iso.org/tc211/term/1213>
  rdf:type skos:Concept ;
  dcterms:dateAccepted "2014-02-15"^^xsd:date ;
  dcterms:source "ISO 19153:2014, 4.7" ;
  reg:status reg:statusValid ;
  rdfs:comment "Note 1 to entry:  A chain of agency, with the proper agreements at each step creates a transitive agency between the agent of the first link and the principal of the last. This chain can be spoken of in either direction, either as “principal -> agent = principal -> agent” (normal or granting order) or “agent -> principal = agent -> principal” (reverse, acceptance, verification or tracing order)."@en ;
  rdfs:label "chain of agency"@en ;
  skos:changeNote "valid" ;
  skos:editorialNote "preferred"^^xsd:string ;
  skos:notation 1213 ;
  skos:note "Note 1 to entry:  A chain of agency, with the proper agreements at each step creates a transitive agency between the agent of the first link and the principal of the last. This chain can be spoken of in either direction, either as “principal -> agent = principal -> agent” (normal or granting order) or “agent -> principal = agent -> principal” (reverse, acceptance, verification or tracing order)."@en ;
  skos:prefLabel "chain of agency"@en ;
.
<http://iso.org/tc211/term/1214>
  rdf:type skos:Concept ;
  dcterms:dateAccepted "2014-02-15"^^xsd:date ;
  dcterms:source "ISO 19153:2014, 4.8" ;
  reg:status reg:statusValid ;
  rdfs:comment "Note 1 to entry:  As with the chain of agency, this chain can be spoken of in either direction."@en ;
  rdfs:label "chain of licence"@en ;
  skos:changeNote "valid" ;
  skos:editorialNote "preferred"^^xsd:string ;
  skos:notation 1214 ;
  skos:note "Note 1 to entry:  As with the chain of agency, this chain can be spoken of in either direction."@en ;
  skos:prefLabel "chain of licence"@en ;
.
<http://iso.org/tc211/term/1215>
  rdf:type skos:Concept ;
  dcterms:dateAccepted "2014-02-15"^^xsd:date ;
  dcterms:provenance "ISO 19153:2014, 4.9" ;
  dcterms:source "FindLaw, modified" ;
  reg:status reg:statusValid ;
  rdfs:label "contract"@en ;
  skos:changeNote "valid" ;
  skos:editorialNote "preferred"^^xsd:string ;
  skos:notation 1215 ;
  skos:prefLabel "contract"@en ;
.
<http://iso.org/tc211/term/1216>
  rdf:type skos:Concept ;
  dcterms:dateAccepted "2014-02-15"^^xsd:date ;
  dcterms:source "ISO 19153:2014, 4.10" ;
  reg:status reg:statusValid ;
  rdfs:comment "Note 1 to entry:  A copyleft is a form of general public licence."@en ;
  rdfs:label "copyleft"@en ;
  skos:changeNote "valid" ;
  skos:editorialNote "preferred"^^xsd:string ;
  skos:notation 1216 ;
  skos:note "Note 1 to entry:  A copyleft is a form of general public licence."@en ;
  skos:prefLabel "copyleft"@en ;
.
<http://iso.org/tc211/term/1217>
  rdf:type skos:Concept ;
  dcterms:dateAccepted "2014-02-15"^^xsd:date ;
  dcterms:source "ISO 19153:2014, 4.11" ;
  reg:status reg:statusValid ;
  rdfs:comment "Note 1 to entry:  The core concept in DRM is the use of digital licences. Instead of buying the digital content, the consumer purchases a licence granting certain rights with respect to the content. A licence is the mechanism by which a rights holder conveys rights to another party, such as a consumer or distributor."@en ;
  rdfs:label "digital licence"@en ;
  skos:changeNote "valid" ;
  skos:editorialNote "preferred"^^xsd:string ;
  skos:notation 1217 ;
  skos:note "Note 1 to entry:  The core concept in DRM is the use of digital licences. Instead of buying the digital content, the consumer purchases a licence granting certain rights with respect to the content. A licence is the mechanism by which a rights holder conveys rights to another party, such as a consumer or distributor."@en ;
  skos:prefLabel "digital licence"@en ;
.
<http://iso.org/tc211/term/1218>
  rdf:type skos:Concept ;
  dcterms:dateAccepted "2014-02-15"^^xsd:date ;
  dcterms:source "ISO 19153:2014, 4.12" ;
  reg:status reg:statusValid ;
  rdfs:comment "Note 1 to entry:  DRM covers a much broader spectrum of capabilities and underlying technologies supporting description, identification, trading, protecting, monitoring, and tracking of all forms of rights usages for both tangible and intangible (electronic) assets, including the management of rights-holders relationships. See, for example, Reference [5][of ISO 19153:2014 - Iannella R. Digital Rights Management (DRM) Architectures. D-Lib. 2001 June, 7 (6) Available at: http://www.dlib.org/dlib/june01/iannella/06iannella.html]. “Digital” refers to the material over which the rights exist. “Rights” applies to the Intellectual Property rights linked to the material. “Management” covers both the defining of policy and enforcing that policy in such a way that rights are respected. The ultimate goal of a distributed DRM system is for content authors to be able to project policies governing their content into remote environments with confidence that those policies will be respected by the remote nodes. For the purposes of this International Standard, DRM is taken to mean technology that enables the secure distribution (and where appropriate, sale) of digital media content on the Internet."@en ;
  rdfs:label "digital rights management"@en ;
  skos:altLabel "DRM"^^<http://www.w3.org/2001/XMLSchema#@en> ;
  skos:changeNote "valid" ;
  skos:editorialNote "preferred"^^xsd:string ;
  skos:notation 1218 ;
  skos:note "Note 1 to entry:  DRM covers a much broader spectrum of capabilities and underlying technologies supporting description, identification, trading, protecting, monitoring, and tracking of all forms of rights usages for both tangible and intangible (electronic) assets, including the management of rights-holders relationships. See, for example, Reference [5][of ISO 19153:2014 - Iannella R. Digital Rights Management (DRM) Architectures. D-Lib. 2001 June, 7 (6) Available at: http://www.dlib.org/dlib/june01/iannella/06iannella.html]. “Digital” refers to the material over which the rights exist. “Rights” applies to the Intellectual Property rights linked to the material. “Management” covers both the defining of policy and enforcing that policy in such a way that rights are respected. The ultimate goal of a distributed DRM system is for content authors to be able to project policies governing their content into remote environments with confidence that those policies will be respected by the remote nodes. For the purposes of this International Standard, DRM is taken to mean technology that enables the secure distribution (and where appropriate, sale) of digital media content on the Internet."@en ;
  skos:prefLabel "digital rights management"@en ;
.
<http://iso.org/tc211/term/1219>
  rdf:type skos:Concept ;
  dcterms:dateAccepted "2014-02-15"^^xsd:date ;
  dcterms:source "ISO 19153:2014, 4.13" ;
  reg:status reg:statusValid ;
  rdfs:comment "Note 1 to entry:  Expected risk is calculated by multiplying the probability of the types of infringement by the cost of that infringement, summed up over all types of infringement."@en ;
  rdfs:label "expected risk"@en ;
  skos:changeNote "valid" ;
  skos:editorialNote "preferred"^^xsd:string ;
  skos:notation 1219 ;
  skos:note "Note 1 to entry:  Expected risk is calculated by multiplying the probability of the types of infringement by the cost of that infringement, summed up over all types of infringement."@en ;
  skos:prefLabel "expected risk"@en ;
.
<http://iso.org/tc211/term/122>
  rdf:type skos:Concept ;
  dcterms:dateAccepted "2005-07-15"^^xsd:date ;
  dcterms:dateAccepted "2008-12-30"^^xsd:date ;
  dcterms:provenance "ISO 19118:2005" ;
  dcterms:source "ISO 19118:2011, 4.10" ;
  reg:status reg:statusValid ;
  rdfs:comment "Note 1 to entry: Transfer of information implies transfer of data."@en ;
  rdfs:comment "비고: 정보의 전송은 데이터의 전송을 의미한다."@kr ;
  rdfs:label "data transfer"@en ;
  skos:changeNote "valid" ;
  skos:definition "매체를 통해 한 지점에서 다른 지점으로 데이터를 이동시키는 것"@kr ;
  skos:editorialNote "preferred" ;
  skos:editorialNote "preferred"^^xsd:string ;
  skos:notation "122" ;
  skos:notation 122 ;
  skos:note "Note 1 to entry: Transfer of information implies transfer of data."@en ;
  skos:note "비고: 정보의 전송은 데이터의 전송을 의미한다."@kr ;
  skos:prefLabel "data transfer"@en ;
  skos:prefLabel "데이터 전송"@kr ;
.
<http://iso.org/tc211/term/1220>
  rdf:type skos:Concept ;
  dcterms:dateAccepted "2014-02-15"^^xsd:date ;
  dcterms:provenance "ISO 19153:2014, 4.14" ;
  dcterms:source "U.S. legal term derived from Title 17 of the United States Code, Section 107" ;
  reg:status reg:statusValid ;
  rdfs:comment "Note 1 to entry:  Fair use is based on case-law precedents derived from general principles. The term is often misapplied to refer to the reasonable expectations of consumers to be able to use purchased content on all owned devices."@en ;
  rdfs:label "fair use"@en ;
  skos:changeNote "valid" ;
  skos:editorialNote "preferred"^^xsd:string ;
  skos:notation 1220 ;
  skos:note "Note 1 to entry:  Fair use is based on case-law precedents derived from general principles. The term is often misapplied to refer to the reasonable expectations of consumers to be able to use purchased content on all owned devices."@en ;
  skos:prefLabel "fair use"@en ;
.
<http://iso.org/tc211/term/1221>
  rdf:type skos:Concept ;
  dcterms:dateAccepted "2014-02-15"^^xsd:date ;
  dcterms:source "ISO 19153:2014, 4.15" ;
  reg:status reg:statusValid ;
  rdfs:comment "Note 1 to entry:  GPLs can be granted by the owner of a resource or can be applied to a resource by law, usually as part of the copyright law. The most obvious GPL concept is fair use in the United States for copyrighted material. Other GPL rights can be demanded by the source of the resource or other “public good” considerations."@en ;
  rdfs:comment "Note 2 to entry:  The most widespread use of GPL is in reference to the GNU GPL, which is commonly abbreviated simply as GPL when it is understood that the term refers to the GNU GPL. One of the basic tenets of the GPL is that anyone who acquires the material shall make it available to anyone else under the same licensing agreement. The GPL does not cover activities other than the copying, distributing, and modifying of the source code. A GPL is also referred to as a copyleft, in contrast to a copyright, which identifies the proprietary rights of material." ;
  rdfs:label "general public licence"@en ;
  skos:altLabel "GPL"^^<http://www.w3.org/2001/XMLSchema#@en> ;
  skos:changeNote "valid" ;
  skos:editorialNote "preferred"^^xsd:string ;
  skos:notation 1221 ;
  skos:note "Note 1 to entry:  GPLs can be granted by the owner of a resource or can be applied to a resource by law, usually as part of the copyright law. The most obvious GPL concept is fair use in the United States for copyrighted material. Other GPL rights can be demanded by the source of the resource or other “public good” considerations."@en ;
  skos:note "Note 2 to entry:  The most widespread use of GPL is in reference to the GNU GPL, which is commonly abbreviated simply as GPL when it is understood that the term refers to the GNU GPL. One of the basic tenets of the GPL is that anyone who acquires the material shall make it available to anyone else under the same licensing agreement. The GPL does not cover activities other than the copying, distributing, and modifying of the source code. A GPL is also referred to as a copyleft, in contrast to a copyright, which identifies the proprietary rights of material."^^<http://www.w3.org/2001/XMLSchema#@en> ;
  skos:prefLabel "general public licence"@en ;
.
<http://iso.org/tc211/term/1222>
  rdf:type skos:Concept ;
  dcterms:dateAccepted "2014-02-15"^^xsd:date ;
  dcterms:source "ISO 19153:2014, 4.16" ;
  reg:status reg:statusValid ;
  rdfs:comment "Note 1 to entry:  Applied to processing resources."@en ;
  rdfs:label "GeoDRM enabled"@en ;
  skos:changeNote "valid" ;
  skos:editorialNote "preferred"^^xsd:string ;
  skos:notation 1222 ;
  skos:note "Note 1 to entry:  Applied to processing resources."@en ;
  skos:prefLabel "GeoDRM enabled"@en ;
.
<http://iso.org/tc211/term/1223>
  rdf:type skos:Concept ;
  dcterms:dateAccepted "2014-02-15"^^xsd:date ;
  dcterms:source "ISO 19153:2014, 4.17" ;
  reg:status reg:statusValid ;
  rdfs:label "GeoDRM extended (applied to resources)"@en ;
  skos:changeNote "valid" ;
  skos:editorialNote "preferred"^^xsd:string ;
  skos:notation 1223 ;
  skos:prefLabel "GeoDRM extended (applied to resources)"@en ;
.
<http://iso.org/tc211/term/1224>
  rdf:type skos:Concept ;
  dcterms:dateAccepted "2014-02-15"^^xsd:date ;
  dcterms:source "ISO 19153:2014, 4.18" ;
  reg:status reg:statusValid ;
  rdfs:label "GeoLicence"@en ;
  skos:changeNote "valid" ;
  skos:editorialNote "preferred"^^xsd:string ;
  skos:notation 1224 ;
  skos:prefLabel "GeoLicence"@en ;
.
<http://iso.org/tc211/term/1225>
  rdf:type skos:Concept ;
  dcterms:dateAccepted "2014-02-15"^^xsd:date ;
  dcterms:source "ISO 19153:2014, 4.19" ;
  reg:status reg:statusValid ;
  rdfs:label "GeoLicence resolution"@en ;
  skos:changeNote "valid" ;
  skos:editorialNote "preferred"^^xsd:string ;
  skos:notation 1225 ;
  skos:prefLabel "GeoLicence resolution"@en ;
.
<http://iso.org/tc211/term/1226>
  rdf:type skos:Concept ;
  dcterms:dateAccepted "2014-02-15"^^xsd:date ;
  dcterms:provenance "ISO 19153:2014, 4.20" ;
  dcterms:source "FindLaw, modified" ;
  reg:status reg:statusValid ;
  rdfs:label "GeoLicence infringement"@en ;
  skos:changeNote "valid" ;
  skos:editorialNote "preferred"^^xsd:string ;
  skos:notation 1226 ;
  skos:prefLabel "GeoLicence infringement"@en ;
.
<http://iso.org/tc211/term/1227>
  rdf:type skos:Concept ;
  dcterms:dateAccepted "2014-02-15"^^xsd:date ;
  dcterms:source "ISO 19153:2014, 4.21" ;
  reg:status reg:statusValid ;
  rdfs:comment "Note 1 to entry:  Infringement of a licence will require the DRM system to be bypassed in some manner. If licences can be infringed without bypassing the DRM system, then the system is not sufficient."@en ;
  rdfs:label "infringement (of a licence)"@en ;
  skos:changeNote "valid" ;
  skos:editorialNote "preferred"^^xsd:string ;
  skos:notation 1227 ;
  skos:note "Note 1 to entry:  Infringement of a licence will require the DRM system to be bypassed in some manner. If licences can be infringed without bypassing the DRM system, then the system is not sufficient."@en ;
  skos:prefLabel "infringement (of a licence)"@en ;
.
<http://iso.org/tc211/term/1228>
  rdf:type skos:Concept ;
  dcterms:dateAccepted "2014-02-15"^^xsd:date ;
  dcterms:source "ISO 19153:2014, 4.22" ;
  reg:status reg:statusValid ;
  rdfs:comment "Note 1 to entry:  Infringement of a right is a fault in the DRM system. If rights can be infringed without bypassing the DRM system, then the system is not properly restricted to that which is necessary."@en ;
  rdfs:label "infringement (of a right)"@en ;
  skos:changeNote "valid" ;
  skos:editorialNote "preferred"^^xsd:string ;
  skos:notation 1228 ;
  skos:note "Note 1 to entry:  Infringement of a right is a fault in the DRM system. If rights can be infringed without bypassing the DRM system, then the system is not properly restricted to that which is necessary."@en ;
  skos:prefLabel "infringement (of a right)"@en ;
.
<http://iso.org/tc211/term/1229>
  rdf:type skos:Concept ;
  dcterms:dateAccepted "2014-02-15"^^xsd:date ;
  dcterms:provenance "ISO 19153:2014, 4.23" ;
  dcterms:source "FindLaw, modified" ;
  reg:status reg:statusValid ;
  rdfs:comment "Note 1 to entry:  In this case, the principal as owner is a principal group, i.e. a group of other principals."@en ;
  rdfs:label "joint ownership"@en ;
  skos:changeNote "valid" ;
  skos:editorialNote "preferred"^^xsd:string ;
  skos:notation 1229 ;
  skos:note "Note 1 to entry:  In this case, the principal as owner is a principal group, i.e. a group of other principals."@en ;
  skos:prefLabel "joint ownership"@en ;
.
<http://iso.org/tc211/term/123>
  rdf:type skos:Concept ;
  dcterms:dateAccepted "2003-05-01"^^xsd:date ;
  dcterms:dateAccepted "2009-12-29"^^xsd:date ;
  dcterms:provenance "KS X ISO 19103" ;
  dcterms:source "ISO/TS 19103:2005" ;
  reg:status reg:statusValid ;
  rdfs:comment "Note 1 to entry: Data types include primitive predefined types and user-definable types."@en ;
  rdfs:comment "비고: 데이터 유형은 미리 정의된 유형과 사용자 정의 유형을 포함한다."@kr ;
  rdfs:label "data type"@en ;
  skos:changeNote "valid" ;
  skos:definition "영역 내의 값을 바탕으로 연산을 통해 나올 수 있는 허용된 값 영역의 사양"@kr ;
  skos:editorialNote "preferred" ;
  skos:editorialNote "preferred"^^xsd:string ;
  skos:notation "123" ;
  skos:notation 123 ;
  skos:note "Note 1 to entry: Data types include primitive predefined types and user-definable types."@en ;
  skos:note "비고: 데이터 유형은 미리 정의된 유형과 사용자 정의 유형을 포함한다."@kr ;
  skos:prefLabel "data type"@en ;
  skos:prefLabel "데이터 유형"@kr ;
.
<http://iso.org/tc211/term/1230>
  rdf:type skos:Concept ;
  dcterms:dateAccepted "2014-02-15"^^xsd:date ;
  dcterms:source "ISO 19153:2014, 4.24" ;
  reg:status reg:statusValid ;
  rdfs:comment "Note 1 to entry:  During this period, the resource is only available to the lessee. Temporal constraints are required for downstream use."@en ;
  rdfs:label "lease"@en ;
  skos:changeNote "valid" ;
  skos:editorialNote "preferred"^^xsd:string ;
  skos:notation 1230 ;
  skos:note "Note 1 to entry:  During this period, the resource is only available to the lessee. Temporal constraints are required for downstream use."@en ;
  skos:prefLabel "lease"@en ;
.
<http://iso.org/tc211/term/1231>
  rdf:type skos:Concept ;
  dcterms:dateAccepted "2014-02-15"^^xsd:date ;
  dcterms:source "ISO 19153:2014, 4.25" ;
  reg:status reg:statusValid ;
  rdfs:label "lend"@en ;
  skos:changeNote "valid" ;
  skos:editorialNote "preferred"^^xsd:string ;
  skos:notation 1231 ;
  skos:prefLabel "lend"@en ;
.
<http://iso.org/tc211/term/1232>
  rdf:type skos:Concept ;
  dcterms:dateAccepted "2014-02-15"^^xsd:date ;
  dcterms:provenance "ISO 19153:2014, 4.26" ;
  dcterms:source "XrML 2.0 specification, part 5, modified" ;
  reg:status reg:statusValid ;
  rdfs:comment "Note 1 to entry:  A licence represents, but is not, a contract that grants a party explicit rights to use Intellectual Property."@en ;
  rdfs:label "licence"@en ;
  skos:changeNote "valid" ;
  skos:editorialNote "preferred"^^xsd:string ;
  skos:notation 1232 ;
  skos:note "Note 1 to entry:  A licence represents, but is not, a contract that grants a party explicit rights to use Intellectual Property."@en ;
  skos:prefLabel "licence"@en ;
.
<http://iso.org/tc211/term/1233>
  rdf:type skos:Concept ;
  dcterms:dateAccepted "2014-02-15"^^xsd:date ;
  dcterms:source "ISO 19153:2014, 4.27" ;
  reg:status reg:statusValid ;
  rdfs:comment "Note 1 to entry:  The extent can be described in spatial, temporal. or any other parameter range appropriate to the rights described in the licence."@en ;
  rdfs:label "licence extents"@en ;
  skos:changeNote "valid" ;
  skos:editorialNote "preferred"^^xsd:string ;
  skos:notation 1233 ;
  skos:note "Note 1 to entry:  The extent can be described in spatial, temporal. or any other parameter range appropriate to the rights described in the licence."@en ;
  skos:prefLabel "licence extents"@en ;
.
<http://iso.org/tc211/term/1234>
  rdf:type skos:Concept ;
  dcterms:dateAccepted "2014-02-15"^^xsd:date ;
  dcterms:provenance "ISO 19153:2014, 4.28" ;
  dcterms:source "New Concepts in BASIS Licensing, modified" ;
  reg:status reg:statusValid ;
  rdfs:label "licence manager"@en ;
  skos:changeNote "valid" ;
  skos:editorialNote "preferred"^^xsd:string ;
  skos:notation 1234 ;
  skos:prefLabel "licence manager"@en ;
.
<http://iso.org/tc211/term/1235>
  rdf:type skos:Concept ;
  dcterms:dateAccepted "2014-02-15"^^xsd:date ;
  dcterms:provenance "ISO 19153:2014, 4.29" ;
  dcterms:source "FindLaw" ;
  reg:status reg:statusValid ;
  rdfs:label "licensee"@en ;
  skos:changeNote "valid" ;
  skos:editorialNote "preferred"^^xsd:string ;
  skos:notation 1235 ;
  skos:prefLabel "licensee"@en ;
.
<http://iso.org/tc211/term/1236>
  rdf:type skos:Concept ;
  dcterms:dateAccepted "2014-02-15"^^xsd:date ;
  dcterms:provenance "ISO 19153:2014, 4.30" ;
  dcterms:source "Derived from FindLaw for “agent”" ;
  reg:status reg:statusValid ;
  rdfs:label "licensing agent"@en ;
  skos:changeNote "valid" ;
  skos:editorialNote "preferred"^^xsd:string ;
  skos:notation 1236 ;
  skos:prefLabel "licensing agent"@en ;
.
<http://iso.org/tc211/term/1237>
  rdf:type skos:Concept ;
  dcterms:dateAccepted "2014-02-15"^^xsd:date ;
  dcterms:provenance "ISO 19153:2014, 4.31" ;
  dcterms:source "FindLaw, modified" ;
  reg:status reg:statusValid ;
  rdfs:comment "Note 1 to entry:  The licensor is a content owner or a licensing agent."@en ;
  rdfs:label "licensor"@en ;
  skos:changeNote "valid" ;
  skos:editorialNote "preferred"^^xsd:string ;
  skos:notation 1237 ;
  skos:note "Note 1 to entry:  The licensor is a content owner or a licensing agent."@en ;
  skos:prefLabel "licensor"@en ;
.
<http://iso.org/tc211/term/124>
  rdf:type skos:Concept ;
  dcterms:dateAccepted "2002-07-01"^^xsd:date ;
  dcterms:dateAccepted "2008-12-30"^^xsd:date ;
  dcterms:provenance "ISO 19101:2002" ;
  dcterms:source "ISO 19115-1:2014, 4.3" ;
  reg:status reg:statusValid ;
  rdfs:comment "Note 1 to entry: A dataset may be a smaller grouping of data which, though limited by some constraint such as spatial extent or feature type, is located physically within a larger dataset. Theoretically, a dataset may be as small as a single feature or feature attribute contained within a larger dataset. A hardcopy map or chart may be considered a dataset."@en ;
  rdfs:comment "비고: 데이터셋은 비록 공간 범위나 피처 유형과 같은 제약 조건으로 한정되어도 보다 큰 데이터셋 내에 물리적으로 존재하는 보다 작은 데이터의 그룹이 될 수 있다. 이론적으로, 데이터셋은 하나의 피처 또는 보다 큰 데이터셋에 포함된 피처 속성 만큼이나 작다. 종이 지도 및 도표는 데이터셋으로 간주된다."@kr ;
  rdfs:label "dataset"@en ;
  skos:changeNote "valid" ;
  skos:definition "식별 가능한 데이터의 모음"@kr ;
  skos:editorialNote "preferred" ;
  skos:editorialNote "preferred"^^xsd:string ;
  skos:notation "124" ;
  skos:notation 124 ;
  skos:note "Note 1 to entry: A dataset may be a smaller grouping of data which, though limited by some constraint such as spatial extent or feature type, is located physically within a larger dataset. Theoretically, a dataset may be as small as a single feature or feature attribute contained within a larger dataset. A hardcopy map or chart may be considered a dataset."@en ;
  skos:note "비고: 데이터셋은 비록 공간 범위나 피처 유형과 같은 제약 조건으로 한정되어도 보다 큰 데이터셋 내에 물리적으로 존재하는 보다 작은 데이터의 그룹이 될 수 있다. 이론적으로, 데이터셋은 하나의 피처 또는 보다 큰 데이터셋에 포함된 피처 속성 만큼이나 작다. 종이 지도 및 도표는 데이터셋으로 간주된다."@kr ;
  skos:prefLabel "dataset"@en ;
  skos:prefLabel "데이터셋"@kr ;
.
<http://iso.org/tc211/term/1240>
  rdf:type skos:Concept ;
  dcterms:dateAccepted "2014-02-15"^^xsd:date ;
  dcterms:source "ISO 19153:2014, 4.33" ;
  reg:status reg:statusValid ;
  rdfs:comment "Note 1 to entry:  All aspects of a DRM system are necessary if they do not prevent legitimate requests from execution."@en ;
  rdfs:label "necessary"@en ;
  skos:changeNote "valid" ;
  skos:editorialNote "preferred"^^xsd:string ;
  skos:notation 1240 ;
  skos:note "Note 1 to entry:  All aspects of a DRM system are necessary if they do not prevent legitimate requests from execution."@en ;
  skos:prefLabel "necessary"@en ;
.
<http://iso.org/tc211/term/1241>
  rdf:type skos:Concept ;
  dcterms:dateAccepted "2014-02-15"^^xsd:date ;
  dcterms:provenance "ISO 19153:2014, 4.34" ;
  dcterms:source "FindLaw, modified" ;
  reg:status reg:statusValid ;
  rdfs:label "owner"@en ;
  skos:changeNote "valid" ;
  skos:editorialNote "preferred"^^xsd:string ;
  skos:notation 1241 ;
  skos:prefLabel "owner"@en ;
.
<http://iso.org/tc211/term/1242>
  rdf:type skos:Concept ;
  dcterms:dateAccepted "2012-12-01"^^xsd:date ;
  dcterms:source "ISO 19152:2012, 4.1.13" ;
  reg:status reg:statusValid ;
  rdfs:comment "Note 1 to entry: In order to be registered as a party, not all members need to be identified and registered individually."@en ;
  rdfs:comment "Note 2 to entry: A basic administrative unit may be a party because it may hold a right of e.g. easement." ;
  rdfs:label "party"@en ;
  skos:changeNote "valid" ;
  skos:editorialNote "preferred"^^xsd:string ;
  skos:notation 1242 ;
  skos:note "Note 1 to entry: In order to be registered as a party, not all members need to be identified and registered individually."@en ;
  skos:note "Note 2 to entry: A basic administrative unit may be a party because it may hold a right of e.g. easement."^^<http://www.w3.org/2001/XMLSchema#@en> ;
  skos:prefLabel "party"@en ;
.
<http://iso.org/tc211/term/1243>
  rdf:type skos:Concept ;
  dcterms:dateAccepted "2014-02-15"^^xsd:date ;
  dcterms:source "ISO 19153:2014, 4.36" ;
  reg:status reg:statusValid ;
  rdfs:comment "Note 1 to entry:  Payment providers can be telephone and cellular companies, banks, credit card corporations, ISPs, network operators, and utility companies. The payment provider bills the consumer, deducts a fee, and forwards the payment to the content provider. The payment provider is thus responsible for the balancing of accounts."@en ;
  rdfs:label "payment provider"@en ;
  skos:changeNote "valid" ;
  skos:editorialNote "preferred"^^xsd:string ;
  skos:notation 1243 ;
  skos:note "Note 1 to entry:  Payment providers can be telephone and cellular companies, banks, credit card corporations, ISPs, network operators, and utility companies. The payment provider bills the consumer, deducts a fee, and forwards the payment to the content provider. The payment provider is thus responsible for the balancing of accounts."@en ;
  skos:prefLabel "payment provider"@en ;
.
<http://iso.org/tc211/term/1244>
  rdf:type skos:Concept ;
  dcterms:dateAccepted "2014-02-15"^^xsd:date ;
  dcterms:source "ISO 19153:2014, 4.37" ;
  reg:status reg:statusValid ;
  rdfs:comment "Note 1 to entry:  Persistent protection mechanisms involve authentication, authorization, and encryption technologies for effectively locking digital contents and limiting distribution to those who pay."@en ;
  rdfs:label "persistent protection mechanism"@en ;
  skos:changeNote "valid" ;
  skos:editorialNote "preferred"^^xsd:string ;
  skos:notation 1244 ;
  skos:note "Note 1 to entry:  Persistent protection mechanisms involve authentication, authorization, and encryption technologies for effectively locking digital contents and limiting distribution to those who pay."@en ;
  skos:prefLabel "persistent protection mechanism"@en ;
.
<http://iso.org/tc211/term/1245>
  rdf:type skos:Concept ;
  dcterms:dateAccepted "2014-02-15"^^xsd:date ;
  dcterms:source "ISO 19153:2014, 4.35" ;
  reg:status reg:statusValid ;
  rdfs:comment "Note 1 to entry:  These two terms [principal and party] are used as near synonyms from ORDL and ISO 21000. There will be no distinction between these two terms made here, but there can be distinctions in legal documents depending on local laws."@en ;
  rdfs:label "principal"@en ;
  rdfs:seeAlso "party" ;
  skos:altLabel "party"@en ;
  skos:changeNote "valid" ;
  skos:editorialNote "preferred"^^xsd:string ;
  skos:notation 1245 ;
  skos:note "Note 1 to entry:  These two terms [principal and party] are used as near synonyms from ORDL and ISO 21000. There will be no distinction between these two terms made here, but there can be distinctions in legal documents depending on local laws."@en ;
  skos:prefLabel "principal"@en ;
.
<http://iso.org/tc211/term/1246>
  rdf:type skos:Concept ;
  dcterms:dateAccepted "2014-02-15"^^xsd:date ;
  dcterms:source "ISO 19153:2014, 4.38" ;
  reg:status reg:statusValid ;
  rdfs:label "protection"@en ;
  skos:changeNote "valid" ;
  skos:editorialNote "preferred"^^xsd:string ;
  skos:notation 1246 ;
  skos:prefLabel "protection"@en ;
.
<http://iso.org/tc211/term/1247>
  rdf:type skos:Concept ;
  dcterms:dateAccepted "2014-02-15"^^xsd:date ;
  dcterms:source "ISO 19153:2014, 4.39" ;
  reg:status reg:statusValid ;
  rdfs:label "provenance"@en ;
  skos:changeNote "valid" ;
  skos:editorialNote "preferred"^^xsd:string ;
  skos:notation 1247 ;
  skos:prefLabel "provenance"@en ;
.
<http://iso.org/tc211/term/1248>
  rdf:type skos:Concept ;
  dcterms:dateAccepted "2014-02-15"^^xsd:date ;
  dcterms:source "ISO 19153:2014, 4.40" ;
  reg:status reg:statusValid ;
  rdfs:comment "Note 1 to entry:  In general, a resource is data, metadata (a type of data describing other resources), or some service or process that can be invoked on other resources. Licences describe rights on resources and, as such, are resources in themselves."@en ;
  rdfs:label "resource <GeoDRM>"@en ;
  skos:changeNote "valid" ;
  skos:editorialNote "preferred"^^xsd:string ;
  skos:notation 1248 ;
  skos:note "Note 1 to entry:  In general, a resource is data, metadata (a type of data describing other resources), or some service or process that can be invoked on other resources. Licences describe rights on resources and, as such, are resources in themselves."@en ;
  skos:prefLabel "resource <GeoDRM>"@en ;
.
<http://iso.org/tc211/term/1249>
  rdf:type skos:Concept ;
  dcterms:dateAccepted "2014-02-15"^^xsd:date ;
  dcterms:source "ISO 19153:2014, 4.41" ;
  reg:status reg:statusValid ;
  rdfs:comment "Note 1 to entry:  Remediation allows more trust because it lowers expected risk. The first act in a remediation sequence is detection of the fault."@en ;
  rdfs:label "remediation"@en ;
  skos:changeNote "valid" ;
  skos:editorialNote "preferred"^^xsd:string ;
  skos:notation 1249 ;
  skos:note "Note 1 to entry:  Remediation allows more trust because it lowers expected risk. The first act in a remediation sequence is detection of the fault."@en ;
  skos:prefLabel "remediation"@en ;
.
<http://iso.org/tc211/term/125>
  rdf:type skos:Concept ;
  dcterms:dateAccepted "2002-12-01"^^xsd:date ;
  dcterms:dateAccepted "2008-12-30"^^xsd:date ;
  dcterms:provenance "ISO 19113" ;
  dcterms:source "ISO 19115:2003, 4.3" ;
  reg:status reg:statusRetired ;
  rdfs:label "dataset series"@en ;
  skos:changeNote "retired" ;
  skos:definition "동일한 제품 사양을 통해 작성된 데이터셋의 모음"@kr ;
  skos:notation "125" ;
  skos:notation 125 ;
  skos:prefLabel "dataset series"@en ;
  skos:prefLabel "데이터셋 시리즈"@kr ;
.
<http://iso.org/tc211/term/1250>
  rdf:type skos:Concept ;
  dcterms:dateAccepted "2014-02-15"^^xsd:date ;
  dcterms:provenance "ISO 19153:2014, 4.42" ;
  dcterms:source "ISO 21000-5, modified" ;
  reg:status reg:statusValid ;
  rdfs:comment "Note 1 to entry:  A right specifies an action (or activity) or a class of actions that a principal can perform on or using the associated resource. A right is essentially a legally recognized entitlement to do something to or with the content of a resource."@en ;
  rdfs:label "right <GeoDRM>"@en ;
  skos:changeNote "valid" ;
  skos:editorialNote "preferred"^^xsd:string ;
  skos:notation 1250 ;
  skos:note "Note 1 to entry:  A right specifies an action (or activity) or a class of actions that a principal can perform on or using the associated resource. A right is essentially a legally recognized entitlement to do something to or with the content of a resource."@en ;
  skos:prefLabel "right <GeoDRM>"@en ;
.
<http://iso.org/tc211/term/1251>
  rdf:type skos:Concept ;
  dcterms:dateAccepted "2014-02-15"^^xsd:date ;
  dcterms:source "ISO 19153:2014, 4.43" ;
  reg:status reg:statusValid ;
  rdfs:comment "Note 1 to entry:  Rights can be by law (copyright), by agreement, or by contract [the licence agreement]. In the case of digital commerce, DRM ensures that licences are adhered to, and that rights holders are compensated as appropriate for each transaction. Agents of the original rights holder can also issue licences, but their ability is only under the agency contract to the original principal."@en ;
  rdfs:label "rights holder"@en ;
  skos:changeNote "valid" ;
  skos:editorialNote "preferred"^^xsd:string ;
  skos:notation 1251 ;
  skos:note "Note 1 to entry:  Rights can be by law (copyright), by agreement, or by contract [the licence agreement]. In the case of digital commerce, DRM ensures that licences are adhered to, and that rights holders are compensated as appropriate for each transaction. Agents of the original rights holder can also issue licences, but their ability is only under the agency contract to the original principal."@en ;
  skos:prefLabel "rights holder"@en ;
.
<http://iso.org/tc211/term/1252>
  rdf:type skos:Concept ;
  dcterms:dateAccepted "2014-02-15"^^xsd:date ;
  dcterms:provenance "ISO 19153:2014, 4.44" ;
  dcterms:source "Thomson Reuters, “Law Dictionary,” FindLaw, for legal professionals, 2010, available at <http://dictionary.lp.findlaw.com/>, Modified" ;
  reg:status reg:statusValid ;
  rdfs:label "rights management <GeoDRM>"@en ;
  skos:changeNote "valid" ;
  skos:editorialNote "preferred"^^xsd:string ;
  skos:notation 1252 ;
  skos:prefLabel "rights management <GeoDRM>"@en ;
.
<http://iso.org/tc211/term/1253>
  rdf:type skos:Concept ;
  dcterms:dateAccepted "2014-02-15"^^xsd:date ;
  dcterms:source "ISO 19153:2014, 4.45" ;
  reg:status reg:statusValid ;
  rdfs:label "risk"@en ;
  skos:changeNote "valid" ;
  skos:editorialNote "preferred"^^xsd:string ;
  skos:notation 1253 ;
  skos:prefLabel "risk"@en ;
.
<http://iso.org/tc211/term/1254>
  rdf:type skos:Concept ;
  dcterms:dateAccepted "2014-02-15"^^xsd:date ;
  dcterms:provenance "ISO 19153:2014, 4.46" ;
  dcterms:source "Derived from Palmer & Dodge, LLP; (FindLaw)" ;
  reg:status reg:statusValid ;
  rdfs:comment "Note 1 to entry:  This is essentially the right to loan one's licence to another principal."@en ;
  rdfs:label "sublicence"@en ;
  skos:changeNote "valid" ;
  skos:editorialNote "preferred"^^xsd:string ;
  skos:notation 1254 ;
  skos:note "Note 1 to entry:  This is essentially the right to loan one's licence to another principal."@en ;
  skos:prefLabel "sublicence"@en ;
.
<http://iso.org/tc211/term/1255>
  rdf:type skos:Concept ;
  dcterms:dateAccepted "2014-02-15"^^xsd:date ;
  dcterms:source "ISO 19153:2014, 4.47" ;
  reg:status reg:statusValid ;
  rdfs:label "sublicensee"@en ;
  skos:changeNote "valid" ;
  skos:editorialNote "preferred"^^xsd:string ;
  skos:notation 1255 ;
  skos:prefLabel "sublicensee"@en ;
.
<http://iso.org/tc211/term/1256>
  rdf:type skos:Concept ;
  dcterms:dateAccepted "2014-02-15"^^xsd:date ;
  dcterms:source "ISO 19153:2014, 4.48" ;
  reg:status reg:statusValid ;
  rdfs:comment "Note 1 to entry:  A sufficient DRM system would have to be bypassed if an infringement would be possible. Proof of sufficiency can be difficult because it can be dependent on an \"attack model\", which describes the sorts of attacks to which the system is immune."@en ;
  rdfs:label "sufficient"@en ;
  skos:changeNote "valid" ;
  skos:editorialNote "preferred"^^xsd:string ;
  skos:notation 1256 ;
  skos:note "Note 1 to entry:  A sufficient DRM system would have to be bypassed if an infringement would be possible. Proof of sufficiency can be difficult because it can be dependent on an \"attack model\", which describes the sorts of attacks to which the system is immune."@en ;
  skos:prefLabel "sufficient"@en ;
.
<http://iso.org/tc211/term/1257>
  rdf:type skos:Concept ;
  dcterms:dateAccepted "2014-02-15"^^xsd:date ;
  dcterms:provenance "ISO 19153:2014, 4.49" ;
  dcterms:source "Web Service Glossary, modified" ;
  reg:status reg:statusValid ;
  rdfs:label "transaction"@en ;
  skos:changeNote "valid" ;
  skos:editorialNote "preferred"^^xsd:string ;
  skos:notation 1257 ;
  skos:prefLabel "transaction"@en ;
.
<http://iso.org/tc211/term/1258>
  rdf:type skos:Concept ;
  dcterms:dateAccepted "2014-02-15"^^xsd:date ;
  dcterms:source "ISO 19153:2014, 4.50" ;
  reg:status reg:statusValid ;
  rdfs:comment "Note 1 to entry:  Trust allows the owner [or his agent] to act with a higher potential risk because the expected risk has been lowered. This is slightly different from the plain language of trust. Normally, trust requires something, but if the principal at risk decides that no risk exists, then trust exists (in the sense here) because risk has been reduced, whatever the reason."@en ;
  rdfs:label "trust"@en ;
  skos:changeNote "valid" ;
  skos:editorialNote "preferred"^^xsd:string ;
  skos:notation 1258 ;
  skos:note "Note 1 to entry:  Trust allows the owner [or his agent] to act with a higher potential risk because the expected risk has been lowered. This is slightly different from the plain language of trust. Normally, trust requires something, but if the principal at risk decides that no risk exists, then trust exists (in the sense here) because risk has been reduced, whatever the reason."@en ;
  skos:prefLabel "trust"@en ;
.
<http://iso.org/tc211/term/1263>
  rdf:type skos:Concept ;
  dcterms:dateAccepted "2012-12-15"^^xsd:date ;
  dcterms:source "ISO 19117:2012, 4.5" ;
  reg:status reg:statusValid ;
  rdfs:label "conditional feature portrayal function"@en ;
  skos:changeNote "valid" ;
  skos:editorialNote "preferred"^^xsd:string ;
  skos:notation 1263 ;
  skos:prefLabel "conditional feature portrayal function"@en ;
.
<http://iso.org/tc211/term/1264>
  rdf:type skos:Concept ;
  dcterms:dateAccepted "2012-12-15"^^xsd:date ;
  dcterms:source "ISO 19117:2012, 4.10" ;
  reg:status reg:statusValid ;
  rdfs:label "feature portrayal function"@en ;
  skos:changeNote "valid" ;
  skos:editorialNote "preferred"^^xsd:string ;
  skos:notation 1264 ;
  skos:prefLabel "feature portrayal function"@en ;
.
<http://iso.org/tc211/term/1269>
  rdf:type skos:Concept ;
  dcterms:dateAccepted "2012-12-15"^^xsd:date ;
  dcterms:source "ISO 19117:2012, 4.23" ;
  reg:status reg:statusValid ;
  rdfs:comment "Note 1 to entry: Portrayal functions can also include parameters and other computations that are not dependent on geographic feature properties."@en ;
  rdfs:label "portrayal function"@en ;
  skos:changeNote "valid" ;
  skos:editorialNote "preferred"^^xsd:string ;
  skos:notation 1269 ;
  skos:note "Note 1 to entry: Portrayal functions can also include parameters and other computations that are not dependent on geographic feature properties."@en ;
  skos:prefLabel "portrayal function"@en ;
.
<http://iso.org/tc211/term/127>
  rdf:type skos:Concept ;
  dcterms:dateAccepted "2002-09-01"^^xsd:date ;
  dcterms:dateAccepted "2007-11-01"^^xsd:date ;
  dcterms:provenance "KS X ISO 19108" ;
  dcterms:source "ISO 19108;2002" ;
  reg:status reg:statusValid ;
  rdfs:label "day"@en ;
  skos:changeNote "valid" ;
  skos:definition "지구 자전 주기와 명목상 같은 지속 기간을 갖는 기간"@kr ;
  skos:editorialNote "preferred" ;
  skos:editorialNote "preferred"^^xsd:string ;
  skos:notation "127" ;
  skos:notation 127 ;
  skos:prefLabel "day"@en ;
  skos:prefLabel "일"@kr ;
.
<http://iso.org/tc211/term/1272>
  rdf:type skos:Concept ;
  dcterms:dateAccepted "2012-12-15"^^xsd:date ;
  dcterms:source "ISO 19117:2012, 4.28" ;
  reg:status reg:statusValid ;
  rdfs:label "simple symbol"@en ;
  skos:changeNote "valid" ;
  skos:editorialNote "preferred"^^xsd:string ;
  skos:notation 1272 ;
  skos:prefLabel "simple symbol"@en ;
.
<http://iso.org/tc211/term/1273>
  rdf:type skos:Concept ;
  dcterms:dateAccepted "2012-12-15"^^xsd:date ;
  dcterms:source "ISO 19117:2012, 4.31" ;
  reg:status reg:statusValid ;
  rdfs:label "symbol"@en ;
  skos:changeNote "valid" ;
  skos:editorialNote "preferred"^^xsd:string ;
  skos:notation 1273 ;
  skos:prefLabel "symbol"@en ;
.
<http://iso.org/tc211/term/1274>
  rdf:type skos:Concept ;
  dcterms:dateAccepted "2012-12-15"^^xsd:date ;
  dcterms:source "ISO 19117:2012, 4.32" ;
  reg:status reg:statusValid ;
  rdfs:label "symbol component"@en ;
  skos:changeNote "valid" ;
  skos:editorialNote "preferred"^^xsd:string ;
  skos:notation 1274 ;
  skos:prefLabel "symbol component"@en ;
.
<http://iso.org/tc211/term/1275>
  rdf:type skos:Concept ;
  dcterms:dateAccepted "2012-12-15"^^xsd:date ;
  dcterms:source "ISO 19117:2012, 4.33" ;
  reg:status reg:statusValid ;
  rdfs:label "symbol definition"@en ;
  skos:changeNote "valid" ;
  skos:editorialNote "preferred"^^xsd:string ;
  skos:notation 1275 ;
  skos:prefLabel "symbol definition"@en ;
.
<http://iso.org/tc211/term/1276>
  rdf:type skos:Concept ;
  dcterms:dateAccepted "2012-12-15"^^xsd:date ;
  dcterms:source "ISO 19117:2012, 4.34" ;
  reg:status reg:statusValid ;
  rdfs:label "symbol reference"@en ;
  skos:changeNote "valid" ;
  skos:editorialNote "preferred"^^xsd:string ;
  skos:notation 1276 ;
  skos:prefLabel "symbol reference"@en ;
.
<http://iso.org/tc211/term/1278>
  rdf:type skos:Concept ;
  dcterms:dateAccepted "2010-06-15"^^xsd:date ;
  dcterms:source "ISO/TS 19130:2010" ;
  reg:status reg:statusValid ;
  rdfs:comment "Note 1 to entry: Error propagation is governed by the mathematical function relating the derived quantity to the quantities from which it was derived."@en ;
  rdfs:label "error propagation"@en ;
  skos:changeNote "valid" ;
  skos:editorialNote "preferred"^^xsd:string ;
  skos:notation 1278 ;
  skos:note "Note 1 to entry: Error propagation is governed by the mathematical function relating the derived quantity to the quantities from which it was derived."@en ;
  skos:prefLabel "error propagation"@en ;
.
<http://iso.org/tc211/term/1279>
  rdf:type skos:Concept ;
  dcterms:dateAccepted "2010-11-01"^^xsd:date ;
  dcterms:source "ISO 19146:2010" ;
  reg:status reg:statusValid ;
  rdfs:label "cross-mapping"@en ;
  skos:changeNote "valid" ;
  skos:editorialNote "preferred"^^xsd:string ;
  skos:notation 1279 ;
  skos:prefLabel "cross-mapping"@en ;
.
<http://iso.org/tc211/term/128>
  rdf:type skos:Concept ;
  dcterms:dateAccepted "2008-11-15"^^xsd:date ;
  dcterms:provenance "ISO/TS 19104:2008" ;
  dcterms:source "ISO 1087-1:2000" ;
  reg:status reg:statusValid ;
  rdfs:label "definition"@en ;
  skos:changeNote "valid" ;
  skos:editorialNote "preferred"^^xsd:string ;
  skos:notation 128 ;
  skos:prefLabel "definition"@en ;
.
<http://iso.org/tc211/term/1280>
  rdf:type skos:Concept ;
  dcterms:dateAccepted "2012-11-01"^^xsd:date ;
  dcterms:source "ISO 19155:2012, 4.8" ;
  reg:status reg:statusValid ;
  rdfs:label "place"@en ;
  skos:changeNote "valid" ;
  skos:editorialNote "preferred"^^xsd:string ;
  skos:notation 1280 ;
  skos:prefLabel "place"@en ;
.
<http://iso.org/tc211/term/1286>
  rdf:type skos:Concept ;
  dcterms:dateAccepted "2012-12-01"^^xsd:date ;
  dcterms:source "ISO 19152:2012, 4.1.1" ;
  reg:status reg:statusValid ;
  rdfs:label "administrative source"@en ;
  skos:changeNote "valid" ;
  skos:editorialNote "preferred"^^xsd:string ;
  skos:notation 1286 ;
  skos:prefLabel "administrative source"@en ;
.
<http://iso.org/tc211/term/1289>
  rdf:type skos:Concept ;
  dcterms:dateAccepted "2012-12-01"^^xsd:date ;
  dcterms:source "ISO 19152:2012, 4.1.5" ;
  reg:status reg:statusValid ;
  rdfs:comment "Note 1 to entry: Boundary face strings are used to represent the boundaries of spatial units by means of line strings in 2D. This 2D representation is a 2D boundary in a 2D land administration system. In a 3D land administration system it represents a series of vertical boundary faces  where an unbounded volume is assumed, surrounded by boundary faces which intersect the Earth’s surface (such as traditionally depicted in the cadastral map)."@en ;
  rdfs:label "boundary face string"@en ;
  skos:changeNote "valid" ;
  skos:editorialNote "preferred"^^xsd:string ;
  skos:notation 1289 ;
  skos:note "Note 1 to entry: Boundary face strings are used to represent the boundaries of spatial units by means of line strings in 2D. This 2D representation is a 2D boundary in a 2D land administration system. In a 3D land administration system it represents a series of vertical boundary faces  where an unbounded volume is assumed, surrounded by boundary faces which intersect the Earth’s surface (such as traditionally depicted in the cadastral map)."@en ;
  skos:prefLabel "boundary face string"@en ;
.
<http://iso.org/tc211/term/129>
  rdf:type skos:Concept ;
  dcterms:dateAccepted "2005-08-15"^^xsd:date ;
  dcterms:dateAccepted "2007-11-01"^^xsd:date ;
  dcterms:provenance "KS X ISO 19123" ;
  dcterms:source "ISO 19123:2005" ;
  reg:status reg:statusValid ;
  rdfs:label "Delaunay triangulation"@en ;
  skos:changeNote "valid" ;
  skos:definition "삼각형을 구성하는 세 개의 정점을 지나는 원의 내부에 다른 삼각형의 어느 정점도 포함하지 않는 삼각망"@kr ;
  skos:editorialNote "preferred" ;
  skos:editorialNote "preferred"^^xsd:string ;
  skos:notation "129" ;
  skos:notation 129 ;
  skos:prefLabel "Delaunay triangulation"@en ;
  skos:prefLabel "델로니 삼각 분할"@kr ;
.
<http://iso.org/tc211/term/1290>
  rdf:type skos:Concept ;
  dcterms:dateAccepted "2012-12-01"^^xsd:date ;
  dcterms:source "ISO 19152:2012, 4.1.6" ;
  reg:status reg:statusValid ;
  rdfs:comment "Note 1 to entry: A building unit may be used for different purposes (e.g. living or commercial) or it can be under  construction."@en ;
  rdfs:label "building unit"@en ;
  skos:changeNote "valid" ;
  skos:editorialNote "preferred"^^xsd:string ;
  skos:notation 1290 ;
  skos:note "Note 1 to entry: A building unit may be used for different purposes (e.g. living or commercial) or it can be under  construction."@en ;
  skos:prefLabel "building unit"@en ;
.
<http://iso.org/tc211/term/1291>
  rdf:type skos:Concept ;
  dcterms:dateAccepted "2013-12-15"^^xsd:date ;
  dcterms:provenance "ISO 19157:2013, 4.2" ;
  dcterms:source "ISO 10303‑227:2005, 3.3.10, modified - Note has been deleted." ;
  reg:status reg:statusValid ;
  rdfs:label "catalogue"@en ;
  skos:changeNote "valid" ;
  skos:editorialNote "preferred"^^xsd:string ;
  skos:notation 1291 ;
  skos:prefLabel "catalogue"@en ;
.
<http://iso.org/tc211/term/1293>
  rdf:type skos:Concept ;
  dcterms:dateAccepted "2013-02-15"^^xsd:date ;
  dcterms:source "ISO 19145:2013, 4.1.5" ;
  reg:status reg:statusValid ;
  rdfs:comment "Note 1 to entry:  The resource can be a device or software."@en ;
  rdfs:label "converter"@en ;
  skos:changeNote "valid" ;
  skos:editorialNote "preferred"^^xsd:string ;
  skos:notation 1293 ;
  skos:note "Note 1 to entry:  The resource can be a device or software."@en ;
  skos:prefLabel "converter"@en ;
.
<http://iso.org/tc211/term/1296>
  rdf:type skos:Concept ;
  dcterms:dateAccepted "2011-12-15"^^xsd:date ;
  dcterms:source "ISO 19156:2011, 4.7" ;
  reg:status reg:statusValid ;
  rdfs:label "feature type"@en ;
  skos:changeNote "valid" ;
  skos:editorialNote "preferred"^^xsd:string ;
  skos:notation 1296 ;
  skos:prefLabel "feature type"@en ;
.
<http://iso.org/tc211/term/1298>
  rdf:type skos:Concept ;
  dcterms:dateAccepted "2013-12-15"^^xsd:date ;
  dcterms:provenance "ISO 19157:2013, 4.18" ;
  dcterms:source "ISO 2859‑5:2005, 3.4, modified – Original Example has been removed. Note 1 to entry has been added." ;
  reg:status reg:statusValid ;
  rdfs:comment "Note 1 to entry:  An item can be any part of a data set, such as a feature, feature relationship, feature attribute, or combination of these."@en ;
  rdfs:label "item"@en ;
  skos:changeNote "valid" ;
  skos:editorialNote "preferred"^^xsd:string ;
  skos:notation 1298 ;
  skos:note "Note 1 to entry:  An item can be any part of a data set, such as a feature, feature relationship, feature attribute, or combination of these."@en ;
  skos:prefLabel "item"@en ;
.
<http://iso.org/tc211/term/1299>
  rdf:type skos:Concept ;
  dcterms:dateAccepted "2010-10-15"^^xsd:date ;
  dcterms:source "ISO 19143:2010" ;
  reg:status reg:statusValid ;
  rdfs:comment "Note 1 to entry: In this International Standard, the entity types are resource types."@en ;
  rdfs:label "join predicate"@en ;
  skos:changeNote "valid" ;
  skos:editorialNote "preferred"^^xsd:string ;
  skos:notation 1299 ;
  skos:note "Note 1 to entry: In this International Standard, the entity types are resource types."@en ;
  skos:prefLabel "join predicate"@en ;
.
<http://iso.org/tc211/term/13>
  rdf:type skos:Concept ;
  dcterms:dateAccepted "2005-06-01"^^xsd:date ;
  dcterms:dateAccepted "2006-05-01"^^xsd:date ;
  dcterms:provenance "ISO 19117:2005" ;
  dcterms:source "ISO 19117:2012, 4.1" ;
  reg:status reg:statusValid ;
  rdfs:comment "Note 1 to entry: Numbers, letters, symbols, and signs are examples of annotation"@en ;
  rdfs:comment "비고: 숫자, 문자, 기호 및 부호 등"@kr ;
  rdfs:label "annotation"@en ;
  skos:changeNote "valid" ;
  skos:definition "명시를 목적으로 해설 자료에 넣는 표기"@kr ;
  skos:editorialNote "preferred" ;
  skos:editorialNote "preferred"^^xsd:string ;
  skos:notation "13" ;
  skos:notation 13 ;
  skos:note "Note 1 to entry: Numbers, letters, symbols, and signs are examples of annotation"@en ;
  skos:note "비고: 숫자, 문자, 기호 및 부호 등"@kr ;
  skos:prefLabel "annotation"@en ;
  skos:prefLabel "주석"@kr ;
.
<http://iso.org/tc211/term/130>
  rdf:type skos:Concept ;
  dcterms:dateAccepted "2005-07-15"^^xsd:date ;
  dcterms:dateAccepted "2009-12-29"^^xsd:date ;
  dcterms:provenance "ISO/TS 19103:2005 ,4.2.12" ;
  dcterms:source "ISO/IEC 19501" ;
  reg:status reg:statusValid ;
  rdfs:label "dependency <UML>"@en ;
  skos:changeNote "valid" ;
  skos:definition "하나의 모델링 요소(독립 요소)가 변경되었을 때 다른 모델링 요소(종속 요소)에 영향을 미치는 두 모델링 요소 간의 관계"@kr ;
  skos:editorialNote "preferred" ;
  skos:editorialNote "preferred"^^xsd:string ;
  skos:notation "130" ;
  skos:notation 130 ;
  skos:prefLabel "dependency <UML>"@en ;
  skos:prefLabel "의존 <UML>"@kr ;
.
<http://iso.org/tc211/term/1300>
  rdf:type skos:Concept ;
  dcterms:dateAccepted "2012-12-01"^^xsd:date ;
  dcterms:source "ISO 19152:2012, 4.1.10" ;
  reg:status reg:statusValid ;
  rdfs:comment "Note 1 to entry: In many countries, land administration information is determined, recorded and disseminated under the umbrella of cadastre and land registry. Both institutions can be unified in a single (state) organization."@en ;
  rdfs:label "land administration"@en ;
  skos:changeNote "valid" ;
  skos:editorialNote "preferred"^^xsd:string ;
  skos:notation 1300 ;
  skos:note "Note 1 to entry: In many countries, land administration information is determined, recorded and disseminated under the umbrella of cadastre and land registry. Both institutions can be unified in a single (state) organization."@en ;
  skos:prefLabel "land administration"@en ;
.
<http://iso.org/tc211/term/1301>
  rdf:type skos:Concept ;
  dcterms:dateAccepted "2012-07-01"^^xsd:date ;
  dcterms:source "ISO 19144-2:2012, 4.1.8" ;
  reg:status reg:statusValid ;
  rdfs:label "land cover metalanguage"@en ;
  skos:changeNote "valid" ;
  skos:editorialNote "preferred"^^xsd:string ;
  skos:notation 1301 ;
  skos:prefLabel "land cover metalanguage"@en ;
.
<http://iso.org/tc211/term/1302>
  rdf:type skos:Concept ;
  dcterms:dateAccepted "2012-12-01"^^xsd:date ;
  dcterms:source "ISO 19152:2012, 4.1.12" ;
  reg:status reg:statusValid ;
  rdfs:label "liminal spatial unit"@en ;
  skos:changeNote "valid" ;
  skos:editorialNote "preferred"^^xsd:string ;
  skos:notation 1302 ;
  skos:prefLabel "liminal spatial unit"@en ;
.
<http://iso.org/tc211/term/1303>
  rdf:type skos:Concept ;
  dcterms:dateAccepted "2013-12-15"^^xsd:date ;
  dcterms:source "ISO 19157:2013, 4.20" ;
  reg:status reg:statusValid ;
  rdfs:label "metaquality"@en ;
  skos:changeNote "valid" ;
  skos:editorialNote "preferred"^^xsd:string ;
  skos:notation 1303 ;
  skos:prefLabel "metaquality"@en ;
.
<http://iso.org/tc211/term/1305>
  rdf:type skos:Concept ;
  dcterms:dateAccepted "2011-12-15"^^xsd:date ;
  dcterms:source "ISO 19156:2011, 4.12" ;
  reg:status reg:statusValid ;
  rdfs:label "observation procedure"@en ;
  skos:changeNote "valid" ;
  skos:editorialNote "preferred"^^xsd:string ;
  skos:notation 1305 ;
  skos:prefLabel "observation procedure"@en ;
.
<http://iso.org/tc211/term/1306>
  rdf:type skos:Concept ;
  dcterms:dateAccepted "2011-12-15"^^xsd:date ;
  dcterms:source "ISO 19156:2011, 4.13" ;
  reg:status reg:statusValid ;
  rdfs:label "observation protocol"@en ;
  skos:changeNote "valid" ;
  skos:editorialNote "preferred"^^xsd:string ;
  skos:notation 1306 ;
  skos:prefLabel "observation protocol"@en ;
.
<http://iso.org/tc211/term/1308>
  rdf:type skos:Concept ;
  dcterms:dateAccepted "2011-12-15"^^xsd:date ;
  dcterms:source "ISO 19156:2011, 4.14" ;
  reg:status reg:statusValid ;
  rdfs:label "observation result"@en ;
  skos:changeNote "valid" ;
  skos:editorialNote "preferred"^^xsd:string ;
  skos:notation 1308 ;
  skos:prefLabel "observation result"@en ;
.
<http://iso.org/tc211/term/131>
  rdf:type skos:Concept ;
  dcterms:dateAccepted "2008-11-15"^^xsd:date ;
  dcterms:provenance "ISO/TS 19104:2008" ;
  dcterms:source "ISO 1087-1:2000" ;
  reg:status reg:statusValid ;
  rdfs:label "deprecated term"@en ;
  skos:changeNote "valid" ;
  skos:editorialNote "preferred"^^xsd:string ;
  skos:notation 131 ;
  skos:prefLabel "deprecated term"@en ;
.
<http://iso.org/tc211/term/1310>
  rdf:type skos:Concept ;
  dcterms:dateAccepted "2012-12-01"^^xsd:date ;
  dcterms:source "ISO 19152:2012, 4.1.14" ;
  reg:status reg:statusValid ;
  rdfs:label "party member"@en ;
  skos:changeNote "valid" ;
  skos:editorialNote "preferred"^^xsd:string ;
  skos:notation 1310 ;
  skos:prefLabel "party member"@en ;
.
<http://iso.org/tc211/term/1312>
  rdf:type skos:Concept ;
  dcterms:dateAccepted "2011-12-15"^^xsd:date ;
  dcterms:provenance "ISO 19156:2011, 4.16" ;
  dcterms:source "Adapted from ISO 19109:2005" ;
  reg:status reg:statusValid ;
  rdfs:comment "Note 1 to entry: The value for an instance of an observable property type can be estimated through an act of observation."@en ;
  rdfs:comment "Note 2 to entry: In chemistry-related applications, the term “determinand” or “analyte” is often used." ;
  rdfs:comment "Note 3 to entry: Adapted from ISO 19109:2005."@en ;
  rdfs:label "property type"@en ;
  skos:changeNote "valid" ;
  skos:editorialNote "preferred"^^xsd:string ;
  skos:notation 1312 ;
  skos:note "Note 1 to entry: The value for an instance of an observable property type can be estimated through an act of observation."@en ;
  skos:note "Note 2 to entry: In chemistry-related applications, the term “determinand” or “analyte” is often used."^^<http://www.w3.org/2001/XMLSchema#@en> ;
  skos:note "Note 3 to entry: Adapted from ISO 19109:2005."^^<http://www.w3.org/2001/XMLSchema#@en> ;
  skos:prefLabel "property type"@en ;
.
<http://iso.org/tc211/term/1316>
  rdf:type skos:Concept ;
  dcterms:dateAccepted "2012-12-01"^^xsd:date ;
  dcterms:source "ISO 19152:2012, 4.1.22" ;
  reg:status reg:statusValid ;
  rdfs:label "spatial source"@en ;
  skos:changeNote "valid" ;
  skos:editorialNote "preferred"^^xsd:string ;
  skos:notation 1316 ;
  skos:prefLabel "spatial source"@en ;
.
<http://iso.org/tc211/term/1318>
  rdf:type skos:Concept ;
  dcterms:dateAccepted "2012-12-01"^^xsd:date ;
  dcterms:source "ISO 19152:2012, 4.1.24" ;
  reg:status reg:statusValid ;
  rdfs:comment "Note 1 to entry: The spatial units in a spatial unit group are not necessarily continuous."@en ;
  rdfs:label "spatial unit group"@en ;
  skos:changeNote "valid" ;
  skos:editorialNote "preferred"^^xsd:string ;
  skos:notation 1318 ;
  skos:note "Note 1 to entry: The spatial units in a spatial unit group are not necessarily continuous."@en ;
  skos:prefLabel "spatial unit group"@en ;
.
<http://iso.org/tc211/term/1322>
  rdf:type skos:Concept ;
  dcterms:dateAccepted "2012-12-15"^^xsd:date ;
  dcterms:source "ISO 19117:2012, 4.17" ;
  reg:status reg:statusValid ;
  rdfs:comment "Note 1 to entry: A parameterized feature portrayal function passes the relevant attribute values from the feature instance for use as input to the parameterized symbol."@en ;
  rdfs:label "parameterized feature portrayal function"@en ;
  skos:changeNote "valid" ;
  skos:editorialNote "preferred"^^xsd:string ;
  skos:notation 1322 ;
  skos:note "Note 1 to entry: A parameterized feature portrayal function passes the relevant attribute values from the feature instance for use as input to the parameterized symbol."@en ;
  skos:prefLabel "parameterized feature portrayal function"@en ;
.
<http://iso.org/tc211/term/1323>
  rdf:type skos:Concept ;
  dcterms:dateAccepted "2012-12-15"^^xsd:date ;
  dcterms:source "ISO 19117:2012, 4.18" ;
  reg:status reg:statusValid ;
  rdfs:comment "Note 1 to entry: The dynamic parameters map to the attribute values of each feature instance being portrayed."@en ;
  rdfs:label "parameterized symbol"@en ;
  skos:changeNote "valid" ;
  skos:editorialNote "preferred"^^xsd:string ;
  skos:notation 1323 ;
  skos:note "Note 1 to entry: The dynamic parameters map to the attribute values of each feature instance being portrayed."@en ;
  skos:prefLabel "parameterized symbol"@en ;
.
<http://iso.org/tc211/term/1324>
  rdf:type skos:Concept ;
  dcterms:dateAccepted "2012-12-15"^^xsd:date ;
  dcterms:source "ISO 19117:2012, 4.21" ;
  reg:status reg:statusValid ;
  rdfs:comment "Note 1 to entry: Content of a portrayal catalogue includes portrayal functions, symbols, and portrayal context (optional)."@en ;
  rdfs:label "portrayal catalogue"@en ;
  skos:changeNote "valid" ;
  skos:editorialNote "preferred"^^xsd:string ;
  skos:notation 1324 ;
  skos:note "Note 1 to entry: Content of a portrayal catalogue includes portrayal functions, symbols, and portrayal context (optional)."@en ;
  skos:prefLabel "portrayal catalogue"@en ;
.
<http://iso.org/tc211/term/1325>
  rdf:type skos:Concept ;
  dcterms:dateAccepted "2012-12-15"^^xsd:date ;
  dcterms:source "ISO 19117:2012, 4.22" ;
  reg:status reg:statusValid ;
  rdfs:comment "Note 1 to entry: Portrayal context can influence the selection of portrayal functions and construction of symbols."@en ;
  rdfs:label "portrayal context"@en ;
  skos:changeNote "valid" ;
  skos:editorialNote "preferred"^^xsd:string ;
  skos:notation 1325 ;
  skos:note "Note 1 to entry: Portrayal context can influence the selection of portrayal functions and construction of symbols."@en ;
  skos:prefLabel "portrayal context"@en ;
.
<http://iso.org/tc211/term/1326>
  rdf:type skos:Concept ;
  dcterms:dateAccepted "2012-12-15"^^xsd:date ;
  dcterms:source "ISO 19117:2012, 4.24" ;
  reg:status reg:statusValid ;
  rdfs:label "portrayal function set"@en ;
  skos:changeNote "valid" ;
  skos:editorialNote "preferred"^^xsd:string ;
  skos:notation 1326 ;
  skos:prefLabel "portrayal function set"@en ;
.
<http://iso.org/tc211/term/1327>
  rdf:type skos:Concept ;
  dcterms:dateAccepted "2012-12-15"^^xsd:date ;
  dcterms:source "ISO 19117:2012, 4.25" ;
  reg:status reg:statusValid ;
  rdfs:comment "Note 1 to entry: A declarative language is rule-based and includes decision and branching statements."@en ;
  rdfs:label "portrayal rule"@en ;
  skos:changeNote "valid" ;
  skos:editorialNote "preferred"^^xsd:string ;
  skos:notation 1327 ;
  skos:note "Note 1 to entry: A declarative language is rule-based and includes decision and branching statements."@en ;
  skos:prefLabel "portrayal rule"@en ;
.
<http://iso.org/tc211/term/1328>
  rdf:type skos:Concept ;
  dcterms:dateAccepted "2012-12-15"^^xsd:date ;
  dcterms:source "ISO 19117:2012, 4.27" ;
  reg:status reg:statusValid ;
  rdfs:label "render"@en ;
  skos:changeNote "valid" ;
  skos:editorialNote "preferred"^^xsd:string ;
  skos:notation 1328 ;
  skos:prefLabel "render"@en ;
.
<http://iso.org/tc211/term/1329>
  rdf:type skos:Concept ;
  dcterms:dateAccepted "2012-12-15"^^xsd:date ;
  dcterms:source "ISO 19117:2012, 4.35" ;
  reg:status reg:statusValid ;
  rdfs:comment "Not 1 to entry: Symbol sets are usually designed for a community of interest to portray information of interest to the community."@en ;
  rdfs:label "symbol set"@en ;
  skos:changeNote "valid" ;
  skos:editorialNote "preferred"^^xsd:string ;
  skos:notation 1329 ;
  skos:note "Not 1 to entry: Symbol sets are usually designed for a community of interest to portray information of interest to the community."@en ;
  skos:prefLabel "symbol set"@en ;
.
<http://iso.org/tc211/term/133>
  rdf:type skos:Concept ;
  dcterms:dateAccepted "2005-10-15"^^xsd:date ;
  dcterms:dateAccepted "2006-12-01"^^xsd:date ;
  dcterms:provenance "KS X ISO 19133" ;
  dcterms:source "ISO 19133:2005" ;
  reg:status reg:statusValid ;
  rdfs:comment "Note 1 to entry: The term comes from the most commonly known algorithm for finding a shortest path in a positively weighted graph, from E. Dijkstra's paper [7]. Although this algorithm is not the only one in use, the requirements for the graph are common to most. The most common relaxation of the requirement is the \"positive weights,\" which are not needed in the Bellman-Ford algorithm [4], [8]."@en ;
  rdfs:comment "비고: 이 용어는 E. Dijkstra의 논문 중, 양의 가중 그래프 방식으로 최단 거리를 찾는 가장 일반적으로 알려진 알고리듬에서 유래되었다. 이 알고리듬만이 유일하게 사용되지는 않지만, 이 그래프가 요구하는 필요 항목들은 대부분의 알고리듬에서도 동일하게 사용된다. \"양의 가중치\"는 필요 항목 중 중요도가 떨어지는 대표적인 것으로 벨만-포드 알고리듬에서는 사용되지 않는다. "@kr ;
  rdfs:label "Dijkstra graph"@en ;
  skos:changeNote "valid" ;
  skos:definition "최단 경로 탐색을 위해 적합하게 설정된 양의 가중 방향 그래프"@kr ;
  skos:editorialNote "preferred" ;
  skos:editorialNote "preferred"^^xsd:string ;
  skos:notation "133" ;
  skos:notation 133 ;
  skos:note "Note 1 to entry: The term comes from the most commonly known algorithm for finding a shortest path in a positively weighted graph, from E. Dijkstra's paper [7]. Although this algorithm is not the only one in use, the requirements for the graph are common to most. The most common relaxation of the requirement is the \"positive weights,\" which are not needed in the Bellman-Ford algorithm [4], [8]."@en ;
  skos:note "비고: 이 용어는 E. Dijkstra의 논문 중, 양의 가중 그래프 방식으로 최단 거리를 찾는 가장 일반적으로 알려진 알고리듬에서 유래되었다. 이 알고리듬만이 유일하게 사용되지는 않지만, 이 그래프가 요구하는 필요 항목들은 대부분의 알고리듬에서도 동일하게 사용된다. \"양의 가중치\"는 필요 항목 중 중요도가 떨어지는 대표적인 것으로 벨만-포드 알고리듬에서는 사용되지 않는다. "@kr ;
  skos:prefLabel "Dijkstra graph"@en ;
  skos:prefLabel "다익스트라 그래프"@kr ;
.
<http://iso.org/tc211/term/1330>
  rdf:type skos:Concept ;
  dcterms:dateAccepted "2012-10-15"^^xsd:date ;
  dcterms:provenance "ISO/TS 19158:2012, 4.1" ;
  dcterms:source "ISO 9000:2005" ;
  reg:status reg:statusValid ;
  rdfs:comment "Note 1 to entry: The customer can be internal or external to the supplier organisation."@en ;
  rdfs:label "customer"@en ;
  skos:changeNote "valid" ;
  skos:editorialNote "preferred"^^xsd:string ;
  skos:notation 1330 ;
  skos:note "Note 1 to entry: The customer can be internal or external to the supplier organisation."@en ;
  skos:prefLabel "customer"@en ;
.
<http://iso.org/tc211/term/1331>
  rdf:type skos:Concept ;
  dcterms:dateAccepted "2012-10-15"^^xsd:date ;
  dcterms:provenance "ISO/TS 19158:2012, 4.2" ;
  dcterms:source "ISO 9000:2005" ;
  reg:status reg:statusValid ;
  rdfs:comment "Note 1 to entry: The process may be broken down further into elemental activities [sub process]as is deemed necessary to control the quality of the process."@en ;
  rdfs:label "process"@en ;
  skos:changeNote "valid" ;
  skos:editorialNote "preferred"^^xsd:string ;
  skos:notation 1331 ;
  skos:note "Note 1 to entry: The process may be broken down further into elemental activities [sub process]as is deemed necessary to control the quality of the process."@en ;
  skos:prefLabel "process"@en ;
.
<http://iso.org/tc211/term/1332>
  rdf:type skos:Concept ;
  dcterms:dateAccepted "2012-10-15"^^xsd:date ;
  dcterms:provenance "ISO/TS 19158:2012, 4.11" ;
  dcterms:source "ISO 9000:2005" ;
  reg:status reg:statusValid ;
  rdfs:comment "Note 1 to entry: The supplier can be internal or external to the customer organization."@en ;
  rdfs:comment "Note 2 to entry: In the context of this Technical Specification, the supplier has provided a product via a process that can have some impact on quality." ;
  rdfs:label "supplier"@en ;
  skos:changeNote "valid" ;
  skos:editorialNote "preferred"^^xsd:string ;
  skos:notation 1332 ;
  skos:note "Note 1 to entry: The supplier can be internal or external to the customer organization."@en ;
  skos:note "Note 2 to entry: In the context of this Technical Specification, the supplier has provided a product via a process that can have some impact on quality."^^<http://www.w3.org/2001/XMLSchema#@en> ;
  skos:prefLabel "supplier"@en ;
.
<http://iso.org/tc211/term/1333>
  rdf:type skos:Concept ;
  dcterms:dateAccepted "2010-12-15"^^xsd:date ;
  dcterms:source "ISO 19142:2010" ;
  reg:status reg:statusValid ;
  rdfs:comment "Note 1 to entry: In this International Standard, the object instances will be feature instances."@en ;
  rdfs:label "join tuple"@en ;
  skos:changeNote "valid" ;
  skos:editorialNote "preferred"^^xsd:string ;
  skos:notation 1333 ;
  skos:note "Note 1 to entry: In this International Standard, the object instances will be feature instances."@en ;
  skos:prefLabel "join tuple"@en ;
.
<http://iso.org/tc211/term/1334>
  rdf:type skos:Concept ;
  dcterms:dateAccepted "2010-12-15"^^xsd:date ;
  dcterms:source "ISO 19142:2010" ;
  reg:status reg:statusValid ;
  rdfs:comment "Note 1 to entry: In this International Standard, the system is a web feature service and the resource is held in a data store that is directly controlled by that service."@en ;
  rdfs:label "local resource"@en ;
  skos:changeNote "valid" ;
  skos:editorialNote "preferred"^^xsd:string ;
  skos:notation 1334 ;
  skos:note "Note 1 to entry: In this International Standard, the system is a web feature service and the resource is held in a data store that is directly controlled by that service."@en ;
  skos:prefLabel "local resource"@en ;
.
<http://iso.org/tc211/term/1335>
  rdf:type skos:Concept ;
  dcterms:dateAccepted "2010-12-15"^^xsd:date ;
  dcterms:source "ISO 19142:2010" ;
  reg:status reg:statusValid ;
  rdfs:comment "Note 1 to entry: In XML, this attribute is commonly called an href and contains a URI reference to the remote resource (see W3C XLink)"@en ;
  rdfs:label "locator attribute"@en ;
  skos:changeNote "valid" ;
  skos:editorialNote "preferred"^^xsd:string ;
  skos:notation 1335 ;
  skos:note "Note 1 to entry: In XML, this attribute is commonly called an href and contains a URI reference to the remote resource (see W3C XLink)"@en ;
  skos:prefLabel "locator attribute"@en ;
.
<http://iso.org/tc211/term/1336>
  rdf:type skos:Concept ;
  dcterms:dateAccepted "2010-12-15"^^xsd:date ;
  dcterms:provenance "ISO 19142:2010" ;
  dcterms:source "IETF RFC 2045:1996" ;
  reg:status reg:statusValid ;
  rdfs:label "Multipurpose Internet Mail Extensions (MIME) type"@en ;
  skos:changeNote "valid" ;
  skos:editorialNote "preferred"^^xsd:string ;
  skos:notation 1336 ;
  skos:prefLabel "Multipurpose Internet Mail Extensions (MIME) type"@en ;
.
<http://iso.org/tc211/term/1337>
  rdf:type skos:Concept ;
  dcterms:dateAccepted "2012-11-01"^^xsd:date ;
  dcterms:source "ISO 19155:2012, 4.9" ;
  reg:status reg:statusValid ;
  rdfs:comment "Note 1 to entry:  The same place may be referenced by multiple Place Identifier instances. Each instance will be associated with a different reference system."@en ;
  rdfs:label "Place Identifier"@en ;
  skos:altLabel "PI"^^<http://www.w3.org/2001/XMLSchema#@en> ;
  skos:changeNote "valid" ;
  skos:editorialNote "preferred"^^xsd:string ;
  skos:notation 1337 ;
  skos:note "Note 1 to entry:  The same place may be referenced by multiple Place Identifier instances. Each instance will be associated with a different reference system."@en ;
  skos:prefLabel "Place Identifier"@en ;
.
<http://iso.org/tc211/term/1338>
  rdf:type skos:Concept ;
  dcterms:dateAccepted "2012-11-01"^^xsd:date ;
  dcterms:source "ISO 19155:2012, 4.10" ;
  reg:status reg:statusValid ;
  rdfs:label "Place Identifier application"@en ;
  skos:altLabel "PI application"^^<http://www.w3.org/2001/XMLSchema#@en> ;
  skos:changeNote "valid" ;
  skos:editorialNote "preferred"^^xsd:string ;
  skos:notation 1338 ;
  skos:prefLabel "Place Identifier application"@en ;
.
<http://iso.org/tc211/term/1339>
  rdf:type skos:Concept ;
  dcterms:dateAccepted "2012-11-01"^^xsd:date ;
  dcterms:source "ISO 19155:2012, 4.11" ;
  reg:status reg:statusValid ;
  rdfs:comment "Note 1 to entry: A source PI can be matched with multiple target Place Identifiers."@en ;
  rdfs:comment "Note 2 to entry: PI matching can be made among coordinates, geographic identifiers and identifiers in the virtual world such as URI." ;
  rdfs:label "Place Identifier matching"@en ;
  skos:altLabel "PI matching"^^<http://www.w3.org/2001/XMLSchema#@en> ;
  skos:changeNote "valid" ;
  skos:editorialNote "preferred"^^xsd:string ;
  skos:notation 1339 ;
  skos:note "Note 1 to entry: A source PI can be matched with multiple target Place Identifiers."@en ;
  skos:note "Note 2 to entry: PI matching can be made among coordinates, geographic identifiers and identifiers in the virtual world such as URI."^^<http://www.w3.org/2001/XMLSchema#@en> ;
  skos:prefLabel "Place Identifier matching"@en ;
.
<http://iso.org/tc211/term/134>
  rdf:type skos:Concept ;
  dcterms:dateAccepted "2003-08-15"^^xsd:date ;
  dcterms:dateAccepted "2009-12-29"^^xsd:date ;
  dcterms:provenance "ISO 19114:2003" ;
  dcterms:source "ISO 19157:2013, 4.10" ;
  reg:status reg:statusValid ;
  rdfs:label "direct evaluation method"@en ;
  skos:changeNote "valid" ;
  skos:definition "데이터셋 내의 항목 검사에 의거한 데이터셋 품질 평가 방법"@kr ;
  skos:editorialNote "preferred" ;
  skos:editorialNote "preferred"^^xsd:string ;
  skos:notation "134" ;
  skos:notation 134 ;
  skos:prefLabel "direct evaluation method"@en ;
  skos:prefLabel "직접 평가법"@kr ;
.
<http://iso.org/tc211/term/1340>
  rdf:type skos:Concept ;
  dcterms:dateAccepted "2012-11-01"^^xsd:date ;
  dcterms:source "ISO 19155:2012, 4.12" ;
  reg:status reg:statusValid ;
  rdfs:label "Place Identifier platform"@en ;
  skos:altLabel "PI platform"^^<http://www.w3.org/2001/XMLSchema#@en> ;
  skos:changeNote "valid" ;
  skos:editorialNote "preferred"^^xsd:string ;
  skos:notation 1340 ;
  skos:prefLabel "Place Identifier platform"@en ;
.
<http://iso.org/tc211/term/1341>
  rdf:type skos:Concept ;
  dcterms:dateAccepted "2010-12-15"^^xsd:date ;
  dcterms:source "ISO 19142:2010" ;
  reg:status reg:statusValid ;
  rdfs:comment "Note 1 to entry: In this International Standard, the system is a web feature service. The resource is not held in any data store that is directly controlled by that service and thus cannot be directly retreived by the service."@en ;
  rdfs:label "remote resource"@en ;
  skos:changeNote "valid" ;
  skos:editorialNote "preferred"^^xsd:string ;
  skos:notation 1341 ;
  skos:note "Note 1 to entry: In this International Standard, the system is a web feature service. The resource is not held in any data store that is directly controlled by that service and thus cannot be directly retreived by the service."@en ;
  skos:prefLabel "remote resource"@en ;
.
<http://iso.org/tc211/term/1342>
  rdf:type skos:Concept ;
  dcterms:dateAccepted "2010-12-15"^^xsd:date ;
  dcterms:source "ISO 19142:2010" ;
  reg:status reg:statusValid ;
  rdfs:comment "Note 1 to entry: The insertion may be accomplished by either replacing the reference inline with a copy of the resource or by relocating the reference to point to a copy of the resource that has been placed in the response document."@en ;
  rdfs:label "resolve"@en ;
  skos:changeNote "valid" ;
  skos:editorialNote "preferred"^^xsd:string ;
  skos:notation 1342 ;
  skos:note "Note 1 to entry: The insertion may be accomplished by either replacing the reference inline with a copy of the resource or by relocating the reference to point to a copy of the resource that has been placed in the response document."@en ;
  skos:prefLabel "resolve"@en ;
.
<http://iso.org/tc211/term/1344>
  rdf:type skos:Concept ;
  dcterms:dateAccepted "2014-11-01"^^xsd:date ;
  dcterms:provenance "ISO 19101-1:2014, 4.1.23" ;
  dcterms:source "ISO/IEC 2382-1:1993, 01.01.22" ;
  reg:status reg:statusValid ;
  rdfs:label "information system"@en ;
  skos:changeNote "valid" ;
  skos:editorialNote "preferred"^^xsd:string ;
  skos:notation 1344 ;
  skos:prefLabel "information system"@en ;
.
<http://iso.org/tc211/term/1346>
  rdf:type skos:Concept ;
  dcterms:dateAccepted "2012-11-15"^^xsd:date ;
  dcterms:provenance "ISO/TS 19150-1:2012" ;
  dcterms:source "ISO 19101-1:2014, 4.1.26" ;
  reg:status reg:statusValid ;
  rdfs:label "ontology"@en ;
  skos:changeNote "valid" ;
  skos:editorialNote "preferred"^^xsd:string ;
  skos:notation 1346 ;
  skos:prefLabel "ontology"@en ;
.
<http://iso.org/tc211/term/135>
  rdf:type skos:Concept ;
  dcterms:dateAccepted "2003-05-01"^^xsd:date ;
  dcterms:dateAccepted "2009-12-29"^^xsd:date ;
  dcterms:provenance "KS X ISO 19107" ;
  dcterms:source "ISO 19107:2003" ;
  reg:status reg:statusValid ;
  rdfs:label "direct position"@en ;
  skos:changeNote "valid" ;
  skos:definition "좌표 참조 체계 내에서 단일 좌표 집합에 의해 기술되는 위치"@kr ;
  skos:editorialNote "preferred" ;
  skos:editorialNote "preferred"^^xsd:string ;
  skos:notation "135" ;
  skos:notation 135 ;
  skos:prefLabel "direct position"@en ;
  skos:prefLabel "직접 위치"@kr ;
.
<http://iso.org/tc211/term/1351>
  rdf:type skos:Concept ;
  dcterms:dateAccepted "2012-11-15"^^xsd:date ;
  dcterms:provenance "ISO/TS 19150-1:2012" ;
  dcterms:source "ISO 19101-1:2014, 4.1.35" ;
  reg:status reg:statusValid ;
  rdfs:comment "Note 1 to entry:  The association of meaning allows data and information to be understood and processed by automated tools as well as by people."@en ;
  rdfs:label "Semantic Web"@en ;
  skos:changeNote "valid" ;
  skos:editorialNote "preferred"^^xsd:string ;
  skos:notation 1351 ;
  skos:note "Note 1 to entry:  The association of meaning allows data and information to be understood and processed by automated tools as well as by people."@en ;
  skos:prefLabel "Semantic Web"@en ;
.
<http://iso.org/tc211/term/1356>
  rdf:type skos:Concept ;
  dcterms:dateAccepted "2013-12-15"^^xsd:date ;
  dcterms:provenance "ISO 19157:2013" ;
  dcterms:source "ISO 19115-1:2014, 4.4" ;
  reg:status reg:statusValid ;
  rdfs:label "dataset series"@en ;
  skos:changeNote "valid" ;
  skos:editorialNote "preferred"^^xsd:string ;
  skos:notation 1356 ;
  skos:prefLabel "dataset series"@en ;
.
<http://iso.org/tc211/term/1358>
  rdf:type skos:Concept ;
  dcterms:dateAccepted "2014-04-01"^^xsd:date ;
  dcterms:source "ISO 19115-1:2014, 4.17" ;
  reg:status reg:statusValid ;
  rdfs:label "resource"@en ;
  skos:changeNote "valid" ;
  skos:editorialNote "preferred"^^xsd:string ;
  skos:notation 1358 ;
  skos:prefLabel "resource"@en ;
.
<http://iso.org/tc211/term/1359>
  rdf:type skos:Concept ;
  dcterms:dateAccepted "2012-12-01"^^xsd:date ;
  dcterms:source "ISO 19152:2012, 4.1.4" ;
  reg:status reg:statusValid ;
  rdfs:comment "Note 1 to entry: Boundary faces are used when the implied vertical and unbounded faces of a boundary face string are not sufficient to describe 3D spatial units. Boundary faces close volumes in height (e.g. every apartment floor), or in depth (e.g. an underground parking garage), or in all other directions to form a bounded volume. The volumes represent legal space (in contrast with physical space)."@en ;
  rdfs:label "boundary face"@en ;
  skos:changeNote "valid" ;
  skos:editorialNote "preferred"^^xsd:string ;
  skos:notation 1359 ;
  skos:note "Note 1 to entry: Boundary faces are used when the implied vertical and unbounded faces of a boundary face string are not sufficient to describe 3D spatial units. Boundary faces close volumes in height (e.g. every apartment floor), or in depth (e.g. an underground parking garage), or in all other directions to form a bounded volume. The volumes represent legal space (in contrast with physical space)."@en ;
  skos:prefLabel "boundary face"@en ;
.
<http://iso.org/tc211/term/136>
  rdf:type skos:Concept ;
  dcterms:dateAccepted "2003-05-01"^^xsd:date ;
  dcterms:dateAccepted "2009-12-29"^^xsd:date ;
  dcterms:provenance "KS X ISO 19107" ;
  dcterms:source "ISO 19107:2003" ;
  reg:status reg:statusValid ;
  rdfs:comment "Note 1 to entry: A directed edge that is in agreement with the orientation of the edge has a + orientation, otherwise, it has the opposite (-) orientation. Directed edge is used in topology to distinguish the right side (-) from the left side (+) of the same edge and the start node (-) and end node (+) of the same edge and in computational topology to represent these concepts."@en ;
  rdfs:comment "비고: 방향성 변은 그 변의 방향과 일치하면 + 방향을, 그렇지 않으면 - 방향을 가진다. 방향성 변은 계산 위상에서 동일한 변의 오른편(-)인지 왼편(+)인지를 구분하기 위해 사용되며, 동일한 변의 시작 절점(-)과 끝 절점(+)을 구분하여 컴퓨터를 이용하는 위상학이 이러한 개념을 표현할 수 있도록 한다. "@kr ;
  rdfs:label "directed edge"@en ;
  skos:changeNote "valid" ;
  skos:definition "하나의 변과 그 변이 갖는 방향성 간의 연관으로 표현된 방향성 위상 객체"@kr ;
  skos:editorialNote "preferred" ;
  skos:editorialNote "preferred"^^xsd:string ;
  skos:notation "136" ;
  skos:notation 136 ;
  skos:note "Note 1 to entry: A directed edge that is in agreement with the orientation of the edge has a + orientation, otherwise, it has the opposite (-) orientation. Directed edge is used in topology to distinguish the right side (-) from the left side (+) of the same edge and the start node (-) and end node (+) of the same edge and in computational topology to represent these concepts."@en ;
  skos:note "비고: 방향성 변은 그 변의 방향과 일치하면 + 방향을, 그렇지 않으면 - 방향을 가진다. 방향성 변은 계산 위상에서 동일한 변의 오른편(-)인지 왼편(+)인지를 구분하기 위해 사용되며, 동일한 변의 시작 절점(-)과 끝 절점(+)을 구분하여 컴퓨터를 이용하는 위상학이 이러한 개념을 표현할 수 있도록 한다. "@kr ;
  skos:prefLabel "directed edge"@en ;
  skos:prefLabel "방향성 변"@kr ;
.
<http://iso.org/tc211/term/1360>
  rdf:type skos:Concept ;
  dcterms:dateAccepted "2012-12-01"^^xsd:date ;
  dcterms:provenance "ISO 19152:2012, 4.1.9" ;
  dcterms:source "UN/ECE, 2004" ;
  reg:status reg:statusValid ;
  rdfs:label "land"@en ;
  skos:changeNote "valid" ;
  skos:editorialNote "preferred"^^xsd:string ;
  skos:notation 1360 ;
  skos:prefLabel "land"@en ;
.
<http://iso.org/tc211/term/1362>
  rdf:type skos:Concept ;
  dcterms:dateAccepted "2012-12-01"^^xsd:date ;
  dcterms:source "ISO 19152:2012, 4.1.17" ;
  reg:status reg:statusValid ;
  rdfs:comment "Note 1 to entry: Due to legal aspects, history of data, inaccurate geometries or missing geometries, geospatial overlay techniques may generate invalid, or no relationships between spatial units, which can be introduced by required relationships."@en ;
  rdfs:comment "Note 2 to entry: Relationships for spatial units may be defined with ISO 19125-2 types." ;
  rdfs:label "required relationship"@en ;
  skos:changeNote "valid" ;
  skos:editorialNote "preferred"^^xsd:string ;
  skos:notation 1362 ;
  skos:note "Note 1 to entry: Due to legal aspects, history of data, inaccurate geometries or missing geometries, geospatial overlay techniques may generate invalid, or no relationships between spatial units, which can be introduced by required relationships."@en ;
  skos:note "Note 2 to entry: Relationships for spatial units may be defined with ISO 19125-2 types."^^<http://www.w3.org/2001/XMLSchema#@en> ;
  skos:prefLabel "required relationship"@en ;
.
<http://iso.org/tc211/term/1363>
  rdf:type skos:Concept ;
  dcterms:dateAccepted "2012-12-01"^^xsd:date ;
  dcterms:source "ISO 19152:2012, 4.1.23" ;
  reg:status reg:statusValid ;
  rdfs:comment "Note 1 to entry: A single area is the norm and multiple areas are the exception."@en ;
  rdfs:comment "Note 2 to entry: Spatial units are structured in a way to support the creation and management of basic administrative units." ;
  rdfs:comment "Note 3 to entry: This International Standard [ISO 19152:2012] supports either 2-dimensional (2D), 3-dimensional (3D), or mixed (2D and 3D) representations of spatial units, which may be described in text (“from this tree to that river”), or based on a single point, or represented as a set of unstructured lines, or as a surface, or as a 3D volume."@en ;
  rdfs:comment "Note 4 to entry: In addition to spatial units represented by a single point, text, or a set of unstructured lines, a spatial unit may have an area equal to zero for administrative reasons."@en ;
  rdfs:label "spatial unit"@en ;
  skos:changeNote "valid" ;
  skos:editorialNote "preferred"^^xsd:string ;
  skos:notation 1363 ;
  skos:note "Note 1 to entry: A single area is the norm and multiple areas are the exception."@en ;
  skos:note "Note 2 to entry: Spatial units are structured in a way to support the creation and management of basic administrative units."^^<http://www.w3.org/2001/XMLSchema#@en> ;
  skos:note "Note 3 to entry: This International Standard [ISO 19152:2012] supports either 2-dimensional (2D), 3-dimensional (3D), or mixed (2D and 3D) representations of spatial units, which may be described in text (“from this tree to that river”), or based on a single point, or represented as a set of unstructured lines, or as a surface, or as a 3D volume."^^<http://www.w3.org/2001/XMLSchema#@en> ;
  skos:note "Note 4 to entry: In addition to spatial units represented by a single point, text, or a set of unstructured lines, a spatial unit may have an area equal to zero for administrative reasons."@en ;
  skos:prefLabel "spatial unit"@en ;
.
<http://iso.org/tc211/term/1365>
  rdf:type skos:Concept ;
  dcterms:dateAccepted "2012-02-15"^^xsd:date ;
  dcterms:source "ISO 19148:2012, 4.11" ;
  reg:status reg:statusValid ;
  rdfs:label "Linear Referencing Method"@en ;
  skos:changeNote "valid" ;
  skos:editorialNote "preferred"^^xsd:string ;
  skos:notation 1365 ;
  skos:prefLabel "Linear Referencing Method"@en ;
.
<http://iso.org/tc211/term/1366>
  rdf:type skos:Concept ;
  dcterms:dateAccepted "2013-12-15"^^xsd:date ;
  dcterms:source "ISO 19157:2013, 4.4" ;
  reg:status reg:statusValid ;
  rdfs:label "conformance quality level"@en ;
  skos:changeNote "valid" ;
  skos:editorialNote "preferred"^^xsd:string ;
  skos:notation 1366 ;
  skos:prefLabel "conformance quality level"@en ;
.
<http://iso.org/tc211/term/1367>
  rdf:type skos:Concept ;
  dcterms:dateAccepted "2013-12-15"^^xsd:date ;
  dcterms:source "ISO 19157:2013, 4.23" ;
  reg:status reg:statusValid ;
  rdfs:label "standalone quality report"@en ;
  skos:changeNote "valid" ;
  skos:editorialNote "preferred"^^xsd:string ;
  skos:notation 1367 ;
  skos:prefLabel "standalone quality report"@en ;
.
<http://iso.org/tc211/term/137>
  rdf:type skos:Concept ;
  dcterms:dateAccepted "2003-05-01"^^xsd:date ;
  dcterms:dateAccepted "2009-12-29"^^xsd:date ;
  dcterms:provenance "KS X ISO 19107" ;
  dcterms:source "ISO 19107:2003" ;
  reg:status reg:statusValid ;
  rdfs:comment "Note 1 to entry: The orientation of the directed edges that compose the exterior boundary of a directed face will appear positive from the direction of this vector; the orientation of a directed face that bounds a topological solid will point away from the topological solid. Adjacent solids would use different orientations for their shared boundary, consistent with the same sort of association between adjacent faces and their shared edges. Directed faces are used in the coboundary relation to maintain the spatial association between face and edge."@en ;
  rdfs:comment "비고: 방향성 면의 외부 경계를 구성하는 방향성 변은 벡터의 방향을 따라 양의 값을 갖는다; 위상 입방체를 구성하는 방향성 면의 방향은 위상 입방체에서 멀어지는 방향이다. 인접하는 입방체는 그들이 공유하는 면에 대해 서로 다른 방향성을 가지며, 이는 이웃하는 면과 그들이 공유하는 변들과의 관계와 일치한다. 방향성 면은 면과 변 결합의 공간적 관계를 유지하기 위한 공유 경계 관계에서 이용된다. "@kr ;
  rdfs:label "directed face"@en ;
  skos:changeNote "valid" ;
  skos:definition "하나의 면과 그 면이 갖는 방향성 간의 연관으로 표현된 방향성 위상 객체"@kr ;
  skos:editorialNote "preferred" ;
  skos:editorialNote "preferred"^^xsd:string ;
  skos:notation "137" ;
  skos:notation 137 ;
  skos:note "Note 1 to entry: The orientation of the directed edges that compose the exterior boundary of a directed face will appear positive from the direction of this vector; the orientation of a directed face that bounds a topological solid will point away from the topological solid. Adjacent solids would use different orientations for their shared boundary, consistent with the same sort of association between adjacent faces and their shared edges. Directed faces are used in the coboundary relation to maintain the spatial association between face and edge."@en ;
  skos:note "비고: 방향성 면의 외부 경계를 구성하는 방향성 변은 벡터의 방향을 따라 양의 값을 갖는다; 위상 입방체를 구성하는 방향성 면의 방향은 위상 입방체에서 멀어지는 방향이다. 인접하는 입방체는 그들이 공유하는 면에 대해 서로 다른 방향성을 가지며, 이는 이웃하는 면과 그들이 공유하는 변들과의 관계와 일치한다. 방향성 면은 면과 변 결합의 공간적 관계를 유지하기 위한 공유 경계 관계에서 이용된다. "@kr ;
  skos:prefLabel "directed face"@en ;
  skos:prefLabel "방향성 면"@kr ;
.
<http://iso.org/tc211/term/1371>
  rdf:type skos:Concept ;
  dcterms:dateAccepted "2012-10-15"^^xsd:date ;
  dcterms:provenance "ISO/TS 19158:2012, 4.7" ;
  dcterms:source "ISO 9000:2005" ;
  reg:status reg:statusValid ;
  rdfs:label "quality assurance"@en ;
  skos:changeNote "valid" ;
  skos:editorialNote "preferred"^^xsd:string ;
  skos:notation 1371 ;
  skos:prefLabel "quality assurance"@en ;
.
<http://iso.org/tc211/term/1372>
  rdf:type skos:Concept ;
  dcterms:dateAccepted "2012-10-15"^^xsd:date ;
  dcterms:provenance "ISO/TS 19158:2012, 4.9" ;
  dcterms:source "ISO 9000:2005" ;
  reg:status reg:statusValid ;
  rdfs:label "quality control"@en ;
  skos:changeNote "valid" ;
  skos:editorialNote "preferred"^^xsd:string ;
  skos:notation 1372 ;
  skos:prefLabel "quality control"@en ;
.
<http://iso.org/tc211/term/1377>
  rdf:type skos:Concept ;
  dcterms:dateAccepted "2012-12-15"^^xsd:date ;
  dcterms:provenance "ISO/TS 19139-2:2012, 4.1" ;
  dcterms:source "W3C XML" ;
  reg:status reg:statusValid ;
  rdfs:label "document <XML>"@en ;
  skos:changeNote "valid" ;
  skos:editorialNote "preferred"^^xsd:string ;
  skos:notation 1377 ;
  skos:prefLabel "document <XML>"@en ;
.
<http://iso.org/tc211/term/1378>
  rdf:type skos:Concept ;
  dcterms:dateAccepted "2014-01-15"^^xsd:date ;
  dcterms:source "ISO/TS 19130-2:2014, 4.1" ;
  reg:status reg:statusValid ;
  rdfs:label "active sensor"@en ;
  skos:changeNote "valid" ;
  skos:editorialNote "preferred"^^xsd:string ;
  skos:notation 1378 ;
  skos:prefLabel "active sensor"@en ;
.
<http://iso.org/tc211/term/1379>
  rdf:type skos:Concept ;
  dcterms:dateAccepted "2014-01-15"^^xsd:date ;
  dcterms:source "ISO/TS 19130-2:2014, 4.2" ;
  reg:status reg:statusValid ;
  rdfs:label "active sonar"@en ;
  skos:changeNote "valid" ;
  skos:editorialNote "preferred"^^xsd:string ;
  skos:notation 1379 ;
  skos:prefLabel "active sonar"@en ;
.
<http://iso.org/tc211/term/138>
  rdf:type skos:Concept ;
  dcterms:dateAccepted "2003-05-01"^^xsd:date ;
  dcterms:dateAccepted "2009-12-29"^^xsd:date ;
  dcterms:provenance "KS X ISO 19107" ;
  dcterms:source "ISO 19107:2003" ;
  reg:status reg:statusValid ;
  rdfs:comment "Note 1 to entry: Directed nodes are used in the coboundary relation to maintain the spatial association between edge and node. The orientation of a node is with respect to an edge, \"+\" for end node, \"-\" for start node. This is consistent with the vector notion of \"result = end - start\"."@en ;
  rdfs:comment "비고: 방향성 절점은 변과 절점 간의 공간적인 관계를 유지하기 위해 공유 경계 측면에서 사용된다. 절점의 방향성은 변에 따르며, \"+\"는 끝 절점, \"-\"는 시작 절점에 부여된다. 이것은 다음의 벡터 기술법과도 일치한다. \"방향 = 종점 - 시점\"."@kr ;
  rdfs:label "directed node"@en ;
  skos:changeNote "valid" ;
  skos:definition "하나의 절점과 그 절점이 갖는 방향성 간의 연관으로 표현된 방향성 위상 객체"@kr ;
  skos:editorialNote "preferred" ;
  skos:editorialNote "preferred"^^xsd:string ;
  skos:notation "138" ;
  skos:notation 138 ;
  skos:note "Note 1 to entry: Directed nodes are used in the coboundary relation to maintain the spatial association between edge and node. The orientation of a node is with respect to an edge, \"+\" for end node, \"-\" for start node. This is consistent with the vector notion of \"result = end - start\"."@en ;
  skos:note "비고: 방향성 절점은 변과 절점 간의 공간적인 관계를 유지하기 위해 공유 경계 측면에서 사용된다. 절점의 방향성은 변에 따르며, \"+\"는 끝 절점, \"-\"는 시작 절점에 부여된다. 이것은 다음의 벡터 기술법과도 일치한다. \"방향 = 종점 - 시점\"."@kr ;
  skos:prefLabel "directed node"@en ;
  skos:prefLabel "방향성 절점"@kr ;
.
<http://iso.org/tc211/term/1380>
  rdf:type skos:Concept ;
  dcterms:dateAccepted "2014-01-15"^^xsd:date ;
  dcterms:source "ISO/TS 19130-2:2014, 4.5" ;
  reg:status reg:statusValid ;
  rdfs:label "area recording"@en ;
  skos:changeNote "valid" ;
  skos:editorialNote "preferred"^^xsd:string ;
  skos:notation 1380 ;
  skos:prefLabel "area recording"@en ;
.
<http://iso.org/tc211/term/1383>
  rdf:type skos:Concept ;
  dcterms:dateAccepted "2014-01-15"^^xsd:date ;
  dcterms:source "ISO/TS 19130-2:2014, 4.11" ;
  reg:status reg:statusValid ;
  rdfs:label "complex image"@en ;
  skos:changeNote "valid" ;
  skos:editorialNote "preferred"^^xsd:string ;
  skos:notation 1383 ;
  skos:prefLabel "complex image"@en ;
.
<http://iso.org/tc211/term/1384>
  rdf:type skos:Concept ;
  dcterms:dateAccepted "2014-01-15"^^xsd:date ;
  dcterms:source "ISO/TS 19130-2:2014, 4.13" ;
  reg:status reg:statusValid ;
  rdfs:comment "Note 1 to entry:  Approximately the complement of the look angle"@en ;
  rdfs:label "depression angle"@en ;
  skos:changeNote "valid" ;
  skos:editorialNote "preferred"^^xsd:string ;
  skos:notation 1384 ;
  skos:note "Note 1 to entry:  Approximately the complement of the look angle"@en ;
  skos:prefLabel "depression angle"@en ;
.
<http://iso.org/tc211/term/1386>
  rdf:type skos:Concept ;
  dcterms:dateAccepted "2014-01-15"^^xsd:date ;
  dcterms:provenance "ISO/TS 19130-2:2014, 4.17" ;
  dcterms:source "IHO Hydrographic Dictionary, S-32, Fifth Edition" ;
  reg:status reg:statusValid ;
  rdfs:label "draught"@en ;
  skos:changeNote "valid" ;
  skos:editorialNote "preferred"^^xsd:string ;
  skos:notation 1386 ;
  skos:prefLabel "draught"@en ;
.
<http://iso.org/tc211/term/1388>
  rdf:type skos:Concept ;
  dcterms:dateAccepted "2014-01-15"^^xsd:date ;
  dcterms:provenance "ISO/TS 19130-2:2014, 4.20" ;
  dcterms:source "Manual of Photogrammetry" ;
  reg:status reg:statusValid ;
  rdfs:comment "Note 1 to entry:  In the airborne case, this would be swath width for a linear array, ground footprint for an area array, and for a whiskbroom scanner it refers to the swath width."@en ;
  rdfs:label "field of view"@en ;
  skos:altLabel "FOV"^^<http://www.w3.org/2001/XMLSchema#@en> ;
  skos:changeNote "valid" ;
  skos:editorialNote "preferred"^^xsd:string ;
  skos:notation 1388 ;
  skos:note "Note 1 to entry:  In the airborne case, this would be swath width for a linear array, ground footprint for an area array, and for a whiskbroom scanner it refers to the swath width."@en ;
  skos:prefLabel "field of view"@en ;
.
<http://iso.org/tc211/term/1389>
  rdf:type skos:Concept ;
  dcterms:dateAccepted "2014-01-15"^^xsd:date ;
  dcterms:provenance "ISO/TS 19130-2:2014, 4.21" ;
  dcterms:source "Adapted from STM E2544" ;
  reg:status reg:statusValid ;
  rdfs:label "first return"@en ;
  skos:changeNote "valid" ;
  skos:editorialNote "preferred"^^xsd:string ;
  skos:notation 1389 ;
  skos:prefLabel "first return"@en ;
.
<http://iso.org/tc211/term/139>
  rdf:type skos:Concept ;
  dcterms:dateAccepted "2003-05-01"^^xsd:date ;
  dcterms:dateAccepted "2009-12-29"^^xsd:date ;
  dcterms:provenance "KS X ISO 19107" ;
  dcterms:source "ISO 19107:2003" ;
  reg:status reg:statusValid ;
  rdfs:comment "Note 1 to entry: Directed solids are used in the coboundary relation to maintain the spatial association between face and topological solid. The orientation of a solid is with respect to a face, \"+\" if the upNormal is outward, \"-\" if inward. This is consistent with the concept of \"up = outward\" for a surface bounding a solid."@en ;
  rdfs:comment "비고: 방향성 입방체는 면과 위상 입방체 간의 공간적인 관계를 유지하기 위해 공유 경계 측면에서 사용된다. 입방체의 방향성은 변을 따르며, \"+\"는 법선 벡터가 바깥쪽인 경우, \"-\"는 안쪽일 경우에 부여된다. 이것은 입방체를 감싸는 표면에서 \"위쪽 = 바깥쪽\" 이라는 개념과도 일치한다. "@kr ;
  rdfs:label "directed solid"@en ;
  skos:changeNote "valid" ;
  skos:definition "하나의 위상 입방체와 그 입방체가 갖는 방향성 간의 연관으로 표현된 방향성 위상 객체"@kr ;
  skos:editorialNote "preferred" ;
  skos:editorialNote "preferred"^^xsd:string ;
  skos:notation "139" ;
  skos:notation 139 ;
  skos:note "Note 1 to entry: Directed solids are used in the coboundary relation to maintain the spatial association between face and topological solid. The orientation of a solid is with respect to a face, \"+\" if the upNormal is outward, \"-\" if inward. This is consistent with the concept of \"up = outward\" for a surface bounding a solid."@en ;
  skos:note "비고: 방향성 입방체는 면과 위상 입방체 간의 공간적인 관계를 유지하기 위해 공유 경계 측면에서 사용된다. 입방체의 방향성은 변을 따르며, \"+\"는 법선 벡터가 바깥쪽인 경우, \"-\"는 안쪽일 경우에 부여된다. 이것은 입방체를 감싸는 표면에서 \"위쪽 = 바깥쪽\" 이라는 개념과도 일치한다. "@kr ;
  skos:prefLabel "directed solid"@en ;
  skos:prefLabel "방향성 입방체"@kr ;
.
<http://iso.org/tc211/term/1390>
  rdf:type skos:Concept ;
  dcterms:dateAccepted "2014-01-15"^^xsd:date ;
  dcterms:provenance "ISO/TS 19130-2:2014, 4.22" ;
  dcterms:source "Adapted from NISTIR 7117" ;
  reg:status reg:statusValid ;
  rdfs:comment "Note 1 to entry:  A complete 3D data sample of the world produced by a LIDAR taken at a certain time, place, and orientation. A single LIDAR frame is also referred to as a range image."@en ;
  rdfs:label "frame<LIDAR>"@en ;
  skos:changeNote "valid" ;
  skos:editorialNote "preferred"^^xsd:string ;
  skos:notation 1390 ;
  skos:note "Note 1 to entry:  A complete 3D data sample of the world produced by a LIDAR taken at a certain time, place, and orientation. A single LIDAR frame is also referred to as a range image."@en ;
  skos:prefLabel "frame<LIDAR>"@en ;
.
<http://iso.org/tc211/term/1391>
  rdf:type skos:Concept ;
  dcterms:dateAccepted "2014-01-15"^^xsd:date ;
  dcterms:provenance "ISO/TS 19130-2:2014, 4.23" ;
  dcterms:source "Adapted from Albota 2002" ;
  reg:status reg:statusValid ;
  rdfs:comment "Note 1 to entry:  These detectors exist in the form of arrays and are bonded with electronic circuitry.  The electronic circuitry produces a measurement corresponding to the time at which the current was generated; resulting in a direct time-of-flight measurement.  A LIDAR that employs this detector technology typically illuminates a large scene with a single pulse.  The direct time-of-flight measurements are then combined with platform location/attitude data along with pointing information to produce a three-dimensional product of the illuminated scene of interest.  Additional processing is applied which removes existing noise present in the data to produce a visually exploitable data set."@en ;
  rdfs:label "geiger mode"@en ;
  skos:changeNote "valid" ;
  skos:editorialNote "preferred"^^xsd:string ;
  skos:notation 1391 ;
  skos:note "Note 1 to entry:  These detectors exist in the form of arrays and are bonded with electronic circuitry.  The electronic circuitry produces a measurement corresponding to the time at which the current was generated; resulting in a direct time-of-flight measurement.  A LIDAR that employs this detector technology typically illuminates a large scene with a single pulse.  The direct time-of-flight measurements are then combined with platform location/attitude data along with pointing information to produce a three-dimensional product of the illuminated scene of interest.  Additional processing is applied which removes existing noise present in the data to produce a visually exploitable data set."@en ;
  skos:prefLabel "geiger mode"@en ;
.
<http://iso.org/tc211/term/1392>
  rdf:type skos:Concept ;
  dcterms:dateAccepted "2014-01-15"^^xsd:date ;
  dcterms:source "ISO/TS 19130-2:2014, 4.30" ;
  reg:status reg:statusValid ;
  rdfs:label "hydrophone<SONAR>"@en ;
  skos:changeNote "valid" ;
  skos:editorialNote "preferred"^^xsd:string ;
  skos:notation 1392 ;
  skos:prefLabel "hydrophone<SONAR>"@en ;
.
<http://iso.org/tc211/term/1393>
  rdf:type skos:Concept ;
  dcterms:dateAccepted "2014-01-15"^^xsd:date ;
  dcterms:provenance "ISO/TS 19130-2:2014, 4.31" ;
  dcterms:source "IHO Hydrographic Dictionary S-32, Fifth Edition" ;
  reg:status reg:statusValid ;
  rdfs:label "heave"@en ;
  skos:changeNote "valid" ;
  skos:editorialNote "preferred"^^xsd:string ;
  skos:notation 1393 ;
  skos:prefLabel "heave"@en ;
.
<http://iso.org/tc211/term/1394>
  rdf:type skos:Concept ;
  dcterms:dateAccepted "2014-01-15"^^xsd:date ;
  dcterms:provenance "ISO/TS 19130-2:2014, 4.32" ;
  dcterms:source "IHO Hydrographic Dictionary S-32, Fifth Edition" ;
  reg:status reg:statusValid ;
  rdfs:label "hydrographic swath<SONAR>"@en ;
  skos:changeNote "valid" ;
  skos:editorialNote "preferred"^^xsd:string ;
  skos:notation 1394 ;
  skos:prefLabel "hydrographic swath<SONAR>"@en ;
.
<http://iso.org/tc211/term/1395>
  rdf:type skos:Concept ;
  dcterms:dateAccepted "2014-01-15"^^xsd:date ;
  dcterms:source "ISO/TS 19130-2:2014, 4.33" ;
  reg:status reg:statusValid ;
  rdfs:comment "Note 1 to entry:  The image coordinates can be in pixels or in a measure of length (linear measure)."@en ;
  rdfs:label "image coordinates"@en ;
  skos:changeNote "valid" ;
  skos:editorialNote "preferred"^^xsd:string ;
  skos:notation 1395 ;
  skos:note "Note 1 to entry:  The image coordinates can be in pixels or in a measure of length (linear measure)."@en ;
  skos:prefLabel "image coordinates"@en ;
.
<http://iso.org/tc211/term/1396>
  rdf:type skos:Concept ;
  dcterms:dateAccepted "2014-01-15"^^xsd:date ;
  dcterms:provenance "ISO/TS 19130-2:2014, 4.36" ;
  dcterms:source "Manual of Photogrammetry" ;
  reg:status reg:statusValid ;
  rdfs:label "instantaneous field of view"@en ;
  skos:changeNote "valid" ;
  skos:editorialNote "preferred"^^xsd:string ;
  skos:notation 1396 ;
  skos:prefLabel "instantaneous field of view"@en ;
.
<http://iso.org/tc211/term/1397>
  rdf:type skos:Concept ;
  dcterms:dateAccepted "2014-01-15"^^xsd:date ;
  dcterms:source "ISO/TS 19130-2:2014, 4.37" ;
  reg:status reg:statusValid ;
  rdfs:comment "Note 1 to entry:  Typically for LIDAR, sufficient calibration has not been done to calculate absolute intensity, so relative intensity is usually reported.  In linear mode systems, this value is typically provided as an integer, resulting from a mapping of the return’s signal power to an integer value via a lookup table."@en ;
  rdfs:label "intensity"@en ;
  skos:changeNote "valid" ;
  skos:editorialNote "preferred"^^xsd:string ;
  skos:notation 1397 ;
  skos:note "Note 1 to entry:  Typically for LIDAR, sufficient calibration has not been done to calculate absolute intensity, so relative intensity is usually reported.  In linear mode systems, this value is typically provided as an integer, resulting from a mapping of the return’s signal power to an integer value via a lookup table."@en ;
  skos:prefLabel "intensity"@en ;
.
<http://iso.org/tc211/term/1399>
  rdf:type skos:Concept ;
  dcterms:dateAccepted "2014-01-15"^^xsd:date ;
  dcterms:provenance "ISO/TS 19130-2:2014, 4.38" ;
  dcterms:source "Adapted from ASTM E2544" ;
  reg:status reg:statusValid ;
  rdfs:label "last return"@en ;
  skos:changeNote "valid" ;
  skos:editorialNote "preferred"^^xsd:string ;
  skos:notation 1399 ;
  skos:prefLabel "last return"@en ;
.
<http://iso.org/tc211/term/14>
  rdf:type skos:Concept ;
  dcterms:dateAccepted "2002-07-01"^^xsd:date ;
  dcterms:dateAccepted "2008-12-30"^^xsd:date ;
  dcterms:provenance "ISO 19101:2002" ;
  dcterms:source "ISO 19101-1:2014, 4.1.1" ;
  reg:status reg:statusValid ;
  rdfs:label "application"@en ;
  skos:changeNote "valid" ;
  skos:definition "사용자 요구 사항의 지원을 위한 데이터의 조작 및 처리"@kr ;
  skos:editorialNote "preferred" ;
  skos:editorialNote "preferred"^^xsd:string ;
  skos:notation "14" ;
  skos:notation 14 ;
  skos:prefLabel "application"@en ;
  skos:prefLabel "응용"@kr ;
.
<http://iso.org/tc211/term/140>
  rdf:type skos:Concept ;
  dcterms:dateAccepted "2003-05-01"^^xsd:date ;
  dcterms:dateAccepted "2009-12-29"^^xsd:date ;
  dcterms:provenance "KS X ISO 19107" ;
  dcterms:source "ISO 19107:2003" ;
  reg:status reg:statusValid ;
  rdfs:label "directed topological object"@en ;
  skos:changeNote "valid" ;
  skos:definition "하나의 위상 원시 객체와 그 위상 원시 객체가 갖는 방향성 간의 연관으로 표현된 위상객체"@kr ;
  skos:editorialNote "preferred" ;
  skos:editorialNote "preferred"^^xsd:string ;
  skos:notation "140" ;
  skos:notation 140 ;
  skos:prefLabel "directed topological object"@en ;
  skos:prefLabel "방향성 위상 객체"@kr ;
.
<http://iso.org/tc211/term/1400>
  rdf:type skos:Concept ;
  dcterms:dateAccepted "2014-01-15"^^xsd:date ;
  dcterms:source "ISO/TS 19130-2:2014, 4.40" ;
  reg:status reg:statusValid ;
  rdfs:comment "Note 1 to entry:  Time of flight (TOF) LIDARs use short laser pulses and precisely record the time each laser pulse was emitted and the time each reflected return(s) is received in order to calculate the distance(s) to the scatterer(s) encountered by the emitted pulse. For topographic LIDAR, these time-of-flight measurements are then combined with precise platform location/attitude data along with pointing data to produce a three-dimensional product of the illuminated scene of interest."@en ;
  rdfs:label "light detection and ranging"@en ;
  rdfs:seeAlso "LIDAR" ;
  skos:altLabel "LIDAR"@en ;
  skos:altLabel "LIDAR"^^<http://www.w3.org/2001/XMLSchema#@en> ;
  skos:changeNote "valid" ;
  skos:editorialNote "preferred"^^xsd:string ;
  skos:notation 1400 ;
  skos:note "Note 1 to entry:  Time of flight (TOF) LIDARs use short laser pulses and precisely record the time each laser pulse was emitted and the time each reflected return(s) is received in order to calculate the distance(s) to the scatterer(s) encountered by the emitted pulse. For topographic LIDAR, these time-of-flight measurements are then combined with precise platform location/attitude data along with pointing data to produce a three-dimensional product of the illuminated scene of interest."@en ;
  skos:prefLabel "light detection and ranging"@en ;
.
<http://iso.org/tc211/term/1401>
  rdf:type skos:Concept ;
  dcterms:dateAccepted "2014-01-15"^^xsd:date ;
  dcterms:provenance "ISO/TS 19130-2:2014, 4.41" ;
  dcterms:source "Adapted from Aull et al., 2002" ;
  reg:status reg:statusValid ;
  rdfs:comment "Note 1 to entry:  A LIDAR system which employs this technology typically uses processing techniques to develop the time-of-flight measurements from the full waveform that is reflected from the targets in the illuminated scene of interest. These time-of-flight measurements are then combined with precise platform location/attitude data along with pointing data to produce a three-dimensional product of the illuminated scene of interest."@en ;
  rdfs:label "linear mode"@en ;
  skos:changeNote "valid" ;
  skos:editorialNote "preferred"^^xsd:string ;
  skos:notation 1401 ;
  skos:note "Note 1 to entry:  A LIDAR system which employs this technology typically uses processing techniques to develop the time-of-flight measurements from the full waveform that is reflected from the targets in the illuminated scene of interest. These time-of-flight measurements are then combined with precise platform location/attitude data along with pointing data to produce a three-dimensional product of the illuminated scene of interest."@en ;
  skos:prefLabel "linear mode"@en ;
.
<http://iso.org/tc211/term/1402>
  rdf:type skos:Concept ;
  dcterms:dateAccepted "2014-01-15"^^xsd:date ;
  dcterms:source "ISO/TS 19130-2:2014, 4.42" ;
  reg:status reg:statusValid ;
  rdfs:comment "Note 1 to entry:  It is approximately the complement of the depression angle."@en ;
  rdfs:label "look angle"@en ;
  skos:changeNote "valid" ;
  skos:editorialNote "preferred"^^xsd:string ;
  skos:notation 1402 ;
  skos:note "Note 1 to entry:  It is approximately the complement of the depression angle."@en ;
  skos:prefLabel "look angle"@en ;
.
<http://iso.org/tc211/term/1405>
  rdf:type skos:Concept ;
  dcterms:dateAccepted "2014-01-15"^^xsd:date ;
  dcterms:source "ISO/TS 19130-2:2014, 4.47" ;
  reg:status reg:statusValid ;
  rdfs:label "passive SONAR"@en ;
  skos:changeNote "valid" ;
  skos:editorialNote "preferred"^^xsd:string ;
  skos:notation 1405 ;
  skos:prefLabel "passive SONAR"@en ;
.
<http://iso.org/tc211/term/1406>
  rdf:type skos:Concept ;
  dcterms:dateAccepted "2014-01-15"^^xsd:date ;
  dcterms:source "ISO/TS 19130-2:2014, 4.48" ;
  reg:status reg:statusValid ;
  rdfs:comment "Note 1 to entry:  Usually stored as a series of range lines, each containing information from a specific range bin.  PHD can be thought of as a table of five columns:  In-phase signal, Quadrature signal, Range, Doppler Angle, and Time."@en ;
  rdfs:label "phase history data"@en ;
  rdfs:seeAlso "video phase history data" ;
  skos:altLabel "PHD"^^<http://www.w3.org/2001/XMLSchema#@en> ;
  skos:altLabel "video phase history data"@en ;
  skos:changeNote "valid" ;
  skos:editorialNote "preferred"^^xsd:string ;
  skos:notation 1406 ;
  skos:note "Note 1 to entry:  Usually stored as a series of range lines, each containing information from a specific range bin.  PHD can be thought of as a table of five columns:  In-phase signal, Quadrature signal, Range, Doppler Angle, and Time."@en ;
  skos:prefLabel "phase history data"@en ;
.
<http://iso.org/tc211/term/1407>
  rdf:type skos:Concept ;
  dcterms:dateAccepted "2014-01-15"^^xsd:date ;
  dcterms:source "ISO/TS 19130-2:2014, 4.50" ;
  reg:status reg:statusValid ;
  rdfs:label "platform down direction"@en ;
  skos:changeNote "valid" ;
  skos:editorialNote "preferred"^^xsd:string ;
  skos:notation 1407 ;
  skos:prefLabel "platform down direction"@en ;
.
<http://iso.org/tc211/term/1408>
  rdf:type skos:Concept ;
  dcterms:dateAccepted "2014-01-15"^^xsd:date ;
  dcterms:source "ISO/TS 19130-2:2014, 4.51" ;
  reg:status reg:statusValid ;
  rdfs:comment "Note 1 to entry:  The distance between points is generally non-uniform and hence all three coordinates (Cartesian or spherical) for each point must be specifically encoded."@en ;
  rdfs:label "point cloud"@en ;
  skos:changeNote "valid" ;
  skos:editorialNote "preferred"^^xsd:string ;
  skos:notation 1408 ;
  skos:note "Note 1 to entry:  The distance between points is generally non-uniform and hence all three coordinates (Cartesian or spherical) for each point must be specifically encoded."@en ;
  skos:prefLabel "point cloud"@en ;
.
<http://iso.org/tc211/term/141>
  rdf:type skos:Concept ;
  dcterms:dateAccepted "2005-08-15"^^xsd:date ;
  dcterms:dateAccepted "2007-11-01"^^xsd:date ;
  dcterms:provenance "KS X ISO 19123" ;
  dcterms:source "ISO 19123:2005" ;
  reg:status reg:statusValid ;
  rdfs:comment "Note 1 to entry: The domain of a discrete coverage consists of a finite set of spatial, temporal, or spatiotemporal objects."@en ;
  rdfs:comment "비고: 불연속 커버리지의 영역은 유한한 집합공간, 시간 또는 시공간 객체로 이루어진다. "@kr ;
  rdfs:label "discrete coverage"@en ;
  skos:changeNote "valid" ;
  skos:definition "동일한 피처(공간 객체, 시간 객체, 시공간 객체) 속성(B.175)의 값이 영역 내 모든 직접 위치에서 동일한 값을 갖는 커버리지"@kr ;
  skos:editorialNote "preferred" ;
  skos:editorialNote "preferred"^^xsd:string ;
  skos:notation "141" ;
  skos:notation 141 ;
  skos:note "Note 1 to entry: The domain of a discrete coverage consists of a finite set of spatial, temporal, or spatiotemporal objects."@en ;
  skos:note "비고: 불연속 커버리지의 영역은 유한한 집합공간, 시간 또는 시공간 객체로 이루어진다. "@kr ;
  skos:prefLabel "discrete coverage"@en ;
  skos:prefLabel "불연속 커버리지"@kr ;
.
<http://iso.org/tc211/term/1412>
  rdf:type skos:Concept ;
  dcterms:dateAccepted "2014-01-15"^^xsd:date ;
  dcterms:source "ISO/TS 19130-2:2014, 4.61" ;
  reg:status reg:statusValid ;
  rdfs:label "resolution (of imagery)"@en ;
  skos:changeNote "valid" ;
  skos:editorialNote "preferred"^^xsd:string ;
  skos:notation 1412 ;
  skos:prefLabel "resolution (of imagery)"@en ;
.
<http://iso.org/tc211/term/1413>
  rdf:type skos:Concept ;
  dcterms:dateAccepted "2014-01-15"^^xsd:date ;
  dcterms:source "ISO/TS 19130-2:2014, 4.62" ;
  reg:status reg:statusValid ;
  rdfs:comment "Note 1 to entry:  There may be multiple returns for a given emitted laser pulse."@en ;
  rdfs:label "return <LIDAR>"@en ;
  skos:changeNote "valid" ;
  skos:editorialNote "preferred"^^xsd:string ;
  skos:notation 1413 ;
  skos:note "Note 1 to entry:  There may be multiple returns for a given emitted laser pulse."@en ;
  skos:prefLabel "return <LIDAR>"@en ;
.
<http://iso.org/tc211/term/1414>
  rdf:type skos:Concept ;
  dcterms:dateAccepted "2014-01-15"^^xsd:date ;
  dcterms:source "ISO/TS 19130-2:2014, 4.63" ;
  reg:status reg:statusValid ;
  rdfs:label "scan"@en ;
  skos:changeNote "valid" ;
  skos:editorialNote "preferred"^^xsd:string ;
  skos:notation 1414 ;
  skos:prefLabel "scan"@en ;
.
<http://iso.org/tc211/term/1416>
  rdf:type skos:Concept ;
  dcterms:dateAccepted "2014-01-15"^^xsd:date ;
  dcterms:source "ISO/TS 19130-2:2014, 4.69" ;
  reg:status reg:statusValid ;
  rdfs:comment "Note 1 to entry:  Sidescan SONAR is used for imaging bottom features and targets in a wide variety of water depths."@en ;
  rdfs:comment "Note 2 to entry:  This includes synthetic aperture sidescan SONAR." ;
  rdfs:label "sidescan SONAR"@en ;
  skos:changeNote "valid" ;
  skos:editorialNote "preferred"^^xsd:string ;
  skos:notation 1416 ;
  skos:note "Note 1 to entry:  Sidescan SONAR is used for imaging bottom features and targets in a wide variety of water depths."@en ;
  skos:note "Note 2 to entry:  This includes synthetic aperture sidescan SONAR."^^<http://www.w3.org/2001/XMLSchema#@en> ;
  skos:prefLabel "sidescan SONAR"@en ;
.
<http://iso.org/tc211/term/1417>
  rdf:type skos:Concept ;
  dcterms:dateAccepted "2014-01-15"^^xsd:date ;
  dcterms:source "ISO/TS 19130-2:2014, 4.70" ;
  reg:status reg:statusValid ;
  rdfs:comment "Note 1 to entry:  Single beam sonar is commonly called a single beam echosounder (abbr: SBES)."@en ;
  rdfs:label "single beam SONAR"@en ;
  skos:changeNote "valid" ;
  skos:editorialNote "preferred"^^xsd:string ;
  skos:notation 1417 ;
  skos:note "Note 1 to entry:  Single beam sonar is commonly called a single beam echosounder (abbr: SBES)."@en ;
  skos:prefLabel "single beam SONAR"@en ;
.
<http://iso.org/tc211/term/1419>
  rdf:type skos:Concept ;
  dcterms:dateAccepted "2014-01-15"^^xsd:date ;
  dcterms:source "ISO/TS 19130-2:2014, 4.71" ;
  reg:status reg:statusValid ;
  rdfs:label "SONAR processing system"@en ;
  skos:changeNote "valid" ;
  skos:editorialNote "preferred"^^xsd:string ;
  skos:notation 1419 ;
  skos:prefLabel "SONAR processing system"@en ;
.
<http://iso.org/tc211/term/1420>
  rdf:type skos:Concept ;
  dcterms:dateAccepted "2014-01-15"^^xsd:date ;
  dcterms:provenance "ISO/TS 19130-2:2014, 4.73" ;
  dcterms:source "Implementation Specification — a Draught Information System for the St. Lawrence Seaway, 4.18, modified — Note 2 to entry has been added." ;
  reg:status reg:statusValid ;
  rdfs:comment "Note 1 to entry:  The effect is a result of Bernoulli's principle of fluid dynamics. The squat represents the increase in effective draught."@en ;
  rdfs:comment "Note 2 to entry:  For a ship underway, the change of level of the bow and stern from the still water condition in response to the elevation and depression of the water level about the hull resulting from the bow and stern wave systems." ;
  rdfs:label "squat"@en ;
  skos:changeNote "valid" ;
  skos:editorialNote "preferred"^^xsd:string ;
  skos:notation 1420 ;
  skos:note "Note 1 to entry:  The effect is a result of Bernoulli's principle of fluid dynamics. The squat represents the increase in effective draught."@en ;
  skos:note "Note 2 to entry:  For a ship underway, the change of level of the bow and stern from the still water condition in response to the elevation and depression of the water level about the hull resulting from the bow and stern wave systems."^^<http://www.w3.org/2001/XMLSchema#@en> ;
  skos:prefLabel "squat"@en ;
.
<http://iso.org/tc211/term/1421>
  rdf:type skos:Concept ;
  dcterms:dateAccepted "2014-01-15"^^xsd:date ;
  dcterms:source "ISO/TS 19130-2:2014, 4.74" ;
  reg:status reg:statusValid ;
  rdfs:comment "Note 1 to entry:  This applies to a HARLIE transceiver, based on a volume phase holographic optical element."@en ;
  rdfs:label "stare"@en ;
  skos:changeNote "valid" ;
  skos:editorialNote "preferred"^^xsd:string ;
  skos:notation 1421 ;
  skos:note "Note 1 to entry:  This applies to a HARLIE transceiver, based on a volume phase holographic optical element."@en ;
  skos:prefLabel "stare"@en ;
.
<http://iso.org/tc211/term/1422>
  rdf:type skos:Concept ;
  dcterms:dateAccepted "2014-01-15"^^xsd:date ;
  dcterms:source "ISO/TS 19130-2:2014, 4.75" ;
  reg:status reg:statusValid ;
  rdfs:comment "Note 1 to entry:  A typical mapping mission may consist of multiple adjacent swaths, with some overlap, and the operator will turn off the laser while the aircraft is oriented for the next swath.  This term may also be referred to as a Pass."@en ;
  rdfs:label "swath <LIDAR>"@en ;
  skos:changeNote "valid" ;
  skos:editorialNote "preferred"^^xsd:string ;
  skos:notation 1422 ;
  skos:note "Note 1 to entry:  A typical mapping mission may consist of multiple adjacent swaths, with some overlap, and the operator will turn off the laser while the aircraft is oriented for the next swath.  This term may also be referred to as a Pass."@en ;
  skos:prefLabel "swath <LIDAR>"@en ;
.
<http://iso.org/tc211/term/1423>
  rdf:type skos:Concept ;
  dcterms:dateAccepted "2014-01-15"^^xsd:date ;
  dcterms:source "ISO/TS 19130-2:2014, 4.76" ;
  reg:status reg:statusValid ;
  rdfs:comment "Note 1 to entry:  Sweep sounding is commonly called multi-channel echosounding (MCES)."@en ;
  rdfs:label "sweep SONAR"@en ;
  skos:changeNote "valid" ;
  skos:editorialNote "preferred"^^xsd:string ;
  skos:notation 1423 ;
  skos:note "Note 1 to entry:  Sweep sounding is commonly called multi-channel echosounding (MCES)."@en ;
  skos:prefLabel "sweep SONAR"@en ;
.
<http://iso.org/tc211/term/1424>
  rdf:type skos:Concept ;
  dcterms:dateAccepted "2014-01-15"^^xsd:date ;
  dcterms:source "ISO/TS 19130-2:2014, 4.77" ;
  reg:status reg:statusValid ;
  rdfs:label "swipe"@en ;
  skos:changeNote "valid" ;
  skos:editorialNote "preferred"^^xsd:string ;
  skos:notation 1424 ;
  skos:prefLabel "swipe"@en ;
.
<http://iso.org/tc211/term/1425>
  rdf:type skos:Concept ;
  dcterms:dateAccepted "2014-01-15"^^xsd:date ;
  dcterms:source "ISO/TS 19130-2:2014, 4.78" ;
  reg:status reg:statusValid ;
  rdfs:label "transducer"@en ;
  skos:changeNote "valid" ;
  skos:editorialNote "preferred"^^xsd:string ;
  skos:notation 1425 ;
  skos:prefLabel "transducer"@en ;
.
<http://iso.org/tc211/term/1426>
  rdf:type skos:Concept ;
  dcterms:dateAccepted "2014-01-15"^^xsd:date ;
  dcterms:source "ISO/TS 19130-2:2014, 4.79" ;
  reg:status reg:statusValid ;
  rdfs:comment "Note 1 to entry:  Transmitter is also called projector in multibeam echosounding."@en ;
  rdfs:label "transmitter"@en ;
  skos:changeNote "valid" ;
  skos:editorialNote "preferred"^^xsd:string ;
  skos:notation 1426 ;
  skos:note "Note 1 to entry:  Transmitter is also called projector in multibeam echosounding."@en ;
  skos:prefLabel "transmitter"@en ;
.
<http://iso.org/tc211/term/1427>
  rdf:type skos:Concept ;
  dcterms:dateAccepted "2014-01-15"^^xsd:date ;
  dcterms:source "ISO/TS 19130-2:2014, 4.80" ;
  reg:status reg:statusValid ;
  rdfs:comment "Note 1 to entry:  Generally referring to an airborne LIDAR system"@en ;
  rdfs:label "topographic LIDAR"@en ;
  skos:changeNote "valid" ;
  skos:editorialNote "preferred"^^xsd:string ;
  skos:notation 1427 ;
  skos:note "Note 1 to entry:  Generally referring to an airborne LIDAR system"@en ;
  skos:prefLabel "topographic LIDAR"@en ;
.
<http://iso.org/tc211/term/1428>
  rdf:type skos:Concept ;
  dcterms:dateAccepted "2014-01-15"^^xsd:date ;
  dcterms:source "ISO/TS 19130-2:2014, 4.81" ;
  reg:status reg:statusValid ;
  rdfs:label "velocity vector <Radar>"@en ;
  skos:changeNote "valid" ;
  skos:editorialNote "preferred"^^xsd:string ;
  skos:notation 1428 ;
  skos:prefLabel "velocity vector <Radar>"@en ;
.
<http://iso.org/tc211/term/1429>
  rdf:type skos:Concept ;
  dcterms:dateAccepted "2014-01-15"^^xsd:date ;
  dcterms:source "ISO/TS 19130-2:2014, 4.48" ;
  reg:status reg:statusValid ;
  rdfs:comment "Note 1 to entry:  Usually stored as a series of range lines, each containing information from a specific range bin.  PHD can be thought of as a table of five columns:  In-phase signal, Quadrature signal, Range, Doppler Angle, and Time."@en ;
  rdfs:label "video phase history data"@en ;
  rdfs:seeAlso "phase history data" ;
  skos:altLabel "phase history data"@en ;
  skos:changeNote "valid" ;
  skos:editorialNote "admitted"^^xsd:string ;
  skos:notation 1429 ;
  skos:note "Note 1 to entry:  Usually stored as a series of range lines, each containing information from a specific range bin.  PHD can be thought of as a table of five columns:  In-phase signal, Quadrature signal, Range, Doppler Angle, and Time."@en ;
  skos:prefLabel "video phase history data"@en ;
.
<http://iso.org/tc211/term/143>
  rdf:type skos:Concept ;
  dcterms:dateAccepted "2005-02-15"^^xsd:date ;
  dcterms:dateAccepted "2006-12-29"^^xsd:date ;
  dcterms:provenance "ISO 19119:2005" ;
  dcterms:provenance "KS X ISO/IEC 10746-2" ;
  dcterms:source "ISO/IEC 10746-2" ;
  reg:status reg:statusValid ;
  rdfs:comment "Note 1 to entry: Distribution transparencies enable complexities associated with system distribution to be hidden from applications where they are irrelevant to their purpose."@en ;
  rdfs:label "distribution transparency"@en ;
  skos:changeNote "valid" ;
  skos:definition "분산 시스템 일부의 잠재적 행태를 특정 사용자에게 숨기는 특성"@kr ;
  skos:editorialNote "preferred" ;
  skos:editorialNote "preferred"^^xsd:string ;
  skos:notation "143" ;
  skos:notation 143 ;
  skos:note "Note 1 to entry: Distribution transparencies enable complexities associated with system distribution to be hidden from applications where they are irrelevant to their purpose."@en ;
  skos:prefLabel "distribution transparency"@en ;
  skos:prefLabel "분산 투명성"@kr ;
.
<http://iso.org/tc211/term/1430>
  rdf:type skos:Concept ;
  dcterms:dateAccepted "2014-11-01"^^xsd:date ;
  dcterms:source "ISO 19101-1:2014, 4.1.10" ;
  reg:status reg:statusValid ;
  rdfs:label "e-government"@en ;
  skos:changeNote "valid" ;
  skos:editorialNote "preferred"^^xsd:string ;
  skos:notation 1430 ;
  skos:prefLabel "e-government"@en ;
.
<http://iso.org/tc211/term/1431>
  rdf:type skos:Concept ;
  dcterms:dateAccepted "2013-12-15"^^xsd:date ;
  dcterms:provenance "ISO 19157:2013" ;
  dcterms:source "ISO 19101-1:2014, 4.1.14" ;
  reg:status reg:statusValid ;
  rdfs:label "feature instance"@en ;
  skos:changeNote "valid" ;
  skos:editorialNote "preferred"^^xsd:string ;
  skos:notation 1431 ;
  skos:prefLabel "feature instance"@en ;
.
<http://iso.org/tc211/term/1432>
  rdf:type skos:Concept ;
  dcterms:dateAccepted "2014-11-01"^^xsd:date ;
  dcterms:provenance "ISO 19101-1:2014, 4.1.31" ;
  dcterms:source "ISO 14721:2012, 1.7.2, modified" ;
  reg:status reg:statusValid ;
  rdfs:comment "Note 1 to entry:  A reference model is based on a small number of unifying concepts and can be used as a basis for education and explaining standards to a non-specialist."@en ;
  rdfs:label "reference model"@en ;
  skos:changeNote "valid" ;
  skos:editorialNote "preferred"^^xsd:string ;
  skos:notation 1432 ;
  skos:note "Note 1 to entry:  A reference model is based on a small number of unifying concepts and can be used as a basis for education and explaining standards to a non-specialist."@en ;
  skos:prefLabel "reference model"@en ;
.
<http://iso.org/tc211/term/1433>
  rdf:type skos:Concept ;
  dcterms:dateAccepted "2014-11-01"^^xsd:date ;
  dcterms:source "ISO 19101-1:2014, 4.1.40" ;
  reg:status reg:statusValid ;
  rdfs:label "Web"@en ;
  rdfs:seeAlso "World Wide Web" ;
  skos:altLabel "World Wide Web"@en ;
  skos:changeNote "valid" ;
  skos:editorialNote "admitted"^^xsd:string ;
  skos:notation 1433 ;
  skos:prefLabel "Web"@en ;
.
<http://iso.org/tc211/term/1434>
  rdf:type skos:Concept ;
  dcterms:dateAccepted "2012-11-15"^^xsd:date ;
  dcterms:provenance "ISO/TS 19150-1:2012" ;
  dcterms:source "ISO 19101-1:2014, 4.1.41" ;
  reg:status reg:statusValid ;
  rdfs:comment "Note 1 to entry:  A Web service usually includes some combination of programming and data. It can also include human resources."@en ;
  rdfs:label "Web service"@en ;
  skos:changeNote "valid" ;
  skos:editorialNote "preferred"^^xsd:string ;
  skos:notation 1434 ;
  skos:note "Note 1 to entry:  A Web service usually includes some combination of programming and data. It can also include human resources."@en ;
  skos:prefLabel "Web service"@en ;
.
<http://iso.org/tc211/term/1435>
  rdf:type skos:Concept ;
  dcterms:dateAccepted "2014-11-01"^^xsd:date ;
  dcterms:source "ISO 19101-1:2014, 4.1.40" ;
  reg:status reg:statusValid ;
  rdfs:label "World Wide Web"@en ;
  rdfs:seeAlso "Web" ;
  skos:altLabel "Web"@en ;
  skos:changeNote "valid" ;
  skos:editorialNote "preferred"^^xsd:string ;
  skos:notation 1435 ;
  skos:prefLabel "World Wide Web"@en ;
.
<http://iso.org/tc211/term/1439>
  rdf:type skos:Concept ;
  dcterms:dateAccepted "2014-04-01"^^xsd:date ;
  dcterms:provenance "ISO 19115-1:2014, 4.16" ;
  dcterms:source "ISO 5127:2001, 4.1.1.10" ;
  reg:status reg:statusValid ;
  rdfs:label "provenance"@en ;
  skos:changeNote "valid" ;
  skos:editorialNote "preferred"^^xsd:string ;
  skos:notation 1439 ;
  skos:prefLabel "provenance"@en ;
.
<http://iso.org/tc211/term/144>
  rdf:type skos:Concept ;
  dcterms:dateAccepted "2003-05-01" ;
  dcterms:dateAccepted "2003-05-01"^^xsd:date ;
  dcterms:dateAccepted "2009-12-29"^^xsd:date ;
  dcterms:provenance "KS X ISO 19103" ;
  dcterms:source "ISO/TS 19103:2005" ;
  reg:status reg:statusAccepted ;
  reg:status reg:statusValid ;
  rdfs:comment "NOTE Domains are used to define the domain set and range set of attributes, operators and functions."@en ;
  rdfs:comment "Note 1 to entry: Domains are used to define the domain set and range set of attributes, operators and functions."@en ;
  rdfs:comment "비고: 영역은 속성, 연산자, 함수에 대한 영역 및 범위를 정의하는 데 사용된다. "@kr ;
  rdfs:label "domain"@en ;
  skos:changeNote "valid" ;
  skos:definition "gedefinieerde set"@nl ;
  skos:definition "잘 정의된 값들의 집합"@kr ;
  skos:editorialNote "preferred" ;
  skos:editorialNote "preferred"^^xsd:string ;
  skos:notation "144" ;
  skos:notation 144 ;
  skos:note "NOTE Domains are used to define the domain set and range set of attributes, operators and functions."@en ;
  skos:note "Note 1 to entry: Domains are used to define the domain set and range set of attributes, operators and functions."@en ;
  skos:note "비고: 영역은 속성, 연산자, 함수에 대한 영역 및 범위를 정의하는 데 사용된다. "@kr ;
  skos:prefLabel "domain"@en ;
  skos:prefLabel "domein"@nl ;
  skos:prefLabel "영역"@kr ;
.
<http://iso.org/tc211/term/1440>
  rdf:type skos:Concept ;
  dcterms:dateAccepted "2012-07-01"^^xsd:date ;
  dcterms:source "ISO 19144-2:2012, 4.1.12" ;
  reg:status reg:statusValid ;
  rdfs:label "physiognomy"@en ;
  skos:changeNote "valid" ;
  skos:editorialNote "preferred"^^xsd:string ;
  skos:notation 1440 ;
  skos:prefLabel "physiognomy"@en ;
.
<http://iso.org/tc211/term/1441>
  rdf:type skos:Concept ;
  dcterms:dateAccepted "2011-12-15"^^xsd:date ;
  dcterms:source "ISO 19156:2011, 4.5" ;
  reg:status reg:statusValid ;
  rdfs:comment "Note 1 to entry: Opposite of in-situ."@en ;
  rdfs:label "ex-situ"@en ;
  skos:changeNote "valid" ;
  skos:editorialNote "preferred"^^xsd:string ;
  skos:notation 1441 ;
  skos:note "Note 1 to entry: Opposite of in-situ."@en ;
  skos:prefLabel "ex-situ"@en ;
.
<http://iso.org/tc211/term/1442>
  rdf:type skos:Concept ;
  dcterms:dateAccepted "2011-12-15"^^xsd:date ;
  dcterms:source "ISO 19156:2011, 4.11" ;
  reg:status reg:statusValid ;
  rdfs:label "observation"@en ;
  skos:changeNote "valid" ;
  skos:editorialNote "preferred"^^xsd:string ;
  skos:notation 1442 ;
  skos:prefLabel "observation"@en ;
.
<http://iso.org/tc211/term/1443>
  rdf:type skos:Concept ;
  dcterms:dateAccepted "2011-12-15"^^xsd:date ;
  dcterms:source "ISO 19156:2011, 4.17" ;
  reg:status reg:statusValid ;
  rdfs:comment "Note 1 to entry: A sampling feature is an artefact of the observational strategy, and has no significance independent of the observational campaign."@en ;
  rdfs:label "sampling feature"@en ;
  skos:changeNote "valid" ;
  skos:editorialNote "preferred"^^xsd:string ;
  skos:notation 1443 ;
  skos:note "Note 1 to entry: A sampling feature is an artefact of the observational strategy, and has no significance independent of the observational campaign."@en ;
  skos:prefLabel "sampling feature"@en ;
.
<http://iso.org/tc211/term/1448>
  rdf:type skos:Concept ;
  dcterms:dateAccepted "2014-07-15"^^xsd:date ;
  dcterms:provenance "ISO/TS 19159-1:2014, 4.3" ;
  dcterms:source "ISO/IEC Guide 99:2007, 4.31" ;
  reg:status reg:statusValid ;
  rdfs:comment "Note 1 to entry:  A calibration curve expresses a one-to-one relation that does not supply a measurement result as it bears no information about the measurement uncertainty."@en ;
  rdfs:label "calibration curve"@en ;
  skos:changeNote "valid" ;
  skos:editorialNote "preferred"^^xsd:string ;
  skos:notation 1448 ;
  skos:note "Note 1 to entry:  A calibration curve expresses a one-to-one relation that does not supply a measurement result as it bears no information about the measurement uncertainty."@en ;
  skos:prefLabel "calibration curve"@en ;
.
<http://iso.org/tc211/term/1449>
  rdf:type skos:Concept ;
  dcterms:dateAccepted "2014-07-15"^^xsd:date ;
  dcterms:provenance "ISO/TS 19159-1:2014, 4.5" ;
  dcterms:source "ISO/IEC Guide 99:2007, 2.53" ;
  reg:status reg:statusValid ;
  rdfs:comment "Note 1 to entry:  See ISO/IEC Guide 98-3:2008, 3.2.3, for an explanation of \"systematic effect\"."@en ;
  rdfs:comment "Note 2 to entry:  The compensation can take different forms, such as an addend or a factor, or can be deduced from a table." ;
  rdfs:label "correction"@en ;
  skos:changeNote "valid" ;
  skos:editorialNote "preferred"^^xsd:string ;
  skos:notation 1449 ;
  skos:note "Note 1 to entry:  See ISO/IEC Guide 98-3:2008, 3.2.3, for an explanation of \"systematic effect\"."@en ;
  skos:note "Note 2 to entry:  The compensation can take different forms, such as an addend or a factor, or can be deduced from a table."^^<http://www.w3.org/2001/XMLSchema#@en> ;
  skos:prefLabel "correction"@en ;
.
<http://iso.org/tc211/term/145>
  rdf:type skos:Concept ;
  dcterms:dateAccepted "2003-02-15" ;
  dcterms:dateAccepted "2003-02-15"^^xsd:date ;
  dcterms:dateAccepted "2007-11-01"^^xsd:date ;
  dcterms:provenance "ISO 19111:2003" ;
  dcterms:provenance "KS X ISO 19111" ;
  dcterms:source "ISO 19111:2007" ;
  reg:status reg:statusAccepted ;
  reg:status reg:statusValid ;
  rdfs:comment "OPMERKING Soms wordt ook de afkorting vertaald: O"@nl ;
  rdfs:label "easting"@en ;
  rdfs:seeAlso "easting"@nl ;
  skos:altLabel "E"@kr ;
  skos:altLabel "E"@nl ;
  skos:altLabel "E"^^<http://www.w3.org/2001/XMLSchema#@en> ;
  skos:altLabel "easting"@nl ;
  skos:changeNote "valid" ;
  skos:definition "afstand in een coördinaatsysteem, oostwaarts (positief) of westwaarts (negatief) vanaf een noord-zuid georiënteerde referentielijn"@nl ;
  skos:definition "남북 방향의 기준선으로부터 동쪽(양수) 혹은 서쪽(음수)으로 표시하는 좌표 체계상의 동쪽방향 거리"@kr ;
  skos:editorialNote "preferred" ;
  skos:editorialNote "preferred"^^xsd:string ;
  skos:notation "145" ;
  skos:notation 145 ;
  skos:note "OPMERKING Soms wordt ook de afkorting vertaald: O"@nl ;
  skos:prefLabel "Oost"@nl ;
  skos:prefLabel "easting"@en ;
  skos:prefLabel "동향 거리"@kr ;
.
<http://iso.org/tc211/term/1450>
  rdf:type skos:Concept ;
  dcterms:dateAccepted "2014-07-15"^^xsd:date ;
  dcterms:source "ISO/TS 19159-1:2014, 4.6" ;
  reg:status reg:statusValid ;
  rdfs:comment "Note 1 to entry:  For calibration of optical sensors dark current is measured by the absence of incident optical radiation."@en ;
  rdfs:label "dark current"@en ;
  skos:changeNote "valid" ;
  skos:editorialNote "preferred"^^xsd:string ;
  skos:notation 1450 ;
  skos:note "Note 1 to entry:  For calibration of optical sensors dark current is measured by the absence of incident optical radiation."@en ;
  skos:prefLabel "dark current"@en ;
.
<http://iso.org/tc211/term/1451>
  rdf:type skos:Concept ;
  dcterms:dateAccepted "2014-07-15"^^xsd:date ;
  dcterms:source "ISO/TS 19159-1:2014, 4.7" ;
  reg:status reg:statusValid ;
  rdfs:label "dark current noise"@en ;
  skos:changeNote "valid" ;
  skos:editorialNote "preferred"^^xsd:string ;
  skos:notation 1451 ;
  skos:prefLabel "dark current noise"@en ;
.
<http://iso.org/tc211/term/1452>
  rdf:type skos:Concept ;
  dcterms:dateAccepted "2014-07-15"^^xsd:date ;
  dcterms:source "ISO/TS 19159-1:2014, 4.8" ;
  reg:status reg:statusValid ;
  rdfs:comment "Note 1 to entry:  This activation is mostly caused by imperfection of the detector."@en ;
  rdfs:label "dark signal non uniformity"@en ;
  skos:altLabel "DSNU"^^<http://www.w3.org/2001/XMLSchema#@en> ;
  skos:changeNote "valid" ;
  skos:editorialNote "preferred"^^xsd:string ;
  skos:notation 1452 ;
  skos:note "Note 1 to entry:  This activation is mostly caused by imperfection of the detector."@en ;
  skos:prefLabel "dark signal non uniformity"@en ;
.
<http://iso.org/tc211/term/1455>
  rdf:type skos:Concept ;
  dcterms:dateAccepted "2014-07-15"^^xsd:date ;
  dcterms:provenance "ISO/TS 19159-1:2014, 4.18" ;
  dcterms:source "ISO/IEC Guide 99:2007, 2.16" ;
  reg:status reg:statusValid ;
  rdfs:comment "Note 1 to entry:  The concept of \"measurement error\" can be used both a) when there is a single reference quantity value to refer to, which occurs if a calibration is made by means of a measurement standard with a measured quantity value having a negligible measurement uncertainty or if a conventional quantity value is given, in which case the measurement error is known, and b) if a measurand is supposed to be represented by a unique true quantity value or a set of true quantity values of negligible range, in which case the measurement error is not known."@en ;
  rdfs:comment "Note 2 to entry:  Measurement error should not be confused with production error or mistake." ;
  rdfs:label "error"@en ;
  rdfs:seeAlso "measurement error, error of measurement" ;
  skos:altLabel "measurement error, error of measurement"@en ;
  skos:changeNote "valid" ;
  skos:editorialNote "admitted"^^xsd:string ;
  skos:notation 1455 ;
  skos:note "Note 1 to entry:  The concept of \"measurement error\" can be used both a) when there is a single reference quantity value to refer to, which occurs if a calibration is made by means of a measurement standard with a measured quantity value having a negligible measurement uncertainty or if a conventional quantity value is given, in which case the measurement error is known, and b) if a measurand is supposed to be represented by a unique true quantity value or a set of true quantity values of negligible range, in which case the measurement error is not known."@en ;
  skos:note "Note 2 to entry:  Measurement error should not be confused with production error or mistake."^^<http://www.w3.org/2001/XMLSchema#@en> ;
  skos:prefLabel "error"@en ;
.
<http://iso.org/tc211/term/1456>
  rdf:type skos:Concept ;
  dcterms:dateAccepted "2014-07-15"^^xsd:date ;
  dcterms:provenance "ISO/TS 19159-1:2014, 4.18" ;
  dcterms:source "ISO/IEC Guide 99:2007, 2.16" ;
  reg:status reg:statusValid ;
  rdfs:comment "Note 1 to entry:  The concept of \"measurement error\" can be used both a) when there is a single reference quantity value to refer to, which occurs if a calibration is made by means of a measurement standard with a measured quantity value having a negligible measurement uncertainty or if a conventional quantity value is given, in which case the measurement error is known, and b) if a measurand is supposed to be represented by a unique true quantity value or a set of true quantity values of negligible range, in which case the measurement error is not known."@en ;
  rdfs:comment "Note 2 to entry:  Measurement error should not be confused with production error or mistake." ;
  rdfs:label "error of measurement"@en ;
  rdfs:seeAlso "measurement error, error" ;
  skos:altLabel "measurement error, error"@en ;
  skos:changeNote "valid" ;
  skos:editorialNote "admitted"^^xsd:string ;
  skos:notation 1456 ;
  skos:note "Note 1 to entry:  The concept of \"measurement error\" can be used both a) when there is a single reference quantity value to refer to, which occurs if a calibration is made by means of a measurement standard with a measured quantity value having a negligible measurement uncertainty or if a conventional quantity value is given, in which case the measurement error is known, and b) if a measurand is supposed to be represented by a unique true quantity value or a set of true quantity values of negligible range, in which case the measurement error is not known."@en ;
  skos:note "Note 2 to entry:  Measurement error should not be confused with production error or mistake."^^<http://www.w3.org/2001/XMLSchema#@en> ;
  skos:prefLabel "error of measurement"@en ;
.
<http://iso.org/tc211/term/1458>
  rdf:type skos:Concept ;
  dcterms:dateAccepted "2014-07-15"^^xsd:date ;
  dcterms:source "ISO/TS 19159-1:2014, 4.11" ;
  reg:status reg:statusValid ;
  rdfs:label "in situ measurement"@en ;
  skos:changeNote "valid" ;
  skos:editorialNote "preferred"^^xsd:string ;
  skos:notation 1458 ;
  skos:prefLabel "in situ measurement"@en ;
.
<http://iso.org/tc211/term/146>
  rdf:type skos:Concept ;
  dcterms:dateAccepted "2003-05-01"^^xsd:date ;
  dcterms:dateAccepted "2009-12-29"^^xsd:date ;
  dcterms:provenance "KS X ISO 19107" ;
  dcterms:source "ISO 19107:2003" ;
  reg:status reg:statusValid ;
  rdfs:comment "Note 1 to entry: The geometric realization of an edge is a curve. The boundary of an edge is the set of one or two nodes associated to the edge within a topological complex."@en ;
  rdfs:comment "비고: 변의 기하 실현은 곡선이다. 변의 경계는 위상 복합체 내에 존재하는 또 다른 변의 한 개 혹은 두 개의 절점 집합이다."@kr ;
  rdfs:label "edge"@en ;
  skos:changeNote "valid" ;
  skos:definition "1차원의 위상 원시 객체"@kr ;
  skos:editorialNote "preferred" ;
  skos:editorialNote "preferred"^^xsd:string ;
  skos:notation "146" ;
  skos:notation 146 ;
  skos:note "Note 1 to entry: The geometric realization of an edge is a curve. The boundary of an edge is the set of one or two nodes associated to the edge within a topological complex."@en ;
  skos:note "비고: 변의 기하 실현은 곡선이다. 변의 경계는 위상 복합체 내에 존재하는 또 다른 변의 한 개 혹은 두 개의 절점 집합이다."@kr ;
  skos:prefLabel "edge"@en ;
  skos:prefLabel "변"@kr ;
.
<http://iso.org/tc211/term/1460>
  rdf:type skos:Concept ;
  dcterms:dateAccepted "2014-07-15"^^xsd:date ;
  dcterms:source "ISO/TS 19159-1:2014, 4.13" ;
  reg:status reg:statusValid ;
  rdfs:comment "Note 1 to entry:  The SI unit is watts per square meter (W/m2)"@en ;
  rdfs:label "irradiance"@en ;
  skos:changeNote "valid" ;
  skos:editorialNote "preferred"^^xsd:string ;
  skos:notation 1460 ;
  skos:note "Note 1 to entry:  The SI unit is watts per square meter (W/m2)"@en ;
  skos:prefLabel "irradiance"@en ;
.
<http://iso.org/tc211/term/1461>
  rdf:type skos:Concept ;
  dcterms:dateAccepted "2014-07-15"^^xsd:date ;
  dcterms:source "ISO/TS 19159-1:2014, 4.14" ;
  reg:status reg:statusValid ;
  rdfs:label "keystone effect"@en ;
  skos:changeNote "valid" ;
  skos:editorialNote "preferred"^^xsd:string ;
  skos:notation 1461 ;
  skos:prefLabel "keystone effect"@en ;
.
<http://iso.org/tc211/term/1463>
  rdf:type skos:Concept ;
  dcterms:dateAccepted "2014-07-15"^^xsd:date ;
  dcterms:provenance "ISO/TS 19159-1:2014, 4.18" ;
  dcterms:source "ISO/IEC Guide 99:2007, 2.16" ;
  reg:status reg:statusValid ;
  rdfs:comment "Note 1 to entry:  The concept of \"measurement error\" can be used both a) when there is a single reference quantity value to refer to, which occurs if a calibration is made by means of a measurement standard with a measured quantity value having a negligible measurement uncertainty or if a conventional quantity value is given, in which case the measurement error is known, and b) if a measurand is supposed to be represented by a unique true quantity value or a set of true quantity values of negligible range, in which case the measurement error is not known."@en ;
  rdfs:comment "Note 2 to entry:  Measurement error should not be confused with production error or mistake." ;
  rdfs:label "measurement error"@en ;
  rdfs:seeAlso "error of measurement, error" ;
  skos:altLabel "error of measurement, error"@en ;
  skos:changeNote "valid" ;
  skos:editorialNote "preferred"^^xsd:string ;
  skos:notation 1463 ;
  skos:note "Note 1 to entry:  The concept of \"measurement error\" can be used both a) when there is a single reference quantity value to refer to, which occurs if a calibration is made by means of a measurement standard with a measured quantity value having a negligible measurement uncertainty or if a conventional quantity value is given, in which case the measurement error is known, and b) if a measurand is supposed to be represented by a unique true quantity value or a set of true quantity values of negligible range, in which case the measurement error is not known."@en ;
  skos:note "Note 2 to entry:  Measurement error should not be confused with production error or mistake."^^<http://www.w3.org/2001/XMLSchema#@en> ;
  skos:prefLabel "measurement error"@en ;
.
<http://iso.org/tc211/term/1465>
  rdf:type skos:Concept ;
  dcterms:dateAccepted "2014-07-15"^^xsd:date ;
  dcterms:provenance "ISO/TS 19159-1:2014, 4.19" ;
  dcterms:source "ISO/IEC Guide 99:2007, 2.15" ;
  reg:status reg:statusValid ;
  rdfs:comment "Note 1 to entry: Measurement precision is usually expressed numerically by measures of imprecision, such as standard deviation, variance, or coefficient of variation under the specified conditions of measurement."@en ;
  rdfs:comment "Note 2 to entry:  The \"specified conditions\" can be, for example, repeatability conditions of measurement, intermediate precision conditions of measurement, or reproducibility conditions of measurement (see ISO 5725-3)." ;
  rdfs:comment "Note 3 to entry:  Measurement precision is used to define measurement repeatability, intermediate measurement precision, and measurement reproducibility."@en ;
  rdfs:comment "Note 4 to entry:  Sometimes \"measurement precision\" is erroneously used to mean measurement accuracy."@en ;
  rdfs:label "measurement precision"@en ;
  rdfs:seeAlso "precision" ;
  skos:altLabel "precision"@en ;
  skos:changeNote "valid" ;
  skos:editorialNote "preferred"^^xsd:string ;
  skos:notation 1465 ;
  skos:note "Note 1 to entry: Measurement precision is usually expressed numerically by measures of imprecision, such as standard deviation, variance, or coefficient of variation under the specified conditions of measurement."@en ;
  skos:note "Note 2 to entry:  The \"specified conditions\" can be, for example, repeatability conditions of measurement, intermediate precision conditions of measurement, or reproducibility conditions of measurement (see ISO 5725-3)."^^<http://www.w3.org/2001/XMLSchema#@en> ;
  skos:note "Note 3 to entry:  Measurement precision is used to define measurement repeatability, intermediate measurement precision, and measurement reproducibility."^^<http://www.w3.org/2001/XMLSchema#@en> ;
  skos:note "Note 4 to entry:  Sometimes \"measurement precision\" is erroneously used to mean measurement accuracy."@en ;
  skos:prefLabel "measurement precision"@en ;
.
<http://iso.org/tc211/term/1468>
  rdf:type skos:Concept ;
  dcterms:dateAccepted "2014-07-15"^^xsd:date ;
  dcterms:provenance "ISO/TS 19159-1:2014, 4.21" ;
  dcterms:source "ISO/IEC Guide 99:2007, 2.42" ;
  reg:status reg:statusValid ;
  rdfs:comment "Note 1 to entry:   A metrological traceability chain is defined through a calibration hierarchy."@en ;
  rdfs:comment "Note 2 to entry:  A metrological traceability chain is used to establish metrological traceability of a measurement result." ;
  rdfs:comment "Note 3 to entry:  A comparison between two measurement standards may be viewed as a calibration if the comparison is used to check and, if necessary, correct the quantity value and measurement uncertainty attributed to one of the measurement standards."@en ;
  rdfs:label "metrological traceability chain"@en ;
  rdfs:seeAlso "traceability chain" ;
  skos:altLabel "traceability chain"@en ;
  skos:changeNote "valid" ;
  skos:editorialNote "preferred"^^xsd:string ;
  skos:notation 1468 ;
  skos:note "Note 1 to entry:   A metrological traceability chain is defined through a calibration hierarchy."@en ;
  skos:note "Note 2 to entry:  A metrological traceability chain is used to establish metrological traceability of a measurement result."^^<http://www.w3.org/2001/XMLSchema#@en> ;
  skos:note "Note 3 to entry:  A comparison between two measurement standards may be viewed as a calibration if the comparison is used to check and, if necessary, correct the quantity value and measurement uncertainty attributed to one of the measurement standards."^^<http://www.w3.org/2001/XMLSchema#@en> ;
  skos:prefLabel "metrological traceability chain"@en ;
.
<http://iso.org/tc211/term/147>
  rdf:type skos:Concept ;
  dcterms:dateAccepted "2003-05-01"^^xsd:date ;
  dcterms:dateAccepted "2009-12-29"^^xsd:date ;
  dcterms:provenance "KS X ISO 19107" ;
  dcterms:source "ISO 19107:2003" ;
  reg:status reg:statusValid ;
  rdfs:comment "Note 1 to entry: The edge-node graph is a subcomplex of the complex within which it is embedded."@en ;
  rdfs:comment "비고: 변-절점 그래프는 그것이 포함된 복합체의 하위 복합체이다."@kr ;
  rdfs:label "edge-node graph"@en ;
  skos:changeNote "valid" ;
  skos:definition "변의 집합과 그것에 관련한 연결 절점의 집합으로 나타낼 수 있는 위상 복합체 내에 내재된 그래프"@kr ;
  skos:editorialNote "preferred" ;
  skos:editorialNote "preferred"^^xsd:string ;
  skos:notation "147" ;
  skos:notation 147 ;
  skos:note "Note 1 to entry: The edge-node graph is a subcomplex of the complex within which it is embedded."@en ;
  skos:note "비고: 변-절점 그래프는 그것이 포함된 복합체의 하위 복합체이다."@kr ;
  skos:prefLabel "edge-node graph"@en ;
  skos:prefLabel "변-절점 그래프"@kr ;
.
<http://iso.org/tc211/term/1470>
  rdf:type skos:Concept ;
  dcterms:dateAccepted "2014-07-15"^^xsd:date ;
  dcterms:provenance "ISO/TS 19159-1:2014, 4.22" ;
  dcterms:source "ISO 12718:2008, 2.26" ;
  reg:status reg:statusValid ;
  rdfs:comment "Note 1 to entry:  Noise is a random fluctuation in a signal disturbing the recognition of a carried information."@en ;
  rdfs:label "noise"@en ;
  skos:changeNote "valid" ;
  skos:editorialNote "preferred"^^xsd:string ;
  skos:notation 1470 ;
  skos:note "Note 1 to entry:  Noise is a random fluctuation in a signal disturbing the recognition of a carried information."@en ;
  skos:prefLabel "noise"@en ;
.
<http://iso.org/tc211/term/1471>
  rdf:type skos:Concept ;
  dcterms:dateAccepted "2014-07-15"^^xsd:date ;
  dcterms:source "ISO/TS 19159-1:2014, 4.23" ;
  reg:status reg:statusValid ;
  rdfs:label "pixel response non-uniformity"@en ;
  skos:altLabel "PRNU"^^<http://www.w3.org/2001/XMLSchema#@en> ;
  skos:changeNote "valid" ;
  skos:editorialNote "preferred"^^xsd:string ;
  skos:notation 1471 ;
  skos:prefLabel "pixel response non-uniformity"@en ;
.
<http://iso.org/tc211/term/1472>
  rdf:type skos:Concept ;
  dcterms:dateAccepted "2014-07-15"^^xsd:date ;
  dcterms:provenance "ISO/TS 19159-1:2014, 4.24" ;
  dcterms:source "IEC 88528-11:2004" ;
  reg:status reg:statusValid ;
  rdfs:label "point-spread function"@en ;
  skos:altLabel "PSF"^^<http://www.w3.org/2001/XMLSchema#@en> ;
  skos:changeNote "valid" ;
  skos:editorialNote "preferred"^^xsd:string ;
  skos:notation 1472 ;
  skos:prefLabel "point-spread function"@en ;
.
<http://iso.org/tc211/term/1474>
  rdf:type skos:Concept ;
  dcterms:dateAccepted "2014-07-15"^^xsd:date ;
  dcterms:provenance "ISO/TS 19159-1:2014, 4.27" ;
  dcterms:source "ISO/IEC Guide 99:2007, 1.1, modified — The Notes have been changed." ;
  reg:status reg:statusValid ;
  rdfs:comment "Note 1 to entry:  A reference can be a measurement unit, a measurement procedure, a reference material, or a combination of such."@en ;
  rdfs:comment "Note 2 to entry:  Symbols for quantities are given in the ISO 80000 and IEC 80000 series Quantities and units. The symbols for quantities are written in italics. A given symbol can indicate different quantities." ;
  rdfs:comment "Note 3 to entry:  A quantity as defined here is a scalar. However, a vector or a tensor, the components of which are quantities, is also considered to be a quantity."@en ;
  rdfs:comment "Note 4 to entry:  The concept \"quantity\" may be generically divided into, e.g. \"physical quantity\", \"chemical quantity\", and \"biological quantity\", or \"base quantity\" and \"derived quantity\"."@en ;
  rdfs:label "quantity"@en ;
  skos:changeNote "valid" ;
  skos:editorialNote "preferred"^^xsd:string ;
  skos:notation 1474 ;
  skos:note "Note 1 to entry:  A reference can be a measurement unit, a measurement procedure, a reference material, or a combination of such."@en ;
  skos:note "Note 2 to entry:  Symbols for quantities are given in the ISO 80000 and IEC 80000 series Quantities and units. The symbols for quantities are written in italics. A given symbol can indicate different quantities."^^<http://www.w3.org/2001/XMLSchema#@en> ;
  skos:note "Note 3 to entry:  A quantity as defined here is a scalar. However, a vector or a tensor, the components of which are quantities, is also considered to be a quantity."^^<http://www.w3.org/2001/XMLSchema#@en> ;
  skos:note "Note 4 to entry:  The concept \"quantity\" may be generically divided into, e.g. \"physical quantity\", \"chemical quantity\", and \"biological quantity\", or \"base quantity\" and \"derived quantity\"."@en ;
  skos:prefLabel "quantity"@en ;
.
<http://iso.org/tc211/term/1475>
  rdf:type skos:Concept ;
  dcterms:dateAccepted "2014-07-15"^^xsd:date ;
  dcterms:source "ISO/TS 19159-1:2014, 4.28" ;
  reg:status reg:statusValid ;
  rdfs:label "reference standard"@en ;
  skos:changeNote "valid" ;
  skos:editorialNote "preferred"^^xsd:string ;
  skos:notation 1475 ;
  skos:prefLabel "reference standard"@en ;
.
<http://iso.org/tc211/term/148>
  rdf:type skos:Concept ;
  dcterms:dateAccepted "2007-09-01"^^xsd:date ;
  dcterms:dateAccepted "2009-12-29"^^xsd:date ;
  dcterms:provenance "KS X ISO 19136" ;
  dcterms:source "ISO 19136:2007" ;
  reg:status reg:statusValid ;
  rdfs:comment "Note 1 to entry: From the XML Information Set: \"Each XML document contains one or more elements, the boundaries of which are either delimited by start-tags and end-tags, or, for empty elements, by an empty-element tag. Each element has a type, identified by name, sometimes called its 'generic identifier' (GI), and may have a set of attribute specifications. Each attribute specification has a name and a value."@en ;
  rdfs:comment "비고: XML Information Set에서는 \"모든 XML 문서는 start 꼬리표와 end 꼬리표로 범위 지워진 한 개 혹은 여러 개의 요소로 구성되며, 내용이 없는 경우에는 empty 꼬리표를 사용한다. 각각의 요소는 종종 '고유 식별자(GI)'라 불리우며 명칭에 의해 식별되는 유형과 속성 사양 집합을 갖는다. 각각의 속성은 명칭과 값을 갖게 된다. "@kr ;
  rdfs:label "element <XML>"@en ;
  skos:changeNote "valid" ;
  skos:definition "자식 요소, 속성 및 문자 데이터 등을 갖는 XML 문서의 기초 정보 항목"@kr ;
  skos:editorialNote "preferred" ;
  skos:editorialNote "preferred"^^xsd:string ;
  skos:notation "148" ;
  skos:notation 148 ;
  skos:note "Note 1 to entry: From the XML Information Set: \"Each XML document contains one or more elements, the boundaries of which are either delimited by start-tags and end-tags, or, for empty elements, by an empty-element tag. Each element has a type, identified by name, sometimes called its 'generic identifier' (GI), and may have a set of attribute specifications. Each attribute specification has a name and a value."@en ;
  skos:note "비고: XML Information Set에서는 \"모든 XML 문서는 start 꼬리표와 end 꼬리표로 범위 지워진 한 개 혹은 여러 개의 요소로 구성되며, 내용이 없는 경우에는 empty 꼬리표를 사용한다. 각각의 요소는 종종 '고유 식별자(GI)'라 불리우며 명칭에 의해 식별되는 유형과 속성 사양 집합을 갖는다. 각각의 속성은 명칭과 값을 갖게 된다. "@kr ;
  skos:prefLabel "element <XML>"@en ;
  skos:prefLabel "요소 <XML>"@kr ;
.
<http://iso.org/tc211/term/1481>
  rdf:type skos:Concept ;
  dcterms:dateAccepted "2014-07-15"^^xsd:date ;
  dcterms:provenance "ISO/TS 19159-1:2014, 4.36" ;
  dcterms:source "ISO/IEC Guide 2:2004, 1.1" ;
  reg:status reg:statusValid ;
  rdfs:comment "Note 1 to entry:  In particular, the activity consists of the processes of formulating, issuing and implementing standards."@en ;
  rdfs:comment "Note 2 to entry:  Important benefits of standardization are improvement of the suitability of products, processes and services for their intended purposes, prevention of barriers to trade and facilitation of technological cooperation." ;
  rdfs:label "standardization"@en ;
  skos:changeNote "valid" ;
  skos:editorialNote "preferred"^^xsd:string ;
  skos:notation 1481 ;
  skos:note "Note 1 to entry:  In particular, the activity consists of the processes of formulating, issuing and implementing standards."@en ;
  skos:note "Note 2 to entry:  Important benefits of standardization are improvement of the suitability of products, processes and services for their intended purposes, prevention of barriers to trade and facilitation of technological cooperation."^^<http://www.w3.org/2001/XMLSchema#@en> ;
  skos:prefLabel "standardization"@en ;
.
<http://iso.org/tc211/term/1483>
  rdf:type skos:Concept ;
  dcterms:dateAccepted "2014-07-15"^^xsd:date ;
  dcterms:provenance "ISO/TS 19159-1:2014, 4.21" ;
  dcterms:source "ISO/IEC Guide 99:2007, 2.42" ;
  reg:status reg:statusValid ;
  rdfs:comment "Note 1 to entry:   A metrological traceability chain is defined through a calibration hierarchy."@en ;
  rdfs:comment "Note 2 to entry:  A metrological traceability chain is used to establish metrological traceability of a measurement result." ;
  rdfs:comment "Note 3 to entry:  A comparison between two measurement standards may be viewed as a calibration if the comparison is used to check and, if necessary, correct the quantity value and measurement uncertainty attributed to one of the measurement standards."@en ;
  rdfs:label "traceability chain"@en ;
  rdfs:seeAlso "metrological traceability chain" ;
  skos:altLabel "metrological traceability chain"@en ;
  skos:changeNote "valid" ;
  skos:editorialNote "admitted"^^xsd:string ;
  skos:notation 1483 ;
  skos:note "Note 1 to entry:   A metrological traceability chain is defined through a calibration hierarchy."@en ;
  skos:note "Note 2 to entry:  A metrological traceability chain is used to establish metrological traceability of a measurement result."^^<http://www.w3.org/2001/XMLSchema#@en> ;
  skos:note "Note 3 to entry:  A comparison between two measurement standards may be viewed as a calibration if the comparison is used to check and, if necessary, correct the quantity value and measurement uncertainty attributed to one of the measurement standards."^^<http://www.w3.org/2001/XMLSchema#@en> ;
  skos:prefLabel "traceability chain"@en ;
.
<http://iso.org/tc211/term/1486>
  rdf:type skos:Concept ;
  dcterms:dateAccepted "2014-07-15"^^xsd:date ;
  dcterms:provenance "ISO/TS 19159-1:2014, 4.40" ;
  dcterms:source "ISO/IEC Guide 99:2007, 2.44, modified — Note 6 has been deleted." ;
  reg:status reg:statusValid ;
  rdfs:comment "Note 1 to entry:  When applicable, measurement uncertainty should be taken into consideration."@en ;
  rdfs:comment "Note 2 to entry:  The item may be, e.g. a process, measurement procedure, material, compound, or measuring system." ;
  rdfs:comment "Note 3 to entry:  The specified requirements may be, e.g. that a manufacturer's specifications are met."@en ;
  rdfs:comment "Note 4 to entry:  Verification should not be confused with calibration. Not every verification is a validation."@en ;
  rdfs:label "verification"@en ;
  skos:changeNote "valid" ;
  skos:editorialNote "preferred"^^xsd:string ;
  skos:notation 1486 ;
  skos:note "Note 1 to entry:  When applicable, measurement uncertainty should be taken into consideration."@en ;
  skos:note "Note 2 to entry:  The item may be, e.g. a process, measurement procedure, material, compound, or measuring system."^^<http://www.w3.org/2001/XMLSchema#@en> ;
  skos:note "Note 3 to entry:  The specified requirements may be, e.g. that a manufacturer's specifications are met."^^<http://www.w3.org/2001/XMLSchema#@en> ;
  skos:note "Note 4 to entry:  Verification should not be confused with calibration. Not every verification is a validation."@en ;
  skos:prefLabel "verification"@en ;
.
<http://iso.org/tc211/term/1487>
  rdf:type skos:Concept ;
  dcterms:dateAccepted "2014-07-15"^^xsd:date ;
  dcterms:source "ISO/TS 19159-1:2014, 4.41" ;
  reg:status reg:statusValid ;
  rdfs:label "vicarious calibration"@en ;
  skos:changeNote "valid" ;
  skos:editorialNote "preferred"^^xsd:string ;
  skos:notation 1487 ;
  skos:prefLabel "vicarious calibration"@en ;
.
<http://iso.org/tc211/term/149>
  rdf:type skos:Concept ;
  dcterms:dateAccepted "2003-02-15" ;
  dcterms:dateAccepted "2003-02-15"^^xsd:date ;
  dcterms:dateAccepted "2007-11-01"^^xsd:date ;
  dcterms:provenance "ISO 19111:2003" ;
  dcterms:provenance "KS X ISO 19111" ;
  dcterms:source "ISO 19111:2007" ;
  reg:status reg:statusAccepted ;
  reg:status reg:statusValid ;
  rdfs:comment "Note 1 to entry: In this International Standard, ellipsoids are always oblate, meaning that the axis of rotation is always the minor axis."@en ;
  rdfs:comment "OPMERKING In deze Internationale Norm zijn ellipsoïden altijd aan de polen afgeplat, ofwel de omwentelingsas is altijd de korte as."@nl ;
  rdfs:comment "비고: 본 표준에서 타원체는 항상 그 회전축이 항상 단축인 회전 타원면이다."@kr ;
  rdfs:label "ellipsoid"@en ;
  skos:changeNote "valid" ;
  skos:definition "oppervlak gevormd door de omwenteling van een ellipsoïde rond een centrale as"@nl ;
  skos:definition "타원을 한 개의 주축 주위로 회전했을 때에 생성되는 표면"@kr ;
  skos:editorialNote "preferred" ;
  skos:editorialNote "preferred"^^xsd:string ;
  skos:notation "149" ;
  skos:notation 149 ;
  skos:note "Note 1 to entry: In this International Standard, ellipsoids are always oblate, meaning that the axis of rotation is always the minor axis."@en ;
  skos:note "OPMERKING In deze Internationale Norm zijn ellipsoïden altijd aan de polen afgeplat, ofwel de omwentelingsas is altijd de korte as."@nl ;
  skos:note "비고: 본 표준에서 타원체는 항상 그 회전축이 항상 단축인 회전 타원면이다."@kr ;
  skos:prefLabel "ellipsoid"@en ;
  skos:prefLabel "ellipsoïde"@nl ;
  skos:prefLabel "타원체"@kr ;
.
<http://iso.org/tc211/term/15>
  rdf:type skos:Concept ;
  dcterms:dateAccepted "2002-07-01" ;
  dcterms:dateAccepted "2002-07-01"^^xsd:date ;
  dcterms:dateAccepted "2008-12-30"^^xsd:date ;
  dcterms:provenance "ISO 19101:2002" ;
  dcterms:source "ISO 19101-1:2014, 4.1.2" ;
  reg:status reg:statusAccepted ;
  reg:status reg:statusValid ;
  rdfs:label "application schema"@en ;
  skos:changeNote "valid" ;
  skos:definition "informatiemodel dat gegevens beschrijft die worden gebruikt door een of meer applicaties"@nl ;
  skos:definition "하나 이상의 응용에서 요구되는 데이터의 개념적 스키마"@kr ;
  skos:editorialNote "preferred" ;
  skos:editorialNote "preferred"^^xsd:string ;
  skos:notation "15" ;
  skos:notation 15 ;
  skos:prefLabel "applicatie schema"@nl ;
  skos:prefLabel "application schema"@en ;
  skos:prefLabel "응용 스키마"@kr ;
.
<http://iso.org/tc211/term/150>
  rdf:type skos:Concept ;
  dcterms:dateAccepted "2003-02-15" ;
  dcterms:dateAccepted "2003-02-15"^^xsd:date ;
  dcterms:dateAccepted "2007-11-01"^^xsd:date ;
  dcterms:provenance "ISO 19111:2003" ;
  dcterms:provenance "KS X ISO 19111" ;
  dcterms:source "ISO 19111:2007" ;
  reg:status reg:statusAccepted ;
  reg:status reg:statusValid ;
  rdfs:comment "Note 1 to entry: Only used as part of a three-dimensional ellipsoidal coordinate system and never on its own."@en ;
  rdfs:comment "OPMERKING Wordt alleen gebruikt als deel van een driedimensionaal ellipsoidaal coördinaatsysteem en nooit op zichzelf staand."@en ;
  rdfs:comment "비고: 3차원 타원체 좌표계의 일부로 사용되며, 독립적으로 사용되지 않는다."@kr ;
  rdfs:label "ellipsoidal height"@en ;
  rdfs:seeAlso "geodetic height" ;
  rdfs:seeAlso "geodetische hoogte"@nl ;
  skos:altLabel "geodetic height"@en ;
  skos:altLabel "geodetische hoogte"@nl ;
  skos:altLabel "h"@kr ;
  skos:altLabel "h"@nl ;
  skos:altLabel "h"^^<http://www.w3.org/2001/XMLSchema#@en> ;
  skos:changeNote "valid" ;
  skos:definition "afstand van een punt tot de ellipsoïde gemeten langs een lijn loodrecht op de ellipsoïde positief indien naar boven of naar de buitenzijde van de ellipsoïde"@nl ;
  skos:definition "타원체로부터 어떤 점까지의 수직선을 따라 측정된 그 점까지의 거리, 타원체의 위쪽 또는 외측으로 향한 경우는 정(+)으로 표현 "@kr ;
  skos:editorialNote "preferred" ;
  skos:editorialNote "preferred"^^xsd:string ;
  skos:notation "150" ;
  skos:notation 150 ;
  skos:note "Note 1 to entry: Only used as part of a three-dimensional ellipsoidal coordinate system and never on its own."@en ;
  skos:note "OPMERKING Wordt alleen gebruikt als deel van een driedimensionaal ellipsoidaal coördinaatsysteem en nooit op zichzelf staand."@en ;
  skos:note "비고: 3차원 타원체 좌표계의 일부로 사용되며, 독립적으로 사용되지 않는다."@kr ;
  skos:prefLabel "ellipsoidal height"@en ;
  skos:prefLabel "ellipsoïde hoogte"@nl ;
  skos:prefLabel "타원체고"@kr ;
.
<http://iso.org/tc211/term/151>
  rdf:type skos:Concept ;
  dcterms:dateAccepted "2005-07-15"^^xsd:date ;
  dcterms:dateAccepted "2008-12-30"^^xsd:date ;
  dcterms:provenance "ISO 19118:2005" ;
  dcterms:source "ISO 19118:2011, 4.13" ;
  reg:status reg:statusValid ;
  rdfs:label "encoding"@en ;
  skos:changeNote "valid" ;
  skos:definition "데이터를 일련의 코드로 전환하는 것"@kr ;
  skos:editorialNote "preferred" ;
  skos:editorialNote "preferred"^^xsd:string ;
  skos:notation "151" ;
  skos:notation 151 ;
  skos:prefLabel "encoding"@en ;
  skos:prefLabel "부호화"@kr ;
.
<http://iso.org/tc211/term/1512>
  rdf:type skos:Concept ;
  dcterms:dateAccepted "2012-12-15"^^xsd:date ;
  dcterms:source "ISO 19117:2012, 4.3" ;
  reg:status reg:statusValid ;
  rdfs:label "complex symbol"@en ;
  skos:changeNote "valid" ;
  skos:editorialNote "preferred"^^xsd:string ;
  skos:notation 1512 ;
  skos:prefLabel "complex symbol"@en ;
.
<http://iso.org/tc211/term/1513>
  rdf:type skos:Concept ;
  dcterms:dateAccepted "2012-12-15"^^xsd:date ;
  dcterms:source "ISO 19117:2012, 4.4" ;
  reg:status reg:statusValid ;
  rdfs:label "compound symbol"@en ;
  skos:changeNote "valid" ;
  skos:editorialNote "preferred"^^xsd:string ;
  skos:notation 1513 ;
  skos:prefLabel "compound symbol"@en ;
.
<http://iso.org/tc211/term/152>
  rdf:type skos:Concept ;
  dcterms:dateAccepted "2005-07-15"^^xsd:date ;
  dcterms:dateAccepted "2008-12-30"^^xsd:date ;
  dcterms:provenance "ISO 19118:2005" ;
  dcterms:source "ISO 19118:2011, 4.14" ;
  reg:status reg:statusValid ;
  rdfs:comment "Note 1 to entry: An encoding rule specifies the types of data to be converted as well as the syntax, structure and codes used in the resulting data structure."@en ;
  rdfs:comment "비고: 부호화 규칙은 결과 데이터 구조에 사용되는 구문법, 구조, 코드 뿐만 아니라 변환된 데이터 형식들을 상세하게 정의한다."@kr ;
  rdfs:label "encoding rule"@en ;
  skos:changeNote "valid" ;
  skos:definition "특정 데이터 구조로의 부호화를 정의하는 식별 가능한 전환 규칙의 모음"@kr ;
  skos:editorialNote "preferred" ;
  skos:editorialNote "preferred"^^xsd:string ;
  skos:notation "152" ;
  skos:notation 152 ;
  skos:note "Note 1 to entry: An encoding rule specifies the types of data to be converted as well as the syntax, structure and codes used in the resulting data structure."@en ;
  skos:note "비고: 부호화 규칙은 결과 데이터 구조에 사용되는 구문법, 구조, 코드 뿐만 아니라 변환된 데이터 형식들을 상세하게 정의한다."@kr ;
  skos:prefLabel "encoding rule"@en ;
  skos:prefLabel "부호화 규칙"@kr ;
.
<http://iso.org/tc211/term/153>
  rdf:type skos:Concept ;
  dcterms:dateAccepted "2005-07-15"^^xsd:date ;
  dcterms:dateAccepted "2008-12-30"^^xsd:date ;
  dcterms:provenance "ISO 19118:2005" ;
  dcterms:source "ISO 19118:2011, 4.15" ;
  reg:status reg:statusValid ;
  rdfs:label "encoding service"@en ;
  skos:changeNote "valid" ;
  skos:definition "부호화 규칙을 제공하는 소프트웨어 컴포넌트"@kr ;
  skos:editorialNote "preferred" ;
  skos:editorialNote "preferred"^^xsd:string ;
  skos:notation "153" ;
  skos:notation 153 ;
  skos:prefLabel "encoding service"@en ;
  skos:prefLabel "부호화 서비스"@kr ;
.
<http://iso.org/tc211/term/154>
  rdf:type skos:Concept ;
  dcterms:dateAccepted "2003-05-01"^^xsd:date ;
  dcterms:dateAccepted "2009-12-29"^^xsd:date ;
  dcterms:provenance "KS X ISO 19107" ;
  dcterms:source "ISO 19107:2003" ;
  reg:status reg:statusValid ;
  rdfs:label "end node"@en ;
  skos:changeNote "valid" ;
  skos:definition "변이 포함된 위상 복합체의 유효한 기하 실현에서 곡선의 끝점에 대응되는 경계 절점"@kr ;
  skos:editorialNote "preferred" ;
  skos:editorialNote "preferred"^^xsd:string ;
  skos:notation "154" ;
  skos:notation 154 ;
  skos:prefLabel "end node"@en ;
  skos:prefLabel "끝 절점"@kr ;
.
<http://iso.org/tc211/term/1547>
  rdf:type skos:Concept ;
  dcterms:dateAccepted "2012-11-15"^^xsd:date ;
  dcterms:provenance "ISO/TS 19150-1:2012, 4.6" ;
  dcterms:source "ISO/TS 27790:2009" ;
  reg:status reg:statusValid ;
  rdfs:label "framework"@en ;
  skos:changeNote "valid" ;
  skos:editorialNote "preferred"^^xsd:string ;
  skos:notation 1547 ;
  skos:prefLabel "framework"@en ;
.
<http://iso.org/tc211/term/1548>
  rdf:type skos:Concept ;
  dcterms:dateAccepted "2012-11-15"^^xsd:date ;
  dcterms:provenance "ISO/TS 19150-1:2012, 4.8" ;
  dcterms:source "Adapted from ISO 5127:2001" ;
  reg:status reg:statusValid ;
  rdfs:label "knowledge"@en ;
  skos:changeNote "valid" ;
  skos:editorialNote "preferred"^^xsd:string ;
  skos:notation 1548 ;
  skos:prefLabel "knowledge"@en ;
.
<http://iso.org/tc211/term/155>
  rdf:type skos:Concept ;
  dcterms:dateAccepted "2003-05-01"^^xsd:date ;
  dcterms:dateAccepted "2009-12-29"^^xsd:date ;
  dcterms:provenance "KS X ISO 19107" ;
  dcterms:source "ISO 19107:2003" ;
  reg:status reg:statusValid ;
  rdfs:label "end point"@en ;
  skos:changeNote "valid" ;
  skos:definition "곡선의 마지막 점"@kr ;
  skos:editorialNote "preferred" ;
  skos:editorialNote "preferred"^^xsd:string ;
  skos:notation "155" ;
  skos:notation 155 ;
  skos:prefLabel "end point"@en ;
  skos:prefLabel "끝점"@kr ;
.
<http://iso.org/tc211/term/1559>
  rdf:type skos:Concept ;
  dcterms:dateAccepted "2014-01-15"^^xsd:date ;
  dcterms:source "ISO/TS 19130-2:2014, 4.14" ;
  reg:status reg:statusValid ;
  rdfs:label "Differential Global Navigational Satellite System"@en ;
  skos:changeNote "valid" ;
  skos:editorialNote "preferred"^^xsd:string ;
  skos:notation 1559 ;
  skos:prefLabel "Differential Global Navigational Satellite System"@en ;
.
<http://iso.org/tc211/term/156>
  rdf:type skos:Concept ;
  dcterms:dateAccepted "2003-02-15" ;
  dcterms:dateAccepted "2003-02-15"^^xsd:date ;
  dcterms:dateAccepted "2007-11-01"^^xsd:date ;
  dcterms:provenance "ISO 19111:2003" ;
  dcterms:provenance "KS X ISO 19111" ;
  dcterms:source "ISO 19111:2007" ;
  reg:status reg:statusAccepted ;
  reg:status reg:statusValid ;
  rdfs:comment "Note 1 to entry: Engineering datum excludes both geodetic and vertical datums."@en ;
  rdfs:comment "OPMERKING Een lokaal datum is nooit een geodetisch of verticaal datum."@en ;
  rdfs:comment "비고: 공학 데이텀은 측지 원점 및 수직 데이텀 모두를 배제한다."@kr ;
  rdfs:label "engineering datum"@en ;
  rdfs:seeAlso "local datum" ;
  rdfs:seeAlso "lokale datum"@nl ;
  skos:altLabel "local datum"@en ;
  skos:altLabel "lokale datum"@nl ;
  skos:changeNote "valid" ;
  skos:definition "datum waarmee de relatie tussen een coördinaatsysteem en een lokale referentie wordt beschreven"@nl ;
  skos:definition "지역 참조와 좌표 체계간의 관계를 설명하는 지역 데이텀"@kr ;
  skos:editorialNote "preferred" ;
  skos:editorialNote "preferred"^^xsd:string ;
  skos:notation "156" ;
  skos:notation 156 ;
  skos:note "Note 1 to entry: Engineering datum excludes both geodetic and vertical datums."@en ;
  skos:note "OPMERKING Een lokaal datum is nooit een geodetisch of verticaal datum."@en ;
  skos:note "비고: 공학 데이텀은 측지 원점 및 수직 데이텀 모두를 배제한다."@kr ;
  skos:prefLabel "engineering datum"@en ;
  skos:prefLabel "lokaal datum"@nl ;
  skos:prefLabel "공학 데이텀"@kr ;
.
<http://iso.org/tc211/term/1560>
  rdf:type skos:Concept ;
  dcterms:dateAccepted "2014-01-15"^^xsd:date ;
  dcterms:provenance "ISO/TS 19130-2:2014, 4.19" ;
  dcterms:source "Adapted from the Manual of Photogrammetry" ;
  reg:status reg:statusValid ;
  rdfs:comment "Note 1 to entry:  The field of regard is the area that is potentially able to be viewed by a system at an instant in time. It is determined by the system’s  FOV  and the range  of directions in which the system is able to point."@en ;
  rdfs:label "field of regard"@en ;
  skos:changeNote "valid" ;
  skos:editorialNote "preferred"^^xsd:string ;
  skos:notation 1560 ;
  skos:note "Note 1 to entry:  The field of regard is the area that is potentially able to be viewed by a system at an instant in time. It is determined by the system’s  FOV  and the range  of directions in which the system is able to point."@en ;
  skos:prefLabel "field of regard"@en ;
.
<http://iso.org/tc211/term/1562>
  rdf:type skos:Concept ;
  dcterms:dateAccepted "2014-01-15"^^xsd:date ;
  dcterms:provenance "ISO/TS 19130-2:2014, 4.43" ;
  dcterms:source "IHO Hydrographic Dictionary S-32, Fifth Edition" ;
  reg:status reg:statusValid ;
  rdfs:label "mean sea level"@en ;
  skos:altLabel "MSL"^^<http://www.w3.org/2001/XMLSchema#@en> ;
  skos:changeNote "valid" ;
  skos:editorialNote "preferred"^^xsd:string ;
  skos:notation 1562 ;
  skos:prefLabel "mean sea level"@en ;
.
<http://iso.org/tc211/term/1563>
  rdf:type skos:Concept ;
  dcterms:dateAccepted "2014-01-15"^^xsd:date ;
  dcterms:provenance "ISO/TS 19130-2:2014, 4.44" ;
  dcterms:source "IHO Hydrographic Dictionary S-32, Fifth Edition" ;
  reg:status reg:statusValid ;
  rdfs:comment "Note 1 to entry:  Depths are measured directly below and transverse to the ship's track. The width of the swath is a function of the number of beams and their aperture."@en ;
  rdfs:label "multibeam SONAR"@en ;
  skos:changeNote "valid" ;
  skos:editorialNote "preferred"^^xsd:string ;
  skos:notation 1563 ;
  skos:note "Note 1 to entry:  Depths are measured directly below and transverse to the ship's track. The width of the swath is a function of the number of beams and their aperture."@en ;
  skos:prefLabel "multibeam SONAR"@en ;
.
<http://iso.org/tc211/term/1564>
  rdf:type skos:Concept ;
  dcterms:dateAccepted "2014-01-15"^^xsd:date ;
  dcterms:provenance "ISO/TS 19130-2:2014, 4.45" ;
  dcterms:source "Adapted from ASTM E2544" ;
  reg:status reg:statusValid ;
  rdfs:label "multiple returns"@en ;
  skos:changeNote "valid" ;
  skos:editorialNote "preferred"^^xsd:string ;
  skos:notation 1564 ;
  skos:prefLabel "multiple returns"@en ;
.
<http://iso.org/tc211/term/1565>
  rdf:type skos:Concept ;
  dcterms:dateAccepted "2014-01-15"^^xsd:date ;
  dcterms:source "ISO/TS 19130-2:2014, 4.53" ;
  reg:status reg:statusValid ;
  rdfs:label "pulse repetition frequency"@en ;
  skos:changeNote "valid" ;
  skos:editorialNote "preferred"^^xsd:string ;
  skos:notation 1565 ;
  skos:prefLabel "pulse repetition frequency"@en ;
.
<http://iso.org/tc211/term/1566>
  rdf:type skos:Concept ;
  dcterms:dateAccepted "2014-01-15"^^xsd:date ;
  dcterms:source "ISO/TS 19130-2:2014, 4.54" ;
  reg:status reg:statusValid ;
  rdfs:label "range <SAR>"@en ;
  skos:changeNote "valid" ;
  skos:editorialNote "preferred"^^xsd:string ;
  skos:notation 1566 ;
  skos:prefLabel "range <SAR>"@en ;
.
<http://iso.org/tc211/term/1567>
  rdf:type skos:Concept ;
  dcterms:dateAccepted "2014-01-15"^^xsd:date ;
  dcterms:source "ISO/TS 19130-2:2014, 4.59" ;
  reg:status reg:statusValid ;
  rdfs:comment "Note 1 to entry:  In LIDAR and SONAR systems, the receiver detects and records reflected pulse returns."@en ;
  rdfs:label "receiver"@en ;
  skos:changeNote "valid" ;
  skos:editorialNote "preferred"^^xsd:string ;
  skos:notation 1567 ;
  skos:note "Note 1 to entry:  In LIDAR and SONAR systems, the receiver detects and records reflected pulse returns."@en ;
  skos:prefLabel "receiver"@en ;
.
<http://iso.org/tc211/term/1568>
  rdf:type skos:Concept ;
  dcterms:dateAccepted "2014-01-15"^^xsd:date ;
  dcterms:provenance "ISO/TS 19130-2:2014, 4.67" ;
  dcterms:source "IHO Hydrographic Dictionary S-32, Fifth Edition" ;
  reg:status reg:statusValid ;
  rdfs:comment "Note 1 to entry:  Settlement is not an increase in displacement."@en ;
  rdfs:comment "Note 2 to entry:  Settlement is measured as an angular tilt about the centre of gravity of the vessel." ;
  rdfs:label "settlement"@en ;
  skos:changeNote "valid" ;
  skos:editorialNote "preferred"^^xsd:string ;
  skos:notation 1568 ;
  skos:note "Note 1 to entry:  Settlement is not an increase in displacement."@en ;
  skos:note "Note 2 to entry:  Settlement is measured as an angular tilt about the centre of gravity of the vessel."^^<http://www.w3.org/2001/XMLSchema#@en> ;
  skos:prefLabel "settlement"@en ;
.
<http://iso.org/tc211/term/1569>
  rdf:type skos:Concept ;
  dcterms:dateAccepted "2014-01-15"^^xsd:date ;
  dcterms:source "ISO/TS 19130-2:2014, 4.72" ;
  reg:status reg:statusValid ;
  rdfs:label "Sound Navigation And Ranging"@en ;
  rdfs:seeAlso "SONAR" ;
  skos:altLabel "SONAR"@en ;
  skos:altLabel "SONAR"^^<http://www.w3.org/2001/XMLSchema#@en> ;
  skos:changeNote "valid" ;
  skos:editorialNote "admitted"^^xsd:string ;
  skos:notation 1569 ;
  skos:prefLabel "Sound Navigation And Ranging"@en ;
.
<http://iso.org/tc211/term/157>
  rdf:type skos:Concept ;
  dcterms:dateAccepted "2005-02-15"^^xsd:date ;
  dcterms:dateAccepted "2009-12-29"^^xsd:date ;
  dcterms:provenance "ISO 19119:2005" ;
  dcterms:provenance "KS X ISO 19119" ;
  dcterms:source "ISO/IEC 10746-3:1996" ;
  reg:status reg:statusValid ;
  rdfs:label "engineering viewpoint"@en ;
  skos:changeNote "valid" ;
  skos:definition "시스템에서 객체들 간의 분산 상호 작용을 위해 요구되는 함수와 메카니즘에 초점을 둔 개방형 분산 처리 시스템과 그 환경에 대한 관점"@kr ;
  skos:editorialNote "preferred" ;
  skos:editorialNote "preferred"^^xsd:string ;
  skos:notation "157" ;
  skos:notation 157 ;
  skos:prefLabel "engineering viewpoint"@en ;
  skos:prefLabel "공학 관점"@kr ;
.
<http://iso.org/tc211/term/1570>
  rdf:type skos:Concept ;
  dcterms:dateAccepted "2012-12-01"^^xsd:date ;
  dcterms:source "ISO 19152:2012, 4.1.2" ;
  reg:status reg:statusValid ;
  rdfs:comment "Note 1 to entry: 'Unique' means that a right, restriction, or responsibility is held by one or more parties (e.g. owners or users) for the whole basic administrative unit. 'Homogeneous' means that a right, restriction or responsibility (e.g. ownership, use, social tenure, lease, or easement) affects the whole basic administrative unit. For a restriction, zero parties are a possibility."@en ;
  rdfs:comment "Note 2 to entry: A basic administrative unit may play the role of party, e.g. when the right holder is a basic administrative unit (and not a person or organization)." ;
  rdfs:comment "Note 3 to entry: A baunit should get a unique identifier when registered, or recorded."@en ;
  rdfs:comment "Note 4 to entry: A baunit can consist of zero spatial units, when a registry exists, and not a cadastre."@en ;
  rdfs:comment "Note 5 to entry: Restrictions and responsibilities can be associated with their own baunits, each with their own type of spatial unit."@en ;
  rdfs:label "basic administrative unit"@en ;
  skos:altLabel "baunit"^^<http://www.w3.org/2001/XMLSchema#@en> ;
  skos:changeNote "valid" ;
  skos:editorialNote "preferred"^^xsd:string ;
  skos:notation 1570 ;
  skos:note "Note 1 to entry: 'Unique' means that a right, restriction, or responsibility is held by one or more parties (e.g. owners or users) for the whole basic administrative unit. 'Homogeneous' means that a right, restriction or responsibility (e.g. ownership, use, social tenure, lease, or easement) affects the whole basic administrative unit. For a restriction, zero parties are a possibility."@en ;
  skos:note "Note 2 to entry: A basic administrative unit may play the role of party, e.g. when the right holder is a basic administrative unit (and not a person or organization)."^^<http://www.w3.org/2001/XMLSchema#@en> ;
  skos:note "Note 3 to entry: A baunit should get a unique identifier when registered, or recorded."^^<http://www.w3.org/2001/XMLSchema#@en> ;
  skos:note "Note 4 to entry: A baunit can consist of zero spatial units, when a registry exists, and not a cadastre."@en ;
  skos:note "Note 5 to entry: Restrictions and responsibilities can be associated with their own baunits, each with their own type of spatial unit."@en ;
  skos:prefLabel "basic administrative unit"@en ;
.
<http://iso.org/tc211/term/1571>
  rdf:type skos:Concept ;
  dcterms:dateAccepted "2012-12-01"^^xsd:date ;
  dcterms:source "ISO 19152:2012, 4.1.8" ;
  reg:status reg:statusValid ;
  rdfs:comment "Note 1 to entry: A group party may be a party member of another group party."@en ;
  rdfs:label "group party"@en ;
  skos:changeNote "valid" ;
  skos:editorialNote "preferred"^^xsd:string ;
  skos:notation 1571 ;
  skos:note "Note 1 to entry: A group party may be a party member of another group party."@en ;
  skos:prefLabel "group party"@en ;
.
<http://iso.org/tc211/term/1572>
  rdf:type skos:Concept ;
  dcterms:dateAccepted "2012-12-01"^^xsd:date ;
  dcterms:source "ISO 19152:2012, 4.1.11" ;
  reg:status reg:statusValid ;
  rdfs:label "level"@en ;
  skos:changeNote "valid" ;
  skos:editorialNote "preferred"^^xsd:string ;
  skos:notation 1572 ;
  skos:prefLabel "level"@en ;
.
<http://iso.org/tc211/term/1573>
  rdf:type skos:Concept ;
  dcterms:dateAccepted "2012-12-01"^^xsd:date ;
  dcterms:source "ISO 19152:2012, 4.1.19" ;
  reg:status reg:statusValid ;
  rdfs:label "restriction"@en ;
  skos:changeNote "valid" ;
  skos:editorialNote "preferred"^^xsd:string ;
  skos:notation 1573 ;
  skos:prefLabel "restriction"@en ;
.
<http://iso.org/tc211/term/1574>
  rdf:type skos:Concept ;
  dcterms:dateAccepted "2012-12-01"^^xsd:date ;
  dcterms:source "ISO 19152:2012, 4.1.21" ;
  reg:status reg:statusValid ;
  rdfs:comment "Note 1 to entry: Any kind of document may be added as a source according to ISO 19115:2003, B.3.2."@en ;
  rdfs:label "source"@en ;
  skos:changeNote "valid" ;
  skos:editorialNote "preferred"^^xsd:string ;
  skos:notation 1574 ;
  skos:note "Note 1 to entry: Any kind of document may be added as a source according to ISO 19115:2003, B.3.2."@en ;
  skos:prefLabel "source"@en ;
.
<http://iso.org/tc211/term/1575>
  rdf:type skos:Concept ;
  dcterms:dateAccepted "2012-12-01"^^xsd:date ;
  dcterms:source "ISO 19152:2012, 4.1.25" ;
  reg:status reg:statusValid ;
  rdfs:comment "Note 1 to entry: A utility network may be attributed with information about its legal, recorded or informal space."@en ;
  rdfs:comment "Note 2 to entry: A utility network can also be modelled as a basic administrative unit." ;
  rdfs:label "utility network"@en ;
  skos:changeNote "valid" ;
  skos:editorialNote "preferred"^^xsd:string ;
  skos:notation 1575 ;
  skos:note "Note 1 to entry: A utility network may be attributed with information about its legal, recorded or informal space."@en ;
  skos:note "Note 2 to entry: A utility network can also be modelled as a basic administrative unit."^^<http://www.w3.org/2001/XMLSchema#@en> ;
  skos:prefLabel "utility network"@en ;
.
<http://iso.org/tc211/term/1577>
  rdf:type skos:Concept ;
  dcterms:dateAccepted "2012-10-15"^^xsd:date ;
  dcterms:source "ISO/TS 19158:2012, 4.5" ;
  reg:status reg:statusValid ;
  rdfs:comment "Note 1 to entry: The assessment procedure is a second-party (customer) conformity assessment activity."@en ;
  rdfs:label "quality assessment procedure"@en ;
  skos:changeNote "valid" ;
  skos:editorialNote "preferred"^^xsd:string ;
  skos:notation 1577 ;
  skos:note "Note 1 to entry: The assessment procedure is a second-party (customer) conformity assessment activity."@en ;
  skos:prefLabel "quality assessment procedure"@en ;
.
<http://iso.org/tc211/term/1578>
  rdf:type skos:Concept ;
  dcterms:dateAccepted "2012-10-15"^^xsd:date ;
  dcterms:source "ISO/TS 19158:2012, 4.6" ;
  reg:status reg:statusValid ;
  rdfs:label "quality assessment result"@en ;
  skos:changeNote "valid" ;
  skos:editorialNote "preferred"^^xsd:string ;
  skos:notation 1578 ;
  skos:prefLabel "quality assessment result"@en ;
.
<http://iso.org/tc211/term/1579>
  rdf:type skos:Concept ;
  dcterms:dateAccepted "2012-10-15"^^xsd:date ;
  dcterms:source "ISO/TS 19158:2012, 4.8" ;
  reg:status reg:statusValid ;
  rdfs:comment "Note 1 to entry: Three quality assurance levels can be achieved as part of the quality assurance framework: basic, operational and full."@en ;
  rdfs:label "quality assurance level"@en ;
  skos:changeNote "valid" ;
  skos:editorialNote "preferred"^^xsd:string ;
  skos:notation 1579 ;
  skos:note "Note 1 to entry: Three quality assurance levels can be achieved as part of the quality assurance framework: basic, operational and full."@en ;
  skos:prefLabel "quality assurance level"@en ;
.
<http://iso.org/tc211/term/158>
  rdf:type skos:Concept ;
  dcterms:dateAccepted "2005-02-15"^^xsd:date ;
  dcterms:dateAccepted "2009-12-29"^^xsd:date ;
  dcterms:provenance "ISO 19119:2005" ;
  dcterms:provenance "KS X ISO 19119" ;
  dcterms:source "ISO/IEC 10746-3:1996" ;
  reg:status reg:statusValid ;
  rdfs:label "enterprise viewpoint"@en ;
  skos:changeNote "valid" ;
  skos:definition "시스템의 용도와 범위, 정책 측면에 초점을 둔 개방형 분산 처리 시스템과 그 환경에 대한 관점"@kr ;
  skos:editorialNote "preferred" ;
  skos:editorialNote "preferred"^^xsd:string ;
  skos:notation "158" ;
  skos:notation 158 ;
  skos:prefLabel "enterprise viewpoint"@en ;
  skos:prefLabel "전사적 관점"@kr ;
.
<http://iso.org/tc211/term/159>
  rdf:type skos:Concept ;
  dcterms:dateAccepted "2005-08-15"^^xsd:date ;
  dcterms:dateAccepted "2007-11-01"^^xsd:date ;
  dcterms:provenance "KS X ISO 19123" ;
  dcterms:source "ISO 19123:2005" ;
  reg:status reg:statusValid ;
  rdfs:label "evaluation<coverage>"@en ;
  skos:changeNote "valid" ;
  skos:definition "커버리지 영역 내의 직접 위치에서 커버리지 값의 결정"@kr ;
  skos:editorialNote "preferred" ;
  skos:editorialNote "preferred"^^xsd:string ;
  skos:notation "159" ;
  skos:notation 159 ;
  skos:prefLabel "evaluation<coverage>"@en ;
  skos:prefLabel "산출 <커버리지>"@kr ;
.
<http://iso.org/tc211/term/160>
  rdf:type skos:Concept ;
  dcterms:dateAccepted "2002-09-01"^^xsd:date ;
  dcterms:dateAccepted "2007-11-01"^^xsd:date ;
  dcterms:provenance "KS X ISO 19108" ;
  dcterms:source "ISO 19108;2002" ;
  reg:status reg:statusValid ;
  rdfs:label "event"@en ;
  skos:changeNote "valid" ;
  skos:definition "어떤 인스턴트에 일어나는 행위"@kr ;
  skos:editorialNote "preferred" ;
  skos:editorialNote "preferred"^^xsd:string ;
  skos:notation "160" ;
  skos:notation 160 ;
  skos:prefLabel "event"@en ;
  skos:prefLabel "사건"@kr ;
.
<http://iso.org/tc211/term/1603>
  rdf:type skos:Concept ;
  dcterms:dateAccepted "2014-07-15"^^xsd:date ;
  dcterms:provenance "ISO/TS 19159-1:2014, 4.17" ;
  dcterms:source "ISO 6709:2008, 4.1, modified – The preferred term is \"measurement accuracy\" rather than \"accuracy\" and Notes 1 to 3 have been added." ;
  reg:status reg:statusValid ;
  rdfs:comment "Note 1 to entry:  The concept \"measurement accuracy\" is not a quantity and is not given a numerical quantity value. A measurement is said to be more accurate when it offers a smaller measurement error."@en ;
  rdfs:comment "Note 2 to entry:  The term \"measurement accuracy\" should not be used for measurement trueness and the term measurement precision should not be used for \"measurement accuracy\", which, however, is related to both these concepts." ;
  rdfs:comment "Note 3 to entry:  \"Measurement accuracy\" is sometimes understood as closeness of agreement between measured quantity values that are being attributed to the measurand."@en ;
  rdfs:label "accuracy of measurement"@en ;
  rdfs:seeAlso "measurement accuracy, accuracy" ;
  skos:altLabel "measurement accuracy, accuracy"@en ;
  skos:changeNote "valid" ;
  skos:editorialNote "admitted"^^xsd:string ;
  skos:notation 1603 ;
  skos:note "Note 1 to entry:  The concept \"measurement accuracy\" is not a quantity and is not given a numerical quantity value. A measurement is said to be more accurate when it offers a smaller measurement error."@en ;
  skos:note "Note 2 to entry:  The term \"measurement accuracy\" should not be used for measurement trueness and the term measurement precision should not be used for \"measurement accuracy\", which, however, is related to both these concepts."^^<http://www.w3.org/2001/XMLSchema#@en> ;
  skos:note "Note 3 to entry:  \"Measurement accuracy\" is sometimes understood as closeness of agreement between measured quantity values that are being attributed to the measurand."^^<http://www.w3.org/2001/XMLSchema#@en> ;
  skos:prefLabel "accuracy of measurement"@en ;
.
<http://iso.org/tc211/term/1604>
  rdf:type skos:Concept ;
  dcterms:dateAccepted "2014-07-15"^^xsd:date ;
  dcterms:source "ISO/TS 19159-1:2014, 4.1" ;
  reg:status reg:statusValid ;
  rdfs:label "blooming"@en ;
  skos:changeNote "valid" ;
  skos:editorialNote "preferred"^^xsd:string ;
  skos:notation 1604 ;
  skos:prefLabel "blooming"@en ;
.
<http://iso.org/tc211/term/1605>
  rdf:type skos:Concept ;
  dcterms:dateAccepted "2014-07-15"^^xsd:date ;
  dcterms:source "ISO/TS 19159-1:2014, 4.4" ;
  reg:status reg:statusValid ;
  rdfs:comment "Note 1 to entry:  With respect to the general definition of validation the “calibration validation” does only refer to a small set of parameters (attribute values) such as the result of a sensor calibration."@en ;
  rdfs:label "calibration validation"@en ;
  skos:changeNote "valid" ;
  skos:editorialNote "preferred"^^xsd:string ;
  skos:notation 1605 ;
  skos:note "Note 1 to entry:  With respect to the general definition of validation the “calibration validation” does only refer to a small set of parameters (attribute values) such as the result of a sensor calibration."@en ;
  skos:prefLabel "calibration validation"@en ;
.
<http://iso.org/tc211/term/1607>
  rdf:type skos:Concept ;
  dcterms:dateAccepted "2014-07-15"^^xsd:date ;
  dcterms:provenance "ISO 6709:2008, 4.1, modified – The preferred term is \"measurement accuracy\" rather than \"accuracy\" and Notes 1 to 3 have been added." ;
  dcterms:source "ISO/TS 19159-1:2014, 4.17" ;
  reg:status reg:statusValid ;
  rdfs:comment "Note 1 to entry:  The concept \"measurement accuracy\" is not a quantity and is not given a numerical quantity value. A measurement is said to be more accurate when it offers a smaller measurement error."@en ;
  rdfs:comment "Note 2 to entry:  The term \"measurement accuracy\" should not be used for measurement trueness and the term measurement precision should not be used for \"measurement accuracy\", which, however, is related to both these concepts." ;
  rdfs:comment "Note 3 to entry:   \"Measurement accuracy\" is sometimes understood as closeness of agreement between measured quantity values that are being attributed to the measurand."@en ;
  rdfs:label "measurement accuracy"@en ;
  rdfs:seeAlso "accuracy of measurement, accuracy" ;
  skos:altLabel "accuracy of measurement, accuracy"@en ;
  skos:changeNote "valid" ;
  skos:editorialNote "preferred"^^xsd:string ;
  skos:notation 1607 ;
  skos:note "Note 1 to entry:  The concept \"measurement accuracy\" is not a quantity and is not given a numerical quantity value. A measurement is said to be more accurate when it offers a smaller measurement error."@en ;
  skos:note "Note 2 to entry:  The term \"measurement accuracy\" should not be used for measurement trueness and the term measurement precision should not be used for \"measurement accuracy\", which, however, is related to both these concepts."^^<http://www.w3.org/2001/XMLSchema#@en> ;
  skos:note "Note 3 to entry:   \"Measurement accuracy\" is sometimes understood as closeness of agreement between measured quantity values that are being attributed to the measurand."^^<http://www.w3.org/2001/XMLSchema#@en> ;
  skos:prefLabel "measurement accuracy"@en ;
.
<http://iso.org/tc211/term/1608>
  rdf:type skos:Concept ;
  dcterms:dateAccepted "2014-07-15"^^xsd:date ;
  dcterms:provenance "ISO/TS 19159-1:2014, 4.35" ;
  dcterms:source "IEC 60050-845" ;
  reg:status reg:statusValid ;
  rdfs:comment "Note 1 to entry:  The spectral responsivity is the response of the sensor with respect to the wavelengths dependent radiance."@en ;
  rdfs:comment "Note 2 to entry:  The definition is described mathematically in IEC 60050-845. The spectral responsivity is quotient of the detector output dY(λ) by the monochromatic detector input dXe(λ) = Xe, λ(λ) • dλ in the wavelength interval dλ as a function of the wavelength λ  s(λ) = dY(λ) / dXc(λ)" ;
  rdfs:label "spectral responsivity"@en ;
  skos:changeNote "valid" ;
  skos:editorialNote "preferred"^^xsd:string ;
  skos:notation 1608 ;
  skos:note "Note 1 to entry:  The spectral responsivity is the response of the sensor with respect to the wavelengths dependent radiance."@en ;
  skos:note "Note 2 to entry:  The definition is described mathematically in IEC 60050-845. The spectral responsivity is quotient of the detector output dY(λ) by the monochromatic detector input dXe(λ) = Xe, λ(λ) • dλ in the wavelength interval dλ as a function of the wavelength λ  s(λ) = dY(λ) / dXc(λ)"^^<http://www.w3.org/2001/XMLSchema#@en> ;
  skos:prefLabel "spectral responsivity"@en ;
.
<http://iso.org/tc211/term/1609>
  rdf:type skos:Concept ;
  dcterms:dateAccepted "2014-07-15"^^xsd:date ;
  dcterms:source "ISO/TS 19159-1:2014, 4.37" ;
  reg:status reg:statusValid ;
  rdfs:comment "Note 1 to entry: Stray light may be reflected light within a telescope."@en ;
  rdfs:comment "Note 2 to entry:  This definition is valid for the optical portion of the spectrum under observation." ;
  rdfs:label "stray light"@en ;
  skos:changeNote "valid" ;
  skos:editorialNote "preferred"^^xsd:string ;
  skos:notation 1609 ;
  skos:note "Note 1 to entry: Stray light may be reflected light within a telescope."@en ;
  skos:note "Note 2 to entry:  This definition is valid for the optical portion of the spectrum under observation."^^<http://www.w3.org/2001/XMLSchema#@en> ;
  skos:prefLabel "stray light"@en ;
.
<http://iso.org/tc211/term/161>
  rdf:type skos:Concept ;
  dcterms:dateAccepted "2000-12-15"^^xsd:date ;
  dcterms:dateAccepted "2007-06-29"^^xsd:date ;
  dcterms:provenance "KS X ISO 19105" ;
  dcterms:source "ISO 19105:2000" ;
  reg:status reg:statusValid ;
  rdfs:comment "Note 1 to entry: Instantiation of an abstract test case with values."@en ;
  rdfs:comment "비고: 추상 시험 케이스를 값을 통해 실체화 시킴"@kr ;
  rdfs:label "executable test case"@en ;
  skos:changeNote "valid" ;
  skos:definition "특정 요구 사항을 만족하는 구현 시험"@kr ;
  skos:editorialNote "preferred" ;
  skos:editorialNote "preferred"^^xsd:string ;
  skos:notation "161" ;
  skos:notation 161 ;
  skos:note "Note 1 to entry: Instantiation of an abstract test case with values."@en ;
  skos:note "비고: 추상 시험 케이스를 값을 통해 실체화 시킴"@kr ;
  skos:prefLabel "executable test case"@en ;
  skos:prefLabel "실행 가능 시험 케이스"@kr ;
.
<http://iso.org/tc211/term/1610>
  rdf:type skos:Concept ;
  dcterms:dateAccepted "2014-07-15"^^xsd:date ;
  dcterms:source "ISO/TS 19159-1:2014, 4.33" ;
  reg:status reg:statusValid ;
  rdfs:comment "Note 1 to entry:  This distortion is often simply called smile."@en ;
  rdfs:label "smile distortion"@en ;
  skos:changeNote "valid" ;
  skos:editorialNote "preferred"^^xsd:string ;
  skos:notation 1610 ;
  skos:note "Note 1 to entry:  This distortion is often simply called smile."@en ;
  skos:prefLabel "smile distortion"@en ;
.
<http://iso.org/tc211/term/162>
  rdf:type skos:Concept ;
  dcterms:dateAccepted "2000-12-15"^^xsd:date ;
  dcterms:dateAccepted "2007-06-29"^^xsd:date ;
  dcterms:provenance "KS X ISO 19105" ;
  dcterms:source "ISO 19105:2000" ;
  reg:status reg:statusValid ;
  rdfs:label "executable test suite"@en ;
  skos:altLabel "ETS"@kr ;
  skos:altLabel "ETS"^^<http://www.w3.org/2001/XMLSchema#@en> ;
  skos:changeNote "valid" ;
  skos:definition "실행 가능 시험 케이스의 집합"@kr ;
  skos:editorialNote "preferred" ;
  skos:editorialNote "preferred"^^xsd:string ;
  skos:notation "162" ;
  skos:notation 162 ;
  skos:prefLabel "executable test suite"@en ;
  skos:prefLabel "실행 가능 시험 스위트"@kr ;
.
<http://iso.org/tc211/term/163>
  rdf:type skos:Concept ;
  dcterms:dateAccepted "2003-05-01"^^xsd:date ;
  dcterms:dateAccepted "2009-12-29"^^xsd:date ;
  dcterms:provenance "KS X ISO 19107" ;
  dcterms:source "ISO 19107:2003" ;
  reg:status reg:statusValid ;
  rdfs:comment "Note 1 to entry: The concept of exterior is applicable to both topological and geometric complexes."@en ;
  rdfs:comment "비고: 외부의 개념은 위상 복합체와 기하 복합체 모두에 적용 가능하다."@kr ;
  rdfs:label "exterior"@en ;
  skos:changeNote "valid" ;
  skos:definition "전체 집합으로부터 경계 및 내부를 제거한 차집합"@kr ;
  skos:editorialNote "preferred" ;
  skos:editorialNote "preferred"^^xsd:string ;
  skos:notation "163" ;
  skos:notation 163 ;
  skos:note "Note 1 to entry: The concept of exterior is applicable to both topological and geometric complexes."@en ;
  skos:note "비고: 외부의 개념은 위상 복합체와 기하 복합체 모두에 적용 가능하다."@kr ;
  skos:prefLabel "exterior"@en ;
  skos:prefLabel "외부"@kr ;
.
<http://iso.org/tc211/term/164>
  rdf:type skos:Concept ;
  dcterms:dateAccepted "2005-06-01"^^xsd:date ;
  dcterms:dateAccepted "2006-05-01"^^xsd:date ;
  dcterms:source "ISO 19117:2005, 4.5" ;
  reg:status reg:statusRetired ;
  rdfs:comment "Note 1 to entry: The electronic map in a car navigation system has to be displayed so that the up-direction of the map is always in the direction the car is moving. To be able to specify the rotation of the map, the current position of the car must be retrieved continuously from an external position device using an external function."@en ;
  rdfs:comment "비고: 차량 내비게이션 시스템의 전자 지도는 차량의 진행 방향이 항상 지도의 위쪽 방향으로 표시되어야 한다. 지도의 회전을 위하여 차량의 현재 위치는 외부 함수를 사용하는 외부 측위 장치를 통해 지속적으로 갱신되어야 한다."@kr ;
  rdfs:label "external function"@en ;
  skos:changeNote "retired" ;
  skos:definition "응용스키마 내부에 포함되지 않는 함수"@kr ;
  skos:notation "164" ;
  skos:notation 164 ;
  skos:note "Note 1 to entry: The electronic map in a car navigation system has to be displayed so that the up-direction of the map is always in the direction the car is moving. To be able to specify the rotation of the map, the current position of the car must be retrieved continuously from an external position device using an external function."@en ;
  skos:note "비고: 차량 내비게이션 시스템의 전자 지도는 차량의 진행 방향이 항상 지도의 위쪽 방향으로 표시되어야 한다. 지도의 회전을 위하여 차량의 현재 위치는 외부 함수를 사용하는 외부 측위 장치를 통해 지속적으로 갱신되어야 한다."@kr ;
  skos:prefLabel "external function"@en ;
  skos:prefLabel "외부 함수"@kr ;
.
<http://iso.org/tc211/term/1647>
  rdf:type skos:Concept ;
  dcterms:dateAccepted "2014-04-01"^^xsd:date ;
  dcterms:provenance "ISO 19115-1:2014, 4.1" ;
  dcterms:source "ISO 24619:2011, 3.1.16" ;
  reg:status reg:statusValid ;
  rdfs:label "citation"@en ;
  skos:changeNote "valid" ;
  skos:editorialNote "preferred"^^xsd:string ;
  skos:notation 1647 ;
  skos:prefLabel "citation"@en ;
.
<http://iso.org/tc211/term/1649>
  rdf:type skos:Concept ;
  dcterms:dateAccepted "2014-04-01"^^xsd:date ;
  dcterms:source "ISO 19115-1:2014, 4.9" ;
  reg:status reg:statusValid ;
  rdfs:label "lineage"@en ;
  skos:changeNote "valid" ;
  skos:editorialNote "preferred"^^xsd:string ;
  skos:notation 1649 ;
  skos:prefLabel "lineage"@en ;
.
<http://iso.org/tc211/term/165>
  rdf:type skos:Concept ;
  dcterms:dateAccepted "2003-05-01"^^xsd:date ;
  dcterms:dateAccepted "2009-12-29"^^xsd:date ;
  dcterms:provenance "KS X ISO 19107" ;
  dcterms:source "ISO 19107:2003" ;
  reg:status reg:statusValid ;
  rdfs:comment "Note 1 to entry: The geometric realization of a face is a surface. The boundary of a face is the set of directed edges within the same topological complex that are associated to the face via the boundary relations. These can be organized as rings."@en ;
  rdfs:comment "비고: 면의 기하 실현은 표면이다. 면의 경계는 동일한 위상 복합체내에 있는 방향성 변의 집합으로, 경계 관계를 통해 면으로 결합된다. 이것은 링으로 결성된다."@kr ;
  rdfs:label "face"@en ;
  skos:changeNote "valid" ;
  skos:definition "2차원의 위상 원시 객체"@kr ;
  skos:editorialNote "preferred" ;
  skos:editorialNote "preferred"^^xsd:string ;
  skos:notation "165" ;
  skos:notation 165 ;
  skos:note "Note 1 to entry: The geometric realization of a face is a surface. The boundary of a face is the set of directed edges within the same topological complex that are associated to the face via the boundary relations. These can be organized as rings."@en ;
  skos:note "비고: 면의 기하 실현은 표면이다. 면의 경계는 동일한 위상 복합체내에 있는 방향성 변의 집합으로, 경계 관계를 통해 면으로 결합된다. 이것은 링으로 결성된다."@kr ;
  skos:prefLabel "face"@en ;
  skos:prefLabel "면"@kr ;
.
<http://iso.org/tc211/term/1650>
  rdf:type skos:Concept ;
  dcterms:dateAccepted "2013-12-15"^^xsd:date ;
  dcterms:provenance "ISO 19157:2013" ;
  dcterms:source "ISO 19115-1:2014, 4.10" ;
  reg:status reg:statusValid ;
  rdfs:label "metadata"@en ;
  skos:changeNote "valid" ;
  skos:editorialNote "preferred"^^xsd:string ;
  skos:notation 1650 ;
  skos:prefLabel "metadata"@en ;
.
<http://iso.org/tc211/term/166>
  rdf:type skos:Concept ;
  dcterms:dateAccepted "2000-12-15"^^xsd:date ;
  dcterms:dateAccepted "2007-06-29"^^xsd:date ;
  dcterms:provenance "KS X ISO 19105" ;
  dcterms:source "ISO 19105:2000" ;
  reg:status reg:statusValid ;
  rdfs:comment "Note 1 to entry: Non-conformance may be with respect to either the test purpose or at least one of the conformance requirements of the relevant standard(s)."@en ;
  rdfs:comment "비고: 부적합은 시험목적 또는 최소한 관련 표준의 적합성 요구 사항 중 하나와 관련이 있다."@kr ;
  rdfs:label "fail verdict"@en ;
  skos:changeNote "valid" ;
  skos:definition "부적합으로 보고된 시험 판정"@kr ;
  skos:editorialNote "preferred" ;
  skos:editorialNote "preferred"^^xsd:string ;
  skos:notation "166" ;
  skos:notation 166 ;
  skos:note "Note 1 to entry: Non-conformance may be with respect to either the test purpose or at least one of the conformance requirements of the relevant standard(s)."@en ;
  skos:note "비고: 부적합은 시험목적 또는 최소한 관련 표준의 적합성 요구 사항 중 하나와 관련이 있다."@kr ;
  skos:prefLabel "fail verdict"@en ;
  skos:prefLabel "실패 판정"@kr ;
.
<http://iso.org/tc211/term/167>
  rdf:type skos:Concept ;
  dcterms:dateAccepted "2000-12-15"^^xsd:date ;
  dcterms:dateAccepted "2007-06-29"^^xsd:date ;
  dcterms:provenance "KS X ISO 19105" ;
  dcterms:source "ISO 19105:2000" ;
  reg:status reg:statusValid ;
  rdfs:comment "Note 1 to entry: If errors are found, one can correctly deduce that the implementation does not conform to the International Standard; however, the absence of errors does not necessarily imply the converse.  The falsification test can only demonstrate non-conformance"@en ;
  rdfs:comment "비고: 오류가 발견되면, 표준에 맞게 구현되었는지 정확히 추론할 수 있다. 그러나 에러가 발견되지 않는 경우가 반드시 그 반대의 경우를 의미하는 것은 아니다. 반증 시험은 부적합 여부만을 판별할 수 있다. 검증 시험과 비교하라. 대부분의 경우 기술 및 경제적 문제로 인해 반증 시험이 적합성 시험에 사용된다."@kr ;
  rdfs:label "falsification test"@en ;
  skos:changeNote "valid" ;
  skos:definition "구현 결과물에 대한 오류를 찾기 위한 시험"@kr ;
  skos:editorialNote "preferred" ;
  skos:editorialNote "preferred"^^xsd:string ;
  skos:notation "167" ;
  skos:notation 167 ;
  skos:note "Note 1 to entry: If errors are found, one can correctly deduce that the implementation does not conform to the International Standard; however, the absence of errors does not necessarily imply the converse.  The falsification test can only demonstrate non-conformance"@en ;
  skos:note "비고: 오류가 발견되면, 표준에 맞게 구현되었는지 정확히 추론할 수 있다. 그러나 에러가 발견되지 않는 경우가 반드시 그 반대의 경우를 의미하는 것은 아니다. 반증 시험은 부적합 여부만을 판별할 수 있다. 검증 시험과 비교하라. 대부분의 경우 기술 및 경제적 문제로 인해 반증 시험이 적합성 시험에 사용된다."@kr ;
  skos:prefLabel "falsification test"@en ;
  skos:prefLabel "오류 검증 시험"@kr ;
.
<http://iso.org/tc211/term/1675>
  rdf:type skos:Concept ;
  dcterms:dateAccepted "2014-01-15"^^xsd:date ;
  dcterms:source "ISO/TS 19130-2:2014, 4.26" ;
  reg:status reg:statusValid ;
  rdfs:comment "Note 1 to entry:  Geographic coordinates are related to a coordinate reference system or compound coordinate reference system. Depth equals negative height"@en ;
  rdfs:label "geographic coordinates"@en ;
  skos:changeNote "valid" ;
  skos:editorialNote "preferred"^^xsd:string ;
  skos:notation 1675 ;
  skos:note "Note 1 to entry:  Geographic coordinates are related to a coordinate reference system or compound coordinate reference system. Depth equals negative height"@en ;
  skos:prefLabel "geographic coordinates"@en ;
.
<http://iso.org/tc211/term/1676>
  rdf:type skos:Concept ;
  dcterms:dateAccepted "2014-01-15"^^xsd:date ;
  dcterms:source "ISO/TS 19130-2:2014, 4.40" ;
  reg:status reg:statusValid ;
  rdfs:comment "Note 1 to entry:  Time of flight (TOF) LIDARs use short laser pulses and precisely record the time each laser pulse was emitted and the time each reflected return(s) is received in order to calculate the distance(s) to the scatterer(s) encountered by the emitted pulse. For topographic LIDAR, these time-of-flight measurements are then combined with precise platform location/attitude data along with pointing data to produce a three-dimensional product of the illuminated scene of interest."@en ;
  rdfs:label "lidar"@en ;
  rdfs:seeAlso "Light Detection and Ranging" ;
  skos:altLabel "Light Detection and Ranging"@en ;
  skos:changeNote "valid" ;
  skos:editorialNote "preferred"^^xsd:string ;
  skos:notation 1676 ;
  skos:note "Note 1 to entry:  Time of flight (TOF) LIDARs use short laser pulses and precisely record the time each laser pulse was emitted and the time each reflected return(s) is received in order to calculate the distance(s) to the scatterer(s) encountered by the emitted pulse. For topographic LIDAR, these time-of-flight measurements are then combined with precise platform location/attitude data along with pointing data to produce a three-dimensional product of the illuminated scene of interest."@en ;
  skos:prefLabel "lidar"@en ;
.
<http://iso.org/tc211/term/1677>
  rdf:type skos:Concept ;
  dcterms:dateAccepted "2014-01-15"^^xsd:date ;
  dcterms:source "ISO/TS 19130-2:2014, 4.72" ;
  reg:status reg:statusValid ;
  rdfs:label "SONAR"@en ;
  rdfs:seeAlso "Sound Navigation and Ranging" ;
  skos:altLabel "Sound Navigation and Ranging"@en ;
  skos:changeNote "valid" ;
  skos:editorialNote "preferred"^^xsd:string ;
  skos:notation 1677 ;
  skos:prefLabel "SONAR"@en ;
.
<http://iso.org/tc211/term/1678>
  rdf:type skos:Concept ;
  dcterms:dateAccepted "2014-11-01"^^xsd:date ;
  dcterms:provenance "ISO 19101-1:2014, 4.1.25" ;
  dcterms:source "ISO/TR 19120:2001, 3.3" ;
  reg:status reg:statusValid ;
  rdfs:label "module"@en ;
  skos:changeNote "valid" ;
  skos:editorialNote "preferred"^^xsd:string ;
  skos:notation 1678 ;
  skos:prefLabel "module"@en ;
.
<http://iso.org/tc211/term/168>
  rdf:type skos:Concept ;
  dcterms:dateAccepted "2002-07-01"^^xsd:date ;
  dcterms:dateAccepted "2008-12-30"^^xsd:date ;
  dcterms:provenance "ISO 19101:2002" ;
  dcterms:source "ISO 19101-1:2014, 4.1.11" ;
  reg:status reg:statusValid ;
  rdfs:comment "Note 1 to entry: A feature may occur as a type or an instance.  Feature type or feature instance shall be used when only one is meant."@en ;
  rdfs:comment "비고: 피처는 유형이나 인스턴스로 나타난다. 피처 유형 및 피처 인스턴스는 단 한 가지의 의미를 갖도록 사용해야 한다."@kr ;
  rdfs:label "feature"@en ;
  skos:changeNote "valid" ;
  skos:definition "실세계 현상의 추상화"@kr ;
  skos:editorialNote "preferred" ;
  skos:editorialNote "preferred"^^xsd:string ;
  skos:notation "168" ;
  skos:notation 168 ;
  skos:note "Note 1 to entry: A feature may occur as a type or an instance.  Feature type or feature instance shall be used when only one is meant."@en ;
  skos:note "비고: 피처는 유형이나 인스턴스로 나타난다. 피처 유형 및 피처 인스턴스는 단 한 가지의 의미를 갖도록 사용해야 한다."@kr ;
  skos:prefLabel "feature"@en ;
  skos:prefLabel "지형지물"@kr ;
.
<http://iso.org/tc211/term/169>
  rdf:type skos:Concept ;
  dcterms:dateAccepted "2005-02-15"^^xsd:date ;
  dcterms:dateAccepted "2009-12-30"^^xsd:date ;
  dcterms:provenance "KS X ISO 19110" ;
  dcterms:source "ISO 19110:2005" ;
  reg:status reg:statusValid ;
  rdfs:label "feature association"@en ;
  skos:changeNote "valid" ;
  skos:definition "동일하거나 혹은 서로 다른 피처 유형을 갖는 인스턴스들 간의 연관 관계"@kr ;
  skos:editorialNote "preferred" ;
  skos:editorialNote "preferred"^^xsd:string ;
  skos:notation "169" ;
  skos:notation 169 ;
  skos:prefLabel "feature association"@en ;
  skos:prefLabel "지형지물 연관"@kr ;
.
<http://iso.org/tc211/term/17>
  rdf:type skos:Concept ;
  dcterms:dateAccepted "2005-07-15"^^xsd:date ;
  dcterms:dateAccepted "2009-12-29"^^xsd:date ;
  dcterms:provenance "ISO/TS 19103:2005 ,4.2.3" ;
  dcterms:source "ISO/IEC 19501" ;
  reg:status reg:statusValid ;
  rdfs:comment "Note 1 to entry: A binary association is an association among exactly two classifiers (including the possibility of an association from a classifier to itself)."@en ;
  rdfs:comment "비고: 이진 연관 관계는 정확하게 두 분류자 간의 연관 관계이다."@kr ;
  rdfs:label "association <UML>"@en ;
  skos:changeNote "valid" ;
  skos:definition "인스턴스간의 연결을 규정하는 두 개 이상 분류자 간의 의미론적 관계"@kr ;
  skos:editorialNote "preferred" ;
  skos:editorialNote "preferred"^^xsd:string ;
  skos:notation "17" ;
  skos:notation 17 ;
  skos:note "Note 1 to entry: A binary association is an association among exactly two classifiers (including the possibility of an association from a classifier to itself)."@en ;
  skos:note "비고: 이진 연관 관계는 정확하게 두 분류자 간의 연관 관계이다."@kr ;
  skos:prefLabel "association <UML>"@en ;
  skos:prefLabel "연관 <UML>"@kr ;
.
<http://iso.org/tc211/term/170>
  rdf:type skos:Concept ;
  dcterms:dateAccepted "2002-07-01" ;
  dcterms:dateAccepted "2002-07-01"^^xsd:date ;
  dcterms:dateAccepted "2008-12-30"^^xsd:date ;
  dcterms:provenance "ISO 19101:2002" ;
  dcterms:source "ISO 19101-1:2014, 4.1.12" ;
  reg:status reg:statusAccepted ;
  reg:status reg:statusValid ;
  rdfs:comment "NOTE 1 A feature attribute has a name, a data type, and a value domain associated to it.  A feature attribute for a feature instance also has an attribute value taken from the value domain."@en ;
  rdfs:comment "NOTE 2 In a feature catalogue, a feature attribute may include a value domain but does not specify attribute values for feature instances."@en ;
  rdfs:comment "Note 1 to entry: A feature attribute has a name, a data type, and a value domain associated to it.  A feature attribute for a feature instance also has an attribute value taken from the value domain."@en ;
  rdfs:comment "Note 2 to entry: In a feature catalogue, a feature attribute may include a value domain but does not specify attribute values for feature instances." ;
  rdfs:comment "Soms 'object attribuut' genoemd"@en ;
  rdfs:comment "비고 1: 피처 속성은 명칭, 데이터 유형, 관련된 영역의 데이터 유형을 갖는다.  피처 인스턴스를 위한 피처속성 또한 값 영역으로부터의 속성 값을 갖는다. "@kr ;
  rdfs:label "feature attribute"@en ;
  skos:changeNote "valid" ;
  skos:definition "kenmerk van een geo-object"@nl ;
  skos:definition "피처의 특징"@kr ;
  skos:editorialNote "preferred" ;
  skos:editorialNote "preferred"^^xsd:string ;
  skos:notation "170" ;
  skos:notation 170 ;
  skos:note "NOTE 1 A feature attribute has a name, a data type, and a value domain associated to it.  A feature attribute for a feature instance also has an attribute value taken from the value domain."@en ;
  skos:note "NOTE 2 In a feature catalogue, a feature attribute may include a value domain but does not specify attribute values for feature instances."^^<http://www.w3.org/2001/XMLSchema#@en> ;
  skos:note "Note 1 to entry: A feature attribute has a name, a data type, and a value domain associated to it.  A feature attribute for a feature instance also has an attribute value taken from the value domain."@en ;
  skos:note "Note 2 to entry: In a feature catalogue, a feature attribute may include a value domain but does not specify attribute values for feature instances."^^<http://www.w3.org/2001/XMLSchema#@en> ;
  skos:note "Soms 'object attribuut' genoemd"@en ;
  skos:note "비고 1: 피처 속성은 명칭, 데이터 유형, 관련된 영역의 데이터 유형을 갖는다.  피처 인스턴스를 위한 피처속성 또한 값 영역으로부터의 속성 값을 갖는다. "@kr ;
  skos:note "비고 2: 지형지물 목록에서, 피처 속성은 값 영역을 포함하나 피처 인스턴스에 대한 속성값을 구체적으로 정의하지는 않는다."@kr ;
  skos:prefLabel "attribuut"@nl ;
  skos:prefLabel "feature attribute"@en ;
  skos:prefLabel "지형지물 속성"@kr ;
.
<http://iso.org/tc211/term/174>
  rdf:type skos:Concept ;
  dcterms:dateAccepted "2002-09-01"^^xsd:date ;
  dcterms:dateAccepted "2007-11-01"^^xsd:date ;
  dcterms:provenance "KS X ISO 19108" ;
  dcterms:source "ISO 19108;2002" ;
  reg:status reg:statusValid ;
  rdfs:label "feature division"@en ;
  skos:changeNote "valid" ;
  skos:definition "기존의 피처가 동일한 피처 유형의 별개 피처 인스턴스들로 대체되는 피처 갱신"@kr ;
  skos:editorialNote "preferred" ;
  skos:editorialNote "preferred"^^xsd:string ;
  skos:notation "174" ;
  skos:notation 174 ;
  skos:prefLabel "feature division"@en ;
  skos:prefLabel "지형지물 분할"@kr ;
.
<http://iso.org/tc211/term/175>
  rdf:type skos:Concept ;
  dcterms:dateAccepted "2002-09-01"^^xsd:date ;
  dcterms:dateAccepted "2007-11-01"^^xsd:date ;
  dcterms:provenance "KS X ISO 19108" ;
  dcterms:source "ISO 19108;2002" ;
  reg:status reg:statusValid ;
  rdfs:label "feature fusion"@en ;
  skos:changeNote "valid" ;
  skos:definition "2개 이상의 기존 피처 인스턴스가 동일한 피처 유형의 단일 인스턴스로 대체되는 피처 갱신"@kr ;
  skos:editorialNote "preferred" ;
  skos:editorialNote "preferred"^^xsd:string ;
  skos:notation "175" ;
  skos:notation 175 ;
  skos:prefLabel "feature fusion"@en ;
  skos:prefLabel "지형지물 융합"@kr ;
.
<http://iso.org/tc211/term/1762>
  rdf:type skos:Concept ;
  dcterms:dateAccepted "2014-04-01"^^xsd:date ;
  dcterms:source "ISO 19115-1:2014, 4.6" ;
  reg:status reg:statusValid ;
  rdfs:label "free text"@en ;
  skos:changeNote "valid" ;
  skos:editorialNote "preferred"^^xsd:string ;
  skos:notation 1762 ;
  skos:prefLabel "free text"@en ;
.
<http://iso.org/tc211/term/177>
  rdf:type skos:Concept ;
  dcterms:dateAccepted "2002-07-01"^^xsd:date ;
  dcterms:dateAccepted "2009-12-30"^^xsd:date ;
  dcterms:provenance "ISO 19101:2002" ;
  dcterms:provenance "KS X ISO 19110" ;
  dcterms:source "ISO 19110:2005" ;
  reg:status reg:statusValid ;
  rdfs:comment "Note 1 to entry: Sometimes feature operations provide a basis for feature type definition."@en ;
  rdfs:comment "비고: 종종 피처 연산은 피처 유형의 정의를 위한 기초를 제공한다."@kr ;
  rdfs:label "feature operation"@en ;
  skos:changeNote "valid" ;
  skos:definition "피처 유형에 해당하는 모든 인스턴스에서 실행 가능한 연산"@kr ;
  skos:editorialNote "preferred" ;
  skos:editorialNote "preferred"^^xsd:string ;
  skos:notation "177" ;
  skos:notation 177 ;
  skos:note "Note 1 to entry: Sometimes feature operations provide a basis for feature type definition."@en ;
  skos:note "비고: 종종 피처 연산은 피처 유형의 정의를 위한 기초를 제공한다."@kr ;
  skos:prefLabel "feature operation"@en ;
  skos:prefLabel "지형지물 연산"@kr ;
.
<http://iso.org/tc211/term/178>
  rdf:type skos:Concept ;
  dcterms:dateAccepted "2005-06-01"^^xsd:date ;
  dcterms:dateAccepted "2006-05-01"^^xsd:date ;
  dcterms:source "ISO 19117:2005, 4.8" ;
  reg:status reg:statusRetired ;
  rdfs:label "feature portrayal rule set"@en ;
  skos:changeNote "retired" ;
  skos:definition "피처 인스턴스에 적용 가능한 묘화 규칙들의 모음"@kr ;
  skos:notation "178" ;
  skos:notation 178 ;
  skos:prefLabel "feature portrayal rule set"@en ;
  skos:prefLabel "지형지물 묘화규칙 집합"@kr ;
.
<http://iso.org/tc211/term/18>
  rdf:type skos:Concept ;
  dcterms:dateAccepted "2004-07-01"^^xsd:date ;
  dcterms:dateAccepted "2004-11-05"^^xsd:date ;
  dcterms:provenance "KS X ISO 19116" ;
  dcterms:source "ISO 19116:2004" ;
  reg:status reg:statusValid ;
  rdfs:comment "Note 1 to entry: In positioning services, this is usually the orientation of the user's platform, such as an aircraft, boat, or automobile."@en ;
  rdfs:comment "비고: 측위 서비스의 경우, 보통 항공기, 배, 자동차 등 사용자 플랫폼의 방향을 의미한다."@kr ;
  rdfs:label "attitude"@en ;
  skos:changeNote "valid" ;
  skos:definition "물체의 좌표 체계 축과 외부 좌표 체계 축 사이의 각도를 통해 기술되는 물체의 방향"@kr ;
  skos:editorialNote "preferred" ;
  skos:editorialNote "preferred"^^xsd:string ;
  skos:notation "18" ;
  skos:notation 18 ;
  skos:note "Note 1 to entry: In positioning services, this is usually the orientation of the user's platform, such as an aircraft, boat, or automobile."@en ;
  skos:note "비고: 측위 서비스의 경우, 보통 항공기, 배, 자동차 등 사용자 플랫폼의 방향을 의미한다."@kr ;
  skos:prefLabel "attitude"@en ;
  skos:prefLabel "자세"@kr ;
.
<http://iso.org/tc211/term/180>
  rdf:type skos:Concept ;
  dcterms:dateAccepted "2002-09-01"^^xsd:date ;
  dcterms:dateAccepted "2007-11-01"^^xsd:date ;
  dcterms:provenance "KS X ISO 19108" ;
  dcterms:source "ISO 19108;2002" ;
  reg:status reg:statusValid ;
  rdfs:label "feature substitution"@en ;
  skos:changeNote "valid" ;
  skos:definition "하나의 피처 인스턴스가 동일한 피처 유형 또는 다른 피처유형을 갖는 인스턴스로 바뀌는 피처 갱신"@kr ;
  skos:editorialNote "preferred" ;
  skos:editorialNote "preferred"^^xsd:string ;
  skos:notation "180" ;
  skos:notation 180 ;
  skos:prefLabel "feature substitution"@en ;
  skos:prefLabel "지형지물 치환"@kr ;
.
<http://iso.org/tc211/term/181>
  rdf:type skos:Concept ;
  dcterms:dateAccepted "2002-09-01"^^xsd:date ;
  dcterms:dateAccepted "2007-11-01"^^xsd:date ;
  dcterms:provenance "KS X ISO 19108" ;
  dcterms:source "ISO 19108;2002" ;
  reg:status reg:statusValid ;
  rdfs:label "feature succession"@en ;
  skos:changeNote "valid" ;
  skos:definition "하나 이상의 피처 인스턴스가 다른 피처 인스턴스로 대체되어, 앞선 피처 인스턴스가 없어짐"@kr ;
  skos:editorialNote "preferred" ;
  skos:editorialNote "preferred"^^xsd:string ;
  skos:notation "181" ;
  skos:notation 181 ;
  skos:prefLabel "feature succession"@en ;
  skos:prefLabel "지형지물 갱신"@kr ;
.
<http://iso.org/tc211/term/182>
  rdf:type skos:Concept ;
  dcterms:dateAccepted "2004-08-01"^^xsd:date ;
  dcterms:dateAccepted "2009-12-29"^^xsd:date ;
  dcterms:provenance "KS X ISO 19125-2" ;
  dcterms:source "ISO 19125-2:2004" ;
  reg:status reg:statusValid ;
  rdfs:label "feature table"@en ;
  skos:changeNote "valid" ;
  skos:definition "행은 피처 속성을 나타내고, 열은 피처를 나타내는 테이블"@kr ;
  skos:editorialNote "preferred" ;
  skos:editorialNote "preferred"^^xsd:string ;
  skos:notation "182" ;
  skos:notation 182 ;
  skos:prefLabel "feature table"@en ;
  skos:prefLabel "지형지물 테이블"@kr ;
.
<http://iso.org/tc211/term/186>
  rdf:type skos:Concept ;
  dcterms:dateAccepted "2005-07-15"^^xsd:date ;
  dcterms:dateAccepted "2008-12-19"^^xsd:date ;
  dcterms:provenance "ISO 19118:2011 ,4.17" ;
  dcterms:source "ISO/IEC 2382-1:1993" ;
  reg:status reg:statusValid ;
  rdfs:label "file"@en ;
  skos:changeNote "valid" ;
  skos:definition "기억 또는 처리를 위해 명명된 레코드 집합의 단위"@kr ;
  skos:editorialNote "preferred" ;
  skos:editorialNote "preferred"^^xsd:string ;
  skos:notation "186" ;
  skos:notation 186 ;
  skos:prefLabel "file"@en ;
  skos:prefLabel "파일"@kr ;
.
<http://iso.org/tc211/term/187>
  rdf:type skos:Concept ;
  dcterms:dateAccepted "2003-02-15" ;
  dcterms:dateAccepted "2003-02-15"^^xsd:date ;
  dcterms:dateAccepted "2007-11-01"^^xsd:date ;
  dcterms:provenance "ISO 19111:2003" ;
  dcterms:provenance "KS X ISO 19111" ;
  dcterms:source "ISO 19111:2007" ;
  reg:status reg:statusAccepted ;
  reg:status reg:statusValid ;
  rdfs:comment "Note 1 to entry: Sometimes inverse flattening 1/f = a/(a-b) is given instead; 1/f is also known as reciprocal flattening."@en ;
  rdfs:comment "OPMERKING Soms wordt de inverse afplatting 1/f = a/(a-b) gegeven; 1/f wordt ook wel de inverse afplatting genoemd."@en ;
  rdfs:comment "비고: 종종 역편평률 1/f=a/(a-b)이 대신한다.  1/f는 역편평률로 알려져 있다."@kr ;
  rdfs:label "flattening"@en ;
  skos:altLabel "f"@kr ;
  skos:altLabel "f"@nl ;
  skos:altLabel "f"^^<http://www.w3.org/2001/XMLSchema#@en> ;
  skos:changeNote "valid" ;
  skos:definition "verhouding van het verschil tussen de halve lange (a) en de halve korte (b) as van een ellipsoïde ten opzichte van de halve lange as; f = (a - b)/a"@nl ;
  skos:definition "타원체의 장반경(a)과 단반경과(b)의 차이를 장반경으로 나눈 값; f=(a-b)/a"@kr ;
  skos:editorialNote "preferred" ;
  skos:editorialNote "preferred"^^xsd:string ;
  skos:notation "187" ;
  skos:notation 187 ;
  skos:note "Note 1 to entry: Sometimes inverse flattening 1/f = a/(a-b) is given instead; 1/f is also known as reciprocal flattening."@en ;
  skos:note "OPMERKING Soms wordt de inverse afplatting 1/f = a/(a-b) gegeven; 1/f wordt ook wel de inverse afplatting genoemd."@en ;
  skos:note "비고: 종종 역편평률 1/f=a/(a-b)이 대신한다.  1/f는 역편평률로 알려져 있다."@kr ;
  skos:prefLabel "afplatting"@nl ;
  skos:prefLabel "flattening"@en ;
  skos:prefLabel "편평률"@kr ;
.
<http://iso.org/tc211/term/188>
  rdf:type skos:Concept ;
  dcterms:dateAccepted "2009-04-01"^^xsd:date ;
  dcterms:source "ISO/TS 19129:2009" ;
  reg:status reg:statusValid ;
  rdfs:label "framework"@en ;
  skos:changeNote "valid" ;
  skos:editorialNote "preferred"^^xsd:string ;
  skos:notation 188 ;
  skos:prefLabel "framework"@en ;
.
<http://iso.org/tc211/term/189>
  rdf:type skos:Concept ;
  dcterms:dateAccepted "2003/08/15"^^xsd:date ;
  dcterms:dateAccepted "2009-12-29"^^xsd:date ;
  dcterms:source "ISO 19114:2003, 4.5" ;
  reg:status reg:statusRetired ;
  rdfs:comment "Note 1 to entry: Full inspection is also known as 100% inspection."@en ;
  rdfs:comment "비고: 전수 검사는 100% 검사로 알려져 있다."@kr ;
  rdfs:label "full inspection"@en ;
  skos:changeNote "retired" ;
  skos:definition "데이터셋 내의 모든 항목에 대한 검사"@kr ;
  skos:notation "189" ;
  skos:notation 189 ;
  skos:note "Note 1 to entry: Full inspection is also known as 100% inspection."@en ;
  skos:note "비고: 전수 검사는 100% 검사로 알려져 있다."@kr ;
  skos:prefLabel "full inspection"@en ;
  skos:prefLabel "전수 검사"@kr ;
.
<http://iso.org/tc211/term/19>
  rdf:type skos:Concept ;
  dcterms:dateAccepted "2009-02-15" ;
  dcterms:dateAccepted "2009-02-15"^^xsd:date ;
  dcterms:provenance "ISO 19115-2:2009" ;
  dcterms:provenance "NEN 3610" ;
  dcterms:source "ISO/IEC 2382-17:1999" ;
  reg:status reg:statusAccepted ;
  reg:status reg:statusValid ;
  rdfs:comment "NOTE Describes a geometrical, topological, thematic, or other characteristic of an entity"@en ;
  rdfs:comment "Note 1 to entry: Describes a geometrical, topological, thematic, or other characteristic of an entity"@en ;
  rdfs:label "attribute"@en ;
  skos:changeNote "valid" ;
  skos:definition "kenmerk van een geo-object"@nl ;
  skos:editorialNote "preferred" ;
  skos:editorialNote "preferred"^^xsd:string ;
  skos:notation "19" ;
  skos:notation 19 ;
  skos:note "NOTE Describes a geometrical, topological, thematic, or other characteristic of an entity"@en ;
  skos:note "Note 1 to entry: Describes a geometrical, topological, thematic, or other characteristic of an entity"@en ;
  skos:prefLabel "attribute"@en ;
  skos:prefLabel "attribuut"@nl ;
.
<http://iso.org/tc211/term/190>
  rdf:type skos:Concept ;
  dcterms:dateAccepted "2003-05-01"^^xsd:date ;
  dcterms:dateAccepted "2009-12-29"^^xsd:date ;
  dcterms:provenance "KS X ISO 19107" ;
  dcterms:source "ISO 19107:2003" ;
  reg:status reg:statusValid ;
  rdfs:label "function"@en ;
  skos:changeNote "valid" ;
  skos:definition "한 개 영역(소스 또는 함수의 영역)에서 각각의 요소를 다른 영역(대상, 공동영역 또는 범위)의 유일한 요소로 연관시키는 규칙"@kr ;
  skos:editorialNote "preferred" ;
  skos:editorialNote "preferred"^^xsd:string ;
  skos:notation "190" ;
  skos:notation 190 ;
  skos:prefLabel "function"@en ;
  skos:prefLabel "함수"@kr ;
.
<http://iso.org/tc211/term/191>
  rdf:type skos:Concept ;
  dcterms:dateAccepted "2005-02-15"^^xsd:date ;
  dcterms:dateAccepted "2009-12-30"^^xsd:date ;
  dcterms:provenance "KS X ISO 19110" ;
  dcterms:source "ISO 19110:2005" ;
  reg:status reg:statusValid ;
  rdfs:comment "Note 1 to entry: In a functional language, feature types may be represented as abstract data types."@en ;
  rdfs:comment "비고: 함수 언어에서 피처 유형은 추상 데이터 유형으로 표현될 수 있다."@kr ;
  rdfs:label "functional language"@en ;
  skos:changeNote "valid" ;
  skos:definition "피처 연산을 기술하는데 사용되는 언어"@kr ;
  skos:editorialNote "preferred" ;
  skos:editorialNote "preferred"^^xsd:string ;
  skos:notation "191" ;
  skos:notation 191 ;
  skos:note "Note 1 to entry: In a functional language, feature types may be represented as abstract data types."@en ;
  skos:note "비고: 함수 언어에서 피처 유형은 추상 데이터 유형으로 표현될 수 있다."@kr ;
  skos:prefLabel "functional language"@en ;
  skos:prefLabel "함수 언어"@kr ;
.
<http://iso.org/tc211/term/192>
  rdf:type skos:Concept ;
  dcterms:dateAccepted "2002-07-01"^^xsd:date ;
  dcterms:dateAccepted "2008-12-30"^^xsd:date ;
  dcterms:provenance "ISO 19101:2002" ;
  dcterms:source "ISO 19101-1:2014, 4.1.17" ;
  reg:status reg:statusValid ;
  rdfs:comment "Note 1 to entry: GDF, S-57, and DIGEST are examples of functional standards."@en ;
  rdfs:comment "비고: GDF, S-57, DIGEST가 사실상 표준의 보기이다.  "@kr ;
  rdfs:label "functional standard"@en ;
  skos:changeNote "valid" ;
  skos:definition "국제적 데이터 생산자나 데이터 사용자 커뮤니티가 현재 사용하고 있는 지리 정보 표준"@kr ;
  skos:editorialNote "preferred" ;
  skos:editorialNote "preferred"^^xsd:string ;
  skos:notation "192" ;
  skos:notation 192 ;
  skos:note "Note 1 to entry: GDF, S-57, and DIGEST are examples of functional standards."@en ;
  skos:note "비고: GDF, S-57, DIGEST가 사실상 표준의 보기이다.  "@kr ;
  skos:prefLabel "functional standard"@en ;
  skos:prefLabel "사실상 표준"@kr ;
.
<http://iso.org/tc211/term/193>
  rdf:type skos:Concept ;
  dcterms:dateAccepted "2003-10-15"^^xsd:date ;
  dcterms:dateAccepted "2009-12-29"^^xsd:date ;
  dcterms:provenance "KS X ISO 19112" ;
  dcterms:source "ISO 19112:2003" ;
  reg:status reg:statusValid ;
  rdfs:comment "Note 1 to entry: The positional information need not be coordinates, but could be descriptive."@en ;
  rdfs:comment "비고: 위치 정보에는 좌표뿐만 아니라 위치에 대한 간접적인 서술 또한 포함된다."@kr ;
  rdfs:label "gazetteer"@en ;
  skos:changeNote "valid" ;
  skos:definition "위치에 대한 정보를  담고 있는 클래스 또는 피처 클래스 인스턴스의 사전"@kr ;
  skos:editorialNote "preferred" ;
  skos:editorialNote "preferred"^^xsd:string ;
  skos:notation "193" ;
  skos:notation 193 ;
  skos:note "Note 1 to entry: The positional information need not be coordinates, but could be descriptive."@en ;
  skos:note "비고: 위치 정보에는 좌표뿐만 아니라 위치에 대한 간접적인 서술 또한 포함된다."@kr ;
  skos:prefLabel "gazetteer"@en ;
  skos:prefLabel "지명 색인"@kr ;
.
<http://iso.org/tc211/term/195>
  rdf:type skos:Concept ;
  dcterms:dateAccepted "2005-10-15"^^xsd:date ;
  dcterms:dateAccepted "2006-12-01"^^xsd:date ;
  dcterms:provenance "KS X ISO 19133" ;
  dcterms:source "ISO 19133:2005" ;
  reg:status reg:statusValid ;
  rdfs:comment "Note 1 to entry: Geocoding usually refers to the translation of \"address\" or \"intersection\" to \"direct position.\" Many services providers also include a \"reverse geocoding\" interface to their geocoder, thus extending the definition of the service as a general translator of location. Because routing services use internal location encodings not usually available to others, a geocoder is an integral part of the internals of such a service."@en ;
  rdfs:comment "비고: 일반적으로 지오코딩은 \"주소\"나 \"교차로\"와 같은 \"간접 위치\"를 \"직접 위치\"로 변환하는 것을 지칭한다. 다수의 서비스 제공자는 자신들의 지오코더에 \"역(逆) 지오코딩\" 인터페이스를 포함하고 있으며, 이로 인해 일반적인 위치 변환 서비스의 정의가 확장되었다. 라우팅 서비스는 일반적으로 내부의 위치 부호화를 사용하기 때문에 지오코더는 필수 요소 중 하나이다. "@kr ;
  rdfs:label "geocoding"@en ;
  skos:changeNote "valid" ;
  skos:definition "위치의 한 형태를 다른 형태로 변환"@kr ;
  skos:editorialNote "preferred" ;
  skos:editorialNote "preferred"^^xsd:string ;
  skos:notation "195" ;
  skos:notation 195 ;
  skos:note "Note 1 to entry: Geocoding usually refers to the translation of \"address\" or \"intersection\" to \"direct position.\" Many services providers also include a \"reverse geocoding\" interface to their geocoder, thus extending the definition of the service as a general translator of location. Because routing services use internal location encodings not usually available to others, a geocoder is an integral part of the internals of such a service."@en ;
  skos:note "비고: 일반적으로 지오코딩은 \"주소\"나 \"교차로\"와 같은 \"간접 위치\"를 \"직접 위치\"로 변환하는 것을 지칭한다. 다수의 서비스 제공자는 자신들의 지오코더에 \"역(逆) 지오코딩\" 인터페이스를 포함하고 있으며, 이로 인해 일반적인 위치 변환 서비스의 정의가 확장되었다. 라우팅 서비스는 일반적으로 내부의 위치 부호화를 사용하기 때문에 지오코더는 필수 요소 중 하나이다. "@kr ;
  skos:prefLabel "geocoding"@en ;
  skos:prefLabel "지오코딩"@kr ;
.
<http://iso.org/tc211/term/196>
  rdf:type skos:Concept ;
  dcterms:dateAccepted "2003-02-15" ;
  dcterms:dateAccepted "2003-02-15"^^xsd:date ;
  dcterms:dateAccepted "2007-11-01"^^xsd:date ;
  dcterms:provenance "ISO 19111:2003" ;
  dcterms:provenance "KS X ISO 19111" ;
  dcterms:source "ISO 19111:2007" ;
  reg:status reg:statusAccepted ;
  reg:status reg:statusValid ;
  rdfs:label "geodetic coordinate system"@en ;
  rdfs:seeAlso "ellipsoidal coordinate system" ;
  rdfs:seeAlso "ellipsoidal coordinate system"@nl ;
  skos:altLabel "ellipsoidal coordinate system"@en ;
  skos:altLabel "ellipsoidal coordinate system"@nl ;
  skos:changeNote "valid" ;
  skos:definition "coördinaatsysteem waarbij de positie wordt bepaald door geodetische lengte, geodetische breedte en (in het driedimensionale geval) ellipsoïde hoogte"@nl ;
  skos:definition "측지 위도 및 측지 경도(3차원의 경우는 타원체고)에 의해서 위치를 기술하는 좌표 체계"@kr ;
  skos:editorialNote "admitted" ;
  skos:editorialNote "admitted"^^xsd:string ;
  skos:notation "196" ;
  skos:notation 196 ;
  skos:prefLabel "geodetic coordinate system"@en ;
  skos:prefLabel "geodetisch coördinaatsysteem"@nl ;
  skos:prefLabel "측지 좌표계"@kr ;
.
<http://iso.org/tc211/term/199>
  rdf:type skos:Concept ;
  dcterms:dateAccepted "2003-02-15" ;
  dcterms:dateAccepted "2003-02-15"^^xsd:date ;
  dcterms:dateAccepted "2007-11-01"^^xsd:date ;
  dcterms:provenance "ISO 19111:2003" ;
  dcterms:provenance "KS X ISO 19111" ;
  dcterms:source "ISO 19111:2007" ;
  reg:status reg:statusAccepted ;
  reg:status reg:statusValid ;
  rdfs:comment "Note 1 to entry: Only used as part of a three-dimensional ellipsoidal coordinate system and never on its own."@en ;
  rdfs:comment "OPMERKING Wordt alleen gebruikt als deel van een driedimensionaal ellipsoidaal coördinaatsysteem en nooit op zichzelf staand."@en ;
  rdfs:comment "비고: 3차원 타원체 좌표계의 일부로 사용되며, 독립적으로 사용되지 않는다."@kr ;
  rdfs:label "geodetic height"@en ;
  rdfs:seeAlso "ellipsoidal height" ;
  rdfs:seeAlso "ellipsoïde hoogte"@nl ;
  skos:altLabel "ellipsoidal height"@en ;
  skos:altLabel "ellipsoïde hoogte"@nl ;
  skos:altLabel "h"@kr ;
  skos:altLabel "h"@nl ;
  skos:altLabel "h"^^<http://www.w3.org/2001/XMLSchema#@en> ;
  skos:changeNote "valid" ;
  skos:definition "afstand van een punt tot de ellipsoïde gemeten langs een lijn loodrecht op de ellipsoïde positief indien naar boven of naar de buitenzijde van de ellipsoïde"@nl ;
  skos:definition "타원체에서 임의의 한 점까지 법선을 따라 측정된 거리. 타원체에서 위쪽 방향 또는 타원체 외부이면 양의 값을 갖는다."@kr ;
  skos:editorialNote "admitted" ;
  skos:editorialNote "admitted"^^xsd:string ;
  skos:notation "199" ;
  skos:notation 199 ;
  skos:note "Note 1 to entry: Only used as part of a three-dimensional ellipsoidal coordinate system and never on its own."@en ;
  skos:note "OPMERKING Wordt alleen gebruikt als deel van een driedimensionaal ellipsoidaal coördinaatsysteem en nooit op zichzelf staand."@en ;
  skos:note "비고: 3차원 타원체 좌표계의 일부로 사용되며, 독립적으로 사용되지 않는다."@kr ;
  skos:prefLabel "geodetic height"@en ;
  skos:prefLabel "geodetische hoogte"@nl ;
  skos:prefLabel "측지 표고"@kr ;
.
<http://iso.org/tc211/term/2>
  rdf:type skos:Concept ;
  dcterms:dateAccepted "2008-11-15"^^xsd:date ;
  dcterms:provenance "ISO/TS 19104:2008" ;
  dcterms:source "ISO 1087-1:2000" ;
  reg:status reg:statusValid ;
  rdfs:label "abbreviation"@en ;
  skos:changeNote "valid" ;
  skos:editorialNote "preferred"^^xsd:string ;
  skos:notation 2 ;
  skos:prefLabel "abbreviation"@en ;
.
<http://iso.org/tc211/term/20>
  rdf:type skos:Concept ;
  dcterms:dateAccepted "2005-07-15" ;
  dcterms:dateAccepted "2005-07-15"^^xsd:date ;
  dcterms:dateAccepted "2009-12-29"^^xsd:date ;
  dcterms:provenance "ISO/TS 19103:2005" ;
  dcterms:provenance "KS X ISO 19103" ;
  dcterms:source "ISO/IEC 19501:2005 (Adapted from)" ;
  reg:status reg:statusAccepted ;
  reg:status reg:statusValid ;
  rdfs:comment "NOTE 1 An attribute is semantically equivalent to a composition association; however, the intent and usage is normally different."@en ;
  rdfs:comment "NOTE 2 \"Feature\" used in this definition is the UML meaning of the term and is not meant as defined in 4.1 of this Technical Specification."@en ;
  rdfs:comment "Note 1 to entry: An attribute is semantically equivalent to a composition association; however, the intent and usage is normally different."@en ;
  rdfs:comment "Note 2 to entry: \"Feature\" used in this definition is the UML meaning of the term and is not meant as defined in 4.1 of this Technical Specification." ;
  rdfs:comment "비고 1: 속성은 의미적으로 합성 연관과 동일하다. 그러나 의미와 용법은 일반적으로 다르다."@kr ;
  rdfs:label "attribute <UML>"@en ;
  skos:changeNote "valid" ;
  skos:definition "element binnen een objecttype waarmee waarden worden beschreven die instanties van het object kunnen hebben"@nl ;
  skos:definition "분류자의 특성으로 분류자의 인스턴스가 가질 수 있는 값의 범위를 기술"@kr ;
  skos:editorialNote "preferred" ;
  skos:editorialNote "preferred"^^xsd:string ;
  skos:notation "20" ;
  skos:notation 20 ;
  skos:note "NOTE 1 An attribute is semantically equivalent to a composition association; however, the intent and usage is normally different."@en ;
  skos:note "NOTE 2 \"Feature\" used in this definition is the UML meaning of the term and is not meant as defined in 4.1 of this Technical Specification."^^<http://www.w3.org/2001/XMLSchema#@en> ;
  skos:note "Note 1 to entry: An attribute is semantically equivalent to a composition association; however, the intent and usage is normally different."@en ;
  skos:note "Note 2 to entry: \"Feature\" used in this definition is the UML meaning of the term and is not meant as defined in 4.1 of this Technical Specification."^^<http://www.w3.org/2001/XMLSchema#@en> ;
  skos:note "비고 1: 속성은 의미적으로 합성 연관과 동일하다. 그러나 의미와 용법은 일반적으로 다르다."@kr ;
  skos:note "비고 2: 정의에 사용된 “특성(Feature)”은 KS X ISO 19103에 정의된 의미가 아닌 UML 용어이다."@kr ;
  skos:prefLabel "attribute <UML>"@en ;
  skos:prefLabel "attribuut <UML>"@nl ;
  skos:prefLabel "속성 <UML>"@kr ;
.
<http://iso.org/tc211/term/200>
  rdf:type skos:Concept ;
  dcterms:dateAccepted "2003-02-15" ;
  dcterms:dateAccepted "2003-02-15"^^xsd:date ;
  dcterms:dateAccepted "2007-11-01"^^xsd:date ;
  dcterms:provenance "ISO 19111:2003" ;
  dcterms:provenance "KS X ISO 19111" ;
  dcterms:source "ISO 19111:2007" ;
  reg:status reg:statusAccepted ;
  reg:status reg:statusValid ;
  rdfs:label "geodetic latitude"@en ;
  rdfs:seeAlso "ellipsoidal latitude" ;
  rdfs:seeAlso "ellipsoïde breedte"@nl ;
  skos:altLabel "ellipsoidal latitude"@en ;
  skos:altLabel "ellipsoïde breedte"@nl ;
  skos:altLabel "j"@kr ;
  skos:altLabel "j"@nl ;
  skos:altLabel "j"^^<http://www.w3.org/2001/XMLSchema#@en> ;
  skos:changeNote "valid" ;
  skos:definition "hoek vanaf het equatoriale vlak van de ellipsoïde door een gegeven punt, noordwaarts wordt als positief genomen"@nl ;
  skos:definition "적도면과 주어진 점을 통과하는 타원체 법선이 이루는 각도(ϕ)로써, 북으로 향하는 것을 정(+)으로 함 "@kr ;
  skos:editorialNote "preferred" ;
  skos:editorialNote "preferred"^^xsd:string ;
  skos:notation "200" ;
  skos:notation 200 ;
  skos:prefLabel "geodetic latitude"@en ;
  skos:prefLabel "geodetische breedte"@nl ;
  skos:prefLabel "측지 위도"@kr ;
.
<http://iso.org/tc211/term/201>
  rdf:type skos:Concept ;
  dcterms:dateAccepted "2003-02-15" ;
  dcterms:dateAccepted "2003-02-15"^^xsd:date ;
  dcterms:dateAccepted "2007-11-01"^^xsd:date ;
  dcterms:provenance "ISO 19111:2003" ;
  dcterms:provenance "KS X ISO 19111" ;
  dcterms:source "ISO 19111:2007" ;
  reg:status reg:statusAccepted ;
  reg:status reg:statusValid ;
  rdfs:label "geodetic longitude"@en ;
  rdfs:seeAlso "ellipsoidal longitude" ;
  rdfs:seeAlso "ellipsoïde lengte"@nl ;
  skos:altLabel "ellipsoidal longitude"@en ;
  skos:altLabel "ellipsoïde lengte"@nl ;
  skos:altLabel "l"@kr ;
  skos:altLabel "l"@nl ;
  skos:altLabel "l"^^<http://www.w3.org/2001/XMLSchema#@en> ;
  skos:changeNote "valid" ;
  skos:definition "hoek vanaf het vlak van de nulmeridiaan tot het meridiaan vlak van een gegeven punt, oostwaarts wordt als positief genomen"@nl ;
  skos:definition "본초 자오선과 주어진 점의 자오선이 이루는 각도(λ)로써 동으로 향하는 것을 정(+)으로 함"@kr ;
  skos:editorialNote "preferred" ;
  skos:editorialNote "preferred"^^xsd:string ;
  skos:notation "201" ;
  skos:notation 201 ;
  skos:prefLabel "geodetic longitude"@en ;
  skos:prefLabel "geodetische lengte"@nl ;
  skos:prefLabel "측지 경도"@kr ;
.
<http://iso.org/tc211/term/202>
  rdf:type skos:Concept ;
  dcterms:dateAccepted "2005-06-15"^^xsd:date ;
  dcterms:dateAccepted "2006-05-01"^^xsd:date ;
  dcterms:provenance "KS X ISO 19109" ;
  dcterms:source "ISO 19109:2005" ;
  reg:status reg:statusValid ;
  rdfs:comment "Note 1 to entry: Geographic information is also used as a term for information concerning phenomena implicitly or explicitly associated with a location relative to the Earth."@en ;
  rdfs:comment "비고: 지리 정보 또한 지표상의 위치에 묵시적 또는 명시적으로 관련하는 현상에 대한 정보를 의미하는 용어로 사용된다."@kr ;
  rdfs:label "geographic data"@en ;
  skos:changeNote "valid" ;
  skos:definition "지표상의 위치를 묵시적 또는 명시적으로 참조하는 데이터"@kr ;
  skos:editorialNote "preferred" ;
  skos:editorialNote "preferred"^^xsd:string ;
  skos:notation "202" ;
  skos:notation 202 ;
  skos:note "Note 1 to entry: Geographic information is also used as a term for information concerning phenomena implicitly or explicitly associated with a location relative to the Earth."@en ;
  skos:note "비고: 지리 정보 또한 지표상의 위치에 묵시적 또는 명시적으로 관련하는 현상에 대한 정보를 의미하는 용어로 사용된다."@kr ;
  skos:prefLabel "geographic data"@en ;
  skos:prefLabel "지리 데이터"@kr ;
.
<http://iso.org/tc211/term/203>
  rdf:type skos:Concept ;
  dcterms:dateAccepted "2004-08-01" ;
  dcterms:dateAccepted "2004-08-01"^^xsd:date ;
  dcterms:dateAccepted "2009-12-29"^^xsd:date ;
  dcterms:provenance "KS X ISO 19125-2" ;
  dcterms:provenance "NEN 3610" ;
  dcterms:source "ISO 19125-2:2004" ;
  reg:status reg:statusAccepted ;
  reg:status reg:statusValid ;
  rdfs:comment "Indien met een geo-object een gebied wordt bedoeld, kan dit in twee of drie dimensies zijn begrensd"@en ;
  rdfs:comment "Of een fenomeen een geo-object is of niet hangt af van de context waarin het object is geplaatst. Is er een associatie met een geo-gerefereerde locatie dan is het een geo-object. Is de associatie er niet dan is het fenomeen geen geo-object. Zo is bijvoorbeeld het fenomeen huis weergegeven op een landkaart een geo-object. Is het weergegeven op een foto dan is het geen geo-object. Met andere woorden: koppeling van geo-informatie maakt van een object een geo-object."@en ;
  rdfs:label "geographic feature"@en ;
  skos:changeNote "valid" ;
  skos:definition "abstractie van een fenomeen in de werkelijkheid dat direct of indirect is geassocieerd met een locatie relatief ten opzichte van de aarde (bijvoorbeeld ten opzichte van het aardoppervlak)"@nl ;
  skos:definition "지구상의 위치와 연관된 실세계 현상의 표현"@kr ;
  skos:editorialNote "preferred" ;
  skos:editorialNote "preferred"^^xsd:string ;
  skos:notation "203" ;
  skos:notation 203 ;
  skos:note "Indien met een geo-object een gebied wordt bedoeld, kan dit in twee of drie dimensies zijn begrensd"@en ;
  skos:note "Of een fenomeen een geo-object is of niet hangt af van de context waarin het object is geplaatst. Is er een associatie met een geo-gerefereerde locatie dan is het een geo-object. Is de associatie er niet dan is het fenomeen geen geo-object. Zo is bijvoorbeeld het fenomeen huis weergegeven op een landkaart een geo-object. Is het weergegeven op een foto dan is het geen geo-object. Met andere woorden: koppeling van geo-informatie maakt van een object een geo-object."^^<http://www.w3.org/2001/XMLSchema#@en> ;
  skos:prefLabel "geo-object"@nl ;
  skos:prefLabel "geographic feature"@en ;
  skos:prefLabel "지리 피처"@kr ;
.
<http://iso.org/tc211/term/204>
  rdf:type skos:Concept ;
  dcterms:dateAccepted "2003-10-15" ;
  dcterms:dateAccepted "2003-10-15"^^xsd:date ;
  dcterms:dateAccepted "2009-12-29"^^xsd:date ;
  dcterms:provenance "KS X ISO 19112" ;
  dcterms:provenance "NEN 3610" ;
  dcterms:source "ISO 19112:2003" ;
  reg:status reg:statusAccepted ;
  reg:status reg:statusValid ;
  rdfs:comment "'Nederland' is een voorbeeld voor een identificatie van een land. '6711 AD' is een voorbeeld van een postcode."@en ;
  rdfs:label "geographic identifier"@en ;
  skos:changeNote "valid" ;
  skos:definition "ruimtelijke referentie door een label of code waarmee een locatie wordt geïdentificeerd"@nl ;
  skos:definition "위치 식별을 위한 코드나 라벨 형식의 공간 참조"@kr ;
  skos:editorialNote "preferred" ;
  skos:editorialNote "preferred"^^xsd:string ;
  skos:notation "204" ;
  skos:notation 204 ;
  skos:note "'Nederland' is een voorbeeld voor een identificatie van een land. '6711 AD' is een voorbeeld van een postcode."@en ;
  skos:prefLabel "geographic identifier"@en ;
  skos:prefLabel "geographische identificatie"@nl ;
  skos:prefLabel "지리 식별자"@kr ;
.
<http://iso.org/tc211/term/205>
  rdf:type skos:Concept ;
  dcterms:dateAccepted "2002-07-01" ;
  dcterms:dateAccepted "2002-07-01"^^xsd:date ;
  dcterms:dateAccepted "2008-12-30"^^xsd:date ;
  dcterms:provenance "ISO 19101:2002" ;
  dcterms:source "ISO 19101-1:2014, 4.1.18" ;
  reg:status reg:statusAccepted ;
  reg:status reg:statusValid ;
  rdfs:label "geographic information"@en ;
  rdfs:seeAlso "geografische informatie"@nl ;
  skos:altLabel "geografische informatie"@nl ;
  skos:changeNote "valid" ;
  skos:definition "informatie met een directe of indirecte referentie naar een plaats ten opzichte van de aarde (bijvoorbeeld ten opzichte van het aardoppervlak)"@nl ;
  skos:definition "지구상의 위치와 직접적 또는 간접적으로 관련된 현상에 대한 정보"@kr ;
  skos:editorialNote "preferred" ;
  skos:editorialNote "preferred"^^xsd:string ;
  skos:notation "205" ;
  skos:notation 205 ;
  skos:prefLabel "geo-informatie"@nl ;
  skos:prefLabel "geographic information"@en ;
  skos:prefLabel "지리 정보"@kr ;
.
<http://iso.org/tc211/term/206>
  rdf:type skos:Concept ;
  dcterms:dateAccepted "2002-07-01"^^xsd:date ;
  dcterms:dateAccepted "2008-12-30"^^xsd:date ;
  dcterms:provenance "ISO 19101:2002" ;
  dcterms:source "ISO 19101-1:2014, 4.1.19" ;
  reg:status reg:statusValid ;
  rdfs:label "geographic information service"@en ;
  skos:changeNote "valid" ;
  skos:definition "사용자에게 지리 정보를 변형, 관리, 제공해 주는 서비스"@kr ;
  skos:editorialNote "preferred" ;
  skos:editorialNote "preferred"^^xsd:string ;
  skos:notation "206" ;
  skos:notation 206 ;
  skos:prefLabel "geographic information service"@en ;
  skos:prefLabel "지리 정보 서비스"@kr ;
.
<http://iso.org/tc211/term/207>
  rdf:type skos:Concept ;
  dcterms:dateAccepted "2002-07-01"^^xsd:date ;
  dcterms:dateAccepted "2008-12-30"^^xsd:date ;
  dcterms:provenance "ISO 19101:2002" ;
  dcterms:source "ISO 19101-1:2014, 4.1.20" ;
  reg:status reg:statusValid ;
  rdfs:label "geographic information system"@en ;
  skos:changeNote "valid" ;
  skos:definition "지구상의 위치와 관련된 현상 정보를 다루는 정보 시스템"@kr ;
  skos:editorialNote "preferred" ;
  skos:editorialNote "preferred"^^xsd:string ;
  skos:notation "207" ;
  skos:notation 207 ;
  skos:prefLabel "geographic information system"@en ;
  skos:prefLabel "지리 정보 시스템"@kr ;
.
<http://iso.org/tc211/term/210>
  rdf:type skos:Concept ;
  dcterms:dateAccepted "2003-05-01"^^xsd:date ;
  dcterms:dateAccepted "2009-12-29"^^xsd:date ;
  dcterms:provenance "KS X ISO 19107" ;
  dcterms:source "ISO 19107:2003" ;
  reg:status reg:statusValid ;
  rdfs:comment "Note 1 to entry: No assumptions about the spatial relationships between the elements can be made."@en ;
  rdfs:comment "비고: 요소들 간의 공간 관계에 관해 어떠한 가정도 불가능하다."@kr ;
  rdfs:label "geometric aggregate"@en ;
  skos:changeNote "valid" ;
  skos:definition "내부 구조를 갖지 않는 기하 객체들의 모음"@kr ;
  skos:editorialNote "preferred" ;
  skos:editorialNote "preferred"^^xsd:string ;
  skos:notation "210" ;
  skos:notation 210 ;
  skos:note "Note 1 to entry: No assumptions about the spatial relationships between the elements can be made."@en ;
  skos:note "비고: 요소들 간의 공간 관계에 관해 어떠한 가정도 불가능하다."@kr ;
  skos:prefLabel "geometric aggregate"@en ;
  skos:prefLabel "기하 집합체"@kr ;
.
<http://iso.org/tc211/term/211>
  rdf:type skos:Concept ;
  dcterms:dateAccepted "2003-05-01"^^xsd:date ;
  dcterms:dateAccepted "2009-12-29"^^xsd:date ;
  dcterms:provenance "KS X ISO 19107" ;
  dcterms:source "ISO 19107:2003" ;
  reg:status reg:statusValid ;
  rdfs:label "geometric boundary"@en ;
  skos:changeNote "valid" ;
  skos:definition "보다 낮은 기하 차원의 기하 원시 객체 집합으로 기하 객체의 범위를 표현하는 경계"@kr ;
  skos:editorialNote "preferred" ;
  skos:editorialNote "preferred"^^xsd:string ;
  skos:notation "211" ;
  skos:notation 211 ;
  skos:prefLabel "geometric boundary"@en ;
  skos:prefLabel "기하 경계"@kr ;
.
<http://iso.org/tc211/term/212>
  rdf:type skos:Concept ;
  dcterms:dateAccepted "2003-05-01"^^xsd:date ;
  dcterms:dateAccepted "2009-12-29"^^xsd:date ;
  dcterms:provenance "KS X ISO 19107" ;
  dcterms:source "ISO 19107:2003" ;
  reg:status reg:statusValid ;
  rdfs:comment "Note 1 to entry: The geometric primitives in the set are disjoint in the sense that no direct position is interior to more than one geometric primitive. The set is closed under boundary operations, meaning that for each element in the geometric complex, there is a collection (also a geometric complex) of geometric primitives that represents the boundary of that element. Recall that the boundary of a point (the only 0D primitive object type in geometry) is empty. Thus, if the largest dimension geometric primitive is a solid (3D), the composition of the boundary operator in this definition terminates after at most three steps. It is also the case that the boundary of any object is a cycle."@en ;
  rdfs:comment "비고: 직접 위치가 하나의 기하 원시 객체보다 더 내부에 있지 않다는 의미에서, 집합 내의 기하 원시 객체는 분리되어 있다. 집합은 경계 연산에서 폐합되어 있으며 이는 기하 복합체의 각 요소들에 대해 이들의 경계를 표현하는 기하 원시 객체 집합(또한 기하 복합체)이 존재하는 것을 의미한다. 점(기하에서 유일하게 0차원을 갖는 원시 객체 유형)의 경계는 비어 있다는 사실을 상기하라. 따라서 만약 최대 차원의 기하 원시 객체가 입방체(3차원)라면, 이 정의에서 경계 연산자의 합성은 최대 세 단계로 종결된다. 이는 순환 경계를 갖는 모든 객체에 대해서 동일하다."@kr ;
  rdfs:label "geometric complex"@en ;
  skos:changeNote "valid" ;
  skos:definition "각 기하 원시 객체의 경계가 동일한 집합 내에서 더 낮은 차원의 기하 원시 객체의 합집합으로 표현될 수 있는 기하 원시 객체들의 집합"@kr ;
  skos:editorialNote "preferred" ;
  skos:editorialNote "preferred"^^xsd:string ;
  skos:notation "212" ;
  skos:notation 212 ;
  skos:note "Note 1 to entry: The geometric primitives in the set are disjoint in the sense that no direct position is interior to more than one geometric primitive. The set is closed under boundary operations, meaning that for each element in the geometric complex, there is a collection (also a geometric complex) of geometric primitives that represents the boundary of that element. Recall that the boundary of a point (the only 0D primitive object type in geometry) is empty. Thus, if the largest dimension geometric primitive is a solid (3D), the composition of the boundary operator in this definition terminates after at most three steps. It is also the case that the boundary of any object is a cycle."@en ;
  skos:note "비고: 직접 위치가 하나의 기하 원시 객체보다 더 내부에 있지 않다는 의미에서, 집합 내의 기하 원시 객체는 분리되어 있다. 집합은 경계 연산에서 폐합되어 있으며 이는 기하 복합체의 각 요소들에 대해 이들의 경계를 표현하는 기하 원시 객체 집합(또한 기하 복합체)이 존재하는 것을 의미한다. 점(기하에서 유일하게 0차원을 갖는 원시 객체 유형)의 경계는 비어 있다는 사실을 상기하라. 따라서 만약 최대 차원의 기하 원시 객체가 입방체(3차원)라면, 이 정의에서 경계 연산자의 합성은 최대 세 단계로 종결된다. 이는 순환 경계를 갖는 모든 객체에 대해서 동일하다."@kr ;
  skos:prefLabel "geometric complex"@en ;
  skos:prefLabel "기하 복합체"@kr ;
.
<http://iso.org/tc211/term/213>
  rdf:type skos:Concept ;
  dcterms:dateAccepted "2003-05-01"^^xsd:date ;
  dcterms:dateAccepted "2009-12-29"^^xsd:date ;
  dcterms:provenance "KS X ISO 19107" ;
  dcterms:source "ISO 19107:2003" ;
  reg:status reg:statusValid ;
  rdfs:comment "Note 1 to entry: Curves, because they are continuous images of a portion of the real line, have geometric dimension 1. Surfaces cannot be mapped to R2 in their entirety, but around each point position, a small neighbourhood can be found that resembles (under continuous functions) the interior of the unit circle in R2, and are therefore 2-dimensional. In this International Standard, most surface patches (instances of GM_SurfacePatch) are mapped to portions of R2 by their defining interpolation mechanisms."@en ;
  rdfs:comment "비고: 곡선은 실선의 연속적 모양이기 때문에 기하차원이 1이다. 표면은 R2에 전부 매핑될 수 없으나, 각 점의 위치 주위에 R2내의 단위 원의 내부와 유사한(연속함수를 사용) 작은 인접군을 발견할 수 있어 2차원이다. 본 표준에서 대부분의 표면 조각(GM_SurfacePatch의 인스턴스)은 정의된 보간 메커니즘에 따라 R2의 부분에 매핑된다."@kr ;
  rdfs:label "geometric dimension"@en ;
  skos:changeNote "valid" ;
  skos:definition "기하 집합에서 각각의 직접 위치가 그 부분 집합 내부의 위치와 연관될 수 있는 최대의 수. 유클리드 n 공간의 Rn과 유사함"@kr ;
  skos:editorialNote "preferred" ;
  skos:editorialNote "preferred"^^xsd:string ;
  skos:notation "213" ;
  skos:notation 213 ;
  skos:note "Note 1 to entry: Curves, because they are continuous images of a portion of the real line, have geometric dimension 1. Surfaces cannot be mapped to R2 in their entirety, but around each point position, a small neighbourhood can be found that resembles (under continuous functions) the interior of the unit circle in R2, and are therefore 2-dimensional. In this International Standard, most surface patches (instances of GM_SurfacePatch) are mapped to portions of R2 by their defining interpolation mechanisms."@en ;
  skos:note "비고: 곡선은 실선의 연속적 모양이기 때문에 기하차원이 1이다. 표면은 R2에 전부 매핑될 수 없으나, 각 점의 위치 주위에 R2내의 단위 원의 내부와 유사한(연속함수를 사용) 작은 인접군을 발견할 수 있어 2차원이다. 본 표준에서 대부분의 표면 조각(GM_SurfacePatch의 인스턴스)은 정의된 보간 메커니즘에 따라 R2의 부분에 매핑된다."@kr ;
  skos:prefLabel "geometric dimension"@en ;
  skos:prefLabel "기하 차원"@kr ;
.
<http://iso.org/tc211/term/214>
  rdf:type skos:Concept ;
  dcterms:dateAccepted "2003-05-01"^^xsd:date ;
  dcterms:dateAccepted "2009-12-29"^^xsd:date ;
  dcterms:provenance "KS X ISO 19107" ;
  dcterms:source "ISO 19107:2003" ;
  reg:status reg:statusValid ;
  rdfs:comment "Note 1 to entry: A geometric object consists of a geometric primitive, a collection of geometric primitives, or a geometric complex treated as a single entity. A geometric object may be the spatial representation of an object such as a feature or a significant part of a feature."@en ;
  rdfs:comment "비고: 기하 객체는 하나의 개체로 취급되는 기하 원시 객체, 기하 원시 객체 집합, 기하 복합체로 구성된다. 기하 객체는 피처 또는 피처의 중요한 부분과 같은 객체의 공간적 표현이라 할 수 있다."@kr ;
  rdfs:label "geometric object"@en ;
  skos:changeNote "valid" ;
  skos:definition "기하 집합을 표현하는 공간 객체"@kr ;
  skos:editorialNote "preferred" ;
  skos:editorialNote "preferred"^^xsd:string ;
  skos:notation "214" ;
  skos:notation 214 ;
  skos:note "Note 1 to entry: A geometric object consists of a geometric primitive, a collection of geometric primitives, or a geometric complex treated as a single entity. A geometric object may be the spatial representation of an object such as a feature or a significant part of a feature."@en ;
  skos:note "비고: 기하 객체는 하나의 개체로 취급되는 기하 원시 객체, 기하 원시 객체 집합, 기하 복합체로 구성된다. 기하 객체는 피처 또는 피처의 중요한 부분과 같은 객체의 공간적 표현이라 할 수 있다."@kr ;
  skos:prefLabel "geometric object"@en ;
  skos:prefLabel "기하 객체"@kr ;
.
<http://iso.org/tc211/term/215>
  rdf:type skos:Concept ;
  dcterms:dateAccepted "2003-05-01"^^xsd:date ;
  dcterms:dateAccepted "2009-12-29"^^xsd:date ;
  dcterms:provenance "KS X ISO 19107" ;
  dcterms:source "ISO 19107:2003" ;
  reg:status reg:statusValid ;
  rdfs:comment "Note 1 to entry: Geometric primitives are non-decomposed objects that present information about geometric configuration. They include points, curves, surfaces, and solids."@en ;
  rdfs:comment "비고: 기하 원시 객체는 기하 구성에 관한 정보를 나타내는 분해가 불가능한 객체이다. 기하 원시 객체는 점, 곡선, 표면, 입방체를 포함한다."@kr ;
  rdfs:label "geometric primitive"@en ;
  skos:changeNote "valid" ;
  skos:definition "단일의, 연결된, 동종의 공간 요소를 나타내는 기하 객체"@kr ;
  skos:editorialNote "preferred" ;
  skos:editorialNote "preferred"^^xsd:string ;
  skos:notation "215" ;
  skos:notation 215 ;
  skos:note "Note 1 to entry: Geometric primitives are non-decomposed objects that present information about geometric configuration. They include points, curves, surfaces, and solids."@en ;
  skos:note "비고: 기하 원시 객체는 기하 구성에 관한 정보를 나타내는 분해가 불가능한 객체이다. 기하 원시 객체는 점, 곡선, 표면, 입방체를 포함한다."@kr ;
  skos:prefLabel "geometric primitive"@en ;
  skos:prefLabel "기하 원시 객체"@kr ;
.
<http://iso.org/tc211/term/216>
  rdf:type skos:Concept ;
  dcterms:dateAccepted "2003-05-01"^^xsd:date ;
  dcterms:dateAccepted "2009-12-29"^^xsd:date ;
  dcterms:provenance "KS X ISO 19107" ;
  dcterms:source "ISO 19107:2003" ;
  reg:status reg:statusValid ;
  rdfs:comment "Note 1 to entry: In such a realization the topological primitives are considered to represent the interiors of the corresponding geometric primitives. Composites are closed."@en ;
  rdfs:comment "비고: 이러한 실현에 있어 위상 원시 객체는 대응하는 기하 원시 객체의 내부를 표현하는 것으로 간주된다. 합성체는 폐합되어 있다."@kr ;
  rdfs:label "geometric realization"@en ;
  skos:changeNote "valid" ;
  skos:definition "위상 복합체를 구성하는 위상 원시 객체와 일 대 일의 대응 관계가 있는 기하 원시 객체로 구성되는 기하 복합체. 이 경우 두 복합체 간의 경계가 일치함"@kr ;
  skos:editorialNote "preferred" ;
  skos:editorialNote "preferred"^^xsd:string ;
  skos:notation "216" ;
  skos:notation 216 ;
  skos:note "Note 1 to entry: In such a realization the topological primitives are considered to represent the interiors of the corresponding geometric primitives. Composites are closed."@en ;
  skos:note "비고: 이러한 실현에 있어 위상 원시 객체는 대응하는 기하 원시 객체의 내부를 표현하는 것으로 간주된다. 합성체는 폐합되어 있다."@kr ;
  skos:prefLabel "geometric realization"@en ;
  skos:prefLabel "기하 실현"@kr ;
.
<http://iso.org/tc211/term/217>
  rdf:type skos:Concept ;
  dcterms:dateAccepted "2003-05-01"^^xsd:date ;
  dcterms:dateAccepted "2009-12-29"^^xsd:date ;
  dcterms:provenance "KS X ISO 19107" ;
  dcterms:source "ISO 19107:2003" ;
  reg:status reg:statusValid ;
  rdfs:comment "Note 1 to entry: This set in most cases is infinite."@en ;
  rdfs:comment "비고: 대부분의 경우에서 집합은 무한 집합이다."@kr ;
  rdfs:label "geometric set"@en ;
  skos:changeNote "valid" ;
  skos:definition "직접 위치의 집합"@kr ;
  skos:editorialNote "preferred" ;
  skos:editorialNote "preferred"^^xsd:string ;
  skos:notation "217" ;
  skos:notation 217 ;
  skos:note "Note 1 to entry: This set in most cases is infinite."@en ;
  skos:note "비고: 대부분의 경우에서 집합은 무한 집합이다."@kr ;
  skos:prefLabel "geometric set"@en ;
  skos:prefLabel "기하 집합"@kr ;
.
<http://iso.org/tc211/term/218>
  rdf:type skos:Concept ;
  dcterms:dateAccepted "2003-02-15" ;
  dcterms:dateAccepted "2003-02-15"^^xsd:date ;
  dcterms:dateAccepted "2007-11-01"^^xsd:date ;
  dcterms:provenance "ISO 19111:2003" ;
  dcterms:provenance "KS X ISO 19111" ;
  dcterms:source "ISO 19111:2007" ;
  reg:status reg:statusAccepted ;
  reg:status reg:statusValid ;
  rdfs:comment "Note 1 to entry: This refers to in particular orthometric height or normal height, which are both approximations of the distance of a point above the mean sea level."@en ;
  rdfs:comment "OPMERKING Dit slaat in het bijzonder op orthometrische hoogten en normaal hoogten welke beide benaderingen zijn van de hoogte van een punt boven gemiddeld zeeniveau."@en ;
  rdfs:comment "비고: 특히 평균 해수면 위쪽 방향에 위치하는 한 점까지의 거리에 대한 근사값인 정사 표고나 정규 표고를 말한다."@kr ;
  rdfs:label "gravity-related height"@en ;
  skos:altLabel "H"@kr ;
  skos:altLabel "H"@nl ;
  skos:altLabel "H"^^<http://www.w3.org/2001/XMLSchema#@en> ;
  skos:changeNote "valid" ;
  skos:definition "hoogte die gerelateerd is aan het zwaartekrachtveld van de aarde"@nl ;
  skos:definition "지구의 중력에 영향을 받는 높이"@kr ;
  skos:editorialNote "preferred" ;
  skos:editorialNote "preferred"^^xsd:string ;
  skos:notation "218" ;
  skos:notation 218 ;
  skos:note "Note 1 to entry: This refers to in particular orthometric height or normal height, which are both approximations of the distance of a point above the mean sea level."@en ;
  skos:note "OPMERKING Dit slaat in het bijzonder op orthometrische hoogten en normaal hoogten welke beide benaderingen zijn van de hoogte van een punt boven gemiddeld zeeniveau."@en ;
  skos:note "비고: 특히 평균 해수면 위쪽 방향에 위치하는 한 점까지의 거리에 대한 근사값인 정사 표고나 정규 표고를 말한다."@kr ;
  skos:prefLabel "gravity-related height"@en ;
  skos:prefLabel "zwaartekracht gerelateerde hoogte"@nl ;
  skos:prefLabel "중력 높이"@kr ;
.
<http://iso.org/tc211/term/219>
  rdf:type skos:Concept ;
  dcterms:dateAccepted "2007-09-01"^^xsd:date ;
  dcterms:dateAccepted "2009-12-29"^^xsd:date ;
  dcterms:provenance "KS X ISO 19136" ;
  dcterms:source "ISO 19136:2007" ;
  reg:status reg:statusValid ;
  rdfs:comment "Note 1 to entry: The geometry property name is the role of the geometry in relation to the feature."@en ;
  rdfs:comment "비고: 기하 특성 명칭은 피처에 관한 기하의 역할이다."@kr ;
  rdfs:label "geometry property <GML>"@en ;
  skos:changeNote "valid" ;
  skos:definition "지리 피처의 기하 현상을 기술하는 GML 피처의 특성"@kr ;
  skos:editorialNote "preferred" ;
  skos:editorialNote "preferred"^^xsd:string ;
  skos:notation "219" ;
  skos:notation 219 ;
  skos:note "Note 1 to entry: The geometry property name is the role of the geometry in relation to the feature."@en ;
  skos:note "비고: 기하 특성 명칭은 피처에 관한 기하의 역할이다."@kr ;
  skos:prefLabel "geometry property <GML>"@en ;
  skos:prefLabel "기하 특성 <GML>"@kr ;
.
<http://iso.org/tc211/term/220>
  rdf:type skos:Concept ;
  dcterms:dateAccepted "2002-09-01"^^xsd:date ;
  dcterms:dateAccepted "2007-11-01"^^xsd:date ;
  dcterms:provenance "ISO 19108;2002" ;
  dcterms:provenance "KS X ISO 19108" ;
  dcterms:source "ISO 8601:2000 (Adapted from)" ;
  reg:status reg:statusValid ;
  rdfs:comment "Note 1 to entry: The introduction of the Gregorian calendar included the cancellation of the accumulated inaccuracies of the Julian year. In the Gregorian calendar, a calendar year is either a common year or a leap year; each year is divided into 12 sequential months."@en ;
  rdfs:comment "비고: 그레고리안 달력은 율리우스력의 누적된 오차를 보정하기 위해 도입되었다. 그레고리안 달력에서는 대개 1년은 365일을 가지고 윤년은 366일을 가지며 12개의 연속적인 달로 나뉜다."@kr ;
  rdfs:label "Gregorian calendar"@en ;
  skos:changeNote "valid" ;
  skos:definition "율리우스력(曆)에 비하여 회귀 연도에 보다 근사하게 윤년을 정의하는, 1582년에 최초로 도입된 범용달력"@kr ;
  skos:editorialNote "preferred" ;
  skos:editorialNote "preferred"^^xsd:string ;
  skos:notation "220" ;
  skos:notation 220 ;
  skos:note "Note 1 to entry: The introduction of the Gregorian calendar included the cancellation of the accumulated inaccuracies of the Julian year. In the Gregorian calendar, a calendar year is either a common year or a leap year; each year is divided into 12 sequential months."@en ;
  skos:note "비고: 그레고리안 달력은 율리우스력의 누적된 오차를 보정하기 위해 도입되었다. 그레고리안 달력에서는 대개 1년은 365일을 가지고 윤년은 366일을 가지며 12개의 연속적인 달로 나뉜다."@kr ;
  skos:prefLabel "Gregorian calendar"@en ;
  skos:prefLabel "그레고리안 달력"@kr ;
.
<http://iso.org/tc211/term/221>
  rdf:type skos:Concept ;
  dcterms:dateAccepted "2003-05-01"^^xsd:date ;
  dcterms:dateAccepted "2007-11-01"^^xsd:date ;
  dcterms:provenance "ISO 19115:2003" ;
  dcterms:provenance "KS X ISO 19123" ;
  dcterms:source "ISO 19123:2005" ;
  reg:status reg:statusValid ;
  rdfs:comment "Note 1 to entry: The curves partition a space into grid cells."@en ;
  rdfs:comment "비고: 곡선은 공간을 격자 셀로 분할한다."@kr ;
  rdfs:label "grid"@en ;
  skos:changeNote "valid" ;
  skos:definition "알고리듬적으로 각 집합의 원소가 다른 집합의 원소와 교차하는 둘 이상의 곡선 집합으로 구성된 네트워크"@kr ;
  skos:editorialNote "preferred" ;
  skos:editorialNote "preferred"^^xsd:string ;
  skos:notation "221" ;
  skos:notation 221 ;
  skos:note "Note 1 to entry: The curves partition a space into grid cells."@en ;
  skos:note "비고: 곡선은 공간을 격자 셀로 분할한다."@kr ;
  skos:prefLabel "grid"@en ;
  skos:prefLabel "격자"@kr ;
.
<http://iso.org/tc211/term/222>
  rdf:type skos:Concept ;
  dcterms:dateAccepted "2009-02-15"^^xsd:date ;
  dcterms:source "ISO 19115-2:2009" ;
  reg:status reg:statusValid ;
  rdfs:label "grid coordinates"@en ;
  skos:changeNote "valid" ;
  skos:editorialNote "preferred"^^xsd:string ;
  skos:notation 222 ;
  skos:prefLabel "grid coordinates"@en ;
.
<http://iso.org/tc211/term/223>
  rdf:type skos:Concept ;
  dcterms:dateAccepted "2005-08-15"^^xsd:date ;
  dcterms:dateAccepted "2007-11-01"^^xsd:date ;
  dcterms:provenance "KS X ISO 19123" ;
  dcterms:source "ISO 19123:2005" ;
  reg:status reg:statusValid ;
  rdfs:label "grid point"@en ;
  skos:changeNote "valid" ;
  skos:definition "격자에서 두 개 이상 곡선의 교차점에 위치하는 점"@kr ;
  skos:editorialNote "preferred" ;
  skos:editorialNote "preferred"^^xsd:string ;
  skos:notation "223" ;
  skos:notation 223 ;
  skos:prefLabel "grid point"@en ;
  skos:prefLabel "격자 점"@kr ;
.
<http://iso.org/tc211/term/224>
  rdf:type skos:Concept ;
  dcterms:dateAccepted "2009-02-15"^^xsd:date ;
  dcterms:source "ISO 19115-2:2009" ;
  reg:status reg:statusValid ;
  rdfs:label "gridded data"@en ;
  skos:changeNote "valid" ;
  skos:editorialNote "preferred"^^xsd:string ;
  skos:notation 224 ;
  skos:prefLabel "gridded data"@en ;
.
<http://iso.org/tc211/term/228>
  rdf:type skos:Concept ;
  dcterms:dateAccepted "2003-05-01"^^xsd:date ;
  dcterms:dateAccepted "2009-12-29"^^xsd:date ;
  dcterms:provenance "KS X ISO 19107" ;
  dcterms:source "ISO 19107:2003" ;
  reg:status reg:statusValid ;
  rdfs:comment "Note 1 to entry: Homomorphisms are distinct from isomorphisms in that no inverse function is required. In an isomorphism, there are essentially two homomorphisms that are functional inverses of one another. Continuous functions are topological homomorphisms because they preserve \"topological characteristics.\" The mapping of topological complexes to their geometric realizations preserves the concept of boundary and is therefore a homomorphism."@en ;
  rdfs:comment "비고: 준동형은 역함수를 필요로 하지 않는다는 점에서 동형과 다르다. 동형에는 본질적으로 서로 역함수 관계에 있는 두 준동형이 있다. 연속 함수가 \"위상 특징\"을 보존하기 때문에, 연속 함수는 위상 준동형이다. 위상 복합체를 그의 기하 실현에 매핑하는 것은 경계의 개념을 보존한다. 따라서 준동형이다."@kr ;
  rdfs:label "homomorphism"@en ;
  skos:changeNote "valid" ;
  skos:definition "하나의 영역이 다른 영역의 구조 보존 함수를 가지고 있는, 두 영역(예: 두 복합체) 간의 관계"@kr ;
  skos:editorialNote "preferred" ;
  skos:editorialNote "preferred"^^xsd:string ;
  skos:notation "228" ;
  skos:notation 228 ;
  skos:note "Note 1 to entry: Homomorphisms are distinct from isomorphisms in that no inverse function is required. In an isomorphism, there are essentially two homomorphisms that are functional inverses of one another. Continuous functions are topological homomorphisms because they preserve \"topological characteristics.\" The mapping of topological complexes to their geometric realizations preserves the concept of boundary and is therefore a homomorphism."@en ;
  skos:note "비고: 준동형은 역함수를 필요로 하지 않는다는 점에서 동형과 다르다. 동형에는 본질적으로 서로 역함수 관계에 있는 두 준동형이 있다. 연속 함수가 \"위상 특징\"을 보존하기 때문에, 연속 함수는 위상 준동형이다. 위상 복합체를 그의 기하 실현에 매핑하는 것은 경계의 개념을 보존한다. 따라서 준동형이다."@kr ;
  skos:prefLabel "homomorphism"@en ;
  skos:prefLabel "준동형"@kr ;
.
<http://iso.org/tc211/term/232>
  rdf:type skos:Concept ;
  dcterms:dateAccepted "2010-06-15"^^xsd:date ;
  dcterms:source "ISO/TS 19130:2010" ;
  reg:status reg:statusValid ;
  rdfs:label "image point"@en ;
  skos:changeNote "valid" ;
  skos:editorialNote "preferred"^^xsd:string ;
  skos:notation 232 ;
  skos:prefLabel "image point"@en ;
.
<http://iso.org/tc211/term/235>
  rdf:type skos:Concept ;
  dcterms:dateAccepted "2000-12-15"^^xsd:date ;
  dcterms:dateAccepted "2007-06-29"^^xsd:date ;
  dcterms:provenance "KS X ISO 19105" ;
  dcterms:source "ISO 19105:2000" ;
  reg:status reg:statusValid ;
  rdfs:comment "Note 1 to entry: In the context of the ISO geographic information standards, this includes specifications of geographic information services and datasets."@en ;
  rdfs:comment "비고: 지리 정보 표준과 관련, 구현은 지리 정보 서비스 및 데이터셋 사양을 포함한다."@kr ;
  rdfs:label "implementation"@en ;
  skos:changeNote "valid" ;
  skos:definition "사양의 실현"@kr ;
  skos:editorialNote "preferred" ;
  skos:editorialNote "preferred"^^xsd:string ;
  skos:notation "235" ;
  skos:notation 235 ;
  skos:note "Note 1 to entry: In the context of the ISO geographic information standards, this includes specifications of geographic information services and datasets."@en ;
  skos:note "비고: 지리 정보 표준과 관련, 구현은 지리 정보 서비스 및 데이터셋 사양을 포함한다."@kr ;
  skos:prefLabel "implementation"@en ;
  skos:prefLabel "구현"@kr ;
.
<http://iso.org/tc211/term/236>
  rdf:type skos:Concept ;
  dcterms:dateAccepted "2000-12-15"^^xsd:date ;
  dcterms:dateAccepted "2007-06-29"^^xsd:date ;
  dcterms:provenance "KS X ISO 19105" ;
  dcterms:source "ISO 19105:2000" ;
  reg:status reg:statusValid ;
  rdfs:label "Implementation Conformance Statement"@en ;
  skos:altLabel "ICS"@kr ;
  skos:altLabel "ICS"^^<http://www.w3.org/2001/XMLSchema#@en> ;
  skos:changeNote "valid" ;
  skos:definition "사양에 규정된 요구 조건에 대한 구현 선택 사항을 기술한 문서"@kr ;
  skos:editorialNote "preferred" ;
  skos:editorialNote "preferred"^^xsd:string ;
  skos:notation "236" ;
  skos:notation 236 ;
  skos:prefLabel "Implementation Conformance Statement"@en ;
  skos:prefLabel "구현 적합성 기술서"@kr ;
.
<http://iso.org/tc211/term/237>
  rdf:type skos:Concept ;
  dcterms:dateAccepted "2000-12-15"^^xsd:date ;
  dcterms:dateAccepted "2007-06-29"^^xsd:date ;
  dcterms:provenance "KS X ISO 19105" ;
  dcterms:source "ISO 19105:2000" ;
  reg:status reg:statusValid ;
  rdfs:comment "Note 1 to entry: IXIT typically provides the details on the organization and storage of concepts in the SUT as well as on the means of access to and modification of the SUT."@en ;
  rdfs:comment "비고: 일반적으로 IXIT는 SUT에 대한 수정 및 접근 방법과 SUT에서 개념의 구성 및 저장에 관한 세부사항을 제공한다."@kr ;
  rdfs:label "Implementation eXtra Information for Testing"@en ;
  skos:altLabel "IXIT"@kr ;
  skos:altLabel "IXIT"^^<http://www.w3.org/2001/XMLSchema#@en> ;
  skos:changeNote "valid" ;
  skos:definition "시험소가 해당 IUT에 대해 적절한 시험 스위트를 수행할 수 있도록 IUT 및 이에 대응하는 SUT에 관련된 모든 정보를 포함하는 문서"@kr ;
  skos:editorialNote "preferred" ;
  skos:editorialNote "preferred"^^xsd:string ;
  skos:notation "237" ;
  skos:notation 237 ;
  skos:note "Note 1 to entry: IXIT typically provides the details on the organization and storage of concepts in the SUT as well as on the means of access to and modification of the SUT."@en ;
  skos:note "비고: 일반적으로 IXIT는 SUT에 대한 수정 및 접근 방법과 SUT에서 개념의 구성 및 저장에 관한 세부사항을 제공한다."@kr ;
  skos:prefLabel "Implementation eXtra Information for Testing"@en ;
  skos:prefLabel "시험용 구현 부가 정보"@kr ;
.
<http://iso.org/tc211/term/238>
  rdf:type skos:Concept ;
  dcterms:dateAccepted "2000-12-15"^^xsd:date ;
  dcterms:dateAccepted "2007-06-29"^^xsd:date ;
  dcterms:provenance "KS X ISO 19105" ;
  dcterms:source "ISO 19105:2000" ;
  reg:status reg:statusValid ;
  rdfs:label "inconclusive verdict"@en ;
  skos:changeNote "valid" ;
  skos:definition "통과 또는 실패로 판정할 수 없는 경우의 시험 판정"@kr ;
  skos:editorialNote "preferred" ;
  skos:editorialNote "preferred"^^xsd:string ;
  skos:notation "238" ;
  skos:notation 238 ;
  skos:prefLabel "inconclusive verdict"@en ;
  skos:prefLabel "판정 보류"@kr ;
.
<http://iso.org/tc211/term/239>
  rdf:type skos:Concept ;
  dcterms:dateAccepted "2003-08-15"^^xsd:date ;
  dcterms:dateAccepted "2009-12-29"^^xsd:date ;
  dcterms:provenance "ISO 19114" ;
  dcterms:source "ISO 19157:2013, 4.17" ;
  reg:status reg:statusValid ;
  rdfs:comment "Note 1 to entry: Examples of external knowledge are dataset lineage, such as production method or source data."@en ;
  rdfs:comment "비고: 외부 지식의 예로서, 생산 방법 또는 원시 데이터와 같은 데이터셋의 연혁을 들 수 있다."@kr ;
  rdfs:label "indirect evaluation method"@en ;
  skos:changeNote "valid" ;
  skos:definition "외부 지식을 바탕으로 데이터셋의 품질을 평가하는 방법"@kr ;
  skos:editorialNote "preferred" ;
  skos:editorialNote "preferred"^^xsd:string ;
  skos:notation "239" ;
  skos:notation 239 ;
  skos:note "Note 1 to entry: Examples of external knowledge are dataset lineage, such as production method or source data."@en ;
  skos:note "비고: 외부 지식의 예로서, 생산 방법 또는 원시 데이터와 같은 데이터셋의 연혁을 들 수 있다."@kr ;
  skos:prefLabel "indirect evaluation method"@en ;
  skos:prefLabel "간접 평가 방법"@kr ;
.
<http://iso.org/tc211/term/24>
  rdf:type skos:Concept ;
  dcterms:dateAccepted "2003-05-01"^^xsd:date ;
  dcterms:dateAccepted "2009-12-29"^^xsd:date ;
  dcterms:provenance "KS X ISO 19107" ;
  dcterms:source "ISO 19107:2003" ;
  reg:status reg:statusValid ;
  rdfs:comment "Note 1 to entry: Logically, a bag is a set of pairs <item, count>."@en ;
  rdfs:comment "비고: 논리적으로 다중 집합은 <항목, 수>쌍의 집합이다."@kr ;
  rdfs:label "bag"@en ;
  skos:changeNote "valid" ;
  skos:definition "유한하며 순서가 없는, 반복 가능한 항목(객체 또는 값)의 모음"@kr ;
  skos:editorialNote "preferred" ;
  skos:editorialNote "preferred"^^xsd:string ;
  skos:notation "24" ;
  skos:notation 24 ;
  skos:note "Note 1 to entry: Logically, a bag is a set of pairs <item, count>."@en ;
  skos:note "비고: 논리적으로 다중 집합은 <항목, 수>쌍의 집합이다."@kr ;
  skos:prefLabel "bag"@en ;
  skos:prefLabel "다중 집합"@kr ;
.
<http://iso.org/tc211/term/240>
  rdf:type skos:Concept ;
  dcterms:dateAccepted "2004-07-01"^^xsd:date ;
  dcterms:dateAccepted "2004-11-05"^^xsd:date ;
  dcterms:provenance "KS X ISO 19116" ;
  dcterms:source "ISO 19116:2004" ;
  reg:status reg:statusValid ;
  rdfs:label "inertial positioning system"@en ;
  skos:changeNote "valid" ;
  skos:definition "초기의 참조점으로부터의 점 또는 객체의 좌표를 구하기 위해 가속도계, 자이로스코프 및 컴퓨터를 컴포넌트로 통합 사용해 상대 위치를 구하는 측위 시스템"@kr ;
  skos:editorialNote "preferred" ;
  skos:editorialNote "preferred"^^xsd:string ;
  skos:notation "240" ;
  skos:notation 240 ;
  skos:prefLabel "inertial positioning system"@en ;
  skos:prefLabel "관성 측위 시스템"@kr ;
.
<http://iso.org/tc211/term/241>
  rdf:type skos:Concept ;
  dcterms:dateAccepted "2005-07-15"^^xsd:date ;
  dcterms:dateAccepted "2008-12-19"^^xsd:date ;
  dcterms:provenance "ISO 19118:2011 ,4.22" ;
  dcterms:source "ISO/IEC 2382-1:1993" ;
  reg:status reg:statusValid ;
  rdfs:label "information"@en ;
  skos:changeNote "valid" ;
  skos:definition "사실이나 사건, 사물, 과정 및 아이디어, 개념 등과 같은 객체에 관하여 특정 상황에서 특정 의미를 갖는 지식"@kr ;
  skos:editorialNote "preferred" ;
  skos:editorialNote "preferred"^^xsd:string ;
  skos:notation "241" ;
  skos:notation 241 ;
  skos:prefLabel "information"@en ;
  skos:prefLabel "정보"@kr ;
.
<http://iso.org/tc211/term/242>
  rdf:type skos:Concept ;
  dcterms:dateAccepted "2005-02-15"^^xsd:date ;
  dcterms:dateAccepted "2006-12-29"^^xsd:date ;
  dcterms:provenance "ISO 19119:2005" ;
  dcterms:provenance "KS X ISO/IEC 10746-2" ;
  dcterms:source "ISO/IEC 10746-3:1996" ;
  reg:status reg:statusValid ;
  rdfs:label "information viewpoint"@en ;
  skos:changeNote "valid" ;
  skos:definition "정보와 정보 처리 과정의 의미론에 초점을 맞춘 개방형 분산 처리 시스템과 그 환경에 대한 관점"@kr ;
  skos:editorialNote "preferred" ;
  skos:editorialNote "preferred"^^xsd:string ;
  skos:notation "242" ;
  skos:notation 242 ;
  skos:prefLabel "information viewpoint"@en ;
  skos:prefLabel "정보 관점"@kr ;
.
<http://iso.org/tc211/term/243>
  rdf:type skos:Concept ;
  dcterms:dateAccepted "2005-07-15"^^xsd:date ;
  dcterms:dateAccepted "2009-12-29"^^xsd:date ;
  dcterms:provenance "ISO/TS 19103:2005 ,4.2.14" ;
  dcterms:source "ISO/IEC 19501" ;
  reg:status reg:statusValid ;
  rdfs:comment "Note 1 to entry: See generalization."@en ;
  rdfs:comment "비고: '일반화'를 참조하라."@kr ;
  rdfs:label "inheritance <UML>"@en ;
  skos:changeNote "valid" ;
  skos:definition "보다 상세한 요소가 보다 일반적인 요소의 구조와 행태를 통합하는 메커니즘"@kr ;
  skos:editorialNote "preferred" ;
  skos:editorialNote "preferred"^^xsd:string ;
  skos:notation "243" ;
  skos:notation 243 ;
  skos:note "Note 1 to entry: See generalization."@en ;
  skos:note "비고: '일반화'를 참조하라."@kr ;
  skos:prefLabel "inheritance <UML>"@en ;
  skos:prefLabel "상속 <UML>"@kr ;
.
<http://iso.org/tc211/term/244>
  rdf:type skos:Concept ;
  dcterms:dateAccepted "2003-05-01"^^xsd:date ;
  dcterms:dateAccepted "2009-12-29"^^xsd:date ;
  dcterms:provenance "KS X ISO 19107" ;
  dcterms:source "ISO 19107:2003" ;
  reg:status reg:statusValid ;
  rdfs:label "instance"@en ;
  skos:changeNote "valid" ;
  skos:definition "클래스를 실현하는 객체"@kr ;
  skos:editorialNote "preferred" ;
  skos:editorialNote "preferred"^^xsd:string ;
  skos:notation "244" ;
  skos:notation 244 ;
  skos:prefLabel "instance"@en ;
  skos:prefLabel "인스턴스"@kr ;
.
<http://iso.org/tc211/term/246>
  rdf:type skos:Concept ;
  dcterms:dateAccepted "2005-07-15"^^xsd:date ;
  dcterms:dateAccepted "2008-12-30"^^xsd:date ;
  dcterms:provenance "ISO 19118:2005" ;
  dcterms:source "ISO 19118:2011, 4.23" ;
  reg:status reg:statusValid ;
  rdfs:label "instance model"@en ;
  skos:changeNote "valid" ;
  skos:definition "응용 스키마에 따른 데이터를 저장하기 위한 표현 모델"@kr ;
  skos:editorialNote "preferred" ;
  skos:editorialNote "preferred"^^xsd:string ;
  skos:notation "246" ;
  skos:notation 246 ;
  skos:prefLabel "instance model"@en ;
  skos:prefLabel "인스턴스 모델"@kr ;
.
<http://iso.org/tc211/term/247>
  rdf:type skos:Concept ;
  dcterms:dateAccepted "2002-09-01"^^xsd:date ;
  dcterms:dateAccepted "2007-11-01"^^xsd:date ;
  dcterms:provenance "KS X ISO 19108" ;
  dcterms:source "ISO 19108;2002" ;
  reg:status reg:statusValid ;
  rdfs:comment "Note 1 to entry: The geometry of time is discussed in 5.2. [of ISO 19108;2002]"@en ;
  rdfs:comment "비고: 시간의 기하는 KS X ISO 19108의 5.2절에서 기술되어 있다."@kr ;
  rdfs:label "instant"@en ;
  skos:changeNote "valid" ;
  skos:definition "특정 시점의 위치를 나타내는 0차원의 기하 원시 객체"@kr ;
  skos:editorialNote "preferred" ;
  skos:editorialNote "preferred"^^xsd:string ;
  skos:notation "247" ;
  skos:notation 247 ;
  skos:note "Note 1 to entry: The geometry of time is discussed in 5.2. [of ISO 19108;2002]"@en ;
  skos:note "비고: 시간의 기하는 KS X ISO 19108의 5.2절에서 기술되어 있다."@kr ;
  skos:prefLabel "instant"@en ;
  skos:prefLabel "인스턴트"@kr ;
.
<http://iso.org/tc211/term/248>
  rdf:type skos:Concept ;
  dcterms:dateAccepted "2005-10-15"^^xsd:date ;
  dcterms:dateAccepted "2006-12-01"^^xsd:date ;
  dcterms:provenance "KS X ISO 19133" ;
  dcterms:source "ISO 19133:2005" ;
  reg:status reg:statusValid ;
  rdfs:comment "Note 1 to entry: A class or data element definition instantiates a type if it creates the ability to create objects or data elements respectively, that can represent the concepts (instance data and /or operations) defined by that type. A class is instantiated by an object if the class defines that object's structure and function. A data schema is instantiated by a data element if the data schema defines that element's structure."@en ;
  rdfs:comment "비고: 만약 클래스 또는 데이터 요소가 객체나 요소를 생성할 수 있다면, 이에 대한 정의는 유형을 인스턴스화하는 것이며, 그 유형을 통해 정의된 개념(인스턴스 데이터, 연산)으로 표현될 수 있다. 만약 클래스가 객체의 구조와 함수를 정의한다면 클래스는 객체에 의해 인스턴스화된다. 만약 데이터 스키마가 요소의 구조를 정의한다면 데이터 스키마는 데이터 요소에 의해 인스턴스화된다."@kr ;
  rdfs:label "instantiate"@en ;
  skos:changeNote "valid" ;
  skos:definition "구체적인 인스턴스를 생성하여 표현(추상화)하거나, 인스턴스를 생성할 수 있도록 하는 것"@kr ;
  skos:editorialNote "preferred" ;
  skos:editorialNote "preferred"^^xsd:string ;
  skos:notation "248" ;
  skos:notation 248 ;
  skos:note "Note 1 to entry: A class or data element definition instantiates a type if it creates the ability to create objects or data elements respectively, that can represent the concepts (instance data and /or operations) defined by that type. A class is instantiated by an object if the class defines that object's structure and function. A data schema is instantiated by a data element if the data schema defines that element's structure."@en ;
  skos:note "비고: 만약 클래스 또는 데이터 요소가 객체나 요소를 생성할 수 있다면, 이에 대한 정의는 유형을 인스턴스화하는 것이며, 그 유형을 통해 정의된 개념(인스턴스 데이터, 연산)으로 표현될 수 있다. 만약 클래스가 객체의 구조와 함수를 정의한다면 클래스는 객체에 의해 인스턴스화된다. 만약 데이터 스키마가 요소의 구조를 정의한다면 데이터 스키마는 데이터 요소에 의해 인스턴스화된다."@kr ;
  skos:prefLabel "instantiate"@en ;
  skos:prefLabel "인스턴스화"@kr ;
.
<http://iso.org/tc211/term/250>
  rdf:type skos:Concept ;
  dcterms:dateAccepted "2004-07-01"^^xsd:date ;
  dcterms:dateAccepted "2004-11-05"^^xsd:date ;
  dcterms:provenance "KS X ISO 19116" ;
  dcterms:source "ISO 19116:2004" ;
  reg:status reg:statusValid ;
  rdfs:comment "Note 1 to entry: The measurements produced by each positioning technology in an integrated system may be any of position, motion, or attitude.  There may be redundant measurements.  When combined, a unified position, motion, or attitude is determined."@en ;
  rdfs:comment "비고: 통합 시스템에서 측위 기술로 측정된 것은 위치, 이동, 또는 자세 등 이다. 중복된 측정이 존재하며, 이들이 결합되었을 때, 통합된 위치, 이동, 자세가 결정된다."@kr ;
  rdfs:label "integrated positioning system"@en ;
  skos:changeNote "valid" ;
  skos:definition "2개 이상의 측위 기술을 통합하는 측위 시스템"@kr ;
  skos:editorialNote "preferred" ;
  skos:editorialNote "preferred"^^xsd:string ;
  skos:notation "250" ;
  skos:notation 250 ;
  skos:note "Note 1 to entry: The measurements produced by each positioning technology in an integrated system may be any of position, motion, or attitude.  There may be redundant measurements.  When combined, a unified position, motion, or attitude is determined."@en ;
  skos:note "비고: 통합 시스템에서 측위 기술로 측정된 것은 위치, 이동, 또는 자세 등 이다. 중복된 측정이 존재하며, 이들이 결합되었을 때, 통합된 위치, 이동, 자세가 결정된다."@kr ;
  skos:prefLabel "integrated positioning system"@en ;
  skos:prefLabel "통합 측위 시스템"@kr ;
.
<http://iso.org/tc211/term/251>
  rdf:type skos:Concept ;
  dcterms:dateAccepted "2005-02-15"^^xsd:date ;
  dcterms:dateAccepted "2009-12-29"^^xsd:date ;
  dcterms:provenance "KS X ISO 19119" ;
  dcterms:source "ISO 19119:2005" ;
  reg:status reg:statusValid ;
  rdfs:comment "Note 1 to entry: See 7.2 [of ISO 19119] for a discussion of interface"@en ;
  rdfs:comment "비고: 인터페이스에 관한 논의는 KS X ISO 19119의 7.2를 참조하라."@kr ;
  rdfs:label "interface"@en ;
  skos:changeNote "valid" ;
  skos:definition "개체의 행태에 대한 특성을 기술하는 명명된 연산 집합"@kr ;
  skos:editorialNote "preferred" ;
  skos:editorialNote "preferred"^^xsd:string ;
  skos:notation "251" ;
  skos:notation 251 ;
  skos:note "Note 1 to entry: See 7.2 [of ISO 19119] for a discussion of interface"@en ;
  skos:note "비고: 인터페이스에 관한 논의는 KS X ISO 19119의 7.2를 참조하라."@kr ;
  skos:prefLabel "interface"@en ;
  skos:prefLabel "인터페이스"@kr ;
.
<http://iso.org/tc211/term/252>
  rdf:type skos:Concept ;
  dcterms:dateAccepted "2005-07-15"^^xsd:date ;
  dcterms:dateAccepted "2009-12-29"^^xsd:date ;
  dcterms:provenance "ISO/TS 19103:2005 ,4.2.16" ;
  dcterms:source "ISO/IEC 19501" ;
  reg:status reg:statusValid ;
  rdfs:label "interface <UML>"@en ;
  skos:changeNote "valid" ;
  skos:definition "요소의 행태에 대한 특성을 기술하는 명명된 연산 집합"@kr ;
  skos:editorialNote "preferred" ;
  skos:editorialNote "preferred"^^xsd:string ;
  skos:notation "252" ;
  skos:notation 252 ;
  skos:prefLabel "interface <UML>"@en ;
  skos:prefLabel "인터페이스 <UML>"@kr ;
.
<http://iso.org/tc211/term/254>
  rdf:type skos:Concept ;
  dcterms:dateAccepted "2003-05-01"^^xsd:date ;
  dcterms:dateAccepted "2009-12-29"^^xsd:date ;
  dcterms:provenance "KS X ISO 19107" ;
  dcterms:source "ISO 19107:2003" ;
  reg:status reg:statusValid ;
  rdfs:comment "Note 1 to entry: The interior of a topological object is the homomorphic image of the interior of any of its geometric realizations. This is not included as a definition because it follows from a theorem of topology."@en ;
  rdfs:comment "비고: 위상 객체의 내부는 그의 기하 실현의 어느 내부와도 준동형 영상이다. 이는 위상 이론을 따르는 것으로 정의에는 포함되지 않는다."@kr ;
  rdfs:label "interior"@en ;
  skos:changeNote "valid" ;
  skos:definition "기하 객체 내에 존재하며, 그 객체의 경계를 제외한 나머지 전체 직접 위치의 집합"@kr ;
  skos:editorialNote "preferred" ;
  skos:editorialNote "preferred"^^xsd:string ;
  skos:notation "254" ;
  skos:notation 254 ;
  skos:note "Note 1 to entry: The interior of a topological object is the homomorphic image of the interior of any of its geometric realizations. This is not included as a definition because it follows from a theorem of topology."@en ;
  skos:note "비고: 위상 객체의 내부는 그의 기하 실현의 어느 내부와도 준동형 영상이다. 이는 위상 이론을 따르는 것으로 정의에는 포함되지 않는다."@kr ;
  skos:prefLabel "interior"@en ;
  skos:prefLabel "내부"@kr ;
.
<http://iso.org/tc211/term/255>
  rdf:type skos:Concept ;
  dcterms:dateAccepted "2005-02-15" ;
  dcterms:dateAccepted "2005-02-15"^^xsd:date ;
  dcterms:dateAccepted "2008-12-19"^^xsd:date ;
  dcterms:provenance "ISO 19119:2005" ;
  dcterms:provenance "KS X ISO 19104" ;
  dcterms:provenance "NEN 3610" ;
  dcterms:source "ISO/IEC 2382-1:1993" ;
  reg:status reg:statusAccepted ;
  reg:status reg:statusValid ;
  rdfs:label "interoperability"@en ;
  skos:changeNote "valid" ;
  skos:definition "mogelijkheid van verschillende autonome, heterogene eenheden, systemen of partijen om met elkaar te communiceren en interacteren"@nl ;
  skos:definition "사용자가 기능적 구성 단위들의 고유 특성을 알지 못해도, 다양한 구성 단위 간의 데이터 전송, 프로그램 실행, 의사소통을 가능하게 하는 성능"@kr ;
  skos:editorialNote "preferred" ;
  skos:editorialNote "preferred"^^xsd:string ;
  skos:notation "255" ;
  skos:notation 255 ;
  skos:prefLabel "interoperabiliteit"@nl ;
  skos:prefLabel "interoperability"@en ;
  skos:prefLabel "상호 운용성"@kr ;
.
<http://iso.org/tc211/term/256>
  rdf:type skos:Concept ;
  dcterms:dateAccepted "2002-09-01"^^xsd:date ;
  dcterms:dateAccepted "2007-11-01"^^xsd:date ;
  dcterms:provenance "KS X ISO 19108" ;
  dcterms:source "ISO 19108;2002" ;
  reg:status reg:statusValid ;
  rdfs:comment "Note 1 to entry: Ratios of values measured on an interval scale have no meaning."@en ;
  rdfs:comment "비고: 간격 척도로 측정된 값의 비율은 의미가 없다."@kr ;
  rdfs:label "interval scale"@en ;
  skos:changeNote "valid" ;
  skos:definition "값의 순서와 값 사이의 거리 차를 설명하는 데 사용할 수 있는 임의의 원점을 가진 척도"@kr ;
  skos:editorialNote "preferred" ;
  skos:editorialNote "preferred"^^xsd:string ;
  skos:notation "256" ;
  skos:notation 256 ;
  skos:note "Note 1 to entry: Ratios of values measured on an interval scale have no meaning."@en ;
  skos:note "비고: 간격 척도로 측정된 값의 비율은 의미가 없다."@kr ;
  skos:prefLabel "interval scale"@en ;
  skos:prefLabel "간격 척도"@kr ;
.
<http://iso.org/tc211/term/257>
  rdf:type skos:Concept ;
  dcterms:dateAccepted "2005-08-15"^^xsd:date ;
  dcterms:dateAccepted "2007-11-01"^^xsd:date ;
  dcterms:provenance "KS X ISO 19123" ;
  dcterms:source "ISO 19123:2005" ;
  reg:status reg:statusValid ;
  rdfs:label "inverse evaluation<coverage>"@en ;
  skos:changeNote "valid" ;
  skos:definition "연관된 피처 속성 값에 근거하여 커버리지 영역에서 객체 집합을 선택하는 것"@kr ;
  skos:editorialNote "preferred" ;
  skos:editorialNote "preferred"^^xsd:string ;
  skos:notation "257" ;
  skos:notation 257 ;
  skos:prefLabel "inverse evaluation<coverage>"@en ;
  skos:prefLabel "역산출 <커버리지>"@kr ;
.
<http://iso.org/tc211/term/258>
  rdf:type skos:Concept ;
  dcterms:dateAccepted "2003-05-01"^^xsd:date ;
  dcterms:dateAccepted "2009-12-29"^^xsd:date ;
  dcterms:provenance "KS X ISO 19107" ;
  dcterms:source "ISO 19107:2003" ;
  reg:status reg:statusValid ;
  rdfs:label "isolated node"@en ;
  skos:changeNote "valid" ;
  skos:definition "어느 변에도 결합되어 있지 않은 절점"@kr ;
  skos:editorialNote "preferred" ;
  skos:editorialNote "preferred"^^xsd:string ;
  skos:notation "258" ;
  skos:notation 258 ;
  skos:prefLabel "isolated node"@en ;
  skos:prefLabel "고립 절점"@kr ;
.
<http://iso.org/tc211/term/259>
  rdf:type skos:Concept ;
  dcterms:dateAccepted "2003-05-01"^^xsd:date ;
  dcterms:dateAccepted "2009-12-29"^^xsd:date ;
  dcterms:provenance "KS X ISO 19107" ;
  dcterms:source "ISO 19107:2003" ;
  reg:status reg:statusValid ;
  rdfs:comment "Note 1 to entry: A geometric complex is isomorphic to a topological complex if their elements are in a 1-to-1, dimension- and boundary-preserving correspondence to one another."@en ;
  rdfs:comment "비고: 기하 복합체는 만일 그 요소가 서로 일 대 일로 차원 및 경계 보존 대응 관계에 있다면, 위상 복합체와 동형이다."@kr ;
  rdfs:label "isomorphism"@en ;
  skos:changeNote "valid" ;
  skos:definition "두 영역(예: 두 개의 복합체)이 일 대 일로 대응되며, 각 영역 간에 구조 보존 함수와 두 함수의 합성이 양방향으로 대응하는 식별 특성 함수 관계"@kr ;
  skos:editorialNote "preferred" ;
  skos:editorialNote "preferred"^^xsd:string ;
  skos:notation "259" ;
  skos:notation 259 ;
  skos:note "Note 1 to entry: A geometric complex is isomorphic to a topological complex if their elements are in a 1-to-1, dimension- and boundary-preserving correspondence to one another."@en ;
  skos:note "비고: 기하 복합체는 만일 그 요소가 서로 일 대 일로 차원 및 경계 보존 대응 관계에 있다면, 위상 복합체와 동형이다."@kr ;
  skos:prefLabel "isomorphism"@en ;
  skos:prefLabel "동형"@kr ;
.
<http://iso.org/tc211/term/26>
  rdf:type skos:Concept ;
  dcterms:dateAccepted "2004-07-01"^^xsd:date ;
  dcterms:dateAccepted "2009-12-29"^^xsd:date ;
  dcterms:provenance "KS X ISO 19106" ;
  dcterms:source "ISO 19106:2004" ;
  reg:status reg:statusValid ;
  rdfs:label "base standard"@en ;
  skos:changeNote "valid" ;
  skos:definition "하나의 프로파일을 구성하는 데 활용될 수 있는 KS(ISO) 지리 정보 표준 또는 이외의 정보 기술 표준"@kr ;
  skos:editorialNote "preferred" ;
  skos:editorialNote "preferred"^^xsd:string ;
  skos:notation "26" ;
  skos:notation 26 ;
  skos:prefLabel "base standard"@en ;
  skos:prefLabel "기반 표준"@kr ;
.
<http://iso.org/tc211/term/260>
  rdf:type skos:Concept ;
  dcterms:dateAccepted "2003-08-15"^^xsd:date ;
  dcterms:dateAccepted "2008-12-19"^^xsd:date ;
  dcterms:provenance "ISO 19114:2003 ,4.7" ;
  dcterms:source "ISO 2859-1" ;
  reg:status reg:statusRetired ;
  rdfs:comment "Note 1 to entry: An item can be any part of a dataset, such as a feature, feature relationship, feature attribute, or combination of these."@en ;
  rdfs:comment "비고: 피처, 피처 관계, 피처 속성 또는 이것들의 조합과 같은 데이터셋의 특정 부분이 항목이 될 수 있다. "@kr ;
  rdfs:label "item"@en ;
  skos:changeNote "retired" ;
  skos:definition "개별적으로 기술될 수 있거나, 고려될 수 있는 것"@kr ;
  skos:notation "260" ;
  skos:notation 260 ;
  skos:note "Note 1 to entry: An item can be any part of a dataset, such as a feature, feature relationship, feature attribute, or combination of these."@en ;
  skos:note "비고: 피처, 피처 관계, 피처 속성 또는 이것들의 조합과 같은 데이터셋의 특정 부분이 항목이 될 수 있다. "@kr ;
  skos:prefLabel "item"@en ;
  skos:prefLabel "항목"@kr ;
.
<http://iso.org/tc211/term/261>
  rdf:type skos:Concept ;
  dcterms:dateAccepted "2005-10-15"^^xsd:date ;
  dcterms:dateAccepted "2009-12-29"^^xsd:date ;
  dcterms:provenance "KS X ISO 19135" ;
  dcterms:source "ISO 19135:2005" ;
  reg:status reg:statusValid ;
  rdfs:comment "Note 1 to entry: Class is used in this context to refer to a set of instances, not the concept abstracted from that set of instances."@en ;
  rdfs:comment "비고: 여기서 클래스는 인스턴스 집합의 추상화된 개념이 아닌, 인스턴스 집합을 언급하기 위해 사용된다."@kr ;
  rdfs:label "item class"@en ;
  skos:changeNote "valid" ;
  skos:definition "공통의 특성을 갖는 항목의 집합"@kr ;
  skos:editorialNote "preferred" ;
  skos:editorialNote "preferred"^^xsd:string ;
  skos:notation "261" ;
  skos:notation 261 ;
  skos:note "Note 1 to entry: Class is used in this context to refer to a set of instances, not the concept abstracted from that set of instances."@en ;
  skos:note "비고: 여기서 클래스는 인스턴스 집합의 추상화된 개념이 아닌, 인스턴스 집합을 언급하기 위해 사용된다."@kr ;
  skos:prefLabel "item class"@en ;
  skos:prefLabel "항목 클래스"@kr ;
.
<http://iso.org/tc211/term/263>
  rdf:type skos:Concept ;
  dcterms:dateAccepted "2002-09-01"^^xsd:date ;
  dcterms:dateAccepted "2007-11-01"^^xsd:date ;
  dcterms:provenance "KS X ISO 19108" ;
  dcterms:source "ISO 19108;2002" ;
  reg:status reg:statusValid ;
  rdfs:label "Julian date"@en ;
  skos:changeNote "valid" ;
  skos:definition "전날 정오 이후 경과한 날을 소수로 표현한 율리우스 일수"@kr ;
  skos:editorialNote "preferred" ;
  skos:editorialNote "preferred"^^xsd:string ;
  skos:notation "263" ;
  skos:notation 263 ;
  skos:prefLabel "Julian date"@en ;
  skos:prefLabel "율리우스날짜"@kr ;
.
<http://iso.org/tc211/term/264>
  rdf:type skos:Concept ;
  dcterms:dateAccepted "2002-09-01"^^xsd:date ;
  dcterms:dateAccepted "2007-11-01"^^xsd:date ;
  dcterms:provenance "KS X ISO 19108" ;
  dcterms:source "ISO 19108;2002" ;
  reg:status reg:statusValid ;
  rdfs:label "Julian day number"@en ;
  skos:changeNote "valid" ;
  skos:definition "기원전 4713년 1월 1일 그린위치 평균 정오 이후 경과한 일수, 율리우스 예상 달력"@kr ;
  skos:editorialNote "preferred" ;
  skos:editorialNote "preferred"^^xsd:string ;
  skos:notation "264" ;
  skos:notation 264 ;
  skos:prefLabel "Julian day number"@en ;
  skos:prefLabel "율리우스 일수"@kr ;
.
<http://iso.org/tc211/term/265>
  rdf:type skos:Concept ;
  dcterms:dateAccepted "2005-10-15"^^xsd:date ;
  dcterms:dateAccepted "2006-12-01"^^xsd:date ;
  dcterms:provenance "KS X ISO 19133" ;
  dcterms:source "ISO 19133:2005" ;
  reg:status reg:statusValid ;
  rdfs:comment "Note 1 to entry: Junction is an alias for node."@en ;
  rdfs:comment "비고: 교차점은 절점의 별칭이다."@kr ;
  rdfs:label "junction"@en ;
  skos:changeNote "valid" ;
  skos:definition "진입 및 진출 링크와 회전의 관련 모음으로 구성된 네트워크상의 단일 위상 절점"@kr ;
  skos:editorialNote "preferred" ;
  skos:editorialNote "preferred"^^xsd:string ;
  skos:notation "265" ;
  skos:notation 265 ;
  skos:note "Note 1 to entry: Junction is an alias for node."@en ;
  skos:note "비고: 교차점은 절점의 별칭이다."@kr ;
  skos:prefLabel "junction"@en ;
  skos:prefLabel "교차점"@kr ;
.
<http://iso.org/tc211/term/266>
  rdf:type skos:Concept ;
  dcterms:dateAccepted "2008-11-15"^^xsd:date ;
  dcterms:provenance "ISO/TS 19104:2008" ;
  dcterms:source "ISO 1087-1:2000" ;
  reg:status reg:statusValid ;
  rdfs:label "language identifier"@en ;
  skos:changeNote "valid" ;
  skos:editorialNote "preferred"^^xsd:string ;
  skos:notation 266 ;
  skos:prefLabel "language identifier"@en ;
.
<http://iso.org/tc211/term/267>
  rdf:type skos:Concept ;
  dcterms:dateAccepted "2005-12-01"^^xsd:date ;
  dcterms:dateAccepted "2009-12-29"^^xsd:date ;
  dcterms:provenance "KS X ISO 19128" ;
  dcterms:source "ISO 19128:2005" ;
  reg:status reg:statusValid ;
  rdfs:label "layer"@en ;
  skos:changeNote "valid" ;
  skos:definition "서버에서 지도로 요청될 수 있는 지리 정보의 기본 단위"@kr ;
  skos:editorialNote "preferred" ;
  skos:editorialNote "preferred"^^xsd:string ;
  skos:notation "267" ;
  skos:notation 267 ;
  skos:prefLabel "layer"@en ;
  skos:prefLabel "레이어"@kr ;
.
<http://iso.org/tc211/term/268>
  rdf:type skos:Concept ;
  dcterms:dateAccepted "2002-07-01"^^xsd:date ;
  dcterms:dateAccepted "2008-12-30"^^xsd:date ;
  dcterms:provenance "ISO 19101:2002" ;
  dcterms:source "ISO 19101-1:2014, 4.1.24" ;
  reg:status reg:statusValid ;
  rdfs:label "lexical language"@en ;
  skos:changeNote "valid" ;
  skos:definition "문자열로 정의된 기호를 통해 표현되는 문법을 갖는 언어"@kr ;
  skos:editorialNote "preferred" ;
  skos:editorialNote "preferred"^^xsd:string ;
  skos:notation "268" ;
  skos:notation 268 ;
  skos:prefLabel "lexical language"@en ;
  skos:prefLabel "어휘 언어"@kr ;
.
<http://iso.org/tc211/term/269>
  rdf:type skos:Concept ;
  dcterms:dateAccepted "2002-09-01"^^xsd:date ;
  dcterms:dateAccepted "2007-11-01"^^xsd:date ;
  dcterms:provenance "KS X ISO 19108" ;
  dcterms:source "ISO 19108;2002" ;
  reg:status reg:statusValid ;
  rdfs:comment "Note 1 to entry: Valid-time life span is the period during which an object exists in the modelled reality.  Transaction-time life span is the period during which a database object is current in the database."@en ;
  rdfs:comment "비고: 유효 시간 수명은 모델링된 현실에서 객체가 존재하는 동안의 기간이다. 처리 시간 수명은 데이터 베이스 객체가 데이터 베이스에서 통용되는 기간이다."@kr ;
  rdfs:label "life span"@en ;
  skos:changeNote "valid" ;
  skos:definition "어떤 대상이 존재하는 기간"@kr ;
  skos:editorialNote "preferred" ;
  skos:editorialNote "preferred"^^xsd:string ;
  skos:notation "269" ;
  skos:notation 269 ;
  skos:note "Note 1 to entry: Valid-time life span is the period during which an object exists in the modelled reality.  Transaction-time life span is the period during which a database object is current in the database."@en ;
  skos:note "비고: 유효 시간 수명은 모델링된 현실에서 객체가 존재하는 동안의 기간이다. 처리 시간 수명은 데이터 베이스 객체가 데이터 베이스에서 통용되는 기간이다."@kr ;
  skos:prefLabel "life span"@en ;
  skos:prefLabel "수명"@kr ;
.
<http://iso.org/tc211/term/27>
  rdf:type skos:Concept ;
  dcterms:dateAccepted "2000-12-15"^^xsd:date ;
  dcterms:dateAccepted "2007-06-29"^^xsd:date ;
  dcterms:provenance "KS X ISO 19105" ;
  dcterms:source "ISO 19105:2000" ;
  reg:status reg:statusValid ;
  rdfs:label "basic test"@en ;
  skos:changeNote "valid" ;
  skos:definition "부적합 경우와 적합한 경우를 명확하게 식별하기 위해 실시하는 최초의 기능 시험"@kr ;
  skos:editorialNote "preferred" ;
  skos:editorialNote "preferred"^^xsd:string ;
  skos:notation "27" ;
  skos:notation 27 ;
  skos:prefLabel "basic test"@en ;
  skos:prefLabel "기본 시험"@kr ;
.
<http://iso.org/tc211/term/270>
  rdf:type skos:Concept ;
  dcterms:dateAccepted "2007-09-01"^^xsd:date ;
  dcterms:dateAccepted "2009-12-29"^^xsd:date ;
  dcterms:provenance "KS X ISO 19136" ;
  dcterms:source "ISO 19136:2007" ;
  reg:status reg:statusValid ;
  rdfs:label "line string"@en ;
  skos:changeNote "valid" ;
  skos:definition "직선 조각으로 구성된 곡선"@kr ;
  skos:editorialNote "preferred" ;
  skos:editorialNote "preferred"^^xsd:string ;
  skos:notation "270" ;
  skos:notation 270 ;
  skos:prefLabel "line string"@en ;
  skos:prefLabel "선열"@kr ;
.
<http://iso.org/tc211/term/271>
  rdf:type skos:Concept ;
  dcterms:dateAccepted "2004-07-01"^^xsd:date ;
  dcterms:dateAccepted "2004-11-05"^^xsd:date ;
  dcterms:provenance "KS X ISO 19116" ;
  dcterms:source "ISO 19116:2004" ;
  reg:status reg:statusValid ;
  rdfs:label "linear positioning system"@en ;
  skos:changeNote "valid" ;
  skos:definition "참조 점으로부터 경로를 따라 거리를 측정하는 측위 시스템"@kr ;
  skos:editorialNote "preferred" ;
  skos:editorialNote "preferred"^^xsd:string ;
  skos:notation "271" ;
  skos:notation 271 ;
  skos:prefLabel "linear positioning system"@en ;
  skos:prefLabel "선형 측위 시스템"@kr ;
.
<http://iso.org/tc211/term/272>
  rdf:type skos:Concept ;
  dcterms:dateAccepted "2004-07-01"^^xsd:date ;
  dcterms:dateAccepted "2004-11-05"^^xsd:date ;
  dcterms:provenance "KS X ISO 19116" ;
  dcterms:source "ISO 19116:2004" ;
  reg:status reg:statusValid ;
  rdfs:comment "Note 1 to entry: Linear reference systems are widely used in transportation, for example highway names and mile or kilometre markers."@en ;
  rdfs:comment "비고: 선형 참조 체계는 운송(예를 들어 고속도로명과 마일 또는 킬로미터의 이정표)에 널리 사용된다"@kr ;
  rdfs:label "linear reference system"@en ;
  skos:changeNote "valid" ;
  skos:definition "선형 지리 피처의 조각과 그 조각에 위치한 점까지의 거리를 통해 위치를 식별하는 참조 체계"@kr ;
  skos:editorialNote "preferred" ;
  skos:editorialNote "preferred"^^xsd:string ;
  skos:notation "272" ;
  skos:notation 272 ;
  skos:note "Note 1 to entry: Linear reference systems are widely used in transportation, for example highway names and mile or kilometre markers."@en ;
  skos:note "비고: 선형 참조 체계는 운송(예를 들어 고속도로명과 마일 또는 킬로미터의 이정표)에 널리 사용된다"@kr ;
  skos:prefLabel "linear reference system"@en ;
  skos:prefLabel "선형 참조 체계"@kr ;
.
<http://iso.org/tc211/term/273>
  rdf:type skos:Concept ;
  dcterms:dateAccepted "2005-10-15"^^xsd:date ;
  dcterms:dateAccepted "2006-12-01"^^xsd:date ;
  dcterms:source "ISO 19133:2005, 4.7" ;
  reg:status reg:statusSuperseded ;
  rdfs:comment "Note 1 to entry:The system includes the complete set of procedures for determining and retaining a record of specific points along a linear feature such as the location reference method(s) together with the procedures for storing, maintaining, and retrieving location information about points and segments on the highways. [NCHRP Synthesis 21, 1974]"@en ;
  rdfs:comment "비고: 고속도로상의 점들이나 구간에 관한 위치 정보를 검색, 유지 관리, 저장하는 위치 참조 방법과 같이, 시스템은 하나의 선형피처를 따라 있는 특정 점들의 레코드들을 결정하고 보유하는 일련의 전체 절차들을 포함한다."@kr ;
  rdfs:label "linear referencing system"@en ;
  skos:changeNote "superseded" ;
  skos:definition "참조 점으로부터 경로를 따라 거리를 측정하는 측위 시스템"@kr ;
  skos:notation "273" ;
  skos:notation 273 ;
  skos:note "Note 1 to entry:The system includes the complete set of procedures for determining and retaining a record of specific points along a linear feature such as the location reference method(s) together with the procedures for storing, maintaining, and retrieving location information about points and segments on the highways. [NCHRP Synthesis 21, 1974]"@en ;
  skos:note "비고: 고속도로상의 점들이나 구간에 관한 위치 정보를 검색, 유지 관리, 저장하는 위치 참조 방법과 같이, 시스템은 하나의 선형피처를 따라 있는 특정 점들의 레코드들을 결정하고 보유하는 일련의 전체 절차들을 포함한다."@kr ;
  skos:prefLabel "linear referencing system"@en ;
  skos:prefLabel "선형 참조 시스템"@kr ;
.
<http://iso.org/tc211/term/274>
  rdf:type skos:Concept ;
  dcterms:dateAccepted "2005-10-15"^^xsd:date ;
  dcterms:dateAccepted "2006-12-01"^^xsd:date ;
  dcterms:provenance "KS X ISO 19133" ;
  dcterms:source "ISO 19133:2005" ;
  reg:status reg:statusValid ;
  rdfs:comment "Note 1 to entry: Link is an alias for directed edge."@en ;
  rdfs:comment "비고: 링크는 방향성 변의 별칭이다."@kr ;
  rdfs:label "link"@en ;
  skos:changeNote "valid" ;
  skos:definition "변과 방향으로 구성되어 있는, 두 절점(교차점) 간의 방향성 있는 위상적 연결"@kr ;
  skos:editorialNote "preferred" ;
  skos:editorialNote "preferred"^^xsd:string ;
  skos:notation "274" ;
  skos:notation 274 ;
  skos:note "Note 1 to entry: Link is an alias for directed edge."@en ;
  skos:note "비고: 링크는 방향성 변의 별칭이다."@kr ;
  skos:prefLabel "link"@en ;
  skos:prefLabel "링크"@kr ;
.
<http://iso.org/tc211/term/275>
  rdf:type skos:Concept ;
  dcterms:dateAccepted "2005-10-15"^^xsd:date ;
  dcterms:dateAccepted "2006-12-01"^^xsd:date ;
  dcterms:provenance "KS X ISO 19133" ;
  dcterms:source "ISO 19133:2005" ;
  reg:status reg:statusValid ;
  rdfs:comment "Note 1 to entry: Link positions are often associated with a target feature that is not part of the network. The most common link measures used for this are the distance from start node or address. The most common use of a link position is to geolocate an \"address.\""@en ;
  rdfs:comment "비고: 링크 위치는 종종 네트워크 내에 없는 대상 피처에 연관된다. 이 경우, 출발점이나 주소로부터의 거리가 가장 일반적인 링크측정으로 사용된다.  \"주소\"를 지리적 위치화하는 것이 가장 일반적인 링크 위치로 사용된다.   "@kr ;
  rdfs:label "link position"@en ;
  skos:changeNote "valid" ;
  skos:definition "해당 링크에 대해 엄격한 단일 측정을 통해 정의된 링크상의 네트워크 내 위치"@kr ;
  skos:editorialNote "preferred" ;
  skos:editorialNote "preferred"^^xsd:string ;
  skos:notation "275" ;
  skos:notation 275 ;
  skos:note "Note 1 to entry: Link positions are often associated with a target feature that is not part of the network. The most common link measures used for this are the distance from start node or address. The most common use of a link position is to geolocate an \"address.\""@en ;
  skos:note "비고: 링크 위치는 종종 네트워크 내에 없는 대상 피처에 연관된다. 이 경우, 출발점이나 주소로부터의 거리가 가장 일반적인 링크측정으로 사용된다.  \"주소\"를 지리적 위치화하는 것이 가장 일반적인 링크 위치로 사용된다.   "@kr ;
  skos:prefLabel "link position"@en ;
  skos:prefLabel "링크 위치"@kr ;
.
<http://iso.org/tc211/term/276>
  rdf:type skos:Concept ;
  dcterms:dateAccepted "2003-10-15"^^xsd:date ;
  dcterms:dateAccepted "2009-12-29"^^xsd:date ;
  dcterms:provenance "KS X ISO 19112" ;
  dcterms:source "ISO 19112:2003" ;
  reg:status reg:statusValid ;
  rdfs:label "location"@en ;
  skos:changeNote "valid" ;
  skos:definition "식별 가능한 지리적 장소"@kr ;
  skos:editorialNote "preferred" ;
  skos:editorialNote "preferred"^^xsd:string ;
  skos:notation "276" ;
  skos:notation 276 ;
  skos:prefLabel "location"@en ;
  skos:prefLabel "위치"@kr ;
.
<http://iso.org/tc211/term/278>
  rdf:type skos:Concept ;
  dcterms:dateAccepted "2005-10-15"^^xsd:date ;
  dcterms:dateAccepted "2006-12-01"^^xsd:date ;
  dcterms:provenance "KS X ISO 19133" ;
  dcterms:source "ISO 19133:2005" ;
  reg:status reg:statusValid ;
  rdfs:label "location based service"@en ;
  skos:altLabel "LBS"@kr ;
  skos:altLabel "LBS"^^<http://www.w3.org/2001/XMLSchema#@en> ;
  skos:changeNote "valid" ;
  skos:definition "서비스를 요구하는 클라이언트, 객체, 사람 등의 위치에 따라 서비스의 응답이나 기타 특성이 결정되는 서비스 "@kr ;
  skos:editorialNote "preferred" ;
  skos:editorialNote "preferred"^^xsd:string ;
  skos:notation "278" ;
  skos:notation 278 ;
  skos:prefLabel "location based service"@en ;
  skos:prefLabel "위치 기반 서비스"@kr ;
.
<http://iso.org/tc211/term/279>
  rdf:type skos:Concept ;
  dcterms:dateAccepted "2005-10-15"^^xsd:date ;
  dcterms:dateAccepted "2006-12-01"^^xsd:date ;
  dcterms:provenance "KS X ISO 19133" ;
  dcterms:source "ISO 19133:2005" ;
  reg:status reg:statusValid ;
  rdfs:label "location dependent service"@en ;
  skos:altLabel "LDS"@kr ;
  skos:altLabel "LDS"^^<http://www.w3.org/2001/XMLSchema#@en> ;
  skos:changeNote "valid" ;
  skos:definition "클라이언트 위치에 따라 서비스의 활용 여부가 결정되는 서비스"@kr ;
  skos:editorialNote "preferred" ;
  skos:editorialNote "preferred"^^xsd:string ;
  skos:notation "279" ;
  skos:notation 279 ;
  skos:prefLabel "location dependent service"@en ;
  skos:prefLabel "위치 종속 서비스"@kr ;
.
<http://iso.org/tc211/term/28>
  rdf:type skos:Concept ;
  dcterms:dateAccepted "2005-07-15"^^xsd:date ;
  dcterms:dateAccepted "2009-12-29"^^xsd:date ;
  dcterms:provenance "ISO/TS 19103:2005" ;
  dcterms:provenance "KS X ISO 19103" ;
  dcterms:source "ISO/IEC 19501:2005 (Adapted from)" ;
  reg:status reg:statusValid ;
  rdfs:label "behaviour <UML>"@en ;
  skos:changeNote "valid" ;
  skos:definition "연산, 사건 또는 그 결과 값까지 포함하여 관측 가능한 효과"@kr ;
  skos:editorialNote "preferred" ;
  skos:editorialNote "preferred"^^xsd:string ;
  skos:notation "28" ;
  skos:notation 28 ;
  skos:prefLabel "behaviour <UML>"@en ;
  skos:prefLabel "행태 <UML>"@kr ;
.
<http://iso.org/tc211/term/280>
  rdf:type skos:Concept ;
  dcterms:dateAccepted "2005-10-15"^^xsd:date ;
  dcterms:dateAccepted "2006-12-01"^^xsd:date ;
  dcterms:provenance "KS X ISO 19133" ;
  dcterms:source "ISO 19133:2005" ;
  reg:status reg:statusValid ;
  rdfs:comment "Note 1 to entry: This rule represents what is \"most natural\" to do at a node (intersection), given the entry link used. The most common version is \"as straight as possible\", or to exit a turn on the most obvious extension of the entry street, which is usually, but not always, the same named street that was the entry. Every node in a route is either associated with an instruction or can be navigated by the main-road rule."@en ;
  rdfs:comment "비고: 이 규칙은 주어진 입구 링크로 사용된 하나의 절점(교차점)에서 무엇을 하는 것이 \"가장 자연스러운가\"를 나타낸다. 가장 일반적인 버전은 \"가능한 한 직진\"이다. 또는 가장 확실한 진입 거리 확장에서 회전해서 나가는 것이다. 이때 진입 거리는 반드시 항상은 아니지만, 보통 진입했던 동일한 이름을 가진 거리이다. 하나의 경로에서의 모든 절점은 하나의 지시에 연관되거나, 혹은 주요 도로규칙에 의해 내비게이션될 수 있다."@kr ;
  rdfs:label "main-road rule"@en ;
  skos:changeNote "valid" ;
  skos:definition "경로 지시 대신에 차량의 회전에 사용되는 기준들의 집합; 절점에 사용된 기본지시"@kr ;
  skos:editorialNote "preferred" ;
  skos:editorialNote "preferred"^^xsd:string ;
  skos:notation "280" ;
  skos:notation 280 ;
  skos:note "Note 1 to entry: This rule represents what is \"most natural\" to do at a node (intersection), given the entry link used. The most common version is \"as straight as possible\", or to exit a turn on the most obvious extension of the entry street, which is usually, but not always, the same named street that was the entry. Every node in a route is either associated with an instruction or can be navigated by the main-road rule."@en ;
  skos:note "비고: 이 규칙은 주어진 입구 링크로 사용된 하나의 절점(교차점)에서 무엇을 하는 것이 \"가장 자연스러운가\"를 나타낸다. 가장 일반적인 버전은 \"가능한 한 직진\"이다. 또는 가장 확실한 진입 거리 확장에서 회전해서 나가는 것이다. 이때 진입 거리는 반드시 항상은 아니지만, 보통 진입했던 동일한 이름을 가진 거리이다. 하나의 경로에서의 모든 절점은 하나의 지시에 연관되거나, 혹은 주요 도로규칙에 의해 내비게이션될 수 있다."@kr ;
  skos:prefLabel "main-road rule"@en ;
  skos:prefLabel "주요 도로 규칙"@kr ;
.
<http://iso.org/tc211/term/281>
  rdf:type skos:Concept ;
  dcterms:dateAccepted "2005-10-15"^^xsd:date ;
  dcterms:dateAccepted "2006-12-01"^^xsd:date ;
  dcterms:provenance "KS X ISO 19133" ;
  dcterms:source "ISO 19133:2005" ;
  reg:status reg:statusValid ;
  rdfs:comment "Note 1 to entry: Maneuvers are used to cluster turns into convenient and legal combinations. They may be as simple as a single turn, a combination of quick turns (\"jogs\" in the American mid-west consisting of a turn followed immediately by a turn in the opposite direction) or very complex combinations consisting of entry, exit, and connecting roadways  (\"magic roundabouts\" in the UK)."@en ;
  rdfs:comment "비고: 기동은 편리하고 정당한 조합으로 회전을 군집화하는 데 사용된다. 이는 단일 회전과 빠른 회전들의 조합(회전하고 즉시 반대 방향으로 회전하는 미국 중서부에서는 \"jogs\")처럼 단순할 수도 있고, 혹은 입구, 출구 및 연결 도로(영국의\"magicroundabouts\")로 구성되는 매우 복잡한 조합일 수 있다."@kr ;
  rdfs:label "maneuver,manœuvre"@en ;
  skos:changeNote "valid" ;
  skos:definition "경로의 조합에 사용된 관련 링크와 회전의 모음"@kr ;
  skos:editorialNote "preferred" ;
  skos:editorialNote "preferred"^^xsd:string ;
  skos:notation "281" ;
  skos:notation 281 ;
  skos:note "Note 1 to entry: Maneuvers are used to cluster turns into convenient and legal combinations. They may be as simple as a single turn, a combination of quick turns (\"jogs\" in the American mid-west consisting of a turn followed immediately by a turn in the opposite direction) or very complex combinations consisting of entry, exit, and connecting roadways  (\"magic roundabouts\" in the UK)."@en ;
  skos:note "비고: 기동은 편리하고 정당한 조합으로 회전을 군집화하는 데 사용된다. 이는 단일 회전과 빠른 회전들의 조합(회전하고 즉시 반대 방향으로 회전하는 미국 중서부에서는 \"jogs\")처럼 단순할 수도 있고, 혹은 입구, 출구 및 연결 도로(영국의\"magicroundabouts\")로 구성되는 매우 복잡한 조합일 수 있다."@kr ;
  skos:prefLabel "maneuver,manœuvre"@en ;
  skos:prefLabel "기동"@kr ;
.
<http://iso.org/tc211/term/282>
  rdf:type skos:Concept ;
  dcterms:dateAccepted "2005-12-01"^^xsd:date ;
  dcterms:dateAccepted "2009-12-29"^^xsd:date ;
  dcterms:provenance "KS X ISO 19128" ;
  dcterms:source "ISO 19128:2005" ;
  reg:status reg:statusValid ;
  rdfs:label "map"@en ;
  skos:changeNote "valid" ;
  skos:definition "지리 정보를 컴퓨터 화면에 표시하기 적합한 수치 영상 파일로 묘화한 것"@kr ;
  skos:editorialNote "preferred" ;
  skos:editorialNote "preferred"^^xsd:string ;
  skos:notation "282" ;
  skos:notation 282 ;
  skos:prefLabel "map"@en ;
  skos:prefLabel "지도"@kr ;
.
<http://iso.org/tc211/term/284>
  rdf:type skos:Concept ;
  dcterms:dateAccepted "2003-02-15" ;
  dcterms:dateAccepted "2003-02-15"^^xsd:date ;
  dcterms:dateAccepted "2007-11-01"^^xsd:date ;
  dcterms:provenance "ISO 19111:2003" ;
  dcterms:provenance "KS X ISO 19111" ;
  dcterms:source "ISO 19111:2007" ;
  reg:status reg:statusAccepted ;
  reg:status reg:statusValid ;
  rdfs:comment "Note 1 to entry: Mean sea level in a local context normally means mean sea level for the region calculated from observations at one or more points over a given period of time. Mean sea level in a global context differs from a global geoid by not more than 2 m."@en ;
  rdfs:comment "OPMERKING Gemiddeld zeeniveau in de lokale context betekent meestal het gemiddeld zeeniveau voor die regio berekend uit waarnemingen op één of meer punten over een gegeven tijdvak. Gemiddeld zeeniveau in de globale context verschilt nooit meer dan 2 meter van de globale geoïde."@en ;
  rdfs:comment "비고: 통상, 지역적 의미로 평균 해수면은, 하나 이상의 지점을 일정한 기간 동안 관측한 그 영역의 평균 해수면을 말한다. 전지구적인 의미로 평균 해수면은 전지구적인 지오이드와 2m 이하의 차로 받아들여진다."@kr ;
  rdfs:label "mean sea level"@en ;
  skos:changeNote "valid" ;
  skos:definition "gemiddeld niveau van het oppervlak van de zee over alle getijfasen en seizoensgebonden variaties"@nl ;
  skos:definition "모든 단계의 조수위와 계절 변화에 대한 해수면의 평균 높이"@kr ;
  skos:editorialNote "preferred" ;
  skos:editorialNote "preferred"^^xsd:string ;
  skos:notation "284" ;
  skos:notation 284 ;
  skos:note "Note 1 to entry: Mean sea level in a local context normally means mean sea level for the region calculated from observations at one or more points over a given period of time. Mean sea level in a global context differs from a global geoid by not more than 2 m."@en ;
  skos:note "OPMERKING Gemiddeld zeeniveau in de lokale context betekent meestal het gemiddeld zeeniveau voor die regio berekend uit waarnemingen op één of meer punten over een gegeven tijdvak. Gemiddeld zeeniveau in de globale context verschilt nooit meer dan 2 meter van de globale geoïde."@en ;
  skos:note "비고: 통상, 지역적 의미로 평균 해수면은, 하나 이상의 지점을 일정한 기간 동안 관측한 그 영역의 평균 해수면을 말한다. 전지구적인 의미로 평균 해수면은 전지구적인 지오이드와 2m 이하의 차로 받아들여진다."@kr ;
  skos:prefLabel "gemiddeld zeeniveau"@nl ;
  skos:prefLabel "mean sea level"@en ;
  skos:prefLabel "평균 해수면"@kr ;
.
<http://iso.org/tc211/term/286>
  rdf:type skos:Concept ;
  dcterms:dateAccepted "2007-09-01"^^xsd:date ;
  dcterms:dateAccepted "2009-12-29"^^xsd:date ;
  dcterms:provenance "KS X ISO 19136" ;
  dcterms:source "ISO 19136:2007" ;
  reg:status reg:statusValid ;
  rdfs:comment "Note 1 to entry: When used as a noun, measure is a synonym for physical quantity."@en ;
  rdfs:comment "비고: 명사로 사용할 경우, 측정은 물리량과 동일한 의미이다."@kr ;
  rdfs:label "measure <GML>"@en ;
  skos:changeNote "valid" ;
  skos:definition "축척에 의한 수치나 스칼라 참조 체계를 이용하여 표시한 값"@kr ;
  skos:editorialNote "preferred" ;
  skos:editorialNote "preferred"^^xsd:string ;
  skos:notation "286" ;
  skos:notation 286 ;
  skos:note "Note 1 to entry: When used as a noun, measure is a synonym for physical quantity."@en ;
  skos:note "비고: 명사로 사용할 경우, 측정은 물리량과 동일한 의미이다."@kr ;
  skos:prefLabel "measure <GML>"@en ;
  skos:prefLabel "측정 <GML>"@kr ;
.
<http://iso.org/tc211/term/287>
  rdf:type skos:Concept ;
  dcterms:dateAccepted "2005-07-15"^^xsd:date ;
  dcterms:dateAccepted "2008-12-30"^^xsd:date ;
  dcterms:provenance "ISO 19118:2005" ;
  dcterms:source "ISO 19118:2011, 4.26" ;
  reg:status reg:statusValid ;
  rdfs:label "medium"@en ;
  skos:changeNote "valid" ;
  skos:definition "데이터를 저장 또는 전달하기 위한 물질 또는 중개 수단"@kr ;
  skos:editorialNote "preferred" ;
  skos:editorialNote "preferred"^^xsd:string ;
  skos:notation "287" ;
  skos:notation 287 ;
  skos:prefLabel "medium"@en ;
  skos:prefLabel "매체"@kr ;
.
<http://iso.org/tc211/term/289>
  rdf:type skos:Concept ;
  dcterms:dateAccepted "2002-12-01" ;
  dcterms:dateAccepted "2002-12-01"^^xsd:date ;
  dcterms:dateAccepted "2008-12-30"^^xsd:date ;
  dcterms:provenance "ISO 19113" ;
  dcterms:source "ISO 19115:2003, 4.5" ;
  reg:status reg:statusSuperseded ;
  rdfs:comment "In de Richtlijn Metagegevens Overheidsinformatie wordt metadata omschreven als: \"Gegevens over informatieobjecten. Zij maken het mogelijk informatieobjecten te vinden, uit te wisselen en te beheren.\""@en ;
  rdfs:label "metadata"@en ;
  skos:changeNote "superseded" ;
  skos:definition "gegevens over gegevens"@nl ;
  skos:definition "데이터에 관한 데이터"@kr ;
  skos:notation "289" ;
  skos:notation 289 ;
  skos:note "In de Richtlijn Metagegevens Overheidsinformatie wordt metadata omschreven als: \"Gegevens over informatieobjecten. Zij maken het mogelijk informatieobjecten te vinden, uit te wisselen en te beheren.\""@en ;
  skos:prefLabel "metadata"@en ;
  skos:prefLabel "metadata"@nl ;
  skos:prefLabel "메타데이터"@kr ;
.
<http://iso.org/tc211/term/29>
  rdf:type skos:Concept ;
  dcterms:dateAccepted "2003-05-01"^^xsd:date ;
  dcterms:dateAccepted "2009-12-29"^^xsd:date ;
  dcterms:provenance "KS X ISO 19107" ;
  dcterms:source "ISO 19107:2003" ;
  reg:status reg:statusValid ;
  rdfs:comment "Note 1 to entry: Boundary is most commonly used in the context of geometry, where the set is a collection of points or a collection of objects that represent those points. In other arenas, the term is used metaphorically to describe the transition between an entity and the rest of its domain of discourse."@en ;
  rdfs:comment "비고: 경계는 기하 환경에서 가장 많이 사용된다. 기하는 점 집합체 또는 그 점들을 표현하는 객체 집합체로 구성된다. 다른 측면에서 경계는 어떤 개체와 그 개체를 제외한 논의의 영역 간의 전이역을 기술하기 위하여 은유적 용어로 사용된다."@kr ;
  rdfs:label "boundary"@en ;
  skos:changeNote "valid" ;
  skos:definition "개체의 한계를 표현하는 집합"@kr ;
  skos:editorialNote "preferred" ;
  skos:editorialNote "preferred"^^xsd:string ;
  skos:notation "29" ;
  skos:notation 29 ;
  skos:note "Note 1 to entry: Boundary is most commonly used in the context of geometry, where the set is a collection of points or a collection of objects that represent those points. In other arenas, the term is used metaphorically to describe the transition between an entity and the rest of its domain of discourse."@en ;
  skos:note "비고: 경계는 기하 환경에서 가장 많이 사용된다. 기하는 점 집합체 또는 그 점들을 표현하는 객체 집합체로 구성된다. 다른 측면에서 경계는 어떤 개체와 그 개체를 제외한 논의의 영역 간의 전이역을 기술하기 위하여 은유적 용어로 사용된다."@kr ;
  skos:prefLabel "boundary"@en ;
  skos:prefLabel "경계"@kr ;
.
<http://iso.org/tc211/term/290>
  rdf:type skos:Concept ;
  dcterms:dateAccepted "2003-05-01"^^xsd:date ;
  dcterms:dateAccepted "2008-12-30"^^xsd:date ;
  dcterms:provenance "ISO 19115:2003" ;
  dcterms:source "ISO 19115-1:2014, 4.11" ;
  reg:status reg:statusValid ;
  rdfs:comment "Note 1 to entry: Metadata elements are unique within a metadata entity."@en ;
  rdfs:comment "Note 2 to entry: Equivalent to an attribute in UML terminology." ;
  rdfs:comment "비고 1: 메타데이터 요소는 메타데이터 개체 내에서 유일하다"@kr ;
  rdfs:label "metadata element"@en ;
  skos:changeNote "valid" ;
  skos:definition "메타데이터를 구성하는 단위"@kr ;
  skos:editorialNote "preferred" ;
  skos:editorialNote "preferred"^^xsd:string ;
  skos:notation "290" ;
  skos:notation 290 ;
  skos:note "Note 1 to entry: Metadata elements are unique within a metadata entity."@en ;
  skos:note "Note 2 to entry: Equivalent to an attribute in UML terminology."^^<http://www.w3.org/2001/XMLSchema#@en> ;
  skos:note "비고 1: 메타데이터 요소는 메타데이터 개체 내에서 유일하다"@kr ;
  skos:note "비고 2: UML 용어에서 속성과 대응되는 용어이다."@kr ;
  skos:prefLabel "metadata element"@en ;
  skos:prefLabel "메타데이터 요소"@kr ;
.
<http://iso.org/tc211/term/291>
  rdf:type skos:Concept ;
  dcterms:dateAccepted "2003-05-01"^^xsd:date ;
  dcterms:dateAccepted "2008-12-30"^^xsd:date ;
  dcterms:provenance "ISO 19115:2003" ;
  dcterms:source "ISO 19115-1:2014, 4.12" ;
  reg:status reg:statusValid ;
  rdfs:comment "Note 1 to entry: May contain one or more metadata entities."@en ;
  rdfs:comment "Note 2 to entry: Equivalent to a class in UML terminology." ;
  rdfs:comment "비고 1: 하나 이상의 메타데이터 개체를 포함할 수 있다."@kr ;
  rdfs:label "metadata entity"@en ;
  skos:changeNote "valid" ;
  skos:definition "데이터의 동일한 측면을 기술하는 메타데이터 요소들의 집합"@kr ;
  skos:editorialNote "preferred" ;
  skos:editorialNote "preferred"^^xsd:string ;
  skos:notation "291" ;
  skos:notation 291 ;
  skos:note "Note 1 to entry: May contain one or more metadata entities."@en ;
  skos:note "Note 2 to entry: Equivalent to a class in UML terminology."^^<http://www.w3.org/2001/XMLSchema#@en> ;
  skos:note "비고 1: 하나 이상의 메타데이터 개체를 포함할 수 있다."@kr ;
  skos:note "비고 2: UML 용어로 클래스에 해당한다."@kr ;
  skos:prefLabel "metadata entity"@en ;
  skos:prefLabel "메타데이터 개체"@kr ;
.
<http://iso.org/tc211/term/292>
  rdf:type skos:Concept ;
  dcterms:dateAccepted "2002-07-01"^^xsd:date ;
  dcterms:dateAccepted "2008-12-30"^^xsd:date ;
  dcterms:source "ISO 19101:2002, 4.21" ;
  reg:status reg:statusRetired ;
  rdfs:comment "Note 1 to entry: ISO 19115 describes a standard for a metadata schema."@en ;
  rdfs:comment "비고: KS X ISO 19115는 메타데이터 스키마를 기술하는 표준이다."@kr ;
  rdfs:label "metadata schema"@en ;
  skos:changeNote "retired" ;
  skos:definition "메타데이터를 기술하는 개념적 스키마"@kr ;
  skos:notation "292" ;
  skos:notation 292 ;
  skos:note "Note 1 to entry: ISO 19115 describes a standard for a metadata schema."@en ;
  skos:note "비고: KS X ISO 19115는 메타데이터 스키마를 기술하는 표준이다."@kr ;
  skos:prefLabel "metadata schema"@en ;
  skos:prefLabel "메타데이터 스키마"@kr ;
.
<http://iso.org/tc211/term/293>
  rdf:type skos:Concept ;
  dcterms:dateAccepted "2003-05-01"^^xsd:date ;
  dcterms:dateAccepted "2008-12-30"^^xsd:date ;
  dcterms:provenance "ISO 19115:2003" ;
  dcterms:source "ISO 19115-1:2014, 4.13" ;
  reg:status reg:statusValid ;
  rdfs:comment "Note 1 to entry: Equivalent to a package in UML terminology"@en ;
  rdfs:comment "비고: UML 용어에서 패키지에 대응되는 용어이다."@kr ;
  rdfs:label "metadata section"@en ;
  skos:changeNote "valid" ;
  skos:definition "관련된 메터데이터 개체와 메타데이터 요소의 모음으로 구성된 메터데이터의 하위 집합"@kr ;
  skos:editorialNote "preferred" ;
  skos:editorialNote "preferred"^^xsd:string ;
  skos:notation "293" ;
  skos:notation 293 ;
  skos:note "Note 1 to entry: Equivalent to a package in UML terminology"@en ;
  skos:note "비고: UML 용어에서 패키지에 대응되는 용어이다."@kr ;
  skos:prefLabel "metadata section"@en ;
  skos:prefLabel "메타데이터 섹션"@kr ;
.
<http://iso.org/tc211/term/294>
  rdf:type skos:Concept ;
  dcterms:dateAccepted "2005-07-15"^^xsd:date ;
  dcterms:dateAccepted "2009-12-29"^^xsd:date ;
  dcterms:provenance "ISO/TS 19103:2005 ,4.2.17" ;
  dcterms:source "ISO/IEC 19501" ;
  reg:status reg:statusValid ;
  rdfs:label "metamodel <UML>"@en ;
  skos:changeNote "valid" ;
  skos:definition "모델을 표현하기 위한 언어를 정의하는 모델"@kr ;
  skos:editorialNote "preferred" ;
  skos:editorialNote "preferred"^^xsd:string ;
  skos:notation "294" ;
  skos:notation 294 ;
  skos:prefLabel "metamodel <UML>"@en ;
  skos:prefLabel "메타모델 <UML>"@kr ;
.
<http://iso.org/tc211/term/295>
  rdf:type skos:Concept ;
  dcterms:dateAccepted "2005-07-15"^^xsd:date ;
  dcterms:dateAccepted "2009-12-29"^^xsd:date ;
  dcterms:provenance "ISO/TS 19103:2005" ;
  dcterms:provenance "KS X ISO 19103" ;
  dcterms:source "ISO/IEC 19501:2005 (Adapted from)" ;
  reg:status reg:statusValid ;
  rdfs:comment "Note 1 to entry: It specifies the algorithm or procedure associated with an operation."@en ;
  rdfs:comment "비고: 방법은 연산과 관련된 알고리듬 또는 순서를 기술한다."@kr ;
  rdfs:label "method <UML>"@en ;
  skos:changeNote "valid" ;
  skos:definition "연산의 구현"@kr ;
  skos:editorialNote "preferred" ;
  skos:editorialNote "preferred"^^xsd:string ;
  skos:notation "295" ;
  skos:notation 295 ;
  skos:note "Note 1 to entry: It specifies the algorithm or procedure associated with an operation."@en ;
  skos:note "비고: 방법은 연산과 관련된 알고리듬 또는 순서를 기술한다."@kr ;
  skos:prefLabel "method <UML>"@en ;
  skos:prefLabel "방법 <UML>"@kr ;
.
<http://iso.org/tc211/term/299>
  rdf:type skos:Concept ;
  dcterms:dateAccepted "2005-06-15" ;
  dcterms:dateAccepted "2005-06-15"^^xsd:date ;
  dcterms:dateAccepted "2006-05-01"^^xsd:date ;
  dcterms:provenance "KS X ISO 19109" ;
  dcterms:provenance "NEN 3610" ;
  dcterms:source "ISO 19109:2005" ;
  reg:status reg:statusAccepted ;
  reg:status reg:statusValid ;
  rdfs:label "model"@en ;
  skos:changeNote "valid" ;
  skos:definition "abstractie van enige aspecten van de werkelijkheid"@nl ;
  skos:definition "현실의 한 부분을 추상화한 것"@kr ;
  skos:editorialNote "preferred" ;
  skos:editorialNote "preferred"^^xsd:string ;
  skos:notation "299" ;
  skos:notation 299 ;
  skos:prefLabel "model"@en ;
  skos:prefLabel "model"@nl ;
  skos:prefLabel "모델"@kr ;
.
<http://iso.org/tc211/term/3>
  rdf:type skos:Concept ;
  dcterms:dateAccepted "2000-12-15"^^xsd:date ;
  dcterms:dateAccepted "2007-06-29"^^xsd:date ;
  dcterms:provenance "KS X ISO 19105" ;
  dcterms:source "ISO 19105:2000" ;
  reg:status reg:statusValid ;
  rdfs:comment "Note 1 to entry: An abstract test case is a formal basis for deriving executable test cases One or more test purposes are encapsulated in the abstract test case. An abstract test case is independent of both the implementation and the values. It should be complete in the sense that it is sufficient to enable a test verdict to be assigned unambiguously to each potentially observable test outcome (i.e. sequence of test events)."@en ;
  rdfs:comment "비고: 추상 시험 케이스는 실행 가능 시험 케이스에 대한 형식적인 틀을 제공하며 하나 이상의 시험 목적을 갖는다. 추상 시험 케이스는 구현과 값의 양쪽에 모두 독립해 있다. 관측 가능한 모든 시험 결과는 시험 판정을 내릴 수 있도록 명확해야 한다(예: 시험 이벤트의 연속)"@kr ;
  rdfs:label "abstract test case"@en ;
  skos:changeNote "valid" ;
  skos:definition "특정한 요구 사항을 수행하기 위한 일반화된 시험"@kr ;
  skos:editorialNote "preferred" ;
  skos:editorialNote "preferred"^^xsd:string ;
  skos:notation "3" ;
  skos:notation 3 ;
  skos:note "Note 1 to entry: An abstract test case is a formal basis for deriving executable test cases One or more test purposes are encapsulated in the abstract test case. An abstract test case is independent of both the implementation and the values. It should be complete in the sense that it is sufficient to enable a test verdict to be assigned unambiguously to each potentially observable test outcome (i.e. sequence of test events)."@en ;
  skos:note "비고: 추상 시험 케이스는 실행 가능 시험 케이스에 대한 형식적인 틀을 제공하며 하나 이상의 시험 목적을 갖는다. 추상 시험 케이스는 구현과 값의 양쪽에 모두 독립해 있다. 관측 가능한 모든 시험 결과는 시험 판정을 내릴 수 있도록 명확해야 한다(예: 시험 이벤트의 연속)"@kr ;
  skos:prefLabel "abstract test case"@en ;
  skos:prefLabel "추상 시험 케이스"@kr ;
.
<http://iso.org/tc211/term/30>
  rdf:type skos:Concept ;
  dcterms:dateAccepted "2003-05-01"^^xsd:date ;
  dcterms:dateAccepted "2009-12-29"^^xsd:date ;
  dcterms:provenance "KS X ISO 19107" ;
  dcterms:source "ISO 19107:2003" ;
  reg:status reg:statusValid ;
  rdfs:label "buffer"@en ;
  skos:changeNote "valid" ;
  skos:definition "지정된 기하 객체로부터 주어진 거리 이내의 모든 직접 위치를 포함하는 기하 객체"@kr ;
  skos:editorialNote "preferred" ;
  skos:editorialNote "preferred"^^xsd:string ;
  skos:notation "30" ;
  skos:notation 30 ;
  skos:prefLabel "buffer"@en ;
  skos:prefLabel "영향 범위"@kr ;
.
<http://iso.org/tc211/term/300>
  rdf:type skos:Concept ;
  dcterms:dateAccepted "2002-09-01"^^xsd:date ;
  dcterms:dateAccepted "2007-11-01"^^xsd:date ;
  dcterms:provenance "KS X ISO 19108" ;
  dcterms:source "ISO 19108;2002" ;
  reg:status reg:statusValid ;
  rdfs:comment "Note 1 to entry: The duration of a month is an integer number of days.  The number of days in a month is determined by the rules of the particular calendar."@en ;
  rdfs:comment "비고: 한 달의 기간은 일로 표현되는 정수이다. 한 달에서 날짜 수는 특정 달력의 규칙에 의해 결정된다."@kr ;
  rdfs:label "month"@en ;
  skos:changeNote "valid" ;
  skos:definition "달의 순환주기와 명목상 같은 지속 기간을 갖는 기간"@kr ;
  skos:editorialNote "preferred" ;
  skos:editorialNote "preferred"^^xsd:string ;
  skos:notation "300" ;
  skos:notation 300 ;
  skos:note "Note 1 to entry: The duration of a month is an integer number of days.  The number of days in a month is determined by the rules of the particular calendar."@en ;
  skos:note "비고: 한 달의 기간은 일로 표현되는 정수이다. 한 달에서 날짜 수는 특정 달력의 규칙에 의해 결정된다."@kr ;
  skos:prefLabel "month"@en ;
  skos:prefLabel "달"@kr ;
.
<http://iso.org/tc211/term/301>
  rdf:type skos:Concept ;
  dcterms:dateAccepted "2004-07-01"^^xsd:date ;
  dcterms:dateAccepted "2004-11-05"^^xsd:date ;
  dcterms:provenance "KS X ISO 19116" ;
  dcterms:source "ISO 19116:2004" ;
  reg:status reg:statusValid ;
  rdfs:label "motion"@en ;
  skos:changeNote "valid" ;
  skos:definition "특정 기준계에서 좌표 값의 변화로 표현되는 시간에 따른 객체의 위치변화"@kr ;
  skos:editorialNote "preferred" ;
  skos:editorialNote "preferred"^^xsd:string ;
  skos:notation "301" ;
  skos:notation 301 ;
  skos:prefLabel "motion"@en ;
  skos:prefLabel "이동"@kr ;
.
<http://iso.org/tc211/term/304>
  rdf:type skos:Concept ;
  dcterms:dateAccepted "2005-07-15"^^xsd:date ;
  dcterms:dateAccepted "2009-12-29"^^xsd:date ;
  dcterms:provenance "ISO/TS 19103:2005" ;
  dcterms:provenance "KS X ISO 19103" ;
  dcterms:source "ISO/IEC 19501:2005 (Adapted from)" ;
  reg:status reg:statusValid ;
  rdfs:comment "Note 1 to entry: Multiplicity specifications may be given for roles within associations, parts within composites, repetitions and other purposes. Essentially a multiplicity is a (possibly infinite) subset of the non-negative integers. Contrast: cardinality."@en ;
  rdfs:comment "비고: 다중성 명세는 연관의 역할로, 합성 및 반복 또는 목적의 부분으로 주어질 수 있다. 필수적으로 다중성은 음이 아닌 정수의 부분 집합(무한대 가능)이다. 관계수와 비교"@kr ;
  rdfs:label "multiplicity <UML>"@en ;
  skos:changeNote "valid" ;
  skos:definition "집합에서 허용 가능한 관계수의 범위에 대한 사양"@kr ;
  skos:editorialNote "preferred" ;
  skos:editorialNote "preferred"^^xsd:string ;
  skos:notation "304" ;
  skos:notation 304 ;
  skos:note "Note 1 to entry: Multiplicity specifications may be given for roles within associations, parts within composites, repetitions and other purposes. Essentially a multiplicity is a (possibly infinite) subset of the non-negative integers. Contrast: cardinality."@en ;
  skos:note "비고: 다중성 명세는 연관의 역할로, 합성 및 반복 또는 목적의 부분으로 주어질 수 있다. 필수적으로 다중성은 음이 아닌 정수의 부분 집합(무한대 가능)이다. 관계수와 비교"@kr ;
  skos:prefLabel "multiplicity <UML>"@en ;
  skos:prefLabel "다중성 <UML>"@kr ;
.
<http://iso.org/tc211/term/306>
  rdf:type skos:Concept ;
  dcterms:dateAccepted "2005-10-15"^^xsd:date ;
  dcterms:dateAccepted "2006-12-01"^^xsd:date ;
  dcterms:provenance "KS X ISO 19133" ;
  dcterms:source "ISO 19133:2005" ;
  reg:status reg:statusValid ;
  rdfs:comment "Note 1 to entry: This is essentially the common term navigation, but the definition decomposes the process in terms used in the packages defined in this International Standard."@en ;
  rdfs:comment "비고: '내비게이션'은 일반적 용어로 사용되나, 본 표준의 용어 정의에서는 각 절차를 분할한다. "@kr ;
  rdfs:label "navigation"@en ;
  skos:changeNote "valid" ;
  skos:definition "라우팅, 경로 운행 및 추적의 조합 "@kr ;
  skos:editorialNote "preferred" ;
  skos:editorialNote "preferred"^^xsd:string ;
  skos:notation "306" ;
  skos:notation 306 ;
  skos:note "Note 1 to entry: This is essentially the common term navigation, but the definition decomposes the process in terms used in the packages defined in this International Standard."@en ;
  skos:note "비고: '내비게이션'은 일반적 용어로 사용되나, 본 표준의 용어 정의에서는 각 절차를 분할한다. "@kr ;
  skos:prefLabel "navigation"@en ;
  skos:prefLabel "내비게이션"@kr ;
.
<http://iso.org/tc211/term/307>
  rdf:type skos:Concept ;
  dcterms:dateAccepted "2003-05-01"^^xsd:date ;
  dcterms:dateAccepted "2009-12-29"^^xsd:date ;
  dcterms:provenance "KS X ISO 19107" ;
  dcterms:source "ISO 19107:2003" ;
  reg:status reg:statusValid ;
  rdfs:label "neighbourhood"@en ;
  skos:changeNote "valid" ;
  skos:definition "내부에 명시된 직접 위치를 포함하고, 정의된 직접 위치로부터의 지정된 거리내에 있는 모든 직접 위치를 포함하는 기하 집합"@kr ;
  skos:editorialNote "preferred" ;
  skos:editorialNote "preferred"^^xsd:string ;
  skos:notation "307" ;
  skos:notation 307 ;
  skos:prefLabel "neighbourhood"@en ;
  skos:prefLabel "인접군"@kr ;
.
<http://iso.org/tc211/term/308>
  rdf:type skos:Concept ;
  dcterms:dateAccepted "2005-10-15"^^xsd:date ;
  dcterms:dateAccepted "2006-12-01"^^xsd:date ;
  dcterms:provenance "KS X ISO 19133" ;
  dcterms:source "ISO 19133:2005" ;
  reg:status reg:statusValid ;
  rdfs:comment "Note 1 to entry: The network is essentially the universe of discourse for the navigation problem.  Networks are a variety of 1-dimensional topological complex. In this light, junction and topological node are synonyms, as are link and directed edge."@en ;
  rdfs:comment "비고: 네트워크는 기본적으로 내비게이션 문제의 논의의 영역이다. 네트워크는 하나의 1차원 위상 복합체이다. 이 점에서 링크와 방향성 변의 관계와 같이 교차점과 위상 절점은 동의어이다."@kr ;
  rdfs:label "network"@en ;
  skos:changeNote "valid" ;
  skos:definition "0차원 객체 집합(교차점)과 이를 연결하는 1차원 객체 집합(링크)으로 구성된 추상 구조. 여기서 링크는 하나의 시작(원점, 소스) 교차점과 종료(도착지, 싱크) 교차점에 각각 연관되어 있다. "@kr ;
  skos:editorialNote "preferred" ;
  skos:editorialNote "preferred"^^xsd:string ;
  skos:notation "308" ;
  skos:notation 308 ;
  skos:note "Note 1 to entry: The network is essentially the universe of discourse for the navigation problem.  Networks are a variety of 1-dimensional topological complex. In this light, junction and topological node are synonyms, as are link and directed edge."@en ;
  skos:note "비고: 네트워크는 기본적으로 내비게이션 문제의 논의의 영역이다. 네트워크는 하나의 1차원 위상 복합체이다. 이 점에서 링크와 방향성 변의 관계와 같이 교차점과 위상 절점은 동의어이다."@kr ;
  skos:prefLabel "network"@en ;
  skos:prefLabel "망"@kr ;
.
<http://iso.org/tc211/term/309>
  rdf:type skos:Concept ;
  dcterms:dateAccepted "2002-09-01"^^xsd:date ;
  dcterms:dateAccepted "2009-12-29"^^xsd:date ;
  dcterms:provenance "KS X ISO 19107" ;
  dcterms:source "ISO 19107:2003" ;
  reg:status reg:statusValid ;
  rdfs:comment "Note 1 to entry: The boundary of a node is the empty set."@en ;
  rdfs:comment "비고: 절점의 경계는 공집합이다."@kr ;
  rdfs:label "node"@en ;
  skos:changeNote "valid" ;
  skos:definition "0차원의 위상 원시 객체"@kr ;
  skos:editorialNote "preferred" ;
  skos:editorialNote "preferred"^^xsd:string ;
  skos:notation "309" ;
  skos:notation 309 ;
  skos:note "Note 1 to entry: The boundary of a node is the empty set."@en ;
  skos:note "비고: 절점의 경계는 공집합이다."@kr ;
  skos:prefLabel "node"@en ;
  skos:prefLabel "절점"@kr ;
.
<http://iso.org/tc211/term/31>
  rdf:type skos:Concept ;
  dcterms:dateAccepted "2002-09-01"^^xsd:date ;
  dcterms:dateAccepted "2007-11-01"^^xsd:date ;
  dcterms:provenance "KS X ISO 19108" ;
  dcterms:source "ISO 19108;2002" ;
  reg:status reg:statusValid ;
  rdfs:label "calendar"@en ;
  skos:changeNote "valid" ;
  skos:definition "일 단위 시간 위치의 정의 근거를 제시하는 불연속 시간 참조 체계"@kr ;
  skos:editorialNote "preferred" ;
  skos:editorialNote "preferred"^^xsd:string ;
  skos:notation "31" ;
  skos:notation 31 ;
  skos:prefLabel "calendar"@en ;
  skos:prefLabel "달력"@kr ;
.
<http://iso.org/tc211/term/310>
  rdf:type skos:Concept ;
  dcterms:dateAccepted "2000-12-15"^^xsd:date ;
  dcterms:dateAccepted "2007-06-29"^^xsd:date ;
  dcterms:provenance "KS X ISO 19105" ;
  dcterms:source "ISO 19105:2000" ;
  reg:status reg:statusValid ;
  rdfs:label "non-conformance"@en ;
  skos:changeNote "valid" ;
  skos:definition "시험 대상(IUT)이 규정된 한 개 이상의 요건을 만족시키지 못해 실패한 것"@kr ;
  skos:editorialNote "preferred" ;
  skos:editorialNote "preferred"^^xsd:string ;
  skos:notation "310" ;
  skos:notation 310 ;
  skos:prefLabel "non-conformance"@en ;
  skos:prefLabel "부적합"@kr ;
.
<http://iso.org/tc211/term/311>
  rdf:type skos:Concept ;
  dcterms:dateAccepted "2003-02-15" ;
  dcterms:dateAccepted "2003-02-15"^^xsd:date ;
  dcterms:dateAccepted "2007-11-01"^^xsd:date ;
  dcterms:provenance "ISO 19111:2003" ;
  dcterms:provenance "KS X ISO 19111" ;
  dcterms:source "ISO 19111:2007" ;
  reg:status reg:statusAccepted ;
  reg:status reg:statusValid ;
  rdfs:label "northing"@en ;
  rdfs:seeAlso "northing"@nl ;
  skos:altLabel "N"@kr ;
  skos:altLabel "N"@nl ;
  skos:altLabel "N"^^<http://www.w3.org/2001/XMLSchema#@en> ;
  skos:altLabel "northing"@nl ;
  skos:changeNote "valid" ;
  skos:definition "afstand in een coördinaatsysteem, noordwaarts (positief) of zuidwaarts (negatief) gerekend vanaf een oost-west georiënteerde referentielijn"@nl ;
  skos:definition "좌표 체계상에서 동서 기준선에서부터 북쪽(양수) 또는 남쪽(음수)으로 관측한 직선거리"@kr ;
  skos:editorialNote "preferred" ;
  skos:editorialNote "preferred"^^xsd:string ;
  skos:notation "311" ;
  skos:notation 311 ;
  skos:prefLabel "Noord"@nl ;
  skos:prefLabel "northing"@en ;
  skos:prefLabel "북향 거리"@kr ;
.
<http://iso.org/tc211/term/312>
  rdf:type skos:Concept ;
  dcterms:dateAccepted "2003-05-01"^^xsd:date ;
  dcterms:dateAccepted "2009-12-29"^^xsd:date ;
  dcterms:provenance "ISO 19107:2003" ;
  dcterms:provenance "KS X ISO 19107" ;
  dcterms:source "OMG/UML UML Semantics, version 1.3, 1997." ;
  reg:status reg:statusValid ;
  rdfs:comment "Note 1 to entry: This term was first used in this way in the general theory of object oriented programming, and later adopted for use in this same sense in UML. An object is an instance of a class. Attributes and relationships represent state. Operations, methods, and state machines represent behavior."@en ;
  rdfs:comment "비고: 상태는 속성과 관계에 의해 표현되고, 행태는 연산, 방법 그리고 상태 메커니즘을 통해 표현된다. 객체는 클래스의 인스턴스이다. 클래스, 인스턴스를 참조"@kr ;
  rdfs:label "object"@en ;
  skos:changeNote "valid" ;
  skos:definition "상태와 행태를 캡슐화한 잘 정의된 경계와 식별특성을 갖는 개체"@kr ;
  skos:editorialNote "preferred" ;
  skos:editorialNote "preferred"^^xsd:string ;
  skos:notation "312" ;
  skos:notation 312 ;
  skos:note "Note 1 to entry: This term was first used in this way in the general theory of object oriented programming, and later adopted for use in this same sense in UML. An object is an instance of a class. Attributes and relationships represent state. Operations, methods, and state machines represent behavior."@en ;
  skos:note "비고: 상태는 속성과 관계에 의해 표현되고, 행태는 연산, 방법 그리고 상태 메커니즘을 통해 표현된다. 객체는 클래스의 인스턴스이다. 클래스, 인스턴스를 참조"@kr ;
  skos:prefLabel "object"@en ;
  skos:prefLabel "객체"@kr ;
.
<http://iso.org/tc211/term/313>
  rdf:type skos:Concept ;
  dcterms:dateAccepted "2003-05-01"^^xsd:date ;
  dcterms:dateAccepted "2009-12-29"^^xsd:date ;
  dcterms:provenance "ISO/TS 19103:2005" ;
  dcterms:provenance "KS X ISO 19103" ;
  dcterms:source "ISO/IEC 19501:2005 (Adapted from)" ;
  reg:status reg:statusValid ;
  rdfs:comment "Note 1 to entry: State is represented by attributes and relationships, behaviour is represented by operations, methods, and state machines. An object is an instance of a class. See: class, instance."@en ;
  rdfs:comment "비고: 상태는 속성과 관계에 의해 표현되고, 행태는 연산, 방법 그리고 상태 메커니즘을 통해 표현된다. 객체는 클래스의 인스턴스이다. 클래스, 인스턴스를 참조"@kr ;
  rdfs:label "object <UML>"@en ;
  skos:changeNote "valid" ;
  skos:definition "상태와 행태를 캡슐화한 잘 정의된 경계와 식별특성을 갖는 개체"@kr ;
  skos:editorialNote "preferred" ;
  skos:editorialNote "preferred"^^xsd:string ;
  skos:notation "313" ;
  skos:notation 313 ;
  skos:note "Note 1 to entry: State is represented by attributes and relationships, behaviour is represented by operations, methods, and state machines. An object is an instance of a class. See: class, instance."@en ;
  skos:note "비고: 상태는 속성과 관계에 의해 표현되고, 행태는 연산, 방법 그리고 상태 메커니즘을 통해 표현된다. 객체는 클래스의 인스턴스이다. 클래스, 인스턴스를 참조"@kr ;
  skos:prefLabel "object <UML>"@en ;
  skos:prefLabel "객체 <UML>"@kr ;
.
<http://iso.org/tc211/term/315>
  rdf:type skos:Concept ;
  dcterms:dateAccepted "2008-11-15"^^xsd:date ;
  dcterms:provenance "ISO/TS 19104:2008" ;
  dcterms:source "ISO 1087-1:2000" ;
  reg:status reg:statusValid ;
  rdfs:label "obsolete term"@en ;
  skos:changeNote "valid" ;
  skos:editorialNote "preferred"^^xsd:string ;
  skos:notation 315 ;
  skos:prefLabel "obsolete term"@en ;
.
<http://iso.org/tc211/term/316>
  rdf:type skos:Concept ;
  dcterms:dateAccepted "2002-08-29"^^xsd:date ;
  dcterms:dateAccepted "2004-07-01"^^xsd:date ;
  dcterms:provenance "ISO 19106:2004" ;
  dcterms:provenance "KS  X ISO/IEC 10000-1" ;
  dcterms:source "ISO/IEC TR 10000-1:1998" ;
  reg:status reg:statusValid ;
  rdfs:label "open systems environment"@en ;
  skos:altLabel "OSE"^^<http://www.w3.org/2001/XMLSchema#@en> ;
  skos:changeNote "valid" ;
  skos:definition "사용자 관점에서 응용, 데이터, 또는 사람에 대한 이식성 및 상호 운용성을 위한 인터페이스, 서비스, 지원 포맷 및 이들의 프로파일로 구성된 포괄적 집합"@kr ;
  skos:editorialNote "preferred" ;
  skos:editorialNote "preferred"^^xsd:string ;
  skos:notation "316" ;
  skos:notation 316 ;
  skos:prefLabel "open systems environment"@en ;
  skos:prefLabel "개방형 시스템 환경"@kr ;
.
<http://iso.org/tc211/term/317>
  rdf:type skos:Concept ;
  dcterms:dateAccepted "2004-07-01"^^xsd:date ;
  dcterms:dateAccepted "2004-11-05"^^xsd:date ;
  dcterms:provenance "KS X ISO 19116" ;
  dcterms:source "ISO 19116:2004" ;
  reg:status reg:statusValid ;
  rdfs:comment "Note 1 to entry: Measurements acquired in the field are affected by many instrumental and environmental factors, including meteorological conditions, computational methods and constraints, imperfect instrument construction, incomplete instrument adjustment or calibration, and, in the case of optical measuring systems, the personal bias of the observer.  Solutions for positions may be affected by the geometric relationships of the observed data and/or mathematical model employed in the processing software."@en ;
  rdfs:comment "비고: 현장에서 요구되는 측량은 기상조건, 계산 방법과 제약 조건, 불완전한 기계의 구성, 미숙한 기계 조정 또는 계기 보정, 특히 광학 측량 시스템의 경우, 관찰자 개인의 편견 등 도구와 환경에 의해 많은 영향을 받는다. 측위 솔루션은 관측된 데이터의 기하학적 관계와 처리하는 소프트웨어에 사용된 수학 모델의 영향을 받을 수 있다."@kr ;
  rdfs:label "operating conditions"@en ;
  skos:changeNote "valid" ;
  skos:definition "측위 시스템에서 좌표 값의 결정에 영향을 주는 매개 변수"@kr ;
  skos:editorialNote "preferred" ;
  skos:editorialNote "preferred"^^xsd:string ;
  skos:notation "317" ;
  skos:notation 317 ;
  skos:note "Note 1 to entry: Measurements acquired in the field are affected by many instrumental and environmental factors, including meteorological conditions, computational methods and constraints, imperfect instrument construction, incomplete instrument adjustment or calibration, and, in the case of optical measuring systems, the personal bias of the observer.  Solutions for positions may be affected by the geometric relationships of the observed data and/or mathematical model employed in the processing software."@en ;
  skos:note "비고: 현장에서 요구되는 측량은 기상조건, 계산 방법과 제약 조건, 불완전한 기계의 구성, 미숙한 기계 조정 또는 계기 보정, 특히 광학 측량 시스템의 경우, 관찰자 개인의 편견 등 도구와 환경에 의해 많은 영향을 받는다. 측위 솔루션은 관측된 데이터의 기하학적 관계와 처리하는 소프트웨어에 사용된 수학 모델의 영향을 받을 수 있다."@kr ;
  skos:prefLabel "operating conditions"@en ;
  skos:prefLabel "연산 조건"@kr ;
.
<http://iso.org/tc211/term/318>
  rdf:type skos:Concept ;
  dcterms:dateAccepted "2005-02-15"^^xsd:date ;
  dcterms:dateAccepted "2009-12-29"^^xsd:date ;
  dcterms:provenance "KS X ISO 19119" ;
  dcterms:source "ISO 19119:2005" ;
  reg:status reg:statusValid ;
  rdfs:comment "Note 1 to entry: An operation has a name and a list of parameters."@en ;
  rdfs:comment "Note 2 to entry: See 7.2 [of ISO 19119] for a discussion of operation" ;
  rdfs:comment "비고 1: 연산은 이름과 매개 변수 목록을 갖는다."@kr ;
  rdfs:label "operation"@en ;
  skos:changeNote "valid" ;
  skos:definition "객체 실행을 호출할 수 있는 변환 및 질의에 대한 사양"@kr ;
  skos:editorialNote "preferred" ;
  skos:editorialNote "preferred"^^xsd:string ;
  skos:notation "318" ;
  skos:notation 318 ;
  skos:note "Note 1 to entry: An operation has a name and a list of parameters."@en ;
  skos:note "Note 2 to entry: See 7.2 [of ISO 19119] for a discussion of operation"^^<http://www.w3.org/2001/XMLSchema#@en> ;
  skos:note "비고 1: 연산은 이름과 매개 변수 목록을 갖는다."@kr ;
  skos:note "비고 2: 연산에 대한 논의는 KS X ISO 19119의 7.2절을 참조하라."@kr ;
  skos:prefLabel "operation"@en ;
  skos:prefLabel "연산"@kr ;
.
<http://iso.org/tc211/term/319>
  rdf:type skos:Concept ;
  dcterms:dateAccepted "2005-07-15"^^xsd:date ;
  dcterms:dateAccepted "2009-12-29"^^xsd:date ;
  dcterms:provenance "ISO/TS 19103:2005 ,4.2.21" ;
  dcterms:source "ISO/IEC 19501" ;
  reg:status reg:statusValid ;
  rdfs:comment "Note 1 to entry: An operation has a signature, which may restrict the actual parameters that are possible."@en ;
  rdfs:comment "Note 2 to entry: Definition from UML Reference Manual: A specification of a transformation or query that an object may be called to execute." ;
  rdfs:comment "Note 3 to entry: An operation has a name and a list of parameters. A method is a procedure that implements an operation. It has an algorithm or procedure description."@en ;
  rdfs:comment "비고 1: 연산은 가능한 실제 매개 변수를 제약할 수 있는 서명을 갖는다."@kr ;
  rdfs:comment "비고 3: 연산은 이름과 매개 변수의 목록을 갖는다. 방법은 연산을 구현하는 절차이며, 알고리듬 또는 절차 설명을 갖는다."@kr ;
  rdfs:label "operation <UML>"@en ;
  skos:changeNote "valid" ;
  skos:definition "행태에 영향을 주기 위하여 객체로 부터 요청될 수 있는 서비스"@kr ;
  skos:editorialNote "preferred" ;
  skos:editorialNote "preferred"^^xsd:string ;
  skos:notation "319" ;
  skos:notation 319 ;
  skos:note "Note 1 to entry: An operation has a signature, which may restrict the actual parameters that are possible."@en ;
  skos:note "Note 2 to entry: Definition from UML Reference Manual: A specification of a transformation or query that an object may be called to execute."^^<http://www.w3.org/2001/XMLSchema#@en> ;
  skos:note "Note 3 to entry: An operation has a name and a list of parameters. A method is a procedure that implements an operation. It has an algorithm or procedure description."^^<http://www.w3.org/2001/XMLSchema#@en> ;
  skos:note "비고 1: 연산은 가능한 실제 매개 변수를 제약할 수 있는 서명을 갖는다."@kr ;
  skos:note "비고 2: UML 참조 매뉴얼에서의 정의: 객체 실행을 호출할 수 있는 변환 및 질의 사양"@kr ;
  skos:note "비고 3: 연산은 이름과 매개 변수의 목록을 갖는다. 방법은 연산을 구현하는 절차이며, 알고리듬 또는 절차 설명을 갖는다."@kr ;
  skos:prefLabel "operation <UML>"@en ;
  skos:prefLabel "연산 <UML>"@kr ;
.
<http://iso.org/tc211/term/32>
  rdf:type skos:Concept ;
  dcterms:dateAccepted "2002-09-01"^^xsd:date ;
  dcterms:dateAccepted "2007-11-01"^^xsd:date ;
  dcterms:provenance "KS X ISO 19108" ;
  dcterms:source "ISO 19108;2002" ;
  reg:status reg:statusValid ;
  rdfs:label "calendar era"@en ;
  skos:changeNote "valid" ;
  skos:definition "기간의 연속을 표현하는 달력의 유형으로 특정 사건으로부터 계산된 기간 표시"@kr ;
  skos:editorialNote "preferred" ;
  skos:editorialNote "preferred"^^xsd:string ;
  skos:notation "32" ;
  skos:notation 32 ;
  skos:prefLabel "calendar era"@en ;
  skos:prefLabel "달력 연대"@kr ;
.
<http://iso.org/tc211/term/320>
  rdf:type skos:Concept ;
  dcterms:dateAccepted "2004-07-01"^^xsd:date ;
  dcterms:dateAccepted "2004-11-05"^^xsd:date ;
  dcterms:provenance "KS X ISO 19116" ;
  dcterms:source "ISO 19116:2004" ;
  reg:status reg:statusValid ;
  rdfs:label "optical positioning system"@en ;
  skos:changeNote "valid" ;
  skos:definition "빛의 특성에 의해 객체의 위치를 결정하는 측위 시스템"@kr ;
  skos:editorialNote "preferred" ;
  skos:editorialNote "preferred"^^xsd:string ;
  skos:notation "320" ;
  skos:notation 320 ;
  skos:prefLabel "optical positioning system"@en ;
  skos:prefLabel "광학 측위 시스템"@kr ;
.
<http://iso.org/tc211/term/321>
  rdf:type skos:Concept ;
  dcterms:dateAccepted "2002-09-01"^^xsd:date ;
  dcterms:dateAccepted "2007-11-01"^^xsd:date ;
  dcterms:provenance "KS X ISO 19108" ;
  dcterms:source "ISO 19108;2002" ;
  reg:status reg:statusValid ;
  rdfs:label "ordinal era"@en ;
  skos:changeNote "valid" ;
  skos:definition "시대순으로 명명된 기간들 중 하나"@kr ;
  skos:editorialNote "preferred" ;
  skos:editorialNote "preferred"^^xsd:string ;
  skos:notation "321" ;
  skos:notation 321 ;
  skos:prefLabel "ordinal era"@en ;
  skos:prefLabel "순서 연대"@kr ;
.
<http://iso.org/tc211/term/322>
  rdf:type skos:Concept ;
  dcterms:dateAccepted "2002-09-01"^^xsd:date ;
  dcterms:dateAccepted "2007-11-01"^^xsd:date ;
  dcterms:provenance "KS X ISO 19108" ;
  dcterms:source "ISO 19108;2002" ;
  reg:status reg:statusValid ;
  rdfs:label "ordinal scale"@en ;
  skos:changeNote "valid" ;
  skos:definition "객체의 상대 위치를 측정하기 위한 기초를 제공하는 척도"@kr ;
  skos:editorialNote "preferred" ;
  skos:editorialNote "preferred"^^xsd:string ;
  skos:notation "322" ;
  skos:notation 322 ;
  skos:prefLabel "ordinal scale"@en ;
  skos:prefLabel "서수 척도"@kr ;
.
<http://iso.org/tc211/term/323>
  rdf:type skos:Concept ;
  dcterms:dateAccepted "2002-09-01"^^xsd:date ;
  dcterms:dateAccepted "2007-11-01"^^xsd:date ;
  dcterms:provenance "KS X ISO 19108" ;
  dcterms:source "ISO 19108;2002" ;
  reg:status reg:statusValid ;
  rdfs:label "ordinal temporal reference system"@en ;
  skos:changeNote "valid" ;
  skos:definition "순서 연대의 계층 구조로 구성된 시간 참조 체계"@kr ;
  skos:editorialNote "preferred" ;
  skos:editorialNote "preferred"^^xsd:string ;
  skos:notation "323" ;
  skos:notation 323 ;
  skos:prefLabel "ordinal temporal reference system"@en ;
  skos:prefLabel "서수 시간 참조 체계"@kr ;
.
<http://iso.org/tc211/term/325>
  rdf:type skos:Concept ;
  dcterms:dateAccepted "2005-07-15"^^xsd:date ;
  dcterms:dateAccepted "2009-12-29"^^xsd:date ;
  dcterms:provenance "ISO/TS 19103:2005" ;
  dcterms:provenance "KS X ISO 19103" ;
  dcterms:source "ISO/IEC 19501:2005 (Adapted from)" ;
  reg:status reg:statusValid ;
  rdfs:comment "Note 1 to entry: Packages may be nested within other packages. Both model elements and diagrams may appear in a package."@en ;
  rdfs:comment "비고: 패키지는 다른 패키지에 속할 수 있다. 모델 요소와 다이어그램 둘 다 하나의 패키지로 나타날 수 있다."@kr ;
  rdfs:label "package <UML>"@en ;
  skos:changeNote "valid" ;
  skos:definition "요소를 그룹으로 조직화하기 위한 일반 목적의 메커니즘"@kr ;
  skos:editorialNote "preferred" ;
  skos:editorialNote "preferred"^^xsd:string ;
  skos:notation "325" ;
  skos:notation 325 ;
  skos:note "Note 1 to entry: Packages may be nested within other packages. Both model elements and diagrams may appear in a package."@en ;
  skos:note "비고: 패키지는 다른 패키지에 속할 수 있다. 모델 요소와 다이어그램 둘 다 하나의 패키지로 나타날 수 있다."@kr ;
  skos:prefLabel "package <UML>"@en ;
  skos:prefLabel "패키지 <UML>"@kr ;
.
<http://iso.org/tc211/term/326>
  rdf:type skos:Concept ;
  dcterms:dateAccepted "2000-12-15"^^xsd:date ;
  dcterms:dateAccepted "2007-06-29"^^xsd:date ;
  dcterms:provenance "KS X ISO 19105" ;
  dcterms:source "ISO 19105:2000" ;
  reg:status reg:statusValid ;
  rdfs:label "pass verdict"@en ;
  skos:changeNote "valid" ;
  skos:definition "시험 적합 판정"@kr ;
  skos:editorialNote "preferred" ;
  skos:editorialNote "preferred"^^xsd:string ;
  skos:notation "326" ;
  skos:notation 326 ;
  skos:prefLabel "pass verdict"@en ;
  skos:prefLabel "통과 판정"@kr ;
.
<http://iso.org/tc211/term/328>
  rdf:type skos:Concept ;
  dcterms:dateAccepted "2004-07-01"^^xsd:date ;
  dcterms:dateAccepted "2004-11-05"^^xsd:date ;
  dcterms:provenance "KS X ISO 19116" ;
  dcterms:source "ISO 19116:2004" ;
  reg:status reg:statusValid ;
  rdfs:comment "Note 1 to entry: Performance indicators can be used as quality-control evidence of the positioning system and/or positioning solution. Internal quality control may include such factors as signal strength of received radio signals [signal-to-noise ratio (SNR)], figures indicating the dilution of precision (DOP) due to geometric constraints in radiolocation systems, and system-specific figure of merit (FOM)."@en ;
  rdfs:comment "비고: 성능 표시는 측위 시스템과/또는 측위 솔루션의 품질관리의 증거로서 사용될 수 있다. 내부 품질 관리는 수신 전파 강도(신호대 잡음비(SNR)), 전파 측위 시스템에서의 기하학적 제약 조건에 의한 정밀도 저하율(DOP)을 나타내는 수치 및 시스템 고유의 성능 계수((FOM)과 같은 요소를 포함할 수 있다."@kr ;
  rdfs:label "performance indicator"@en ;
  skos:changeNote "valid" ;
  skos:definition "성능수준을 나타내는 측위 시스템의 내부 매개 변수"@kr ;
  skos:editorialNote "preferred" ;
  skos:editorialNote "preferred"^^xsd:string ;
  skos:notation "328" ;
  skos:notation 328 ;
  skos:note "Note 1 to entry: Performance indicators can be used as quality-control evidence of the positioning system and/or positioning solution. Internal quality control may include such factors as signal strength of received radio signals [signal-to-noise ratio (SNR)], figures indicating the dilution of precision (DOP) due to geometric constraints in radiolocation systems, and system-specific figure of merit (FOM)."@en ;
  skos:note "비고: 성능 표시는 측위 시스템과/또는 측위 솔루션의 품질관리의 증거로서 사용될 수 있다. 내부 품질 관리는 수신 전파 강도(신호대 잡음비(SNR)), 전파 측위 시스템에서의 기하학적 제약 조건에 의한 정밀도 저하율(DOP)을 나타내는 수치 및 시스템 고유의 성능 계수((FOM)과 같은 요소를 포함할 수 있다."@kr ;
  skos:prefLabel "performance indicator"@en ;
  skos:prefLabel "성능 표시"@kr ;
.
<http://iso.org/tc211/term/329>
  rdf:type skos:Concept ;
  dcterms:dateAccepted "2000-12-15"^^xsd:date ;
  dcterms:dateAccepted "2007-06-29"^^xsd:date ;
  dcterms:provenance "KS X ISO 19105" ;
  dcterms:source "ISO 19105:2000" ;
  reg:status reg:statusValid ;
  rdfs:comment "Note 1 to entry: This is not a part of conformance testing"@en ;
  rdfs:comment "비고: 성능 시험은 적합성 시험의 일부가 아니다."@kr ;
  rdfs:label "performance testing"@en ;
  skos:changeNote "valid" ;
  skos:definition "다양한 조건 하에서 처리량, 반응도 등 IUT의 성능에 대한 측정 "@kr ;
  skos:editorialNote "preferred" ;
  skos:editorialNote "preferred"^^xsd:string ;
  skos:notation "329" ;
  skos:notation 329 ;
  skos:note "Note 1 to entry: This is not a part of conformance testing"@en ;
  skos:note "비고: 성능 시험은 적합성 시험의 일부가 아니다."@kr ;
  skos:prefLabel "performance testing"@en ;
  skos:prefLabel "성능 시험"@kr ;
.
<http://iso.org/tc211/term/330>
  rdf:type skos:Concept ;
  dcterms:dateAccepted "2002-09-01"^^xsd:date ;
  dcterms:dateAccepted "2007-11-01"^^xsd:date ;
  dcterms:provenance "KS X ISO 19108" ;
  dcterms:source "ISO 19108;2002" ;
  reg:status reg:statusValid ;
  rdfs:comment "Note 1 to entry: A period is bounded by two different temporal positions."@en ;
  rdfs:comment "비고: 기간은 두 개의 서로 다른 시간 위치로 경계지워진다."@kr ;
  rdfs:label "period"@en ;
  skos:changeNote "valid" ;
  skos:definition "시간의 범위를 표현하는 1차원 기하 원시 객체"@kr ;
  skos:editorialNote "preferred" ;
  skos:editorialNote "preferred"^^xsd:string ;
  skos:notation "330" ;
  skos:notation 330 ;
  skos:note "Note 1 to entry: A period is bounded by two different temporal positions."@en ;
  skos:note "비고: 기간은 두 개의 서로 다른 시간 위치로 경계지워진다."@kr ;
  skos:prefLabel "period"@en ;
  skos:prefLabel "기간"@kr ;
.
<http://iso.org/tc211/term/331>
  rdf:type skos:Concept ;
  dcterms:dateAccepted "2002-09-01"^^xsd:date ;
  dcterms:dateAccepted "2007-11-01"^^xsd:date ;
  dcterms:provenance "ISO 19108;2002" ;
  dcterms:provenance "KS X ISO 19108" ;
  dcterms:source "ISO 31-2:1992 (Adapted from)" ;
  reg:status reg:statusValid ;
  rdfs:label "periodic time"@en ;
  skos:changeNote "valid" ;
  skos:definition "한 사이클의 기간"@kr ;
  skos:editorialNote "preferred" ;
  skos:editorialNote "preferred"^^xsd:string ;
  skos:notation "331" ;
  skos:notation 331 ;
  skos:prefLabel "periodic time"@en ;
  skos:prefLabel "주기"@kr ;
.
<http://iso.org/tc211/term/333>
  rdf:type skos:Concept ;
  dcterms:dateAccepted "2001-12-31"^^xsd:date ;
  dcterms:dateAccepted "2005-08-10"^^xsd:date ;
  dcterms:provenance "ISO 19136:2007" ;
  dcterms:provenance "KS A ISO 31-0" ;
  dcterms:source "ISO 31-0:1992" ;
  reg:status reg:statusValid ;
  rdfs:comment "Note 1 to entry: In GML a physical quantity is always a value described using a numeric amount with a scale or using a scalar reference system.  Physical quantity is a synonym for measure when the latter is used as a noun."@en ;
  rdfs:comment "비고: GML에서 물리량은 언제나 축척이나 스케일러 참조 체계를 이용하여 계산된 총수 값으로 기술된다. 명사로 사용할 경우, 물리량은 측정과 동일한 의미이다."@kr ;
  rdfs:label "physical quantity"@en ;
  skos:changeNote "valid" ;
  skos:definition "물리적 현상들의 양을 설명하는 데 사용되는 양"@kr ;
  skos:editorialNote "preferred" ;
  skos:editorialNote "preferred"^^xsd:string ;
  skos:notation "333" ;
  skos:notation 333 ;
  skos:note "Note 1 to entry: In GML a physical quantity is always a value described using a numeric amount with a scale or using a scalar reference system.  Physical quantity is a synonym for measure when the latter is used as a noun."@en ;
  skos:note "비고: GML에서 물리량은 언제나 축척이나 스케일러 참조 체계를 이용하여 계산된 총수 값으로 기술된다. 명사로 사용할 경우, 물리량은 측정과 동일한 의미이다."@kr ;
  skos:prefLabel "physical quantity"@en ;
  skos:prefLabel "물리량"@kr ;
.
<http://iso.org/tc211/term/335>
  rdf:type skos:Concept ;
  dcterms:dateAccepted "2003-05-01"^^xsd:date ;
  dcterms:dateAccepted "2009-12-29"^^xsd:date ;
  dcterms:provenance "KS X ISO 19107" ;
  dcterms:source "ISO 19107:2003" ;
  reg:status reg:statusValid ;
  rdfs:label "planar topological complex"@en ;
  skos:changeNote "valid" ;
  skos:definition "유클리드 기하학의 2공간에 내재될 수 있는 기하 실현을 갖는 위상 복합체"@kr ;
  skos:editorialNote "preferred" ;
  skos:editorialNote "preferred"^^xsd:string ;
  skos:notation "335" ;
  skos:notation 335 ;
  skos:prefLabel "planar topological complex"@en ;
  skos:prefLabel "평면 위상 복합체"@kr ;
.
<http://iso.org/tc211/term/336>
  rdf:type skos:Concept ;
  dcterms:dateAccepted "2002-09-01"^^xsd:date ;
  dcterms:dateAccepted "2009-12-29"^^xsd:date ;
  dcterms:provenance "ISO 19108;2002" ;
  dcterms:provenance "KS X ISO 19107" ;
  dcterms:source "ISO 19107:2003" ;
  reg:status reg:statusValid ;
  rdfs:comment "Note 1 to entry: The boundary of a point is the empty set."@en ;
  rdfs:comment "비고: 점의 경계는 공집합이다."@kr ;
  rdfs:label "point"@en ;
  skos:changeNote "valid" ;
  skos:definition "위치를 표현하는 0차원의 기하 원시 객체"@kr ;
  skos:editorialNote "preferred" ;
  skos:editorialNote "preferred"^^xsd:string ;
  skos:notation "336" ;
  skos:notation 336 ;
  skos:note "Note 1 to entry: The boundary of a point is the empty set."@en ;
  skos:note "비고: 점의 경계는 공집합이다."@kr ;
  skos:prefLabel "point"@en ;
  skos:prefLabel "점"@kr ;
.
<http://iso.org/tc211/term/337>
  rdf:type skos:Concept ;
  dcterms:dateAccepted "2005-08-15"^^xsd:date ;
  dcterms:dateAccepted "2007-11-01"^^xsd:date ;
  dcterms:provenance "KS X ISO 19123" ;
  dcterms:source "ISO 19123:2005" ;
  reg:status reg:statusValid ;
  rdfs:label "point coverage"@en ;
  skos:changeNote "valid" ;
  skos:definition "점으로 구성된 영역을 갖는 커버리지"@kr ;
  skos:editorialNote "preferred" ;
  skos:editorialNote "preferred"^^xsd:string ;
  skos:notation "337" ;
  skos:notation 337 ;
  skos:prefLabel "point coverage"@en ;
  skos:prefLabel "점 커버리지"@kr ;
.
<http://iso.org/tc211/term/34>
  rdf:type skos:Concept ;
  dcterms:dateAccepted "2005-10-15"^^xsd:date ;
  dcterms:dateAccepted "2006-12-01"^^xsd:date ;
  dcterms:provenance "KS X ISO 19133" ;
  dcterms:source "ISO 19133:2005" ;
  reg:status reg:statusValid ;
  rdfs:comment "Note 1 to entry: Navigation is the process of finding the candidate route that optimizes a chosen cost function."@en ;
  rdfs:comment "비고: 내비게이션은 선택된 비용 함수를 최적화하는 후보 경로를 찾는 과정이다."@kr ;
  rdfs:label "candidate route"@en ;
  skos:changeNote "valid" ;
  skos:definition "라우팅 요청의 제약 조건에 대하여 최적화된 비용 함수를 만족시키는 경로"@kr ;
  skos:editorialNote "preferred" ;
  skos:editorialNote "preferred"^^xsd:string ;
  skos:notation "34" ;
  skos:notation 34 ;
  skos:note "Note 1 to entry: Navigation is the process of finding the candidate route that optimizes a chosen cost function."@en ;
  skos:note "비고: 내비게이션은 선택된 비용 함수를 최적화하는 후보 경로를 찾는 과정이다."@kr ;
  skos:prefLabel "candidate route"@en ;
  skos:prefLabel "후보 경로"@kr ;
.
<http://iso.org/tc211/term/340>
  rdf:type skos:Concept ;
  dcterms:dateAccepted "2005-08-15"^^xsd:date ;
  dcterms:dateAccepted "2007-11-01"^^xsd:date ;
  dcterms:provenance "KS X ISO 19123" ;
  dcterms:source "ISO 19123:2005" ;
  reg:status reg:statusValid ;
  rdfs:label "polygon coverage"@en ;
  skos:changeNote "valid" ;
  skos:definition "다각형으로 구성된 영역을 갖는 커버리지"@kr ;
  skos:editorialNote "preferred" ;
  skos:editorialNote "preferred"^^xsd:string ;
  skos:notation "340" ;
  skos:notation 340 ;
  skos:prefLabel "polygon coverage"@en ;
  skos:prefLabel "다각형 커버리지"@kr ;
.
<http://iso.org/tc211/term/341>
  rdf:type skos:Concept ;
  dcterms:dateAccepted "2003-08-15"^^xsd:date ;
  dcterms:dateAccepted "2009-12-11"^^xsd:date ;
  dcterms:provenance "ISO 19114:2003 ,4.8" ;
  dcterms:source "ISO 3534-2" ;
  reg:status reg:statusRetired ;
  rdfs:label "population"@en ;
  skos:changeNote "retired" ;
  skos:definition "고려해야 할 모든 항목"@kr ;
  skos:notation "341" ;
  skos:notation 341 ;
  skos:prefLabel "population"@en ;
  skos:prefLabel "모집단"@kr ;
.
<http://iso.org/tc211/term/342>
  rdf:type skos:Concept ;
  dcterms:dateAccepted "2005-06-01" ;
  dcterms:dateAccepted "2005-06-01"^^xsd:date ;
  dcterms:dateAccepted "2006-05-01"^^xsd:date ;
  dcterms:provenance "ISO 19117:2005" ;
  dcterms:source "ISO 19117:2012, 4.20" ;
  reg:status reg:statusAccepted ;
  reg:status reg:statusValid ;
  rdfs:comment "Presentatie van informatie door visualisatie, hoorbaar maken, tastbaar maken (tactiel) of combinaties hiervan."@en ;
  rdfs:label "portrayal"@en ;
  skos:changeNote "valid" ;
  skos:definition "presentatie van informatie aan mensen"@nl ;
  skos:definition "정보를 인간에게 보여주는 것"@kr ;
  skos:editorialNote "preferred" ;
  skos:editorialNote "preferred"^^xsd:string ;
  skos:notation "342" ;
  skos:notation 342 ;
  skos:note "Presentatie van informatie door visualisatie, hoorbaar maken, tastbaar maken (tactiel) of combinaties hiervan."@en ;
  skos:prefLabel "portrayal"@en ;
  skos:prefLabel "presentatie"@nl ;
  skos:prefLabel "묘화"@kr ;
.
<http://iso.org/tc211/term/343>
  rdf:type skos:Concept ;
  dcterms:dateAccepted "2005-06-01"^^xsd:date ;
  dcterms:dateAccepted "2006-05-01"^^xsd:date ;
  dcterms:source "ISO 19117:2005, 4.15" ;
  reg:status reg:statusRetired ;
  rdfs:label "portrayal catalogue"@en ;
  skos:changeNote "retired" ;
  skos:definition "완전하게 정의된 묘화의 모음"@kr ;
  skos:notation "343" ;
  skos:notation 343 ;
  skos:prefLabel "portrayal catalogue"@en ;
  skos:prefLabel "묘화 목록"@kr ;
.
<http://iso.org/tc211/term/344>
  rdf:type skos:Concept ;
  dcterms:dateAccepted "2005-06-01"^^xsd:date ;
  dcterms:dateAccepted "2006-05-01"^^xsd:date ;
  dcterms:source "ISO 19117:2005, 4.16" ;
  reg:status reg:statusRetired ;
  rdfs:label "portrayal rule"@en ;
  skos:changeNote "retired" ;
  skos:definition "피처에 어떤 묘화 사양을 적용할지에 대한 규칙"@kr ;
  skos:notation "344" ;
  skos:notation 344 ;
  skos:prefLabel "portrayal rule"@en ;
  skos:prefLabel "묘화 규칙"@kr ;
.
<http://iso.org/tc211/term/345>
  rdf:type skos:Concept ;
  dcterms:dateAccepted "2005-06-01"^^xsd:date ;
  dcterms:dateAccepted "2006-05-01"^^xsd:date ;
  dcterms:provenance "ISO 19117:2005" ;
  dcterms:source "ISO 19117:2012, 4.26" ;
  reg:status reg:statusValid ;
  rdfs:label "portrayal service"@en ;
  skos:changeNote "valid" ;
  skos:definition "피처를 묘화하는데 사용되는 일반적인 인터페이스"@kr ;
  skos:editorialNote "preferred" ;
  skos:editorialNote "preferred"^^xsd:string ;
  skos:notation "345" ;
  skos:notation 345 ;
  skos:prefLabel "portrayal service"@en ;
  skos:prefLabel "묘화 서비스"@kr ;
.
<http://iso.org/tc211/term/346>
  rdf:type skos:Concept ;
  dcterms:dateAccepted "2005-06-01"^^xsd:date ;
  dcterms:dateAccepted "2006-05-01"^^xsd:date ;
  dcterms:source "ISO 19117:2005, 4.18" ;
  reg:status reg:statusRetired ;
  rdfs:label "portrayal specification"@en ;
  skos:changeNote "retired" ;
  skos:definition "피처 인스턴스의 묘화에 사용되는 연산의 모음"@kr ;
  skos:notation "346" ;
  skos:notation 346 ;
  skos:prefLabel "portrayal specification"@en ;
  skos:prefLabel "묘화 사양"@kr ;
.
<http://iso.org/tc211/term/347>
  rdf:type skos:Concept ;
  dcterms:dateAccepted "2005-10-15"^^xsd:date ;
  dcterms:dateAccepted "2006-12-01"^^xsd:date ;
  dcterms:provenance "KS X ISO 19133" ;
  dcterms:source "ISO 19133:2005" ;
  reg:status reg:statusValid ;
  rdfs:comment "Note 1 to entry: A direct position is a semantic subtype of position. Direct positions as described can only define a point and therefore not all positions can be represented by a direct position. That is consistent with the \"is type of\" relation.  An 19107 geometry is also a position, just not a direct position."@en ;
  rdfs:comment "비고: 직접 위치는 의미론적으로 위치의 하위 유형이다. 직접 위치는 단지 점으로만 기술되며, 모든 위치를 직접 위치로 표현할 수는 없다. 이는 관계의 \"유형(is type of)\"과 일관성을 갖는다. KS X ISO 19107의 기하 또한 위치이며, 반드시 직접 위치는 아니다."@kr ;
  rdfs:label "position"@en ;
  skos:changeNote "valid" ;
  skos:definition "객체 또는 사람이 잠정적으로 차지하는 하나의 점이나 기하를 기술하는 데이터 유형"@kr ;
  skos:editorialNote "preferred" ;
  skos:editorialNote "preferred"^^xsd:string ;
  skos:notation "347" ;
  skos:notation 347 ;
  skos:note "Note 1 to entry: A direct position is a semantic subtype of position. Direct positions as described can only define a point and therefore not all positions can be represented by a direct position. That is consistent with the \"is type of\" relation.  An 19107 geometry is also a position, just not a direct position."@en ;
  skos:note "비고: 직접 위치는 의미론적으로 위치의 하위 유형이다. 직접 위치는 단지 점으로만 기술되며, 모든 위치를 직접 위치로 표현할 수는 없다. 이는 관계의 \"유형(is type of)\"과 일관성을 갖는다. KS X ISO 19107의 기하 또한 위치이며, 반드시 직접 위치는 아니다."@kr ;
  skos:prefLabel "position"@en ;
  skos:prefLabel "위치"@kr ;
.
<http://iso.org/tc211/term/348>
  rdf:type skos:Concept ;
  dcterms:dateAccepted "2004-07-01"^^xsd:date ;
  dcterms:dateAccepted "2004-11-05"^^xsd:date ;
  dcterms:provenance "KS X ISO 19116" ;
  dcterms:source "ISO 19116:2004" ;
  reg:status reg:statusValid ;
  rdfs:comment "Note 1 to entry: The phrase \"absolute accuracy\" is sometimes used for this concept to distinguish it from relative positional accuracy.  Where the true coordinate value may not be perfectly known, accuracy is normally tested by comparison to available values that can best be accepted as true."@en ;
  rdfs:comment "비고: \"상대 위치 정확도\"와 개념 구별을 위해, 종종 위치 정확도에 \"절대 정확도\"라는 용어가 사용된다. 완벽하게 알려지지 않은 참 좌표 값의 정확도는 보통 참값으로 수용할 수 있는 가용한 최적의 값과 비교를 통해 결정된다.  "@kr ;
  rdfs:label "positional accuracy"@en ;
  skos:changeNote "valid" ;
  skos:definition "특정 참조 체계에서 관측에 의해 결정된 좌표 값이 참값 또는 허용 값에 근접하는 정도"@kr ;
  skos:editorialNote "preferred" ;
  skos:editorialNote "preferred"^^xsd:string ;
  skos:notation "348" ;
  skos:notation 348 ;
  skos:note "Note 1 to entry: The phrase \"absolute accuracy\" is sometimes used for this concept to distinguish it from relative positional accuracy.  Where the true coordinate value may not be perfectly known, accuracy is normally tested by comparison to available values that can best be accepted as true."@en ;
  skos:note "비고: \"상대 위치 정확도\"와 개념 구별을 위해, 종종 위치 정확도에 \"절대 정확도\"라는 용어가 사용된다. 완벽하게 알려지지 않은 참 좌표 값의 정확도는 보통 참값으로 수용할 수 있는 가용한 최적의 값과 비교를 통해 결정된다.  "@kr ;
  skos:prefLabel "positional accuracy"@en ;
  skos:prefLabel "위치 정확도"@kr ;
.
<http://iso.org/tc211/term/349>
  rdf:type skos:Concept ;
  dcterms:dateAccepted "2004-07-01"^^xsd:date ;
  dcterms:dateAccepted "2004-11-05"^^xsd:date ;
  dcterms:provenance "KS X ISO 19116" ;
  dcterms:source "ISO 19116:2004" ;
  reg:status reg:statusValid ;
  rdfs:comment "Note 1 to entry: Examples include inertial, integrated, linear, optical, and satellite positioning systems."@en ;
  rdfs:comment "비고: 관성, 통합, 선형, 광학, 및 위성 측위 시스템이 포함된다. "@kr ;
  rdfs:label "positioning system"@en ;
  skos:changeNote "valid" ;
  skos:definition "위치 측정을 위해 기구나 계산 컴포넌트를 갖는 시스템"@kr ;
  skos:editorialNote "preferred" ;
  skos:editorialNote "preferred"^^xsd:string ;
  skos:notation "349" ;
  skos:notation 349 ;
  skos:note "Note 1 to entry: Examples include inertial, integrated, linear, optical, and satellite positioning systems."@en ;
  skos:note "비고: 관성, 통합, 선형, 광학, 및 위성 측위 시스템이 포함된다. "@kr ;
  skos:prefLabel "positioning system"@en ;
  skos:prefLabel "측위 시스템"@kr ;
.
<http://iso.org/tc211/term/35>
  rdf:type skos:Concept ;
  dcterms:dateAccepted "2000-12-15"^^xsd:date ;
  dcterms:dateAccepted "2007-06-29"^^xsd:date ;
  dcterms:provenance "KS X ISO 19105" ;
  dcterms:source "ISO 19105:2000" ;
  reg:status reg:statusValid ;
  rdfs:label "capability test"@en ;
  skos:changeNote "valid" ;
  skos:definition "시험용 구현(IUT: Implementation under test)이 시험 목적에 기술된 바와 같이 표준 표준의 특정한 특성을 따르는지를 판단하기 위해 설계된 시험"@kr ;
  skos:editorialNote "preferred" ;
  skos:editorialNote "preferred"^^xsd:string ;
  skos:notation "35" ;
  skos:notation 35 ;
  skos:prefLabel "capability test"@en ;
  skos:prefLabel "기능 시험"@kr ;
.
<http://iso.org/tc211/term/350>
  rdf:type skos:Concept ;
  dcterms:dateAccepted "2004-07-01"^^xsd:date ;
  dcterms:dateAccepted "2004-11-05"^^xsd:date ;
  dcterms:source "ISO 19116:2004, 4.22" ;
  reg:status reg:statusValid ;
  rdfs:comment "Note 1 to entry: Precision is usually expressed as a statistical value based upon a set of repeated measurements such as the standard deviation from the sample mean."@en ;
  rdfs:comment "비고: 정밀도는 보통 표본 평균값으로부터의 표준 편차처럼 반복 측정에 기초한 통계 값으로 표현된다."@kr ;
  rdfs:label "precision"@en ;
  skos:changeNote "valid" ;
  skos:definition "측정치 집합의 재현성에 대한 척도"@kr ;
  skos:editorialNote "preferred" ;
  skos:editorialNote "preferred"^^xsd:string ;
  skos:notation "350" ;
  skos:notation 350 ;
  skos:note "Note 1 to entry: Precision is usually expressed as a statistical value based upon a set of repeated measurements such as the standard deviation from the sample mean."@en ;
  skos:note "비고: 정밀도는 보통 표본 평균값으로부터의 표준 편차처럼 반복 측정에 기초한 통계 값으로 표현된다."@kr ;
  skos:prefLabel "precision"@en ;
  skos:prefLabel "정밀도"@kr ;
.
<http://iso.org/tc211/term/351>
  rdf:type skos:Concept ;
  dcterms:dateAccepted "2008-11-15"^^xsd:date ;
  dcterms:provenance "ISO/TS 19104:2008" ;
  dcterms:source "ISO 1087-1" ;
  reg:status reg:statusValid ;
  rdfs:label "preferred term"@en ;
  skos:changeNote "valid" ;
  skos:editorialNote "preferred"^^xsd:string ;
  skos:notation 351 ;
  skos:prefLabel "preferred term"@en ;
.
<http://iso.org/tc211/term/352>
  rdf:type skos:Concept ;
  dcterms:dateAccepted "2003-02-15" ;
  dcterms:dateAccepted "2003-02-15"^^xsd:date ;
  dcterms:dateAccepted "2007-11-01"^^xsd:date ;
  dcterms:provenance "ISO 19111:2003" ;
  dcterms:provenance "KS X ISO 19111" ;
  dcterms:source "ISO 19111:2007" ;
  reg:status reg:statusAccepted ;
  reg:status reg:statusValid ;
  rdfs:label "prime meridian"@en ;
  rdfs:seeAlso "nul meridiaan"@nl ;
  rdfs:seeAlso "zero meridian" ;
  skos:altLabel "nul meridiaan"@nl ;
  skos:altLabel "zero meridian"@en ;
  skos:changeNote "valid" ;
  skos:definition "meridiaan waarvandaan de lengtegraden van de overige meridianen worden bepaald"@nl ;
  skos:definition "다른 자오선의 경도 측정에 기준으로 사용되는 0도"@kr ;
  skos:editorialNote "preferred" ;
  skos:editorialNote "preferred"^^xsd:string ;
  skos:notation "352" ;
  skos:notation 352 ;
  skos:prefLabel "nulmeridiaan"@nl ;
  skos:prefLabel "prime meridian"@en ;
  skos:prefLabel "본초 자오선"@kr ;
.
<http://iso.org/tc211/term/355>
  rdf:type skos:Concept ;
  dcterms:dateAccepted "2002-12-01"^^xsd:date ;
  dcterms:dateAccepted "2007-11-01"^^xsd:date ;
  dcterms:source "ISO 19113:2002, 4.20" ;
  reg:status reg:statusRetired ;
  rdfs:label "product specification"@en ;
  skos:changeNote "retired" ;
  skos:definition "논의의 영역과 이를 데이터셋에 매핑하기 위한 사양에 대한 기술"@kr ;
  skos:notation "355" ;
  skos:notation 355 ;
  skos:prefLabel "product specification"@en ;
  skos:prefLabel "제품 사양"@kr ;
.
<http://iso.org/tc211/term/356>
  rdf:type skos:Concept ;
  dcterms:dateAccepted "2004-07-01"^^xsd:date ;
  dcterms:provenance "ISO 19106:2004" ;
  dcterms:source "ISO/IEC TR 10000-1:1998" ;
  reg:status reg:statusValid ;
  rdfs:comment "Note 1 to entry: A profile is derived from base standards so that by definition, conformance to a profile is conformance to the base standards from which it is derived."@en ;
  rdfs:label "profile"@en ;
  skos:changeNote "valid" ;
  skos:editorialNote "preferred"^^xsd:string ;
  skos:notation 356 ;
  skos:note "Note 1 to entry: A profile is derived from base standards so that by definition, conformance to a profile is conformance to the base standards from which it is derived."@en ;
  skos:prefLabel "profile"@en ;
.
<http://iso.org/tc211/term/359>
  rdf:type skos:Concept ;
  dcterms:dateAccepted "2002-07-01"^^xsd:date ;
  dcterms:dateAccepted "2008-12-30"^^xsd:date ;
  dcterms:provenance "KS X ISO 19101" ;
  dcterms:source "ISO 19101:2002" ;
  reg:status reg:statusSuperseded ;
  rdfs:label "quality"@en ;
  skos:changeNote "superseded" ;
  skos:definition "요구 사항에 대한 만족도를 나타내는 제품의 종합적인 특징"@kr ;
  skos:notation "359" ;
  skos:notation 359 ;
  skos:prefLabel "quality"@en ;
  skos:prefLabel "품질"@kr ;
.
<http://iso.org/tc211/term/36>
  rdf:type skos:Concept ;
  dcterms:dateAccepted "2005-07-15"^^xsd:date ;
  dcterms:dateAccepted "2009-12-29"^^xsd:date ;
  dcterms:provenance "ISO/TS 19103:2005" ;
  dcterms:provenance "KS X ISO 19103" ;
  dcterms:source "ISO/IEC 19501:2005 (Adapted from)" ;
  reg:status reg:statusValid ;
  rdfs:comment "Note 1 to entry: Contrast: multiplicity."@en ;
  rdfs:comment "비고: 반대: 다중성"@kr ;
  rdfs:label "cardinality <UML>"@en ;
  skos:changeNote "valid" ;
  skos:definition "집합 내 요소의 수"@kr ;
  skos:editorialNote "preferred" ;
  skos:editorialNote "preferred"^^xsd:string ;
  skos:notation "36" ;
  skos:notation 36 ;
  skos:note "Note 1 to entry: Contrast: multiplicity."@en ;
  skos:note "비고: 반대: 다중성"@kr ;
  skos:prefLabel "cardinality <UML>"@en ;
  skos:prefLabel "관계 수 <UML>"@kr ;
.
<http://iso.org/tc211/term/360>
  rdf:type skos:Concept ;
  dcterms:dateAccepted "2002-07-01"^^xsd:date ;
  dcterms:dateAccepted "2008-12-30"^^xsd:date ;
  dcterms:provenance "ISO 19101:2002" ;
  dcterms:source "ISO 19101-1:2014, 4.1.29" ;
  reg:status reg:statusValid ;
  rdfs:label "quality schema"@en ;
  skos:changeNote "valid" ;
  skos:definition "지리 데이터의 품질 측면을 정의하는 개념적 스키마"@kr ;
  skos:editorialNote "preferred" ;
  skos:editorialNote "preferred"^^xsd:string ;
  skos:notation "360" ;
  skos:notation 360 ;
  skos:prefLabel "quality schema"@en ;
  skos:prefLabel "품질 스키마"@kr ;
.
<http://iso.org/tc211/term/363>
  rdf:type skos:Concept ;
  dcterms:dateAccepted "2005-08-15"^^xsd:date ;
  dcterms:dateAccepted "2007-11-01"^^xsd:date ;
  dcterms:provenance "KS X ISO 19123" ;
  dcterms:source "ISO 19123:2005" ;
  reg:status reg:statusValid ;
  rdfs:label "range <coverage>"@en ;
  skos:changeNote "valid" ;
  skos:definition "커버리지 영역 내의 함수와 함수 요소에 연관된 피처 속성 값의 집합"@kr ;
  skos:editorialNote "preferred" ;
  skos:editorialNote "preferred"^^xsd:string ;
  skos:notation "363" ;
  skos:notation 363 ;
  skos:prefLabel "range <coverage>"@en ;
  skos:prefLabel "범위 <커버리지>"@kr ;
.
<http://iso.org/tc211/term/364>
  rdf:type skos:Concept ;
  dcterms:dateAccepted "2005-08-15"^^xsd:date ;
  dcterms:dateAccepted "2007-11-01"^^xsd:date ;
  dcterms:provenance "KS X ISO 19123" ;
  dcterms:source "ISO 19123:2005" ;
  reg:status reg:statusValid ;
  rdfs:comment "Note 1 to entry: A raster is a type of grid."@en ;
  rdfs:comment "비고: 래스터는 격자의 유형이다."@kr ;
  rdfs:label "raster"@en ;
  skos:changeNote "valid" ;
  skos:definition "음극 선관에 표시를 형성하거나 또는 그에 대응하는 평행 스캐닝 선의 일반적 직사각형의 패턴"@kr ;
  skos:editorialNote "preferred" ;
  skos:editorialNote "preferred"^^xsd:string ;
  skos:notation "364" ;
  skos:notation 364 ;
  skos:note "Note 1 to entry: A raster is a type of grid."@en ;
  skos:note "비고: 래스터는 격자의 유형이다."@kr ;
  skos:prefLabel "raster"@en ;
  skos:prefLabel "래스터"@kr ;
.
<http://iso.org/tc211/term/366>
  rdf:type skos:Concept ;
  dcterms:dateAccepted "2003-05-01"^^xsd:date ;
  dcterms:dateAccepted "2009-12-29"^^xsd:date ;
  dcterms:provenance "KS X ISO 19107" ;
  dcterms:source "ISO 19107:2003" ;
  reg:status reg:statusValid ;
  rdfs:comment "Note 1 to entry: Logically, a record is a set of pairs <name, item >."@en ;
  rdfs:comment "비고: 논리적으로 레코드는 <이름, 항목> 쌍의 집합이다."@kr ;
  rdfs:label "record"@en ;
  skos:changeNote "valid" ;
  skos:definition "유한적인 관련 항목(객체 또는 값)의 명명된 모음"@kr ;
  skos:editorialNote "preferred" ;
  skos:editorialNote "preferred"^^xsd:string ;
  skos:notation "366" ;
  skos:notation 366 ;
  skos:note "Note 1 to entry: Logically, a record is a set of pairs <name, item >."@en ;
  skos:note "비고: 논리적으로 레코드는 <이름, 항목> 쌍의 집합이다."@kr ;
  skos:prefLabel "record"@en ;
  skos:prefLabel "레코드"@kr ;
.
<http://iso.org/tc211/term/367>
  rdf:type skos:Concept ;
  dcterms:dateAccepted "2005-08-15"^^xsd:date ;
  dcterms:dateAccepted "2007-11-01"^^xsd:date ;
  dcterms:provenance "KS X ISO 19123" ;
  dcterms:source "ISO 19123:2005" ;
  reg:status reg:statusValid ;
  rdfs:comment "Note 1 to entry: If the coordinate reference system is related to the earth by a datum, the grid is a georectified grid."@en ;
  rdfs:comment "비고: 좌표 참조 체계가 데이텀에 의해 지구와 관련된다면, 해당 격자는 지리 정사 격자이다."@kr ;
  rdfs:label "rectified grid"@en ;
  skos:changeNote "valid" ;
  skos:definition "격자 좌표와 외부 좌표 참조 체계의 좌표 간의 어파인 변환을 거친 격자"@kr ;
  skos:editorialNote "preferred" ;
  skos:editorialNote "preferred"^^xsd:string ;
  skos:notation "367" ;
  skos:notation 367 ;
  skos:note "Note 1 to entry: If the coordinate reference system is related to the earth by a datum, the grid is a georectified grid."@en ;
  skos:note "비고: 좌표 참조 체계가 데이텀에 의해 지구와 관련된다면, 해당 격자는 지리 정사 격자이다."@kr ;
  skos:prefLabel "rectified grid"@en ;
  skos:prefLabel "정사 격자"@kr ;
.
<http://iso.org/tc211/term/368>
  rdf:type skos:Concept ;
  dcterms:dateAccepted "2003-08-15"^^xsd:date ;
  dcterms:dateAccepted "2009-12-29"^^xsd:date ;
  dcterms:source "ISO 19114:2003, 4.9" ;
  reg:status reg:statusRetired ;
  rdfs:label "reference data"@en ;
  skos:changeNote "retired" ;
  skos:definition "직접적인 외부 품질 산출 방법에 참조로 활용되는 논의의 영역을 대표하는 것으로 인정된 데이터"@kr ;
  skos:notation "368" ;
  skos:notation 368 ;
  skos:prefLabel "reference data"@en ;
  skos:prefLabel "참조 데이터"@kr ;
.
<http://iso.org/tc211/term/369>
  rdf:type skos:Concept ;
  dcterms:dateAccepted "2005-08-15"^^xsd:date ;
  dcterms:dateAccepted "2007-11-01"^^xsd:date ;
  dcterms:provenance "KS X ISO 19123" ;
  dcterms:source "ISO 19123:2005" ;
  reg:status reg:statusValid ;
  rdfs:comment "Note 1 to entry: If the coordinate reference system is related to the earth by a datum, the grid is a georeferenceable grid."@en ;
  rdfs:comment "비고: 좌표 참조 체계가 데이텀에 의해 지구와 관련된다면, 해당 격자는 지리 참조 가능 격자이다."@kr ;
  rdfs:label "referenceable grid"@en ;
  skos:changeNote "valid" ;
  skos:definition "격자 좌표 값을 외부 좌표 참조 체계의 좌표값으로 변환시키는 데 사용될 수 있는 변환과 연관된 격자"@kr ;
  skos:editorialNote "preferred" ;
  skos:editorialNote "preferred"^^xsd:string ;
  skos:notation "369" ;
  skos:notation 369 ;
  skos:note "Note 1 to entry: If the coordinate reference system is related to the earth by a datum, the grid is a georeferenceable grid."@en ;
  skos:note "비고: 좌표 참조 체계가 데이텀에 의해 지구와 관련된다면, 해당 격자는 지리 참조 가능 격자이다."@kr ;
  skos:prefLabel "referenceable grid"@en ;
  skos:prefLabel "참조 가능 격자"@kr ;
.
<http://iso.org/tc211/term/37>
  rdf:type skos:Concept ;
  dcterms:dateAccepted "2003-02-15" ;
  dcterms:dateAccepted "2003-02-15"^^xsd:date ;
  dcterms:dateAccepted "2007-11-01"^^xsd:date ;
  dcterms:provenance "ISO 19111:2003" ;
  dcterms:source "ISO 19111:2007, 4.2" ;
  reg:status reg:statusAccepted ;
  reg:status reg:statusValid ;
  rdfs:comment "Note 1 to entry: n is 2 or 3 for the purposes of this International Standard."@en ;
  rdfs:comment "OPMERKING n is 2 of 3 voor zover het de toepassing binnen deze Internationale Norm betreft."@en ;
  rdfs:comment "비고: 본 표준에서 n은 1, 2, 3을 나타낸다."@kr ;
  rdfs:label "Cartesian coordinate system"@en ;
  skos:changeNote "valid" ;
  skos:definition "Coördinaat systeem wat de positie geeft van punten ten opzichte van loodrecht op elkaar staande assen."@nl ;
  skos:definition "상호 직교하는 n개의 축을 기준으로 점의 위치를 나타내는 좌표 체계"@kr ;
  skos:editorialNote "preferred" ;
  skos:editorialNote "preferred"^^xsd:string ;
  skos:notation "37" ;
  skos:notation 37 ;
  skos:note "Note 1 to entry: n is 2 or 3 for the purposes of this International Standard."@en ;
  skos:note "OPMERKING n is 2 of 3 voor zover het de toepassing binnen deze Internationale Norm betreft."@en ;
  skos:note "비고: 본 표준에서 n은 1, 2, 3을 나타낸다."@kr ;
  skos:prefLabel "Cartesiaans Coördinaat Systeem"@nl ;
  skos:prefLabel "Cartesian coordinate system"@en ;
  skos:prefLabel "직각 좌표계"@kr ;
.
<http://iso.org/tc211/term/370>
  rdf:type skos:Concept ;
  dcterms:dateAccepted "2005-07-15"^^xsd:date ;
  dcterms:dateAccepted "2009-12-29"^^xsd:date ;
  dcterms:provenance "ISO/TS 19103:2005" ;
  dcterms:provenance "KS X ISO 19103" ;
  dcterms:source "ISO/IEC 19501:2005 (Adapted from)" ;
  reg:status reg:statusValid ;
  rdfs:comment "Note 1 to entry: For example, a design class is a refinement of an analysis class"@en ;
  rdfs:comment "비고: 예를 들어, 설계 클래스는 분석 클래스의 정제이다."@kr ;
  rdfs:label "refinement <UML>"@en ;
  skos:changeNote "valid" ;
  skos:definition "이미 일정 상세 수준으로 명세된 것과 보다 완전한 사양 간의 관계"@kr ;
  skos:editorialNote "preferred" ;
  skos:editorialNote "preferred"^^xsd:string ;
  skos:notation "370" ;
  skos:notation 370 ;
  skos:note "Note 1 to entry: For example, a design class is a refinement of an analysis class"@en ;
  skos:note "비고: 예를 들어, 설계 클래스는 분석 클래스의 정제이다."@kr ;
  skos:prefLabel "refinement <UML>"@en ;
  skos:prefLabel "정제 <UML>"@kr ;
.
<http://iso.org/tc211/term/371>
  rdf:type skos:Concept ;
  dcterms:dateAccepted "2005-10-15" ;
  dcterms:dateAccepted "2005-10-15"^^xsd:date ;
  dcterms:dateAccepted "2009-12-29"^^xsd:date ;
  dcterms:provenance "ISO 19135:2005" ;
  dcterms:provenance "KS X ISO 19135" ;
  dcterms:source "Annex E, ISO/IEC JTC1 Procedures (Adapted from)" ;
  reg:status reg:statusAccepted ;
  reg:status reg:statusValid ;
  rdfs:label "register"@en ;
  skos:changeNote "valid" ;
  skos:definition "verzameling van bestanden van identificatiecodes gerelateerd aan items met de beschrijving van de gerelateerde items"@nl ;
  skos:definition "연관 항목의 설명과 함께 항목에 부여된 식별자를 포함하는 파일의 집합"@kr ;
  skos:editorialNote "preferred" ;
  skos:editorialNote "preferred"^^xsd:string ;
  skos:notation "371" ;
  skos:notation 371 ;
  skos:prefLabel "register"@en ;
  skos:prefLabel "register"@nl ;
  skos:prefLabel "등록물"@kr ;
.
<http://iso.org/tc211/term/372>
  rdf:type skos:Concept ;
  dcterms:dateAccepted "2005-10-15" ;
  dcterms:dateAccepted "2005-10-15"^^xsd:date ;
  dcterms:dateAccepted "2009-12-29"^^xsd:date ;
  dcterms:provenance "KS X ISO 19135" ;
  dcterms:source "ISO 19135:2005" ;
  reg:status reg:statusAccepted ;
  reg:status reg:statusValid ;
  rdfs:label "register owner"@en ;
  skos:changeNote "valid" ;
  skos:definition "organisatie die een register opzet"@nl ;
  skos:definition "등록물을 구축한 기구"@kr ;
  skos:editorialNote "preferred" ;
  skos:editorialNote "preferred"^^xsd:string ;
  skos:notation "372" ;
  skos:notation 372 ;
  skos:prefLabel "register owner"@en ;
  skos:prefLabel "registerhouder"@nl ;
  skos:prefLabel "등록물 소유자"@kr ;
.
<http://iso.org/tc211/term/373>
  rdf:type skos:Concept ;
  dcterms:dateAccepted "2005-10-15" ;
  dcterms:dateAccepted "2005-10-15"^^xsd:date ;
  dcterms:dateAccepted "2009-12-29"^^xsd:date ;
  dcterms:provenance "ISO 19135:2005" ;
  dcterms:provenance "KS X ISO 19135" ;
  dcterms:source "Annex E, ISO/IEC JTC1 Procedures (Adapted from)" ;
  reg:status reg:statusAccepted ;
  reg:status reg:statusValid ;
  rdfs:label "registration"@en ;
  skos:changeNote "valid" ;
  skos:definition "toewijzing van een permanent, uniek en eenduidige identificatie van een item"@nl ;
  skos:definition "항목에 대해 영구적이고 유일하며 명백한 식별자를 부여하는 것"@kr ;
  skos:editorialNote "preferred" ;
  skos:editorialNote "preferred"^^xsd:string ;
  skos:notation "373" ;
  skos:notation 373 ;
  skos:prefLabel "registration"@en ;
  skos:prefLabel "registreren"@nl ;
  skos:prefLabel "등록"@kr ;
.
<http://iso.org/tc211/term/375>
  rdf:type skos:Concept ;
  dcterms:dateAccepted "2005-10-15" ;
  dcterms:dateAccepted "2005-10-15"^^xsd:date ;
  dcterms:dateAccepted "2009-12-29"^^xsd:date ;
  dcterms:provenance "ISO 19135:2005" ;
  dcterms:provenance "KS X ISO 19135" ;
  dcterms:source "ISO/IEC 11179-3:2003 (Adapted from)" ;
  reg:status reg:statusAccepted ;
  reg:status reg:statusValid ;
  rdfs:label "registry"@en ;
  skos:changeNote "valid" ;
  skos:definition "information systeem waarin een een register wordt onderhouden"@nl ;
  skos:definition "등록물을 유지, 관리하는 정보 시스템 "@kr ;
  skos:editorialNote "preferred" ;
  skos:editorialNote "preferred"^^xsd:string ;
  skos:notation "375" ;
  skos:notation 375 ;
  skos:prefLabel "register"@nl ;
  skos:prefLabel "registry"@en ;
  skos:prefLabel "등록소"@kr ;
.
<http://iso.org/tc211/term/376>
  rdf:type skos:Concept ;
  dcterms:dateAccepted "2005-07-15"^^xsd:date ;
  dcterms:dateAccepted "2009-12-29"^^xsd:date ;
  dcterms:provenance "ISO/TS 19103:2005" ;
  dcterms:provenance "KS X ISO 19103" ;
  dcterms:source "ISO/IEC 19501:2005 (Adapted from)" ;
  reg:status reg:statusValid ;
  rdfs:comment "Note 1 to entry: Kinds of relationships include association, generalization, metarelationship, flow and several kinds grouped under dependency."@en ;
  rdfs:comment "비고: 관계에는 연관, 일반화, 메타 관계, 흐름 및 몇몇 의존 관계가 포함된다."@kr ;
  rdfs:label "relationship <UML>"@en ;
  skos:changeNote "valid" ;
  skos:definition "모델 요소들 사이의 의미론적 연결"@kr ;
  skos:editorialNote "preferred" ;
  skos:editorialNote "preferred"^^xsd:string ;
  skos:notation "376" ;
  skos:notation 376 ;
  skos:note "Note 1 to entry: Kinds of relationships include association, generalization, metarelationship, flow and several kinds grouped under dependency."@en ;
  skos:note "비고: 관계에는 연관, 일반화, 메타 관계, 흐름 및 몇몇 의존 관계가 포함된다."@kr ;
  skos:prefLabel "relationship <UML>"@en ;
  skos:prefLabel "관계 <UML>"@kr ;
.
<http://iso.org/tc211/term/377>
  rdf:type skos:Concept ;
  dcterms:dateAccepted "2004-07-01"^^xsd:date ;
  dcterms:dateAccepted "2004-11-05"^^xsd:date ;
  dcterms:provenance "KS X ISO 19116" ;
  dcterms:source "ISO 19116:2004" ;
  reg:status reg:statusValid ;
  rdfs:comment "Note 1 to entry: The spatial relationship of one point relative to another may be one-, two- or three-dimensional."@en ;
  rdfs:comment "비고: 다른 지점에 상대적인 한 지점의 공간 관계는 1, 2, 3차원일 수 있다. "@kr ;
  rdfs:label "relative position"@en ;
  skos:changeNote "valid" ;
  skos:definition "다른 점의 위치에 대한 관계로 정의되는 특정 점의 위치"@kr ;
  skos:editorialNote "preferred" ;
  skos:editorialNote "preferred"^^xsd:string ;
  skos:notation "377" ;
  skos:notation 377 ;
  skos:note "Note 1 to entry: The spatial relationship of one point relative to another may be one-, two- or three-dimensional."@en ;
  skos:note "비고: 다른 지점에 상대적인 한 지점의 공간 관계는 1, 2, 3차원일 수 있다. "@kr ;
  skos:prefLabel "relative position"@en ;
  skos:prefLabel "상대 위치"@kr ;
.
<http://iso.org/tc211/term/378>
  rdf:type skos:Concept ;
  dcterms:dateAccepted "2004-07-01"^^xsd:date ;
  dcterms:dateAccepted "2004-11-05"^^xsd:date ;
  dcterms:provenance "KS X ISO 19116" ;
  dcterms:source "ISO 19116:2004" ;
  reg:status reg:statusValid ;
  rdfs:comment "Note 1 to entry: Closely related terms such as local accuracy are employed in various countries, agencies and application groups.  Where such terms are utilized, it is necessary to provide a description of the term."@en ;
  rdfs:comment "비고: 지역 정확도와 같은 유사 의미의 관련 용어가 여러 나라, 기관 및 응용 그룹에서 사용된다. 이러한 용어를 사용하는 경우, 용어에 대한 설명을 제공해야 한다. "@kr ;
  rdfs:label "relative positional accuracy"@en ;
  skos:changeNote "valid" ;
  skos:definition "특정 참조 체계에서 좌표의 오차 값이 참값 또는 허용 값에 근접하는 정도"@kr ;
  skos:editorialNote "preferred" ;
  skos:editorialNote "preferred"^^xsd:string ;
  skos:notation "378" ;
  skos:notation 378 ;
  skos:note "Note 1 to entry: Closely related terms such as local accuracy are employed in various countries, agencies and application groups.  Where such terms are utilized, it is necessary to provide a description of the term."@en ;
  skos:note "비고: 지역 정확도와 같은 유사 의미의 관련 용어가 여러 나라, 기관 및 응용 그룹에서 사용된다. 이러한 용어를 사용하는 경우, 용어에 대한 설명을 제공해야 한다. "@kr ;
  skos:prefLabel "relative positional accuracy"@en ;
  skos:prefLabel "상대 위치 정확도"@kr ;
.
<http://iso.org/tc211/term/379>
  rdf:type skos:Concept ;
  dcterms:dateAccepted "2008-06-01"^^xsd:date ;
  dcterms:source "ISO/TS 19101-2:2008" ;
  reg:status reg:statusValid ;
  rdfs:label "remote sensing"@en ;
  skos:changeNote "valid" ;
  skos:editorialNote "preferred"^^xsd:string ;
  skos:notation 379 ;
  skos:prefLabel "remote sensing"@en ;
.
<http://iso.org/tc211/term/380>
  rdf:type skos:Concept ;
  dcterms:dateAccepted "2005-12-01"^^xsd:date ;
  dcterms:dateAccepted "2009-12-29"^^xsd:date ;
  dcterms:provenance "KS X ISO 19128" ;
  dcterms:source "ISO 19128:2005" ;
  reg:status reg:statusValid ;
  rdfs:label "request"@en ;
  skos:changeNote "valid" ;
  skos:definition "클라이언트로부터의 연산 호출"@kr ;
  skos:editorialNote "preferred" ;
  skos:editorialNote "preferred"^^xsd:string ;
  skos:notation "380" ;
  skos:notation 380 ;
  skos:prefLabel "request"@en ;
  skos:prefLabel "요청"@kr ;
.
<http://iso.org/tc211/term/383>
  rdf:type skos:Concept ;
  dcterms:dateAccepted "2003-05-01"^^xsd:date ;
  dcterms:dateAccepted "2008-12-30"^^xsd:date ;
  dcterms:source "ISO 19115:2003, 4.10" ;
  reg:status reg:statusSuperseded ;
  rdfs:label "resource"@en ;
  skos:changeNote "superseded" ;
  skos:definition "요구 사항을 수행하기 위한 자산이나 수단"@kr ;
  skos:notation "383" ;
  skos:notation 383 ;
  skos:prefLabel "resource"@en ;
  skos:prefLabel "자원"@kr ;
.
<http://iso.org/tc211/term/384>
  rdf:type skos:Concept ;
  dcterms:dateAccepted "2005-12-01"^^xsd:date ;
  dcterms:dateAccepted "2009-12-29"^^xsd:date ;
  dcterms:provenance "KS X ISO 19128" ;
  dcterms:source "ISO 19128:2005" ;
  reg:status reg:statusValid ;
  rdfs:label "response"@en ;
  skos:changeNote "valid" ;
  skos:definition "서버로부터 클라이언트로 반환되는 연산의 결과"@kr ;
  skos:editorialNote "preferred" ;
  skos:editorialNote "preferred"^^xsd:string ;
  skos:notation "384" ;
  skos:notation 384 ;
  skos:prefLabel "response"@en ;
  skos:prefLabel "응답"@kr ;
.
<http://iso.org/tc211/term/385>
  rdf:type skos:Concept ;
  dcterms:dateAccepted "2003-05-01"^^xsd:date ;
  dcterms:dateAccepted "2009-12-29"^^xsd:date ;
  dcterms:provenance "KS X ISO 19107" ;
  dcterms:source "ISO 19107:2003" ;
  reg:status reg:statusValid ;
  rdfs:comment "Note 1 to entry: Rings are used to describe boundary components of surfaces in 2D and 3D coordinate systems."@en ;
  rdfs:comment "비고: 링은 2차원 및 3차원 좌표 체계에서 표면의 경계 컴포넌트를 기술하는 데 사용된다."@kr ;
  rdfs:label "ring"@en ;
  skos:changeNote "valid" ;
  skos:definition "순환하는 단순 곡선"@kr ;
  skos:editorialNote "preferred" ;
  skos:editorialNote "preferred"^^xsd:string ;
  skos:notation "385" ;
  skos:notation 385 ;
  skos:note "Note 1 to entry: Rings are used to describe boundary components of surfaces in 2D and 3D coordinate systems."@en ;
  skos:note "비고: 링은 2차원 및 3차원 좌표 체계에서 표면의 경계 컴포넌트를 기술하는 데 사용된다."@kr ;
  skos:prefLabel "ring"@en ;
  skos:prefLabel "링"@kr ;
.
<http://iso.org/tc211/term/386>
  rdf:type skos:Concept ;
  dcterms:dateAccepted "2000-12-15"^^xsd:date ;
  dcterms:dateAccepted "2007-06-29"^^xsd:date ;
  dcterms:provenance "KS X ISO 19105" ;
  dcterms:source "ISO 19105:2000" ;
  reg:status reg:statusValid ;
  rdfs:comment "Note 1 to entry: This is not a part of conformance testing"@en ;
  rdfs:comment "비고: 강도 시험은 적합성 시험의 일부가 아니다."@kr ;
  rdfs:label "robustness testing"@en ;
  skos:changeNote "valid" ;
  skos:definition "IUT가 오류를 포함하고 있는 데이터를 얼마나 잘 처리하는지를 결정하는 과정"@kr ;
  skos:editorialNote "preferred" ;
  skos:editorialNote "preferred"^^xsd:string ;
  skos:notation "386" ;
  skos:notation 386 ;
  skos:note "Note 1 to entry: This is not a part of conformance testing"@en ;
  skos:note "비고: 강도 시험은 적합성 시험의 일부가 아니다."@kr ;
  skos:prefLabel "robustness testing"@en ;
  skos:prefLabel "강도 시험"@kr ;
.
<http://iso.org/tc211/term/387>
  rdf:type skos:Concept ;
  dcterms:dateAccepted "2005-10-15"^^xsd:date ;
  dcterms:dateAccepted "2006-12-01"^^xsd:date ;
  dcterms:provenance "KS X ISO 19133" ;
  dcterms:source "ISO 19133:2005" ;
  reg:status reg:statusValid ;
  rdfs:label "route"@en ;
  skos:changeNote "valid" ;
  skos:definition "네트워크 내 보통 두 위치 간의 경로를 기술하는 링크 및 부분적 링크의 연속"@kr ;
  skos:editorialNote "preferred" ;
  skos:editorialNote "preferred"^^xsd:string ;
  skos:notation "387" ;
  skos:notation 387 ;
  skos:prefLabel "route"@en ;
  skos:prefLabel "경로"@kr ;
.
<http://iso.org/tc211/term/389>
  rdf:type skos:Concept ;
  dcterms:dateAccepted "2005-10-15"^^xsd:date ;
  dcterms:dateAccepted "2006-12-01"^^xsd:date ;
  dcterms:provenance "KS X ISO 19133" ;
  dcterms:source "ISO 19133:2005" ;
  reg:status reg:statusValid ;
  rdfs:comment "Note 1 to entry: To minimize the number of instructions needed to complete a route traversal, a default instruction can be assumed at junctions without specifically associated instructions. This default is called the main-road rule."@en ;
  rdfs:comment "비고: 경로 운행에 필요한 지시를 최소화하기 위해 기본지시는 특별한 지시가 없는 교차점을 가질 수 있다. 이 기본 지시를 주요 도로 규칙이라 한다."@kr ;
  rdfs:label "route instruction"@en ;
  skos:changeNote "valid" ;
  skos:definition "운행 가능한 경로 네트워크 상의 점에 필요한 정보"@kr ;
  skos:editorialNote "preferred" ;
  skos:editorialNote "preferred"^^xsd:string ;
  skos:notation "389" ;
  skos:notation 389 ;
  skos:note "Note 1 to entry: To minimize the number of instructions needed to complete a route traversal, a default instruction can be assumed at junctions without specifically associated instructions. This default is called the main-road rule."@en ;
  skos:note "비고: 경로 운행에 필요한 지시를 최소화하기 위해 기본지시는 특별한 지시가 없는 교차점을 가질 수 있다. 이 기본 지시를 주요 도로 규칙이라 한다."@kr ;
  skos:prefLabel "route instruction"@en ;
  skos:prefLabel "경로 지시"@kr ;
.
<http://iso.org/tc211/term/39>
  rdf:type skos:Concept ;
  dcterms:dateAccepted "2002-08-16"^^xsd:date ;
  dcterms:dateAccepted "2008-12-19"^^xsd:date ;
  dcterms:provenance "ISO 19118:2011 ,4.2" ;
  dcterms:source "ISO/IEC 2382-1:1993" ;
  reg:status reg:statusValid ;
  rdfs:label "character"@en ;
  skos:changeNote "valid" ;
  skos:definition "데이터를 표현, 구성 또는 제어하기 위해 사용되는 요소 집합의 원소"@kr ;
  skos:editorialNote "preferred" ;
  skos:editorialNote "preferred"^^xsd:string ;
  skos:notation "39" ;
  skos:notation 39 ;
  skos:prefLabel "character"@en ;
  skos:prefLabel "문자"@kr ;
.
<http://iso.org/tc211/term/390>
  rdf:type skos:Concept ;
  dcterms:dateAccepted "2005-10-15"^^xsd:date ;
  dcterms:dateAccepted "2006-12-01"^^xsd:date ;
  dcterms:provenance "KS X ISO 19133" ;
  dcterms:source "ISO 19133:2005" ;
  reg:status reg:statusValid ;
  rdfs:label "route traversal"@en ;
  skos:changeNote "valid" ;
  skos:definition "경로를 따라가는 과정"@kr ;
  skos:editorialNote "preferred" ;
  skos:editorialNote "preferred"^^xsd:string ;
  skos:notation "390" ;
  skos:notation 390 ;
  skos:prefLabel "route traversal"@en ;
  skos:prefLabel "경로 운행"@kr ;
.
<http://iso.org/tc211/term/391>
  rdf:type skos:Concept ;
  dcterms:dateAccepted "2005-10-15"^^xsd:date ;
  dcterms:dateAccepted "2006-12-01"^^xsd:date ;
  dcterms:provenance "KS X ISO 19133" ;
  dcterms:source "ISO 19133:2005" ;
  reg:status reg:statusValid ;
  rdfs:label "routing"@en ;
  skos:changeNote "valid" ;
  skos:definition "네트워크 상의 위치들 사이에 최적(최소 비용 함수) 경로 탐색"@kr ;
  skos:editorialNote "preferred" ;
  skos:editorialNote "preferred"^^xsd:string ;
  skos:notation "391" ;
  skos:notation 391 ;
  skos:prefLabel "routing"@en ;
  skos:prefLabel "라우팅"@kr ;
.
<http://iso.org/tc211/term/392>
  rdf:type skos:Concept ;
  dcterms:dateAccepted "2004-07-01"^^xsd:date ;
  dcterms:dateAccepted "2004-11-05"^^xsd:date ;
  dcterms:provenance "KS X ISO 19116" ;
  dcterms:source "ISO 19116:2004" ;
  reg:status reg:statusValid ;
  rdfs:comment "Note 1 to entry: In this context, satellite positioning implies the use of radio signals transmitted from \"active\" artificial objects orbiting the Earth and received by \"passive\" instruments on or near the Earth's surface to determine position, velocity, and/or attitude of an object.  Examples are GPS and GLONASS."@en ;
  rdfs:comment "비고: 위성 측위는 객체의 위치, 속도, 자세의 계산을 위해, 지구 궤도상의 '능동적'인 인공물에서 송신되어 지상 또는  지구 표면 근처의 '수동적'인 수신기에 의해 수신된 전파를 이용하는 것을 의미한다. (예: GPS, GLONASS)"@kr ;
  rdfs:label "satellite positioning system"@en ;
  skos:changeNote "valid" ;
  skos:definition "위성으로부터 수신된 신호를 바탕으로한 측위 시스템"@kr ;
  skos:editorialNote "preferred" ;
  skos:editorialNote "preferred"^^xsd:string ;
  skos:notation "392" ;
  skos:notation 392 ;
  skos:note "Note 1 to entry: In this context, satellite positioning implies the use of radio signals transmitted from \"active\" artificial objects orbiting the Earth and received by \"passive\" instruments on or near the Earth's surface to determine position, velocity, and/or attitude of an object.  Examples are GPS and GLONASS."@en ;
  skos:note "비고: 위성 측위는 객체의 위치, 속도, 자세의 계산을 위해, 지구 궤도상의 '능동적'인 인공물에서 송신되어 지상 또는  지구 표면 근처의 '수동적'인 수신기에 의해 수신된 전파를 이용하는 것을 의미한다. (예: GPS, GLONASS)"@kr ;
  skos:prefLabel "satellite positioning system"@en ;
  skos:prefLabel "위성 측위 시스템"@kr ;
.
<http://iso.org/tc211/term/395>
  rdf:type skos:Concept ;
  dcterms:dateAccepted "2002-07-01"^^xsd:date ;
  dcterms:dateAccepted "2008-12-30"^^xsd:date ;
  dcterms:provenance "ISO 19101:2002" ;
  dcterms:source "ISO 19101-1:2014, 4.1.34" ;
  reg:status reg:statusValid ;
  rdfs:label "schema"@en ;
  skos:changeNote "valid" ;
  skos:definition "모델의 형식적 기술"@kr ;
  skos:editorialNote "preferred" ;
  skos:editorialNote "preferred"^^xsd:string ;
  skos:notation "395" ;
  skos:notation 395 ;
  skos:prefLabel "schema"@en ;
  skos:prefLabel "스키마"@kr ;
.
<http://iso.org/tc211/term/396>
  rdf:type skos:Concept ;
  dcterms:dateAccepted "2005-07-15"^^xsd:date ;
  dcterms:dateAccepted "2008-12-30"^^xsd:date ;
  dcterms:provenance "ISO 19118:2005" ;
  dcterms:source "ISO 19118:2011, 4.29" ;
  reg:status reg:statusValid ;
  rdfs:label "schema model"@en ;
  skos:changeNote "valid" ;
  skos:definition "스키마를 저장하기 위한 표현 모델"@kr ;
  skos:editorialNote "preferred" ;
  skos:editorialNote "preferred"^^xsd:string ;
  skos:notation "396" ;
  skos:notation 396 ;
  skos:prefLabel "schema model"@en ;
  skos:prefLabel "스키마 모델"@kr ;
.
<http://iso.org/tc211/term/397>
  rdf:type skos:Concept ;
  dcterms:dateAccepted "2007-10-15"^^xsd:date ;
  dcterms:dateAccepted "2009-12-29"^^xsd:date ;
  dcterms:provenance "KS X ISO 19132" ;
  dcterms:source "ISO 19132:2007" ;
  reg:status reg:statusValid ;
  rdfs:label "segment"@en ;
  skos:changeNote "valid" ;
  skos:definition "집합의 부분인 점 또는 다각형"@kr ;
  skos:editorialNote "preferred" ;
  skos:editorialNote "preferred"^^xsd:string ;
  skos:notation "397" ;
  skos:notation 397 ;
  skos:prefLabel "segment"@en ;
  skos:prefLabel "조각"@kr ;
.
<http://iso.org/tc211/term/398>
  rdf:type skos:Concept ;
  dcterms:dateAccepted "2007-09-01"^^xsd:date ;
  dcterms:dateAccepted "2009-12-29"^^xsd:date ;
  dcterms:provenance "KS X ISO 19136" ;
  dcterms:source "ISO 19136:2007" ;
  reg:status reg:statusValid ;
  rdfs:label "semantic type"@en ;
  skos:changeNote "valid" ;
  skos:definition "어떠한 공통적인 특징을 공유하여 특정 영역에서 고유한 유형의 이름을 부여 받은 객체의 카테고리"@kr ;
  skos:editorialNote "preferred" ;
  skos:editorialNote "preferred"^^xsd:string ;
  skos:notation "398" ;
  skos:notation 398 ;
  skos:prefLabel "semantic type"@en ;
  skos:prefLabel "의미론적 유형"@kr ;
.
<http://iso.org/tc211/term/4>
  rdf:type skos:Concept ;
  dcterms:dateAccepted "2000-12-15"^^xsd:date ;
  dcterms:dateAccepted "2007-06-29"^^xsd:date ;
  dcterms:provenance "KS X ISO 19105" ;
  dcterms:source "ISO 19105:2000" ;
  reg:status reg:statusValid ;
  rdfs:label "abstract test method"@en ;
  skos:changeNote "valid" ;
  skos:definition "특정 시험 절차와 상관 없이 독립적인 시험 구현을 위한 방법"@kr ;
  skos:editorialNote "preferred" ;
  skos:editorialNote "preferred"^^xsd:string ;
  skos:notation "4" ;
  skos:notation 4 ;
  skos:prefLabel "abstract test method"@en ;
  skos:prefLabel "추상 시험 방법"@kr ;
.
<http://iso.org/tc211/term/403>
  rdf:type skos:Concept ;
  dcterms:dateAccepted "2003-05-01"^^xsd:date ;
  dcterms:dateAccepted "2009-12-29"^^xsd:date ;
  dcterms:provenance "KS X ISO 19107" ;
  dcterms:source "ISO 19107:2003" ;
  reg:status reg:statusValid ;
  rdfs:comment "Note 1 to entry: Logically, a sequence is a set of pairs <item, offset>. LISP syntax, which delimits sequences with parentheses and separates elements in the sequence with commas, is used in this International Standard."@en ;
  rdfs:comment "비고: 논리적으로 연속은 <항목, 오프셋>쌍의 집합이다. 본 표준에서는 괄호로 연속을 구분하고, 연속 내 요소는 콤마로 분리하는 LISP의 문법이 사용된다."@kr ;
  rdfs:label "sequence"@en ;
  skos:changeNote "valid" ;
  skos:definition "유한하며 순서를 갖는, 서로 관련성이 있는 반복될 수 있는 항목(객체 또는 값)의 모음 "@kr ;
  skos:editorialNote "preferred" ;
  skos:editorialNote "preferred"^^xsd:string ;
  skos:notation "403" ;
  skos:notation 403 ;
  skos:note "Note 1 to entry: Logically, a sequence is a set of pairs <item, offset>. LISP syntax, which delimits sequences with parentheses and separates elements in the sequence with commas, is used in this International Standard."@en ;
  skos:note "비고: 논리적으로 연속은 <항목, 오프셋>쌍의 집합이다. 본 표준에서는 괄호로 연속을 구분하고, 연속 내 요소는 콤마로 분리하는 LISP의 문법이 사용된다."@kr ;
  skos:prefLabel "sequence"@en ;
  skos:prefLabel "연속"@kr ;
.
<http://iso.org/tc211/term/404>
  rdf:type skos:Concept ;
  dcterms:dateAccepted "2005-12-01"^^xsd:date ;
  dcterms:dateAccepted "2009-12-29"^^xsd:date ;
  dcterms:provenance "KS X ISO 19128" ;
  dcterms:source "ISO 19128:2005" ;
  reg:status reg:statusValid ;
  rdfs:label "server"@en ;
  skos:changeNote "valid" ;
  skos:definition "서비스의 특정 인스턴스"@kr ;
  skos:editorialNote "preferred" ;
  skos:editorialNote "preferred"^^xsd:string ;
  skos:notation "404" ;
  skos:notation 404 ;
  skos:prefLabel "server"@en ;
  skos:prefLabel "서버"@kr ;
.
<http://iso.org/tc211/term/405>
  rdf:type skos:Concept ;
  dcterms:dateAccepted "2005-02-15"^^xsd:date ;
  dcterms:dateAccepted "2009-12-29"^^xsd:date ;
  dcterms:provenance "ISO 19119:2005" ;
  dcterms:provenance "KS X ISO 19119" ;
  dcterms:source "ISO/IEC TR 14252 (Adapted from)" ;
  reg:status reg:statusValid ;
  rdfs:comment "Note 1 to entry: See 7.2 [of ISO 19119] for a discussion of service"@en ;
  rdfs:comment "비고: 서비스에 관한 논의는 KS X ISO 19110의 7.2절을 참조하라."@kr ;
  rdfs:label "service"@en ;
  skos:changeNote "valid" ;
  skos:definition "개체의 인터페이스를 통해 제공되는 기능성의 개별 부분"@kr ;
  skos:editorialNote "preferred" ;
  skos:editorialNote "preferred"^^xsd:string ;
  skos:notation "405" ;
  skos:notation 405 ;
  skos:note "Note 1 to entry: See 7.2 [of ISO 19119] for a discussion of service"@en ;
  skos:note "비고: 서비스에 관한 논의는 KS X ISO 19110의 7.2절을 참조하라."@kr ;
  skos:prefLabel "service"@en ;
  skos:prefLabel "서비스"@kr ;
.
<http://iso.org/tc211/term/406>
  rdf:type skos:Concept ;
  dcterms:dateAccepted "2005-02-15"^^xsd:date ;
  dcterms:dateAccepted "2009-12-29"^^xsd:date ;
  dcterms:provenance "KS X ISO 19119" ;
  dcterms:source "ISO 19119:2005" ;
  reg:status reg:statusValid ;
  rdfs:label "service chain"@en ;
  skos:changeNote "valid" ;
  skos:definition "인접된 서비스 쌍에 대하여, 첫 번째 활동이 연속된 다음 활동의 발생을 위해 반드시 필요한 서비스의 연속"@kr ;
  skos:editorialNote "preferred" ;
  skos:editorialNote "preferred"^^xsd:string ;
  skos:notation "406" ;
  skos:notation 406 ;
  skos:prefLabel "service chain"@en ;
  skos:prefLabel "서비스 연결"@kr ;
.
<http://iso.org/tc211/term/407>
  rdf:type skos:Concept ;
  dcterms:dateAccepted "2002-07-01"^^xsd:date ;
  dcterms:dateAccepted "2008-12-30"^^xsd:date ;
  dcterms:source "ISO 19101:2002, 4.27" ;
  reg:status reg:statusRetired ;
  rdfs:comment "0"@en ;
  rdfs:label "service interface"@en ;
  skos:changeNote "retired" ;
  skos:definition "인간이나 자동화된 시스템 간의 공유 경계"@kr ;
  skos:notation "407" ;
  skos:notation 407 ;
  skos:note "0"@en ;
  skos:prefLabel "service interface"@en ;
  skos:prefLabel "서비스 인터페이스"@kr ;
.
<http://iso.org/tc211/term/408>
  rdf:type skos:Concept ;
  dcterms:dateAccepted "2005-12-01"^^xsd:date ;
  dcterms:dateAccepted "2009-12-29"^^xsd:date ;
  dcterms:provenance "KS X ISO 19128" ;
  dcterms:source "ISO 19128:2005" ;
  reg:status reg:statusValid ;
  rdfs:label "service metadata"@en ;
  skos:changeNote "valid" ;
  skos:definition "서버에서 활용할 수 있는 연산과 지리 정보를 기술하는 메타데이터"@kr ;
  skos:editorialNote "preferred" ;
  skos:editorialNote "preferred"^^xsd:string ;
  skos:notation "408" ;
  skos:notation 408 ;
  skos:prefLabel "service metadata"@en ;
  skos:prefLabel "서비스 메타데이터"@kr ;
.
<http://iso.org/tc211/term/409>
  rdf:type skos:Concept ;
  dcterms:dateAccepted "2003-05-01"^^xsd:date ;
  dcterms:dateAccepted "2009-12-29"^^xsd:date ;
  dcterms:provenance "KS X ISO 19107" ;
  dcterms:source "ISO 19107:2003" ;
  reg:status reg:statusValid ;
  rdfs:label "set"@en ;
  skos:changeNote "valid" ;
  skos:definition "순서를 갖지 않으며 반복을 허락하지 않는 관련 항목들(객체 또는 값)의 모음"@kr ;
  skos:editorialNote "preferred" ;
  skos:editorialNote "preferred"^^xsd:string ;
  skos:notation "409" ;
  skos:notation 409 ;
  skos:prefLabel "set"@en ;
  skos:prefLabel "집합"@kr ;
.
<http://iso.org/tc211/term/41>
  rdf:type skos:Concept ;
  dcterms:dateAccepted "2003-05-01"^^xsd:date ;
  dcterms:dateAccepted "2009-12-29"^^xsd:date ;
  dcterms:provenance "KS X ISO 19107" ;
  dcterms:source "ISO 19107:2003" ;
  reg:status reg:statusValid ;
  rdfs:label "circular sequence"@en ;
  skos:changeNote "valid" ;
  skos:definition "논리적인 시작점이 존재하지 않기 때문에 어떤 한 점에서 수열을 이동하더라도 항상 동일한 연속; 따라서 연속의 마지막 항목이 첫 항목에 앞서는 것으로 간주됨"@kr ;
  skos:editorialNote "preferred" ;
  skos:editorialNote "preferred"^^xsd:string ;
  skos:notation "41" ;
  skos:notation 41 ;
  skos:prefLabel "circular sequence"@en ;
  skos:prefLabel "순환 연속"@kr ;
.
<http://iso.org/tc211/term/410>
  rdf:type skos:Concept ;
  dcterms:dateAccepted "2003-05-01"^^xsd:date ;
  dcterms:dateAccepted "2009-12-29"^^xsd:date ;
  dcterms:provenance "KS X ISO 19107" ;
  dcterms:source "ISO 19107:2003" ;
  reg:status reg:statusValid ;
  rdfs:comment "Note 1 to entry: Shells are used to describe boundary components of solids in 3D coordinate systems."@en ;
  rdfs:comment "비고: 외면은 3차원 좌표 체계에서 입방체의 경계 컴포넌트를 기술하기 위해 사용된다."@kr ;
  rdfs:label "shell"@en ;
  skos:changeNote "valid" ;
  skos:definition "순환하는 단순 표면"@kr ;
  skos:editorialNote "preferred" ;
  skos:editorialNote "preferred"^^xsd:string ;
  skos:notation "410" ;
  skos:notation 410 ;
  skos:note "Note 1 to entry: Shells are used to describe boundary components of solids in 3D coordinate systems."@en ;
  skos:note "비고: 외면은 3차원 좌표 체계에서 입방체의 경계 컴포넌트를 기술하기 위해 사용된다."@kr ;
  skos:prefLabel "shell"@en ;
  skos:prefLabel "외면"@kr ;
.
<http://iso.org/tc211/term/411>
  rdf:type skos:Concept ;
  dcterms:dateAccepted "2003-05-01"^^xsd:date ;
  dcterms:dateAccepted "2009-12-29"^^xsd:date ;
  dcterms:provenance "KS X ISO 19107" ;
  dcterms:source "ISO 19107:2003" ;
  reg:status reg:statusValid ;
  rdfs:comment "Note 1 to entry: This implies that no interior direct position is involved in a self-intersection of any kind."@en ;
  rdfs:comment "비고: 이는 내부의 직접 위치가 어느 종류의 자기 교차도 수반하지 않음을 의미한다."@kr ;
  rdfs:label "simple"@en ;
  skos:changeNote "valid" ;
  skos:definition "내부가 균등하여(모든 점은 동형의 인접군을 가짐) 적절한 차원의 유클리드 좌표공간의 개방 부분 집합 어느 곳에서도 국지적으로 동형인 기하 객체의 특성"@kr ;
  skos:editorialNote "preferred" ;
  skos:editorialNote "preferred"^^xsd:string ;
  skos:notation "411" ;
  skos:notation 411 ;
  skos:note "Note 1 to entry: This implies that no interior direct position is involved in a self-intersection of any kind."@en ;
  skos:note "비고: 이는 내부의 직접 위치가 어느 종류의 자기 교차도 수반하지 않음을 의미한다."@kr ;
  skos:prefLabel "simple"@en ;
  skos:prefLabel "단순"@kr ;
.
<http://iso.org/tc211/term/412>
  rdf:type skos:Concept ;
  dcterms:dateAccepted "2004-08-01"^^xsd:date ;
  dcterms:dateAccepted "2007-11-01"^^xsd:date ;
  dcterms:provenance "KS X ISO 19125-1" ;
  dcterms:source "ISO 19125-1:2004" ;
  reg:status reg:statusValid ;
  rdfs:label "simple feature"@en ;
  skos:changeNote "valid" ;
  skos:definition "공간 속성, 비공간 속성을 모두 갖는 정점들 간의 선형 보간에 의해 2차원 기하로 제한된 피처"@kr ;
  skos:editorialNote "preferred" ;
  skos:editorialNote "preferred"^^xsd:string ;
  skos:notation "412" ;
  skos:notation 412 ;
  skos:prefLabel "simple feature"@en ;
  skos:prefLabel "단순 지형지물"@kr ;
.
<http://iso.org/tc211/term/415>
  rdf:type skos:Concept ;
  dcterms:dateAccepted "2005-10-15"^^xsd:date ;
  dcterms:dateAccepted "2006-12-01"^^xsd:date ;
  dcterms:provenance "KS X ISO 19133" ;
  dcterms:source "ISO 19133:2005" ;
  reg:status reg:statusValid ;
  rdfs:label "slope"@en ;
  skos:changeNote "valid" ;
  skos:definition "곡선 길이에 관한 표고 변화율"@kr ;
  skos:editorialNote "preferred" ;
  skos:editorialNote "preferred"^^xsd:string ;
  skos:notation "415" ;
  skos:notation 415 ;
  skos:prefLabel "slope"@en ;
  skos:prefLabel "경사"@kr ;
.
<http://iso.org/tc211/term/416>
  rdf:type skos:Concept ;
  dcterms:dateAccepted "2003-05-01"^^xsd:date ;
  dcterms:dateAccepted "2009-12-29"^^xsd:date ;
  dcterms:provenance "KS X ISO 19107" ;
  dcterms:source "ISO 19107:2003" ;
  reg:status reg:statusValid ;
  rdfs:comment "Note 1 to entry: A solid is realizable locally as a three parameter set of direct positions. The boundary of a solid is the set of oriented, closed surfaces that comprise the limits of the solid."@en ;
  rdfs:comment "비고: 입방체는 직접 위치의 세 매개 변수 집합으로 국지적으로 실현될 수 있다. 입방체의 경계는 입방체의 경계를 포함하는 방향성이 있으며 폐합된 표면의 집합이다."@kr ;
  rdfs:label "solid"@en ;
  skos:changeNote "valid" ;
  skos:definition "유클리드 3차원 공간 구역의 연속 영상을 표현하는 3차원 기하 원시 객체"@kr ;
  skos:editorialNote "preferred" ;
  skos:editorialNote "preferred"^^xsd:string ;
  skos:notation "416" ;
  skos:notation 416 ;
  skos:note "Note 1 to entry: A solid is realizable locally as a three parameter set of direct positions. The boundary of a solid is the set of oriented, closed surfaces that comprise the limits of the solid."@en ;
  skos:note "비고: 입방체는 직접 위치의 세 매개 변수 집합으로 국지적으로 실현될 수 있다. 입방체의 경계는 입방체의 경계를 포함하는 방향성이 있으며 폐합된 표면의 집합이다."@kr ;
  skos:prefLabel "solid"@en ;
  skos:prefLabel "입방체"@kr ;
.
<http://iso.org/tc211/term/417>
  rdf:type skos:Concept ;
  dcterms:dateAccepted "2005-10-15"^^xsd:date ;
  dcterms:dateAccepted "2009-12-29"^^xsd:date ;
  dcterms:provenance "KS X ISO 19135" ;
  dcterms:source "ISO 19135:2005" ;
  reg:status reg:statusValid ;
  rdfs:label "source reference"@en ;
  skos:changeNote "valid" ;
  skos:definition "외부 출처로부터 등록물에 채택된 항목의 출처에 대한 참조"@kr ;
  skos:editorialNote "preferred" ;
  skos:editorialNote "preferred"^^xsd:string ;
  skos:notation "417" ;
  skos:notation 417 ;
  skos:prefLabel "source reference"@en ;
  skos:prefLabel "출처참조"@kr ;
.
<http://iso.org/tc211/term/418>
  rdf:type skos:Concept ;
  dcterms:dateAccepted "2005-06-01"^^xsd:date ;
  dcterms:dateAccepted "2006-05-01"^^xsd:date ;
  dcterms:provenance "ISO 19117:2005" ;
  dcterms:source "ISO 19117:2012, 4.29" ;
  reg:status reg:statusValid ;
  rdfs:label "spatial attribute"@en ;
  skos:changeNote "valid" ;
  skos:definition "좌표, 수학적 함수와/또는 경계 위상 관계 등으로 피처의 공간적 표현을 기술하는 피처 속성"@kr ;
  skos:editorialNote "preferred" ;
  skos:editorialNote "preferred"^^xsd:string ;
  skos:notation "418" ;
  skos:notation 418 ;
  skos:prefLabel "spatial attribute"@en ;
  skos:prefLabel "공간 속성"@kr ;
.
<http://iso.org/tc211/term/419>
  rdf:type skos:Concept ;
  dcterms:dateAccepted "2003-05-01"^^xsd:date ;
  dcterms:dateAccepted "2009-12-29"^^xsd:date ;
  dcterms:provenance "KS X ISO 19107" ;
  dcterms:source "ISO 19107:2003" ;
  reg:status reg:statusValid ;
  rdfs:label "spatial object"@en ;
  skos:changeNote "valid" ;
  skos:definition "피처의 공간 특성을 표현하는 데 사용된 객체"@kr ;
  skos:editorialNote "preferred" ;
  skos:editorialNote "preferred"^^xsd:string ;
  skos:notation "419" ;
  skos:notation 419 ;
  skos:prefLabel "spatial object"@en ;
  skos:prefLabel "공간 객체"@kr ;
.
<http://iso.org/tc211/term/420>
  rdf:type skos:Concept ;
  dcterms:dateAccepted "2003-05-01"^^xsd:date ;
  dcterms:dateAccepted "2009-12-29"^^xsd:date ;
  dcterms:provenance "KS X ISO 19107" ;
  dcterms:source "ISO 19107:2003" ;
  reg:status reg:statusValid ;
  rdfs:comment "Note 1 to entry: Any UML operation on a spatial object would be classified as a spatial operator as are the query operators in clause 8 of IS 19107."@en ;
  rdfs:comment "비고: 공간 객체에 대한 모든 UML 연산은 공간연산으로 분류된다(KS X ISO 19107, 8절)."@kr ;
  rdfs:label "spatial operator"@en ;
  skos:changeNote "valid" ;
  skos:definition "영역이나 범위 내에 적어도 하나의 공간 매개 변수를 갖는 함수 또는 절차"@kr ;
  skos:editorialNote "preferred" ;
  skos:editorialNote "preferred"^^xsd:string ;
  skos:notation "420" ;
  skos:notation 420 ;
  skos:note "Note 1 to entry: Any UML operation on a spatial object would be classified as a spatial operator as are the query operators in clause 8 of IS 19107."@en ;
  skos:note "비고: 공간 객체에 대한 모든 UML 연산은 공간연산으로 분류된다(KS X ISO 19107, 8절)."@kr ;
  skos:prefLabel "spatial operator"@en ;
  skos:prefLabel "공간 연산자"@kr ;
.
<http://iso.org/tc211/term/421>
  rdf:type skos:Concept ;
  dcterms:dateAccepted "2003-02-15" ;
  dcterms:dateAccepted "2003-02-15"^^xsd:date ;
  dcterms:dateAccepted "2007-11-01"^^xsd:date ;
  dcterms:provenance "ISO 19111:2003" ;
  dcterms:provenance "KS X ISO 19111" ;
  dcterms:source "ISO 19111:2007" ;
  reg:status reg:statusAccepted ;
  reg:status reg:statusValid ;
  rdfs:comment "Note 1 to entry: This may take the form of a label, code or coordinate tuple."@en ;
  rdfs:comment "OPMERKING Dit kan in de vorm van een label, code of coördinaattupel zijn."@en ;
  rdfs:comment "비고: 공간 참조는 라벨, 코드 또는 좌표 튜플의 형태를 가질 수 있다."@kr ;
  rdfs:label "spatial reference"@en ;
  skos:changeNote "valid" ;
  skos:definition "beschrijving van een positie in de werkelijke wereld"@nl ;
  skos:definition "실세계에서의 위치에 대한 기술"@kr ;
  skos:editorialNote "preferred" ;
  skos:editorialNote "preferred"^^xsd:string ;
  skos:notation "421" ;
  skos:notation 421 ;
  skos:note "Note 1 to entry: This may take the form of a label, code or coordinate tuple."@en ;
  skos:note "OPMERKING Dit kan in de vorm van een label, code of coördinaattupel zijn."@en ;
  skos:note "비고: 공간 참조는 라벨, 코드 또는 좌표 튜플의 형태를 가질 수 있다."@kr ;
  skos:prefLabel "ruimtelijke referentie"@nl ;
  skos:prefLabel "spatial reference"@en ;
  skos:prefLabel "공간 참조"@kr ;
.
<http://iso.org/tc211/term/422>
  rdf:type skos:Concept ;
  dcterms:dateAccepted "2003-10-15" ;
  dcterms:dateAccepted "2003-10-15"^^xsd:date ;
  dcterms:dateAccepted "2009-12-29"^^xsd:date ;
  dcterms:provenance "KS X ISO 19112" ;
  dcterms:provenance "NEN 3610" ;
  dcterms:source "ISO 19112:2003" ;
  reg:status reg:statusAccepted ;
  reg:status reg:statusValid ;
  rdfs:comment "Identificatie van een positie kan door coördinaten (directe locatie) en door geografische identificatoren (indirecte locatie)."@en ;
  rdfs:label "spatial reference system"@en ;
  skos:changeNote "valid" ;
  skos:definition "model (systeem) voor identificatie van een positie (locatie) in de werkelijkheid"@nl ;
  skos:definition "실세계에서 위치의 식별을 위한 시스템"@kr ;
  skos:editorialNote "preferred" ;
  skos:editorialNote "preferred"^^xsd:string ;
  skos:notation "422" ;
  skos:notation 422 ;
  skos:note "Identificatie van een positie kan door coördinaten (directe locatie) en door geografische identificatoren (indirecte locatie)."@en ;
  skos:prefLabel "ruimtelijk referentiesysteem"@nl ;
  skos:prefLabel "spatial reference system"@en ;
  skos:prefLabel "공간 참조 체계"@kr ;
.
<http://iso.org/tc211/term/423>
  rdf:type skos:Concept ;
  dcterms:dateAccepted "2005-08-15"^^xsd:date ;
  dcterms:dateAccepted "2007-11-01"^^xsd:date ;
  dcterms:provenance "KS X ISO 19123" ;
  dcterms:source "ISO 19123:2005" ;
  reg:status reg:statusValid ;
  rdfs:comment "Note 1 to entry: The spatiotemporal domain of a continuous coverage consists of a set of direct positions defined in relation to a collection of spatiotemporal objects."@en ;
  rdfs:comment "비고: 연속 커버리지의 시공간 영역은 시공간객체의 모음에 대한 관계로 정의된 직접 위치의 집합으로 구성된다."@kr ;
  rdfs:label "spatiotemporal domain <coverage>"@en ;
  skos:changeNote "valid" ;
  skos:definition "시공간 객체로 구성된 영역"@kr ;
  skos:editorialNote "preferred" ;
  skos:editorialNote "preferred"^^xsd:string ;
  skos:notation "423" ;
  skos:notation 423 ;
  skos:note "Note 1 to entry: The spatiotemporal domain of a continuous coverage consists of a set of direct positions defined in relation to a collection of spatiotemporal objects."@en ;
  skos:note "비고: 연속 커버리지의 시공간 영역은 시공간객체의 모음에 대한 관계로 정의된 직접 위치의 집합으로 구성된다."@kr ;
  skos:prefLabel "spatiotemporal domain <coverage>"@en ;
  skos:prefLabel "시공간 영역 <커버리지>"@kr ;
.
<http://iso.org/tc211/term/424>
  rdf:type skos:Concept ;
  dcterms:dateAccepted "2005-08-15"^^xsd:date ;
  dcterms:dateAccepted "2007-11-01"^^xsd:date ;
  dcterms:provenance "KS X ISO 19123" ;
  dcterms:source "ISO 19123:2005" ;
  reg:status reg:statusValid ;
  rdfs:label "spatiotemporal object"@en ;
  skos:changeNote "valid" ;
  skos:definition "공간 및 시간에서 직접 위치의 집합을 표현하는 객체"@kr ;
  skos:editorialNote "preferred" ;
  skos:editorialNote "preferred"^^xsd:string ;
  skos:notation "424" ;
  skos:notation 424 ;
  skos:prefLabel "spatiotemporal object"@en ;
  skos:prefLabel "시공간 객체"@kr ;
.
<http://iso.org/tc211/term/425>
  rdf:type skos:Concept ;
  dcterms:dateAccepted "2005-07-15"^^xsd:date ;
  dcterms:dateAccepted "2009-12-29"^^xsd:date ;
  dcterms:provenance "ISO/TS 19103:2005" ;
  dcterms:provenance "KS X ISO 19103" ;
  dcterms:source "ISO/IEC 19501:2005 (Adapted from)" ;
  reg:status reg:statusValid ;
  rdfs:comment "Note 1 to entry: Contrast: implementation."@en ;
  rdfs:comment "비고: 구현과 대조해 보라."@kr ;
  rdfs:label "specification <UML>"@en ;
  skos:changeNote "valid" ;
  skos:definition "대상 또는 행위에 대한 선언적 기술"@kr ;
  skos:editorialNote "preferred" ;
  skos:editorialNote "preferred"^^xsd:string ;
  skos:notation "425" ;
  skos:notation 425 ;
  skos:note "Note 1 to entry: Contrast: implementation."@en ;
  skos:note "비고: 구현과 대조해 보라."@kr ;
  skos:prefLabel "specification <UML>"@en ;
  skos:prefLabel "사양 <UML>"@kr ;
.
<http://iso.org/tc211/term/428>
  rdf:type skos:Concept ;
  dcterms:dateAccepted "2003-05-01"^^xsd:date ;
  dcterms:dateAccepted "2009-12-29"^^xsd:date ;
  dcterms:provenance "KS X ISO 19107" ;
  dcterms:source "ISO 19107:2003" ;
  reg:status reg:statusValid ;
  rdfs:label "start node"@en ;
  skos:changeNote "valid" ;
  skos:definition "변이 포함된 위상 복합체의 유효한 기하 실현에서, 곡선으로서 그 변의 시작 점에 해당하는 변의 경계 상의 절점"@kr ;
  skos:editorialNote "preferred" ;
  skos:editorialNote "preferred"^^xsd:string ;
  skos:notation "428" ;
  skos:notation 428 ;
  skos:prefLabel "start node"@en ;
  skos:prefLabel "시작 절점"@kr ;
.
<http://iso.org/tc211/term/429>
  rdf:type skos:Concept ;
  dcterms:dateAccepted "2003-05-01"^^xsd:date ;
  dcterms:dateAccepted "2009-12-29"^^xsd:date ;
  dcterms:provenance "KS X ISO 19107" ;
  dcterms:source "ISO 19107:2003" ;
  reg:status reg:statusValid ;
  rdfs:label "start point"@en ;
  skos:changeNote "valid" ;
  skos:definition "곡선 최초의 점"@kr ;
  skos:editorialNote "preferred" ;
  skos:editorialNote "preferred"^^xsd:string ;
  skos:notation "429" ;
  skos:notation 429 ;
  skos:prefLabel "start point"@en ;
  skos:prefLabel "시작점"@kr ;
.
<http://iso.org/tc211/term/43>
  rdf:type skos:Concept ;
  dcterms:dateAccepted "2003-05-01"^^xsd:date ;
  dcterms:dateAccepted "2009-12-29"^^xsd:date ;
  dcterms:provenance "ISO/TS 19103:2005" ;
  dcterms:provenance "KS X ISO 19103" ;
  dcterms:source "ISO/IEC 19501:2005 (Adapted from)" ;
  reg:status reg:statusValid ;
  rdfs:comment "Note 1 to entry: A class may use a set of interfaces to specify collections of operations it provides to its environment. See: interface."@en ;
  rdfs:comment "비고: 인터페이스의 집합을 사용하여 연산의 집합을 클래스로 기술할 수 있다."@kr ;
  rdfs:label "class <UML>"@en ;
  skos:changeNote "valid" ;
  skos:definition "동일한 속성, 연산, 방법 및 관계와 의미론을 공유하는 객체 집합의 기술"@kr ;
  skos:editorialNote "preferred" ;
  skos:editorialNote "preferred"^^xsd:string ;
  skos:notation "43" ;
  skos:notation 43 ;
  skos:note "Note 1 to entry: A class may use a set of interfaces to specify collections of operations it provides to its environment. See: interface."@en ;
  skos:note "비고: 인터페이스의 집합을 사용하여 연산의 집합을 클래스로 기술할 수 있다."@kr ;
  skos:prefLabel "class <UML>"@en ;
  skos:prefLabel "클래스 <UML>"@kr ;
.
<http://iso.org/tc211/term/432>
  rdf:type skos:Concept ;
  dcterms:dateAccepted "2005-07-15"^^xsd:date ;
  dcterms:dateAccepted "2009-12-29"^^xsd:date ;
  dcterms:provenance "ISO/TS 19103:2005 ,4.2.26" ;
  dcterms:source "ISO/IEC 19501" ;
  reg:status reg:statusValid ;
  rdfs:comment "Note 1 to entry: Stereotypes must be based on certain existing types or classes in the metamodel. Stereotypes may extend the semantics, but not the structure of pre-existing types and classes. Certain stereotypes are predefined in the UML, others may be user defined. Stereotypes are one of three extensibility mechanisms in UML. The others are constraint and tagged value."@en ;
  rdfs:comment "비고: 스테레오타입은 메타 모델 내에 존재하는 어떤 유형 또는 클래스에 기초해야 한다. 스테레오타입은 의미론을 확장해도 상관없지만, 이미 존재하는 유형과 클래스의 구조는 확장할 수 없다. 스테레오타입은 UML 내에서 사전 규정되거나 또는 사용자가 규정할 수 있다. 스테레오타입은 UML의 세 가지 확장 가능한 메커니즘 중의 하나로 나머지 둘은 제약 조건과 꼬리표 값이다."@kr ;
  rdfs:label "stereotype <UML>"@en ;
  skos:changeNote "valid" ;
  skos:definition "메타 모델의 의미론을 확장하는 모델링 요소의 새로운 유형"@kr ;
  skos:editorialNote "preferred" ;
  skos:editorialNote "preferred"^^xsd:string ;
  skos:notation "432" ;
  skos:notation 432 ;
  skos:note "Note 1 to entry: Stereotypes must be based on certain existing types or classes in the metamodel. Stereotypes may extend the semantics, but not the structure of pre-existing types and classes. Certain stereotypes are predefined in the UML, others may be user defined. Stereotypes are one of three extensibility mechanisms in UML. The others are constraint and tagged value."@en ;
  skos:note "비고: 스테레오타입은 메타 모델 내에 존재하는 어떤 유형 또는 클래스에 기초해야 한다. 스테레오타입은 의미론을 확장해도 상관없지만, 이미 존재하는 유형과 클래스의 구조는 확장할 수 없다. 스테레오타입은 UML 내에서 사전 규정되거나 또는 사용자가 규정할 수 있다. 스테레오타입은 UML의 세 가지 확장 가능한 메커니즘 중의 하나로 나머지 둘은 제약 조건과 꼬리표 값이다."@kr ;
  skos:prefLabel "stereotype <UML>"@en ;
  skos:prefLabel "스테레오타입 <UML>"@kr ;
.
<http://iso.org/tc211/term/433>
  rdf:type skos:Concept ;
  dcterms:dateAccepted "2003-05-01"^^xsd:date ;
  dcterms:dateAccepted "2009-12-29"^^xsd:date ;
  dcterms:provenance "KS X ISO 19107" ;
  dcterms:source "ISO 19107:2003" ;
  reg:status reg:statusValid ;
  rdfs:comment "Note 1 to entry: The weaker forms of substitutability make various restrictions on the context of the implied substitution."@en ;
  rdfs:comment "비고: 보다 약한 유형의 대체성은 함축된 대용의 상황에서 다양한 제한을 만든다."@kr ;
  rdfs:label "strong substitutability"@en ;
  skos:changeNote "valid" ;
  skos:definition "클래스의 특정 인스턴스를 위한 능력으로, 이는 상속을 통한 자손이거나, 특정 상황에서 그것의 조상의 인스턴스 대신 사용되는 다른 클래스, 유형 또는 인터페이스의 실현을 의미  "@kr ;
  skos:editorialNote "preferred" ;
  skos:editorialNote "preferred"^^xsd:string ;
  skos:notation "433" ;
  skos:notation 433 ;
  skos:note "Note 1 to entry: The weaker forms of substitutability make various restrictions on the context of the implied substitution."@en ;
  skos:note "비고: 보다 약한 유형의 대체성은 함축된 대용의 상황에서 다양한 제한을 만든다."@kr ;
  skos:prefLabel "strong substitutability"@en ;
  skos:prefLabel "강한 대체성"@kr ;
.
<http://iso.org/tc211/term/434>
  rdf:type skos:Concept ;
  dcterms:dateAccepted "2003-05-01"^^xsd:date ;
  dcterms:dateAccepted "2009-12-29"^^xsd:date ;
  dcterms:provenance "KS X ISO 19107" ;
  dcterms:source "ISO 19107:2003" ;
  reg:status reg:statusValid ;
  rdfs:comment "Note 1 to entry: Since the definitions of geometric complex and topological complex require only that they be closed under boundary operations, the set of any primitives of a particular dimension and below is always a subcomplex of the original, larger complex. Thus, any full planar topological complex contains an edge-node graph as a subcomplex."@en ;
  rdfs:comment "비고: 기하 복합체 및 위상 복합체의 정의에서는 이들이 경계 연산에서 폐합되어야 함을 요구하기 때문에, 특정차원 및 하위 차원의 모든 원시객체 집합은 항상 원시의, 더 큰 복합체의 하위 복합체이다. 따라서 모든 완전 평면 위상 복합체는 하위 복합체로 변-절점 그래프를 포함한다."@kr ;
  rdfs:label "subcomplex"@en ;
  skos:changeNote "valid" ;
  skos:definition "복합체의 요소 전체가 보다 큰 복합체에 포함되어 있는 복합체"@kr ;
  skos:editorialNote "preferred" ;
  skos:editorialNote "preferred"^^xsd:string ;
  skos:notation "434" ;
  skos:notation 434 ;
  skos:note "Note 1 to entry: Since the definitions of geometric complex and topological complex require only that they be closed under boundary operations, the set of any primitives of a particular dimension and below is always a subcomplex of the original, larger complex. Thus, any full planar topological complex contains an edge-node graph as a subcomplex."@en ;
  skos:note "비고: 기하 복합체 및 위상 복합체의 정의에서는 이들이 경계 연산에서 폐합되어야 함을 요구하기 때문에, 특정차원 및 하위 차원의 모든 원시객체 집합은 항상 원시의, 더 큰 복합체의 하위 복합체이다. 따라서 모든 완전 평면 위상 복합체는 하위 복합체로 변-절점 그래프를 포함한다."@kr ;
  skos:prefLabel "subcomplex"@en ;
  skos:prefLabel "하위 복합체"@kr ;
.
<http://iso.org/tc211/term/435>
  rdf:type skos:Concept ;
  dcterms:dateAccepted "2005-10-15"^^xsd:date ;
  dcterms:dateAccepted "2009-12-29"^^xsd:date ;
  dcterms:provenance "KS X ISO 19135" ;
  dcterms:source "ISO 19135:2005" ;
  reg:status reg:statusValid ;
  rdfs:label "submitting organization"@en ;
  skos:changeNote "valid" ;
  skos:definition "등록물 소유자로부터 등록물의 내용에 대한 변경을 제안하도록 위임 받은 기구"@kr ;
  skos:editorialNote "preferred" ;
  skos:editorialNote "preferred"^^xsd:string ;
  skos:notation "435" ;
  skos:notation 435 ;
  skos:prefLabel "submitting organization"@en ;
  skos:prefLabel "제출 기구"@kr ;
.
<http://iso.org/tc211/term/436>
  rdf:type skos:Concept ;
  dcterms:dateAccepted "2005-10-15"^^xsd:date ;
  dcterms:dateAccepted "2009-12-29"^^xsd:date ;
  dcterms:provenance "KS X ISO 19135" ;
  dcterms:source "ISO 19135:2005" ;
  reg:status reg:statusValid ;
  rdfs:label "subregister"@en ;
  skos:changeNote "valid" ;
  skos:definition "정보 영역의 한 부분에 대한 항목을 포함하는 계층적 등록물의 일부"@kr ;
  skos:editorialNote "preferred" ;
  skos:editorialNote "preferred"^^xsd:string ;
  skos:notation "436" ;
  skos:notation 436 ;
  skos:prefLabel "subregister"@en ;
  skos:prefLabel "하위 등록물"@kr ;
.
<http://iso.org/tc211/term/437>
  rdf:type skos:Concept ;
  dcterms:dateAccepted "2003-05-01"^^xsd:date ;
  dcterms:dateAccepted "2009-12-29"^^xsd:date ;
  dcterms:provenance "KS X ISO 19107" ;
  dcterms:source "ISO 19107:2003" ;
  reg:status reg:statusValid ;
  rdfs:comment "Note 1 to entry: The boundary of a surface is the set of oriented, closed curves that delineate the limits of the surface. Surfaces that are isomorphic to a sphere, or to an n-torus (a topological sphere with n \"handles\") have no boundary. Such surfaces are called cycles."@en ;
  rdfs:comment "비고: 표면의 경계는 표면의 한계를 그리는 방향성을 갖는, 폐합 곡선의 집합이다. 구 또는 n-원환제(n\"핸들\"을 갖는 위상구)와 동형인 표면은 경계를 갖지 않는다. 이러한 표면을 순환이라고 부른다."@kr ;
  rdfs:label "surface"@en ;
  skos:changeNote "valid" ;
  skos:definition "평면 구역의 연속 영상을 국지적으로 표현하는 2차원 기하 원시 객체"@kr ;
  skos:editorialNote "preferred" ;
  skos:editorialNote "preferred"^^xsd:string ;
  skos:notation "437" ;
  skos:notation 437 ;
  skos:note "Note 1 to entry: The boundary of a surface is the set of oriented, closed curves that delineate the limits of the surface. Surfaces that are isomorphic to a sphere, or to an n-torus (a topological sphere with n \"handles\") have no boundary. Such surfaces are called cycles."@en ;
  skos:note "비고: 표면의 경계는 표면의 한계를 그리는 방향성을 갖는, 폐합 곡선의 집합이다. 구 또는 n-원환제(n\"핸들\"을 갖는 위상구)와 동형인 표면은 경계를 갖지 않는다. 이러한 표면을 순환이라고 부른다."@kr ;
  skos:prefLabel "surface"@en ;
  skos:prefLabel "표면"@kr ;
.
<http://iso.org/tc211/term/438>
  rdf:type skos:Concept ;
  dcterms:dateAccepted "2003-05-01"^^xsd:date ;
  dcterms:dateAccepted "2009-12-29"^^xsd:date ;
  dcterms:provenance "KS X ISO 19107" ;
  dcterms:source "ISO 19107:2003" ;
  reg:status reg:statusValid ;
  rdfs:label "surface patch"@en ;
  skos:changeNote "valid" ;
  skos:definition "동종의 보간법 및 정의 방법을 사용하여 표면의 연속적인 부분을 표현하는데 사용되는 2차원의 연결된 기하 객체"@kr ;
  skos:editorialNote "preferred" ;
  skos:editorialNote "preferred"^^xsd:string ;
  skos:notation "438" ;
  skos:notation 438 ;
  skos:prefLabel "surface patch"@en ;
  skos:prefLabel "표면 조각"@kr ;
.
<http://iso.org/tc211/term/44>
  rdf:type skos:Concept ;
  dcterms:dateAccepted "2005-07-15"^^xsd:date ;
  dcterms:dateAccepted "2009-12-29"^^xsd:date ;
  dcterms:provenance "ISO/TS 19103:2005 ,4.2.8" ;
  dcterms:source "ISO/IEC 19501" ;
  reg:status reg:statusValid ;
  rdfs:comment "Note 1 to entry: Classifiers include interfaces, classes, datatypes, and components."@en ;
  rdfs:comment "비고: 분류자에는 인터페이스, 클래스, 데이터 유형, 컴포넌트 등이 포함된다."@kr ;
  rdfs:label "classifier <UML>"@en ;
  skos:changeNote "valid" ;
  skos:definition "행위 및 구조적 특성을 기술하는 메커니즘"@kr ;
  skos:editorialNote "preferred" ;
  skos:editorialNote "preferred"^^xsd:string ;
  skos:notation "44" ;
  skos:notation 44 ;
  skos:note "Note 1 to entry: Classifiers include interfaces, classes, datatypes, and components."@en ;
  skos:note "비고: 분류자에는 인터페이스, 클래스, 데이터 유형, 컴포넌트 등이 포함된다."@kr ;
  skos:prefLabel "classifier <UML>"@en ;
  skos:prefLabel "분류자 <UML>"@kr ;
.
<http://iso.org/tc211/term/440>
  rdf:type skos:Concept ;
  dcterms:dateAccepted "2000-12-15"^^xsd:date ;
  dcterms:dateAccepted "2007-06-29"^^xsd:date ;
  dcterms:provenance "KS X ISO 19105" ;
  dcterms:source "ISO 19105:2000" ;
  reg:status reg:statusValid ;
  rdfs:label "System Under Test"@en ;
  skos:altLabel "SUT"@kr ;
  skos:altLabel "SUT"^^<http://www.w3.org/2001/XMLSchema#@en> ;
  skos:changeNote "valid" ;
  skos:definition "IUT를 지원하는 데 필요한 컴퓨터 하드웨어, 소프트웨어 및 통신망"@kr ;
  skos:editorialNote "preferred" ;
  skos:editorialNote "preferred"^^xsd:string ;
  skos:notation "440" ;
  skos:notation 440 ;
  skos:prefLabel "System Under Test"@en ;
  skos:prefLabel "시험용 시스템"@kr ;
.
<http://iso.org/tc211/term/441>
  rdf:type skos:Concept ;
  dcterms:dateAccepted "2007-09-01"^^xsd:date ;
  dcterms:dateAccepted "2009-12-29"^^xsd:date ;
  dcterms:provenance "KS X ISO 19136" ;
  dcterms:source "ISO 19136:2007" ;
  reg:status reg:statusValid ;
  rdfs:comment "Note 1 to entry: A tag with no forward slash (e.g. <Road> ) is called a start-tag (also opening tag), and one with a forward slash (e.g. </Road> is called an end-tag (also closing tag)."@en ;
  rdfs:comment "비고: 앞쪽에 사선(/) 표시가 없는 꼬리표(예,<도로>)는 시작-꼬리표(또는 오픈 태그)라 하고, 앞쪽에 사선 표시가 되어 있는 꼬리표(예,</도로>)는 종료-꼬리표(또는 마감 꼬리표)라 한다."@kr ;
  rdfs:label "tag <XML>"@en ;
  skos:changeNote "valid" ;
  skos:definition "XML 문서에서 요소의 범위를 정하는 내용의 마크업"@kr ;
  skos:editorialNote "preferred" ;
  skos:editorialNote "preferred"^^xsd:string ;
  skos:notation "441" ;
  skos:notation 441 ;
  skos:note "Note 1 to entry: A tag with no forward slash (e.g. <Road> ) is called a start-tag (also opening tag), and one with a forward slash (e.g. </Road> is called an end-tag (also closing tag)."@en ;
  skos:note "비고: 앞쪽에 사선(/) 표시가 없는 꼬리표(예,<도로>)는 시작-꼬리표(또는 오픈 태그)라 하고, 앞쪽에 사선 표시가 되어 있는 꼬리표(예,</도로>)는 종료-꼬리표(또는 마감 꼬리표)라 한다."@kr ;
  skos:prefLabel "tag <XML>"@en ;
  skos:prefLabel "꼬리표 <XML>"@kr ;
.
<http://iso.org/tc211/term/442>
  rdf:type skos:Concept ;
  dcterms:dateAccepted "2005-07-15"^^xsd:date ;
  dcterms:dateAccepted "2009-12-29"^^xsd:date ;
  dcterms:provenance "ISO/TS 19103:2005 ,4.2.27" ;
  dcterms:source "ISO/IEC 19501" ;
  reg:status reg:statusValid ;
  rdfs:comment "Note 1 to entry: In a tagged value, the name is referred as the tag. Certain tags are predefined in the UML; others may be user defined. Tagged values are one of three extensibility mechanisms in UML. The others are constraint and stereotype."@en ;
  rdfs:comment "비고: 꼬리표 값에서 이름은 꼬리표로 언급된다. 꼬리표는 UML에서 사전 규정되거나 또는 사용자가 규정할 수 있다. 꼬리표 값은 UML에서 세 가지 확장 가능한 메카니즘 중의 하나로 나머지 둘은 제약 조건과 스테레오타입이 있다."@kr ;
  rdfs:label "tagged value <UML>"@en ;
  skos:changeNote "valid" ;
  skos:definition "이름-값쌍으로서 기술된 특성의 명시적 정의"@kr ;
  skos:editorialNote "preferred" ;
  skos:editorialNote "preferred"^^xsd:string ;
  skos:notation "442" ;
  skos:notation 442 ;
  skos:note "Note 1 to entry: In a tagged value, the name is referred as the tag. Certain tags are predefined in the UML; others may be user defined. Tagged values are one of three extensibility mechanisms in UML. The others are constraint and stereotype."@en ;
  skos:note "비고: 꼬리표 값에서 이름은 꼬리표로 언급된다. 꼬리표는 UML에서 사전 규정되거나 또는 사용자가 규정할 수 있다. 꼬리표 값은 UML에서 세 가지 확장 가능한 메카니즘 중의 하나로 나머지 둘은 제약 조건과 스테레오타입이 있다."@kr ;
  skos:prefLabel "tagged value <UML>"@en ;
  skos:prefLabel "꼬리표값 <UML>"@kr ;
.
<http://iso.org/tc211/term/443>
  rdf:type skos:Concept ;
  dcterms:dateAccepted "2005-10-15"^^xsd:date ;
  dcterms:dateAccepted "2009-12-29"^^xsd:date ;
  dcterms:provenance "ISO 19135:2005" ;
  dcterms:provenance "KS X ISO 19135" ;
  dcterms:source "Annex E, ISO/IEC JTC1Procedures(Adapted from)" ;
  reg:status reg:statusValid ;
  rdfs:label "technical standard"@en ;
  skos:changeNote "valid" ;
  skos:definition "등록을 요하는 항목 클래스의 정의를 포함하는 표준"@kr ;
  skos:editorialNote "preferred" ;
  skos:editorialNote "preferred"^^xsd:string ;
  skos:notation "443" ;
  skos:notation 443 ;
  skos:prefLabel "technical standard"@en ;
  skos:prefLabel "기술 표준"@kr ;
.
<http://iso.org/tc211/term/444>
  rdf:type skos:Concept ;
  dcterms:dateAccepted "2005-02-15"^^xsd:date ;
  dcterms:dateAccepted "2006-12-29"^^xsd:date ;
  dcterms:provenance "ISO 19119:2005" ;
  dcterms:provenance "KS X ISO/IEC 10746-2" ;
  dcterms:source "ISO/10746-3:1996" ;
  reg:status reg:statusValid ;
  rdfs:label "technology viewpoint"@en ;
  skos:changeNote "valid" ;
  skos:definition "시스템 내 기술 선택에 초점을 맞춘 개방형 분산 처리 시스템과 그 환경에 관한 관점"@kr ;
  skos:editorialNote "preferred" ;
  skos:editorialNote "preferred"^^xsd:string ;
  skos:notation "444" ;
  skos:notation 444 ;
  skos:prefLabel "technology viewpoint"@en ;
  skos:prefLabel "기술 관점"@kr ;
.
<http://iso.org/tc211/term/445>
  rdf:type skos:Concept ;
  dcterms:dateAccepted "2002-09-01"^^xsd:date ;
  dcterms:dateAccepted "2007-11-01"^^xsd:date ;
  dcterms:provenance "KS X ISO 19108" ;
  dcterms:source "ISO 19108;2002" ;
  reg:status reg:statusValid ;
  rdfs:label "temporal coordinate"@en ;
  skos:changeNote "valid" ;
  skos:definition "시간 좌표계에 근거하여 사용되는 간격 척도의 원점으로부터의 거리"@kr ;
  skos:editorialNote "preferred" ;
  skos:editorialNote "preferred"^^xsd:string ;
  skos:notation "445" ;
  skos:notation 445 ;
  skos:prefLabel "temporal coordinate"@en ;
  skos:prefLabel "시간 좌표"@kr ;
.
<http://iso.org/tc211/term/446>
  rdf:type skos:Concept ;
  dcterms:dateAccepted "2002-09-01"^^xsd:date ;
  dcterms:dateAccepted "2007-11-01"^^xsd:date ;
  dcterms:provenance "KS X ISO 19108" ;
  dcterms:source "ISO 19108;2002" ;
  reg:status reg:statusValid ;
  rdfs:label "temporal coordinate system"@en ;
  skos:changeNote "valid" ;
  skos:definition "단일 시간 단위로 측정된 길이를 통해 정의된 간격 척도를 기초로 하는 시간 참조 체계"@kr ;
  skos:editorialNote "preferred" ;
  skos:editorialNote "preferred"^^xsd:string ;
  skos:notation "446" ;
  skos:notation 446 ;
  skos:prefLabel "temporal coordinate system"@en ;
  skos:prefLabel "시간좌표계"@kr ;
.
<http://iso.org/tc211/term/447>
  rdf:type skos:Concept ;
  dcterms:dateAccepted "2002-09-01"^^xsd:date ;
  dcterms:dateAccepted "2007-11-01"^^xsd:date ;
  dcterms:provenance "KS X ISO 19108" ;
  dcterms:source "ISO 19108;2002" ;
  reg:status reg:statusValid ;
  rdfs:label "temporal feature association"@en ;
  skos:changeNote "valid" ;
  skos:definition "시간 또는 시간 제약 조건을 참조하여 특성화한 피처 연관"@kr ;
  skos:editorialNote "preferred" ;
  skos:editorialNote "preferred"^^xsd:string ;
  skos:notation "447" ;
  skos:notation 447 ;
  skos:prefLabel "temporal feature association"@en ;
  skos:prefLabel "시간 지형지물 연관"@kr ;
.
<http://iso.org/tc211/term/448>
  rdf:type skos:Concept ;
  dcterms:dateAccepted "2002-09-01"^^xsd:date ;
  dcterms:dateAccepted "2007-11-01"^^xsd:date ;
  dcterms:provenance "KS X ISO 19108" ;
  dcterms:source "ISO 19108;2002" ;
  reg:status reg:statusValid ;
  rdfs:label "temporal feature operation"@en ;
  skos:changeNote "valid" ;
  skos:definition "시간 함수로 기술된 피처 연산"@kr ;
  skos:editorialNote "preferred" ;
  skos:editorialNote "preferred"^^xsd:string ;
  skos:notation "448" ;
  skos:notation 448 ;
  skos:prefLabel "temporal feature operation"@en ;
  skos:prefLabel "시간 지형지물 연산"@kr ;
.
<http://iso.org/tc211/term/449>
  rdf:type skos:Concept ;
  dcterms:dateAccepted "2002-09-01"^^xsd:date ;
  dcterms:dateAccepted "2007-11-01"^^xsd:date ;
  dcterms:provenance "KS X ISO 19108" ;
  dcterms:source "ISO 19108;2002" ;
  reg:status reg:statusValid ;
  rdfs:label "temporal position"@en ;
  skos:changeNote "valid" ;
  skos:definition "시간 참조 체계에 따른 위치"@kr ;
  skos:editorialNote "preferred" ;
  skos:editorialNote "preferred"^^xsd:string ;
  skos:notation "449" ;
  skos:notation 449 ;
  skos:prefLabel "temporal position"@en ;
  skos:prefLabel "시간 위치"@kr ;
.
<http://iso.org/tc211/term/45>
  rdf:type skos:Concept ;
  dcterms:dateAccepted "2005-12-01"^^xsd:date ;
  dcterms:dateAccepted "2009-12-29"^^xsd:date ;
  dcterms:provenance "KS X ISO 19128" ;
  dcterms:source "ISO 19128:2005" ;
  reg:status reg:statusValid ;
  rdfs:label "client"@en ;
  skos:changeNote "valid" ;
  skos:definition "서버에게 연산을 호출할 수 있는 소프트웨어 컴포넌트"@kr ;
  skos:editorialNote "preferred" ;
  skos:editorialNote "preferred"^^xsd:string ;
  skos:notation "45" ;
  skos:notation 45 ;
  skos:prefLabel "client"@en ;
  skos:prefLabel "클라이언트"@kr ;
.
<http://iso.org/tc211/term/450>
  rdf:type skos:Concept ;
  dcterms:dateAccepted "2002-09-01"^^xsd:date ;
  dcterms:dateAccepted "2007-11-01"^^xsd:date ;
  dcterms:provenance "KS X ISO 19108" ;
  dcterms:source "ISO 19108;2002" ;
  reg:status reg:statusValid ;
  rdfs:label "temporal reference system"@en ;
  skos:changeNote "valid" ;
  skos:definition "시간의 측정을 위한 참조 체계"@kr ;
  skos:editorialNote "preferred" ;
  skos:editorialNote "preferred"^^xsd:string ;
  skos:notation "450" ;
  skos:notation 450 ;
  skos:prefLabel "temporal reference system"@en ;
  skos:prefLabel "시간 참조 체계"@kr ;
.
<http://iso.org/tc211/term/451>
  rdf:type skos:Concept ;
  dcterms:dateAccepted "2008-11-15"^^xsd:date ;
  dcterms:provenance "ISO/TS 19104:2008" ;
  dcterms:source "ISO 1087-1" ;
  reg:status reg:statusValid ;
  rdfs:comment "Note 1 to entry: A term may contain symbols and can have variants, e.g. different forms of spelling."@en ;
  rdfs:label "term"@en ;
  skos:changeNote "valid" ;
  skos:editorialNote "preferred"^^xsd:string ;
  skos:notation 451 ;
  skos:note "Note 1 to entry: A term may contain symbols and can have variants, e.g. different forms of spelling."@en ;
  skos:prefLabel "term"@en ;
.
<http://iso.org/tc211/term/452>
  rdf:type skos:Concept ;
  dcterms:dateAccepted "2008-11-15"^^xsd:date ;
  dcterms:source "ISO/TS 19104:2008" ;
  reg:status reg:statusValid ;
  rdfs:comment "Note 1 to entry: A term equivalent should be accompanied by a definition of the designated concept expressed in the same language as the term equivalent"@en ;
  rdfs:label "term equivalent"@en ;
  skos:changeNote "valid" ;
  skos:editorialNote "preferred"^^xsd:string ;
  skos:notation 452 ;
  skos:note "Note 1 to entry: A term equivalent should be accompanied by a definition of the designated concept expressed in the same language as the term equivalent"@en ;
  skos:prefLabel "term equivalent"@en ;
.
<http://iso.org/tc211/term/453>
  rdf:type skos:Concept ;
  dcterms:dateAccepted "2008-11-15"^^xsd:date ;
  dcterms:source "ISO/TS 19104:2008" ;
  reg:status reg:statusValid ;
  rdfs:label "term instance classification"@en ;
  skos:changeNote "valid" ;
  skos:editorialNote "preferred"^^xsd:string ;
  skos:notation 453 ;
  skos:prefLabel "term instance classification"@en ;
.
<http://iso.org/tc211/term/455>
  rdf:type skos:Concept ;
  dcterms:dateAccepted "2008-11-15"^^xsd:date ;
  dcterms:source "ISO/TS 19104:2008" ;
  reg:status reg:statusValid ;
  rdfs:label "terminological record"@en ;
  skos:changeNote "valid" ;
  skos:editorialNote "preferred"^^xsd:string ;
  skos:notation 455 ;
  skos:prefLabel "terminological record"@en ;
.
<http://iso.org/tc211/term/457>
  rdf:type skos:Concept ;
  dcterms:dateAccepted "2005-08-15"^^xsd:date ;
  dcterms:dateAccepted "2007-11-01"^^xsd:date ;
  dcterms:provenance "KS X ISO 19123" ;
  dcterms:source "ISO 19123:2005" ;
  reg:status reg:statusValid ;
  rdfs:comment "Note 1 to entry: A tessellation composed of congruent regular polygons or polyhedra is a regular tessellation. One composed of regular, but non-congruent polygons or polyhedra is a semi-regular tessellation. Otherwise the tessellation is irregular."@en ;
  rdfs:comment "비고: 합동 정다각형 또는 정다면체로 구성된 테셀러이션은 정규 테셀러이션이다. 정다각형 또는 정다면체이긴 하지만, 합동이 아닌 것은 반-정규 테셀러이션이다. 그렇지 않으면 테셀러이션은 불규칙하다. "@kr ;
  rdfs:label "tessellation"@en ;
  skos:changeNote "valid" ;
  skos:definition "분할되는 공간과 같은 차원을 갖는 인접한 부분 공간의 집합으로의 공간의 분할"@kr ;
  skos:editorialNote "preferred" ;
  skos:editorialNote "preferred"^^xsd:string ;
  skos:notation "457" ;
  skos:notation 457 ;
  skos:note "Note 1 to entry: A tessellation composed of congruent regular polygons or polyhedra is a regular tessellation. One composed of regular, but non-congruent polygons or polyhedra is a semi-regular tessellation. Otherwise the tessellation is irregular."@en ;
  skos:note "비고: 합동 정다각형 또는 정다면체로 구성된 테셀러이션은 정규 테셀러이션이다. 정다각형 또는 정다면체이긴 하지만, 합동이 아닌 것은 반-정규 테셀러이션이다. 그렇지 않으면 테셀러이션은 불규칙하다. "@kr ;
  skos:prefLabel "tessellation"@en ;
  skos:prefLabel "공간 분할"@kr ;
.
<http://iso.org/tc211/term/458>
  rdf:type skos:Concept ;
  dcterms:dateAccepted "2000-12-15"^^xsd:date ;
  dcterms:dateAccepted "2007-06-29"^^xsd:date ;
  dcterms:provenance "KS X ISO 19105" ;
  dcterms:source "ISO 19105:2000" ;
  reg:status reg:statusValid ;
  rdfs:label "testing laboratory"@en ;
  skos:changeNote "valid" ;
  skos:definition "적합성 평가 과정을 수행하는 조직"@kr ;
  skos:editorialNote "preferred" ;
  skos:editorialNote "preferred"^^xsd:string ;
  skos:notation "458" ;
  skos:notation 458 ;
  skos:prefLabel "testing laboratory"@en ;
  skos:prefLabel "시험소"@kr ;
.
<http://iso.org/tc211/term/46>
  rdf:type skos:Concept ;
  dcterms:dateAccepted "2003-05-01"^^xsd:date ;
  dcterms:dateAccepted "2009-12-29"^^xsd:date ;
  dcterms:provenance "KS X ISO 19107" ;
  dcterms:source "ISO 19107:2003" ;
  reg:status reg:statusValid ;
  rdfs:label "closure"@en ;
  skos:changeNote "valid" ;
  skos:definition "위상 객체 또는 기하 객체의 내부와 경계의 합집합"@kr ;
  skos:editorialNote "preferred" ;
  skos:editorialNote "preferred"^^xsd:string ;
  skos:notation "46" ;
  skos:notation 46 ;
  skos:prefLabel "closure"@en ;
  skos:prefLabel "폐합"@kr ;
.
<http://iso.org/tc211/term/460>
  rdf:type skos:Concept ;
  dcterms:dateAccepted "2005-08-15"^^xsd:date ;
  dcterms:dateAccepted "2007-11-01"^^xsd:date ;
  dcterms:provenance "KS X ISO 19123" ;
  dcterms:source "ISO 19123:2005" ;
  reg:status reg:statusValid ;
  rdfs:label "Thiessen polygon"@en ;
  skos:changeNote "valid" ;
  skos:definition "집합 내의 어떤 직접 위치에서도 다각형 내부에 위치한 점까지의 거리가 다른 다각형 내에 위치한 거리보다 가까운 다각형"@kr ;
  skos:editorialNote "preferred" ;
  skos:editorialNote "preferred"^^xsd:string ;
  skos:notation "460" ;
  skos:notation 460 ;
  skos:prefLabel "Thiessen polygon"@en ;
  skos:prefLabel "티센 다각형"@kr ;
.
<http://iso.org/tc211/term/461>
  rdf:type skos:Concept ;
  dcterms:dateAccepted "2003-05-01"^^xsd:date ;
  dcterms:dateAccepted "2009-12-29"^^xsd:date ;
  dcterms:provenance "KS X ISO 19107" ;
  dcterms:source "ISO 19107:2003" ;
  reg:status reg:statusValid ;
  rdfs:comment "Note 1 to entry: The boundary of a topological complex corresponds to the boundary of the geometric realization of the topological complex."@en ;
  rdfs:comment "비고: 위상 복합체의 경계는 위상 복합체의 기하 실현의 경계와 일치한다."@kr ;
  rdfs:label "topological boundary"@en ;
  skos:changeNote "valid" ;
  skos:definition "위상 객체의 범위를 한정하는 보다 작은 위상 차원의 방향성을 갖는 위상 원시 객체 집합을 통해 표현된 경계"@kr ;
  skos:editorialNote "preferred" ;
  skos:editorialNote "preferred"^^xsd:string ;
  skos:notation "461" ;
  skos:notation 461 ;
  skos:note "Note 1 to entry: The boundary of a topological complex corresponds to the boundary of the geometric realization of the topological complex."@en ;
  skos:note "비고: 위상 복합체의 경계는 위상 복합체의 기하 실현의 경계와 일치한다."@kr ;
  skos:prefLabel "topological boundary"@en ;
  skos:prefLabel "위상 경계"@kr ;
.
<http://iso.org/tc211/term/462>
  rdf:type skos:Concept ;
  dcterms:dateAccepted "2002-09-01"^^xsd:date ;
  dcterms:dateAccepted "2009-12-29"^^xsd:date ;
  dcterms:provenance "ISO 19108;2002" ;
  dcterms:provenance "KS X ISO 19107" ;
  dcterms:source "ISO 19107:2003" ;
  reg:status reg:statusValid ;
  rdfs:comment "Note 1 to entry: Closed under the boundary operations means that if a topological primitive is in the topological complex, then its boundary objects are also in the topological complex."@en ;
  rdfs:comment "비고: 경계 연산에 대하여 닫혀져 있다는 것은 위상 원시 객체가 위상 복합체 내에 있다면 그것의 경계 객체들도 위상 복합체 내에 있음을 의미한다."@kr ;
  rdfs:label "topological complex"@en ;
  skos:changeNote "valid" ;
  skos:definition "경계 연산에 대하여 닫혀진 위상 원시 객체의 모음"@kr ;
  skos:editorialNote "preferred" ;
  skos:editorialNote "preferred"^^xsd:string ;
  skos:notation "462" ;
  skos:notation 462 ;
  skos:note "Note 1 to entry: Closed under the boundary operations means that if a topological primitive is in the topological complex, then its boundary objects are also in the topological complex."@en ;
  skos:note "비고: 경계 연산에 대하여 닫혀져 있다는 것은 위상 원시 객체가 위상 복합체 내에 있다면 그것의 경계 객체들도 위상 복합체 내에 있음을 의미한다."@kr ;
  skos:prefLabel "topological complex"@en ;
  skos:prefLabel "위상 복합체"@kr ;
.
<http://iso.org/tc211/term/463>
  rdf:type skos:Concept ;
  dcterms:dateAccepted "2003-05-01"^^xsd:date ;
  dcterms:dateAccepted "2009-12-29"^^xsd:date ;
  dcterms:provenance "KS X ISO 19107" ;
  dcterms:source "ISO 19107:2003" ;
  reg:status reg:statusValid ;
  rdfs:comment "Note 1 to entry: The free variables mentioned above can usually be thought of as a local coordinate system. In a 3D coordinate space, a plane can be written as P(u, v) = A + u X + v Y, where u and v are real numbers and A is any point on the plane, and X and Y are two vectors tangent to the plane. Since the locations on the plane can be distinguished by u and v (here universally), the plane is 2D and (u, v) is a coordinate system for the points on the plane. On generic surfaces, this cannot, in general, be done universally. If we take a plane tangent to the surface, and project points on the surface onto this plane, we will normally get a local  isomorphism for small neighbourhoods of the point of tangency. This \"local coordinate\" system for the underlying surface is sufficient to establish the surface as a 2D topological object. Since this International Standard deals only with spatial coordinates, any 3D object can rely on coordinates to establish its topological dimension. In a 4D model (spatio-temporal), tangent spaces also play an important role in establishing topological dimension for objects up to 3D."@en ;
  rdfs:comment "비고: 자유 변수는 일반적으로 지역 좌표계로 여겨질 수 있다. 3차원 좌표공간에서 평면은 P(u,v)=A+uX+vY로 표시될 수 있다. 여기에서 u와 v는 실수이고, A는 평면상의 점이다. X와 Y는 평면에 접하는 두 벡터이다. 평면상의 위치는 u 및 v에 의해 구분할 수 있기 때문에, 평면은 2차원이고, (u,v)는 평면상의 점에 대한 좌표 체계이다. 일반적으로 일반 표면에 대해서는 이와 같이 보편화할 수 없다. 만일 면에 접하는 평면을 취하고, 면 위의 점들을 이 평면에 투영한다면, 명목상 접촉점의 작은 인접군에 대한 지역적 동형을 얻게 된다. 기초 표면에 대한 이 지역 좌표계는 표면을 2차원 위상 객체로 확립하기에 충분하다. KS X ISO 19107 표준은 공간 좌표만을 다루기 때문에, 어떤 3차원 객체도 위상 차원을 만드는 좌표에 사용될 수 있다. 마찬가지로, 4차원 모델(시공간적인)에서 객체 위상 차원을 3차원으로 확립하는 데 있어 접촉 공간이 중요한 역할을 한다."@kr ;
  rdfs:label "topological dimension"@en ;
  skos:changeNote "valid" ;
  skos:definition "기하 객체 내에서 가까운 직접 위치들을 구분하기 위하여 필요한 자유변수의 최소수"@kr ;
  skos:editorialNote "preferred" ;
  skos:editorialNote "preferred"^^xsd:string ;
  skos:notation "463" ;
  skos:notation 463 ;
  skos:note "Note 1 to entry: The free variables mentioned above can usually be thought of as a local coordinate system. In a 3D coordinate space, a plane can be written as P(u, v) = A + u X + v Y, where u and v are real numbers and A is any point on the plane, and X and Y are two vectors tangent to the plane. Since the locations on the plane can be distinguished by u and v (here universally), the plane is 2D and (u, v) is a coordinate system for the points on the plane. On generic surfaces, this cannot, in general, be done universally. If we take a plane tangent to the surface, and project points on the surface onto this plane, we will normally get a local  isomorphism for small neighbourhoods of the point of tangency. This \"local coordinate\" system for the underlying surface is sufficient to establish the surface as a 2D topological object. Since this International Standard deals only with spatial coordinates, any 3D object can rely on coordinates to establish its topological dimension. In a 4D model (spatio-temporal), tangent spaces also play an important role in establishing topological dimension for objects up to 3D."@en ;
  skos:note "비고: 자유 변수는 일반적으로 지역 좌표계로 여겨질 수 있다. 3차원 좌표공간에서 평면은 P(u,v)=A+uX+vY로 표시될 수 있다. 여기에서 u와 v는 실수이고, A는 평면상의 점이다. X와 Y는 평면에 접하는 두 벡터이다. 평면상의 위치는 u 및 v에 의해 구분할 수 있기 때문에, 평면은 2차원이고, (u,v)는 평면상의 점에 대한 좌표 체계이다. 일반적으로 일반 표면에 대해서는 이와 같이 보편화할 수 없다. 만일 면에 접하는 평면을 취하고, 면 위의 점들을 이 평면에 투영한다면, 명목상 접촉점의 작은 인접군에 대한 지역적 동형을 얻게 된다. 기초 표면에 대한 이 지역 좌표계는 표면을 2차원 위상 객체로 확립하기에 충분하다. KS X ISO 19107 표준은 공간 좌표만을 다루기 때문에, 어떤 3차원 객체도 위상 차원을 만드는 좌표에 사용될 수 있다. 마찬가지로, 4차원 모델(시공간적인)에서 객체 위상 차원을 3차원으로 확립하는 데 있어 접촉 공간이 중요한 역할을 한다."@kr ;
  skos:prefLabel "topological dimension"@en ;
  skos:prefLabel "위상 차원"@kr ;
.
<http://iso.org/tc211/term/465>
  rdf:type skos:Concept ;
  dcterms:dateAccepted "2003-05-01"^^xsd:date ;
  dcterms:dateAccepted "2009-12-29"^^xsd:date ;
  dcterms:provenance "KS X ISO 19107" ;
  dcterms:source "ISO 19107:2003" ;
  reg:status reg:statusValid ;
  rdfs:comment "Note 1 to entry: Topological expressions are used for many calculations in computational topology."@en ;
  rdfs:comment "비고: 위상 표현은 계산 위상에서 다수의 연산에 사용된다."@kr ;
  rdfs:label "topological expression"@en ;
  skos:changeNote "valid" ;
  skos:definition "다변량 다항식처럼 연산되는 방향성을 갖는 기하 원시 객체의 모음"@kr ;
  skos:editorialNote "preferred" ;
  skos:editorialNote "preferred"^^xsd:string ;
  skos:notation "465" ;
  skos:notation 465 ;
  skos:note "Note 1 to entry: Topological expressions are used for many calculations in computational topology."@en ;
  skos:note "비고: 위상 표현은 계산 위상에서 다수의 연산에 사용된다."@kr ;
  skos:prefLabel "topological expression"@en ;
  skos:prefLabel "위상 표현"@kr ;
.
<http://iso.org/tc211/term/466>
  rdf:type skos:Concept ;
  dcterms:dateAccepted "2003-05-01"^^xsd:date ;
  dcterms:dateAccepted "2009-12-29"^^xsd:date ;
  dcterms:provenance "KS X ISO 19107" ;
  dcterms:source "ISO 19107:2003" ;
  reg:status reg:statusValid ;
  rdfs:comment "Note 1 to entry: A topological object is a topological primitive, a collection of topological primitives, or a topological complex."@en ;
  rdfs:comment "비고: 위상 객체는 위상 원시 객체, 위상 원시 객체 모음 또는 위상 복합체이다."@kr ;
  rdfs:label "topological object"@en ;
  skos:changeNote "valid" ;
  skos:definition "변형이 계속되어도 변하지 않는 공간적 특성을 나타내는 공간 객체"@kr ;
  skos:editorialNote "preferred" ;
  skos:editorialNote "preferred"^^xsd:string ;
  skos:notation "466" ;
  skos:notation 466 ;
  skos:note "Note 1 to entry: A topological object is a topological primitive, a collection of topological primitives, or a topological complex."@en ;
  skos:note "비고: 위상 객체는 위상 원시 객체, 위상 원시 객체 모음 또는 위상 복합체이다."@kr ;
  skos:prefLabel "topological object"@en ;
  skos:prefLabel "위상 객체"@kr ;
.
<http://iso.org/tc211/term/467>
  rdf:type skos:Concept ;
  dcterms:dateAccepted "2002-09-01"^^xsd:date ;
  dcterms:dateAccepted "2009-12-29"^^xsd:date ;
  dcterms:provenance "ISO 19108;2002" ;
  dcterms:provenance "KS X ISO 19107" ;
  dcterms:source "ISO 19107:2003" ;
  reg:status reg:statusValid ;
  rdfs:comment "Note 1 to entry: A topological primitive corresponds to the interior of a geometric primitive of the same dimension in a geometric realization."@en ;
  rdfs:comment "비고: 위상 원시 객체는 기하 실현에서 동일한 차원의 기하 원시 객체의 내부와 일치한다."@kr ;
  rdfs:label "topological primitive"@en ;
  skos:changeNote "valid" ;
  skos:definition "분해할 수 없는 하나의 요소를 표현하는 위상 객체"@kr ;
  skos:editorialNote "preferred" ;
  skos:editorialNote "preferred"^^xsd:string ;
  skos:notation "467" ;
  skos:notation 467 ;
  skos:note "Note 1 to entry: A topological primitive corresponds to the interior of a geometric primitive of the same dimension in a geometric realization."@en ;
  skos:note "비고: 위상 원시 객체는 기하 실현에서 동일한 차원의 기하 원시 객체의 내부와 일치한다."@kr ;
  skos:prefLabel "topological primitive"@en ;
  skos:prefLabel "위상 원시 객체"@kr ;
.
<http://iso.org/tc211/term/468>
  rdf:type skos:Concept ;
  dcterms:dateAccepted "2003-05-01"^^xsd:date ;
  dcterms:dateAccepted "2009-12-29"^^xsd:date ;
  dcterms:provenance "KS X ISO 19107" ;
  dcterms:source "ISO 19107:2003" ;
  reg:status reg:statusValid ;
  rdfs:comment "Note 1 to entry: The boundary of a topological solid consists of a set of directed faces."@en ;
  rdfs:comment "비고: 위상 입방체의 경계는 방향성 면의 집합으로 이루어진다."@kr ;
  rdfs:label "topological solid"@en ;
  skos:changeNote "valid" ;
  skos:definition "3차원의 위상 원시 객체"@kr ;
  skos:editorialNote "preferred" ;
  skos:editorialNote "preferred"^^xsd:string ;
  skos:notation "468" ;
  skos:notation 468 ;
  skos:note "Note 1 to entry: The boundary of a topological solid consists of a set of directed faces."@en ;
  skos:note "비고: 위상 입방체의 경계는 방향성 면의 집합으로 이루어진다."@kr ;
  skos:prefLabel "topological solid"@en ;
  skos:prefLabel "위상 입방체"@kr ;
.
<http://iso.org/tc211/term/47>
  rdf:type skos:Concept ;
  dcterms:dateAccepted "2007-10-15"^^xsd:date ;
  dcterms:dateAccepted "2009-12-29"^^xsd:date ;
  dcterms:provenance "KS X ISO 19132" ;
  dcterms:source "ISO 19132:2007" ;
  reg:status reg:statusValid ;
  rdfs:label "cluster"@en ;
  skos:changeNote "valid" ;
  skos:definition "그 위치가 소규모 인접군 지역 내에 존재하는 잠재적으로 이질적인(서로 다른 질의 기준을 만족할 수 있는) 대상들의 모음"@kr ;
  skos:editorialNote "preferred" ;
  skos:editorialNote "preferred"^^xsd:string ;
  skos:notation "47" ;
  skos:notation 47 ;
  skos:prefLabel "cluster"@en ;
  skos:prefLabel "클러스터"@kr ;
.
<http://iso.org/tc211/term/470>
  rdf:type skos:Concept ;
  dcterms:dateAccepted "2005-10-15"^^xsd:date ;
  dcterms:dateAccepted "2006-12-01"^^xsd:date ;
  dcterms:provenance "KS X ISO 19133" ;
  dcterms:source "ISO 19133:2005" ;
  reg:status reg:statusValid ;
  rdfs:label "tracking"@en ;
  skos:changeNote "valid" ;
  skos:definition "차량의 위치에 대한 모니터링 및 보고"@kr ;
  skos:editorialNote "preferred" ;
  skos:editorialNote "preferred"^^xsd:string ;
  skos:notation "470" ;
  skos:notation 470 ;
  skos:prefLabel "tracking"@en ;
  skos:prefLabel "추적"@kr ;
.
<http://iso.org/tc211/term/471>
  rdf:type skos:Concept ;
  dcterms:dateAccepted "2002-09-01"^^xsd:date ;
  dcterms:dateAccepted "2008-12-19"^^xsd:date ;
  dcterms:provenance "ISO 19108;2002" ;
  dcterms:provenance "KS X ISO 19104" ;
  dcterms:source "Jensen et al. (1994)" ;
  reg:status reg:statusValid ;
  rdfs:label "transaction time"@en ;
  skos:changeNote "valid" ;
  skos:definition "한 정보가 데이터 베이스 내에 현존하며, 수정될 수 있는 시간"@kr ;
  skos:editorialNote "preferred" ;
  skos:editorialNote "preferred"^^xsd:string ;
  skos:notation "471" ;
  skos:notation 471 ;
  skos:prefLabel "transaction time"@en ;
  skos:prefLabel "처리 시간"@kr ;
.
<http://iso.org/tc211/term/473>
  rdf:type skos:Concept ;
  dcterms:dateAccepted "2005-07-15"^^xsd:date ;
  dcterms:dateAccepted "2008-12-30"^^xsd:date ;
  dcterms:provenance "ISO 19118:2005" ;
  dcterms:source "ISO 19118:2011, 4.31" ;
  reg:status reg:statusValid ;
  rdfs:label "transfer protocol"@en ;
  skos:changeNote "valid" ;
  skos:definition "분산 시스템 간의 상호 작용을 정의하기 위한 규칙의 공통 집합"@kr ;
  skos:editorialNote "preferred" ;
  skos:editorialNote "preferred"^^xsd:string ;
  skos:notation "473" ;
  skos:notation 473 ;
  skos:prefLabel "transfer protocol"@en ;
  skos:prefLabel "전송 프로토콜"@kr ;
.
<http://iso.org/tc211/term/474>
  rdf:type skos:Concept ;
  dcterms:dateAccepted "2005-10-15"^^xsd:date ;
  dcterms:dateAccepted "2006-12-01"^^xsd:date ;
  dcterms:provenance "KS X ISO 19133" ;
  dcterms:source "ISO 19133:2005" ;
  reg:status reg:statusValid ;
  rdfs:comment "Note 1 to entry: Traversability is usually a function of physical, cultural, or legal conditions. If traversable is false, then the object cannot be navigated. This effectively removes a link from the usable network. In the case of a node, it effectively removes the node and all associated links from the useable network. In the case of a turn, it simply removes it from any viable route.  Non-traversable entities are not included in maneuvers or routes."@en ;
  rdfs:comment "비고: 운행 가능성은 보통 하나의 물리적, 문화적, 법률적 조건 함수이다. 만약 운행 가능성이 거짓일 경우라면, 객체를 내비게이션할 수 없다. 이는 효과적 네트워크로부터 링크를 제거한다. 절점의 경우에는, 효과적으로 사용가능한 네트워크로부터 절점과 모든 연관된 링크를 제거한다. 회전의 경우에는, 단순히 어떠한 실행 가능 경로에서 이를 제거한다. 운행할 수 없는 개체는 기동이나 경로에 포함될 수 없다."@kr ;
  rdfs:label "traversable"@en ;
  skos:changeNote "valid" ;
  skos:definition "보다 상세한 내비게이션 제약 조건과 반대의 개념으로, 모든 교통 운행을 허용하거나 제약하는 링크나 회전의 조건  "@kr ;
  skos:editorialNote "preferred" ;
  skos:editorialNote "preferred"^^xsd:string ;
  skos:notation "474" ;
  skos:notation 474 ;
  skos:note "Note 1 to entry: Traversability is usually a function of physical, cultural, or legal conditions. If traversable is false, then the object cannot be navigated. This effectively removes a link from the usable network. In the case of a node, it effectively removes the node and all associated links from the useable network. In the case of a turn, it simply removes it from any viable route.  Non-traversable entities are not included in maneuvers or routes."@en ;
  skos:note "비고: 운행 가능성은 보통 하나의 물리적, 문화적, 법률적 조건 함수이다. 만약 운행 가능성이 거짓일 경우라면, 객체를 내비게이션할 수 없다. 이는 효과적 네트워크로부터 링크를 제거한다. 절점의 경우에는, 효과적으로 사용가능한 네트워크로부터 절점과 모든 연관된 링크를 제거한다. 회전의 경우에는, 단순히 어떠한 실행 가능 경로에서 이를 제거한다. 운행할 수 없는 개체는 기동이나 경로에 포함될 수 없다."@kr ;
  skos:prefLabel "traversable"@en ;
  skos:prefLabel "운행 가능성"@kr ;
.
<http://iso.org/tc211/term/475>
  rdf:type skos:Concept ;
  dcterms:dateAccepted "2009-04-01"^^xsd:date ;
  dcterms:source "ISO/TS 19129:2009" ;
  reg:status reg:statusValid ;
  rdfs:label "traversal order"@en ;
  skos:changeNote "valid" ;
  skos:editorialNote "preferred"^^xsd:string ;
  skos:notation 475 ;
  skos:prefLabel "traversal order"@en ;
.
<http://iso.org/tc211/term/476>
  rdf:type skos:Concept ;
  dcterms:dateAccepted "2005-08-15"^^xsd:date ;
  dcterms:dateAccepted "2007-11-01"^^xsd:date ;
  dcterms:provenance "KS X ISO 19123" ;
  dcterms:source "ISO 19123:2005" ;
  reg:status reg:statusValid ;
  rdfs:label "triangulated irregular network"@en ;
  skos:changeNote "valid" ;
  skos:definition "삼각형으로 구성된 공간 분할"@kr ;
  skos:editorialNote "preferred" ;
  skos:editorialNote "preferred"^^xsd:string ;
  skos:notation "476" ;
  skos:notation 476 ;
  skos:prefLabel "triangulated irregular network"@en ;
  skos:prefLabel "불규칙 삼각망"@kr ;
.
<http://iso.org/tc211/term/477>
  rdf:type skos:Concept ;
  dcterms:dateAccepted "2007-07-01"^^xsd:date ;
  dcterms:dateAccepted "2009-12-29"^^xsd:date ;
  dcterms:provenance "ISO 19111:2007" ;
  dcterms:provenance "KS X ISO 19136" ;
  dcterms:source "ISO 19136:2007" ;
  reg:status reg:statusValid ;
  rdfs:comment "Note 1 to entry: The number of values in a tuple is immutable"@en ;
  rdfs:comment "비고: 튜플에서의 숫자 값은 불변이다."@kr ;
  rdfs:label "tuple"@en ;
  skos:changeNote "valid" ;
  skos:definition "값의 순서화된 목록"@kr ;
  skos:editorialNote "preferred" ;
  skos:editorialNote "preferred"^^xsd:string ;
  skos:notation "477" ;
  skos:notation 477 ;
  skos:note "Note 1 to entry: The number of values in a tuple is immutable"@en ;
  skos:note "비고: 튜플에서의 숫자 값은 불변이다."@kr ;
  skos:prefLabel "tuple"@en ;
  skos:prefLabel "튜플"@kr ;
.
<http://iso.org/tc211/term/478>
  rdf:type skos:Concept ;
  dcterms:dateAccepted "2005-10-15"^^xsd:date ;
  dcterms:dateAccepted "2006-12-01"^^xsd:date ;
  dcterms:provenance "KS X ISO 19133" ;
  dcterms:source "ISO 19133:2005" ;
  reg:status reg:statusValid ;
  rdfs:label "turn"@en ;
  skos:changeNote "valid" ;
  skos:definition "교차점 위치와 그 교차점을 위한 입구 및 출구 링크를 구성하고 있는 경로 또는 네트워크의 일부분"@kr ;
  skos:editorialNote "preferred" ;
  skos:editorialNote "preferred"^^xsd:string ;
  skos:notation "478" ;
  skos:notation 478 ;
  skos:prefLabel "turn"@en ;
  skos:prefLabel "회전"@kr ;
.
<http://iso.org/tc211/term/48>
  rdf:type skos:Concept ;
  dcterms:dateAccepted "2003-05-01"^^xsd:date ;
  dcterms:dateAccepted "2009-12-29"^^xsd:date ;
  dcterms:provenance "KS X ISO 19107" ;
  dcterms:source "ISO 19107:2003" ;
  reg:status reg:statusValid ;
  rdfs:comment "Note 1 to entry: If a node is on the boundary of an edge, that edge is on the coboundary of that node. Any orientation parameter associated to one of these relations would also be associated to the other. So that if the node is the end node of the edge (defined as the end of the positive directed edge), then the positive orientation of the node (defined as the positive directed node) would have the edge on its coboundary, see ISO 19107 Figure 35."@en ;
  rdfs:comment "비고: 만약 절점이 변의 경계에 위치한다면, 변은 절점의 공유 경계에 위치한다. 이러한 관계를 갖는 하나의 방향 매개 변수는 또한 반대의 경우와도 연관된다. 절점이 (양의 방향성 변의 끝으로 정의된) 변의 끝 절점이라면, (양의 방향성 절점으로 정의된) 절점의 양의 방향이 그 공유 경계상의 변을 가질 수 있다(KS X ISO 19107 그림35 참조). "@kr ;
  rdfs:label "coboundary"@en ;
  skos:changeNote "valid" ;
  skos:definition "특정 위상 객체를 구성하는 높은 위상 차원의 위상 원시 객체 집합으로, 이 위상 객체는 위상 원시 객체의 각 경계에 존재함"@kr ;
  skos:editorialNote "preferred" ;
  skos:editorialNote "preferred"^^xsd:string ;
  skos:notation "48" ;
  skos:notation 48 ;
  skos:note "Note 1 to entry: If a node is on the boundary of an edge, that edge is on the coboundary of that node. Any orientation parameter associated to one of these relations would also be associated to the other. So that if the node is the end node of the edge (defined as the end of the positive directed edge), then the positive orientation of the node (defined as the positive directed node) would have the edge on its coboundary, see ISO 19107 Figure 35."@en ;
  skos:note "비고: 만약 절점이 변의 경계에 위치한다면, 변은 절점의 공유 경계에 위치한다. 이러한 관계를 갖는 하나의 방향 매개 변수는 또한 반대의 경우와도 연관된다. 절점이 (양의 방향성 변의 끝으로 정의된) 변의 끝 절점이라면, (양의 방향성 절점으로 정의된) 절점의 양의 방향이 그 공유 경계상의 변을 가질 수 있다(KS X ISO 19107 그림35 참조). "@kr ;
  skos:prefLabel "coboundary"@en ;
  skos:prefLabel "공유 경계"@kr ;
.
<http://iso.org/tc211/term/480>
  rdf:type skos:Concept ;
  dcterms:dateAccepted "2004-07-01"^^xsd:date ;
  dcterms:dateAccepted "2008-12-19"^^xsd:date ;
  dcterms:provenance "ISO 19116:2004" ;
  dcterms:provenance "KS X ISO 19104" ;
  dcterms:source "Guide to the Expression of Uncertainty in Measurement (GUM), 1995" ;
  reg:status reg:statusValid ;
  rdfs:comment "Note 1 to entry: When the quality of accuracy or precision of measured values, such as coordinates, is to be characterized quantitatively, the quality parameter is an estimate of the uncertainty of the measurement results. Because accuracy is a qualitative concept, one should not use it quantitatively, that is associate numbers with it; numbers should be associated with measures of uncertainty instead."@en ;
  rdfs:comment "비고: 좌표와 같은 측정값의 정밀도와 정확도의 품질이 정량적 특성을 지닐 때, 품질 매개 변수는 측정 결과 불확실성의 하나의 추정치이다. 정확도는 정성적인 개념이기 때문에, 이를 정량적으로 사용해서는 안 된다. 즉, 불확실성을 가진 연관수이다. 대신 그 수는 불확실성의 측정과 연관되어야 한다. "@kr ;
  rdfs:label "uncertainty"@en ;
  skos:changeNote "valid" ;
  skos:definition "측정 결과와 관련, 측정량을 합리적으로 속성화할 수 있는 특징적인 분산 값을 나타내는 매개 변수"@kr ;
  skos:editorialNote "preferred" ;
  skos:editorialNote "preferred"^^xsd:string ;
  skos:notation "480" ;
  skos:notation 480 ;
  skos:note "Note 1 to entry: When the quality of accuracy or precision of measured values, such as coordinates, is to be characterized quantitatively, the quality parameter is an estimate of the uncertainty of the measurement results. Because accuracy is a qualitative concept, one should not use it quantitatively, that is associate numbers with it; numbers should be associated with measures of uncertainty instead."@en ;
  skos:note "비고: 좌표와 같은 측정값의 정밀도와 정확도의 품질이 정량적 특성을 지닐 때, 품질 매개 변수는 측정 결과 불확실성의 하나의 추정치이다. 정확도는 정성적인 개념이기 때문에, 이를 정량적으로 사용해서는 안 된다. 즉, 불확실성을 가진 연관수이다. 대신 그 수는 불확실성의 측정과 연관되어야 한다. "@kr ;
  skos:prefLabel "uncertainty"@en ;
  skos:prefLabel "불확실성"@kr ;
.
<http://iso.org/tc211/term/481>
  rdf:type skos:Concept ;
  dcterms:dateAccepted "2007-09-01"^^xsd:date ;
  dcterms:dateAccepted "2009-12-29"^^xsd:date ;
  dcterms:provenance "KS X ISO 19136" ;
  dcterms:source "ISO 19136:2007" ;
  reg:status reg:statusValid ;
  rdfs:comment "Note 1 to entry: The general syntax is <scheme>::<scheme-specific-part>. The hierarchical syntax with a namespace is <scheme>://<authority><path>?<query> - see RFC 2396."@en ;
  rdfs:comment "비고: 일반적인 문법은 <scheme>::<scheme-specific-part>이다. 이름 공간과 함께 계층적 문법은 <scheme>://<authority><path>?<query>이다. RFC 2396을 참고하라."@kr ;
  rdfs:label "Uniform Resource Identifier"@en ;
  skos:altLabel "URI"@kr ;
  skos:altLabel "URI"^^<http://www.w3.org/2001/XMLSchema#@en> ;
  skos:changeNote "valid" ;
  skos:definition "IETF RFC 2396에 대한 적합성을 만족하는, 자원에 대한 고유한 식별자"@kr ;
  skos:editorialNote "preferred" ;
  skos:editorialNote "preferred"^^xsd:string ;
  skos:notation "481" ;
  skos:notation 481 ;
  skos:note "Note 1 to entry: The general syntax is <scheme>::<scheme-specific-part>. The hierarchical syntax with a namespace is <scheme>://<authority><path>?<query> - see RFC 2396."@en ;
  skos:note "비고: 일반적인 문법은 <scheme>::<scheme-specific-part>이다. 이름 공간과 함께 계층적 문법은 <scheme>://<authority><path>?<query>이다. RFC 2396을 참고하라."@kr ;
  skos:prefLabel "URI"@kr ;
  skos:prefLabel "Uniform Resource Identifier"@en ;
.
<http://iso.org/tc211/term/483>
  rdf:type skos:Concept ;
  dcterms:dateAccepted "2004-07-01"^^xsd:date ;
  dcterms:dateAccepted "2008-12-30"^^xsd:date ;
  dcterms:provenance "ISO 19116:2004" ;
  dcterms:provenance "KS X ISO 19116" ;
  dcterms:source "ISO 31-0:1992, 2.1 (Adapted from)" ;
  reg:status reg:statusValid ;
  rdfs:comment "Note 1 to entry: In positioning services, the usual units of measurement are either angular units or linear units.  Implementations of positioning services must clearly distinguish between SI units and non-SI units.  When non-SI units are employed, it is requird that their relation to SI units be specified."@en ;
  rdfs:comment "비고: 측위 서비스에서 측정 단위는 각 단위 또는 선형 단위이다. 측위 서비스의 구현에서는 국제 표준 단위를 사용하는지, 사용하지 않는지를 명확하게 구분해야 한다. 국제 표준 단위를 사용하지 않는 경우는 국제 표준 단위와의 관계를 명시해야 한다. "@kr ;
  rdfs:label "unit of measure"@en ;
  skos:changeNote "valid" ;
  skos:definition "단위 등가 집단으로부터 선택된 참조 양"@kr ;
  skos:editorialNote "preferred" ;
  skos:editorialNote "preferred"^^xsd:string ;
  skos:notation "483" ;
  skos:notation 483 ;
  skos:note "Note 1 to entry: In positioning services, the usual units of measurement are either angular units or linear units.  Implementations of positioning services must clearly distinguish between SI units and non-SI units.  When non-SI units are employed, it is requird that their relation to SI units be specified."@en ;
  skos:note "비고: 측위 서비스에서 측정 단위는 각 단위 또는 선형 단위이다. 측위 서비스의 구현에서는 국제 표준 단위를 사용하는지, 사용하지 않는지를 명확하게 구분해야 한다. 국제 표준 단위를 사용하지 않는 경우는 국제 표준 단위와의 관계를 명시해야 한다. "@kr ;
  skos:prefLabel "unit of measure"@en ;
  skos:prefLabel "측정단위"@kr ;
.
<http://iso.org/tc211/term/484>
  rdf:type skos:Concept ;
  dcterms:dateAccepted "2003-05-01"^^xsd:date ;
  dcterms:dateAccepted "2009-12-29"^^xsd:date ;
  dcterms:provenance "KS X ISO 19107" ;
  dcterms:source "ISO 19107:2003" ;
  reg:status reg:statusValid ;
  rdfs:comment "Note 1 to entry: The universal face is normally not part of any feature, and is used to represent the unbounded portion of the data set. Its interior boundary (it has no exterior boundary) would normally be considered the exterior boundary of the map represented by the data set. This International Standard does not special case the universal face, but application schemas may find it convenient to do so."@en ;
  rdfs:comment "비고: 보통 무한 면은 특정 피처의 일부분이 아니며, 데이터 집합의 경계가 없는 부분의 표현에 사용된다. 무한 면의 내부 경계(무한 면은 외부 경계를 갖지 않는다.)는 통상적으로 데이터 집합을 통해 표현된 지도의 외부 경계로 간주될 수 있다. KS X ISO 19107은 무한 면의 특정 사례를 다루지 않지만, 응용 스키마에서는 편의를 위해 무한 면의 특정 사례를 다룰 수 있다. "@kr ;
  rdfs:label "universal face"@en ;
  skos:changeNote "valid" ;
  skos:definition "경계가 없는 2차원 복합체 면"@kr ;
  skos:editorialNote "preferred" ;
  skos:editorialNote "preferred"^^xsd:string ;
  skos:notation "484" ;
  skos:notation 484 ;
  skos:note "Note 1 to entry: The universal face is normally not part of any feature, and is used to represent the unbounded portion of the data set. Its interior boundary (it has no exterior boundary) would normally be considered the exterior boundary of the map represented by the data set. This International Standard does not special case the universal face, but application schemas may find it convenient to do so."@en ;
  skos:note "비고: 보통 무한 면은 특정 피처의 일부분이 아니며, 데이터 집합의 경계가 없는 부분의 표현에 사용된다. 무한 면의 내부 경계(무한 면은 외부 경계를 갖지 않는다.)는 통상적으로 데이터 집합을 통해 표현된 지도의 외부 경계로 간주될 수 있다. KS X ISO 19107은 무한 면의 특정 사례를 다루지 않지만, 응용 스키마에서는 편의를 위해 무한 면의 특정 사례를 다룰 수 있다. "@kr ;
  skos:prefLabel "universal face"@en ;
  skos:prefLabel "무한 면"@kr ;
.
<http://iso.org/tc211/term/485>
  rdf:type skos:Concept ;
  dcterms:dateAccepted "2003-05-01"^^xsd:date ;
  dcterms:dateAccepted "2009-12-29"^^xsd:date ;
  dcterms:provenance "KS X ISO 19107" ;
  dcterms:source "ISO 19107:2003" ;
  reg:status reg:statusValid ;
  rdfs:comment "Note 1 to entry: The universal solid is the 3-dimensional counterpart of the universal face, and is also normally not part of any feature."@en ;
  rdfs:comment "비고: 무한 입방체는 무한 면의 3차원의 대응물이며, 또한 통상적으로 피처의 부분이 아니다."@kr ;
  rdfs:label "universal solid"@en ;
  skos:changeNote "valid" ;
  skos:definition "경계가 없는 3차원 복합체 위상 입방체"@kr ;
  skos:editorialNote "preferred" ;
  skos:editorialNote "preferred"^^xsd:string ;
  skos:notation "485" ;
  skos:notation 485 ;
  skos:note "Note 1 to entry: The universal solid is the 3-dimensional counterpart of the universal face, and is also normally not part of any feature."@en ;
  skos:note "비고: 무한 입방체는 무한 면의 3차원의 대응물이며, 또한 통상적으로 피처의 부분이 아니다."@kr ;
  skos:prefLabel "universal solid"@en ;
  skos:prefLabel "무한 입방체"@kr ;
.
<http://iso.org/tc211/term/486>
  rdf:type skos:Concept ;
  dcterms:dateAccepted "2002-07-01" ;
  dcterms:dateAccepted "2002-07-01"^^xsd:date ;
  dcterms:dateAccepted "2008-12-30"^^xsd:date ;
  dcterms:provenance "ISO 19101:2002" ;
  dcterms:source "ISO 19101-1:2014, 4.1.38" ;
  reg:status reg:statusAccepted ;
  reg:status reg:statusValid ;
  rdfs:label "universe of discourse"@en ;
  rdfs:seeAlso "beschouwingsgebied"@nl ;
  skos:altLabel "beschouwingsgebied"@nl ;
  skos:changeNote "valid" ;
  skos:definition "beeld van de echte of hypothetische wereld dat binnen de context van een domein alles van belang omvat"@nl ;
  skos:definition "모든 관심 있는 것을 포함하는 실세계나 가상 세계에 대한 견해"@kr ;
  skos:editorialNote "preferred" ;
  skos:editorialNote "preferred"^^xsd:string ;
  skos:notation "486" ;
  skos:notation 486 ;
  skos:prefLabel "universe of discourse"@en ;
  skos:prefLabel "werkelijkheid"@nl ;
  skos:prefLabel "논의의 영역"@kr ;
.
<http://iso.org/tc211/term/487>
  rdf:type skos:Concept ;
  dcterms:dateAccepted "2002-09-01"^^xsd:date ;
  dcterms:dateAccepted "2008-12-19"^^xsd:date ;
  dcterms:provenance "ISO 19108;2002" ;
  dcterms:provenance "KS X ISO 19104" ;
  dcterms:source "Jensen et al. (1994)" ;
  reg:status reg:statusValid ;
  rdfs:label "valid time"@en ;
  skos:changeNote "valid" ;
  skos:definition "한 정보가 추상화된 현실 속에서 \"참\"이 되는 시간"@kr ;
  skos:editorialNote "preferred" ;
  skos:editorialNote "preferred"^^xsd:string ;
  skos:notation "487" ;
  skos:notation 487 ;
  skos:prefLabel "valid time"@en ;
  skos:prefLabel "유효시간"@kr ;
.
<http://iso.org/tc211/term/489>
  rdf:type skos:Concept ;
  dcterms:dateAccepted "2005-07-15" ;
  dcterms:dateAccepted "2005-07-15"^^xsd:date ;
  dcterms:dateAccepted "2009-12-29"^^xsd:date ;
  dcterms:provenance "ISO/TS 19103:2005" ;
  dcterms:provenance "KS X ISO 19103" ;
  dcterms:source "ISO/IEC 19501:2005 (Adapted from)" ;
  reg:status reg:statusAccepted ;
  reg:status reg:statusValid ;
  rdfs:comment "NOTE 1 A value may consider a possible state of an object within a class or type (domain)."@en ;
  rdfs:comment "NOTE 2 A data value is an instance of a data type, a value without identity"@en ;
  rdfs:comment "Note 1 to entry: A value may consider a possible state of an object within a class or type (domain)."@en ;
  rdfs:comment "Note 2 to entry: A data value is an instance of a data type, a value without identity" ;
  rdfs:comment "비고 1: 값은 클래스 또는 유형(영역) 내에서 객체가 가질 수 있는 상태의 표현일 수 있다."@kr ;
  rdfs:label "value <UML>"@en ;
  skos:changeNote "valid" ;
  skos:definition "element van het type domein"@nl ;
  skos:definition "유형 영역의 요소"@kr ;
  skos:editorialNote "preferred" ;
  skos:editorialNote "preferred"^^xsd:string ;
  skos:notation "489" ;
  skos:notation 489 ;
  skos:note "NOTE 1 A value may consider a possible state of an object within a class or type (domain)."@en ;
  skos:note "NOTE 2 A data value is an instance of a data type, a value without identity"^^<http://www.w3.org/2001/XMLSchema#@en> ;
  skos:note "Note 1 to entry: A value may consider a possible state of an object within a class or type (domain)."@en ;
  skos:note "Note 2 to entry: A data value is an instance of a data type, a value without identity"^^<http://www.w3.org/2001/XMLSchema#@en> ;
  skos:note "비고 1: 값은 클래스 또는 유형(영역) 내에서 객체가 가질 수 있는 상태의 표현일 수 있다."@kr ;
  skos:note "비고 2: 데이터 값은 데이터 유형의 인스턴스이며, 그 값은 식별특성을 갖지 않는다."@kr ;
  skos:prefLabel "value <UML>"@en ;
  skos:prefLabel "value <UML>"@nl ;
  skos:prefLabel "값 <UML>"@kr ;
.
<http://iso.org/tc211/term/49>
  rdf:type skos:Concept ;
  dcterms:dateAccepted "2005-07-15"^^xsd:date ;
  dcterms:dateAccepted "2008-12-30"^^xsd:date ;
  dcterms:provenance "ISO 19118:2005" ;
  dcterms:source "ISO 19118:2011, 4.3" ;
  reg:status reg:statusValid ;
  rdfs:label "code"@en ;
  skos:changeNote "valid" ;
  skos:definition "특정한 형식에 따른 라벨의 표현"@kr ;
  skos:editorialNote "preferred" ;
  skos:editorialNote "preferred"^^xsd:string ;
  skos:notation "49" ;
  skos:notation 49 ;
  skos:prefLabel "code"@en ;
  skos:prefLabel "코드"@kr ;
.
<http://iso.org/tc211/term/490>
  rdf:type skos:Concept ;
  dcterms:dateAccepted "2005-07-15" ;
  dcterms:dateAccepted "2005-07-15"^^xsd:date ;
  dcterms:dateAccepted "2009-12-29"^^xsd:date ;
  dcterms:provenance "KS X ISO 19103" ;
  dcterms:source "ISO/TS 19103:2005" ;
  reg:status reg:statusAccepted ;
  reg:status reg:statusValid ;
  rdfs:label "value domain"@en ;
  skos:changeNote "valid" ;
  skos:definition "verzameling van afgesproken waarden"@nl ;
  skos:definition "수용된 값의 집합"@kr ;
  skos:editorialNote "preferred" ;
  skos:editorialNote "preferred"^^xsd:string ;
  skos:notation "490" ;
  skos:notation 490 ;
  skos:prefLabel "value domain"@en ;
  skos:prefLabel "value domain"@nl ;
  skos:prefLabel "값 영역"@kr ;
.
<http://iso.org/tc211/term/491>
  rdf:type skos:Concept ;
  dcterms:dateAccepted "2005-08-15"^^xsd:date ;
  dcterms:dateAccepted "2007-11-01"^^xsd:date ;
  dcterms:provenance "KS X ISO 19123" ;
  dcterms:source "ISO 19123:2005" ;
  reg:status reg:statusValid ;
  rdfs:comment "Note 1 to entry: A directed line segment represents a vector if the length and direction of the line segment are equal to the magnitude and direction of the vector.  The term vector data refers to data that represents the spatial configuration of features as a set of directed line segments."@en ;
  rdfs:comment "비고: 선 조각의 길이 및 방향이 벡터의 크기 및 방향과 같다면, 방향성 선 조각은 벡터를 표현한다. 벡터 데이터라는 용어는 피처의 공간 구성을 방향성 선 조각의 집합으로 표현하는 데이터를 의미한다."@kr ;
  rdfs:label "vector"@en ;
  skos:changeNote "valid" ;
  skos:definition "크기와 방향을 함께 갖는 양"@kr ;
  skos:editorialNote "preferred" ;
  skos:editorialNote "preferred"^^xsd:string ;
  skos:notation "491" ;
  skos:notation 491 ;
  skos:note "Note 1 to entry: A directed line segment represents a vector if the length and direction of the line segment are equal to the magnitude and direction of the vector.  The term vector data refers to data that represents the spatial configuration of features as a set of directed line segments."@en ;
  skos:note "비고: 선 조각의 길이 및 방향이 벡터의 크기 및 방향과 같다면, 방향성 선 조각은 벡터를 표현한다. 벡터 데이터라는 용어는 피처의 공간 구성을 방향성 선 조각의 집합으로 표현하는 데이터를 의미한다."@kr ;
  skos:prefLabel "vector"@en ;
  skos:prefLabel "벡터"@kr ;
.
<http://iso.org/tc211/term/492>
  rdf:type skos:Concept ;
  dcterms:dateAccepted "2003-05-01"^^xsd:date ;
  dcterms:dateAccepted "2009-12-29"^^xsd:date ;
  dcterms:provenance "KS X ISO 19107" ;
  dcterms:source "ISO 19107:2003" ;
  reg:status reg:statusValid ;
  rdfs:label "vector geometry"@en ;
  skos:changeNote "valid" ;
  skos:definition "구조적 기하 원시 객체를 사용하여 만들어진 기하의 표현"@kr ;
  skos:editorialNote "preferred" ;
  skos:editorialNote "preferred"^^xsd:string ;
  skos:notation "492" ;
  skos:notation 492 ;
  skos:prefLabel "vector geometry"@en ;
  skos:prefLabel "벡터 기하"@kr ;
.
<http://iso.org/tc211/term/493>
  rdf:type skos:Concept ;
  dcterms:dateAccepted "2005-10-15"^^xsd:date ;
  dcterms:dateAccepted "2006-12-01"^^xsd:date ;
  dcterms:provenance "KS X ISO 19133" ;
  dcterms:source "ISO 19133:2005" ;
  reg:status reg:statusValid ;
  rdfs:comment "Note 1 to entry:: Classifications based on construction include automobile, truck, bus, bicycle, etc. Classifications based on purpose include taxi, emergency vehicle, etc. Vehicle classification can be used to determine the application of navigation constraints."@en ;
  rdfs:comment "비고: 구조를 바탕으로 한 분류로는 자동차, 트럭, 버스, 자전거 등이 있다. 목적을 바탕으로 한 분류에는 택시, 응급차량 등이 있다. 차종은 내비게이션  제약 조건을 고려한 응용의 결정에 사용될 수 있다."@kr ;
  rdfs:label "vehicle classification"@en ;
  skos:changeNote "valid" ;
  skos:definition "의도된 목적 또는 구조 특성을 바탕으로한 차량의 유형"@kr ;
  skos:editorialNote "preferred" ;
  skos:editorialNote "preferred"^^xsd:string ;
  skos:notation "493" ;
  skos:notation 493 ;
  skos:note "Note 1 to entry:: Classifications based on construction include automobile, truck, bus, bicycle, etc. Classifications based on purpose include taxi, emergency vehicle, etc. Vehicle classification can be used to determine the application of navigation constraints."@en ;
  skos:note "비고: 구조를 바탕으로 한 분류로는 자동차, 트럭, 버스, 자전거 등이 있다. 목적을 바탕으로 한 분류에는 택시, 응급차량 등이 있다. 차종은 내비게이션  제약 조건을 고려한 응용의 결정에 사용될 수 있다."@kr ;
  skos:prefLabel "vehicle classification"@en ;
  skos:prefLabel "차종"@kr ;
.
<http://iso.org/tc211/term/495>
  rdf:type skos:Concept ;
  dcterms:dateAccepted "2000-12-15"^^xsd:date ;
  dcterms:dateAccepted "2007-06-29"^^xsd:date ;
  dcterms:provenance "KS X ISO 19105" ;
  dcterms:source "ISO 19105:2000" ;
  reg:status reg:statusValid ;
  rdfs:label "verification test"@en ;
  skos:changeNote "valid" ;
  skos:definition "시험 대상(IUT)이 올바른지에 대한 엄격한 증명을 위해 개발된 시험"@kr ;
  skos:editorialNote "preferred" ;
  skos:editorialNote "preferred"^^xsd:string ;
  skos:notation "495" ;
  skos:notation 495 ;
  skos:prefLabel "verification test"@en ;
  skos:prefLabel "검증 시험"@kr ;
.
<http://iso.org/tc211/term/497>
  rdf:type skos:Concept ;
  dcterms:dateAccepted "2005-02-15"^^xsd:date ;
  dcterms:dateAccepted "2006-12-29"^^xsd:date ;
  dcterms:provenance "ISO 19119:2005" ;
  dcterms:provenance "KS X ISO/IEC 10746-2" ;
  dcterms:source "ISO/IEC 10746-2:1996" ;
  reg:status reg:statusValid ;
  rdfs:label "viewpoint (on a system)"@en ;
  skos:changeNote "valid" ;
  skos:definition "시스템의 특정 목적에 대한 집중을 위해 선택된 구조적 개념 및 구조화 규칙의 집합을 사용하는 추상화의 형태"@kr ;
  skos:editorialNote "preferred" ;
  skos:editorialNote "preferred"^^xsd:string ;
  skos:notation "497" ;
  skos:notation 497 ;
  skos:prefLabel "viewpoint (on a system)"@en ;
  skos:prefLabel "관점 <시스템>"@kr ;
.
<http://iso.org/tc211/term/498>
  rdf:type skos:Concept ;
  dcterms:dateAccepted "2005-10-15"^^xsd:date ;
  dcterms:dateAccepted "2006-12-01"^^xsd:date ;
  dcterms:provenance "KS X ISO 19133" ;
  dcterms:source "ISO 19133:2005" ;
  reg:status reg:statusValid ;
  rdfs:label "waypoint"@en ;
  skos:changeNote "valid" ;
  skos:definition "요청된 라우팅을 잠정적으로 만족시키는, 후보 경로의 선택 역할을 담당하는 네트워크상 위치"@kr ;
  skos:editorialNote "preferred" ;
  skos:editorialNote "preferred"^^xsd:string ;
  skos:notation "498" ;
  skos:notation 498 ;
  skos:prefLabel "waypoint"@en ;
  skos:prefLabel "경로점"@kr ;
.
<http://iso.org/tc211/term/499>
  rdf:type skos:Concept ;
  dcterms:dateAccepted "2005-02-15"^^xsd:date ;
  dcterms:dateAccepted "2009-12-29"^^xsd:date ;
  dcterms:provenance "KS X ISO 19119" ;
  dcterms:source "ISO 19119:2005" ;
  reg:status reg:statusValid ;
  rdfs:label "workflow"@en ;
  skos:changeNote "valid" ;
  skos:definition "전체 또는 부분적으로 문서나 정보, 업무 등이 절차 규칙에 따라 한 부분에서 다른 부분으로 전달되는 업무 절차의 자동화 "@kr ;
  skos:editorialNote "preferred" ;
  skos:editorialNote "preferred"^^xsd:string ;
  skos:notation "499" ;
  skos:notation 499 ;
  skos:prefLabel "workflow"@en ;
  skos:prefLabel "작업 흐름"@kr ;
.
<http://iso.org/tc211/term/5>
  rdf:type skos:Concept ;
  dcterms:dateAccepted "2000-12-15"^^xsd:date ;
  dcterms:dateAccepted "2007-06-29"^^xsd:date ;
  dcterms:provenance "KS X ISO 19105" ;
  dcterms:source "ISO 19105:2000" ;
  reg:status reg:statusValid ;
  rdfs:comment "Note 1 to entry: Abstract test modules may be nested in a hierarchical way."@en ;
  rdfs:comment "비고: 추상 시험 모듈은 계층적 구조를 가질 수 있다."@kr ;
  rdfs:label "abstract test module"@en ;
  skos:changeNote "valid" ;
  skos:definition "관련된 추상 시험 케이스의 집합"@kr ;
  skos:editorialNote "preferred" ;
  skos:editorialNote "preferred"^^xsd:string ;
  skos:notation "5" ;
  skos:notation 5 ;
  skos:note "Note 1 to entry: Abstract test modules may be nested in a hierarchical way."@en ;
  skos:note "비고: 추상 시험 모듈은 계층적 구조를 가질 수 있다."@kr ;
  skos:prefLabel "abstract test module"@en ;
  skos:prefLabel "추상 시험 모듈"@kr ;
.
<http://iso.org/tc211/term/50>
  rdf:type skos:Concept ;
  dcterms:dateAccepted "2007-09-01"^^xsd:date ;
  dcterms:dateAccepted "2009-12-29"^^xsd:date ;
  dcterms:provenance "KS X ISO 19136" ;
  dcterms:source "ISO 19136:2007" ;
  reg:status reg:statusValid ;
  rdfs:label "codelist"@en ;
  skos:changeNote "valid" ;
  skos:definition "각 코드에 따른 허용 값을 제시하는 값 영역"@kr ;
  skos:editorialNote "preferred" ;
  skos:editorialNote "preferred"^^xsd:string ;
  skos:notation "50" ;
  skos:notation 50 ;
  skos:prefLabel "codelist"@en ;
  skos:prefLabel "코드 목록"@kr ;
.
<http://iso.org/tc211/term/501>
  rdf:type skos:Concept ;
  dcterms:dateAccepted "2003-02-15" ;
  dcterms:dateAccepted "2003-02-15"^^xsd:date ;
  dcterms:dateAccepted "2007-11-01"^^xsd:date ;
  dcterms:provenance "ISO 19111:2003" ;
  dcterms:provenance "KS X ISO 19111" ;
  dcterms:source "ISO 19111:2007" ;
  reg:status reg:statusAccepted ;
  reg:status reg:statusValid ;
  rdfs:comment "Note 1 to entry: Engineering datum excludes both geodetic and vertical datums."@en ;
  rdfs:comment "OPMERKING Een lokaal datum is nooit een geodetisch of verticaal datum."@en ;
  rdfs:comment "비고: 공학 데이텀은 측지 원점 및 수직 데이텀 모두를 포함하지 않는다."@kr ;
  rdfs:label "local datum"@en ;
  rdfs:seeAlso "engineering datum" ;
  rdfs:seeAlso "lokale datum"@nl ;
  skos:altLabel "engineering datum"@en ;
  skos:altLabel "lokale datum"@nl ;
  skos:changeNote "valid" ;
  skos:definition "datum welke de relatie van een coördinaatsysteem ten opzichte van een lokale referentie beschrijft"@nl ;
  skos:definition "좌표 체계와 지역 참조와의 관계를 설명하는 공학 데이텀"@kr ;
  skos:editorialNote "admitted" ;
  skos:editorialNote "admitted"^^xsd:string ;
  skos:notation "501" ;
  skos:notation 501 ;
  skos:note "Note 1 to entry: Engineering datum excludes both geodetic and vertical datums."@en ;
  skos:note "OPMERKING Een lokaal datum is nooit een geodetisch of verticaal datum."@en ;
  skos:note "비고: 공학 데이텀은 측지 원점 및 수직 데이텀 모두를 포함하지 않는다."@kr ;
  skos:prefLabel "local datum"@en ;
  skos:prefLabel "lokaal datum"@nl ;
  skos:prefLabel "지역데이텀"@kr ;
.
<http://iso.org/tc211/term/502>
  rdf:type skos:Concept ;
  dcterms:dateAccepted "2003-02-15" ;
  dcterms:dateAccepted "2003-02-15"^^xsd:date ;
  dcterms:dateAccepted "2007-11-01"^^xsd:date ;
  dcterms:provenance "ISO 19111:2003" ;
  dcterms:provenance "KS X ISO 19111" ;
  dcterms:source "ISO 19111:2007" ;
  reg:status reg:statusAccepted ;
  reg:status reg:statusValid ;
  rdfs:label "ellipsoidal coordinate system"@en ;
  rdfs:seeAlso "geodetic coordinate system" ;
  rdfs:seeAlso "geodetisch coördinaat systeem"@nl ;
  skos:altLabel "geodetic coordinate system"@en ;
  skos:altLabel "geodetisch coördinaat systeem"@nl ;
  skos:changeNote "valid" ;
  skos:definition "coördinaatsysteem waarbij de positie wordt bepaald door geodetische lengte, geodetische breedte en (in het driedimensionale geval) ellipsoïde hoogte"@nl ;
  skos:definition "타원체고, 측지 경도, 측지 위도를 통해 위치를 표현하는 좌표 체계"@kr ;
  skos:editorialNote "preferred" ;
  skos:editorialNote "preferred"^^xsd:string ;
  skos:notation "502" ;
  skos:notation 502 ;
  skos:prefLabel "ellipsoidaal coördinaatsysteem"@nl ;
  skos:prefLabel "ellipsoidal coordinate system"@en ;
  skos:prefLabel "타원체 좌표계"@kr ;
.
<http://iso.org/tc211/term/503>
  rdf:type skos:Concept ;
  dcterms:dateAccepted "2003-02-15" ;
  dcterms:dateAccepted "2003-02-15"^^xsd:date ;
  dcterms:dateAccepted "2007-11-01"^^xsd:date ;
  dcterms:provenance "ISO 19111:2003" ;
  dcterms:provenance "KS X ISO 19111" ;
  dcterms:source "ISO 19111:2007" ;
  reg:status reg:statusAccepted ;
  reg:status reg:statusValid ;
  rdfs:label "ellipsoidal latitude"@en ;
  rdfs:seeAlso "geodetic latitude" ;
  rdfs:seeAlso "geodetische breedte"@nl ;
  skos:altLabel "geodetic latitude"@en ;
  skos:altLabel "geodetische breedte"@nl ;
  skos:altLabel "j"@kr ;
  skos:altLabel "j"@nl ;
  skos:altLabel "j"^^<http://www.w3.org/2001/XMLSchema#@en> ;
  skos:changeNote "valid" ;
  skos:definition "hoek vanaf het equatoriale vlak van de ellipsoïde door een gegeven punt, noordwaarts wordt als positief genomen"@nl ;
  skos:definition "타원체상의 어떤 점을 통과하는 수직선과 적도면과의 각도로서, 북으로 향하는 것을 정(+)으로 함"@kr ;
  skos:editorialNote "admitted" ;
  skos:editorialNote "admitted"^^xsd:string ;
  skos:notation "503" ;
  skos:notation 503 ;
  skos:prefLabel "ellipsoidal latitude"@en ;
  skos:prefLabel "ellipsoïde breedte"@nl ;
  skos:prefLabel "타원체 위도"@kr ;
.
<http://iso.org/tc211/term/504>
  rdf:type skos:Concept ;
  dcterms:dateAccepted "2003-02-15" ;
  dcterms:dateAccepted "2003-02-15"^^xsd:date ;
  dcterms:dateAccepted "2007-11-01"^^xsd:date ;
  dcterms:provenance "ISO 19111:2003" ;
  dcterms:provenance "KS X ISO 19111" ;
  dcterms:source "ISO 19111:2007" ;
  reg:status reg:statusAccepted ;
  reg:status reg:statusValid ;
  rdfs:label "ellipsoidal longitude"@en ;
  rdfs:seeAlso "geodetic longitude" ;
  rdfs:seeAlso "geodetische lengte"@nl ;
  skos:altLabel "geodetic longitude"@en ;
  skos:altLabel "geodetische lengte"@nl ;
  skos:altLabel "l"@kr ;
  skos:altLabel "l"@nl ;
  skos:altLabel "l"^^<http://www.w3.org/2001/XMLSchema#@en> ;
  skos:changeNote "valid" ;
  skos:definition "hoek vanaf het vlak van de nulmeridiaan tot het meridiaan vlak van een gegeven punt, oostwaarts wordt als positief genomen"@nl ;
  skos:definition "본초 자오선면으로부터 어떤 점의 자오선면까지의 각도로서, 동으로 향하는 것을 정(+)으로 함"@kr ;
  skos:editorialNote "admitted" ;
  skos:editorialNote "admitted"^^xsd:string ;
  skos:notation "504" ;
  skos:notation 504 ;
  skos:prefLabel "ellipsoidal longitude"@en ;
  skos:prefLabel "ellipsoïde lengte"@nl ;
  skos:prefLabel "타원체 경도"@kr ;
.
<http://iso.org/tc211/term/505>
  rdf:type skos:Concept ;
  dcterms:dateAccepted "2003-02-15" ;
  dcterms:dateAccepted "2003-02-15"^^xsd:date ;
  dcterms:dateAccepted "2007-11-01"^^xsd:date ;
  dcterms:provenance "ISO 19111:2003" ;
  dcterms:provenance "KS X ISO 19111" ;
  dcterms:source "ISO 19111:2007" ;
  reg:status reg:statusAccepted ;
  reg:status reg:statusValid ;
  rdfs:label "zero meridian"@en ;
  rdfs:seeAlso "nul meridiaan"@nl ;
  rdfs:seeAlso "prime meridian" ;
  skos:altLabel "nul meridiaan"@nl ;
  skos:altLabel "prime meridian"@en ;
  skos:changeNote "valid" ;
  skos:definition "meridiaan waarvandaan de lengtegraden van de overige meridianen worden bepaald"@nl ;
  skos:definition "본초 자오선, 다른 자오선의 경도 정량화에 사용되는 기준 자오선 "@kr ;
  skos:editorialNote "admitted" ;
  skos:editorialNote "admitted"^^xsd:string ;
  skos:notation "505" ;
  skos:notation 505 ;
  skos:prefLabel "0도 자오선"@kr ;
  skos:prefLabel "nulmeridiaan"@nl ;
  skos:prefLabel "zero meridian"@en ;
.
<http://iso.org/tc211/term/506>
  rdf:type skos:Concept ;
  dcterms:dateAccepted "2005-10-15"^^xsd:date ;
  dcterms:dateAccepted "2009-12-29"^^xsd:date ;
  dcterms:provenance "KS X ISO 19135" ;
  dcterms:source "ISO 19135:2005" ;
  reg:status reg:statusValid ;
  rdfs:comment "Note 1 to entry: A non-substantive change does not change the semantics or technical meaning of the item.  Clarification does not result in a change to the registration status of the register item."@en ;
  rdfs:comment "비고: 명시는 본질적, 기술적 의미를 바꾸지 않는다. 명시로는 등록물 항목의 등록상태가 변경되지 않는다."@kr ;
  rdfs:label "clarification"@en ;
  skos:changeNote "valid" ;
  skos:definition "등록물 항목에 대한 설명"@kr ;
  skos:editorialNote "preferred" ;
  skos:editorialNote "preferred"^^xsd:string ;
  skos:notation "506" ;
  skos:notation 506 ;
  skos:note "Note 1 to entry: A non-substantive change does not change the semantics or technical meaning of the item.  Clarification does not result in a change to the registration status of the register item."@en ;
  skos:note "비고: 명시는 본질적, 기술적 의미를 바꾸지 않는다. 명시로는 등록물 항목의 등록상태가 변경되지 않는다."@kr ;
  skos:prefLabel "clarification"@en ;
  skos:prefLabel "명시"@kr ;
.
<http://iso.org/tc211/term/507>
  rdf:type skos:Concept ;
  dcterms:dateAccepted "2005-10-15"^^xsd:date ;
  dcterms:dateAccepted "2009-12-29"^^xsd:date ;
  dcterms:source "ISO 19135:2005, 4.1.7" ;
  reg:status reg:statusValid ;
  rdfs:comment "0"@en ;
  rdfs:label "locale"@en ;
  skos:changeNote "valid" ;
  skos:definition "문자열 해석에 적용 가능한 문화 및 언어적 환경"@kr ;
  skos:editorialNote "preferred" ;
  skos:editorialNote "preferred"^^xsd:string ;
  skos:notation "507" ;
  skos:notation 507 ;
  skos:note "0"@en ;
  skos:prefLabel "locale"@en ;
  skos:prefLabel "현장"@kr ;
.
<http://iso.org/tc211/term/508>
  rdf:type skos:Concept ;
  dcterms:dateAccepted "2005-10-15" ;
  dcterms:dateAccepted "2005-10-15"^^xsd:date ;
  dcterms:dateAccepted "2009-12-29"^^xsd:date ;
  dcterms:provenance "KS X ISO 19135" ;
  dcterms:source "ISO 19135:2005" ;
  reg:status reg:statusAccepted ;
  reg:status reg:statusValid ;
  rdfs:comment "NOTE In the case of an ISO register, the register manager performs the functions of the registration authority specified in the ISO/IEC Directives."@en ;
  rdfs:comment "Note 1 to entry: In the case of an ISO register, the register manager performs the functions of the registration authority specified in the ISO/IEC Directives."@en ;
  rdfs:comment "비고: ISO 등록물의 경우, 등록물 관리자는 ISO/IEC Directives에 명시된 등록 당국의 기능을 수행한다. "@kr ;
  rdfs:label "register manager"@en ;
  skos:changeNote "valid" ;
  skos:definition "organisatie die verantwoordelijk is voor het beheer van een register"@nl ;
  skos:definition "등록물 소유자로부터 등록물의 관리를 위임 받은 기구"@kr ;
  skos:editorialNote "preferred" ;
  skos:editorialNote "preferred"^^xsd:string ;
  skos:notation "508" ;
  skos:notation 508 ;
  skos:note "NOTE In the case of an ISO register, the register manager performs the functions of the registration authority specified in the ISO/IEC Directives."@en ;
  skos:note "Note 1 to entry: In the case of an ISO register, the register manager performs the functions of the registration authority specified in the ISO/IEC Directives."@en ;
  skos:note "비고: ISO 등록물의 경우, 등록물 관리자는 ISO/IEC Directives에 명시된 등록 당국의 기능을 수행한다. "@kr ;
  skos:prefLabel "register manager"@en ;
  skos:prefLabel "register manager"@nl ;
  skos:prefLabel "등록물 관리자"@kr ;
.
<http://iso.org/tc211/term/509>
  rdf:type skos:Concept ;
  dcterms:dateAccepted "2005-10-15"^^xsd:date ;
  dcterms:dateAccepted "2009-12-29"^^xsd:date ;
  dcterms:provenance "KS X ISO 19135" ;
  dcterms:source "ISO 19135:2005" ;
  reg:status reg:statusValid ;
  rdfs:comment "Note 1 to entry: The status of the retired item changes from 'valid' to 'retired'. A retired item is kept in the register to support the interpretation of data produced before its retirement."@en ;
  rdfs:comment "비고: 철회 항목의 상태는 \"유효\"에서 \"철회\"로 변경된다. 철회 항목은 철회 이전에 생산된 데이터의 해석을 위해 등록물에 보관된다. "@kr ;
  rdfs:label "retirement"@en ;
  skos:changeNote "valid" ;
  skos:definition "등록물 항목이 새로운 데이터의 생산에 더 이상 적합하지 않다는 선언"@kr ;
  skos:editorialNote "preferred" ;
  skos:editorialNote "preferred"^^xsd:string ;
  skos:notation "509" ;
  skos:notation 509 ;
  skos:note "Note 1 to entry: The status of the retired item changes from 'valid' to 'retired'. A retired item is kept in the register to support the interpretation of data produced before its retirement."@en ;
  skos:note "비고: 철회 항목의 상태는 \"유효\"에서 \"철회\"로 변경된다. 철회 항목은 철회 이전에 생산된 데이터의 해석을 위해 등록물에 보관된다. "@kr ;
  skos:prefLabel "retirement"@en ;
  skos:prefLabel "철회"@kr ;
.
<http://iso.org/tc211/term/51>
  rdf:type skos:Concept ;
  dcterms:dateAccepted "2007-09-01"^^xsd:date ;
  dcterms:dateAccepted "2009-12-29"^^xsd:date ;
  dcterms:provenance "KS X ISO 19136" ;
  dcterms:source "ISO 19136:2007" ;
  reg:status reg:statusValid ;
  rdfs:label "codespace"@en ;
  skos:changeNote "valid" ;
  skos:definition "코드, 이름, 용어, 분류 체계 등에 대한 규정"@kr ;
  skos:editorialNote "preferred" ;
  skos:editorialNote "preferred"^^xsd:string ;
  skos:notation "51" ;
  skos:notation 51 ;
  skos:prefLabel "codespace"@en ;
  skos:prefLabel "코드 영역"@kr ;
.
<http://iso.org/tc211/term/510>
  rdf:type skos:Concept ;
  dcterms:dateAccepted "2005-10-15"^^xsd:date ;
  dcterms:dateAccepted "2009-12-29"^^xsd:date ;
  dcterms:source "ISO 19135:2005, 4.1.18" ;
  reg:status reg:statusValid ;
  rdfs:comment "Note 1 to entry: The status of the replaced item changes from \"valid\" to \"superseded.\""@en ;
  rdfs:comment "비고: 대체된 아이템의 상태가 \"유효\"에서 \"교체\"로 바뀐다."@kr ;
  rdfs:label "supersession"@en ;
  skos:changeNote "valid" ;
  skos:definition "하나 이상의 새로운 항목에 의한 등록물 항목의 대체"@kr ;
  skos:editorialNote "preferred" ;
  skos:editorialNote "preferred"^^xsd:string ;
  skos:notation "510" ;
  skos:notation 510 ;
  skos:note "Note 1 to entry: The status of the replaced item changes from \"valid\" to \"superseded.\""@en ;
  skos:note "비고: 대체된 아이템의 상태가 \"유효\"에서 \"교체\"로 바뀐다."@kr ;
  skos:prefLabel "supersession"@en ;
  skos:prefLabel "교체"@kr ;
.
<http://iso.org/tc211/term/518>
  rdf:type skos:Concept ;
  dcterms:dateAccepted "2010-06-15"^^xsd:date ;
  dcterms:source "ISO/TS 19130:2010" ;
  reg:status reg:statusValid ;
  rdfs:comment "Note 1 to entry: In remote sensing and aerial photogrammetry an object point is a point defined in an Earth-fixed coordinate reference system."@en ;
  rdfs:label "object point"@en ;
  skos:changeNote "valid" ;
  skos:editorialNote "preferred"^^xsd:string ;
  skos:notation 518 ;
  skos:note "Note 1 to entry: In remote sensing and aerial photogrammetry an object point is a point defined in an Earth-fixed coordinate reference system."@en ;
  skos:prefLabel "object point"@en ;
.
<http://iso.org/tc211/term/519>
  rdf:type skos:Concept ;
  dcterms:dateAccepted "2014-01-15"^^xsd:date ;
  dcterms:source "ISO/TS 19130-2:2014, 4.46" ;
  reg:status reg:statusValid ;
  rdfs:label "objective"@en ;
  skos:changeNote "valid" ;
  skos:editorialNote "preferred"^^xsd:string ;
  skos:notation 519 ;
  skos:prefLabel "objective"@en ;
.
<http://iso.org/tc211/term/52>
  rdf:type skos:Concept ;
  dcterms:dateAccepted "2005-06-15"^^xsd:date ;
  dcterms:dateAccepted "2006-05-01"^^xsd:date ;
  dcterms:provenance "KS X ISO 19109" ;
  dcterms:source "ISO 19109:2005" ;
  reg:status reg:statusValid ;
  rdfs:label "complex feature"@en ;
  skos:changeNote "valid" ;
  skos:definition "다수의 피처들로 구성된 피처"@kr ;
  skos:editorialNote "preferred" ;
  skos:editorialNote "preferred"^^xsd:string ;
  skos:notation "52" ;
  skos:notation 52 ;
  skos:prefLabel "complex feature"@en ;
  skos:prefLabel "복합 지형지물"@kr ;
.
<http://iso.org/tc211/term/521>
  rdf:type skos:Concept ;
  dcterms:dateAccepted "2010-06-15"^^xsd:date ;
  dcterms:source "ISO/TS 19130:2010" ;
  reg:status reg:statusValid ;
  rdfs:label "principal point of best symmetry"@en ;
  skos:changeNote "valid" ;
  skos:editorialNote "preferred"^^xsd:string ;
  skos:notation 521 ;
  skos:prefLabel "principal point of best symmetry"@en ;
.
<http://iso.org/tc211/term/532>
  rdf:type skos:Concept ;
  dcterms:dateAccepted "2007-09-01" ;
  dcterms:dateAccepted "2007-09-01"^^xsd:date ;
  dcterms:dateAccepted "2009-12-29"^^xsd:date ;
  dcterms:provenance "KS X ISO 19136" ;
  dcterms:source "ISO 19136:2007" ;
  reg:status reg:statusAccepted ;
  reg:status reg:statusValid ;
  rdfs:comment "NOTE In this document an attribute is an XML attribute unless otherwise specified. The syntax of an XML attribute is  \"Attribute::= Name = AttValue\". An attribute typically acts as an XML element modifier (e.g.  <Road gml:id = \"r1\" />; here gml:id is an attribute."@en ;
  rdfs:comment "Note 1 to entry: In this document an attribute is an XML attribute unless otherwise specified. The syntax of an XML attribute is  \"Attribute::= Name = AttValue\". An attribute typically acts as an XML element modifier (e.g.  <Road gml:id = \"r1\" />; here gml:id is an attribute."@en ;
  rdfs:comment "비고: 이 문서에서 '속성'은 XML 속성을 의미한다. XML 속성의 문법은 “Attribute::= Name = AttValue”와 같으며, 속성은 XML에서 제어자(modifier)로 사용된다.(예. <Road gml:id = “r1” />;에서 gml:id가 속성임)"@kr ;
  rdfs:label "attribute <XML>"@en ;
  skos:changeNote "valid" ;
  skos:definition "naam-waarde combinatie binnen een element"@nl ;
  skos:definition "요소가 갖는 이름-값 쌍"@kr ;
  skos:editorialNote "preferred" ;
  skos:editorialNote "preferred"^^xsd:string ;
  skos:notation "532" ;
  skos:notation 532 ;
  skos:note "NOTE In this document an attribute is an XML attribute unless otherwise specified. The syntax of an XML attribute is  \"Attribute::= Name = AttValue\". An attribute typically acts as an XML element modifier (e.g.  <Road gml:id = \"r1\" />; here gml:id is an attribute."@en ;
  skos:note "Note 1 to entry: In this document an attribute is an XML attribute unless otherwise specified. The syntax of an XML attribute is  \"Attribute::= Name = AttValue\". An attribute typically acts as an XML element modifier (e.g.  <Road gml:id = \"r1\" />; here gml:id is an attribute."@en ;
  skos:note "비고: 이 문서에서 '속성'은 XML 속성을 의미한다. XML 속성의 문법은 “Attribute::= Name = AttValue”와 같으며, 속성은 XML에서 제어자(modifier)로 사용된다.(예. <Road gml:id = “r1” />;에서 gml:id가 속성임)"@kr ;
  skos:prefLabel "attribute <XML>"@en ;
  skos:prefLabel "attribuut <XML>"@nl ;
  skos:prefLabel "속성 <XML>"@kr ;
.
<http://iso.org/tc211/term/534>
  rdf:type skos:Concept ;
  dcterms:dateAccepted "2007-09-01"^^xsd:date ;
  dcterms:dateAccepted "2009-12-29"^^xsd:date ;
  dcterms:provenance "KS X ISO 19136" ;
  dcterms:source "ISO 19136:2007" ;
  reg:status reg:statusValid ;
  rdfs:comment "Note 1 to entry: It corresponds to feature attribute and feature association role in ISO 19109.  If a GML property of a feature has an xlink:href attribute that references a feature, the property represents a feature association role."@en ;
  rdfs:comment "비고: 속성(property)은 KS X ISO 19109의 피처 속성, 피처 연관 규칙에 해당한다. 피처의 GML 속성은 피처를 참조하는 xlink:href 속성을 갖고, 그 속성은 피처 연관 규칙을 나타낸다."@kr ;
  rdfs:label "property <GML>"@en ;
  skos:changeNote "valid" ;
  skos:definition "GML 객체의 자식 요소"@kr ;
  skos:editorialNote "preferred" ;
  skos:editorialNote "preferred"^^xsd:string ;
  skos:notation "534" ;
  skos:notation 534 ;
  skos:note "Note 1 to entry: It corresponds to feature attribute and feature association role in ISO 19109.  If a GML property of a feature has an xlink:href attribute that references a feature, the property represents a feature association role."@en ;
  skos:note "비고: 속성(property)은 KS X ISO 19109의 피처 속성, 피처 연관 규칙에 해당한다. 피처의 GML 속성은 피처를 참조하는 xlink:href 속성을 갖고, 그 속성은 피처 연관 규칙을 나타낸다."@kr ;
  skos:prefLabel "property <GML>"@en ;
  skos:prefLabel "속성 <GML>"@kr ;
.
<http://iso.org/tc211/term/535>
  rdf:type skos:Concept ;
  dcterms:dateAccepted "2005-10-15"^^xsd:date ;
  dcterms:dateAccepted "2009-12-29"^^xsd:date ;
  dcterms:provenance "KS X ISO 19135" ;
  dcterms:source "ISO 19135:2005" ;
  reg:status reg:statusValid ;
  rdfs:label "principal register"@en ;
  skos:changeNote "valid" ;
  skos:definition "계층적 등록물에서 각각의 하위 등록물에 대한 기술을 포함하는 등록물"@kr ;
  skos:editorialNote "preferred" ;
  skos:editorialNote "preferred"^^xsd:string ;
  skos:notation "535" ;
  skos:notation 535 ;
  skos:prefLabel "principal register"@en ;
  skos:prefLabel "주 등록물"@kr ;
.
<http://iso.org/tc211/term/55>
  rdf:type skos:Concept ;
  dcterms:dateAccepted "2003-05-01"^^xsd:date ;
  dcterms:dateAccepted "2009-12-29"^^xsd:date ;
  dcterms:provenance "KS X ISO 19107" ;
  dcterms:source "ISO 19107:2003" ;
  reg:status reg:statusValid ;
  rdfs:comment "Note 1 to entry: A composite curve, as a set of direct positions, has all the properties of a curve."@en ;
  rdfs:comment "비고: 직접 위치의 집합으로서의 합성 곡선은 곡선의 모든 특성을 갖는다."@kr ;
  rdfs:label "composite curve"@en ;
  skos:changeNote "valid" ;
  skos:definition "첫 번째 곡선을 제외한 각각의 곡선이 연속적으로 앞 곡선의 끝점에서 시작되는 곡선의 연속"@kr ;
  skos:editorialNote "preferred" ;
  skos:editorialNote "preferred"^^xsd:string ;
  skos:notation "55" ;
  skos:notation 55 ;
  skos:note "Note 1 to entry: A composite curve, as a set of direct positions, has all the properties of a curve."@en ;
  skos:note "비고: 직접 위치의 집합으로서의 합성 곡선은 곡선의 모든 특성을 갖는다."@kr ;
  skos:prefLabel "composite curve"@en ;
  skos:prefLabel "합성 곡선"@kr ;
.
<http://iso.org/tc211/term/551>
  rdf:type skos:Concept ;
  dcterms:dateAccepted "2009-02-15"^^xsd:date ;
  dcterms:source "ISO 19115-2:2009" ;
  reg:status reg:statusValid ;
  rdfs:comment "Note 1 to entry: The physical parameters are the result of measurement by a sensor or a prediction from a model"@en ;
  rdfs:label "image"@en ;
  skos:changeNote "valid" ;
  skos:editorialNote "preferred"^^xsd:string ;
  skos:notation 551 ;
  skos:note "Note 1 to entry: The physical parameters are the result of measurement by a sensor or a prediction from a model"@en ;
  skos:prefLabel "image"@en ;
.
<http://iso.org/tc211/term/558>
  rdf:type skos:Concept ;
  dcterms:dateAccepted "2008-06-01"^^xsd:date ;
  dcterms:source "ISO/TS 19101-2:2008" ;
  reg:status reg:statusValid ;
  rdfs:comment "Note 1 to entry:: The data base contains facts, inferences, and procedures needed for problem solution [Webster Computer]"@en ;
  rdfs:label "knowledge base"@en ;
  skos:changeNote "valid" ;
  skos:editorialNote "preferred"^^xsd:string ;
  skos:notation 558 ;
  skos:note "Note 1 to entry:: The data base contains facts, inferences, and procedures needed for problem solution [Webster Computer]"@en ;
  skos:prefLabel "knowledge base"@en ;
.
<http://iso.org/tc211/term/559>
  rdf:type skos:Concept ;
  dcterms:dateAccepted "2006-12-01"^^xsd:date ;
  dcterms:dateAccepted "2008-12-19"^^xsd:date ;
  dcterms:provenance "ISO/TS 19138:2006" ;
  dcterms:provenance "KS X ISO 19104" ;
  dcterms:source "International Vocabulary of Basic and General Terms in Metrology (VIM)" ;
  reg:status reg:statusValid ;
  rdfs:label "measurand"@en ;
  skos:changeNote "valid" ;
  skos:definition "측정에 따라 얻어진 특정량"@kr ;
  skos:editorialNote "preferred" ;
  skos:editorialNote "preferred"^^xsd:string ;
  skos:notation "559" ;
  skos:notation 559 ;
  skos:prefLabel "measurand"@en ;
  skos:prefLabel "측정량"@kr ;
.
<http://iso.org/tc211/term/56>
  rdf:type skos:Concept ;
  dcterms:dateAccepted "2003-05-01"^^xsd:date ;
  dcterms:dateAccepted "2009-12-29"^^xsd:date ;
  dcterms:provenance "KS X ISO 19107" ;
  dcterms:source "ISO 19107:2003" ;
  reg:status reg:statusValid ;
  rdfs:comment "Note 1 to entry: A composite solid, as a set of direct positions, has all the properties of a solid."@en ;
  rdfs:comment "비고: 직접 위치의 집합으로서의 합성 입방체는 입방체의 모든 특성을 갖는다."@kr ;
  rdfs:label "composite solid"@en ;
  skos:changeNote "valid" ;
  skos:definition "공유 경계 표면을 따라 서로 연결된 입방체의 집합"@kr ;
  skos:editorialNote "preferred" ;
  skos:editorialNote "preferred"^^xsd:string ;
  skos:notation "56" ;
  skos:notation 56 ;
  skos:note "Note 1 to entry: A composite solid, as a set of direct positions, has all the properties of a solid."@en ;
  skos:note "비고: 직접 위치의 집합으로서의 합성 입방체는 입방체의 모든 특성을 갖는다."@kr ;
  skos:prefLabel "composite solid"@en ;
  skos:prefLabel "합성 입방체"@kr ;
.
<http://iso.org/tc211/term/560>
  rdf:type skos:Concept ;
  dcterms:dateAccepted "2008-06-01"^^xsd:date ;
  dcterms:provenance "ISO/TS 19101-2:2008" ;
  dcterms:source "International Vocabulary of Basic and General Terms in Metrology (VIM)" ;
  reg:status reg:statusValid ;
  rdfs:label "measurement"@en ;
  skos:changeNote "valid" ;
  skos:editorialNote "preferred"^^xsd:string ;
  skos:notation 560 ;
  skos:prefLabel "measurement"@en ;
.
<http://iso.org/tc211/term/57>
  rdf:type skos:Concept ;
  dcterms:dateAccepted "2003-05-01"^^xsd:date ;
  dcterms:dateAccepted "2009-12-29"^^xsd:date ;
  dcterms:provenance "KS X ISO 19107" ;
  dcterms:source "ISO 19107:2003" ;
  reg:status reg:statusValid ;
  rdfs:comment "Note 1 to entry: A composite surface, as a set of direct positions, has all the properties of a surface."@en ;
  rdfs:comment "비고: 직접위치의 집합으로서의 합성 표면은 표면의 모든 특성을 갖는다."@kr ;
  rdfs:label "composite surface"@en ;
  skos:changeNote "valid" ;
  skos:definition "공유 경계 곡선을 따라 서로 연결된 표면의 집합"@kr ;
  skos:editorialNote "preferred" ;
  skos:editorialNote "preferred"^^xsd:string ;
  skos:notation "57" ;
  skos:notation 57 ;
  skos:note "Note 1 to entry: A composite surface, as a set of direct positions, has all the properties of a surface."@en ;
  skos:note "비고: 직접위치의 집합으로서의 합성 표면은 표면의 모든 특성을 갖는다."@kr ;
  skos:prefLabel "composite surface"@en ;
  skos:prefLabel "합성 표면"@kr ;
.
<http://iso.org/tc211/term/572>
  rdf:type skos:Concept ;
  dcterms:dateAccepted "2008-06-01"^^xsd:date ;
  dcterms:provenance "ISO/TS 19101-2:2008" ;
  dcterms:source "ISO 31-6" ;
  reg:status reg:statusValid ;
  rdfs:label "radiant energy"@en ;
  skos:changeNote "valid" ;
  skos:editorialNote "preferred"^^xsd:string ;
  skos:notation 572 ;
  skos:prefLabel "radiant energy"@en ;
.
<http://iso.org/tc211/term/598>
  rdf:type skos:Concept ;
  dcterms:dateAccepted "2007-07-01" ;
  dcterms:dateAccepted "2007-07-01"^^xsd:date ;
  dcterms:dateAccepted "2007-11-01"^^xsd:date ;
  dcterms:provenance "KS X ISO 19111" ;
  dcterms:source "ISO 19111:2007" ;
  reg:status reg:statusAccepted ;
  reg:status reg:statusValid ;
  rdfs:label "affine coordinate system"@en ;
  skos:changeNote "valid" ;
  skos:definition "coördinaat systeem in de Euclidische ruimte met rechte assen die niet noodzakelijkerwijs loodrecht op elkaar staan"@nl ;
  skos:definition "유클리디안 공간에서 직선축들로 구성된 좌표 체계로서 축들이 반드시 직교할 필요는 없음"@kr ;
  skos:editorialNote "preferred" ;
  skos:editorialNote "preferred"^^xsd:string ;
  skos:notation "598" ;
  skos:notation 598 ;
  skos:prefLabel "affien coördinaat systeem"@nl ;
  skos:prefLabel "affine coordinate system"@en ;
  skos:prefLabel "어파인 좌표계"@kr ;
.
<http://iso.org/tc211/term/6>
  rdf:type skos:Concept ;
  dcterms:dateAccepted "2000-12-15"^^xsd:date ;
  dcterms:dateAccepted "2007-06-29"^^xsd:date ;
  dcterms:provenance "KS X ISO 19105" ;
  dcterms:source "ISO 19105:2000" ;
  reg:status reg:statusValid ;
  rdfs:comment "Note 1 to entry: Abstract test suites are described in a conformance clause."@en ;
  rdfs:comment "비고: 추상 시험 스위트는 적합성 조항에서 기술되어 있다."@kr ;
  rdfs:label "abstract test suite"@en ;
  skos:altLabel "ATS"^^<http://www.w3.org/2001/XMLSchema#@en> ;
  skos:changeNote "valid" ;
  skos:definition "적합성 시험에 요구되는 모든 사항들을 규정한 추상 시험 모듈"@kr ;
  skos:editorialNote "preferred" ;
  skos:editorialNote "preferred"^^xsd:string ;
  skos:notation "6" ;
  skos:notation 6 ;
  skos:note "Note 1 to entry: Abstract test suites are described in a conformance clause."@en ;
  skos:note "비고: 추상 시험 스위트는 적합성 조항에서 기술되어 있다."@kr ;
  skos:prefLabel "abstract test suite"@en ;
  skos:prefLabel "추상 시험 스위트"@kr ;
.
<http://iso.org/tc211/term/600>
  rdf:type skos:Concept ;
  dcterms:dateAccepted "2007-07-01" ;
  dcterms:dateAccepted "2007-07-01"^^xsd:date ;
  dcterms:dateAccepted "2007-11-01"^^xsd:date ;
  dcterms:provenance "KS X ISO 19111" ;
  dcterms:source "ISO 19111:2007" ;
  reg:status reg:statusAccepted ;
  reg:status reg:statusValid ;
  rdfs:label "concatenated operation"@en ;
  skos:changeNote "valid" ;
  skos:definition "coördinaatbewerking bestaande uit achter elkaar toegepaste of meervoudige coördinaatbewerkingen"@nl ;
  skos:definition "다수의 좌표 연산을 순차적으로 수행하는 응용으로 구성된 좌표 연산"@kr ;
  skos:editorialNote "preferred" ;
  skos:editorialNote "preferred"^^xsd:string ;
  skos:notation "600" ;
  skos:notation 600 ;
  skos:prefLabel "aaneengeschakelde bewerking"@nl ;
  skos:prefLabel "concatenated operation"@en ;
  skos:prefLabel "연쇄 연산"@kr ;
.
<http://iso.org/tc211/term/603>
  rdf:type skos:Concept ;
  dcterms:dateAccepted "2007-07-01" ;
  dcterms:dateAccepted "2007-07-01"^^xsd:date ;
  dcterms:dateAccepted "2007-11-01"^^xsd:date ;
  dcterms:provenance "KS X ISO 19111" ;
  dcterms:source "ISO 19111:2007" ;
  reg:status reg:statusAccepted ;
  reg:status reg:statusValid ;
  rdfs:label "cylindrical coordinate system"@en ;
  skos:changeNote "valid" ;
  skos:definition "driedimensionaal coördinaatsysteem met twee afstandgebaseerde en een hoekgebaseerde coördinaat"@nl ;
  skos:definition "두 개의 거리와 하나의 각도 좌표로 구성된 3차원 좌표 체계"@kr ;
  skos:editorialNote "preferred" ;
  skos:editorialNote "preferred"^^xsd:string ;
  skos:notation "603" ;
  skos:notation 603 ;
  skos:prefLabel "cilindrisch coördinaat systeem"@nl ;
  skos:prefLabel "cylindrical coordinate system"@en ;
  skos:prefLabel "원통 좌표계"@kr ;
.
<http://iso.org/tc211/term/605>
  rdf:type skos:Concept ;
  dcterms:dateAccepted "2007-07-01" ;
  dcterms:dateAccepted "2007-07-01"^^xsd:date ;
  dcterms:dateAccepted "2007-11-01"^^xsd:date ;
  dcterms:provenance "KS X ISO 19111" ;
  dcterms:source "ISO 19111:2007" ;
  reg:status reg:statusAccepted ;
  reg:status reg:statusValid ;
  rdfs:comment "Note 1 to entry: A depth above the reference surface will have a negative value"@en ;
  rdfs:comment "OPMERKING Een diepte boven het referentievlak heeft een negatieve waarde"@en ;
  rdfs:comment "비고: 기준면보다 높이 위치한 지점의 깊이는 음의 값을 갖는다."@kr ;
  rdfs:label "depth"@en ;
  skos:changeNote "valid" ;
  skos:definition "afstand van een punt tot een gekozen referentievlak neerwaarts gemeten langs een lijn welke loodrecht op dat referentievlak staat"@nl ;
  skos:definition "선택된 기준면으로부터 직하 방향으로 측정된 한 점까지의 거리"@kr ;
  skos:editorialNote "preferred" ;
  skos:editorialNote "preferred"^^xsd:string ;
  skos:notation "605" ;
  skos:notation 605 ;
  skos:note "Note 1 to entry: A depth above the reference surface will have a negative value"@en ;
  skos:note "OPMERKING Een diepte boven het referentievlak heeft een negatieve waarde"@en ;
  skos:note "비고: 기준면보다 높이 위치한 지점의 깊이는 음의 값을 갖는다."@kr ;
  skos:prefLabel "depth"@en ;
  skos:prefLabel "diepte"@nl ;
  skos:prefLabel "깊이"@kr ;
.
<http://iso.org/tc211/term/61>
  rdf:type skos:Concept ;
  dcterms:dateAccepted "2003-05-01"^^xsd:date ;
  dcterms:dateAccepted "2009-12-29"^^xsd:date ;
  dcterms:provenance "KS X ISO 19107" ;
  dcterms:source "ISO 19107:2003" ;
  reg:status reg:statusValid ;
  rdfs:label "computational geometry"@en ;
  skos:changeNote "valid" ;
  skos:definition "기하 연산을 구현하기 위한 기하 표현의 계산과 조작"@kr ;
  skos:editorialNote "preferred" ;
  skos:editorialNote "preferred"^^xsd:string ;
  skos:notation "61" ;
  skos:notation 61 ;
  skos:prefLabel "computational geometry"@en ;
  skos:prefLabel "계산 기하"@kr ;
.
<http://iso.org/tc211/term/614>
  rdf:type skos:Concept ;
  dcterms:dateAccepted "2007-07-01" ;
  dcterms:dateAccepted "2007-07-01"^^xsd:date ;
  dcterms:dateAccepted "2007-11-01"^^xsd:date ;
  dcterms:provenance "KS X ISO 19111" ;
  dcterms:source "ISO 19111:2007" ;
  reg:status reg:statusAccepted ;
  reg:status reg:statusValid ;
  rdfs:comment "Note 1 to entry: A height below the reference surface will have a negative value."@en ;
  rdfs:comment "OPMERKING Een hoogte onder het referentievlak heeft een negatieve waarde."@en ;
  rdfs:comment "비고: 기준면 아래의 높이(깊이)는 음의 값이다."@kr ;
  rdfs:label "height"@en ;
  skos:altLabel "h, H"@nl ;
  skos:altLabel "h, H"^^<http://www.w3.org/2001/XMLSchema#@en> ;
  skos:altLabel "h; H"@kr ;
  skos:changeNote "valid" ;
  skos:definition "afstand van een punt tot een gekozen referentievlak gemeten naar boven langs een lijn die loodrecht staat op het referentievlak"@nl ;
  skos:definition "선택된 기준면으로부터 기준면 위쪽에 위치한 한 점까지의 수직 거리"@kr ;
  skos:editorialNote "preferred" ;
  skos:editorialNote "preferred"^^xsd:string ;
  skos:notation "614" ;
  skos:notation 614 ;
  skos:note "Note 1 to entry: A height below the reference surface will have a negative value."@en ;
  skos:note "OPMERKING Een hoogte onder het referentievlak heeft een negatieve waarde."@en ;
  skos:note "비고: 기준면 아래의 높이(깊이)는 음의 값이다."@kr ;
  skos:prefLabel "height"@en ;
  skos:prefLabel "hoogte"@nl ;
  skos:prefLabel "높이"@kr ;
.
<http://iso.org/tc211/term/617>
  rdf:type skos:Concept ;
  dcterms:dateAccepted "2007-07-01" ;
  dcterms:dateAccepted "2007-07-01"^^xsd:date ;
  dcterms:dateAccepted "2007-11-01"^^xsd:date ;
  dcterms:provenance "KS X ISO 19111" ;
  dcterms:source "ISO 19111:2007" ;
  reg:status reg:statusAccepted ;
  reg:status reg:statusValid ;
  rdfs:label "linear coordinate system"@en ;
  skos:changeNote "valid" ;
  skos:definition "eendimensionaal coördinaatsysteem waarbij een lijnvormig geo-object de as vormt"@nl ;
  skos:definition "축이 선형 피처로 이루어진 1차원 좌표 체계"@kr ;
  skos:editorialNote "preferred" ;
  skos:editorialNote "preferred"^^xsd:string ;
  skos:notation "617" ;
  skos:notation 617 ;
  skos:prefLabel "lineair coördinaat systeem"@nl ;
  skos:prefLabel "linear coordinate system"@en ;
  skos:prefLabel "선형 좌표계"@kr ;
.
<http://iso.org/tc211/term/618>
  rdf:type skos:Concept ;
  dcterms:dateAccepted "2007-07-01" ;
  dcterms:dateAccepted "2007-07-01"^^xsd:date ;
  dcterms:dateAccepted "2007-11-01"^^xsd:date ;
  dcterms:provenance "KS X ISO 19111" ;
  dcterms:source "ISO 19111:2007" ;
  reg:status reg:statusAccepted ;
  reg:status reg:statusValid ;
  rdfs:label "map projection"@en ;
  skos:changeNote "valid" ;
  skos:definition "coordinate conversion from an ellipsoidal coordinate system to a plane"@nl ;
  skos:definition "타원 체좌표계를 평면으로 좌표 전환"@kr ;
  skos:editorialNote "preferred" ;
  skos:editorialNote "preferred"^^xsd:string ;
  skos:notation "618" ;
  skos:notation 618 ;
  skos:prefLabel "kaartprojectie"@nl ;
  skos:prefLabel "map projection"@en ;
  skos:prefLabel "지도 투영"@kr ;
.
<http://iso.org/tc211/term/619>
  rdf:type skos:Concept ;
  dcterms:dateAccepted "2008-06-01"^^xsd:date ;
  dcterms:source "ISO/TS 19101-2:2008" ;
  reg:status reg:statusValid ;
  rdfs:comment "Note 1 to entry: This term originated as a contraction of \"picture element\""@en ;
  rdfs:comment "Note 2 to entry: Related to the concept of a grid cell" ;
  rdfs:label "pixel"@en ;
  skos:changeNote "valid" ;
  skos:editorialNote "preferred"^^xsd:string ;
  skos:notation 619 ;
  skos:note "Note 1 to entry: This term originated as a contraction of \"picture element\""@en ;
  skos:note "Note 2 to entry: Related to the concept of a grid cell"^^<http://www.w3.org/2001/XMLSchema#@en> ;
  skos:prefLabel "pixel"@en ;
.
<http://iso.org/tc211/term/62>
  rdf:type skos:Concept ;
  dcterms:dateAccepted "2003-05-01"^^xsd:date ;
  dcterms:dateAccepted "2009-12-29"^^xsd:date ;
  dcterms:provenance "KS X ISO 19107" ;
  dcterms:source "ISO 19107:2003" ;
  reg:status reg:statusValid ;
  rdfs:label "computational topology"@en ;
  skos:changeNote "valid" ;
  skos:definition "계산 기하에서 위상 객체에 대하여 일반적으로 수행되는 위상 개념, 구조, 대수 및 부가적 확장 또는 정의 연산"@kr ;
  skos:editorialNote "preferred" ;
  skos:editorialNote "preferred"^^xsd:string ;
  skos:notation "62" ;
  skos:notation 62 ;
  skos:prefLabel "computational topology"@en ;
  skos:prefLabel "계산 위상"@kr ;
.
<http://iso.org/tc211/term/620>
  rdf:type skos:Concept ;
  dcterms:dateAccepted "2007-07-01" ;
  dcterms:dateAccepted "2007-07-01"^^xsd:date ;
  dcterms:dateAccepted "2007-11-01"^^xsd:date ;
  dcterms:provenance "KS X ISO 19111" ;
  dcterms:source "ISO 19111:2007" ;
  reg:status reg:statusAccepted ;
  reg:status reg:statusValid ;
  rdfs:comment "Note 1 to entry: For the three-dimensional case, see spherical coordinate system (4.44)."@en ;
  rdfs:comment "OPMERKING Voor het driedimensionale geval, zie het bol coördinaatsysteem (4.44)."@en ;
  rdfs:comment "비고: 3차원의 경우 구면 좌표계를 참조"@kr ;
  rdfs:label "polar coordinate system"@en ;
  skos:changeNote "valid" ;
  skos:definition "tweedimensionaal coördinaatsysteem waarbij de positie aangeduid wordt met een afstand en richting vanaf het nulpunt"@nl ;
  skos:definition "원점으로부터 거리 및 방향으로 위치를 기술하는 2차원 좌표 체계"@kr ;
  skos:editorialNote "preferred" ;
  skos:editorialNote "preferred"^^xsd:string ;
  skos:notation "620" ;
  skos:notation 620 ;
  skos:note "Note 1 to entry: For the three-dimensional case, see spherical coordinate system (4.44)."@en ;
  skos:note "OPMERKING Voor het driedimensionale geval, zie het bol coördinaatsysteem (4.44)."@en ;
  skos:note "비고: 3차원의 경우 구면 좌표계를 참조"@kr ;
  skos:prefLabel "polair coördinaatsysteem"@nl ;
  skos:prefLabel "polar coordinate system"@en ;
  skos:prefLabel "극 좌표계"@kr ;
.
<http://iso.org/tc211/term/622>
  rdf:type skos:Concept ;
  dcterms:dateAccepted "2007-07-01" ;
  dcterms:dateAccepted "2007-07-01"^^xsd:date ;
  dcterms:dateAccepted "2007-11-01"^^xsd:date ;
  dcterms:provenance "KS X ISO 19111" ;
  dcterms:source "ISO 19111:2007" ;
  reg:status reg:statusAccepted ;
  reg:status reg:statusValid ;
  rdfs:comment "Note 1 to entry: This equates to the semi-diameter of the ellipsoid measured in its equatorial plane."@en ;
  rdfs:comment "OPMERKING Dit is gelijk aan de halve diameter van de ellipsoïde zoals bepaald in het equatoriale vlak."@en ;
  rdfs:comment "비고: 지구 타원체의 장반경은 적도 반경이다."@kr ;
  rdfs:label "semi-major axis"@en ;
  skos:altLabel "a"@kr ;
  skos:altLabel "a"@nl ;
  skos:altLabel "a"^^<http://www.w3.org/2001/XMLSchema#@en> ;
  skos:changeNote "valid" ;
  skos:definition "halve diameter van de langste as van een ellipsoïde"@nl ;
  skos:definition "타원체의 최장 반지름"@kr ;
  skos:editorialNote "preferred" ;
  skos:editorialNote "preferred"^^xsd:string ;
  skos:notation "622" ;
  skos:notation 622 ;
  skos:note "Note 1 to entry: This equates to the semi-diameter of the ellipsoid measured in its equatorial plane."@en ;
  skos:note "OPMERKING Dit is gelijk aan de halve diameter van de ellipsoïde zoals bepaald in het equatoriale vlak."@en ;
  skos:note "비고: 지구 타원체의 장반경은 적도 반경이다."@kr ;
  skos:prefLabel "halve lange as"@nl ;
  skos:prefLabel "semi-major axis"@en ;
  skos:prefLabel "장반경"@kr ;
.
<http://iso.org/tc211/term/623>
  rdf:type skos:Concept ;
  dcterms:dateAccepted "2007-07-01" ;
  dcterms:dateAccepted "2007-07-01"^^xsd:date ;
  dcterms:dateAccepted "2007-11-01"^^xsd:date ;
  dcterms:provenance "KS X ISO 19111" ;
  dcterms:source "ISO 19111:2007" ;
  reg:status reg:statusAccepted ;
  reg:status reg:statusValid ;
  rdfs:comment "Note 1 to entry: The shortest axis coincides with the rotation axis of the ellipsoid and therefore contains both poles."@en ;
  rdfs:comment "OPMERKING De kortste as is gelijk aan de omwentelingsas van de ellipsoïde en bevat daarmee beide polen."@en ;
  rdfs:comment "비고: 지구 타원체의 단반경은 타원체의 중심으로부터 어느 한쪽 극까지의 거리이다."@kr ;
  rdfs:label "semi-minor axis"@en ;
  skos:altLabel "b"@kr ;
  skos:altLabel "b"@nl ;
  skos:altLabel "b"^^<http://www.w3.org/2001/XMLSchema#@en> ;
  skos:changeNote "valid" ;
  skos:definition "halve diameter van de kortste as van een ellipsoïde"@nl ;
  skos:definition "타원체의 최단 반지름"@kr ;
  skos:editorialNote "preferred" ;
  skos:editorialNote "preferred"^^xsd:string ;
  skos:notation "623" ;
  skos:notation 623 ;
  skos:note "Note 1 to entry: The shortest axis coincides with the rotation axis of the ellipsoid and therefore contains both poles."@en ;
  skos:note "OPMERKING De kortste as is gelijk aan de omwentelingsas van de ellipsoïde en bevat daarmee beide polen."@en ;
  skos:note "비고: 지구 타원체의 단반경은 타원체의 중심으로부터 어느 한쪽 극까지의 거리이다."@kr ;
  skos:prefLabel "halve korte as"@nl ;
  skos:prefLabel "semi-minor axis"@en ;
  skos:prefLabel "단반경"@kr ;
.
<http://iso.org/tc211/term/627>
  rdf:type skos:Concept ;
  dcterms:dateAccepted "2007-07-01" ;
  dcterms:dateAccepted "2007-07-01"^^xsd:date ;
  dcterms:dateAccepted "2007-11-01"^^xsd:date ;
  dcterms:provenance "KS X ISO 19111" ;
  dcterms:source "ISO 19111:2007" ;
  reg:status reg:statusAccepted ;
  reg:status reg:statusValid ;
  rdfs:comment "Note 1 to entry: In this International Standard, the subtypes of units are length units, angular units, time units, scale units and pixel spacing units."@en ;
  rdfs:comment "OPMERKING In deze Internationale Standaard zijn de subtypen van eenheden de lengte-eenheden, hoekeenheden, tijdeenheden, schaaleenheden en pixelafstandeenheden."@en ;
  rdfs:comment "비고: KS X ISO 19111 표준에서 단위의 하위 유형은 길이 단위, 각 단위, 시간 단위, 척도 단위 및 픽셀 간격 단위이다.  "@kr ;
  rdfs:label "unit"@en ;
  skos:changeNote "valid" ;
  skos:definition "bepaalde hoeveelheid waarin een gemeten parameter wordt uitgedrukt"@nl ;
  skos:definition "치수 매개 변수를 표현하는 정의된 양"@kr ;
  skos:editorialNote "preferred" ;
  skos:editorialNote "preferred"^^xsd:string ;
  skos:notation "627" ;
  skos:notation 627 ;
  skos:note "Note 1 to entry: In this International Standard, the subtypes of units are length units, angular units, time units, scale units and pixel spacing units."@en ;
  skos:note "OPMERKING In deze Internationale Standaard zijn de subtypen van eenheden de lengte-eenheden, hoekeenheden, tijdeenheden, schaaleenheden en pixelafstandeenheden."@en ;
  skos:note "비고: KS X ISO 19111 표준에서 단위의 하위 유형은 길이 단위, 각 단위, 시간 단위, 척도 단위 및 픽셀 간격 단위이다.  "@kr ;
  skos:prefLabel "eenheid"@nl ;
  skos:prefLabel "unit"@en ;
  skos:prefLabel "단위"@kr ;
.
<http://iso.org/tc211/term/629>
  rdf:type skos:Concept ;
  dcterms:dateAccepted "2007-07-01" ;
  dcterms:dateAccepted "2007-07-01"^^xsd:date ;
  dcterms:dateAccepted "2007-11-01"^^xsd:date ;
  dcterms:provenance "KS X ISO 19111" ;
  dcterms:source "ISO 19111:2007" ;
  reg:status reg:statusAccepted ;
  reg:status reg:statusValid ;
  rdfs:comment "Note 1 to entry: In most cases, the vertical datum will be related to mean sea level. Ellipsoidal heights are treated as related to a three-dimensional ellipsoidal coordinate system referenced to a geodetic datum. Vertical datums include sounding datums (used for hydrographic purposes), in which case the heights may be negative heights or depths."@en ;
  rdfs:comment "OPMERKING In de meeste gevallen is het verticale datum gerelateerd aan het gemiddeldr zeeniveau. Ellipsoïde hoogten worden beschouwd als gerelateerd aan een driedimensionaal coördinaatsysteem wat gerefereerd is ten opzichte van een geodetisch datum. Onder verticale datums vallen bijvoorbeeld hydrografische datums waarbij de hoogten getoond kunen worden als negatieve hoogten of diepten."@en ;
  rdfs:comment "비고: 대부분의 경우, 수직 데이텀은 평균 해수면과 관련된다. 타원체고는 측지 원점을 기준으로 하는 3차원 타원체 좌표계와 관련되는 것으로 간주된다. 수직 데이텀은 수심 데이텀(수로학적인 목적으로 사용됨)을 포함한다. 이 경우 높이는 음(-)의 높이 또는 깊이가 된다."@kr ;
  rdfs:label "vertical datum"@en ;
  skos:changeNote "valid" ;
  skos:definition "datum welke de relatie tussen zwaartekracht gerelateerde hoogten of diepten ten opzichte van de aarde beschrijft"@nl ;
  skos:definition "지구와 중력 높이 또는 깊이와의 관계를 기술하는 데이텀"@kr ;
  skos:editorialNote "preferred" ;
  skos:editorialNote "preferred"^^xsd:string ;
  skos:notation "629" ;
  skos:notation 629 ;
  skos:note "Note 1 to entry: In most cases, the vertical datum will be related to mean sea level. Ellipsoidal heights are treated as related to a three-dimensional ellipsoidal coordinate system referenced to a geodetic datum. Vertical datums include sounding datums (used for hydrographic purposes), in which case the heights may be negative heights or depths."@en ;
  skos:note "OPMERKING In de meeste gevallen is het verticale datum gerelateerd aan het gemiddeldr zeeniveau. Ellipsoïde hoogten worden beschouwd als gerelateerd aan een driedimensionaal coördinaatsysteem wat gerefereerd is ten opzichte van een geodetisch datum. Onder verticale datums vallen bijvoorbeeld hydrografische datums waarbij de hoogten getoond kunen worden als negatieve hoogten of diepten."@en ;
  skos:note "비고: 대부분의 경우, 수직 데이텀은 평균 해수면과 관련된다. 타원체고는 측지 원점을 기준으로 하는 3차원 타원체 좌표계와 관련되는 것으로 간주된다. 수직 데이텀은 수심 데이텀(수로학적인 목적으로 사용됨)을 포함한다. 이 경우 높이는 음(-)의 높이 또는 깊이가 된다."@kr ;
  skos:prefLabel "verticaal datum"@nl ;
  skos:prefLabel "vertical datum"@en ;
  skos:prefLabel "수직 데이텀"@kr ;
.
<http://iso.org/tc211/term/63>
  rdf:type skos:Concept ;
  dcterms:dateAccepted "2005-02-15"^^xsd:date ;
  dcterms:dateAccepted "2009-12-29"^^xsd:date ;
  dcterms:provenance "ISO 19119:2005" ;
  dcterms:provenance "KS X ISO 19119" ;
  dcterms:source "ISO/IEC 10746-3:1996" ;
  reg:status reg:statusValid ;
  rdfs:label "computational viewpoint"@en ;
  skos:changeNote "valid" ;
  skos:definition "시스템을 인터페이스를 통해 상호 작용하는 기능적 객체들로 분해함으로써 분산 처리를 가능하게 하는 개방형 시스템 및 그 환경에 대한 관점"@kr ;
  skos:editorialNote "preferred" ;
  skos:editorialNote "preferred"^^xsd:string ;
  skos:notation "63" ;
  skos:notation 63 ;
  skos:prefLabel "computational viewpoint"@en ;
  skos:prefLabel "계산 관점"@kr ;
.
<http://iso.org/tc211/term/630>
  rdf:type skos:Concept ;
  dcterms:dateAccepted "2007-02-01"^^xsd:date ;
  dcterms:dateAccepted "2007-11-01"^^xsd:date ;
  dcterms:provenance "KS X ISO 19134" ;
  dcterms:source "ISO 19134:2007" ;
  reg:status reg:statusValid ;
  rdfs:label "transportation mode"@en ;
  skos:changeNote "valid" ;
  skos:definition "여행자가 교통을 위해 선택 가능한 수단"@kr ;
  skos:editorialNote "preferred" ;
  skos:editorialNote "preferred"^^xsd:string ;
  skos:notation "630" ;
  skos:notation 630 ;
  skos:prefLabel "transportation mode"@en ;
  skos:prefLabel "교통 수단"@kr ;
.
<http://iso.org/tc211/term/632>
  rdf:type skos:Concept ;
  dcterms:dateAccepted "2006-12-01"^^xsd:date ;
  dcterms:dateAccepted "2007-11-01"^^xsd:date ;
  dcterms:provenance "ISO 19138:2006" ;
  dcterms:source "ISO 19157:2013, 4.7" ;
  reg:status reg:statusValid ;
  rdfs:comment "Note 1 to entry: Data quality basic measures are abstract data types. They cannot be used directly when reporting data quality."@en ;
  rdfs:comment "비고: 데이터 품질 기본척도는 추상 데이터 유형으로 데이터의 품질을 보고할 때 직접적으로 사용될 수 없다."@kr ;
  rdfs:label "data quality basic measure"@en ;
  skos:changeNote "valid" ;
  skos:definition "데이터 품질 측정 값을 생성하는 데 기준으로 사용되는 일반적인 데이터 품질 척도"@kr ;
  skos:editorialNote "preferred" ;
  skos:editorialNote "preferred"^^xsd:string ;
  skos:notation "632" ;
  skos:notation 632 ;
  skos:note "Note 1 to entry: Data quality basic measures are abstract data types. They cannot be used directly when reporting data quality."@en ;
  skos:note "비고: 데이터 품질 기본척도는 추상 데이터 유형으로 데이터의 품질을 보고할 때 직접적으로 사용될 수 없다."@kr ;
  skos:prefLabel "data quality basic measure"@en ;
  skos:prefLabel "데이터 품질 기본 척도"@kr ;
.
<http://iso.org/tc211/term/639>
  rdf:type skos:Concept ;
  dcterms:dateAccepted "2008-06-01"^^xsd:date ;
  dcterms:source "ISO/TS 19101-2:2008" ;
  reg:status reg:statusValid ;
  rdfs:comment "Note 1 to entry: For imagery, resolution refers to radiometric, spectral, spatial and temporal resolutions."@en ;
  rdfs:label "resolution (of a sensor)"@en ;
  skos:changeNote "valid" ;
  skos:editorialNote "preferred"^^xsd:string ;
  skos:notation 639 ;
  skos:note "Note 1 to entry: For imagery, resolution refers to radiometric, spectral, spatial and temporal resolutions."@en ;
  skos:prefLabel "resolution (of a sensor)"@en ;
.
<http://iso.org/tc211/term/64>
  rdf:type skos:Concept ;
  dcterms:dateAccepted "2008-11-15"^^xsd:date ;
  dcterms:provenance "ISO/TS 19104:2008" ;
  dcterms:source "ISO 1087-1:2000" ;
  reg:status reg:statusValid ;
  rdfs:comment "Note 1 to entry: Concepts are not necessarily bound to particular languages.  They are, however, influenced by the social or cultural background which often leads to different categorizations."@en ;
  rdfs:label "concept"@en ;
  skos:changeNote "valid" ;
  skos:editorialNote "preferred"^^xsd:string ;
  skos:notation 64 ;
  skos:note "Note 1 to entry: Concepts are not necessarily bound to particular languages.  They are, however, influenced by the social or cultural background which often leads to different categorizations."@en ;
  skos:prefLabel "concept"@en ;
.
<http://iso.org/tc211/term/640>
  rdf:type skos:Concept ;
  dcterms:dateAccepted "2008-06-01"^^xsd:date ;
  dcterms:provenance "ISO/TS 19101-2:2008" ;
  dcterms:source "ISO 22028-1 (Derived from)" ;
  reg:status reg:statusValid ;
  rdfs:comment "Note 1 to entry: A scene may correspond to a remotely sensed view of the natural world or to a computer-generated virtual scene simulating such a view"@en ;
  rdfs:label "scene"@en ;
  skos:changeNote "valid" ;
  skos:editorialNote "preferred"^^xsd:string ;
  skos:notation 640 ;
  skos:note "Note 1 to entry: A scene may correspond to a remotely sensed view of the natural world or to a computer-generated virtual scene simulating such a view"@en ;
  skos:prefLabel "scene"@en ;
.
<http://iso.org/tc211/term/642>
  rdf:type skos:Concept ;
  dcterms:dateAccepted "2008-06-01"^^xsd:date ;
  dcterms:source "ISO 19141:2008" ;
  reg:status reg:statusValid ;
  rdfs:label "foliation"@en ;
  skos:changeNote "valid" ;
  skos:editorialNote "preferred"^^xsd:string ;
  skos:notation 642 ;
  skos:prefLabel "foliation"@en ;
.
<http://iso.org/tc211/term/643>
  rdf:type skos:Concept ;
  dcterms:dateAccepted "2008-06-01"^^xsd:date ;
  dcterms:source "ISO 19141:2008" ;
  reg:status reg:statusValid ;
  rdfs:label "leaf <one parameter set of geometries>"@en ;
  skos:changeNote "valid" ;
  skos:editorialNote "preferred"^^xsd:string ;
  skos:notation 643 ;
  skos:prefLabel "leaf <one parameter set of geometries>"@en ;
.
<http://iso.org/tc211/term/644>
  rdf:type skos:Concept ;
  dcterms:dateAccepted "2008-06-01"^^xsd:date ;
  dcterms:source "ISO 19141:2008" ;
  reg:status reg:statusValid ;
  rdfs:label "one parameter set of geometries"@en ;
  skos:changeNote "valid" ;
  skos:editorialNote "preferred"^^xsd:string ;
  skos:notation 644 ;
  skos:prefLabel "one parameter set of geometries"@en ;
.
<http://iso.org/tc211/term/645>
  rdf:type skos:Concept ;
  dcterms:dateAccepted "2008-06-01"^^xsd:date ;
  dcterms:source "ISO 19141:2008" ;
  reg:status reg:statusValid ;
  rdfs:comment "Note 1 to entry: This is a generalization of the concept of a geometric prism that is the convex hull of two congruent polygons in 3D-space. Such polyhedrons can be viewed as a foliation of congruent polygons."@en ;
  rdfs:label "prism <one parameter set of geometries>"@en ;
  skos:changeNote "valid" ;
  skos:editorialNote "preferred"^^xsd:string ;
  skos:notation 645 ;
  skos:note "Note 1 to entry: This is a generalization of the concept of a geometric prism that is the convex hull of two congruent polygons in 3D-space. Such polyhedrons can be viewed as a foliation of congruent polygons."@en ;
  skos:prefLabel "prism <one parameter set of geometries>"@en ;
.
<http://iso.org/tc211/term/646>
  rdf:type skos:Concept ;
  dcterms:dateAccepted "2008-06-01"^^xsd:date ;
  dcterms:source "ISO 19141:2008" ;
  reg:status reg:statusValid ;
  rdfs:label "trajectory"@en ;
  skos:changeNote "valid" ;
  skos:editorialNote "preferred"^^xsd:string ;
  skos:notation 646 ;
  skos:prefLabel "trajectory"@en ;
.
<http://iso.org/tc211/term/656>
  rdf:type skos:Concept ;
  dcterms:dateAccepted "2007-10-15"^^xsd:date ;
  dcterms:dateAccepted "2009-12-29"^^xsd:date ;
  dcterms:provenance "KS X ISO 19132" ;
  dcterms:source "ISO 19132:2007" ;
  reg:status reg:statusValid ;
  rdfs:comment "Note 1 to entry: cf. passive object. An active object can represent a user, or an active service that depends on internal (and therefore not visible) triggers to start actions. Active and passive states can exist for the same object, and such a service can transition between these two states depending on invocation of an activation or deactivation operation protocol."@en ;
  rdfs:comment "비고: 활성 객체는 사용자 또는 내부 트리거를 통해 활성화되는(따라서 눈으로 볼 수 없는) 활성 서비스를 나타낼 수 있다. 활성 및 수동 상태는 동일 객체에 대하여 존재할 수 있으며, 이러한 서비스는 활성화 또는 비활성화 연산 프로토콜의 호출을 통해 상태가 변한다."@kr ;
  rdfs:label "active object"@en ;
  skos:changeNote "valid" ;
  skos:definition "독립적인 동작이 가능한 객체, 따라서 별도의 외부 자극 없이도 스스로 다른 객체와의 상호작용이 가능함"@kr ;
  skos:editorialNote "preferred" ;
  skos:editorialNote "preferred"^^xsd:string ;
  skos:notation "656" ;
  skos:notation 656 ;
  skos:note "Note 1 to entry: cf. passive object. An active object can represent a user, or an active service that depends on internal (and therefore not visible) triggers to start actions. Active and passive states can exist for the same object, and such a service can transition between these two states depending on invocation of an activation or deactivation operation protocol."@en ;
  skos:note "비고: 활성 객체는 사용자 또는 내부 트리거를 통해 활성화되는(따라서 눈으로 볼 수 없는) 활성 서비스를 나타낼 수 있다. 활성 및 수동 상태는 동일 객체에 대하여 존재할 수 있으며, 이러한 서비스는 활성화 또는 비활성화 연산 프로토콜의 호출을 통해 상태가 변한다."@kr ;
  skos:prefLabel "active object"@en ;
  skos:prefLabel "활성 객체"@kr ;
.
<http://iso.org/tc211/term/658>
  rdf:type skos:Concept ;
  dcterms:dateAccepted "2007-10-15"^^xsd:date ;
  dcterms:dateAccepted "2009-12-29"^^xsd:date ;
  dcterms:provenance "KS X ISO 19132" ;
  dcterms:source "ISO 19132:2007" ;
  reg:status reg:statusValid ;
  rdfs:comment "Note 1 to entry: cf. interoperate. Basic services lack any persistent, user-specific state information between invocations and are not meant for direct access by users. Because they act in a functional manner, they are readily replaceable at runtime by other services using the same interfaces."@en ;
  rdfs:comment "비고: 기본 서비스는 사용자별 상태 정보와 호출 간의 지속성이 부족하다. 이는 사용자가 기본 서비스에 직접 접근하는 것을 의미하지는 않는다. 기본 서비스는 기능적으로 사용되며, 동일한 인터페이스를 따르는 다른 서비스로 실시간 교체가 가능하다."@kr ;
  rdfs:label "basic service"@en ;
  skos:changeNote "valid" ;
  skos:definition "서비스 또는 응용에 기본 함수를 제공하는 서비스"@kr ;
  skos:editorialNote "preferred" ;
  skos:editorialNote "preferred"^^xsd:string ;
  skos:notation "658" ;
  skos:notation 658 ;
  skos:note "Note 1 to entry: cf. interoperate. Basic services lack any persistent, user-specific state information between invocations and are not meant for direct access by users. Because they act in a functional manner, they are readily replaceable at runtime by other services using the same interfaces."@en ;
  skos:note "비고: 기본 서비스는 사용자별 상태 정보와 호출 간의 지속성이 부족하다. 이는 사용자가 기본 서비스에 직접 접근하는 것을 의미하지는 않는다. 기본 서비스는 기능적으로 사용되며, 동일한 인터페이스를 따르는 다른 서비스로 실시간 교체가 가능하다."@kr ;
  skos:prefLabel "basic service"@en ;
  skos:prefLabel "기본 서비스"@kr ;
.
<http://iso.org/tc211/term/659>
  rdf:type skos:Concept ;
  dcterms:dateAccepted "2007-10-15"^^xsd:date ;
  dcterms:dateAccepted "2009-12-29"^^xsd:date ;
  dcterms:provenance "KS X ISO 19132" ;
  dcterms:source "ISO 19132:2007" ;
  reg:status reg:statusValid ;
  rdfs:comment "Note 1 to entry: The interpolation of continuous change is usually done by taking into consideration constraints on the \"curve\" joining the two data points (time1, value1) and (time2, value2), looking at the value as a function of time. For example, if the continuous change is for the motion of a vehicle, then the constraints of physics and of the paths appropriate for that vehicle must be taken into consideration."@en ;
  rdfs:comment "비고: 연속 변환의 보간법은 일반적으로 \"곡선\"상 두 개의 데이터 점((시간1,값1), (시간2,값2))과 시간 함수 값을 제약 조건으로 사용한다. 예를 들어, 차량의 이동에 대한 연속 변환의 경우 반드시 제약 조건으로 물리학과 도로 상태를 고려해야 한다."@kr ;
  rdfs:label "continuous change"@en ;
  skos:changeNote "valid" ;
  skos:definition "속성이 거리 관측 유형인 변환에서 속성의 값은 알려진 두 측정 간의 매개 값을 사용한 것으로 가정할 수 있다."@kr ;
  skos:editorialNote "preferred" ;
  skos:editorialNote "preferred"^^xsd:string ;
  skos:notation "659" ;
  skos:notation 659 ;
  skos:note "Note 1 to entry: The interpolation of continuous change is usually done by taking into consideration constraints on the \"curve\" joining the two data points (time1, value1) and (time2, value2), looking at the value as a function of time. For example, if the continuous change is for the motion of a vehicle, then the constraints of physics and of the paths appropriate for that vehicle must be taken into consideration."@en ;
  skos:note "비고: 연속 변환의 보간법은 일반적으로 \"곡선\"상 두 개의 데이터 점((시간1,값1), (시간2,값2))과 시간 함수 값을 제약 조건으로 사용한다. 예를 들어, 차량의 이동에 대한 연속 변환의 경우 반드시 제약 조건으로 물리학과 도로 상태를 고려해야 한다."@kr ;
  skos:prefLabel "continuous change"@en ;
  skos:prefLabel "연속 변환"@kr ;
.
<http://iso.org/tc211/term/66>
  rdf:type skos:Concept ;
  dcterms:dateAccepted "2008-11-15"^^xsd:date ;
  dcterms:provenance "ISO/TS 19104:2008" ;
  dcterms:source "ISO 1087-1:2000" ;
  reg:status reg:statusValid ;
  rdfs:label "concept system"@en ;
  skos:changeNote "valid" ;
  skos:editorialNote "preferred"^^xsd:string ;
  skos:notation 66 ;
  skos:prefLabel "concept system"@en ;
.
<http://iso.org/tc211/term/660>
  rdf:type skos:Concept ;
  dcterms:dateAccepted "2007-10-15"^^xsd:date ;
  dcterms:dateAccepted "2009-12-29"^^xsd:date ;
  dcterms:provenance "KS X ISO 19132" ;
  dcterms:source "ISO 19132:2007" ;
  reg:status reg:statusValid ;
  rdfs:comment "Note 1 to entry:: Compare with integration. While the conceptual schema of the information transferred shall be agreed upon to some level, coupling applications can be and are usually flexible in the data representation of that information as long as the semantics content is correct and mappable to some canonical representation of the conceptual schema. The most common mapping technology used for XML messages is XSLT, and the transformation stylesheet can be supplied either by the service broker or by the service provider. It is considered a best practice for a service provider to supply his functionality through several logically equivalent messaging APIs, each represented by a different URI linked to an XSLT transformation bridge, and implemented by the same internal code."@en ;
  rdfs:comment "Note 2 to entry:: Loose coupling and tight coupling are not at present well-defined terms in the literature. Generally, \"tight\" coupling means that there is some sort of incurred dependency between requester and responder in the use of the interface, while \"loose\" means no such dependency. The nature of that dependency is not consistently defined between authors.  In that light, \"tight\" coupling or \"tight\" integration are both bad practices, and have been viewed as such since the inception of the terms. Some literature refers to integration as \"tight coupling\", but that is a less accurate description." ;
  rdfs:comment "비고 1: 통합과 비교하라. 전송된 정보의 개념적 스키마는 일정 수준 일치할 수 있으나, 결합 응용은 일반적으로 의미론적 내용이 정확하며 개념적 스키마의 정규 표현과 매핑 가능한 정보를 표현하는 데이터에서 유연하게 사용된다. 가장 일반적인 매핑 기술로 사용되는 XML 메시지는 XSLT이며, 변환 스타일시트는 서비스 브로커 또는 서비스 제공자에 의해 공급될 수 있다. 서비스 제공자는 논리적으로 대응하는 다양한 메시징 API를 통해 그 기능을 제공하고, XSLT 변환 브리지에 링크된 각기 다른 URI에 의한 표현을 고려하며, 동일한 내부 코드를 통해 구현되도록 한다."@kr ;
  rdfs:label "coupling"@en ;
  skos:changeNote "valid" ;
  skos:definition "두 개 이상의 시스템 간 정보의 전송 또는 메시징을 통한 연계"@kr ;
  skos:editorialNote "preferred" ;
  skos:editorialNote "preferred"^^xsd:string ;
  skos:notation "660" ;
  skos:notation 660 ;
  skos:note "Note 1 to entry:: Compare with integration. While the conceptual schema of the information transferred shall be agreed upon to some level, coupling applications can be and are usually flexible in the data representation of that information as long as the semantics content is correct and mappable to some canonical representation of the conceptual schema. The most common mapping technology used for XML messages is XSLT, and the transformation stylesheet can be supplied either by the service broker or by the service provider. It is considered a best practice for a service provider to supply his functionality through several logically equivalent messaging APIs, each represented by a different URI linked to an XSLT transformation bridge, and implemented by the same internal code."@en ;
  skos:note "Note 2 to entry:: Loose coupling and tight coupling are not at present well-defined terms in the literature. Generally, \"tight\" coupling means that there is some sort of incurred dependency between requester and responder in the use of the interface, while \"loose\" means no such dependency. The nature of that dependency is not consistently defined between authors.  In that light, \"tight\" coupling or \"tight\" integration are both bad practices, and have been viewed as such since the inception of the terms. Some literature refers to integration as \"tight coupling\", but that is a less accurate description."^^<http://www.w3.org/2001/XMLSchema#@en> ;
  skos:note "비고 1: 통합과 비교하라. 전송된 정보의 개념적 스키마는 일정 수준 일치할 수 있으나, 결합 응용은 일반적으로 의미론적 내용이 정확하며 개념적 스키마의 정규 표현과 매핑 가능한 정보를 표현하는 데이터에서 유연하게 사용된다. 가장 일반적인 매핑 기술로 사용되는 XML 메시지는 XSLT이며, 변환 스타일시트는 서비스 브로커 또는 서비스 제공자에 의해 공급될 수 있다. 서비스 제공자는 논리적으로 대응하는 다양한 메시징 API를 통해 그 기능을 제공하고, XSLT 변환 브리지에 링크된 각기 다른 URI에 의한 표현을 고려하며, 동일한 내부 코드를 통해 구현되도록 한다."@kr ;
  skos:note "비고 2: 약결합과 강결합은 현재 잘 정의된 용어는 아니다. 일반적으로 \"강\" 결합이란,  인터페이스의 활용에서 요청자와 응답자 간에 발생하는 의존도를 의미한다. 반면 \"약\"결합은 이와 같은 의존도가 없음을 의미한다. 의존도의 본질은 개발자 간에 일관성 있게 정의되지 않고 있다. 이런 맥락에서 \"강\" 결합 또는 \"강\" 통합은 좋지 않은 예시로써, 용어가 생긴 이래로 계속 검토되고 있다. 어떤 문헌에서는 \"강결합\"으로 통합을 참조하고 있으나, 다소 정확하지 않게 기술되어 있다. "@kr ;
  skos:prefLabel "coupling"@en ;
  skos:prefLabel "결합"@kr ;
.
<http://iso.org/tc211/term/661>
  rdf:type skos:Concept ;
  dcterms:dateAccepted "2005-10-17"^^xsd:date ;
  dcterms:dateAccepted "2007-11-29"^^xsd:date ;
  dcterms:provenance "ISO 19132:2007" ;
  dcterms:provenance "KS X ISO/IEC TR 21000-1" ;
  dcterms:source "ISO/IEC TR 21000-1:2004" ;
  reg:status reg:statusValid ;
  rdfs:label "digital item"@en ;
  skos:changeNote "valid" ;
  skos:definition "표준화된 표현, 식별, 메타데이터 프레임워크를 갖는 구조화된 디지털 객체[자산, 일, 서비스, 데이터 또는 정보]"@kr ;
  skos:editorialNote "preferred" ;
  skos:editorialNote "preferred"^^xsd:string ;
  skos:notation "661" ;
  skos:notation 661 ;
  skos:prefLabel "digital item"@en ;
  skos:prefLabel "디지털 항목"@kr ;
.
<http://iso.org/tc211/term/662>
  rdf:type skos:Concept ;
  dcterms:dateAccepted "2007-10-15"^^xsd:date ;
  dcterms:dateAccepted "2009-12-29"^^xsd:date ;
  dcterms:provenance "KS X ISO 19132" ;
  dcterms:source "ISO 19132:2007" ;
  reg:status reg:statusValid ;
  rdfs:comment "Note 1 to entry: Legal changes of parcel changes are discrete, having occurred at a specific time."@en ;
  rdfs:comment "비고: 토지 필지의 법적인 변동은 불연속적이며, 특정한 시각에 발생한 경우이다. "@kr ;
  rdfs:label "discrete change"@en ;
  skos:changeNote "valid" ;
  skos:definition "두 개의 알려진 측정값 사이에 어떠한 값도 취하지 않는 속성 값의 변화"@kr ;
  skos:editorialNote "preferred" ;
  skos:editorialNote "preferred"^^xsd:string ;
  skos:notation "662" ;
  skos:notation 662 ;
  skos:note "Note 1 to entry: Legal changes of parcel changes are discrete, having occurred at a specific time."@en ;
  skos:note "비고: 토지 필지의 법적인 변동은 불연속적이며, 특정한 시각에 발생한 경우이다. "@kr ;
  skos:prefLabel "discrete change"@en ;
  skos:prefLabel "불연속 변환"@kr ;
.
<http://iso.org/tc211/term/663>
  rdf:type skos:Concept ;
  dcterms:dateAccepted "2007-10-15"^^xsd:date ;
  dcterms:dateAccepted "2009-12-29"^^xsd:date ;
  dcterms:provenance "KS X ISO 19132" ;
  dcterms:source "ISO 19132:2007" ;
  reg:status reg:statusValid ;
  rdfs:comment "Note 1 to entry:: See Theodoridis - 1999"@en ;
  rdfs:comment "비고: Theodoridis(1999)를 참조하라."@kr ;
  rdfs:label "discrete spatiotemporal object"@en ;
  skos:changeNote "valid" ;
  skos:definition "상이한 시간에 동일한 공간피처를 시간에 따라 기술한 시간연속객체"@kr ;
  skos:editorialNote "preferred" ;
  skos:editorialNote "preferred"^^xsd:string ;
  skos:notation "663" ;
  skos:notation 663 ;
  skos:note "Note 1 to entry:: See Theodoridis - 1999"@en ;
  skos:note "비고: Theodoridis(1999)를 참조하라."@kr ;
  skos:prefLabel "discrete spatiotemporal object"@en ;
  skos:prefLabel "불연속 시공간객체"@kr ;
.
<http://iso.org/tc211/term/664>
  rdf:type skos:Concept ;
  dcterms:dateAccepted "2007-10-15"^^xsd:date ;
  dcterms:dateAccepted "2009-12-29"^^xsd:date ;
  dcterms:provenance "KS X ISO 19132" ;
  dcterms:source "ISO 19132:2007" ;
  reg:status reg:statusValid ;
  rdfs:comment "Note 1 to entry: A measure \"d\" is positive if d(x, y) > 0 for every x, y where x/=y and d(x,x) = 0. A measure \"d\" is symmetric if d(x, y) = d(y, x)  for every x, y. A measure \"d\" satisfies the triangular inequality if d(x, y) <= d(x, a) + d(a, y) for every a, x and y. All numeric or vector valued attributes have such a metric, the most common being the Euclidean metric based on the square root of the sum of the squares of the differences in each dimension. Other non-Euclidean metrics take \"curvature of space\" into account (such as along the surface of the spheroid)."@en ;
  rdfs:comment "비고: 만일 x≠y이고 d(x,x)=0인 모든 x,y에 대해 d(x,y) > 0 이면 측정 값 \"d\"는 양수이다. 모든 x,y에 대해 d(x,y) = d(y,x) 이면 측정 값 \"d\"는 대칭이다. 만일 모든 a, x, y 에 대하여 d(x,y) ≤ d(x,a) + d(a,y) 이면 측정 값 \"d\"는 삼각형의 부등식을 만족시킨다. 미터법과 같이 모든 숫자 또는 백터 값을 갖는 속성은 각 차원의 차이 값의 제곱의 합에 대한 제곱근을 기초로 한 가장 일반적인 유클리디안 계량법이다. 다른 비유클리디안 계량법에서는 \"공간의 곡률\"(회전 타원체의 표면을 따르는)을 고려한다. "@kr ;
  rdfs:label "distance measure"@en ;
  rdfs:seeAlso "distance metric" ;
  skos:altLabel "distance metric"@en ;
  skos:changeNote "valid" ;
  skos:definition "속성 유형은 양수이고, 대칭이며 삼각형의 부등식을 만족시키는 거리 값"@kr ;
  skos:editorialNote "preferred" ;
  skos:editorialNote "preferred"^^xsd:string ;
  skos:notation "664" ;
  skos:notation 664 ;
  skos:note "Note 1 to entry: A measure \"d\" is positive if d(x, y) > 0 for every x, y where x/=y and d(x,x) = 0. A measure \"d\" is symmetric if d(x, y) = d(y, x)  for every x, y. A measure \"d\" satisfies the triangular inequality if d(x, y) <= d(x, a) + d(a, y) for every a, x and y. All numeric or vector valued attributes have such a metric, the most common being the Euclidean metric based on the square root of the sum of the squares of the differences in each dimension. Other non-Euclidean metrics take \"curvature of space\" into account (such as along the surface of the spheroid)."@en ;
  skos:note "비고: 만일 x≠y이고 d(x,x)=0인 모든 x,y에 대해 d(x,y) > 0 이면 측정 값 \"d\"는 양수이다. 모든 x,y에 대해 d(x,y) = d(y,x) 이면 측정 값 \"d\"는 대칭이다. 만일 모든 a, x, y 에 대하여 d(x,y) ≤ d(x,a) + d(a,y) 이면 측정 값 \"d\"는 삼각형의 부등식을 만족시킨다. 미터법과 같이 모든 숫자 또는 백터 값을 갖는 속성은 각 차원의 차이 값의 제곱의 합에 대한 제곱근을 기초로 한 가장 일반적인 유클리디안 계량법이다. 다른 비유클리디안 계량법에서는 \"공간의 곡률\"(회전 타원체의 표면을 따르는)을 고려한다. "@kr ;
  skos:prefLabel "distance measure"@en ;
  skos:prefLabel "거리 관측"@kr ;
.
<http://iso.org/tc211/term/665>
  rdf:type skos:Concept ;
  dcterms:dateAccepted "2007-10-15"^^xsd:date ;
  dcterms:dateAccepted "2009-12-29"^^xsd:date ;
  dcterms:provenance "KS X ISO 19132" ;
  dcterms:source "ISO 19132:2007" ;
  reg:status reg:statusValid ;
  rdfs:comment "Note 1 to entry: A measure \"d\" is positive if d(x, y) > 0 for every x, y where x/=y and d(x,x) = 0. A measure \"d\" is symmetric if d(x, y) = d(y, x)  for every x, y. A measure \"d\" satisfies the triangular inequality if d(x, y) <= d(x, a) + d(a, y) for every a, x and y. All numeric or vector valued attributes have such a metric, the most common being the Euclidean metric based on the square root of the sum of the squares of the differences in each dimension. Other non-Euclidean metrics take \"curvature of space\" into account (such as along the surface of the spheroid)."@en ;
  rdfs:comment "비고: 만일 x≠y이고 d(x,x)=0인 모든 x,y에 대해 d(x,y) > 0 이면 측정 값 \"d\"는 양수이다. 모든 x,y에 대해 d(x,y) = d(y,x) 이면 측정 값 \"d\"는 대칭이다. 만일 모든 a, x, y 에 대하여 d(x,y) ≤ d(x,a) + d(a,y) 이면 측정 값 \"d\"는 삼각형의 부등식을 만족시킨다. 미터법과 같이 모든 숫자 또는 백터 값을 갖는 속성은 각 차원의 차이 값의 제곱의 합에 대한 제곱근을 기초로 한 가장 일반적인 유클리디안 계량법이다. 다른 비유클리디안 계량법에서는 \"공간의 곡률\"(회전 타원체의 표면을 따르는)을 고려한다. "@kr ;
  rdfs:label "distance metric"@en ;
  rdfs:seeAlso "distance measure" ;
  skos:altLabel "distance measure"@en ;
  skos:changeNote "valid" ;
  skos:definition "속성 유형은 양수이고, 대칭이며 삼각형의 부등식을 만족시키는 거리 값"@kr ;
  skos:editorialNote "admitted" ;
  skos:editorialNote "admitted"^^xsd:string ;
  skos:notation "665" ;
  skos:notation 665 ;
  skos:note "Note 1 to entry: A measure \"d\" is positive if d(x, y) > 0 for every x, y where x/=y and d(x,x) = 0. A measure \"d\" is symmetric if d(x, y) = d(y, x)  for every x, y. A measure \"d\" satisfies the triangular inequality if d(x, y) <= d(x, a) + d(a, y) for every a, x and y. All numeric or vector valued attributes have such a metric, the most common being the Euclidean metric based on the square root of the sum of the squares of the differences in each dimension. Other non-Euclidean metrics take \"curvature of space\" into account (such as along the surface of the spheroid)."@en ;
  skos:note "비고: 만일 x≠y이고 d(x,x)=0인 모든 x,y에 대해 d(x,y) > 0 이면 측정 값 \"d\"는 양수이다. 모든 x,y에 대해 d(x,y) = d(y,x) 이면 측정 값 \"d\"는 대칭이다. 만일 모든 a, x, y 에 대하여 d(x,y) ≤ d(x,a) + d(a,y) 이면 측정 값 \"d\"는 삼각형의 부등식을 만족시킨다. 미터법과 같이 모든 숫자 또는 백터 값을 갖는 속성은 각 차원의 차이 값의 제곱의 합에 대한 제곱근을 기초로 한 가장 일반적인 유클리디안 계량법이다. 다른 비유클리디안 계량법에서는 \"공간의 곡률\"(회전 타원체의 표면을 따르는)을 고려한다. "@kr ;
  skos:prefLabel "distance metric"@en ;
  skos:prefLabel "거리 관측"@kr ;
.
<http://iso.org/tc211/term/667>
  rdf:type skos:Concept ;
  dcterms:dateAccepted "2007-10-15"^^xsd:date ;
  dcterms:dateAccepted "2009-12-29"^^xsd:date ;
  dcterms:provenance "KS X ISO 19132" ;
  dcterms:source "ISO 19132:2007" ;
  reg:status reg:statusValid ;
  rdfs:comment "Note 1 to entry: An identity is usually a persistent and constant key member attribute value of the object. Since it is temporally constant and unique, it will be the same in any state associated to the object regardless of its timestamp. A moving object's identity is independent of both time and location."@en ;
  rdfs:comment "비고: 불변하는 객체의 키 속성 값을 일반적으로 식별 특성이라 한다. 이는 시간적으로 불변하고 유일하기 때문에 어떤 상태에서도 동일하며, 타임 스탬프에 무관하게 객체에 결합될 수 있다. 이동 객체의 식별 특성은 시간과 위치 모두에 무관하다."@kr ;
  rdfs:label "identity"@en ;
  skos:changeNote "valid" ;
  skos:definition "자체 상태와 무관하게 객체 식별에 충분한 데이터"@kr ;
  skos:editorialNote "preferred" ;
  skos:editorialNote "preferred"^^xsd:string ;
  skos:notation "667" ;
  skos:notation 667 ;
  skos:note "Note 1 to entry: An identity is usually a persistent and constant key member attribute value of the object. Since it is temporally constant and unique, it will be the same in any state associated to the object regardless of its timestamp. A moving object's identity is independent of both time and location."@en ;
  skos:note "비고: 불변하는 객체의 키 속성 값을 일반적으로 식별 특성이라 한다. 이는 시간적으로 불변하고 유일하기 때문에 어떤 상태에서도 동일하며, 타임 스탬프에 무관하게 객체에 결합될 수 있다. 이동 객체의 식별 특성은 시간과 위치 모두에 무관하다."@kr ;
  skos:prefLabel "identity"@en ;
  skos:prefLabel "식별 특성"@kr ;
.
<http://iso.org/tc211/term/668>
  rdf:type skos:Concept ;
  dcterms:dateAccepted "2007-10-15"^^xsd:date ;
  dcterms:dateAccepted "2009-12-29"^^xsd:date ;
  dcterms:provenance "KS X ISO 19132" ;
  dcterms:source "ISO 19132:2007" ;
  reg:status reg:statusValid ;
  rdfs:comment "Note 1 to entry: cf. coupling. Integration and coupling are the two major mechanisms for the interoperation of systems."@en ;
  rdfs:comment "비고: 통합과 결합은 시스템의 상호 운용을 위한 2가지 주요 메커니즘이다."@kr ;
  rdfs:label "integration"@en ;
  skos:changeNote "valid" ;
  skos:definition "공통의 데이터 및 방법을 사용한 둘 이상의 시스템 연계('결합' 참고)"@kr ;
  skos:editorialNote "preferred" ;
  skos:editorialNote "preferred"^^xsd:string ;
  skos:notation "668" ;
  skos:notation 668 ;
  skos:note "Note 1 to entry: cf. coupling. Integration and coupling are the two major mechanisms for the interoperation of systems."@en ;
  skos:note "비고: 통합과 결합은 시스템의 상호 운용을 위한 2가지 주요 메커니즘이다."@kr ;
  skos:prefLabel "integration"@en ;
  skos:prefLabel "통합"@kr ;
.
<http://iso.org/tc211/term/669>
  rdf:type skos:Concept ;
  dcterms:dateAccepted "2007-10-15"^^xsd:date ;
  dcterms:dateAccepted "2009-12-29"^^xsd:date ;
  dcterms:provenance "KS X ISO 19132" ;
  dcterms:source "ISO 19132:2007" ;
  reg:status reg:statusValid ;
  rdfs:comment "Note 1 to entry: cf. interoperability"@en ;
  rdfs:comment "비고: '상호 운용성' 참고"@kr ;
  rdfs:label "interoperate"@en ;
  skos:changeNote "valid" ;
  skos:definition "사용자가 기능적 구성 단위들의 고유 특성을 알지 못해도, 다양한 구성 단위 간의 데이터 전송, 프로그램을 실행, 의사소통"@kr ;
  skos:editorialNote "preferred" ;
  skos:editorialNote "preferred"^^xsd:string ;
  skos:notation "669" ;
  skos:notation 669 ;
  skos:note "Note 1 to entry: cf. interoperability"@en ;
  skos:note "비고: '상호 운용성' 참고"@kr ;
  skos:prefLabel "interoperate"@en ;
  skos:prefLabel "상호운용"@kr ;
.
<http://iso.org/tc211/term/67>
  rdf:type skos:Concept ;
  dcterms:dateAccepted "2002-07-01"^^xsd:date ;
  dcterms:dateAccepted "2008-12-30"^^xsd:date ;
  dcterms:provenance "ISO 19101:2002" ;
  dcterms:source "ISO 19101-1:2014, 4.1.4" ;
  reg:status reg:statusValid ;
  rdfs:comment "Note 1 to entry: One conceptual formalism can be expressed in several conceptual schema languages."@en ;
  rdfs:comment "비고: 한 개의 개념 형식은 복수의 개념적 스키마 언어로 표현될 수 있다."@kr ;
  rdfs:label "conceptual formalism"@en ;
  skos:changeNote "valid" ;
  skos:definition "개념적 모델을 기술하기 위해 사용된 모델링 개념의 집합"@kr ;
  skos:editorialNote "preferred" ;
  skos:editorialNote "preferred"^^xsd:string ;
  skos:notation "67" ;
  skos:notation 67 ;
  skos:note "Note 1 to entry: One conceptual formalism can be expressed in several conceptual schema languages."@en ;
  skos:note "비고: 한 개의 개념 형식은 복수의 개념적 스키마 언어로 표현될 수 있다."@kr ;
  skos:prefLabel "conceptual formalism"@en ;
  skos:prefLabel "개념적 형식"@kr ;
.
<http://iso.org/tc211/term/670>
  rdf:type skos:Concept ;
  dcterms:dateAccepted "2007-10-15"^^xsd:date ;
  dcterms:dateAccepted "2009-12-29"^^xsd:date ;
  dcterms:provenance "KS X ISO 19132" ;
  dcterms:source "ISO 19132:2007" ;
  reg:status reg:statusValid ;
  rdfs:label "license"@en ;
  skos:changeNote "valid" ;
  skos:definition "불법이 아닌 권리를 행사하는 법적 권한으로, 시스템 관계자에게 허가된 승인 또는 승인의 증명"@kr ;
  skos:editorialNote "preferred" ;
  skos:editorialNote "preferred"^^xsd:string ;
  skos:notation "670" ;
  skos:notation 670 ;
  skos:prefLabel "license"@en ;
  skos:prefLabel "라이선스"@kr ;
.
<http://iso.org/tc211/term/672>
  rdf:type skos:Concept ;
  dcterms:dateAccepted "2007-10-15"^^xsd:date ;
  dcterms:dateAccepted "2009-12-29"^^xsd:date ;
  dcterms:provenance "KS X ISO 19132" ;
  dcterms:source "ISO 19132:2007" ;
  reg:status reg:statusValid ;
  rdfs:comment "Note 1 to entry: cf. coupling"@en ;
  rdfs:comment "비고: '결합' 참고"@kr ;
  rdfs:label "loosely coupled interface"@en ;
  skos:changeNote "valid" ;
  skos:definition "공통 분류 정의를 바탕으로 하며, 메시지 포맷 명세와 표현 그리고 서비스의 내부 구현과 무관한 메시지 기반의 서비스 인터페이스"@kr ;
  skos:editorialNote "preferred" ;
  skos:editorialNote "preferred"^^xsd:string ;
  skos:notation "672" ;
  skos:notation 672 ;
  skos:note "Note 1 to entry: cf. coupling"@en ;
  skos:note "비고: '결합' 참고"@kr ;
  skos:prefLabel "loosely coupled interface"@en ;
  skos:prefLabel "약결합 인터페이스"@kr ;
.
<http://iso.org/tc211/term/677>
  rdf:type skos:Concept ;
  dcterms:dateAccepted "2007-10-15"^^xsd:date ;
  dcterms:dateAccepted "2009-12-29"^^xsd:date ;
  dcterms:provenance "KS X ISO 19132" ;
  dcterms:source "ISO 19132:2007" ;
  reg:status reg:statusValid ;
  rdfs:comment "Note 1 to entry:: A passive object is usually accessed through an external interface, through which it receives requests, processes those requests and returns data as a response to that request. Since objects can implement more than one type, it is possible for a single object to pass through active and passive states. For example, a tracking service can lie dormant until a tracking request activates a period where the internals of the object initiate tracking activities based on internal triggers as specified within the request. When the tracking request is deactivated, the object may return to a passive state."@en ;
  rdfs:comment "비고: 보통 수동 객체는 외부 인터페이스를 통해 접근할 수 있으며, 요청을 받게 되면 이를 처리하고, 응답 데이터를 반환한다. 객체가 하나 이상의 유형을 갖기 때문에 하나의 객체가 능동 또는 수동 상태를 가질 수 있다. 예를 들면, 특정 요청에 따라 내부 트리거를 기반으로 추적 활동을 시작하는 객체의 경우, 추적 서비스는 추적 요청이 활성화된 기간동안 수면 상태에 놓일 수 있으며, 추적 요청이 해제되면, 객체는 수동 상태로 되돌아갈 수 있다."@kr ;
  rdfs:label "passive object"@en ;
  skos:changeNote "valid" ;
  skos:definition "외부 자극에만 반응할 수 있으며, 자체적으로 활동하지 못하는 객체"@kr ;
  skos:editorialNote "preferred" ;
  skos:editorialNote "preferred"^^xsd:string ;
  skos:notation "677" ;
  skos:notation 677 ;
  skos:note "Note 1 to entry:: A passive object is usually accessed through an external interface, through which it receives requests, processes those requests and returns data as a response to that request. Since objects can implement more than one type, it is possible for a single object to pass through active and passive states. For example, a tracking service can lie dormant until a tracking request activates a period where the internals of the object initiate tracking activities based on internal triggers as specified within the request. When the tracking request is deactivated, the object may return to a passive state."@en ;
  skos:note "비고: 보통 수동 객체는 외부 인터페이스를 통해 접근할 수 있으며, 요청을 받게 되면 이를 처리하고, 응답 데이터를 반환한다. 객체가 하나 이상의 유형을 갖기 때문에 하나의 객체가 능동 또는 수동 상태를 가질 수 있다. 예를 들면, 특정 요청에 따라 내부 트리거를 기반으로 추적 활동을 시작하는 객체의 경우, 추적 서비스는 추적 요청이 활성화된 기간동안 수면 상태에 놓일 수 있으며, 추적 요청이 해제되면, 객체는 수동 상태로 되돌아갈 수 있다."@kr ;
  skos:prefLabel "passive object"@en ;
  skos:prefLabel "수동 객체"@kr ;
.
<http://iso.org/tc211/term/678>
  rdf:type skos:Concept ;
  dcterms:dateAccepted "2007-10-15"^^xsd:date ;
  dcterms:dateAccepted "2009-12-29"^^xsd:date ;
  dcterms:provenance "KS X ISO 19132" ;
  dcterms:source "ISO 19132:2007" ;
  reg:status reg:statusValid ;
  rdfs:label "passive tracking"@en ;
  skos:changeNote "valid" ;
  skos:definition "차량 또는 여행자의 추적 장치가 정해진 위치의 외부 센서 범위를 통과할 때, 차량 또는 여행자의 위치 측정이 가능하도록 외부에 설치한 고정 센서에 따른 추적"@kr ;
  skos:editorialNote "preferred" ;
  skos:editorialNote "preferred"^^xsd:string ;
  skos:notation "678" ;
  skos:notation 678 ;
  skos:prefLabel "passive tracking"@en ;
  skos:prefLabel "수동 추적"@kr ;
.
<http://iso.org/tc211/term/679>
  rdf:type skos:Concept ;
  dcterms:dateAccepted "2007-10-15"^^xsd:date ;
  dcterms:dateAccepted "2009-12-29"^^xsd:date ;
  dcterms:provenance "KS X ISO 19132" ;
  dcterms:source "ISO 19132:2007" ;
  reg:status reg:statusValid ;
  rdfs:label "resource (ICT)"@en ;
  skos:changeNote "valid" ;
  skos:definition "시스템 관계자를 통해 제어되는 디지털 항목"@kr ;
  skos:editorialNote "preferred" ;
  skos:editorialNote "preferred"^^xsd:string ;
  skos:notation "679" ;
  skos:notation 679 ;
  skos:prefLabel "resource (ICT)"@en ;
  skos:prefLabel "자원 <ICT>"@kr ;
.
<http://iso.org/tc211/term/68>
  rdf:type skos:Concept ;
  dcterms:dateAccepted "2002-07-01"^^xsd:date ;
  dcterms:dateAccepted "2008-12-30"^^xsd:date ;
  dcterms:provenance "ISO 19101:2002" ;
  dcterms:source "ISO 19101-1:2014, 4.1.5" ;
  reg:status reg:statusValid ;
  rdfs:label "conceptual model"@en ;
  skos:changeNote "valid" ;
  skos:definition "논의의 영역의 개념을 정의한 모델"@kr ;
  skos:editorialNote "preferred" ;
  skos:editorialNote "preferred"^^xsd:string ;
  skos:notation "68" ;
  skos:notation 68 ;
  skos:prefLabel "conceptual model"@en ;
  skos:prefLabel "개념적 모델"@kr ;
.
<http://iso.org/tc211/term/680>
  rdf:type skos:Concept ;
  dcterms:dateAccepted "2007-10-15"^^xsd:date ;
  dcterms:dateAccepted "2009-12-29"^^xsd:date ;
  dcterms:provenance "KS X ISO 19132" ;
  dcterms:source "ISO 19132:2007" ;
  reg:status reg:statusValid ;
  rdfs:label "right"@en ;
  skos:changeNote "valid" ;
  skos:definition "시스템 관계자가 관련 자원을 운용하거나 사용할 수 있는 행위, 활동 또는 행위의 클래스"@kr ;
  skos:editorialNote "preferred" ;
  skos:editorialNote "preferred"^^xsd:string ;
  skos:notation "680" ;
  skos:notation 680 ;
  skos:prefLabel "right"@en ;
  skos:prefLabel "권한"@kr ;
.
<http://iso.org/tc211/term/681>
  rdf:type skos:Concept ;
  dcterms:dateAccepted "2007-10-15"^^xsd:date ;
  dcterms:dateAccepted "2009-12-29"^^xsd:date ;
  dcterms:provenance "KS X ISO 19132" ;
  dcterms:source "ISO 19132:2007" ;
  reg:status reg:statusValid ;
  rdfs:label "rights management"@en ;
  skos:changeNote "valid" ;
  skos:definition "시스템 관계자에게 허가된 권한(B.379)의 제어, 관리, 할당 및 추적"@kr ;
  skos:editorialNote "preferred" ;
  skos:editorialNote "preferred"^^xsd:string ;
  skos:notation "681" ;
  skos:notation 681 ;
  skos:prefLabel "rights management"@en ;
  skos:prefLabel "권한 관리"@kr ;
.
<http://iso.org/tc211/term/683>
  rdf:type skos:Concept ;
  dcterms:dateAccepted "2007-10-15"^^xsd:date ;
  dcterms:dateAccepted "2009-12-29"^^xsd:date ;
  dcterms:provenance "KS X ISO 19132" ;
  dcterms:source "ISO 19132:2007" ;
  reg:status reg:statusValid ;
  rdfs:label "service broker"@en ;
  skos:changeNote "valid" ;
  skos:definition "특정 사용자 요구 사항에 대하여 하위 수준의 서비스를 결합하거나 제공하는 응용"@kr ;
  skos:editorialNote "preferred" ;
  skos:editorialNote "preferred"^^xsd:string ;
  skos:notation "683" ;
  skos:notation 683 ;
  skos:prefLabel "service broker"@en ;
  skos:prefLabel "서비스 브로커"@kr ;
.
<http://iso.org/tc211/term/684>
  rdf:type skos:Concept ;
  dcterms:dateAccepted "2007-10-15"^^xsd:date ;
  dcterms:dateAccepted "2009-12-29"^^xsd:date ;
  dcterms:provenance "KS X ISO 19132" ;
  dcterms:source "ISO 19132:2007" ;
  reg:status reg:statusValid ;
  rdfs:comment "Note 1 to entry: The most common SOAs in use today are Web services (using SOAP, UDDI, and WSDL), CORBA and DCOM."@en ;
  rdfs:comment "비고: 최근 가장 일반적인 SOA는 웹서비스(SOAP, UDDI 및 WSDL 사용)와 CORBA, DCOM 이다."@kr ;
  rdfs:label "service oriented architecture"@en ;
  skos:altLabel "SOA"@kr ;
  skos:altLabel "SOA"^^<http://www.w3.org/2001/XMLSchema#@en> ;
  skos:changeNote "valid" ;
  skos:definition "결합된 서비스로 구성된 소프트웨어 구조"@kr ;
  skos:editorialNote "preferred" ;
  skos:editorialNote "preferred"^^xsd:string ;
  skos:notation "684" ;
  skos:notation 684 ;
  skos:note "Note 1 to entry: The most common SOAs in use today are Web services (using SOAP, UDDI, and WSDL), CORBA and DCOM."@en ;
  skos:note "비고: 최근 가장 일반적인 SOA는 웹서비스(SOAP, UDDI 및 WSDL 사용)와 CORBA, DCOM 이다."@kr ;
  skos:prefLabel "service oriented architecture"@en ;
  skos:prefLabel "서비스 지향 아키텍처"@kr ;
.
<http://iso.org/tc211/term/685>
  rdf:type skos:Concept ;
  dcterms:dateAccepted "2007-10-15"^^xsd:date ;
  dcterms:dateAccepted "2009-12-29"^^xsd:date ;
  dcterms:provenance "KS X ISO 19132" ;
  dcterms:source "ISO 19132:2007" ;
  reg:status reg:statusValid ;
  rdfs:comment "Note 1 to entry: See timestamp."@en ;
  rdfs:comment "비고: 타임 스탬프를 참조하라"@kr ;
  rdfs:label "spacestamp"@en ;
  skos:changeNote "valid" ;
  skos:definition "객체 상태가 측정된 시간 또는 주어진 시간에 있어서 객체의 공간 속성 값"@kr ;
  skos:editorialNote "preferred" ;
  skos:editorialNote "preferred"^^xsd:string ;
  skos:notation "685" ;
  skos:notation 685 ;
  skos:note "Note 1 to entry: See timestamp."@en ;
  skos:note "비고: 타임 스탬프를 참조하라"@kr ;
  skos:prefLabel "spacestamp"@en ;
  skos:prefLabel "공간 스탬프"@kr ;
.
<http://iso.org/tc211/term/686>
  rdf:type skos:Concept ;
  dcterms:dateAccepted "2007-10-15"^^xsd:date ;
  dcterms:dateAccepted "2009-12-29"^^xsd:date ;
  dcterms:provenance "KS X ISO 19132" ;
  dcterms:source "ISO 19132:2007" ;
  reg:status reg:statusValid ;
  rdfs:comment "Note 1 to entry: State is usually associated to an object by its identity and to a time by a timestamp."@en ;
  rdfs:comment "비고: 상태는 보통 식별특성으로 객체와 연관되거나 타임 스탬프에 의해 시간과 연관된다."@kr ;
  rdfs:label "state (of an object)"@en ;
  skos:changeNote "valid" ;
  skos:definition "주어진 시간에 객체의 모든 속성들의 내부 값 또는 측정 가능한 설명을 반영하는 불변의 데이터 객체"@kr ;
  skos:editorialNote "preferred" ;
  skos:editorialNote "preferred"^^xsd:string ;
  skos:notation "686" ;
  skos:notation 686 ;
  skos:note "Note 1 to entry: State is usually associated to an object by its identity and to a time by a timestamp."@en ;
  skos:note "비고: 상태는 보통 식별특성으로 객체와 연관되거나 타임 스탬프에 의해 시간과 연관된다."@kr ;
  skos:prefLabel "state (of an object)"@en ;
  skos:prefLabel "상태 (하나의 객체에서)"@kr ;
.
<http://iso.org/tc211/term/687>
  rdf:type skos:Concept ;
  dcterms:dateAccepted "2007-10-15"^^xsd:date ;
  dcterms:dateAccepted "2009-12-29"^^xsd:date ;
  dcterms:provenance "KS X ISO 19132" ;
  dcterms:source "ISO 19132:2007" ;
  reg:status reg:statusValid ;
  rdfs:comment "Note 1 to entry:: There is little logical difference between traveller and target except that the former is normally used for a moving object which is being tracked, and the latter is used for either an object that is not moving, or an object for which a location is needed only once. A traveller is the subject of a tracking service; a target is the subject of a locating service. Since this International Standard does not make a distinction between the protocols for these logically similar services, but does need to differentiate between the two concepts, both terms will be used as appropriate to the underlying semantics of the situation. Since all of these terms refer to entities represented by objects within the system, they can be combined with adjectives defined for objects. So, an active target (a target represented by an active object) can be used to represent a moving object, since the act of motion is modifying the target's internal state and is therefore initiating actions."@en ;
  rdfs:comment "비고: 보통 여행자는 흔적이 남는 움직이는 객체를 이용하고, 대상은 움직이지 않는 객체나 위치가 단 한번 필요한 객체에 사용된다. 이를 제외하고는 여행자와 대상은 논리적 차이가 거의 없다. 여행자는 추적 서비스를 목적으로 하는 반면 대상은 위치하고 있는 서비스를 주제로 한다. 본 표준에서는 논리적으로 유사한 서비스의 프로토콜 간에 큰 차별성이 없으므로, 두 개념 간에 별도의 구별이 필요하지 않으며, 이 두 용어는 상황의 의미론에 기초를 두는데 사용될 것이다. 이러한 용어들은 시스템 내에서 객체로 표현된 개체를 참조하기 때문에 객체를 정의하는 형용사로 결합될 수 있다. 따라서 활성 대상(활성 객체로 표현된 대상)은 움직이는 객체의 표현에 사용될 수 있다. 이동은 대상의 내부 상태를 변경하는 것이므로, 활동을 시작하게 되는 것이다."@kr ;
  rdfs:label "target"@en ;
  skos:changeNote "valid" ;
  skos:definition "위치하고 있는 객체나 사람"@kr ;
  skos:editorialNote "preferred" ;
  skos:editorialNote "preferred"^^xsd:string ;
  skos:notation "687" ;
  skos:notation 687 ;
  skos:note "Note 1 to entry:: There is little logical difference between traveller and target except that the former is normally used for a moving object which is being tracked, and the latter is used for either an object that is not moving, or an object for which a location is needed only once. A traveller is the subject of a tracking service; a target is the subject of a locating service. Since this International Standard does not make a distinction between the protocols for these logically similar services, but does need to differentiate between the two concepts, both terms will be used as appropriate to the underlying semantics of the situation. Since all of these terms refer to entities represented by objects within the system, they can be combined with adjectives defined for objects. So, an active target (a target represented by an active object) can be used to represent a moving object, since the act of motion is modifying the target's internal state and is therefore initiating actions."@en ;
  skos:note "비고: 보통 여행자는 흔적이 남는 움직이는 객체를 이용하고, 대상은 움직이지 않는 객체나 위치가 단 한번 필요한 객체에 사용된다. 이를 제외하고는 여행자와 대상은 논리적 차이가 거의 없다. 여행자는 추적 서비스를 목적으로 하는 반면 대상은 위치하고 있는 서비스를 주제로 한다. 본 표준에서는 논리적으로 유사한 서비스의 프로토콜 간에 큰 차별성이 없으므로, 두 개념 간에 별도의 구별이 필요하지 않으며, 이 두 용어는 상황의 의미론에 기초를 두는데 사용될 것이다. 이러한 용어들은 시스템 내에서 객체로 표현된 개체를 참조하기 때문에 객체를 정의하는 형용사로 결합될 수 있다. 따라서 활성 대상(활성 객체로 표현된 대상)은 움직이는 객체의 표현에 사용될 수 있다. 이동은 대상의 내부 상태를 변경하는 것이므로, 활동을 시작하게 되는 것이다."@kr ;
  skos:prefLabel "target"@en ;
  skos:prefLabel "대상"@kr ;
.
<http://iso.org/tc211/term/688>
  rdf:type skos:Concept ;
  dcterms:dateAccepted "2007-10-15"^^xsd:date ;
  dcterms:dateAccepted "2009-12-29"^^xsd:date ;
  dcterms:provenance "KS X ISO 19132" ;
  dcterms:source "ISO 19132:2007" ;
  reg:status reg:statusValid ;
  rdfs:comment "Note 1 to entry: Temporal sequences are not assumed to be evenly spaced in time, nor equidistance in space. For discrete change, the default logic is to sample at temporal points of change if possible, so that the timestamp is the first temporal instance where the attributes listed have taken on that combination of values. For sake of space savings, some samples in a sequence only list those values that have changed since the immediately preceding temporal sample. For this reason, a sample should only be considered in the context of its containing sequence. For rigid motions (such as vehicle tracking), only centroid (a point value) and orientation (direction of travel) are needed for a temporal sequence describing location and spatial extent. A motion in combination with an object deformation would require more information."@en ;
  rdfs:comment "비고: 시간 연속은 시간적 또는 공간적으로 균등한 간격을 갖는 것으로 가정하지 않는다. 불연속변환을 위한 디폴트 논리는 가능하다면 변화의 시간 점을 견본으로 하는 것이다. 이에 따라 타임 스탬프는 속성 목록이 조합된 값을 갖는 첫 번째 시간 인스턴스이다. 연속에서 어떤 샘플은 공간 절약을 위해 단지 바로 이전의 시간 샘플의 변화 값만을 목록화 한다. 이러한 이유로, 샘플은 그 연속에 대한 상황을 고려해야만 한다. 정밀한 이동(차량 추적과 같이)에서는 위치와 공간 범위의 기술을 위해 시간연속에 중심(점 값)과 방향(여행 방향)만이 요구된다. 객체의 변형이 조합된 이동은 보다 많은 정보가 요구된다. "@kr ;
  rdfs:label "temporal sequence"@en ;
  skos:changeNote "valid" ;
  skos:definition "동일 객체의 표현 순서와 연관된 타임 스탬프의 정렬된 연속"@kr ;
  skos:editorialNote "preferred" ;
  skos:editorialNote "preferred"^^xsd:string ;
  skos:notation "688" ;
  skos:notation 688 ;
  skos:note "Note 1 to entry: Temporal sequences are not assumed to be evenly spaced in time, nor equidistance in space. For discrete change, the default logic is to sample at temporal points of change if possible, so that the timestamp is the first temporal instance where the attributes listed have taken on that combination of values. For sake of space savings, some samples in a sequence only list those values that have changed since the immediately preceding temporal sample. For this reason, a sample should only be considered in the context of its containing sequence. For rigid motions (such as vehicle tracking), only centroid (a point value) and orientation (direction of travel) are needed for a temporal sequence describing location and spatial extent. A motion in combination with an object deformation would require more information."@en ;
  skos:note "비고: 시간 연속은 시간적 또는 공간적으로 균등한 간격을 갖는 것으로 가정하지 않는다. 불연속변환을 위한 디폴트 논리는 가능하다면 변화의 시간 점을 견본으로 하는 것이다. 이에 따라 타임 스탬프는 속성 목록이 조합된 값을 갖는 첫 번째 시간 인스턴스이다. 연속에서 어떤 샘플은 공간 절약을 위해 단지 바로 이전의 시간 샘플의 변화 값만을 목록화 한다. 이러한 이유로, 샘플은 그 연속에 대한 상황을 고려해야만 한다. 정밀한 이동(차량 추적과 같이)에서는 위치와 공간 범위의 기술을 위해 시간연속에 중심(점 값)과 방향(여행 방향)만이 요구된다. 객체의 변형이 조합된 이동은 보다 많은 정보가 요구된다. "@kr ;
  skos:prefLabel "temporal sequence"@en ;
  skos:prefLabel "시간 연속"@kr ;
.
<http://iso.org/tc211/term/689>
  rdf:type skos:Concept ;
  dcterms:dateAccepted "2007-10-15"^^xsd:date ;
  dcterms:dateAccepted "2009-12-29"^^xsd:date ;
  dcterms:provenance "KS X ISO 19132" ;
  dcterms:source "ISO 19132:2007" ;
  reg:status reg:statusValid ;
  rdfs:label "timestamp"@en ;
  skos:changeNote "valid" ;
  skos:definition "객체의 상태가 측정, 기록된 시간의 값"@kr ;
  skos:editorialNote "preferred" ;
  skos:editorialNote "preferred"^^xsd:string ;
  skos:notation "689" ;
  skos:notation 689 ;
  skos:prefLabel "timestamp"@en ;
  skos:prefLabel "타임 스템프"@kr ;
.
<http://iso.org/tc211/term/69>
  rdf:type skos:Concept ;
  dcterms:dateAccepted "2002-07-01" ;
  dcterms:dateAccepted "2002-07-01"^^xsd:date ;
  dcterms:dateAccepted "2008-12-30"^^xsd:date ;
  dcterms:provenance "ISO 19101:2002" ;
  dcterms:source "ISO 19101-1:2014, 4.1.6" ;
  reg:status reg:statusAccepted ;
  reg:status reg:statusValid ;
  rdfs:label "conceptual schema"@en ;
  skos:changeNote "valid" ;
  skos:definition "formele definitie van objecten, attributen, relaties en regels in een bepaald domein"@nl ;
  skos:definition "개념적 모델의 정형화된 기술"@kr ;
  skos:editorialNote "preferred" ;
  skos:editorialNote "preferred"^^xsd:string ;
  skos:notation "69" ;
  skos:notation 69 ;
  skos:prefLabel "conceptual schema"@en ;
  skos:prefLabel "informatiemodel"@nl ;
  skos:prefLabel "개념적 스키마"@kr ;
.
<http://iso.org/tc211/term/690>
  rdf:type skos:Concept ;
  dcterms:dateAccepted "2007-10-15"^^xsd:date ;
  dcterms:dateAccepted "2009-12-29"^^xsd:date ;
  dcterms:provenance "KS X ISO 19132" ;
  dcterms:source "ISO 19132:2007" ;
  reg:status reg:statusValid ;
  rdfs:comment "Note 1 to entry:: The most common tracking devices are cell phones, GNSS chips, RFID (Radio Frequency ID) tags, or printed tags which are scanable by optical sensors  such as \"bar codes\"."@en ;
  rdfs:comment "Note 2 to entry:: The common usage of  \"vehicle\" means a \"form of conveyance\" or, more simply \"thing that conveys (carries) something else\".  Thus, a tracked object that carries a tracking device to allow it to be tracked is, by definition, a conveyance or vehicle for that device.  Thus, a cell phone that carries a GNSS device is the vehicle for that device, and the traveller carrying the cell phone, allowing him to be tracked, is the vehicle for the phone and all of its internal electronics." ;
  rdfs:comment "비고 1: 가장 일반적인 추적 장치는 휴대폰, GNSS 칩, RFID(라디오 주파수 ID) 태그 및 \"바코드\" 같은 광학 센서에 의해 스캔되는 프린트 태그가 있다."@kr ;
  rdfs:label "tracking device"@en ;
  skos:changeNote "valid" ;
  skos:definition "잘 알려진 위치의 전화 등 외부 객체를 통해 감지하거나 위치 판단을 위해 차량을 통해 운반되는 장치(태그) 및 장치 내부 전자부품"@kr ;
  skos:editorialNote "preferred" ;
  skos:editorialNote "preferred"^^xsd:string ;
  skos:notation "690" ;
  skos:notation 690 ;
  skos:note "Note 1 to entry:: The most common tracking devices are cell phones, GNSS chips, RFID (Radio Frequency ID) tags, or printed tags which are scanable by optical sensors  such as \"bar codes\"."@en ;
  skos:note "Note 2 to entry:: The common usage of  \"vehicle\" means a \"form of conveyance\" or, more simply \"thing that conveys (carries) something else\".  Thus, a tracked object that carries a tracking device to allow it to be tracked is, by definition, a conveyance or vehicle for that device.  Thus, a cell phone that carries a GNSS device is the vehicle for that device, and the traveller carrying the cell phone, allowing him to be tracked, is the vehicle for the phone and all of its internal electronics."^^<http://www.w3.org/2001/XMLSchema#@en> ;
  skos:note "비고 1: 가장 일반적인 추적 장치는 휴대폰, GNSS 칩, RFID(라디오 주파수 ID) 태그 및 \"바코드\" 같은 광학 센서에 의해 스캔되는 프린트 태그가 있다."@kr ;
  skos:note "비고 2: \"차량\"은 일반적으로\"운반 형태\"이거나 더 간략하게는 \"어떤 무언가를 운반하는 것\"을 의미한다. 그러므로 용어 정의에 따르면, 추적을 허용하는 추적 장치 운반 객체는 그 장치를 운반하는 운반체 또는 차량이다. 이런 맥락에서 GNSS 장치를 운반하는 휴대폰도 그 장치에 대한 차량이며, 자신을 트랙할 수 있는 휴대폰을 소지하고 다니는 여행자 또한 그 장치에 대한 차량이다."@kr ;
  skos:prefLabel "tracking device"@en ;
  skos:prefLabel "추적 장치"@kr ;
.
<http://iso.org/tc211/term/691>
  rdf:type skos:Concept ;
  dcterms:dateAccepted "2007-10-15"^^xsd:date ;
  dcterms:dateAccepted "2009-12-29"^^xsd:date ;
  dcterms:provenance "KS X ISO 19132" ;
  dcterms:source "ISO 19132:2007" ;
  reg:status reg:statusValid ;
  rdfs:comment "Note 1 to entry: Users are usually objects that act as proxies for people accessing the functionality of the system."@en ;
  rdfs:comment "비고: 사용자는 일반적으로 사람을 대신하여 시스템의 기능에 접근하는 객체이다."@kr ;
  rdfs:label "user"@en ;
  skos:changeNote "valid" ;
  skos:definition "시스템에게 서비스를 요청하는 활성 객체"@kr ;
  skos:editorialNote "preferred" ;
  skos:editorialNote "preferred"^^xsd:string ;
  skos:notation "691" ;
  skos:notation 691 ;
  skos:note "Note 1 to entry: Users are usually objects that act as proxies for people accessing the functionality of the system."@en ;
  skos:note "비고: 사용자는 일반적으로 사람을 대신하여 시스템의 기능에 접근하는 객체이다."@kr ;
  skos:prefLabel "user"@en ;
  skos:prefLabel "사용자"@kr ;
.
<http://iso.org/tc211/term/692>
  rdf:type skos:Concept ;
  dcterms:dateAccepted "2007-09-01"^^xsd:date ;
  dcterms:dateAccepted "2009-12-29"^^xsd:date ;
  dcterms:provenance "KS X ISO 19136" ;
  dcterms:source "ISO 19136:2007" ;
  reg:status reg:statusValid ;
  rdfs:label "child element <XML>"@en ;
  skos:changeNote "valid" ;
  skos:definition "요소의 직접적인 자 요소"@kr ;
  skos:editorialNote "preferred" ;
  skos:editorialNote "preferred"^^xsd:string ;
  skos:notation "692" ;
  skos:notation 692 ;
  skos:prefLabel "child element <XML>"@en ;
  skos:prefLabel "자식 요소 <XML>"@kr ;
.
<http://iso.org/tc211/term/693>
  rdf:type skos:Concept ;
  dcterms:dateAccepted "2007-09-01"^^xsd:date ;
  dcterms:dateAccepted "2009-12-29"^^xsd:date ;
  dcterms:provenance "KS X ISO 19136" ;
  dcterms:source "ISO 19136:2007" ;
  reg:status reg:statusValid ;
  rdfs:label "observable type"@en ;
  skos:changeNote "valid" ;
  skos:definition "관측의 결과가 물리량인 데이터 유형"@kr ;
  skos:editorialNote "preferred" ;
  skos:editorialNote "preferred"^^xsd:string ;
  skos:notation "693" ;
  skos:notation 693 ;
  skos:prefLabel "observable type"@en ;
  skos:prefLabel "관측 유형"@kr ;
.
<http://iso.org/tc211/term/695>
  rdf:type skos:Concept ;
  dcterms:dateAccepted "2007-09-01"^^xsd:date ;
  dcterms:dateAccepted "2009-12-29"^^xsd:date ;
  dcterms:provenance "KS X ISO 19136" ;
  dcterms:source "ISO 19136:2007" ;
  reg:status reg:statusValid ;
  rdfs:label "polygon"@en ;
  skos:changeNote "valid" ;
  skos:definition "하나의 외부 경계와 0 또는 그 이상의 내부 경계에 의해 정의되는 평면 표면"@kr ;
  skos:editorialNote "preferred" ;
  skos:editorialNote "preferred"^^xsd:string ;
  skos:notation "695" ;
  skos:notation 695 ;
  skos:prefLabel "polygon"@en ;
  skos:prefLabel "다각형"@kr ;
.
<http://iso.org/tc211/term/696>
  rdf:type skos:Concept ;
  dcterms:dateAccepted "2007-09-01"^^xsd:date ;
  dcterms:dateAccepted "2009-12-29"^^xsd:date ;
  dcterms:provenance "KS X ISO 19136" ;
  dcterms:source "ISO 19136:2007" ;
  reg:status reg:statusValid ;
  rdfs:label "range"@en ;
  skos:changeNote "valid" ;
  skos:definition "함수 f가 자신의 영역에서 가질 수 있는 모든 값들의 집합"@kr ;
  skos:editorialNote "preferred" ;
  skos:editorialNote "preferred"^^xsd:string ;
  skos:notation "696" ;
  skos:notation 696 ;
  skos:prefLabel "range"@en ;
  skos:prefLabel "범위"@kr ;
.
<http://iso.org/tc211/term/697>
  rdf:type skos:Concept ;
  dcterms:dateAccepted "2007-09-01"^^xsd:date ;
  dcterms:dateAccepted "2009-12-29"^^xsd:date ;
  dcterms:provenance "KS X ISO 19136" ;
  dcterms:source "ISO 19136:2007" ;
  reg:status reg:statusValid ;
  rdfs:comment "Note 1 to entry: The W3C XML Schema provides an XML interchange format for schema information. A single schema document provides descriptions of components associated with a single XML namespace, but several documents may describe components in the same schema, i.e. the same target namespace."@en ;
  rdfs:comment "비고: W3C XML 스키마는 스키마 정보를 위한 XML 전송 포맷을 제공한다. 하나의 스키마 문서는 하나의 XML 이름 공간과 관련된 컴포넌트에 대한 기술을 제공한다. 그러나 몇몇 문서들은 동일한 스키마에서의 컴포넌트를 기술할 수 있다(예: 동일한 대상 이름 공간)."@kr ;
  rdfs:label "schema document <XML Schema>"@en ;
  skos:changeNote "valid" ;
  skos:definition "스키마 컴포넌트에 대한 정의와 선언을 포함한 XML 문서"@kr ;
  skos:editorialNote "preferred" ;
  skos:editorialNote "preferred"^^xsd:string ;
  skos:notation "697" ;
  skos:notation 697 ;
  skos:note "Note 1 to entry: The W3C XML Schema provides an XML interchange format for schema information. A single schema document provides descriptions of components associated with a single XML namespace, but several documents may describe components in the same schema, i.e. the same target namespace."@en ;
  skos:note "비고: W3C XML 스키마는 스키마 정보를 위한 XML 전송 포맷을 제공한다. 하나의 스키마 문서는 하나의 XML 이름 공간과 관련된 컴포넌트에 대한 기술을 제공한다. 그러나 몇몇 문서들은 동일한 스키마에서의 컴포넌트를 기술할 수 있다(예: 동일한 대상 이름 공간)."@kr ;
  skos:prefLabel "schema document <XML Schema>"@en ;
  skos:prefLabel "스키마 문서 <XML 스키마>"@kr ;
.
<http://iso.org/tc211/term/698>
  rdf:type skos:Concept ;
  dcterms:dateAccepted "2007-09-01"^^xsd:date ;
  dcterms:dateAccepted "2009-12-29"^^xsd:date ;
  dcterms:provenance "KS X ISO 19136" ;
  dcterms:source "ISO 19136:2007" ;
  reg:status reg:statusValid ;
  rdfs:label "schema <XML Schema>"@en ;
  skos:changeNote "valid" ;
  skos:definition "동일한 대상 이름 공간내에 있는 스키마 컴포넌트의 모음"@kr ;
  skos:editorialNote "preferred" ;
  skos:editorialNote "preferred"^^xsd:string ;
  skos:notation "698" ;
  skos:notation 698 ;
  skos:prefLabel "schema <XML Schema>"@en ;
  skos:prefLabel "스키마 <XML 스키마>"@kr ;
.
<http://iso.org/tc211/term/699>
  rdf:type skos:Concept ;
  dcterms:dateAccepted "2007-09-01"^^xsd:date ;
  dcterms:dateAccepted "2009-12-29"^^xsd:date ;
  dcterms:provenance "KS X ISO 19136" ;
  dcterms:source "ISO 19136:2007" ;
  reg:status reg:statusValid ;
  rdfs:label "UML application schema"@en ;
  skos:changeNote "valid" ;
  skos:definition "KS X ISO 19109에 따라 UML로 기술된 응용 스키마"@kr ;
  skos:editorialNote "preferred" ;
  skos:editorialNote "preferred"^^xsd:string ;
  skos:notation "699" ;
  skos:notation 699 ;
  skos:prefLabel "UML application schema"@en ;
  skos:prefLabel "UML 응용 스키마"@kr ;
.
<http://iso.org/tc211/term/7>
  rdf:type skos:Concept ;
  dcterms:dateAccepted "2000-12-15"^^xsd:date ;
  dcterms:dateAccepted "2007-06-29"^^xsd:date ;
  dcterms:provenance "KS X ISO 19105" ;
  dcterms:source "ISO 19105:2000" ;
  reg:status reg:statusValid ;
  rdfs:comment "Note 1 to entry: This includes the planning and execution of several kinds of tests (e.g. functional, volume, performance tests) that demonstrate that the implementation satisfies the user requirements."@en ;
  rdfs:comment "Note 2 to entry: This is not a part of conformance testing" ;
  rdfs:comment "비고 1: 사용자 요구 사항에 맞게 구현되는지를 시연하는 여러 종류의 시험(기능 시험, 용량 시험, 성능 시험 등)을 기획하고 실행하는 것이 검수 시험에 포함된다."@kr ;
  rdfs:label "acceptance testing <user>"@en ;
  skos:changeNote "valid" ;
  skos:definition "구현된 결과가 검수 기준을 만족하는지에 대한 결정 과정"@kr ;
  skos:editorialNote "preferred" ;
  skos:editorialNote "preferred"^^xsd:string ;
  skos:notation "7" ;
  skos:notation 7 ;
  skos:note "Note 1 to entry: This includes the planning and execution of several kinds of tests (e.g. functional, volume, performance tests) that demonstrate that the implementation satisfies the user requirements."@en ;
  skos:note "Note 2 to entry: This is not a part of conformance testing"^^<http://www.w3.org/2001/XMLSchema#@en> ;
  skos:note "비고 1: 사용자 요구 사항에 맞게 구현되는지를 시연하는 여러 종류의 시험(기능 시험, 용량 시험, 성능 시험 등)을 기획하고 실행하는 것이 검수 시험에 포함된다."@kr ;
  skos:note "비고 2: 검수 시험은 적합성 시험의 일부가 아니다."@kr ;
  skos:prefLabel "acceptance testing <user>"@en ;
  skos:prefLabel "검수 시험<사용자>"@kr ;
.
<http://iso.org/tc211/term/70>
  rdf:type skos:Concept ;
  dcterms:dateAccepted "2002-07-01"^^xsd:date ;
  dcterms:dateAccepted "2008-12-30"^^xsd:date ;
  dcterms:provenance "ISO 19101:2002" ;
  dcterms:source "ISO 19101-1:2014, 4.1.7" ;
  reg:status reg:statusValid ;
  rdfs:comment "Note 1 to entry: A conceptual schema language may be lexical or graphical. Several conceptual schema languages can be based on the same conceptual formalism."@en ;
  rdfs:comment "비고: 개념적 스키마 언어는 어휘적이거나 그래픽적일 수 있다. 몇몇 개념적 스키마 언어들은 동일한 개념적 형식에 근거할 수 있다."@kr ;
  rdfs:label "conceptual schema language"@en ;
  skos:changeNote "valid" ;
  skos:definition "개념적 스키마의 표현을 위해 개념적 형식에 근거한 형식 언어"@kr ;
  skos:editorialNote "preferred" ;
  skos:editorialNote "preferred"^^xsd:string ;
  skos:notation "70" ;
  skos:notation 70 ;
  skos:note "Note 1 to entry: A conceptual schema language may be lexical or graphical. Several conceptual schema languages can be based on the same conceptual formalism."@en ;
  skos:note "비고: 개념적 스키마 언어는 어휘적이거나 그래픽적일 수 있다. 몇몇 개념적 스키마 언어들은 동일한 개념적 형식에 근거할 수 있다."@kr ;
  skos:prefLabel "conceptual schema language"@en ;
  skos:prefLabel "개념적 스키마 언어"@kr ;
.
<http://iso.org/tc211/term/702>
  rdf:type skos:Concept ;
  dcterms:dateAccepted "2007-07-01" ;
  dcterms:dateAccepted "2007-07-01"^^xsd:date ;
  dcterms:dateAccepted "2007-11-01"^^xsd:date ;
  dcterms:provenance "KS X ISO 19111" ;
  dcterms:source "ISO 19111:2007" ;
  reg:status reg:statusAccepted ;
  reg:status reg:statusValid ;
  rdfs:comment "Note 1 to entry: Coordinate reference systems are independent of each other if coordinate values in one cannot be converted or transformed into coordinate values in the other."@en ;
  rdfs:comment "OPMERKING Coördinaatreferentiesystemen zijn onafhankelijk van elkaar als coördinaatwaarden in één stelsel niet kunnen worden geconverteerd of getransformeerd in het andere."@en ;
  rdfs:comment "비고: 하나의 좌표 참조 체계의 좌표 값이 다른 좌표 참조 체계의 좌표 값으로 전환될 수 없다면, 이들 좌표 참조 체계는 서로 독립적이다.  "@kr ;
  rdfs:label "compound coordinate reference system"@en ;
  skos:changeNote "valid" ;
  skos:definition "coördinaatreferentiesysteem wat op zijn minst twee onafhankelijke coördinaatsystemen gebruikt"@nl ;
  skos:definition "최소 두 개의 독립된 좌표 참조 체계를 사용하는 좌표 참조 체계"@kr ;
  skos:editorialNote "preferred" ;
  skos:editorialNote "preferred"^^xsd:string ;
  skos:notation "702" ;
  skos:notation 702 ;
  skos:note "Note 1 to entry: Coordinate reference systems are independent of each other if coordinate values in one cannot be converted or transformed into coordinate values in the other."@en ;
  skos:note "OPMERKING Coördinaatreferentiesystemen zijn onafhankelijk van elkaar als coördinaatwaarden in één stelsel niet kunnen worden geconverteerd of getransformeerd in het andere."@en ;
  skos:note "비고: 하나의 좌표 참조 체계의 좌표 값이 다른 좌표 참조 체계의 좌표 값으로 전환될 수 없다면, 이들 좌표 참조 체계는 서로 독립적이다.  "@kr ;
  skos:prefLabel "compound coordinate reference system"@en ;
  skos:prefLabel "samengesteld coördinaatreferentiesysteem"@nl ;
  skos:prefLabel "합성 좌표 참조 체계"@kr ;
.
<http://iso.org/tc211/term/703>
  rdf:type skos:Concept ;
  dcterms:dateAccepted "2007-07-01" ;
  dcterms:dateAccepted "2007-07-01"^^xsd:date ;
  dcterms:dateAccepted "2007-11-01"^^xsd:date ;
  dcterms:provenance "KS X ISO 19111" ;
  dcterms:provenance "NEN 3610" ;
  dcterms:source "ISO 19111:2007" ;
  reg:status reg:statusAccepted ;
  reg:status reg:statusValid ;
  rdfs:comment "Note 1 to entry: For geodetic and vertical datums, the object will be the Earth."@en ;
  rdfs:comment "OPMERKING Voor geodetische en verticale datums is het object de aarde."@en ;
  rdfs:comment "비고: 측지 원점 및 수직 데이텀의 경우, \"객체\"는 지구이다."@kr ;
  rdfs:label "coordinate reference system"@en ;
  skos:changeNote "valid" ;
  skos:definition "coördinaatsysteem dat aan een object is gerelateerd door een datum"@nl ;
  skos:definition "데이텀에 의해 객체와 관련된 좌표 체계"@kr ;
  skos:editorialNote "preferred" ;
  skos:editorialNote "preferred"^^xsd:string ;
  skos:notation "703" ;
  skos:notation 703 ;
  skos:note "Note 1 to entry: For geodetic and vertical datums, the object will be the Earth."@en ;
  skos:note "OPMERKING Voor geodetische en verticale datums is het object de aarde."@en ;
  skos:note "비고: 측지 원점 및 수직 데이텀의 경우, \"객체\"는 지구이다."@kr ;
  skos:prefLabel "coordinate reference system"@en ;
  skos:prefLabel "coördinaatreferentiesysteem"@nl ;
  skos:prefLabel "좌표 참조 체계"@kr ;
.
<http://iso.org/tc211/term/704>
  rdf:type skos:Concept ;
  dcterms:dateAccepted "2007-07-01" ;
  dcterms:dateAccepted "2007-07-01"^^xsd:date ;
  dcterms:dateAccepted "2007-11-01"^^xsd:date ;
  dcterms:provenance "KS X ISO 19111" ;
  dcterms:provenance "NEN 3610" ;
  dcterms:source "ISO 19111:2007" ;
  reg:status reg:statusAccepted ;
  reg:status reg:statusValid ;
  rdfs:label "datum"@en ;
  skos:changeNote "valid" ;
  skos:definition "parameter of set van parameters voor het definiëren van het nulpunt, de schaal en de oriëntatie van een coördinaatsysteem"@nl ;
  skos:definition "좌표 체계의 기점, 축척, 방향을 정의하는 매개 변수 또는 매개 변수의 집합"@kr ;
  skos:editorialNote "preferred" ;
  skos:editorialNote "preferred"^^xsd:string ;
  skos:notation "704" ;
  skos:notation 704 ;
  skos:prefLabel "datum"@en ;
  skos:prefLabel "datum"@nl ;
  skos:prefLabel "데이텀"@kr ;
.
<http://iso.org/tc211/term/706>
  rdf:type skos:Concept ;
  dcterms:dateAccepted "2007-07-01" ;
  dcterms:dateAccepted "2007-07-01"^^xsd:date ;
  dcterms:dateAccepted "2007-11-01"^^xsd:date ;
  dcterms:provenance "KS X ISO 19111" ;
  dcterms:source "ISO 19111:2007" ;
  reg:status reg:statusAccepted ;
  reg:status reg:statusValid ;
  rdfs:label "engineering coordinate reference system"@en ;
  skos:changeNote "valid" ;
  skos:definition "coördinaatreferentiesysteem gebaseerd op een lokaal datum"@nl ;
  skos:definition "공학 데이텀에 기반한 좌표 참조 체계"@kr ;
  skos:editorialNote "preferred" ;
  skos:editorialNote "preferred"^^xsd:string ;
  skos:notation "706" ;
  skos:notation 706 ;
  skos:prefLabel "engineering coordinate reference system"@en ;
  skos:prefLabel "lokaal coördinaatreferentiesysteem"@nl ;
  skos:prefLabel "공학 좌표계"@kr ;
.
<http://iso.org/tc211/term/707>
  rdf:type skos:Concept ;
  dcterms:dateAccepted "2007-07-01" ;
  dcterms:dateAccepted "2007-07-01"^^xsd:date ;
  dcterms:dateAccepted "2007-11-01"^^xsd:date ;
  dcterms:provenance "KS X ISO 19111" ;
  dcterms:source "ISO 19111:2007" ;
  reg:status reg:statusAccepted ;
  reg:status reg:statusValid ;
  rdfs:label "geodetic coordinate reference system"@en ;
  skos:changeNote "valid" ;
  skos:definition "coördinaatreferentiesysteem gebaseerd op een geodetisch datum"@nl ;
  skos:definition "측지 원점을 바탕으로하는 좌표 참조 체계"@kr ;
  skos:editorialNote "preferred" ;
  skos:editorialNote "preferred"^^xsd:string ;
  skos:notation "707" ;
  skos:notation 707 ;
  skos:prefLabel "geodetic coordinate reference system"@en ;
  skos:prefLabel "geodetisch coördinaatreferentiesysteem"@nl ;
  skos:prefLabel "측지 좌표 참조 체계"@kr ;
.
<http://iso.org/tc211/term/708>
  rdf:type skos:Concept ;
  dcterms:dateAccepted "2007-07-01" ;
  dcterms:dateAccepted "2007-07-01"^^xsd:date ;
  dcterms:dateAccepted "2007-11-01"^^xsd:date ;
  dcterms:provenance "KS X ISO 19111" ;
  dcterms:source "ISO 19111:2007" ;
  reg:status reg:statusAccepted ;
  reg:status reg:statusValid ;
  rdfs:label "geodetic datum"@en ;
  skos:changeNote "valid" ;
  skos:definition "datum welke de relatie tussen een twee- of driedimensionaal coördinaatsysteem ten opzichte van de aarde beschrijft"@nl ;
  skos:definition "지구에 대한 2차원 또는 3차원 좌표 체계의 관계를 기술하는 데이텀"@kr ;
  skos:editorialNote "preferred" ;
  skos:editorialNote "preferred"^^xsd:string ;
  skos:notation "708" ;
  skos:notation 708 ;
  skos:prefLabel "geodetic datum"@en ;
  skos:prefLabel "geodetisch datum"@nl ;
  skos:prefLabel "측지 원점"@kr ;
.
<http://iso.org/tc211/term/709>
  rdf:type skos:Concept ;
  dcterms:dateAccepted "2007-07-01" ;
  dcterms:dateAccepted "2007-07-01"^^xsd:date ;
  dcterms:dateAccepted "2007-11-01"^^xsd:date ;
  dcterms:provenance "KS X ISO 19111" ;
  dcterms:source "ISO 19111:2007" ;
  reg:status reg:statusAccepted ;
  reg:status reg:statusValid ;
  rdfs:label "image coordinate reference system"@en ;
  skos:changeNote "valid" ;
  skos:definition "coördinaatreferentiesysteem gebaseerd op een beelddatum"@nl ;
  skos:definition "영상 데이텀을 바탕으로하는 좌표 참조 체계"@kr ;
  skos:editorialNote "preferred" ;
  skos:editorialNote "preferred"^^xsd:string ;
  skos:notation "709" ;
  skos:notation 709 ;
  skos:prefLabel "beeld coördinaatreferentiesysteem"@nl ;
  skos:prefLabel "image coordinate reference system"@en ;
  skos:prefLabel "영상 좌표 참조 체계"@kr ;
.
<http://iso.org/tc211/term/71>
  rdf:type skos:Concept ;
  dcterms:dateAccepted "2000-12-15"^^xsd:date ;
  dcterms:dateAccepted "2007-06-29"^^xsd:date ;
  dcterms:provenance "KS X ISO 19105" ;
  dcterms:source "ISO 19105:2000" ;
  reg:status reg:statusValid ;
  rdfs:label "conformance"@en ;
  skos:changeNote "valid" ;
  skos:definition "명시된 요구 사항을 구현한 것에 대한 충실도"@kr ;
  skos:editorialNote "preferred" ;
  skos:editorialNote "preferred"^^xsd:string ;
  skos:notation "71" ;
  skos:notation 71 ;
  skos:prefLabel "conformance"@en ;
  skos:prefLabel "적합성"@kr ;
.
<http://iso.org/tc211/term/710>
  rdf:type skos:Concept ;
  dcterms:dateAccepted "2007-07-01" ;
  dcterms:dateAccepted "2007-07-01"^^xsd:date ;
  dcterms:dateAccepted "2007-11-01"^^xsd:date ;
  dcterms:provenance "KS X ISO 19111" ;
  dcterms:source "ISO 19111:2007" ;
  reg:status reg:statusAccepted ;
  reg:status reg:statusValid ;
  rdfs:label "image datum"@en ;
  skos:changeNote "valid" ;
  skos:definition "lokaal datum welk de relatie definieert tussen een coördinaatsysteem en een beeld"@nl ;
  skos:definition "영상과 좌표 체계의 관계를 정의하는 공학 데이텀"@kr ;
  skos:editorialNote "preferred" ;
  skos:editorialNote "preferred"^^xsd:string ;
  skos:notation "710" ;
  skos:notation 710 ;
  skos:prefLabel "beelddatum"@nl ;
  skos:prefLabel "image datum"@en ;
  skos:prefLabel "영상 데이텀"@kr ;
.
<http://iso.org/tc211/term/711>
  rdf:type skos:Concept ;
  dcterms:dateAccepted "2007-07-01" ;
  dcterms:dateAccepted "2007-07-01"^^xsd:date ;
  dcterms:dateAccepted "2007-11-01"^^xsd:date ;
  dcterms:provenance "KS X ISO 19111" ;
  dcterms:source "ISO 19111:2007" ;
  reg:status reg:statusAccepted ;
  reg:status reg:statusValid ;
  rdfs:comment "Note 1 to entry: This term is often used for the pole-to-pole arc rather than the complete closed figure."@en ;
  rdfs:comment "OPMERKING Deze term wordt vaak gebruikt voor de pool tot pool boog in plaats van de volledige, gesloten omtrek."@en ;
  rdfs:comment "비고: 이 용어는 완벽하게 폐합된 지형지물이라기 보다는 극과 극을 연결하는 호로 사용된다."@kr ;
  rdfs:label "meridian"@en ;
  skos:changeNote "valid" ;
  skos:definition "doorsnijding van een ellipsoïde door een vlak welke de kortste as van de ellipsoïde bevat"@nl ;
  skos:definition "타원체와 그 타원체의 최단 반경을 포함하는 평면 간의 교차선"@kr ;
  skos:editorialNote "preferred" ;
  skos:editorialNote "preferred"^^xsd:string ;
  skos:notation "711" ;
  skos:notation 711 ;
  skos:note "Note 1 to entry: This term is often used for the pole-to-pole arc rather than the complete closed figure."@en ;
  skos:note "OPMERKING Deze term wordt vaak gebruikt voor de pool tot pool boog in plaats van de volledige, gesloten omtrek."@en ;
  skos:note "비고: 이 용어는 완벽하게 폐합된 지형지물이라기 보다는 극과 극을 연결하는 호로 사용된다."@kr ;
  skos:prefLabel "meridiaan"@nl ;
  skos:prefLabel "meridian"@en ;
  skos:prefLabel "자오선"@kr ;
.
<http://iso.org/tc211/term/713>
  rdf:type skos:Concept ;
  dcterms:dateAccepted "2007-07-01" ;
  dcterms:dateAccepted "2007-07-01"^^xsd:date ;
  dcterms:dateAccepted "2007-11-01"^^xsd:date ;
  dcterms:provenance "KS X ISO 19111" ;
  dcterms:source "ISO 19111:2007" ;
  reg:status reg:statusAccepted ;
  reg:status reg:statusValid ;
  rdfs:comment "Note 1 to entry: Not to be confused with an ellipsoidal coordinate system based on an ellipsoid 'degenerated' into a sphere."@en ;
  rdfs:comment "OPMERKING Niet te verwarren met een ellipsoidaal coördinaat systeem gebaseerd op een ellipsoïde die 'gedegenereerd' is in een bol."@en ;
  rdfs:label "spherical coordinate system"@en ;
  skos:changeNote "valid" ;
  skos:definition "driedimensionaal coördinaatsysteem waarbij één afstand en twee hoeken vanuit de oorsprong worden bepaald, vaak verbonden aan een geodetisch coördinaatreferentiesysteem"@nl ;
  skos:definition "일반적으로 측지 좌표 참조 체계와 연관되어 원점으로부터의 측정된 하나의 길이와 두 개의 각도 좌표를 갖는 3차원 좌표 체계"@kr ;
  skos:editorialNote "preferred" ;
  skos:editorialNote "preferred"^^xsd:string ;
  skos:notation "713" ;
  skos:notation 713 ;
  skos:note "Note 1 to entry: Not to be confused with an ellipsoidal coordinate system based on an ellipsoid 'degenerated' into a sphere."@en ;
  skos:note "OPMERKING Niet te verwarren met een ellipsoidaal coördinaat systeem gebaseerd op een ellipsoïde die 'gedegenereerd' is in een bol."@en ;
  skos:prefLabel "bol coördinaatsysteem"@nl ;
  skos:prefLabel "spherical coordinate system"@en ;
  skos:prefLabel "구면 좌표계"@kr ;
.
<http://iso.org/tc211/term/715>
  rdf:type skos:Concept ;
  dcterms:dateAccepted "2007-07-01" ;
  dcterms:dateAccepted "2007-07-01"^^xsd:date ;
  dcterms:dateAccepted "2007-11-01"^^xsd:date ;
  dcterms:provenance "KS X ISO 19111" ;
  dcterms:source "ISO 19111:2007" ;
  reg:status reg:statusAccepted ;
  reg:status reg:statusValid ;
  rdfs:label "vertical coordinate reference system"@en ;
  skos:changeNote "valid" ;
  skos:definition "eendimensionaal coördinaatreferentiesysteem gebaseerd op een verticaal datum"@nl ;
  skos:definition "수직 데이텀을 바탕으로한 1차원 좌표 참조 체계"@kr ;
  skos:editorialNote "preferred" ;
  skos:editorialNote "preferred"^^xsd:string ;
  skos:notation "715" ;
  skos:notation 715 ;
  skos:prefLabel "verticaal coördinaatreferentiesysteem"@nl ;
  skos:prefLabel "vertical coordinate reference system"@en ;
  skos:prefLabel "수직 좌표 참조 체계"@kr ;
.
<http://iso.org/tc211/term/716>
  rdf:type skos:Concept ;
  dcterms:dateAccepted "2007-07-01" ;
  dcterms:dateAccepted "2007-07-01"^^xsd:date ;
  dcterms:dateAccepted "2007-11-01"^^xsd:date ;
  dcterms:provenance "KS X ISO 19111" ;
  dcterms:source "ISO 19111:2007" ;
  reg:status reg:statusAccepted ;
  reg:status reg:statusValid ;
  rdfs:label "vertical coordinate system"@en ;
  skos:changeNote "valid" ;
  skos:definition "een dimensionaal coördinaatsysteem gebruikt voor zwaartekracht gerelateerde hoogte- of dieptemetingen"@nl ;
  skos:definition "중력 높이 또는 깊이의 측정에 사용되는 1차원 좌표 체계"@kr ;
  skos:editorialNote "preferred" ;
  skos:editorialNote "preferred"^^xsd:string ;
  skos:notation "716" ;
  skos:notation 716 ;
  skos:prefLabel "verticaal coördinaatsysteem"@nl ;
  skos:prefLabel "vertical coordinate system"@en ;
  skos:prefLabel "수직 좌표계"@kr ;
.
<http://iso.org/tc211/term/717>
  rdf:type skos:Concept ;
  dcterms:dateAccepted "2008-06-01"^^xsd:date ;
  dcterms:source "ISO 19141:2008" ;
  reg:status reg:statusValid ;
  rdfs:comment "Note 1 to entry: A rigid geometric object may undergo translation or rotation, but remains congruent with its base representation."@en ;
  rdfs:comment "Note 2 to entry:  The local origin and ordinate vectors establish an engineering coordinate reference system (ISO 19111), also called a local frame or a local Euclidean coordinate system." ;
  rdfs:label "base representation <moving features>"@en ;
  skos:changeNote "valid" ;
  skos:editorialNote "preferred"^^xsd:string ;
  skos:notation 717 ;
  skos:note "Note 1 to entry: A rigid geometric object may undergo translation or rotation, but remains congruent with its base representation."@en ;
  skos:note "Note 2 to entry:  The local origin and ordinate vectors establish an engineering coordinate reference system (ISO 19111), also called a local frame or a local Euclidean coordinate system."^^<http://www.w3.org/2001/XMLSchema#@en> ;
  skos:prefLabel "base representation <moving features>"@en ;
.
<http://iso.org/tc211/term/72>
  rdf:type skos:Concept ;
  dcterms:dateAccepted "2000-12-15"^^xsd:date ;
  dcterms:dateAccepted "2007-06-29"^^xsd:date ;
  dcterms:provenance "KS X ISO 19105" ;
  dcterms:source "ISO 19105:2000" ;
  reg:status reg:statusValid ;
  rdfs:label "conformance assessment process"@en ;
  skos:changeNote "valid" ;
  skos:definition "표준 표준에 따라 적합성을 만족하도록 구현되었는지를 평가하는 과정"@kr ;
  skos:editorialNote "preferred" ;
  skos:editorialNote "preferred"^^xsd:string ;
  skos:notation "72" ;
  skos:notation 72 ;
  skos:prefLabel "conformance assessment process"@en ;
  skos:prefLabel "적합성 평가 과정"@kr ;
.
<http://iso.org/tc211/term/720>
  rdf:type skos:Concept ;
  dcterms:dateAccepted "2008-06-01"^^xsd:date ;
  dcterms:source "ISO/TS 19101-2:2008" ;
  reg:status reg:statusValid ;
  rdfs:label "sensor model"@en ;
  skos:changeNote "valid" ;
  skos:editorialNote "preferred"^^xsd:string ;
  skos:notation 720 ;
  skos:prefLabel "sensor model"@en ;
.
<http://iso.org/tc211/term/724>
  rdf:type skos:Concept ;
  dcterms:dateAccepted "2005-07-15"^^xsd:date ;
  dcterms:dateAccepted "2009-12-29"^^xsd:date ;
  dcterms:provenance "ISO/TS 19103:2005 ,4.2.9" ;
  dcterms:source "ISO/IEC 19501" ;
  reg:status reg:statusValid ;
  rdfs:comment "Note 1 to entry: A component represents a physical piece of implementation of a system, including software code (source, binary or executable) or equivalents such as scripts or command files."@en ;
  rdfs:comment "비고: 컴포넌트는 소프트웨어 코드, 명령 파일 또는 스크립트 등을 포함하는 시스템의 물리적 구현 단위이다."@kr ;
  rdfs:label "component <UML>"@en ;
  skos:changeNote "valid" ;
  skos:definition "내부 구현을 캡슐화하고 인터페이스의 집합을 노출시킨, 적용 및 교체가 가능한 모듈화된 시스템의 한 부분"@kr ;
  skos:editorialNote "preferred" ;
  skos:editorialNote "preferred"^^xsd:string ;
  skos:notation "724" ;
  skos:notation 724 ;
  skos:note "Note 1 to entry: A component represents a physical piece of implementation of a system, including software code (source, binary or executable) or equivalents such as scripts or command files."@en ;
  skos:note "비고: 컴포넌트는 소프트웨어 코드, 명령 파일 또는 스크립트 등을 포함하는 시스템의 물리적 구현 단위이다."@kr ;
  skos:prefLabel "component <UML>"@en ;
  skos:prefLabel "컴포넌트 <UML>"@kr ;
.
<http://iso.org/tc211/term/725>
  rdf:type skos:Concept ;
  dcterms:dateAccepted "2005-07-15"^^xsd:date ;
  dcterms:dateAccepted "2009-12-29"^^xsd:date ;
  dcterms:provenance "ISO/TS 19103:2005 ,4.2.10" ;
  dcterms:source "ISO/IEC 19501" ;
  reg:status reg:statusValid ;
  rdfs:comment "Note 1 to entry: Parts with non-fixed multiplicity may be created after the composite itself, but once created they live and die with it (i.e., they share lifetimes). Such parts can also be explicitly removed before the death of the composite. Composition may be recursive. Synonym: composite aggregation."@en ;
  rdfs:comment "비고: 합성 이후 정해지지 않은 다중성이 추가 생성될 수 있지만, 한번 생성된 부분들은 합성과 생명 주기를 같이한다. 물론 이러한 부분들은 합성 연관이 해체되기 전, 명시적으로 제거할 수 있다. 합성은 순환적일 수 있다. 동의어: 합성 연관"@kr ;
  rdfs:label "composition <UML>"@en ;
  skos:changeNote "valid" ;
  skos:definition "부분 인스턴스는 동시에 하나의 합성에 포함되며, 합성 객체가 부분들의 생성, 제거에 대한 책임을 갖는 집합 연관의 형태"@kr ;
  skos:editorialNote "preferred" ;
  skos:editorialNote "preferred"^^xsd:string ;
  skos:notation "725" ;
  skos:notation 725 ;
  skos:note "Note 1 to entry: Parts with non-fixed multiplicity may be created after the composite itself, but once created they live and die with it (i.e., they share lifetimes). Such parts can also be explicitly removed before the death of the composite. Composition may be recursive. Synonym: composite aggregation."@en ;
  skos:note "비고: 합성 이후 정해지지 않은 다중성이 추가 생성될 수 있지만, 한번 생성된 부분들은 합성과 생명 주기를 같이한다. 물론 이러한 부분들은 합성 연관이 해체되기 전, 명시적으로 제거할 수 있다. 합성은 순환적일 수 있다. 동의어: 합성 연관"@kr ;
  skos:prefLabel "composition <UML>"@en ;
  skos:prefLabel "합성 <UML>"@kr ;
.
<http://iso.org/tc211/term/726>
  rdf:type skos:Concept ;
  dcterms:dateAccepted "2005-07-15"^^xsd:date ;
  dcterms:dateAccepted "2009-12-29"^^xsd:date ;
  dcterms:provenance "ISO/TS 19103:2005 ,4.2.13" ;
  dcterms:source "ISO/IEC 19501" ;
  reg:status reg:statusValid ;
  rdfs:comment "Note 1 to entry: An instance of the more specific element may be used where the more general element is allowed. See: inheritance."@en ;
  rdfs:comment "비고: 보다 일반적인 요소가 허용되는 곳에 보다 상세 요소의 인스턴스를 사용할 수 있다. 상속을 참조하라."@kr ;
  rdfs:label "generalization <UML>"@en ;
  skos:changeNote "valid" ;
  skos:definition "구성 항목의 상속을 표시하는 기법으로, 하나의 구성 요소가 보다 일반화되며 다른 구성 요소는 보다 세분화됨을 표시하는 관계"@kr ;
  skos:editorialNote "preferred" ;
  skos:editorialNote "preferred"^^xsd:string ;
  skos:notation "726" ;
  skos:notation 726 ;
  skos:note "Note 1 to entry: An instance of the more specific element may be used where the more general element is allowed. See: inheritance."@en ;
  skos:note "비고: 보다 일반적인 요소가 허용되는 곳에 보다 상세 요소의 인스턴스를 사용할 수 있다. 상속을 참조하라."@kr ;
  skos:prefLabel "generalization <UML>"@en ;
  skos:prefLabel "일반화 <UML>"@kr ;
.
<http://iso.org/tc211/term/727>
  rdf:type skos:Concept ;
  dcterms:dateAccepted "2005-07-15"^^xsd:date ;
  dcterms:dateAccepted "2009-12-29"^^xsd:date ;
  dcterms:provenance "ISO/TS 19103:2005 ,4.2.15" ;
  dcterms:source "ISO/IEC 19501" ;
  reg:status reg:statusValid ;
  rdfs:comment "Note 1 to entry: See: object."@en ;
  rdfs:comment "비고: 객체를 참조하라."@kr ;
  rdfs:label "instance <UML>"@en ;
  skos:changeNote "valid" ;
  skos:definition "유일한 식별특성을 가지며, 연산의 집합이 적용될 수 있고, 연산의 효과를 저장할 수 있는 상태를 갖는 개체"@kr ;
  skos:editorialNote "preferred" ;
  skos:editorialNote "preferred"^^xsd:string ;
  skos:notation "727" ;
  skos:notation 727 ;
  skos:note "Note 1 to entry: See: object."@en ;
  skos:note "비고: 객체를 참조하라."@kr ;
  skos:prefLabel "instance <UML>"@en ;
  skos:prefLabel "인스턴스 <UML>"@kr ;
.
<http://iso.org/tc211/term/728>
  rdf:type skos:Concept ;
  dcterms:dateAccepted "2005-07-15"^^xsd:date ;
  dcterms:dateAccepted "2009-12-29"^^xsd:date ;
  dcterms:provenance "ISO/TS 19103:2005" ;
  dcterms:provenance "KS X ISO 19103" ;
  dcterms:source "ISO/IEC 19501:2005 (Adapted from)" ;
  reg:status reg:statusValid ;
  rdfs:comment "Note 1 to entry: A type may have attributes and associations."@en ;
  rdfs:comment "비고: 유형은 속성과 연관을 가질 수 있다."@kr ;
  rdfs:label "type <UML>"@en ;
  skos:changeNote "valid" ;
  skos:definition "대상 객체의 물리적 구현을 정의하지 않고, 객체에 적용할 수 있는 연산으로 객체의 영역을 기술한 정형화된 클래스"@kr ;
  skos:editorialNote "preferred" ;
  skos:editorialNote "preferred"^^xsd:string ;
  skos:notation "728" ;
  skos:notation 728 ;
  skos:note "Note 1 to entry: A type may have attributes and associations."@en ;
  skos:note "비고: 유형은 속성과 연관을 가질 수 있다."@kr ;
  skos:prefLabel "type <UML>"@en ;
  skos:prefLabel "유형 <UML>"@kr ;
.
<http://iso.org/tc211/term/729>
  rdf:type skos:Concept ;
  dcterms:dateAccepted "2007-07-01" ;
  dcterms:dateAccepted "2007-07-01"^^xsd:date ;
  dcterms:dateAccepted "2007-11-01"^^xsd:date ;
  dcterms:provenance "KS X ISO 19111" ;
  dcterms:source "ISO 19111:2007" ;
  reg:status reg:statusAccepted ;
  reg:status reg:statusValid ;
  rdfs:label "coordinate set"@en ;
  skos:changeNote "valid" ;
  skos:definition "verzameling coördinaattupels gerelateerd aan hetzelfde coördinaatreferentiesysteem"@nl ;
  skos:definition "동일한 좌표 참조 체계를 사용하는 좌표 튜플의 모음"@kr ;
  skos:editorialNote "preferred" ;
  skos:editorialNote "preferred"^^xsd:string ;
  skos:notation "729" ;
  skos:notation 729 ;
  skos:prefLabel "coordinate set"@en ;
  skos:prefLabel "coördinaten set"@nl ;
  skos:prefLabel "좌표 집합"@kr ;
.
<http://iso.org/tc211/term/73>
  rdf:type skos:Concept ;
  dcterms:dateAccepted "2000-12-15"^^xsd:date ;
  dcterms:dateAccepted "2007-06-29"^^xsd:date ;
  dcterms:provenance "KS X ISO 19105" ;
  dcterms:source "ISO 19105:2000" ;
  reg:status reg:statusValid ;
  rdfs:label "conformance clause"@en ;
  skos:changeNote "valid" ;
  skos:definition "표준의 요구사항 충족을 위해 필요한 것이 무엇인지를 정의하는 조항"@kr ;
  skos:editorialNote "preferred" ;
  skos:editorialNote "preferred"^^xsd:string ;
  skos:notation "73" ;
  skos:notation 73 ;
  skos:prefLabel "conformance clause"@en ;
  skos:prefLabel "적합성 조항"@kr ;
.
<http://iso.org/tc211/term/733>
  rdf:type skos:Concept ;
  dcterms:dateAccepted "2008-07-15"^^xsd:date ;
  dcterms:source "ISO 6709:2008" ;
  reg:status reg:statusValid ;
  rdfs:label "altitude"@en ;
  skos:changeNote "valid" ;
  skos:editorialNote "preferred"^^xsd:string ;
  skos:notation 733 ;
  skos:prefLabel "altitude"@en ;
.
<http://iso.org/tc211/term/734>
  rdf:type skos:Concept ;
  dcterms:dateAccepted "2005-10-15"^^xsd:date ;
  dcterms:dateAccepted "2006-12-01"^^xsd:date ;
  dcterms:provenance "KS X ISO 19133" ;
  dcterms:source "ISO 19133:2005" ;
  reg:status reg:statusValid ;
  rdfs:label "constraint"@en ;
  skos:changeNote "valid" ;
  skos:definition "차종, 물리적 또는 시간적 제약 조건과 같이, 차량에 의한 링크 또는 회전의 제한"@kr ;
  skos:editorialNote "preferred" ;
  skos:editorialNote "preferred"^^xsd:string ;
  skos:notation "734" ;
  skos:notation 734 ;
  skos:prefLabel "constraint"@en ;
  skos:prefLabel "제약 조건"@kr ;
.
<http://iso.org/tc211/term/735>
  rdf:type skos:Concept ;
  dcterms:dateAccepted "2007-07-01" ;
  dcterms:dateAccepted "2007-07-01"^^xsd:date ;
  dcterms:dateAccepted "2007-11-01"^^xsd:date ;
  dcterms:provenance "KS X ISO 19111" ;
  dcterms:source "ISO 19111:2007" ;
  reg:status reg:statusAccepted ;
  reg:status reg:statusValid ;
  rdfs:comment "Note 1 to entry: The number of coordinates in the coordinate tuple equals the dimension of the coordinate system; the order of coordinates in the coordinate tuple is identical to the order of the axes of the coordinate system."@en ;
  rdfs:comment "OPMERKING Het aantal coördinaten in een coördinaattupel is gelijk aan de dimensie van het coördinaatsysteem; de volgorde van de coördinaten in een coördinaattupel is gelijk aan de volgorde van de assen van het coördinaatsysteem."@en ;
  rdfs:comment "비고: 좌표 튜플의 좌표 개수는 좌표 체계의 차원과 같다. 좌표 튜플의 좌표 순서는 좌표 체계의 축 순서와 같다."@kr ;
  rdfs:label "coordinate tuple"@en ;
  skos:changeNote "valid" ;
  skos:definition "tupel bestaande uit een serie coördinaten"@nl ;
  skos:definition "좌표의 연속으로 구성된 튜플"@kr ;
  skos:editorialNote "preferred" ;
  skos:editorialNote "preferred"^^xsd:string ;
  skos:notation "735" ;
  skos:notation 735 ;
  skos:note "Note 1 to entry: The number of coordinates in the coordinate tuple equals the dimension of the coordinate system; the order of coordinates in the coordinate tuple is identical to the order of the axes of the coordinate system."@en ;
  skos:note "OPMERKING Het aantal coördinaten in een coördinaattupel is gelijk aan de dimensie van het coördinaatsysteem; de volgorde van de coördinaten in een coördinaattupel is gelijk aan de volgorde van de assen van het coördinaatsysteem."@en ;
  skos:note "비고: 좌표 튜플의 좌표 개수는 좌표 체계의 차원과 같다. 좌표 튜플의 좌표 순서는 좌표 체계의 축 순서와 같다."@kr ;
  skos:prefLabel "coordinate tuple"@en ;
  skos:prefLabel "coördinaattupel"@nl ;
  skos:prefLabel "좌표 튜플"@kr ;
.
<http://iso.org/tc211/term/736>
  rdf:type skos:Concept ;
  dcterms:dateAccepted "2006-12-01"^^xsd:date ;
  dcterms:dateAccepted "2007-11-30"^^xsd:date ;
  dcterms:provenance "ISO 19138:2006" ;
  dcterms:source "ISO 19157:2013, 4.5" ;
  reg:status reg:statusValid ;
  rdfs:label "correctness"@en ;
  skos:changeNote "valid" ;
  skos:definition "논의의 영역에 대한 부합 정도"@kr ;
  skos:editorialNote "preferred" ;
  skos:editorialNote "preferred"^^xsd:string ;
  skos:notation "736" ;
  skos:notation 736 ;
  skos:prefLabel "correctness"@en ;
  skos:prefLabel "정확성"@kr ;
.
<http://iso.org/tc211/term/738>
  rdf:type skos:Concept ;
  dcterms:dateAccepted "2006-12-01"^^xsd:date ;
  dcterms:dateAccepted "2007-11-01"^^xsd:date ;
  dcterms:source "ISO/TS 19138:2006, 4.4" ;
  reg:status reg:statusRetired ;
  rdfs:label "error"@en ;
  skos:changeNote "retired" ;
  skos:definition "논의의 영역과의 불일치"@kr ;
  skos:notation "738" ;
  skos:notation 738 ;
  skos:prefLabel "error"@en ;
  skos:prefLabel "오류"@kr ;
.
<http://iso.org/tc211/term/74>
  rdf:type skos:Concept ;
  dcterms:dateAccepted "2002-12-01"^^xsd:date ;
  dcterms:dateAccepted "2009-12-29"^^xsd:date ;
  dcterms:provenance "ISO 19113" ;
  dcterms:source "ISO 19114:2003, 4.1" ;
  reg:status reg:statusRetired ;
  rdfs:label "conformance quality level"@en ;
  skos:changeNote "retired" ;
  skos:definition "데이터셋이 제품 사양이나 사용자의 요구사항을 만족했는지를 결정하는데 사용되는 데이터 품질 결과에 대한 임계 값 또는 임계 값의 집합"@kr ;
  skos:notation "74" ;
  skos:notation 74 ;
  skos:prefLabel "conformance quality level"@en ;
  skos:prefLabel "적합성 품질 수준"@kr ;
.
<http://iso.org/tc211/term/740>
  rdf:type skos:Concept ;
  dcterms:dateAccepted "2005-10-15"^^xsd:date ;
  dcterms:dateAccepted "2006-12-01"^^xsd:date ;
  dcterms:provenance "KS X ISO 19133" ;
  dcterms:source "ISO 19133:2005" ;
  reg:status reg:statusValid ;
  rdfs:label "navigation constraint"@en ;
  skos:changeNote "valid" ;
  skos:definition "차종, 물리적, 시간적 제약 조건과 같이 차량의 링크나 회전에 대한 제약 조건"@kr ;
  skos:editorialNote "preferred" ;
  skos:editorialNote "preferred"^^xsd:string ;
  skos:notation "740" ;
  skos:notation 740 ;
  skos:prefLabel "navigation constraint"@en ;
  skos:prefLabel "내비게이션 제약 조건"@kr ;
.
<http://iso.org/tc211/term/744>
  rdf:type skos:Concept ;
  dcterms:dateAccepted "2005-10-15"^^xsd:date ;
  dcterms:dateAccepted "2006-12-01"^^xsd:date ;
  dcterms:provenance "KS X ISO 19133" ;
  dcterms:source "ISO 19133:2005" ;
  reg:status reg:statusValid ;
  rdfs:comment "Note 1 to entry: Includes pedestrians. See ISO 14825. In this International Standard, traveller can be replaced by vehicle without any change of intent."@en ;
  rdfs:comment "비고: 보행자를 포함한다. KS X ISO 14825를 참고하라. 본 표준에서는 어떠한 의도 변경 없이, 여행자가 차량으로 대체될 수 있다."@kr ;
  rdfs:label "traveller"@en ;
  rdfs:seeAlso "vehicle" ;
  skos:altLabel "vehicle"@en ;
  skos:changeNote "valid" ;
  skos:definition "내비게이션 또는 추적될 수 있는 사람 주체(차량과 비교)"@kr ;
  skos:editorialNote "preferred" ;
  skos:editorialNote "preferred"^^xsd:string ;
  skos:notation "744" ;
  skos:notation 744 ;
  skos:note "Note 1 to entry: Includes pedestrians. See ISO 14825. In this International Standard, traveller can be replaced by vehicle without any change of intent."@en ;
  skos:note "비고: 보행자를 포함한다. KS X ISO 14825를 참고하라. 본 표준에서는 어떠한 의도 변경 없이, 여행자가 차량으로 대체될 수 있다."@kr ;
  skos:prefLabel "traveller"@en ;
  skos:prefLabel "여행자"@kr ;
.
<http://iso.org/tc211/term/745>
  rdf:type skos:Concept ;
  dcterms:dateAccepted "2005-10-15"^^xsd:date ;
  dcterms:dateAccepted "2006-12-01"^^xsd:date ;
  dcterms:provenance "KS X ISO 19133" ;
  dcterms:source "ISO 19133:2005" ;
  reg:status reg:statusValid ;
  rdfs:comment "Note 1 to entry: Includes pedestrians. See ISO 14825. In this International Standard, vehicle can be replaced by traveller without any change of intent."@en ;
  rdfs:comment "비고: 보행자를 포함한다. KS X ISO 14825를 참고하라. 본 표준에서는 어떠한 의도 변경 없이, 차량이 여행자로 대체될 수 있다."@kr ;
  rdfs:label "vehicle"@en ;
  rdfs:seeAlso "traveller" ;
  skos:altLabel "traveller"@en ;
  skos:changeNote "valid" ;
  skos:definition "내비게이션 또는 추적될 수 있는 객체(여행자와 비교)"@kr ;
  skos:editorialNote "preferred" ;
  skos:editorialNote "preferred"^^xsd:string ;
  skos:notation "745" ;
  skos:notation 745 ;
  skos:note "Note 1 to entry: Includes pedestrians. See ISO 14825. In this International Standard, vehicle can be replaced by traveller without any change of intent."@en ;
  skos:note "비고: 보행자를 포함한다. KS X ISO 14825를 참고하라. 본 표준에서는 어떠한 의도 변경 없이, 차량이 여행자로 대체될 수 있다."@kr ;
  skos:prefLabel "vehicle"@en ;
  skos:prefLabel "차량"@kr ;
.
<http://iso.org/tc211/term/746>
  rdf:type skos:Concept ;
  dcterms:dateAccepted "2007-10-15"^^xsd:date ;
  dcterms:dateAccepted "2009-12-29"^^xsd:date ;
  dcterms:provenance "KS X ISO 19132" ;
  dcterms:source "ISO 19132:2007" ;
  reg:status reg:statusValid ;
  rdfs:comment "Note 1 to entry: Temporal versions differ from samples in that a complete description is required. In this sense a version is a complete sample able to be considered outside the domain of the temporal sequence to which it may belong."@en ;
  rdfs:comment "비고: 시간 버전은 완벽한 설명이 필요한 샘플과 구별된다. 이 점에서 버전은 이것이 포함될 수 있는 시간 연속 영역 외부의 완전한 샘플이다."@kr ;
  rdfs:label "version (temporal)"@en ;
  skos:changeNote "valid" ;
  skos:definition "특정 시간에 제시된 인스턴스 객체의 완전성에 대한 표현"@kr ;
  skos:editorialNote "preferred" ;
  skos:editorialNote "preferred"^^xsd:string ;
  skos:notation "746" ;
  skos:notation 746 ;
  skos:note "Note 1 to entry: Temporal versions differ from samples in that a complete description is required. In this sense a version is a complete sample able to be considered outside the domain of the temporal sequence to which it may belong."@en ;
  skos:note "비고: 시간 버전은 완벽한 설명이 필요한 샘플과 구별된다. 이 점에서 버전은 이것이 포함될 수 있는 시간 연속 영역 외부의 완전한 샘플이다."@kr ;
  skos:prefLabel "version (temporal)"@en ;
  skos:prefLabel "버전(시간)"@kr ;
.
<http://iso.org/tc211/term/75>
  rdf:type skos:Concept ;
  dcterms:dateAccepted "2000-12-15"^^xsd:date ;
  dcterms:dateAccepted "2007-06-29"^^xsd:date ;
  dcterms:provenance "KS X ISO 19105" ;
  dcterms:source "ISO 19105:2000" ;
  reg:status reg:statusValid ;
  rdfs:label "conformance test report"@en ;
  skos:changeNote "valid" ;
  skos:definition "시험의 상세 내용과 표준에 대한 적합성 여부를 요약한 보고서"@kr ;
  skos:editorialNote "preferred" ;
  skos:editorialNote "preferred"^^xsd:string ;
  skos:notation "75" ;
  skos:notation 75 ;
  skos:prefLabel "conformance test report"@en ;
  skos:prefLabel "적합성 시험 보고서"@kr ;
.
<http://iso.org/tc211/term/754>
  rdf:type skos:Concept ;
  dcterms:dateAccepted "2008-06-01"^^xsd:date ;
  dcterms:source "ISO 19141:2008" ;
  reg:status reg:statusValid ;
  rdfs:label "design coordinate reference system"@en ;
  skos:changeNote "valid" ;
  skos:editorialNote "preferred"^^xsd:string ;
  skos:notation 754 ;
  skos:prefLabel "design coordinate reference system"@en ;
.
<http://iso.org/tc211/term/755>
  rdf:type skos:Concept ;
  dcterms:dateAccepted "2002-07-01"^^xsd:date ;
  dcterms:dateAccepted "2008-12-30"^^xsd:date ;
  dcterms:provenance "ISO 19101:2002" ;
  dcterms:source "ISO 19101-1:2014, 4.1.21" ;
  reg:status reg:statusValid ;
  rdfs:label "graphical language"@en ;
  skos:changeNote "valid" ;
  skos:definition "그래픽 기호를 통해 문법을 표현하는 언어"@kr ;
  skos:editorialNote "preferred" ;
  skos:editorialNote "preferred"^^xsd:string ;
  skos:notation "755" ;
  skos:notation 755 ;
  skos:prefLabel "graphical language"@en ;
  skos:prefLabel "그래픽 언어"@kr ;
.
<http://iso.org/tc211/term/756>
  rdf:type skos:Concept ;
  dcterms:dateAccepted "2003-05-01"^^xsd:date ;
  dcterms:dateAccepted "2009-12-29"^^xsd:date ;
  dcterms:provenance "KS X ISO 19107" ;
  dcterms:source "ISO 19107:2003" ;
  reg:status reg:statusValid ;
  rdfs:comment "Note 1 to entry: In geographic information systems, a graph can have more than one edge joining two nodes, and can have an edge that has the same node at both ends."@en ;
  rdfs:comment "비고: 지리 정보 시스템에서, 그래프는 두 개 절점을 연결하는 하나 이상의 변과, 두 개의 끝점이 같은 절점으로 된 변으로 구성될 수 있다. "@kr ;
  rdfs:label "graph"@en ;
  skos:changeNote "valid" ;
  skos:definition "변에 의해 결합된 절점의 집합"@kr ;
  skos:editorialNote "preferred" ;
  skos:editorialNote "preferred"^^xsd:string ;
  skos:notation "756" ;
  skos:notation 756 ;
  skos:note "Note 1 to entry: In geographic information systems, a graph can have more than one edge joining two nodes, and can have an edge that has the same node at both ends."@en ;
  skos:note "비고: 지리 정보 시스템에서, 그래프는 두 개 절점을 연결하는 하나 이상의 변과, 두 개의 끝점이 같은 절점으로 된 변으로 구성될 수 있다. "@kr ;
  skos:prefLabel "graph"@en ;
  skos:prefLabel "그래프"@kr ;
.
<http://iso.org/tc211/term/757>
  rdf:type skos:Concept ;
  dcterms:dateAccepted "2005-08-15"^^xsd:date ;
  dcterms:dateAccepted "2007-11-01"^^xsd:date ;
  dcterms:provenance "KS X ISO 19123" ;
  dcterms:source "ISO 19123:2005" ;
  reg:status reg:statusValid ;
  rdfs:label "geometry value object"@en ;
  skos:changeNote "valid" ;
  skos:definition "기하 값 쌍의 집합으로 구성된 객체"@kr ;
  skos:editorialNote "preferred" ;
  skos:editorialNote "preferred"^^xsd:string ;
  skos:notation "757" ;
  skos:notation 757 ;
  skos:prefLabel "geometry value object"@en ;
  skos:prefLabel "기하 값 객체"@kr ;
.
<http://iso.org/tc211/term/758>
  rdf:type skos:Concept ;
  dcterms:dateAccepted "2005-08-15"^^xsd:date ;
  dcterms:dateAccepted "2007-11-01"^^xsd:date ;
  dcterms:provenance "KS X ISO 19123" ;
  dcterms:source "ISO 19123:2005" ;
  reg:status reg:statusValid ;
  rdfs:label "geometry value pair"@en ;
  skos:changeNote "valid" ;
  skos:definition "공간 객체, 시간 객체, 시공간 객체 및 피처 속성 값의 레코드로 구성된 일련의 값 쌍 "@kr ;
  skos:editorialNote "preferred" ;
  skos:editorialNote "preferred"^^xsd:string ;
  skos:notation "758" ;
  skos:notation 758 ;
  skos:prefLabel "geometry value pair"@en ;
  skos:prefLabel "기하 값 쌍"@kr ;
.
<http://iso.org/tc211/term/76>
  rdf:type skos:Concept ;
  dcterms:dateAccepted "2000-12-15"^^xsd:date ;
  dcterms:dateAccepted "2007-06-29"^^xsd:date ;
  dcterms:provenance "KS X ISO 19105" ;
  dcterms:source "ISO 19105:2000" ;
  reg:status reg:statusValid ;
  rdfs:label "conformance testing"@en ;
  skos:changeNote "valid" ;
  skos:definition "구현된 제품의 적합 정도를 결정하기 위한 시험"@kr ;
  skos:editorialNote "preferred" ;
  skos:editorialNote "preferred"^^xsd:string ;
  skos:notation "76" ;
  skos:notation 76 ;
  skos:prefLabel "conformance testing"@en ;
  skos:prefLabel "적합성 시험"@kr ;
.
<http://iso.org/tc211/term/762>
  rdf:type skos:Concept ;
  dcterms:dateAccepted "2007-07-01" ;
  dcterms:dateAccepted "2007-07-01"^^xsd:date ;
  dcterms:dateAccepted "2007-11-01"^^xsd:date ;
  dcterms:provenance "KS X ISO 19111" ;
  dcterms:source "ISO 19111:2007" ;
  reg:status reg:statusAccepted ;
  reg:status reg:statusValid ;
  rdfs:comment "Note 1 to entry: A coordinate conversion uses parameters which have specified values that are not determined empirically."@en ;
  rdfs:comment "OPMERKING Een coördinaat conversie gebruikt parameters die gespecificeerde waarden hebben die niet empirisch bepaald zijn."@en ;
  rdfs:comment "비고: 좌표 전환은 경험적으로 산출된 값이 아닌 특정 값을 매개 변수로 사용한다."@kr ;
  rdfs:label "coordinate conversion"@en ;
  skos:changeNote "valid" ;
  skos:definition "coördinaatbewerking waarbij beide coördinaatreferentiesystemen op hetzelfde datum gebaseerd zijn."@nl ;
  skos:definition "동일한 데이텀을 기준으로 하는 두 개의 좌표 참조 체계에서의 좌표 연산"@kr ;
  skos:editorialNote "preferred" ;
  skos:editorialNote "preferred"^^xsd:string ;
  skos:notation "762" ;
  skos:notation 762 ;
  skos:note "Note 1 to entry: A coordinate conversion uses parameters which have specified values that are not determined empirically."@en ;
  skos:note "OPMERKING Een coördinaat conversie gebruikt parameters die gespecificeerde waarden hebben die niet empirisch bepaald zijn."@en ;
  skos:note "비고: 좌표 전환은 경험적으로 산출된 값이 아닌 특정 값을 매개 변수로 사용한다."@kr ;
  skos:prefLabel "Coördinaat conversie"@nl ;
  skos:prefLabel "coordinate conversion"@en ;
  skos:prefLabel "좌표 전환"@kr ;
.
<http://iso.org/tc211/term/763>
  rdf:type skos:Concept ;
  dcterms:dateAccepted "2007-07-01" ;
  dcterms:dateAccepted "2007-07-01"^^xsd:date ;
  dcterms:dateAccepted "2007-11-01"^^xsd:date ;
  dcterms:provenance "KS X ISO 19111" ;
  dcterms:source "ISO 19111:2007" ;
  reg:status reg:statusAccepted ;
  reg:status reg:statusValid ;
  rdfs:comment "Note 1 to entry: A coordinate transformation uses parameters which are derived empirically by a set of points with known coordinates in both coordinate reference systems."@en ;
  rdfs:comment "OPMERKING Een coördinaat transformatie gebruikt parameters die empirisch zijn afgeleid uit een set punten met bekende coördinaten in beide coördinaatreferentiesystemen."@en ;
  rdfs:comment "비고: 좌표 변환은 경험적 매개 변수를 사용한다. 이는 두 개의 좌표 참조 체계에서 미리 알려진 좌표 점의 집합을 통해 도출된 것이다."@kr ;
  rdfs:label "coordinate transformation"@en ;
  skos:changeNote "valid" ;
  skos:definition "coördinaatbewerking waarbij de twee coördinaatreferentiesystemen zijn gebaseerd op verschillende datums"@nl ;
  skos:definition "서로 다른 데이텀을 기준으로 하는 두 개의 좌표 참조 체계에서의 좌표 연산"@kr ;
  skos:editorialNote "preferred" ;
  skos:editorialNote "preferred"^^xsd:string ;
  skos:notation "763" ;
  skos:notation 763 ;
  skos:note "Note 1 to entry: A coordinate transformation uses parameters which are derived empirically by a set of points with known coordinates in both coordinate reference systems."@en ;
  skos:note "OPMERKING Een coördinaat transformatie gebruikt parameters die empirisch zijn afgeleid uit een set punten met bekende coördinaten in beide coördinaatreferentiesystemen."@en ;
  skos:note "비고: 좌표 변환은 경험적 매개 변수를 사용한다. 이는 두 개의 좌표 참조 체계에서 미리 알려진 좌표 점의 집합을 통해 도출된 것이다."@kr ;
  skos:prefLabel "coordinate transformation"@en ;
  skos:prefLabel "coördinaat transformatie"@nl ;
  skos:prefLabel "좌표 변환"@kr ;
.
<http://iso.org/tc211/term/764>
  rdf:type skos:Concept ;
  dcterms:dateAccepted "2007-07-01" ;
  dcterms:dateAccepted "2007-07-01"^^xsd:date ;
  dcterms:dateAccepted "2007-11-01"^^xsd:date ;
  dcterms:provenance "KS X ISO 19111" ;
  dcterms:source "ISO 19111:2007" ;
  reg:status reg:statusAccepted ;
  reg:status reg:statusValid ;
  rdfs:label "geoid"@en ;
  skos:changeNote "valid" ;
  skos:definition "equipotentiaal vlak van het zwaartekrachtveld van de aarde dat overal loodrecht staat op de richting van de zwaartekracht en dat het best aansluit bij het lokale of globale gemiddeld zeeniveau"@nl ;
  skos:definition "어디에서나 중력 방향에 수직이며, 국지적 또는 전지구적으로 평균 해수면에 가장 근접하는 지구 중력 등위 표면"@kr ;
  skos:editorialNote "preferred" ;
  skos:editorialNote "preferred"^^xsd:string ;
  skos:notation "764" ;
  skos:notation 764 ;
  skos:prefLabel "geoid"@en ;
  skos:prefLabel "geoide"@nl ;
  skos:prefLabel "지오이드"@kr ;
.
<http://iso.org/tc211/term/765>
  rdf:type skos:Concept ;
  dcterms:dateAccepted "2007-07-01" ;
  dcterms:dateAccepted "2007-07-01"^^xsd:date ;
  dcterms:dateAccepted "2007-11-01"^^xsd:date ;
  dcterms:provenance "KS X ISO 19111" ;
  dcterms:source "ISO 19111:2007" ;
  reg:status reg:statusAccepted ;
  reg:status reg:statusValid ;
  rdfs:label "projected coordinate reference system"@en ;
  skos:changeNote "valid" ;
  skos:definition "2차원 측지 좌표 참조 체계로부터 지도 투영을 통해 파생된 좌표 참조 체계"@kr ;
  skos:definition "coördinaatreferentiesysteem afgeleid van een tweedimensionaal geodetisch referentiesysteem door het toepassen van een kaartprojectie"@nl ;
  skos:editorialNote "preferred" ;
  skos:editorialNote "preferred"^^xsd:string ;
  skos:notation "765" ;
  skos:notation 765 ;
  skos:prefLabel "geprojecteerd coördinaatreferentiesysteem"@nl ;
  skos:prefLabel "projected coordinate reference system"@en ;
  skos:prefLabel "투영 좌표 참조 체계"@kr ;
.
<http://iso.org/tc211/term/77>
  rdf:type skos:Concept ;
  dcterms:dateAccepted "2000-12-15"^^xsd:date ;
  dcterms:dateAccepted "2007-06-29"^^xsd:date ;
  dcterms:provenance "KS X ISO 19105" ;
  dcterms:source "ISO 19105:2000" ;
  reg:status reg:statusValid ;
  rdfs:label "conforming implementation"@en ;
  skos:changeNote "valid" ;
  skos:definition "적합성 요건을 만족시키는 구현"@kr ;
  skos:editorialNote "preferred" ;
  skos:editorialNote "preferred"^^xsd:string ;
  skos:notation "77" ;
  skos:notation 77 ;
  skos:prefLabel "conforming implementation"@en ;
  skos:prefLabel "적합성 구현"@kr ;
.
<http://iso.org/tc211/term/774>
  rdf:type skos:Concept ;
  dcterms:dateAccepted "2010-10-15"^^xsd:date ;
  dcterms:source "ISO 19143:2010" ;
  reg:status reg:statusValid ;
  rdfs:label "feature reference"@en ;
  skos:changeNote "valid" ;
  skos:editorialNote "preferred"^^xsd:string ;
  skos:notation 774 ;
  skos:prefLabel "feature reference"@en ;
.
<http://iso.org/tc211/term/78>
  rdf:type skos:Concept ;
  dcterms:dateAccepted "2003-05-01"^^xsd:date ;
  dcterms:dateAccepted "2009-12-29"^^xsd:date ;
  dcterms:provenance "KS X ISO 19107" ;
  dcterms:source "ISO 19107:2003" ;
  reg:status reg:statusValid ;
  rdfs:comment "Note 1 to entry: A topological object is connected if and only if all its geometric realizations are connected. This is not included as a definition because it follows from a theorem of topology."@en ;
  rdfs:comment "비고: 위상 객체는 기하 실현이 실제로 연결되어 있어야만 '연결되었다'라고 할 수 있다. 이는 위상학적 규칙을 따라야 하는 것으로 정의에 포함되지는 않는다."@kr ;
  rdfs:label "connected"@en ;
  skos:changeNote "valid" ;
  skos:definition "객체에서 임의의 두 개의 직접 위치가 그 객체 내부에 완전하게 포함되는 곡선상에 위치할 수 있는 것을 의미하는 기하 객체의 특성"@kr ;
  skos:editorialNote "preferred" ;
  skos:editorialNote "preferred"^^xsd:string ;
  skos:notation "78" ;
  skos:notation 78 ;
  skos:note "Note 1 to entry: A topological object is connected if and only if all its geometric realizations are connected. This is not included as a definition because it follows from a theorem of topology."@en ;
  skos:note "비고: 위상 객체는 기하 실현이 실제로 연결되어 있어야만 '연결되었다'라고 할 수 있다. 이는 위상학적 규칙을 따라야 하는 것으로 정의에 포함되지는 않는다."@kr ;
  skos:prefLabel "connected"@en ;
  skos:prefLabel "연결"@kr ;
.
<http://iso.org/tc211/term/785>
  rdf:type skos:Concept ;
  dcterms:dateAccepted "2010-12-15"^^xsd:date ;
  dcterms:provenance "ISO 19142:2010" ;
  dcterms:source "W3C XLink:2001" ;
  reg:status reg:statusValid ;
  rdfs:label "traversal <XML>"@en ;
  skos:changeNote "valid" ;
  skos:editorialNote "preferred"^^xsd:string ;
  skos:notation 785 ;
  skos:prefLabel "traversal <XML>"@en ;
.
<http://iso.org/tc211/term/789>
  rdf:type skos:Concept ;
  dcterms:dateAccepted "2008-06-01"^^xsd:date ;
  dcterms:source "ISO/TS 19101-2:2008" ;
  reg:status reg:statusValid ;
  rdfs:label "digital elevation model"@en ;
  skos:changeNote "valid" ;
  skos:editorialNote "preferred"^^xsd:string ;
  skos:notation 789 ;
  skos:prefLabel "digital elevation model"@en ;
.
<http://iso.org/tc211/term/79>
  rdf:type skos:Concept ;
  dcterms:dateAccepted "2003-05-01"^^xsd:date ;
  dcterms:dateAccepted "2009-12-29"^^xsd:date ;
  dcterms:provenance "KS X ISO 19107" ;
  dcterms:source "ISO 19107:2003" ;
  reg:status reg:statusValid ;
  rdfs:label "connected node"@en ;
  skos:changeNote "valid" ;
  skos:definition "한 개 이상의 변으로 시작하거나 끝나는 절점"@kr ;
  skos:editorialNote "preferred" ;
  skos:editorialNote "preferred"^^xsd:string ;
  skos:notation "79" ;
  skos:notation 79 ;
  skos:prefLabel "connected node"@en ;
  skos:prefLabel "연결 절점"@kr ;
.
<http://iso.org/tc211/term/790>
  rdf:type skos:Concept ;
  dcterms:dateAccepted "2008-06-01"^^xsd:date ;
  dcterms:source "ISO/TS 19101-2:2008" ;
  reg:status reg:statusValid ;
  rdfs:label "digital number"@en ;
  skos:altLabel "DN"^^<http://www.w3.org/2001/XMLSchema#@en> ;
  skos:changeNote "valid" ;
  skos:editorialNote "preferred"^^xsd:string ;
  skos:notation 790 ;
  skos:prefLabel "digital number"@en ;
.
<http://iso.org/tc211/term/792>
  rdf:type skos:Concept ;
  dcterms:dateAccepted "2008-06-01"^^xsd:date ;
  dcterms:source "ISO/TS 19101-2:2008" ;
  reg:status reg:statusValid ;
  rdfs:label "geographic imagery"@en ;
  skos:changeNote "valid" ;
  skos:editorialNote "preferred"^^xsd:string ;
  skos:notation 792 ;
  skos:prefLabel "geographic imagery"@en ;
.
<http://iso.org/tc211/term/793>
  rdf:type skos:Concept ;
  dcterms:dateAccepted "2008-06-01"^^xsd:date ;
  dcterms:provenance "ISO/TS 19101-2:2008" ;
  dcterms:source "ISO 22028-1 (Derived from)" ;
  reg:status reg:statusValid ;
  rdfs:comment "Note 1 to entry:  A geographic imagery scene is a representation of an environmental landscape; it may correspond to a remotely sensed view of the natural world or to a computer-generated virtual scene simulating such a view"@en ;
  rdfs:label "geographic imagery scene"@en ;
  skos:changeNote "valid" ;
  skos:editorialNote "preferred"^^xsd:string ;
  skos:notation 793 ;
  skos:note "Note 1 to entry:  A geographic imagery scene is a representation of an environmental landscape; it may correspond to a remotely sensed view of the natural world or to a computer-generated virtual scene simulating such a view"@en ;
  skos:prefLabel "geographic imagery scene"@en ;
.
<http://iso.org/tc211/term/794>
  rdf:type skos:Concept ;
  dcterms:dateAccepted "2008-06-01"^^xsd:date ;
  dcterms:provenance "ISO/TS 19101-2:2008" ;
  dcterms:source "International Vocabulary of Basic and General Terms in Metrology (VIM) (Derived from)" ;
  reg:status reg:statusValid ;
  rdfs:label "metric traceability"@en ;
  skos:changeNote "valid" ;
  skos:editorialNote "preferred"^^xsd:string ;
  skos:notation 794 ;
  skos:prefLabel "metric traceability"@en ;
.
<http://iso.org/tc211/term/795>
  rdf:type skos:Concept ;
  dcterms:dateAccepted "2008-06-01"^^xsd:date ;
  dcterms:source "ISO/TS 19101-2:2008" ;
  reg:status reg:statusValid ;
  rdfs:comment "Note 1 to entry: The amount of displacement depends on the resolution and the level of detail of the elevation information and on the software implementation."@en ;
  rdfs:label "orthoimage"@en ;
  skos:changeNote "valid" ;
  skos:editorialNote "preferred"^^xsd:string ;
  skos:notation 795 ;
  skos:note "Note 1 to entry: The amount of displacement depends on the resolution and the level of detail of the elevation information and on the software implementation."@en ;
  skos:prefLabel "orthoimage"@en ;
.
<http://iso.org/tc211/term/8>
  rdf:type skos:Concept ;
  dcterms:dateAccepted "2002-12-01"^^xsd:date ;
  dcterms:dateAccepted "2008-12-19"^^xsd:date ;
  dcterms:provenance "ISO 19113:2002" ;
  dcterms:provenance "KS X ISO 19104" ;
  dcterms:source "ISO 3534-1:1993" ;
  reg:status reg:statusSuperseded ;
  rdfs:comment "Note 1 to entry: A test result can be observations or measurements."@en ;
  rdfs:comment "비고: 시험 결과는 관측 값 또는 측정 값이 될 수 있다."@kr ;
  rdfs:label "accuracy"@en ;
  skos:changeNote "superseded" ;
  skos:definition "시험 결과와 기준 값 간의 일치도를 표시하는 척도"@kr ;
  skos:notation "8" ;
  skos:notation 8 ;
  skos:note "Note 1 to entry: A test result can be observations or measurements."@en ;
  skos:note "비고: 시험 결과는 관측 값 또는 측정 값이 될 수 있다."@kr ;
  skos:prefLabel "accuracy"@en ;
  skos:prefLabel "정확도"@kr ;
.
<http://iso.org/tc211/term/800>
  rdf:type skos:Concept ;
  dcterms:dateAccepted "2011-10-15"^^xsd:date ;
  dcterms:source "ISO 19118:2011, 4.32" ;
  reg:status reg:statusValid ;
  rdfs:comment "Note 1 to entry: A transfer unit does not have to be identifiable like a dataset."@en ;
  rdfs:label "transfer unit"@en ;
  skos:changeNote "valid" ;
  skos:editorialNote "preferred"^^xsd:string ;
  skos:notation 800 ;
  skos:note "Note 1 to entry: A transfer unit does not have to be identifiable like a dataset."@en ;
  skos:prefLabel "transfer unit"@en ;
.
<http://iso.org/tc211/term/801>
  rdf:type skos:Concept ;
  dcterms:dateAccepted "2005-10-15"^^xsd:date ;
  dcterms:provenance "ISO 19135:2005" ;
  dcterms:source "ISO/IEC 11179-3:2003(Adapted from)" ;
  reg:status reg:statusValid ;
  rdfs:label "identifier"@en ;
  skos:changeNote "valid" ;
  skos:editorialNote "preferred"^^xsd:string ;
  skos:notation 801 ;
  skos:prefLabel "identifier"@en ;
.
<http://iso.org/tc211/term/807>
  rdf:type skos:Concept ;
  dcterms:dateAccepted "2010-10-15"^^xsd:date ;
  dcterms:source "ISO 19143:2010" ;
  reg:status reg:statusValid ;
  rdfs:label "predicate"@en ;
  skos:changeNote "valid" ;
  skos:editorialNote "preferred"^^xsd:string ;
  skos:notation 807 ;
  skos:prefLabel "predicate"@en ;
.
<http://iso.org/tc211/term/808>
  rdf:type skos:Concept ;
  dcterms:dateAccepted "2010-10-15"^^xsd:date ;
  dcterms:source "ISO 19143:2010" ;
  reg:status reg:statusValid ;
  rdfs:label "predicate expression"@en ;
  skos:changeNote "valid" ;
  skos:editorialNote "preferred"^^xsd:string ;
  skos:notation 808 ;
  skos:prefLabel "predicate expression"@en ;
.
<http://iso.org/tc211/term/809>
  rdf:type skos:Concept ;
  dcterms:dateAccepted "2010-10-15"^^xsd:date ;
  dcterms:source "ISO 19143:2010" ;
  reg:status reg:statusValid ;
  rdfs:label "property"@en ;
  skos:changeNote "valid" ;
  skos:editorialNote "preferred"^^xsd:string ;
  skos:notation 809 ;
  skos:prefLabel "property"@en ;
.
<http://iso.org/tc211/term/81>
  rdf:type skos:Concept ;
  dcterms:dateAccepted "2005-07-15"^^xsd:date ;
  dcterms:dateAccepted "2009-12-29"^^xsd:date ;
  dcterms:provenance "ISO/TS 19103:2005 ,4.2.11" ;
  dcterms:source "ISO/IEC 19501" ;
  reg:status reg:statusValid ;
  rdfs:comment "Note 1 to entry: Certain constraints are predefined in the UML, others may be user defined.  Constraints are one of three extensibility mechanisms in UML. See: tagged value, stereotype."@en ;
  rdfs:comment "비고: 영역은 속성, 연산자, 함수에 대한 영역 집합 및 범위 집합을 정의하는데 사용된다."@kr ;
  rdfs:label "constraint <UML>"@en ;
  skos:changeNote "valid" ;
  skos:definition "의미론적 조건 또는 제한"@kr ;
  skos:editorialNote "preferred" ;
  skos:editorialNote "preferred"^^xsd:string ;
  skos:notation "81" ;
  skos:notation 81 ;
  skos:note "Note 1 to entry: Certain constraints are predefined in the UML, others may be user defined.  Constraints are one of three extensibility mechanisms in UML. See: tagged value, stereotype."@en ;
  skos:note "비고: 영역은 속성, 연산자, 함수에 대한 영역 집합 및 범위 집합을 정의하는데 사용된다."@kr ;
  skos:prefLabel "constraint <UML>"@en ;
  skos:prefLabel "제약 조건 <UML>"@kr ;
.
<http://iso.org/tc211/term/810>
  rdf:type skos:Concept ;
  dcterms:dateAccepted "2009-08-15"^^xsd:date ;
  dcterms:source "ISO 19144-1:2009" ;
  reg:status reg:statusValid ;
  rdfs:label "classification system"@en ;
  skos:changeNote "valid" ;
  skos:editorialNote "preferred"^^xsd:string ;
  skos:notation 810 ;
  skos:prefLabel "classification system"@en ;
.
<http://iso.org/tc211/term/813>
  rdf:type skos:Concept ;
  dcterms:dateAccepted "2009-08-15"^^xsd:date ;
  dcterms:source "ISO 19144-1:2009" ;
  reg:status reg:statusValid ;
  rdfs:comment "Note 1 to entry: Taken from FAO LCCS version 2 (see Reference [2] in ISO 19144-1:2009)."@en ;
  rdfs:label "legend"@en ;
  skos:changeNote "valid" ;
  skos:editorialNote "preferred"^^xsd:string ;
  skos:notation 813 ;
  skos:note "Note 1 to entry: Taken from FAO LCCS version 2 (see Reference [2] in ISO 19144-1:2009)."@en ;
  skos:prefLabel "legend"@en ;
.
<http://iso.org/tc211/term/815>
  rdf:type skos:Concept ;
  dcterms:dateAccepted "2009-08-15"^^xsd:date ;
  dcterms:source "ISO 19144-1:2009" ;
  reg:status reg:statusValid ;
  rdfs:comment "Note 1 to entry: Taken from FAO LCCS version 2 (see Reference [2] in ISO 19144-1)"@en ;
  rdfs:comment "Note 2 to entry: See Annex B [of ISO 19144-1] for an examination of this and a priori classification" ;
  rdfs:label "a posteriori classification"@en ;
  skos:changeNote "valid" ;
  skos:editorialNote "preferred"^^xsd:string ;
  skos:notation 815 ;
  skos:note "Note 1 to entry: Taken from FAO LCCS version 2 (see Reference [2] in ISO 19144-1)"@en ;
  skos:note "Note 2 to entry: See Annex B [of ISO 19144-1] for an examination of this and a priori classification"^^<http://www.w3.org/2001/XMLSchema#@en> ;
  skos:prefLabel "a posteriori classification"@en ;
.
<http://iso.org/tc211/term/816>
  rdf:type skos:Concept ;
  dcterms:dateAccepted "2009-08-15"^^xsd:date ;
  dcterms:source "ISO 19144-1:2009" ;
  reg:status reg:statusValid ;
  rdfs:comment "Note 1 to entry: Taken from FAO LCCS version 2 (see Reference [2] in ISO 19144-1)"@en ;
  rdfs:comment "Note 2 to entry: The approach is based upon definition of classes before any data collection actually takes place" ;
  rdfs:comment "Note 3 to entry: See Annex B [of ISO 19144-1] for an examination of this and a posteriori classification"@en ;
  rdfs:label "a priori classification"@en ;
  skos:changeNote "valid" ;
  skos:editorialNote "preferred"^^xsd:string ;
  skos:notation 816 ;
  skos:note "Note 1 to entry: Taken from FAO LCCS version 2 (see Reference [2] in ISO 19144-1)"@en ;
  skos:note "Note 2 to entry: The approach is based upon definition of classes before any data collection actually takes place"^^<http://www.w3.org/2001/XMLSchema#@en> ;
  skos:note "Note 3 to entry: See Annex B [of ISO 19144-1] for an examination of this and a posteriori classification"^^<http://www.w3.org/2001/XMLSchema#@en> ;
  skos:prefLabel "a priori classification"@en ;
.
<http://iso.org/tc211/term/819>
  rdf:type skos:Concept ;
  dcterms:dateAccepted "2012-07-01"^^xsd:date ;
  dcterms:provenance "ISO 19144-2:2012, 4.1.7" ;
  dcterms:source "UNFAO LCCS 2:2005" ;
  reg:status reg:statusValid ;
  rdfs:comment "Note 1 to entry: Land cover is distinct from land use."@en ;
  rdfs:label "land cover"@en ;
  skos:changeNote "valid" ;
  skos:editorialNote "preferred"^^xsd:string ;
  skos:notation 819 ;
  skos:note "Note 1 to entry: Land cover is distinct from land use."@en ;
  skos:prefLabel "land cover"@en ;
.
<http://iso.org/tc211/term/82>
  rdf:type skos:Concept ;
  dcterms:dateAccepted "2009-04-01"^^xsd:date ;
  dcterms:source "ISO/TS 19129:2009" ;
  reg:status reg:statusValid ;
  rdfs:comment "Note 1 to entry: The term \"information view\" comes from the ISO Reference Model for Open Distributed Processing (RM-ODP) as specified in 19101-2."@en ;
  rdfs:label "content model"@en ;
  skos:changeNote "valid" ;
  skos:editorialNote "preferred"^^xsd:string ;
  skos:notation 82 ;
  skos:note "Note 1 to entry: The term \"information view\" comes from the ISO Reference Model for Open Distributed Processing (RM-ODP) as specified in 19101-2."@en ;
  skos:prefLabel "content model"@en ;
.
<http://iso.org/tc211/term/824>
  rdf:type skos:Concept ;
  dcterms:dateAccepted "2007-09-01"^^xsd:date ;
  dcterms:dateAccepted "2009-12-29"^^xsd:date ;
  dcterms:provenance "KS X ISO 19136" ;
  dcterms:source "ISO 19136:2007" ;
  reg:status reg:statusValid ;
  rdfs:label "GML document"@en ;
  skos:changeNote "valid" ;
  skos:definition "GML 스키마에 정의된 AbstractFeature, Dicitionary, TopoComplex 등 중 하나의 기본 요소 또는 이들을 대체할 수 있는 요소를 갖는 XML 문서"@kr ;
  skos:editorialNote "preferred" ;
  skos:editorialNote "preferred"^^xsd:string ;
  skos:notation "824" ;
  skos:notation 824 ;
  skos:prefLabel "GML document"@en ;
  skos:prefLabel "GML 문서"@kr ;
.
<http://iso.org/tc211/term/825>
  rdf:type skos:Concept ;
  dcterms:dateAccepted "2007-09-01"^^xsd:date ;
  dcterms:dateAccepted "2009-12-29"^^xsd:date ;
  dcterms:provenance "KS X ISO 19136" ;
  dcterms:source "ISO 19136:2007" ;
  reg:status reg:statusValid ;
  rdfs:label "GML profile"@en ;
  skos:changeNote "valid" ;
  skos:definition "GML 스키마의 부분 집합"@kr ;
  skos:editorialNote "preferred" ;
  skos:editorialNote "preferred"^^xsd:string ;
  skos:notation "825" ;
  skos:notation 825 ;
  skos:prefLabel "GML profile"@en ;
  skos:prefLabel "GML 프로파일"@kr ;
.
<http://iso.org/tc211/term/826>
  rdf:type skos:Concept ;
  dcterms:dateAccepted "2007-09-01"^^xsd:date ;
  dcterms:dateAccepted "2009-12-29"^^xsd:date ;
  dcterms:provenance "KS X ISO 19136" ;
  dcterms:source "ISO 19136:2007" ;
  reg:status reg:statusValid ;
  rdfs:label "GML schema"@en ;
  skos:changeNote "valid" ;
  skos:definition "XML 이름 공간으로 표준에 기술된 \"http://www.opengis.net/gml/3.2\"를 사용하는 스키마 컴포넌트"@kr ;
  skos:editorialNote "preferred" ;
  skos:editorialNote "preferred"^^xsd:string ;
  skos:notation "826" ;
  skos:notation 826 ;
  skos:prefLabel "GML schema"@en ;
  skos:prefLabel "GML 스키마"@kr ;
.
<http://iso.org/tc211/term/83>
  rdf:type skos:Concept ;
  dcterms:dateAccepted "2005-08-15"^^xsd:date ;
  dcterms:dateAccepted "2007-11-01"^^xsd:date ;
  dcterms:provenance "KS X ISO 19123" ;
  dcterms:source "ISO 19123:2005" ;
  reg:status reg:statusValid ;
  rdfs:comment "Note 1 to entry: Although the domain of a continuous coverage is ordinarily bounded in terms of its spatial and/or temporal extent, it can be subdivided into an infinite number of direct positions."@en ;
  rdfs:comment "비고: 연속 커버리지의 영역이 통상적으로 시간 또는 공간 범위의 표현으로 한정될지라도, 이는 무한한 수의 위치로 세분될 수 있다."@kr ;
  rdfs:label "continuous coverage"@en ;
  skos:changeNote "valid" ;
  skos:definition "동일한 피처(공간 객체, 시간 객체, 시공간 객체) 속성값이 영역 내 서로 다른 직접 위치에서 다른 값을 갖는 커버리지"@kr ;
  skos:editorialNote "preferred" ;
  skos:editorialNote "preferred"^^xsd:string ;
  skos:notation "83" ;
  skos:notation 83 ;
  skos:note "Note 1 to entry: Although the domain of a continuous coverage is ordinarily bounded in terms of its spatial and/or temporal extent, it can be subdivided into an infinite number of direct positions."@en ;
  skos:note "비고: 연속 커버리지의 영역이 통상적으로 시간 또는 공간 범위의 표현으로 한정될지라도, 이는 무한한 수의 위치로 세분될 수 있다."@kr ;
  skos:prefLabel "continuous coverage"@en ;
  skos:prefLabel "연속 커버리지"@kr ;
.
<http://iso.org/tc211/term/831>
  rdf:type skos:Concept ;
  dcterms:dateAccepted "2009-02-15"^^xsd:date ;
  dcterms:source "ISO 19115-2:2009" ;
  reg:status reg:statusValid ;
  rdfs:label "platform"@en ;
  skos:changeNote "valid" ;
  skos:editorialNote "preferred"^^xsd:string ;
  skos:notation 831 ;
  skos:prefLabel "platform"@en ;
.
<http://iso.org/tc211/term/832>
  rdf:type skos:Concept ;
  dcterms:dateAccepted "2009-02-15"^^xsd:date ;
  dcterms:source "ISO 19115-2:2009" ;
  reg:status reg:statusValid ;
  rdfs:label "polarization"@en ;
  skos:changeNote "valid" ;
  skos:editorialNote "preferred"^^xsd:string ;
  skos:notation 832 ;
  skos:prefLabel "polarization"@en ;
.
<http://iso.org/tc211/term/835>
  rdf:type skos:Concept ;
  dcterms:dateAccepted "2009-02-15"^^xsd:date ;
  dcterms:source "ISO 19115-2:2009" ;
  reg:status reg:statusValid ;
  rdfs:label "spectral resolution"@en ;
  skos:changeNote "valid" ;
  skos:editorialNote "preferred"^^xsd:string ;
  skos:notation 835 ;
  skos:prefLabel "spectral resolution"@en ;
.
<http://iso.org/tc211/term/838>
  rdf:type skos:Concept ;
  dcterms:dateAccepted "2007-04-15"^^xsd:date ;
  dcterms:dateAccepted "2008-12-19"^^xsd:date ;
  dcterms:provenance "ISO/TS 19139:2007" ;
  dcterms:provenance "KS X ISO 19104" ;
  dcterms:source "W3C XML" ;
  reg:status reg:statusValid ;
  rdfs:label "namespace"@en ;
  skos:changeNote "valid" ;
  skos:definition "URI를 통해 식별 가능한, XML 문서에서 요소 명과 속성 명으로서 사용된 이름들의 모음 "@kr ;
  skos:editorialNote "preferred" ;
  skos:editorialNote "preferred"^^xsd:string ;
  skos:notation "838" ;
  skos:notation 838 ;
  skos:prefLabel "namespace"@en ;
  skos:prefLabel "이름 공간"@kr ;
.
<http://iso.org/tc211/term/839>
  rdf:type skos:Concept ;
  dcterms:dateAccepted "2007-04-15"^^xsd:date ;
  dcterms:dateAccepted "2008-12-19"^^xsd:date ;
  dcterms:provenance "ISO/TS 19139:2007 ,4.3" ;
  dcterms:source "Booch 1999(Adapted from)" ;
  reg:status reg:statusValid ;
  rdfs:label "realization"@en ;
  skos:changeNote "valid" ;
  skos:definition "분류자 간에 한 분류자가 다른 분류자의 실행을 보증하는 계약을 명시하는 분류자 간의 의미론적 관계"@kr ;
  skos:editorialNote "preferred" ;
  skos:editorialNote "preferred"^^xsd:string ;
  skos:notation "839" ;
  skos:notation 839 ;
  skos:prefLabel "realization"@en ;
  skos:prefLabel "실현"@kr ;
.
<http://iso.org/tc211/term/84>
  rdf:type skos:Concept ;
  dcterms:dateAccepted "2005-10-15"^^xsd:date ;
  dcterms:dateAccepted "2009-12-29"^^xsd:date ;
  dcterms:provenance "KS X ISO 19135" ;
  dcterms:source "ISO 19135:2005" ;
  reg:status reg:statusValid ;
  rdfs:label "control body"@en ;
  skos:changeNote "valid" ;
  skos:definition "등록물의 내용에 대한 결정권을 갖는 전문가 집단"@kr ;
  skos:editorialNote "preferred" ;
  skos:editorialNote "preferred"^^xsd:string ;
  skos:notation "84" ;
  skos:notation 84 ;
  skos:prefLabel "control body"@en ;
  skos:prefLabel "통제 기구"@kr ;
.
<http://iso.org/tc211/term/840>
  rdf:type skos:Concept ;
  dcterms:dateAccepted "2007-04-15"^^xsd:date ;
  dcterms:dateAccepted "2008-12-19"^^xsd:date ;
  dcterms:provenance "ISO/TS 19139:2007" ;
  dcterms:provenance "KS X ISO 19104" ;
  dcterms:source "http://searchsmallbizit.techtarget.com" ;
  reg:status reg:statusValid ;
  rdfs:comment "Note 1 to entry: There are several different kinds of polymorphism"@en ;
  rdfs:comment "비고: 다양한 유형의 다형이 존재한다."@kr ;
  rdfs:label "polymorphism"@en ;
  skos:changeNote "valid" ;
  skos:definition "다른 상황에서 다른 의미 또는 용도로 활용될 수 있는, 특히 변수, 함수 또는 객체 등의 개체와 같이 하나 이상의 형태를 가질 수 있는 특성"@kr ;
  skos:editorialNote "preferred" ;
  skos:editorialNote "preferred"^^xsd:string ;
  skos:notation "840" ;
  skos:notation 840 ;
  skos:note "Note 1 to entry: There are several different kinds of polymorphism"@en ;
  skos:note "비고: 다양한 유형의 다형이 존재한다."@kr ;
  skos:prefLabel "polymorphism"@en ;
  skos:prefLabel "다형"@kr ;
.
<http://iso.org/tc211/term/841>
  rdf:type skos:Concept ;
  dcterms:dateAccepted "2009-08-15"^^xsd:date ;
  dcterms:source "ISO 19111-2:2009" ;
  reg:status reg:statusValid ;
  rdfs:label "parametric coordinate system"@en ;
  skos:changeNote "valid" ;
  skos:editorialNote "preferred"^^xsd:string ;
  skos:notation 841 ;
  skos:prefLabel "parametric coordinate system"@en ;
.
<http://iso.org/tc211/term/842>
  rdf:type skos:Concept ;
  dcterms:dateAccepted "2009-08-15"^^xsd:date ;
  dcterms:source "ISO 19111-2:2009" ;
  reg:status reg:statusValid ;
  rdfs:label "parametric coordinate reference system"@en ;
  skos:changeNote "valid" ;
  skos:editorialNote "preferred"^^xsd:string ;
  skos:notation 842 ;
  skos:prefLabel "parametric coordinate reference system"@en ;
.
<http://iso.org/tc211/term/843>
  rdf:type skos:Concept ;
  dcterms:dateAccepted "2009-08-15"^^xsd:date ;
  dcterms:source "ISO 19111-2:2009" ;
  reg:status reg:statusValid ;
  rdfs:comment "Note 1 to entry: The object is normally the Earth."@en ;
  rdfs:label "parametric datum"@en ;
  skos:changeNote "valid" ;
  skos:editorialNote "preferred"^^xsd:string ;
  skos:notation 843 ;
  skos:note "Note 1 to entry: The object is normally the Earth."@en ;
  skos:prefLabel "parametric datum"@en ;
.
<http://iso.org/tc211/term/844>
  rdf:type skos:Concept ;
  dcterms:dateAccepted "2009-08-15"^^xsd:date ;
  dcterms:source "ISO 19111-2:2009" ;
  reg:status reg:statusValid ;
  rdfs:comment "Note 1 to entry: Normally the spatial component is \"horizontal\" and the parametric component is \"vertical\"."@en ;
  rdfs:label "spatio-parametric coordinate reference system"@en ;
  skos:changeNote "valid" ;
  skos:editorialNote "preferred"^^xsd:string ;
  skos:notation 844 ;
  skos:note "Note 1 to entry: Normally the spatial component is \"horizontal\" and the parametric component is \"vertical\"."@en ;
  skos:prefLabel "spatio-parametric coordinate reference system"@en ;
.
<http://iso.org/tc211/term/845>
  rdf:type skos:Concept ;
  dcterms:dateAccepted "2009-08-15"^^xsd:date ;
  dcterms:source "ISO 19111-2:2009" ;
  reg:status reg:statusValid ;
  rdfs:label "spatio-parametric-temporal coordinate reference system"@en ;
  skos:changeNote "valid" ;
  skos:editorialNote "preferred"^^xsd:string ;
  skos:notation 845 ;
  skos:prefLabel "spatio-parametric-temporal coordinate reference system"@en ;
.
<http://iso.org/tc211/term/846>
  rdf:type skos:Concept ;
  dcterms:dateAccepted "2008-06-01"^^xsd:date ;
  dcterms:source "ISO/TS 19101-2:2008" ;
  reg:status reg:statusValid ;
  rdfs:label "band"@en ;
  skos:changeNote "valid" ;
  skos:editorialNote "preferred"^^xsd:string ;
  skos:notation 846 ;
  skos:prefLabel "band"@en ;
.
<http://iso.org/tc211/term/847>
  rdf:type skos:Concept ;
  dcterms:dateAccepted "2008-06-01"^^xsd:date ;
  dcterms:provenance "ISO/TS 19101-2:2008" ;
  dcterms:source "CEOS WGCV" ;
  reg:status reg:statusValid ;
  rdfs:label "calibration"@en ;
  skos:changeNote "valid" ;
  skos:editorialNote "preferred"^^xsd:string ;
  skos:notation 847 ;
  skos:prefLabel "calibration"@en ;
.
<http://iso.org/tc211/term/848>
  rdf:type skos:Concept ;
  dcterms:dateAccepted "2009-08-15"^^xsd:date ;
  dcterms:source "ISO 19144-1:2009" ;
  reg:status reg:statusValid ;
  rdfs:label "classification"@en ;
  skos:changeNote "valid" ;
  skos:editorialNote "preferred"^^xsd:string ;
  skos:notation 848 ;
  skos:prefLabel "classification"@en ;
.
<http://iso.org/tc211/term/849>
  rdf:type skos:Concept ;
  dcterms:dateAccepted "2009-08-15"^^xsd:date ;
  dcterms:source "ISO 19144-1:2009" ;
  reg:status reg:statusValid ;
  rdfs:label "classified object"@en ;
  skos:changeNote "valid" ;
  skos:editorialNote "preferred"^^xsd:string ;
  skos:notation 849 ;
  skos:prefLabel "classified object"@en ;
.
<http://iso.org/tc211/term/85>
  rdf:type skos:Concept ;
  dcterms:dateAccepted "2005-07-15"^^xsd:date ;
  dcterms:dateAccepted "2008-12-30"^^xsd:date ;
  dcterms:provenance "ISO 19118:2005" ;
  dcterms:source "ISO 19118:2011, 4.7" ;
  reg:status reg:statusValid ;
  rdfs:label "conversion rule"@en ;
  skos:changeNote "valid" ;
  skos:definition "입력 데이터 구조의 인스턴스를 출력 자료 구조의 인스턴스로 바꾸는 규칙"@kr ;
  skos:editorialNote "preferred" ;
  skos:editorialNote "preferred"^^xsd:string ;
  skos:notation "85" ;
  skos:notation 85 ;
  skos:prefLabel "conversion rule"@en ;
  skos:prefLabel "전환 규칙"@kr ;
.
<http://iso.org/tc211/term/850>
  rdf:type skos:Concept ;
  dcterms:dateAccepted "2009-08-15"^^xsd:date ;
  dcterms:source "ISO 19144-1:2009" ;
  reg:status reg:statusValid ;
  rdfs:comment "Note 1 to entry:: Classifiers can be defined algorithmically or according to a set of classification system specific rules."@en ;
  rdfs:label "classifier"@en ;
  skos:changeNote "valid" ;
  skos:editorialNote "preferred"^^xsd:string ;
  skos:notation 850 ;
  skos:note "Note 1 to entry:: Classifiers can be defined algorithmically or according to a set of classification system specific rules."@en ;
  skos:prefLabel "classifier"@en ;
.
<http://iso.org/tc211/term/851>
  rdf:type skos:Concept ;
  dcterms:dateAccepted "2009-11-01"^^xsd:date ;
  dcterms:source "ISO 19126:2009" ;
  reg:status reg:statusValid ;
  rdfs:comment "Note 1 to entry: The common characteristic may be a shared namespace for the assignment of names and/or codes."@en ;
  rdfs:label "compound registry"@en ;
  skos:changeNote "valid" ;
  skos:editorialNote "preferred"^^xsd:string ;
  skos:notation 851 ;
  skos:note "Note 1 to entry: The common characteristic may be a shared namespace for the assignment of names and/or codes."@en ;
  skos:prefLabel "compound registry"@en ;
.
<http://iso.org/tc211/term/852>
  rdf:type skos:Concept ;
  dcterms:dateAccepted "2009-11-01"^^xsd:date ;
  dcterms:source "ISO 19126:2009" ;
  reg:status reg:statusValid ;
  rdfs:label "feature association concept"@en ;
  skos:changeNote "valid" ;
  skos:editorialNote "preferred"^^xsd:string ;
  skos:notation 852 ;
  skos:prefLabel "feature association concept"@en ;
.
<http://iso.org/tc211/term/853>
  rdf:type skos:Concept ;
  dcterms:dateAccepted "2009-11-01"^^xsd:date ;
  dcterms:source "ISO 19126:2009" ;
  reg:status reg:statusValid ;
  rdfs:label "feature attribute concept"@en ;
  skos:changeNote "valid" ;
  skos:editorialNote "preferred"^^xsd:string ;
  skos:notation 853 ;
  skos:prefLabel "feature attribute concept"@en ;
.
<http://iso.org/tc211/term/854>
  rdf:type skos:Concept ;
  dcterms:dateAccepted "2002-07-01"^^xsd:date ;
  dcterms:dateAccepted "2008-12-30"^^xsd:date ;
  dcterms:provenance "ISO 19101:2002" ;
  dcterms:source "ISO 19101-1:2014, 4.1.13" ;
  reg:status reg:statusValid ;
  rdfs:label "feature catalogue"@en ;
  skos:changeNote "valid" ;
  skos:definition "피처 유형, 피처 속성 및 여러 지리 데이터 집합 간의 피처 연관, 적용 가능한 피처 연산에 대한 정의와 설명을 담은 목록 "@kr ;
  skos:editorialNote "preferred" ;
  skos:editorialNote "preferred"^^xsd:string ;
  skos:notation "854" ;
  skos:notation 854 ;
  skos:prefLabel "feature catalogue"@en ;
  skos:prefLabel "지형지물 목록"@kr ;
.
<http://iso.org/tc211/term/855>
  rdf:type skos:Concept ;
  dcterms:dateAccepted "2009-11-01"^^xsd:date ;
  dcterms:source "ISO 19126:2009" ;
  reg:status reg:statusValid ;
  rdfs:label "feature concept"@en ;
  skos:changeNote "valid" ;
  skos:editorialNote "preferred"^^xsd:string ;
  skos:notation 855 ;
  skos:prefLabel "feature concept"@en ;
.
<http://iso.org/tc211/term/856>
  rdf:type skos:Concept ;
  dcterms:dateAccepted "2009-08-15"^^xsd:date ;
  dcterms:provenance "ISO 19144-1:2009" ;
  dcterms:source "ISO 19126:2009" ;
  reg:status reg:statusValid ;
  rdfs:label "feature concept dictionary"@en ;
  skos:changeNote "valid" ;
  skos:editorialNote "preferred"^^xsd:string ;
  skos:notation 856 ;
  skos:prefLabel "feature concept dictionary"@en ;
.
<http://iso.org/tc211/term/857>
  rdf:type skos:Concept ;
  dcterms:dateAccepted "2009-11-01"^^xsd:date ;
  dcterms:source "ISO 19126:2009" ;
  reg:status reg:statusValid ;
  rdfs:label "feature operation concept"@en ;
  skos:changeNote "valid" ;
  skos:editorialNote "preferred"^^xsd:string ;
  skos:notation 857 ;
  skos:prefLabel "feature operation concept"@en ;
.
<http://iso.org/tc211/term/859>
  rdf:type skos:Concept ;
  dcterms:dateAccepted "2005-10-15"^^xsd:date ;
  dcterms:dateAccepted "2009-12-29"^^xsd:date ;
  dcterms:provenance "KS X ISO 19135" ;
  dcterms:source "ISO 19135:2005" ;
  reg:status reg:statusValid ;
  rdfs:label "hierarchical register"@en ;
  skos:changeNote "valid" ;
  skos:definition "주 등록물과 하위 등록물 집합으로 구성되어 있는, 등록물 항목의 영역에 대한 등록물의 구조화된 집합 "@kr ;
  skos:editorialNote "preferred" ;
  skos:editorialNote "preferred"^^xsd:string ;
  skos:notation "859" ;
  skos:notation 859 ;
  skos:prefLabel "hierarchical register"@en ;
  skos:prefLabel "계층적 등록물"@kr ;
.
<http://iso.org/tc211/term/86>
  rdf:type skos:Concept ;
  dcterms:dateAccepted "2003-05-01"^^xsd:date ;
  dcterms:dateAccepted "2008-12-19"^^xsd:date ;
  dcterms:provenance "ISO 19107:2003" ;
  dcterms:provenance "KS X ISO 19104" ;
  dcterms:source "Dictionary of Computing, Fourth Edition, Oxford University Press" ;
  reg:status reg:statusValid ;
  rdfs:comment "Note 1 to entry: \"Smallest\" is the set theoretic smallest, not an indication of a measurement. The definition can be rewritten as \"the intersection of all convex sets that contain the geometric object\"."@en ;
  rdfs:comment "비고: \"최소\"는 이론상 가장 작은 것으로, 이는 측정 결과를 말하는 것은 아니다. 볼록 외곽은 \"기하 객체를 포함하는 모든 볼록 집합의 교차점\"으로 재정의될 수 있다."@kr ;
  rdfs:label "convex hull"@en ;
  skos:changeNote "valid" ;
  skos:definition "기하 객체를 포함하는 최소의 볼록 집합"@kr ;
  skos:editorialNote "preferred" ;
  skos:editorialNote "preferred"^^xsd:string ;
  skos:notation "86" ;
  skos:notation 86 ;
  skos:note "Note 1 to entry: \"Smallest\" is the set theoretic smallest, not an indication of a measurement. The definition can be rewritten as \"the intersection of all convex sets that contain the geometric object\"."@en ;
  skos:note "비고: \"최소\"는 이론상 가장 작은 것으로, 이는 측정 결과를 말하는 것은 아니다. 볼록 외곽은 \"기하 객체를 포함하는 모든 볼록 집합의 교차점\"으로 재정의될 수 있다."@kr ;
  skos:prefLabel "convex hull"@en ;
  skos:prefLabel "볼록 외곽"@kr ;
.
<http://iso.org/tc211/term/860>
  rdf:type skos:Concept ;
  dcterms:dateAccepted "2008-06-01"^^xsd:date ;
  dcterms:source "ISO/TS 19101-2:2008" ;
  reg:status reg:statusValid ;
  rdfs:comment "Note 1 to entry: In this Technical Specification, it is assumed that the phenomena have been sensed or detected by one or more devices such as radar, cameras, photometers, and infrared and multispectral scanners"@en ;
  rdfs:label "imagery"@en ;
  skos:changeNote "valid" ;
  skos:editorialNote "preferred"^^xsd:string ;
  skos:notation 860 ;
  skos:note "Note 1 to entry: In this Technical Specification, it is assumed that the phenomena have been sensed or detected by one or more devices such as radar, cameras, photometers, and infrared and multispectral scanners"@en ;
  skos:prefLabel "imagery"@en ;
.
<http://iso.org/tc211/term/861>
  rdf:type skos:Concept ;
  dcterms:dateAccepted "2009-08-15"^^xsd:date ;
  dcterms:source "ISO 19144-1:2009" ;
  reg:status reg:statusValid ;
  rdfs:comment "Note 1 to entry: The result of a classification process is termed legend class in this part of ISO 19144 in order to avoid confusion with the term \"class\" as used in UML modelling."@en ;
  rdfs:label "legend class"@en ;
  skos:changeNote "valid" ;
  skos:editorialNote "preferred"^^xsd:string ;
  skos:notation 861 ;
  skos:note "Note 1 to entry: The result of a classification process is termed legend class in this part of ISO 19144 in order to avoid confusion with the term \"class\" as used in UML modelling."@en ;
  skos:prefLabel "legend class"@en ;
.
<http://iso.org/tc211/term/862>
  rdf:type skos:Concept ;
  dcterms:dateAccepted "2008-06-01"^^xsd:date ;
  dcterms:provenance "ISO/TS 19101-2:2008" ;
  dcterms:source "International Vocabulary of Basic and General Terms in Metrology (VIM)" ;
  reg:status reg:statusValid ;
  rdfs:label "measurable quantity"@en ;
  skos:changeNote "valid" ;
  skos:editorialNote "preferred"^^xsd:string ;
  skos:notation 862 ;
  skos:prefLabel "measurable quantity"@en ;
.
<http://iso.org/tc211/term/863>
  rdf:type skos:Concept ;
  dcterms:dateAccepted "2009-11-01"^^xsd:date ;
  dcterms:source "ISO 19126:2009" ;
  reg:status reg:statusValid ;
  rdfs:comment "Note 1 to entry: Many feature attributes take nominal rather than numerical values.  The value domain of such an attribute is usually specified as an enumeration or a code list."@en ;
  rdfs:label "nominal value"@en ;
  skos:changeNote "valid" ;
  skos:editorialNote "preferred"^^xsd:string ;
  skos:notation 863 ;
  skos:note "Note 1 to entry: Many feature attributes take nominal rather than numerical values.  The value domain of such an attribute is usually specified as an enumeration or a code list."@en ;
  skos:prefLabel "nominal value"@en ;
.
<http://iso.org/tc211/term/864>
  rdf:type skos:Concept ;
  dcterms:dateAccepted "2009-02-15"^^xsd:date ;
  dcterms:source "ISO 19115-2:2009" ;
  reg:status reg:statusValid ;
  rdfs:comment "Note 1 to entry: In this part of ISO 19115, the measuring system will usually be a remote sensing platform. In a navigation context, the measuring system might be a GPS satellite."@en ;
  rdfs:label "pass"@en ;
  skos:changeNote "valid" ;
  skos:editorialNote "preferred"^^xsd:string ;
  skos:notation 864 ;
  skos:note "Note 1 to entry: In this part of ISO 19115, the measuring system will usually be a remote sensing platform. In a navigation context, the measuring system might be a GPS satellite."@en ;
  skos:prefLabel "pass"@en ;
.
<http://iso.org/tc211/term/865>
  rdf:type skos:Concept ;
  dcterms:dateAccepted "2008-06-01"^^xsd:date ;
  dcterms:source "ISO/TS 19101-2:2008" ;
  reg:status reg:statusValid ;
  rdfs:comment "Note 1 to entry: Picture originals could be obtained from printed maps, printed pictures of a geographic imagery scene, or drawings of geographic information, etc."@en ;
  rdfs:label "picture original"@en ;
  skos:changeNote "valid" ;
  skos:editorialNote "preferred"^^xsd:string ;
  skos:notation 865 ;
  skos:note "Note 1 to entry: Picture originals could be obtained from printed maps, printed pictures of a geographic imagery scene, or drawings of geographic information, etc."@en ;
  skos:prefLabel "picture original"@en ;
.
<http://iso.org/tc211/term/866>
  rdf:type skos:Concept ;
  dcterms:dateAccepted "2008-06-01"^^xsd:date ;
  dcterms:source "ISO/TS 19101-2:2008" ;
  reg:status reg:statusValid ;
  rdfs:comment "Note 1 to entry: Picture portrayals are geared for visual display whether in hardcopy or softcopy."@en ;
  rdfs:label "picture portrayal"@en ;
  skos:changeNote "valid" ;
  skos:editorialNote "preferred"^^xsd:string ;
  skos:notation 866 ;
  skos:note "Note 1 to entry: Picture portrayals are geared for visual display whether in hardcopy or softcopy."@en ;
  skos:prefLabel "picture portrayal"@en ;
.
<http://iso.org/tc211/term/867>
  rdf:type skos:Concept ;
  dcterms:dateAccepted "2008-06-01"^^xsd:date ;
  dcterms:provenance "ISO/TS 19101-2:2008" ;
  dcterms:source "ISO/IEC 10746-2" ;
  reg:status reg:statusValid ;
  rdfs:label "policy"@en ;
  skos:changeNote "valid" ;
  skos:editorialNote "preferred"^^xsd:string ;
  skos:notation 867 ;
  skos:prefLabel "policy"@en ;
.
<http://iso.org/tc211/term/868>
  rdf:type skos:Concept ;
  dcterms:dateAccepted "2008-06-01"^^xsd:date ;
  dcterms:provenance "ISO/TS 19101-2:2008" ;
  dcterms:source "ISO 31-6" ;
  reg:status reg:statusValid ;
  rdfs:label "radiance"@en ;
  skos:changeNote "valid" ;
  skos:editorialNote "preferred"^^xsd:string ;
  skos:notation 868 ;
  skos:prefLabel "radiance"@en ;
.
<http://iso.org/tc211/term/87>
  rdf:type skos:Concept ;
  dcterms:dateAccepted "2003-05-01"^^xsd:date ;
  dcterms:dateAccepted "2009-12-29"^^xsd:date ;
  dcterms:provenance "ISO 19107:2003" ;
  dcterms:provenance "KS X ISO 19107" ;
  dcterms:source "Dictionary of Computing, Fourth Edition, Oxford University Press" ;
  reg:status reg:statusValid ;
  rdfs:comment "Note 1 to entry: Convex sets are \"simply connected\", meaning that they have no interior holes, and can normally be considered topologically isomorphic to a Euclidean ball of the appropriate dimension. So the surface of a sphere can be considered to be geodesically convex."@en ;
  rdfs:label "convex set"@en ;
  skos:changeNote "valid" ;
  skos:definition "내부의 임의 두 직접 위치를 잇는 직선 조각상의 모든 점을 포함할 수 있는 기하 집합"@kr ;
  skos:editorialNote "preferred" ;
  skos:editorialNote "preferred"^^xsd:string ;
  skos:notation "87" ;
  skos:notation 87 ;
  skos:note "Note 1 to entry: Convex sets are \"simply connected\", meaning that they have no interior holes, and can normally be considered topologically isomorphic to a Euclidean ball of the appropriate dimension. So the surface of a sphere can be considered to be geodesically convex."@en ;
  skos:prefLabel "convex set"@en ;
  skos:prefLabel "볼록 집합"@kr ;
.
<http://iso.org/tc211/term/871>
  rdf:type skos:Concept ;
  dcterms:dateAccepted "2008-06-01"^^xsd:date ;
  dcterms:provenance "ISO/TS 19101-2:2008" ;
  dcterms:source "CEOS WGCV" ;
  reg:status reg:statusValid ;
  rdfs:label "validation"@en ;
  skos:changeNote "valid" ;
  skos:editorialNote "preferred"^^xsd:string ;
  skos:notation 871 ;
  skos:prefLabel "validation"@en ;
.
<http://iso.org/tc211/term/873>
  rdf:type skos:Concept ;
  dcterms:dateAccepted "2010-11-01"^^xsd:date ;
  dcterms:provenance "ISO 19146:2010" ;
  dcterms:source "ISO 12620:1999 (derived from)" ;
  reg:status reg:statusValid ;
  rdfs:comment "Note 1 to entry: Adapted from ISO 12620:1999."@en ;
  rdfs:comment "Note 2 to entry: An associative relation exists between the concepts \"education\" and \"teaching\", \"baking\" and \"oven\"." ;
  rdfs:label "associative concept system"@en ;
  skos:changeNote "valid" ;
  skos:editorialNote "preferred"^^xsd:string ;
  skos:notation 873 ;
  skos:note "Note 1 to entry: Adapted from ISO 12620:1999."@en ;
  skos:note "Note 2 to entry: An associative relation exists between the concepts \"education\" and \"teaching\", \"baking\" and \"oven\"."^^<http://www.w3.org/2001/XMLSchema#@en> ;
  skos:prefLabel "associative concept system"@en ;
.
<http://iso.org/tc211/term/874>
  rdf:type skos:Concept ;
  dcterms:dateAccepted "2010-11-01"^^xsd:date ;
  dcterms:provenance "ISO 19146:2010" ;
  dcterms:source "ISO 1087-1:2000" ;
  reg:status reg:statusValid ;
  rdfs:label "broader concept"@en ;
  rdfs:seeAlso "superordinate concept" ;
  skos:altLabel "superordinate concept"@en ;
  skos:changeNote "valid" ;
  skos:editorialNote "admitted"^^xsd:string ;
  skos:notation 874 ;
  skos:prefLabel "broader concept"@en ;
.
<http://iso.org/tc211/term/875>
  rdf:type skos:Concept ;
  dcterms:dateAccepted "2010-11-01"^^xsd:date ;
  dcterms:provenance "ISO 19146:2010" ;
  dcterms:source "ISO 1087-1:2000" ;
  reg:status reg:statusValid ;
  rdfs:comment "Note 1 to entry: Characteristics are used for describing concepts."@en ;
  rdfs:label "characteristic"@en ;
  skos:changeNote "valid" ;
  skos:editorialNote "preferred"^^xsd:string ;
  skos:notation 875 ;
  skos:note "Note 1 to entry: Characteristics are used for describing concepts."@en ;
  skos:prefLabel "characteristic"@en ;
.
<http://iso.org/tc211/term/876>
  rdf:type skos:Concept ;
  dcterms:dateAccepted "2010-11-01"^^xsd:date ;
  dcterms:provenance "ISO 19146:2010" ;
  dcterms:source "ISO 1087-1:2000" ;
  reg:status reg:statusValid ;
  rdfs:comment "Note 1 to entry: The delimiting characteristic support for the back may be used for distinguishing the concepts \"stool\" and \"chair\"."@en ;
  rdfs:label "delimiting characteristic"@en ;
  skos:changeNote "valid" ;
  skos:editorialNote "preferred"^^xsd:string ;
  skos:notation 876 ;
  skos:note "Note 1 to entry: The delimiting characteristic support for the back may be used for distinguishing the concepts \"stool\" and \"chair\"."@en ;
  skos:prefLabel "delimiting characteristic"@en ;
.
<http://iso.org/tc211/term/879>
  rdf:type skos:Concept ;
  dcterms:dateAccepted "2010-11-01"^^xsd:date ;
  dcterms:provenance "ISO 19146:2010" ;
  dcterms:source "ISO 12620:1999 (derived from)" ;
  reg:status reg:statusValid ;
  rdfs:comment "Note 1 to entry: Adapted from ISO 12620:1999"@en ;
  rdfs:comment "Note 2 to entry: Within a database or other terminology collection, a set of domains will generally be defined. More than one domain can be associated with a given concept." ;
  rdfs:label "domain <general vocabulary)"@en ;
  skos:changeNote "valid" ;
  skos:editorialNote "preferred"^^xsd:string ;
  skos:notation 879 ;
  skos:note "Note 1 to entry: Adapted from ISO 12620:1999"@en ;
  skos:note "Note 2 to entry: Within a database or other terminology collection, a set of domains will generally be defined. More than one domain can be associated with a given concept."^^<http://www.w3.org/2001/XMLSchema#@en> ;
  skos:prefLabel "domain <general vocabulary)"@en ;
.
<http://iso.org/tc211/term/88>
  rdf:type skos:Concept ;
  dcterms:dateAccepted "2003-02-15" ;
  dcterms:dateAccepted "2003-02-15"^^xsd:date ;
  dcterms:dateAccepted "2007-11-01"^^xsd:date ;
  dcterms:provenance "ISO 19111:2003" ;
  dcterms:provenance "KS X ISO 19111" ;
  dcterms:provenance "NEN 3610" ;
  dcterms:source "ISO 19111:2007" ;
  reg:status reg:statusAccepted ;
  reg:status reg:statusValid ;
  rdfs:comment "Note 1 to entry: In a coordinate reference system, the coordinate numbers are qualified by units."@en ;
  rdfs:comment "OPMERKING In een coördinaatreferentiesysteem worden de coördinaatwaarden gekwalificeerd door eenheden."@en ;
  rdfs:comment "비고: 좌표 참조 체계에서 좌표를 나타내는 숫자는 적합한 단위를 사용해야 한다."@kr ;
  rdfs:label "coordinate"@en ;
  rdfs:seeAlso "coordinate"@nl ;
  skos:altLabel "coordinate"@nl ;
  skos:changeNote "valid" ;
  skos:definition "getal in een sequentie van n getallen om de positie van een punt in een n-dimensionale ruimte te bepalen"@nl ;
  skos:definition "n차원의 공간에서 점의 위치를 표현하는 n개의 숫자 연속"@kr ;
  skos:editorialNote "preferred" ;
  skos:editorialNote "preferred"^^xsd:string ;
  skos:notation "88" ;
  skos:notation 88 ;
  skos:note "Note 1 to entry: In a coordinate reference system, the coordinate numbers are qualified by units."@en ;
  skos:note "OPMERKING In een coördinaatreferentiesysteem worden de coördinaatwaarden gekwalificeerd door eenheden."@en ;
  skos:note "비고: 좌표 참조 체계에서 좌표를 나타내는 숫자는 적합한 단위를 사용해야 한다."@kr ;
  skos:prefLabel "coordinate"@en ;
  skos:prefLabel "coördinaat"@nl ;
  skos:prefLabel "좌표"@kr ;
.
<http://iso.org/tc211/term/880>
  rdf:type skos:Concept ;
  dcterms:dateAccepted "2010-11-01"^^xsd:date ;
  dcterms:source "ISO 19146:2010" ;
  reg:status reg:statusValid ;
  rdfs:comment "Note 1 to entry: A concept may be associated with several domains and separately identified as a domain concept in relation to each."@en ;
  rdfs:label "domain concept"@en ;
  skos:changeNote "valid" ;
  skos:editorialNote "preferred"^^xsd:string ;
  skos:notation 880 ;
  skos:note "Note 1 to entry: A concept may be associated with several domains and separately identified as a domain concept in relation to each."@en ;
  skos:prefLabel "domain concept"@en ;
.
<http://iso.org/tc211/term/881>
  rdf:type skos:Concept ;
  dcterms:dateAccepted "2010-11-01"^^xsd:date ;
  dcterms:provenance "ISO 19146:2010" ;
  dcterms:source "ISO 1087-1:2000" ;
  reg:status reg:statusValid ;
  rdfs:label "essential characteristic"@en ;
  skos:changeNote "valid" ;
  skos:editorialNote "preferred"^^xsd:string ;
  skos:notation 881 ;
  skos:prefLabel "essential characteristic"@en ;
.
<http://iso.org/tc211/term/882>
  rdf:type skos:Concept ;
  dcterms:dateAccepted "2010-11-01"^^xsd:date ;
  dcterms:provenance "ISO 19146:2010" ;
  dcterms:source "ISO 1087-1:2000" ;
  reg:status reg:statusValid ;
  rdfs:comment "Note 1 to entry: Examples of general concepts are \"planet\", \"tower\"."@en ;
  rdfs:label "general concept"@en ;
  skos:changeNote "valid" ;
  skos:editorialNote "preferred"^^xsd:string ;
  skos:notation 882 ;
  skos:note "Note 1 to entry: Examples of general concepts are \"planet\", \"tower\"."@en ;
  skos:prefLabel "general concept"@en ;
.
<http://iso.org/tc211/term/883>
  rdf:type skos:Concept ;
  dcterms:dateAccepted "2010-11-01"^^xsd:date ;
  dcterms:provenance "ISO 19146:2010" ;
  dcterms:source "ISO 1087-1:2000" ;
  reg:status reg:statusValid ;
  rdfs:label "generic concept"@en ;
  skos:changeNote "valid" ;
  skos:editorialNote "preferred"^^xsd:string ;
  skos:notation 883 ;
  skos:prefLabel "generic concept"@en ;
.
<http://iso.org/tc211/term/884>
  rdf:type skos:Concept ;
  dcterms:dateAccepted "2010-11-01"^^xsd:date ;
  dcterms:provenance "ISO 19146:2010" ;
  dcterms:source "ISO 12620:1999 (derived from)" ;
  reg:status reg:statusValid ;
  rdfs:comment "Note 1 to entry: Adapted from ISO 12620:1999"@en ;
  rdfs:label "generic concept system"@en ;
  skos:changeNote "valid" ;
  skos:editorialNote "preferred"^^xsd:string ;
  skos:notation 884 ;
  skos:note "Note 1 to entry: Adapted from ISO 12620:1999"@en ;
  skos:prefLabel "generic concept system"@en ;
.
<http://iso.org/tc211/term/885>
  rdf:type skos:Concept ;
  dcterms:dateAccepted "2010-11-01"^^xsd:date ;
  dcterms:provenance "ISO 19146:2010" ;
  dcterms:source "ISO 1087-1:2000" ;
  reg:status reg:statusValid ;
  rdfs:comment "Note 1 to entry: A generic relation exists between the concepts \"word\" and \"pronoun\", \"vehicle\" and \"car\", \"person\" and \"child\"."@en ;
  rdfs:label "generic relation"@en ;
  rdfs:seeAlso "genus-species relation" ;
  skos:altLabel "genus-species relation"@en ;
  skos:changeNote "valid" ;
  skos:editorialNote "preferred"^^xsd:string ;
  skos:notation 885 ;
  skos:note "Note 1 to entry: A generic relation exists between the concepts \"word\" and \"pronoun\", \"vehicle\" and \"car\", \"person\" and \"child\"."@en ;
  skos:prefLabel "generic relation"@en ;
.
<http://iso.org/tc211/term/886>
  rdf:type skos:Concept ;
  dcterms:dateAccepted "2010-11-01"^^xsd:date ;
  dcterms:provenance "ISO 19146:2010" ;
  dcterms:source "ISO 1087-1:2000" ;
  reg:status reg:statusValid ;
  rdfs:comment "Note 1 to entry: A generic relation exists between the concepts \"word\" and \"pronoun\", \"vehicle\" and \"car\", \"person\" and \"child\"."@en ;
  rdfs:label "genus-species relation"@en ;
  rdfs:seeAlso "generic relation" ;
  skos:altLabel "generic relation"@en ;
  skos:changeNote "valid" ;
  skos:editorialNote "admitted"^^xsd:string ;
  skos:notation 886 ;
  skos:note "Note 1 to entry: A generic relation exists between the concepts \"word\" and \"pronoun\", \"vehicle\" and \"car\", \"person\" and \"child\"."@en ;
  skos:prefLabel "genus-species relation"@en ;
.
<http://iso.org/tc211/term/887>
  rdf:type skos:Concept ;
  dcterms:dateAccepted "2010-11-01"^^xsd:date ;
  dcterms:provenance "ISO 19146:2010" ;
  dcterms:source "ISO 1087-1:2000" ;
  reg:status reg:statusValid ;
  rdfs:comment "Note 1 to entry: An example of homonymy is:   bark     1 \"sound made by a dog\"    2 \"outside covering of the stem of woody plants\"    3 \"sailing vessel\""@en ;
  rdfs:comment "Note 2 to entry: The designations in the relation of homonymy are called homonyms." ;
  rdfs:label "homonymy"@en ;
  skos:changeNote "valid" ;
  skos:editorialNote "preferred"^^xsd:string ;
  skos:notation 887 ;
  skos:note "Note 1 to entry: An example of homonymy is:   bark     1 \"sound made by a dog\"    2 \"outside covering of the stem of woody plants\"    3 \"sailing vessel\""@en ;
  skos:note "Note 2 to entry: The designations in the relation of homonymy are called homonyms."^^<http://www.w3.org/2001/XMLSchema#@en> ;
  skos:prefLabel "homonymy"@en ;
.
<http://iso.org/tc211/term/888>
  rdf:type skos:Concept ;
  dcterms:dateAccepted "2010-11-01"^^xsd:date ;
  dcterms:provenance "ISO 19146:2010" ;
  dcterms:source "ISO 1087-1:2000" ;
  reg:status reg:statusValid ;
  rdfs:label "intension"@en ;
  skos:changeNote "valid" ;
  skos:editorialNote "preferred"^^xsd:string ;
  skos:notation 888 ;
  skos:prefLabel "intension"@en ;
.
<http://iso.org/tc211/term/889>
  rdf:type skos:Concept ;
  dcterms:dateAccepted "2010-11-01"^^xsd:date ;
  dcterms:provenance "ISO 19146:2010" ;
  dcterms:source "ISO 1087-1:2000" ;
  reg:status reg:statusValid ;
  rdfs:comment "Note 1 to entry: The designations in the relation of monosemy are called monosemes."@en ;
  rdfs:label "monosemy"@en ;
  skos:changeNote "valid" ;
  skos:editorialNote "preferred"^^xsd:string ;
  skos:notation 889 ;
  skos:note "Note 1 to entry: The designations in the relation of monosemy are called monosemes."@en ;
  skos:prefLabel "monosemy"@en ;
.
<http://iso.org/tc211/term/890>
  rdf:type skos:Concept ;
  dcterms:dateAccepted "2008-11-15"^^xsd:date ;
  dcterms:provenance "ISO/TS 19104:2008" ;
  dcterms:source "ISO 1087-1:2000" ;
  reg:status reg:statusValid ;
  rdfs:label "narrower concept"@en ;
  rdfs:seeAlso "subordinate concept" ;
  skos:altLabel "subordinate concept"@en ;
  skos:changeNote "valid" ;
  skos:editorialNote "preferred"^^xsd:string ;
  skos:notation 890 ;
  skos:prefLabel "narrower concept"@en ;
.
<http://iso.org/tc211/term/891>
  rdf:type skos:Concept ;
  dcterms:dateAccepted "2010-11-01"^^xsd:date ;
  dcterms:provenance "ISO 19146:2010" ;
  dcterms:source "ISO 1087-1:2000" ;
  reg:status reg:statusValid ;
  rdfs:comment "Note 1 to entry: A partitive relation exists between the concepts \"week\" and \"day\", \"molecule\" and \"atom\"."@en ;
  rdfs:label "partitive relation"@en ;
  rdfs:seeAlso "part-whole relation" ;
  skos:altLabel "part-whole relation"@en ;
  skos:changeNote "valid" ;
  skos:editorialNote "preferred"^^xsd:string ;
  skos:notation 891 ;
  skos:note "Note 1 to entry: A partitive relation exists between the concepts \"week\" and \"day\", \"molecule\" and \"atom\"."@en ;
  skos:prefLabel "partitive relation"@en ;
.
<http://iso.org/tc211/term/892>
  rdf:type skos:Concept ;
  dcterms:dateAccepted "2010-11-01"^^xsd:date ;
  dcterms:provenance "ISO 19146:2010" ;
  dcterms:source "ISO 1087-1:2000" ;
  reg:status reg:statusValid ;
  rdfs:comment "Note 1 to entry: A partitive relation exists between the concepts \"week\" and \"day\", \"molecule\" and \"atom\"."@en ;
  rdfs:label "part-whole relation"@en ;
  rdfs:seeAlso "partitive relation" ;
  skos:altLabel "partitive relation"@en ;
  skos:changeNote "valid" ;
  skos:editorialNote "admitted"^^xsd:string ;
  skos:notation 892 ;
  skos:note "Note 1 to entry: A partitive relation exists between the concepts \"week\" and \"day\", \"molecule\" and \"atom\"."@en ;
  skos:prefLabel "part-whole relation"@en ;
.
<http://iso.org/tc211/term/893>
  rdf:type skos:Concept ;
  dcterms:dateAccepted "2010-11-01"^^xsd:date ;
  dcterms:provenance "ISO 19146:2010" ;
  dcterms:source "ISO 1087-1:2000" ;
  reg:status reg:statusValid ;
  rdfs:comment "Note 1 to entry: An example of polysemy is:   bridge   1  \"structure to carry traffic over a gap\"    2  \"part of a string instrument\"    3  \"dental plate\""@en ;
  rdfs:comment "Note 2 to entry: The designation in the relation of polysemy are called polysemes." ;
  rdfs:label "polysemy"@en ;
  skos:changeNote "valid" ;
  skos:editorialNote "preferred"^^xsd:string ;
  skos:notation 893 ;
  skos:note "Note 1 to entry: An example of polysemy is:   bridge   1  \"structure to carry traffic over a gap\"    2  \"part of a string instrument\"    3  \"dental plate\""@en ;
  skos:note "Note 2 to entry: The designation in the relation of polysemy are called polysemes."^^<http://www.w3.org/2001/XMLSchema#@en> ;
  skos:prefLabel "polysemy"@en ;
.
<http://iso.org/tc211/term/894>
  rdf:type skos:Concept ;
  dcterms:dateAccepted "2010-11-01"^^xsd:date ;
  dcterms:provenance "ISO 19146:2010" ;
  dcterms:source "ISO 1087-1:2000" ;
  reg:status reg:statusValid ;
  rdfs:label "superordinate concept"@en ;
  rdfs:seeAlso "broader concept" ;
  skos:altLabel "broader concept"@en ;
  skos:changeNote "valid" ;
  skos:editorialNote "preferred"^^xsd:string ;
  skos:notation 894 ;
  skos:prefLabel "superordinate concept"@en ;
.
<http://iso.org/tc211/term/895>
  rdf:type skos:Concept ;
  dcterms:dateAccepted "2008-11-15"^^xsd:date ;
  dcterms:provenance "ISO/TS 19104:2008" ;
  dcterms:source "ISO 1087-1:2000" ;
  reg:status reg:statusValid ;
  rdfs:label "subordinate concept"@en ;
  rdfs:seeAlso "narrower concept" ;
  skos:altLabel "narrower concept"@en ;
  skos:changeNote "valid" ;
  skos:editorialNote "preferred"^^xsd:string ;
  skos:notation 895 ;
  skos:prefLabel "subordinate concept"@en ;
.
<http://iso.org/tc211/term/896>
  rdf:type skos:Concept ;
  dcterms:dateAccepted "2010-11-01"^^xsd:date ;
  dcterms:provenance "ISO 19146:2010" ;
  dcterms:source "ISO 1087-1:2000" ;
  reg:status reg:statusValid ;
  rdfs:comment "Note 1 to entry: The relation of synonymy exists, for example, between deuterium and heavy hydrogen."@en ;
  rdfs:comment "Note 2 to entry: Terms which are interchangeable in all contexts are called synonyms; if they are interchangeable only in some contexts, they are called quasi-synonyms." ;
  rdfs:label "synonymy"@en ;
  skos:changeNote "valid" ;
  skos:editorialNote "preferred"^^xsd:string ;
  skos:notation 896 ;
  skos:note "Note 1 to entry: The relation of synonymy exists, for example, between deuterium and heavy hydrogen."@en ;
  skos:note "Note 2 to entry: Terms which are interchangeable in all contexts are called synonyms; if they are interchangeable only in some contexts, they are called quasi-synonyms."^^<http://www.w3.org/2001/XMLSchema#@en> ;
  skos:prefLabel "synonymy"@en ;
.
<http://iso.org/tc211/term/897>
  rdf:type skos:Concept ;
  dcterms:dateAccepted "2010-11-01"^^xsd:date ;
  dcterms:provenance "ISO 19146:2010" ;
  dcterms:source "ISO 1087-1:2000" ;
  reg:status reg:statusValid ;
  rdfs:label "system of concepts"@en ;
  rdfs:seeAlso "concept system" ;
  skos:altLabel "concept system"@en ;
  skos:changeNote "valid" ;
  skos:editorialNote "admitted"^^xsd:string ;
  skos:notation 897 ;
  skos:prefLabel "system of concepts"@en ;
.
<http://iso.org/tc211/term/898>
  rdf:type skos:Concept ;
  dcterms:dateAccepted "2010-11-01"^^xsd:date ;
  dcterms:provenance "ISO 19146:2010" ;
  dcterms:source "ISO 1087-1:2000" ;
  reg:status reg:statusValid ;
  rdfs:label "technical dictionary"@en ;
  rdfs:seeAlso "terminological dictionary" ;
  skos:altLabel "terminological dictionary"@en ;
  skos:changeNote "valid" ;
  skos:editorialNote "admitted"^^xsd:string ;
  skos:notation 898 ;
  skos:prefLabel "technical dictionary"@en ;
.
<http://iso.org/tc211/term/9>
  rdf:type skos:Concept ;
  dcterms:dateAccepted "2005-07-15"^^xsd:date ;
  dcterms:dateAccepted "2009-12-29"^^xsd:date ;
  dcterms:provenance "ISO/TS 19103:2005" ;
  dcterms:provenance "KS X ISO 19103" ;
  dcterms:source "ISO/IEC 19501:2005 (Adapted from)" ;
  reg:status reg:statusValid ;
  rdfs:comment "Note 1 to entry: An actor may be considered to play a separate role with regard to each use case with which it communicates."@en ;
  rdfs:comment "비고: 행위자는 유즈 케이스 별로 별도의 역할을 수행하는 것으로 정의될 수 있다."@kr ;
  rdfs:label "actor <UML>"@en ;
  skos:changeNote "valid" ;
  skos:definition "유즈 케이스와 상호 작용 시, 그 유즈 케이스의 사용자가 수행하는 역할의 집합"@kr ;
  skos:editorialNote "preferred" ;
  skos:editorialNote "preferred"^^xsd:string ;
  skos:notation "9" ;
  skos:notation 9 ;
  skos:note "Note 1 to entry: An actor may be considered to play a separate role with regard to each use case with which it communicates."@en ;
  skos:note "비고: 행위자는 유즈 케이스 별로 별도의 역할을 수행하는 것으로 정의될 수 있다."@kr ;
  skos:prefLabel "actor <UML>"@en ;
  skos:prefLabel "행위자 <UML>"@kr ;
.
<http://iso.org/tc211/term/90>
  rdf:type skos:Concept ;
  dcterms:dateAccepted "2003-05-01"^^xsd:date ;
  dcterms:dateAccepted "2009-12-29"^^xsd:date ;
  dcterms:provenance "KS X ISO 19107" ;
  dcterms:source "ISO 19107:2003" ;
  reg:status reg:statusValid ;
  rdfs:label "coordinate dimension"@en ;
  skos:changeNote "valid" ;
  skos:definition "좌표 체계에서 위치를 기술하는 데 필요한 측정 또는 축의 수"@kr ;
  skos:editorialNote "preferred" ;
  skos:editorialNote "preferred"^^xsd:string ;
  skos:notation "90" ;
  skos:notation 90 ;
  skos:prefLabel "coordinate dimension"@en ;
  skos:prefLabel "좌표 차원"@kr ;
.
<http://iso.org/tc211/term/900>
  rdf:type skos:Concept ;
  dcterms:dateAccepted "2010-11-01"^^xsd:date ;
  dcterms:provenance "ISO 19146:2010" ;
  dcterms:source "ISO 1087-1:2000" ;
  reg:status reg:statusValid ;
  rdfs:comment "Note 1 to entry: The more common terminological data include entry term, definition, note, grammatical label, subject label, language identifier, country identifier and source identifier."@en ;
  rdfs:label "terminological data"@en ;
  skos:changeNote "valid" ;
  skos:editorialNote "preferred"^^xsd:string ;
  skos:notation 900 ;
  skos:note "Note 1 to entry: The more common terminological data include entry term, definition, note, grammatical label, subject label, language identifier, country identifier and source identifier."@en ;
  skos:prefLabel "terminological data"@en ;
.
<http://iso.org/tc211/term/901>
  rdf:type skos:Concept ;
  dcterms:dateAccepted "2010-11-01"^^xsd:date ;
  dcterms:provenance "ISO 19146:2010" ;
  dcterms:source "ISO 1087-1:2000" ;
  reg:status reg:statusValid ;
  rdfs:label "terminological dictionary"@en ;
  rdfs:seeAlso "technical dictionary" ;
  skos:altLabel "technical dictionary"@en ;
  skos:changeNote "valid" ;
  skos:editorialNote "preferred"^^xsd:string ;
  skos:notation 901 ;
  skos:prefLabel "terminological dictionary"@en ;
.
<http://iso.org/tc211/term/902>
  rdf:type skos:Concept ;
  dcterms:dateAccepted "2010-11-01"^^xsd:date ;
  dcterms:provenance "ISO 19146:2010" ;
  dcterms:source "ISO 1087-2:2000" ;
  reg:status reg:statusValid ;
  rdfs:label "terminological entry"@en ;
  skos:changeNote "valid" ;
  skos:editorialNote "preferred"^^xsd:string ;
  skos:notation 902 ;
  skos:prefLabel "terminological entry"@en ;
.
<http://iso.org/tc211/term/903>
  rdf:type skos:Concept ;
  dcterms:dateAccepted "2010-11-01"^^xsd:date ;
  dcterms:provenance "ISO 19146:2010" ;
  dcterms:source "ISO 1087-1:2000" ;
  reg:status reg:statusValid ;
  rdfs:comment "Note 1 to entry: The vocabulary may be monolingual, bilingual or multilingual."@en ;
  rdfs:label "vocabulary"@en ;
  skos:changeNote "valid" ;
  skos:editorialNote "preferred"^^xsd:string ;
  skos:notation 903 ;
  skos:note "Note 1 to entry: The vocabulary may be monolingual, bilingual or multilingual."@en ;
  skos:prefLabel "vocabulary"@en ;
.
<http://iso.org/tc211/term/904>
  rdf:type skos:Concept ;
  dcterms:dateAccepted "2008-07-15"^^xsd:date ;
  dcterms:source "ISO 6709:2008" ;
  reg:status reg:statusValid ;
  rdfs:comment "Note 1 to entry: Coordinate resolution may have linear or angular units depending on the characteristics of the coordinate system"@en ;
  rdfs:label "resolution <coordinate>"@en ;
  skos:changeNote "valid" ;
  skos:editorialNote "preferred"^^xsd:string ;
  skos:notation 904 ;
  skos:note "Note 1 to entry: Coordinate resolution may have linear or angular units depending on the characteristics of the coordinate system"@en ;
  skos:prefLabel "resolution <coordinate>"@en ;
.
<http://iso.org/tc211/term/905>
  rdf:type skos:Concept ;
  dcterms:dateAccepted "2008-07-15"^^xsd:date ;
  dcterms:source "ISO 6709:2008" ;
  reg:status reg:statusValid ;
  rdfs:comment "Note 1 to entry: In the case of latitude or longitude, it may also include a character indicating hemisphere"@en ;
  rdfs:label "sexagesimal degree"@en ;
  skos:changeNote "valid" ;
  skos:editorialNote "preferred"^^xsd:string ;
  skos:notation 905 ;
  skos:note "Note 1 to entry: In the case of latitude or longitude, it may also include a character indicating hemisphere"@en ;
  skos:prefLabel "sexagesimal degree"@en ;
.
<http://iso.org/tc211/term/906>
  rdf:type skos:Concept ;
  dcterms:dateAccepted "2007-09-01"^^xsd:date ;
  dcterms:dateAccepted "2009-12-29"^^xsd:date ;
  dcterms:provenance "KS X ISO 19136" ;
  dcterms:source "ISO 19136:2007" ;
  reg:status reg:statusValid ;
  rdfs:label "GML application schema"@en ;
  skos:changeNote "valid" ;
  skos:definition "표준이 기술하는 규칙에 따라 XML 스키마로 기술된 응용 스키마"@kr ;
  skos:editorialNote "preferred" ;
  skos:editorialNote "preferred"^^xsd:string ;
  skos:notation "906" ;
  skos:notation 906 ;
  skos:prefLabel "GML application schema"@en ;
  skos:prefLabel "GML 응용 스키마"@kr ;
.
<http://iso.org/tc211/term/907>
  rdf:type skos:Concept ;
  dcterms:dateAccepted "2008-11-15"^^xsd:date ;
  dcterms:provenance "ISO/TS 19104:2008" ;
  dcterms:source "ISO 870:2007" ;
  reg:status reg:statusValid ;
  rdfs:comment "Note 1 to entry: The purpose of concept harmonisation is to improve communication"@en ;
  rdfs:label "concept harmonization"@en ;
  skos:changeNote "valid" ;
  skos:editorialNote "preferred"^^xsd:string ;
  skos:notation 907 ;
  skos:note "Note 1 to entry: The purpose of concept harmonisation is to improve communication"@en ;
  skos:prefLabel "concept harmonization"@en ;
.
<http://iso.org/tc211/term/908>
  rdf:type skos:Concept ;
  dcterms:dateAccepted "2008-11-15"^^xsd:date ;
  dcterms:provenance "ISO/TS 19104:2008" ;
  dcterms:source "ISO 1087-1:2000" ;
  reg:status reg:statusValid ;
  rdfs:comment "Note 1 to entry: In terminology work, three types of designations are distinguished: symbols, appellations and terms."@en ;
  rdfs:label "designation"@en ;
  rdfs:seeAlso "designator" ;
  skos:altLabel "designator"@en ;
  skos:changeNote "valid" ;
  skos:editorialNote "preferred"^^xsd:string ;
  skos:notation 908 ;
  skos:note "Note 1 to entry: In terminology work, three types of designations are distinguished: symbols, appellations and terms."@en ;
  skos:prefLabel "designation"@en ;
.
<http://iso.org/tc211/term/909>
  rdf:type skos:Concept ;
  dcterms:dateAccepted "2008-11-15"^^xsd:date ;
  dcterms:provenance "ISO/TS 19104:2008" ;
  dcterms:source "ISO 1087-1:2000" ;
  reg:status reg:statusValid ;
  rdfs:comment "Note 1 to entry: In terminology work three types of designations are distinguished: symbols, appellations and terms"@en ;
  rdfs:label "designator"@en ;
  rdfs:seeAlso "designation" ;
  skos:altLabel "designation"@en ;
  skos:changeNote "valid" ;
  skos:editorialNote "admitted"^^xsd:string ;
  skos:notation 909 ;
  skos:note "Note 1 to entry: In terminology work three types of designations are distinguished: symbols, appellations and terms"@en ;
  skos:prefLabel "designator"@en ;
.
<http://iso.org/tc211/term/91>
  rdf:type skos:Concept ;
  dcterms:dateAccepted "2003-02-15" ;
  dcterms:dateAccepted "2003-02-15"^^xsd:date ;
  dcterms:dateAccepted "2007-11-01"^^xsd:date ;
  dcterms:provenance "ISO 19111:2003" ;
  dcterms:provenance "KS X ISO 19111" ;
  dcterms:source "ISO 19111:2007" ;
  reg:status reg:statusAccepted ;
  reg:status reg:statusValid ;
  rdfs:comment "Note 1 to entry: Supertype of coordinate transformation and coordinate conversion."@en ;
  rdfs:comment "OPMERKING Een supertype van de coördinaat transformatie en de coördinaat conversie."@en ;
  rdfs:comment "비고: 좌표 변환과 좌표 전환의 상위 유형"@kr ;
  rdfs:label "coordinate operation"@en ;
  skos:changeNote "valid" ;
  skos:definition "verandering van coördinaten, gebaseerd op een één op één relatie van het ene coördinaatreferentiesysteem tot het andere."@nl ;
  skos:definition "하나의 좌표 참조 체계로부터 다른 좌표 참조 체계로의 1대1 관계를 갖는 좌표 변경"@kr ;
  skos:editorialNote "preferred" ;
  skos:editorialNote "preferred"^^xsd:string ;
  skos:notation "91" ;
  skos:notation 91 ;
  skos:note "Note 1 to entry: Supertype of coordinate transformation and coordinate conversion."@en ;
  skos:note "OPMERKING Een supertype van de coördinaat transformatie en de coördinaat conversie."@en ;
  skos:note "비고: 좌표 변환과 좌표 전환의 상위 유형"@kr ;
  skos:prefLabel "coordinate operation"@en ;
  skos:prefLabel "coördinaatbewerking"@nl ;
  skos:prefLabel "좌표 연산"@kr ;
.
<http://iso.org/tc211/term/910>
  rdf:type skos:Concept ;
  dcterms:dateAccepted "2008-11-15"^^xsd:date ;
  dcterms:provenance "ISO/TS 19104:2008" ;
  dcterms:source "ISO 1087-1:2000" ;
  reg:status reg:statusValid ;
  rdfs:label "extension"@en ;
  skos:changeNote "valid" ;
  skos:editorialNote "preferred"^^xsd:string ;
  skos:notation 910 ;
  skos:prefLabel "extension"@en ;
.
<http://iso.org/tc211/term/911>
  rdf:type skos:Concept ;
  dcterms:dateAccepted "2008-11-15"^^xsd:date ;
  dcterms:provenance "ISO/TS 19104:2008" ;
  dcterms:source "ISO 5127-1" ;
  reg:status reg:statusValid ;
  rdfs:comment "Note 1 to entry: In this Technical Specification, language refers to natural language or special languages but not programming languages or artificial languages unless specifically identified"@en ;
  rdfs:label "language"@en ;
  skos:changeNote "valid" ;
  skos:editorialNote "preferred"^^xsd:string ;
  skos:notation 911 ;
  skos:note "Note 1 to entry: In this Technical Specification, language refers to natural language or special languages but not programming languages or artificial languages unless specifically identified"@en ;
  skos:prefLabel "language"@en ;
.
<http://iso.org/tc211/term/912>
  rdf:type skos:Concept ;
  dcterms:dateAccepted "2008-11-15"^^xsd:date ;
  dcterms:source "ISO/TS 19104:2008" ;
  reg:status reg:statusValid ;
  rdfs:label "terminological record identifier"@en ;
  skos:changeNote "valid" ;
  skos:editorialNote "preferred"^^xsd:string ;
  skos:notation 912 ;
  skos:prefLabel "terminological record identifier"@en ;
.
<http://iso.org/tc211/term/913>
  rdf:type skos:Concept ;
  dcterms:dateAccepted "2008-11-15"^^xsd:date ;
  dcterms:source "ISO/TS 19104:2008" ;
  reg:status reg:statusValid ;
  rdfs:label "terminology repository"@en ;
  skos:changeNote "valid" ;
  skos:editorialNote "preferred"^^xsd:string ;
  skos:notation 913 ;
  skos:prefLabel "terminology repository"@en ;
.
<http://iso.org/tc211/term/914>
  rdf:type skos:Concept ;
  dcterms:dateAccepted "2011-06-15"^^xsd:date ;
  dcterms:source "ISO 19110:2005/Amd 1:2011," ;
  reg:status reg:statusValid ;
  rdfs:label "feature inheritance"@en ;
  skos:changeNote "valid" ;
  skos:editorialNote "preferred"^^xsd:string ;
  skos:notation 914 ;
  skos:prefLabel "feature inheritance"@en ;
.
<http://iso.org/tc211/term/915>
  rdf:type skos:Concept ;
  dcterms:dateAccepted "2011-06-15"^^xsd:date ;
  dcterms:source "ISO 19110:2005/Amd 1:2011," ;
  reg:status reg:statusValid ;
  rdfs:label "feature relationship"@en ;
  skos:changeNote "valid" ;
  skos:editorialNote "preferred"^^xsd:string ;
  skos:notation 915 ;
  skos:prefLabel "feature relationship"@en ;
.
<http://iso.org/tc211/term/916>
  rdf:type skos:Concept ;
  dcterms:dateAccepted "2009-04-01"^^xsd:date ;
  dcterms:provenance "ISO/TS 19129:2009" ;
  dcterms:source "ANSI T1.523-2001" ;
  reg:status reg:statusValid ;
  rdfs:comment "Note 1 to entry: Whereas data compaction reduces the amount of data used to represent a given amount of information, data compression does not."@en ;
  rdfs:comment "Note 2 to entry: Data compaction can be done through aggregation of like values in adjacent grid cells, tiling schemes or other means of eliminating information that is not relevant." ;
  rdfs:label "data compaction"@en ;
  skos:changeNote "valid" ;
  skos:editorialNote "preferred"^^xsd:string ;
  skos:notation 916 ;
  skos:note "Note 1 to entry: Whereas data compaction reduces the amount of data used to represent a given amount of information, data compression does not."@en ;
  skos:note "Note 2 to entry: Data compaction can be done through aggregation of like values in adjacent grid cells, tiling schemes or other means of eliminating information that is not relevant."^^<http://www.w3.org/2001/XMLSchema#@en> ;
  skos:prefLabel "data compaction"@en ;
.
<http://iso.org/tc211/term/918>
  rdf:type skos:Concept ;
  dcterms:dateAccepted "2009-04-01"^^xsd:date ;
  dcterms:source "ISO/TS 19129:2009" ;
  reg:status reg:statusValid ;
  rdfs:comment "Note 1 to entry: A matrix is a mathematical term"@en ;
  rdfs:label "matrix"@en ;
  skos:changeNote "valid" ;
  skos:editorialNote "preferred"^^xsd:string ;
  skos:notation 918 ;
  skos:note "Note 1 to entry: A matrix is a mathematical term"@en ;
  skos:prefLabel "matrix"@en ;
.
<http://iso.org/tc211/term/919>
  rdf:type skos:Concept ;
  dcterms:dateAccepted "2009-04-01"^^xsd:date ;
  dcterms:provenance "ISO/TS 19129:2009" ;
  dcterms:source "IBM Rational System Developer" ;
  reg:status reg:statusValid ;
  rdfs:label "UML template"@en ;
  skos:changeNote "valid" ;
  skos:editorialNote "preferred"^^xsd:string ;
  skos:notation 919 ;
  skos:prefLabel "UML template"@en ;
.
<http://iso.org/tc211/term/922>
  rdf:type skos:Concept ;
  dcterms:dateAccepted "2010-06-15"^^xsd:date ;
  dcterms:source "ISO/TS 19130:2010" ;
  reg:status reg:statusValid ;
  rdfs:label "adjustable model parameters"@en ;
  skos:changeNote "valid" ;
  skos:editorialNote "preferred"^^xsd:string ;
  skos:notation 922 ;
  skos:prefLabel "adjustable model parameters"@en ;
.
<http://iso.org/tc211/term/925>
  rdf:type skos:Concept ;
  dcterms:dateAccepted "2010-06-15"^^xsd:date ;
  dcterms:source "ISO/TS 19130:2010" ;
  reg:status reg:statusValid ;
  rdfs:comment "Note 1 to entry: It is usually expressed in ECEF coordinates in metres."@en ;
  rdfs:label "aperture reference point"@en ;
  skos:altLabel "ARP"^^<http://www.w3.org/2001/XMLSchema#@en> ;
  skos:changeNote "valid" ;
  skos:editorialNote "preferred"^^xsd:string ;
  skos:notation 925 ;
  skos:note "Note 1 to entry: It is usually expressed in ECEF coordinates in metres."@en ;
  skos:prefLabel "aperture reference point"@en ;
.
<http://iso.org/tc211/term/927>
  rdf:type skos:Concept ;
  dcterms:dateAccepted "2010-06-15"^^xsd:date ;
  dcterms:source "ISO/TS 19130:2010" ;
  reg:status reg:statusValid ;
  rdfs:comment "Note 1 to entry: This is usually measured in terms of the impulse response of the SAR sensor and processing system. It is a function of the size of the synthetic aperture, or alternatively the dwell time (i.e. a larger aperture results in a longer dwell time results in better resolution)."@en ;
  rdfs:label "azimuth resolution <SAR>"@en ;
  skos:changeNote "valid" ;
  skos:editorialNote "preferred"^^xsd:string ;
  skos:notation 927 ;
  skos:note "Note 1 to entry: This is usually measured in terms of the impulse response of the SAR sensor and processing system. It is a function of the size of the synthetic aperture, or alternatively the dwell time (i.e. a larger aperture results in a longer dwell time results in better resolution)."@en ;
  skos:prefLabel "azimuth resolution <SAR>"@en ;
.
<http://iso.org/tc211/term/928>
  rdf:type skos:Concept ;
  dcterms:dateAccepted "2010-06-15"^^xsd:date ;
  dcterms:source "ISO/TS 19130:2010" ;
  reg:status reg:statusValid ;
  rdfs:comment "Note 1 to entry: Beam width is usually measured in radians and as the angular width between two points that have 50% of the power (3 dB below) of the centre of the beam. It is a property of the antenna. Power emitted outside of this angle is too little to provide a usable return."@en ;
  rdfs:label "beam width <SAR>"@en ;
  skos:changeNote "valid" ;
  skos:editorialNote "preferred"^^xsd:string ;
  skos:notation 928 ;
  skos:note "Note 1 to entry: Beam width is usually measured in radians and as the angular width between two points that have 50% of the power (3 dB below) of the centre of the beam. It is a property of the antenna. Power emitted outside of this angle is too little to provide a usable return."@en ;
  skos:prefLabel "beam width <SAR>"@en ;
.
<http://iso.org/tc211/term/93>
  rdf:type skos:Concept ;
  dcterms:dateAccepted "2003-02-15" ;
  dcterms:dateAccepted "2003-02-15"^^xsd:date ;
  dcterms:dateAccepted "2007-11-01"^^xsd:date ;
  dcterms:provenance "ISO 19111:2003" ;
  dcterms:provenance "KS X ISO 19111" ;
  dcterms:provenance "NEN 3610" ;
  dcterms:source "ISO 19111:2007" ;
  reg:status reg:statusAccepted ;
  reg:status reg:statusValid ;
  rdfs:label "coordinate system"@en ;
  skos:changeNote "valid" ;
  skos:definition "set van wiskundige regels voor het toekennen van coördinaten aan punten"@nl ;
  skos:definition "점에 어떤 좌표를 부여할지를 규정하기 위한 수학적 규칙의 집합"@kr ;
  skos:editorialNote "preferred" ;
  skos:editorialNote "preferred"^^xsd:string ;
  skos:notation "93" ;
  skos:notation 93 ;
  skos:prefLabel "coordinate system"@en ;
  skos:prefLabel "coördinaatsysteem"@nl ;
  skos:prefLabel "좌표 체계"@kr ;
.
<http://iso.org/tc211/term/930>
  rdf:type skos:Concept ;
  dcterms:dateAccepted "2010-06-15"^^xsd:date ;
  dcterms:source "ISO/TS 19130:2010" ;
  reg:status reg:statusValid ;
  rdfs:label "calibrated focal length"@en ;
  skos:changeNote "valid" ;
  skos:editorialNote "preferred"^^xsd:string ;
  skos:notation 930 ;
  skos:prefLabel "calibrated focal length"@en ;
.
<http://iso.org/tc211/term/932>
  rdf:type skos:Concept ;
  dcterms:dateAccepted "2010-06-15"^^xsd:date ;
  dcterms:source "ISO/TS 19130:2010" ;
  reg:status reg:statusValid ;
  rdfs:label "Correspondence Model"@en ;
  skos:changeNote "valid" ;
  skos:editorialNote "preferred"^^xsd:string ;
  skos:notation 932 ;
  skos:prefLabel "Correspondence Model"@en ;
.
<http://iso.org/tc211/term/933>
  rdf:type skos:Concept ;
  dcterms:dateAccepted "2010-06-15"^^xsd:date ;
  dcterms:source "ISO/TS 19130:2010" ;
  reg:status reg:statusValid ;
  rdfs:label "cross-track"@en ;
  skos:changeNote "valid" ;
  skos:editorialNote "preferred"^^xsd:string ;
  skos:notation 933 ;
  skos:prefLabel "cross-track"@en ;
.
<http://iso.org/tc211/term/937>
  rdf:type skos:Concept ;
  dcterms:dateAccepted "2010-06-15"^^xsd:date ;
  dcterms:source "ISO/TS 19130:2010" ;
  reg:status reg:statusValid ;
  rdfs:comment "Note 1 to entry: When there are four fiducial marks, fiducial centre is the intersection of the two lines connecting the pairs of opposite fiducial marks."@en ;
  rdfs:label "fiducial centre"@en ;
  skos:changeNote "valid" ;
  skos:editorialNote "preferred"^^xsd:string ;
  skos:notation 937 ;
  skos:note "Note 1 to entry: When there are four fiducial marks, fiducial centre is the intersection of the two lines connecting the pairs of opposite fiducial marks."@en ;
  skos:prefLabel "fiducial centre"@en ;
.
<http://iso.org/tc211/term/939>
  rdf:type skos:Concept ;
  dcterms:dateAccepted "2010-06-15"^^xsd:date ;
  dcterms:source "ISO/TS 19130:2010" ;
  reg:status reg:statusValid ;
  rdfs:label "frame sensor"@en ;
  skos:changeNote "valid" ;
  skos:editorialNote "preferred"^^xsd:string ;
  skos:notation 939 ;
  skos:prefLabel "frame sensor"@en ;
.
<http://iso.org/tc211/term/942>
  rdf:type skos:Concept ;
  dcterms:dateAccepted "2009-02-15"^^xsd:date ;
  dcterms:source "ISO 19115-2:2009" ;
  reg:status reg:statusValid ;
  rdfs:label "geolocation information"@en ;
  skos:changeNote "valid" ;
  skos:editorialNote "preferred"^^xsd:string ;
  skos:notation 942 ;
  skos:prefLabel "geolocation information"@en ;
.
<http://iso.org/tc211/term/944>
  rdf:type skos:Concept ;
  dcterms:dateAccepted "2010-06-15"^^xsd:date ;
  dcterms:source "ISO/TS 19130:2010" ;
  reg:status reg:statusValid ;
  rdfs:label "georeferencing"@en ;
  skos:changeNote "valid" ;
  skos:editorialNote "preferred"^^xsd:string ;
  skos:notation 944 ;
  skos:prefLabel "georeferencing"@en ;
.
<http://iso.org/tc211/term/945>
  rdf:type skos:Concept ;
  dcterms:dateAccepted "2010-06-15"^^xsd:date ;
  dcterms:source "ISO/TS 19130:2010" ;
  reg:status reg:statusValid ;
  rdfs:label "grazing angle <SAR>"@en ;
  skos:changeNote "valid" ;
  skos:editorialNote "preferred"^^xsd:string ;
  skos:notation 945 ;
  skos:prefLabel "grazing angle <SAR>"@en ;
.
<http://iso.org/tc211/term/947>
  rdf:type skos:Concept ;
  dcterms:dateAccepted "2010-06-15"^^xsd:date ;
  dcterms:source "ISO/TS 19130:2010" ;
  reg:status reg:statusValid ;
  rdfs:comment "Note 1 to entry: Ground range of an image is represented by the distance from the nadir point of the antenna to a point in the scene. Usually measured in the horizontal plane, but can also be measured as true distance along the ground, DEM, geoid or ellipsoid surface."@en ;
  rdfs:label "ground range <SAR>"@en ;
  skos:changeNote "valid" ;
  skos:editorialNote "preferred"^^xsd:string ;
  skos:notation 947 ;
  skos:note "Note 1 to entry: Ground range of an image is represented by the distance from the nadir point of the antenna to a point in the scene. Usually measured in the horizontal plane, but can also be measured as true distance along the ground, DEM, geoid or ellipsoid surface."@en ;
  skos:prefLabel "ground range <SAR>"@en ;
.
<http://iso.org/tc211/term/951>
  rdf:type skos:Concept ;
  dcterms:dateAccepted "2010-06-15"^^xsd:date ;
  dcterms:source "ISO/TS 19130:2010" ;
  reg:status reg:statusValid ;
  rdfs:label "image formation <SAR>"@en ;
  skos:changeNote "valid" ;
  skos:editorialNote "preferred"^^xsd:string ;
  skos:notation 951 ;
  skos:prefLabel "image formation <SAR>"@en ;
.
<http://iso.org/tc211/term/952>
  rdf:type skos:Concept ;
  dcterms:dateAccepted "2010-06-15"^^xsd:date ;
  dcterms:source "ISO/TS 19130:2010" ;
  reg:status reg:statusValid ;
  rdfs:comment "Note 1 to entry: The ground control point may be marked in the image, or the user may be provided with an unambiguous description of the ground control point so that it can be found in the image."@en ;
  rdfs:label "image-identifiable ground control point"@en ;
  skos:changeNote "valid" ;
  skos:editorialNote "preferred"^^xsd:string ;
  skos:notation 952 ;
  skos:note "Note 1 to entry: The ground control point may be marked in the image, or the user may be provided with an unambiguous description of the ground control point so that it can be found in the image."@en ;
  skos:prefLabel "image-identifiable ground control point"@en ;
.
<http://iso.org/tc211/term/953>
  rdf:type skos:Concept ;
  dcterms:dateAccepted "2010-06-15"^^xsd:date ;
  dcterms:source "ISO/TS 19130:2010" ;
  reg:status reg:statusValid ;
  rdfs:label "image plane"@en ;
  skos:changeNote "valid" ;
  skos:editorialNote "preferred"^^xsd:string ;
  skos:notation 953 ;
  skos:prefLabel "image plane"@en ;
.
<http://iso.org/tc211/term/954>
  rdf:type skos:Concept ;
  dcterms:dateAccepted "2010-06-15"^^xsd:date ;
  dcterms:source "ISO/TS 19130:2010" ;
  reg:status reg:statusValid ;
  rdfs:label "incident angle"@en ;
  skos:changeNote "valid" ;
  skos:editorialNote "preferred"^^xsd:string ;
  skos:notation 954 ;
  skos:prefLabel "incident angle"@en ;
.
<http://iso.org/tc211/term/955>
  rdf:type skos:Concept ;
  dcterms:dateAccepted "2014-01-15"^^xsd:date ;
  dcterms:source "ISO/TS 19130-2:2014, 4.39" ;
  reg:status reg:statusValid ;
  rdfs:comment "Note 1 to entry:  The effect makes buildings “lay over” onto the ground toward the sensor velocity vector, akin to perspective views in projective imagery."@en ;
  rdfs:label "layover"@en ;
  skos:changeNote "valid" ;
  skos:editorialNote "preferred"^^xsd:string ;
  skos:notation 955 ;
  skos:note "Note 1 to entry:  The effect makes buildings “lay over” onto the ground toward the sensor velocity vector, akin to perspective views in projective imagery."@en ;
  skos:prefLabel "layover"@en ;
.
<http://iso.org/tc211/term/958>
  rdf:type skos:Concept ;
  dcterms:dateAccepted "2010-06-15"^^xsd:date ;
  dcterms:source "ISO/TS 19130:2010" ;
  reg:status reg:statusValid ;
  rdfs:label "perspective centre"@en ;
  rdfs:seeAlso "projection centre" ;
  skos:altLabel "projection centre"@en ;
  skos:changeNote "valid" ;
  skos:editorialNote "preferred"^^xsd:string ;
  skos:notation 958 ;
  skos:prefLabel "perspective centre"@en ;
.
<http://iso.org/tc211/term/96>
  rdf:type skos:Concept ;
  dcterms:dateAccepted "2002-09-01"^^xsd:date ;
  dcterms:dateAccepted "2008-12-19"^^xsd:date ;
  dcterms:provenance "ISO 19108;2002" ;
  dcterms:provenance "KS X ISO 19104" ;
  dcterms:source "ITU-R Rec.TF.686-1 (1997)" ;
  reg:status reg:statusValid ;
  rdfs:label "Coordinated Universal Time (UTC)"@en ;
  skos:changeNote "valid" ;
  skos:definition "제 도량형 협회와 표준시와 표준 주파수를 보급하는 국제 지구 자전 협회(IERS: International Earth Rotation Service)가 유지 관리하는 시간 척도"@kr ;
  skos:editorialNote "preferred" ;
  skos:editorialNote "preferred"^^xsd:string ;
  skos:notation "96" ;
  skos:notation 96 ;
  skos:prefLabel "Coordinated Universal Time (UTC)"@en ;
  skos:prefLabel "협정 세계시"@kr ;
.
<http://iso.org/tc211/term/960>
  rdf:type skos:Concept ;
  dcterms:dateAccepted "2010-06-15"^^xsd:date ;
  dcterms:source "ISO/TS 19130:2010" ;
  reg:status reg:statusValid ;
  rdfs:label "Physical Sensor Model"@en ;
  skos:changeNote "valid" ;
  skos:editorialNote "preferred"^^xsd:string ;
  skos:notation 960 ;
  skos:prefLabel "Physical Sensor Model"@en ;
.
<http://iso.org/tc211/term/963>
  rdf:type skos:Concept ;
  dcterms:dateAccepted "2010-06-15"^^xsd:date ;
  dcterms:source "ISO/TS 19130:2010" ;
  reg:status reg:statusValid ;
  rdfs:label "pushbroom sensor"@en ;
  skos:changeNote "valid" ;
  skos:editorialNote "preferred"^^xsd:string ;
  skos:notation 963 ;
  skos:prefLabel "pushbroom sensor"@en ;
.
<http://iso.org/tc211/term/965>
  rdf:type skos:Concept ;
  dcterms:dateAccepted "2010-06-15"^^xsd:date ;
  dcterms:source "ISO/TS 19130:2010" ;
  reg:status reg:statusValid ;
  rdfs:label "range bin <SAR>"@en ;
  skos:changeNote "valid" ;
  skos:editorialNote "preferred"^^xsd:string ;
  skos:notation 965 ;
  skos:prefLabel "range bin <SAR>"@en ;
.
<http://iso.org/tc211/term/968>
  rdf:type skos:Concept ;
  dcterms:dateAccepted "2010-06-15"^^xsd:date ;
  dcterms:source "ISO/TS 19130:2010" ;
  reg:status reg:statusValid ;
  rdfs:comment "Note 1 to entry: Steering the antenna also allows dwell time to be increased and provides the ability to collect strips at angles non-parallel to the flight direction and with better resolution than Stripmap mode."@en ;
  rdfs:label "scan mode"@en ;
  skos:changeNote "valid" ;
  skos:editorialNote "preferred"^^xsd:string ;
  skos:notation 968 ;
  skos:note "Note 1 to entry: Steering the antenna also allows dwell time to be increased and provides the ability to collect strips at angles non-parallel to the flight direction and with better resolution than Stripmap mode."@en ;
  skos:prefLabel "scan mode"@en ;
.
<http://iso.org/tc211/term/97>
  rdf:type skos:Concept ;
  dcterms:dateAccepted "2005-10-15"^^xsd:date ;
  dcterms:dateAccepted "2006-12-01"^^xsd:date ;
  dcterms:provenance "KS X ISO 19133" ;
  dcterms:source "ISO 19133:2005" ;
  reg:status reg:statusValid ;
  rdfs:comment "Note 1 to entry: The normal mechanism is to apply a cost to each part of a route, and to define the total route cost as the sum of the cost of the parts. This is necessary for the operation of the most common navigation algorithms. The units of cost functions are not limited to monetary costs and values only, but include such measures as time, distance, and possibly others. The only requirement is that the function be additive and at least non-negative. This last criteria can be softened as long as no zero or less cost is associated with any loop in the network, as this will prevent the existence of a \"minimal cost\" route."@en ;
  rdfs:comment "비고: 보통의 메커니즘은 경로의 각 부분에 비용을 할당하고, 전체 경로에 대한 비용을 각 부분 비용의 합으로 정의하는 것이다. 이는 대부분의 일반적인 내비게이션 알고리듬 연산에 필수적으로 사용된다. 비용 함수의 단위는 화폐 비용이나 가치만으로 제한되지 않으며, 시간, 거리 등 다양한 척도가 사용될 수 있다. 다만 함수는 덧셈이 가능해야 하며, 음의 값을 가질 수 없다. 이 마지막 기준은 값이 0이 아니거나 또는 비용이 네트워크상의 루프와 연관되어야 하는 것으로 완화될 수 있으며, 이는 \"최소 비용\" 경로의 존재를 예방한다."@kr ;
  rdfs:label "cost function"@en ;
  skos:changeNote "valid" ;
  skos:definition "경로 측정(비용)과 관련된 함수"@kr ;
  skos:editorialNote "preferred" ;
  skos:editorialNote "preferred"^^xsd:string ;
  skos:notation "97" ;
  skos:notation 97 ;
  skos:note "Note 1 to entry: The normal mechanism is to apply a cost to each part of a route, and to define the total route cost as the sum of the cost of the parts. This is necessary for the operation of the most common navigation algorithms. The units of cost functions are not limited to monetary costs and values only, but include such measures as time, distance, and possibly others. The only requirement is that the function be additive and at least non-negative. This last criteria can be softened as long as no zero or less cost is associated with any loop in the network, as this will prevent the existence of a \"minimal cost\" route."@en ;
  skos:note "비고: 보통의 메커니즘은 경로의 각 부분에 비용을 할당하고, 전체 경로에 대한 비용을 각 부분 비용의 합으로 정의하는 것이다. 이는 대부분의 일반적인 내비게이션 알고리듬 연산에 필수적으로 사용된다. 비용 함수의 단위는 화폐 비용이나 가치만으로 제한되지 않으며, 시간, 거리 등 다양한 척도가 사용될 수 있다. 다만 함수는 덧셈이 가능해야 하며, 음의 값을 가질 수 없다. 이 마지막 기준은 값이 0이 아니거나 또는 비용이 네트워크상의 루프와 연관되어야 하는 것으로 완화될 수 있으며, 이는 \"최소 비용\" 경로의 존재를 예방한다."@kr ;
  skos:prefLabel "cost function"@en ;
  skos:prefLabel "비용 함수"@kr ;
.
<http://iso.org/tc211/term/971>
  rdf:type skos:Concept ;
  dcterms:dateAccepted "2010-06-15"^^xsd:date ;
  dcterms:source "ISO/TS 19130:2010" ;
  reg:status reg:statusValid ;
  rdfs:label "slant plane <SAR>"@en ;
  skos:changeNote "valid" ;
  skos:editorialNote "preferred"^^xsd:string ;
  skos:notation 971 ;
  skos:prefLabel "slant plane <SAR>"@en ;
.
<http://iso.org/tc211/term/972>
  rdf:type skos:Concept ;
  dcterms:dateAccepted "2010-06-15"^^xsd:date ;
  dcterms:source "ISO/TS 19130:2010" ;
  reg:status reg:statusValid ;
  rdfs:label "slant range <SAR>"@en ;
  skos:changeNote "valid" ;
  skos:editorialNote "preferred"^^xsd:string ;
  skos:notation 972 ;
  skos:prefLabel "slant range <SAR>"@en ;
.
<http://iso.org/tc211/term/973>
  rdf:type skos:Concept ;
  dcterms:dateAccepted "2010-06-15"^^xsd:date ;
  dcterms:source "ISO/TS 19130:2010" ;
  reg:status reg:statusValid ;
  rdfs:label "slant range direction <SAR>"@en ;
  rdfs:seeAlso "range direction <SAR>" ;
  skos:altLabel "range direction <SAR>"@en ;
  skos:changeNote "valid" ;
  skos:editorialNote "preferred"^^xsd:string ;
  skos:notation 973 ;
  skos:prefLabel "slant range direction <SAR>"@en ;
.
<http://iso.org/tc211/term/974>
  rdf:type skos:Concept ;
  dcterms:dateAccepted "2010-06-15"^^xsd:date ;
  dcterms:source "ISO/TS 19130:2010" ;
  reg:status reg:statusValid ;
  rdfs:comment "Note 1 to entry: Spotlight mode provides the ability to collect higher resolution SAR data over relatively smaller patches of ground surface."@en ;
  rdfs:label "spotlight mode <SAR>"@en ;
  skos:changeNote "valid" ;
  skos:editorialNote "preferred"^^xsd:string ;
  skos:notation 974 ;
  skos:note "Note 1 to entry: Spotlight mode provides the ability to collect higher resolution SAR data over relatively smaller patches of ground surface."@en ;
  skos:prefLabel "spotlight mode <SAR>"@en ;
.
<http://iso.org/tc211/term/975>
  rdf:type skos:Concept ;
  dcterms:dateAccepted "2010-06-15"^^xsd:date ;
  dcterms:source "ISO/TS 19130:2010" ;
  reg:status reg:statusValid ;
  rdfs:label "squint angle <SAR>"@en ;
  skos:changeNote "valid" ;
  skos:editorialNote "preferred"^^xsd:string ;
  skos:notation 975 ;
  skos:prefLabel "squint angle <SAR>"@en ;
.
<http://iso.org/tc211/term/978>
  rdf:type skos:Concept ;
  dcterms:dateAccepted "2010-06-15"^^xsd:date ;
  dcterms:source "ISO/TS 19130:2010" ;
  reg:status reg:statusValid ;
  rdfs:label "True Replacement Model"@en ;
  skos:changeNote "valid" ;
  skos:editorialNote "preferred"^^xsd:string ;
  skos:notation 978 ;
  skos:prefLabel "True Replacement Model"@en ;
.
<http://iso.org/tc211/term/982>
  rdf:type skos:Concept ;
  dcterms:dateAccepted "2009-02-15"^^xsd:date ;
  dcterms:source "ISO 19115-2:2009" ;
  reg:status reg:statusValid ;
  rdfs:label "georectified"@en ;
  skos:changeNote "valid" ;
  skos:editorialNote "preferred"^^xsd:string ;
  skos:notation 982 ;
  skos:prefLabel "georectified"@en ;
.
<http://iso.org/tc211/term/983>
  rdf:type skos:Concept ;
  dcterms:dateAccepted "2009-02-15"^^xsd:date ;
  dcterms:source "ISO 19115-2:2009" ;
  reg:status reg:statusValid ;
  rdfs:label "ground control point"@en ;
  skos:changeNote "valid" ;
  skos:editorialNote "preferred"^^xsd:string ;
  skos:notation 983 ;
  skos:prefLabel "ground control point"@en ;
.
<http://iso.org/tc211/term/985>
  rdf:type skos:Concept ;
  dcterms:dateAccepted "2010-06-15"^^xsd:date ;
  dcterms:source "ISO/TS 19130:2010" ;
  reg:status reg:statusValid ;
  rdfs:label "active sensing system"@en ;
  skos:changeNote "valid" ;
  skos:editorialNote "preferred"^^xsd:string ;
  skos:notation 985 ;
  skos:prefLabel "active sensing system"@en ;
.
<http://iso.org/tc211/term/986>
  rdf:type skos:Concept ;
  dcterms:dateAccepted "2010-06-15"^^xsd:date ;
  dcterms:source "ISO/TS 19130:2010" ;
  reg:status reg:statusValid ;
  rdfs:label "along-track"@en ;
  skos:changeNote "valid" ;
  skos:editorialNote "preferred"^^xsd:string ;
  skos:notation 986 ;
  skos:prefLabel "along-track"@en ;
.
<http://iso.org/tc211/term/988>
  rdf:type skos:Concept ;
  dcterms:dateAccepted "2010-06-15"^^xsd:date ;
  dcterms:source "ISO/TS 19130:2010" ;
  reg:status reg:statusValid ;
  rdfs:label "broadside <SAR>"@en ;
  skos:changeNote "valid" ;
  skos:editorialNote "preferred"^^xsd:string ;
  skos:notation 988 ;
  skos:prefLabel "broadside <SAR>"@en ;
.
<http://iso.org/tc211/term/99>
  rdf:type skos:Concept ;
  dcterms:dateAccepted "2005-08-15"^^xsd:date ;
  dcterms:dateAccepted "2007-11-01"^^xsd:date ;
  dcterms:provenance "KS X ISO 19123" ;
  dcterms:source "ISO 19123:2005" ;
  reg:status reg:statusValid ;
  rdfs:comment "Note 1 to entry:: In other words, a coverage is a feature that has multiple values for each attribute type, where each direct position within the geometric representation of the feature has a single value for each attribute type."@en ;
  rdfs:comment "비고: 커버리지는 다른 말로 각각의 속성 유형에 대한 다양한 값을 갖는 피처이며, 피처의 기하학적 표현 내에서 각각의 직접 위치는 각 속성 유형별로 하나의 값을 갖는다."@kr ;
  rdfs:label "coverage"@en ;
  skos:changeNote "valid" ;
  skos:definition "시공간 영역(공간, 시간, 시공간) 내에서 함수처럼 그 범위 내의 특정 직접 위치에 대한 값을 반환하는 피처"@kr ;
  skos:editorialNote "preferred" ;
  skos:editorialNote "preferred"^^xsd:string ;
  skos:notation "99" ;
  skos:notation 99 ;
  skos:note "Note 1 to entry:: In other words, a coverage is a feature that has multiple values for each attribute type, where each direct position within the geometric representation of the feature has a single value for each attribute type."@en ;
  skos:note "비고: 커버리지는 다른 말로 각각의 속성 유형에 대한 다양한 값을 갖는 피처이며, 피처의 기하학적 표현 내에서 각각의 직접 위치는 각 속성 유형별로 하나의 값을 갖는다."@kr ;
  skos:prefLabel "coverage"@en ;
  skos:prefLabel "커버리지"@kr ;
.
<http://iso.org/tc211/term/990>
  rdf:type skos:Concept ;
  dcterms:dateAccepted "2010-06-15"^^xsd:date ;
  dcterms:source "ISO/TS 19130:2010" ;
  reg:status reg:statusValid ;
  rdfs:label "Doppler angle <SAR>"@en ;
  skos:changeNote "valid" ;
  skos:editorialNote "preferred"^^xsd:string ;
  skos:notation 990 ;
  skos:prefLabel "Doppler angle <SAR>"@en ;
.
<http://iso.org/tc211/term/991>
  rdf:type skos:Concept ;
  dcterms:dateAccepted "2010-06-15"^^xsd:date ;
  dcterms:source "ISO/TS 19130:2010" ;
  reg:status reg:statusValid ;
  rdfs:comment "Note 1 to entry: In the SAR context, it is the frequency shift imposed on a radar signal due to relative motion between the transmitter and the object being illuminated."@en ;
  rdfs:label "Doppler shift"@en ;
  skos:changeNote "valid" ;
  skos:editorialNote "preferred"^^xsd:string ;
  skos:notation 991 ;
  skos:note "Note 1 to entry: In the SAR context, it is the frequency shift imposed on a radar signal due to relative motion between the transmitter and the object being illuminated."@en ;
  skos:prefLabel "Doppler shift"@en ;
.
<http://iso.org/tc211/term/994>
  rdf:type skos:Concept ;
  dcterms:dateAccepted "2010-06-15"^^xsd:date ;
  dcterms:source "ISO/TS 19130:2010" ;
  reg:status reg:statusValid ;
  rdfs:comment "Note 1 to entry: When a camera is calibrated the distances between fiducial marks are precisely measured and assigned coordinates that assist in correcting for film distortion."@en ;
  rdfs:label "fiducial mark"@en ;
  skos:changeNote "valid" ;
  skos:editorialNote "preferred"^^xsd:string ;
  skos:notation 994 ;
  skos:note "Note 1 to entry: When a camera is calibrated the distances between fiducial marks are precisely measured and assigned coordinates that assist in correcting for film distortion."@en ;
  skos:prefLabel "fiducial mark"@en ;
.
<http://iso.org/tc211/term/995>
  rdf:type skos:Concept ;
  dcterms:dateAccepted "2010-06-15"^^xsd:date ;
  dcterms:source "ISO/TS 19130:2010" ;
  reg:status reg:statusValid ;
  rdfs:label "geolocating"@en ;
  skos:changeNote "valid" ;
  skos:editorialNote "preferred"^^xsd:string ;
  skos:notation 995 ;
  skos:prefLabel "geolocating"@en ;
.
<http://iso.org/tc211/term/996>
  rdf:type skos:Concept ;
  dcterms:dateAccepted "2010-06-15"^^xsd:date ;
  dcterms:source "ISO/TS 19130:2010" ;
  reg:status reg:statusValid ;
  rdfs:comment "Note 1 to entry: While there are many methods for geopositioning, this Technical Specification is focused on geopositioning from image coordinates"@en ;
  rdfs:label "geopositioning"@en ;
  skos:changeNote "valid" ;
  skos:editorialNote "preferred"^^xsd:string ;
  skos:notation 996 ;
  skos:note "Note 1 to entry: While there are many methods for geopositioning, this Technical Specification is focused on geopositioning from image coordinates"@en ;
  skos:prefLabel "geopositioning"@en ;
.
<http://iso.org/tc211/term/999>
  rdf:type skos:Concept ;
  dcterms:dateAccepted "2010-06-15"^^xsd:date ;
  dcterms:source "ISO/TS 19130:2010" ;
  reg:status reg:statusValid ;
  rdfs:comment "Note 1 to entry: It is usually the centre point of an image (Spotlight) or an image line (Stripmap). It is usually expressed in ECEF coordinates in metres."@en ;
  rdfs:label "ground reference point"@en ;
  skos:altLabel "GRP"^^<http://www.w3.org/2001/XMLSchema#@en> ;
  skos:changeNote "valid" ;
  skos:editorialNote "preferred"^^xsd:string ;
  skos:notation 999 ;
  skos:note "Note 1 to entry: It is usually the centre point of an image (Spotlight) or an image line (Stripmap). It is usually expressed in ECEF coordinates in metres."@en ;
  skos:prefLabel "ground reference point"@en ;
.
reg:statusAccepted
  rdf:type reg:Status ;
  rdfs:label "accepted"@en ;
.
reg:statusDeprecated
  rdfs:label "deprecated"@en ;
.
reg:statusExperimental
  rdfs:label "experimental"@en ;
.
reg:statusInvalid
  rdfs:label "invalid"@en ;
.
reg:statusNotAccepted
  rdfs:label "notAccepted"@en ;
.
reg:statusReserved
  rdfs:label "reserved"@en ;
.
reg:statusRetired
  rdf:type reg:Status ;
  rdfs:label "retired"@en ;
.
reg:statusStable
  rdfs:label "stable"@en ;
.
reg:statusSubmitted
  rdfs:label "submitted"@en ;
.
reg:statusSuperseded
  rdf:type reg:Status ;
  rdfs:label "superseded"@en ;
.
reg:statusValid
  rdf:type reg:Status ;
  rdfs:label "valid"@en ;
.
